@prefix rdf:	<http://www.w3.org/1999/02/22-rdf-syntax-ns#> .
@prefix ns1:	<http://semantic.digital-agenda-data.eu/codelist/> .
@prefix skos:	<http://www.w3.org/2004/02/skos/core#> .
@prefix xsd:	<http://www.w3.org/2001/XMLSchema#> .
@prefix dct:	<http://purl.org/dc/terms/> .
@prefix rdfs:	<http://www.w3.org/2000/01/rdf-schema#> .
@prefix ns6:	<http://semantic.digital-agenda-data.eu/codelist/source/> .
@prefix ns7:	<http://semantic.digital-agenda-data.eu/def/> .
@prefix ns8:	<http://semantic.digital-agenda-data.eu/def/class/> .
@prefix foaf:	<http://xmlns.com/foaf/0.1/> .
@prefix ns10:	<https://ec.europa.eu/digital-agenda/en/news/> .
@prefix ns11:	<http://ec.europa.eu/information_society/eeurope/i2010/benchmarking/index_en.htm#> .
@prefix ns12:	<http://ec.europa.eu/digital-agenda/> .
@prefix ns13:	<https://ec.europa.eu/digital-single-market/en/news/> .
@prefix ns14:	<https://www.europeandataportal.eu/en/> .
@prefix ns15:	<http://www.cept.org/eco/deliverables/> .
@prefix ns16:	<http://www.obs.coe.int/eservices/> .
@prefix ns17:	<http://www.epsiplatform.eu/content/> .
@prefix ns18:	<http://ec.europa.eu/eurostat/web/digital-economy-and-society/data/> .
@prefix ns19:	<http://ec.europa.eu/eurostat/web/lfs/data/> .
@prefix ns20:	<http://ec.europa.eu/eurostat/web/international-trade/data/> .
@prefix ns21:	<http://ec.europa.eu/eurostat/web/products-datasets/-/> .
@prefix ns22:	<http://ec.europa.eu/eurostat/web/science-technology-innovation/data/> .
@prefix ns23:	<http://ec.europa.eu/eurostat/web/national-accounts/data/> .
@prefix ns24:	<http://ec.europa.eu/eurostat/web/population-demography-migration-projections/population-data/> .
@prefix ns25:	<http://ec.europa.eu/digital-agenda/en/news/> .
@prefix ns26:	<http://epp.eurostat.ec.europa.eu/portal/page/portal/employment_unemployment_lfs/methodology/> .
@prefix ns27:	<http://ec.europa.eu/digital-agenda/en/digital-agenda-you/> .

ns1:source
	rdf:type	skos:ConceptScheme ;
	dct:modified	"2020-02-17T11:02:44"^^xsd:dateTime ;
	rdfs:isDefinedBy	<http://digital-agenda-data.eu/> ;
	skos:prefLabel	"Sources used by Digital Agenda Scoreboard indicators" ;
	skos:notation	"CL_SOURCE" ;
	skos:hasTopConcept	ns6:abac , ns6:bench_gp , ns6:berec_roam , ns6:biac , ns6:capgemini , ns6:cnect-estat , ns6:cocom , ns6:corda , ns6:desi_1a1_fbbc , ns6:desi_1a2_fbbtu , ns6:desi_1b1_4g , ns6:desi_1b2_mbbtu , ns6:desi_1c1_ngac , ns6:desi_1c2_sfbb , ns6:desi_1d1_ubbc , ns6:desi_1d2_ubbta , ns6:desi_1e1_bbpi , ns6:desi_2b1_ictspec , ns6:desi_3c1_bank , ns6:desi_3c2_shop , ns6:desi_4a1_eis , ns6:desi_4b1_smeso , ns6:desi_4b2_ecomturn , ns6:desi_4b3_sellcb , ns6:desi_5a1_egovu , ns6:desi_5a2_prefform , ns6:desi_5a3_osercomp , ns6:desi_5a4_psb , ns6:desi_5a5_opendata , ns6:desi_5b1_ehs , ns6:eco_report_03_efis_comm , ns6:egov_bench12 , ns6:egov_bench12_17 , ns6:einfraegi , ns6:einfrageant , ns6:einfraprace , ns6:eoa_smart12-26 , ns6:eoa_yearbook2014 , ns6:epsi , ns6:epsiplatform , ns6:estat-ent , ns6:estat-hh , ns6:estat-lfs , ns6:estat-lfs-sks , ns6:estat-trade , ns6:estat_gba_nabsfin07 , ns6:estat_isoc_bde15b_e , ns6:estat_isoc_bde15b_h , ns6:estat_isoc_bde15b_p , ns6:estat_isoc_bde15cbc , ns6:estat_isoc_bde15cua , ns6:estat_isoc_bde15dec , ns6:estat_isoc_bde15dip , ns6:estat_isoc_bde15disc , ns6:estat_isoc_bde15dth , ns6:estat_isoc_bde15ee , ns6:estat_isoc_ci_ac_i , ns6:estat_isoc_ci_eu_en2 , ns6:estat_isoc_ci_eu_i , ns6:estat_isoc_ci_ifp_fu , ns6:estat_isoc_ci_ifp_iu , ns6:estat_isoc_ci_im_i , ns6:estat_isoc_cicce_use , ns6:estat_isoc_cisci_ax , ns6:estat_isoc_cisci_pb , ns6:estat_isoc_cisci_prv , ns6:estat_isoc_cismt , ns6:estat_isoc_ec_eseln2 , ns6:estat_isoc_ec_ibuy , ns6:estat_isoc_ec_iprb , ns6:estat_isoc_pibi_ictbn2 , ns6:estat_isoc_r_gov_i , ns6:estat_isoc_r_iuse_i , ns6:estat_isoc_sk_cskl_i , ns6:estat_isoc_sk_dskl_i , ns6:estat_isoc_sk_how_i , ns6:estat_isoc_sk_iskl_i , ns6:estat_isoc_ske_ittn2 , ns6:estat_isoc_sks_itspt , ns6:estat_lfst_hhnhwhtc , ns6:estat_nama_gdp_c , ns6:estat_randd , ns6:estat_tps00188 , ns6:eun12 , ns6:euripidis-estat , ns6:eurostat_ed , ns6:eurostat_nat_acc , ns6:eurostat_pop , ns6:idate , ns6:ihs_tech , ns6:ipv6obs , ns6:jrc-ictspec3 , ns6:jrc_ict_randd , ns6:mis , ns6:nif_database , ns6:old_desi_1b3_spec , ns6:old_desi_1d1_fbbp , ns6:old_desi_5b1_mdataexch , ns6:old_desi_5b2_epresc , ns6:point_topic , ns6:samknows , ns6:smart11_39 , ns6:desi_1b3_5g , ns6:desi_2a1_bds , ns6:desi_2a2_abds , ns6:desi_2a3_abss , ns6:desi_2b2_fictspec , ns6:desi_2b3_ictg , ns6:desi_3a1_notiu , ns6:desi_3a2_iu , ns6:desi_3b1_news , ns6:desi_3b2_mvg , ns6:desi_3b3_vod , ns6:desi_3b4_vidcall , ns6:desi_3b5_socnet , ns6:desi_3b6_profsocnet , ns6:desi_3b7_courseon , ns6:desi_3b8_convoton , ns6:desi_3c3_sell , ns6:desi_4a2_socmed , ns6:desi_4a3_bigdat , ns6:desi_4a4_cloud , ns6:desi_5b2_mdataexch , ns6:desi_5b3_epresc , ns6:old_desi_2a1_iu , ns6:old_desi_2a2_bds , ns6:old_desi_2b1_ictspec , ns6:old_desi_2b2_stemg , ns6:old_desi_3a1_news , ns6:old_desi_3a2_mvg , ns6:old_desi_3a3_vod , ns6:old_desi_3a4_iptv , ns6:old_desi_3b1_vidcall , ns6:old_desi_3b2_socnet , ns6:old_desi_4a1_eis , ns6:old_desi_4a2_rfid , ns6:old_desi_4a3_socmed , ns6:old_desi_4a4_einv , ns6:old_desi_4a5_cloud , ns6:estathh_cocom ;
	skos:inScheme	ns7:scheme .
ns6:abac
	rdf:type	ns8:Source , skos:Concept ;
	skos:prefLabel	"ABAC" ;
	foaf:page	<http://europa.eu/rapid/press-release_MEMO-05-94_en.htm?locale=en> ;
	skos:notation	"abac" ;
	skos:definition	"ABAC is a transversal, transactional information system allowing for the execution and monitoring of all budgetary and accounting operations by the Commission, an Agency or Institution." ;
	skos:topConceptOf	ns1:source .
ns6:bench_gp
	rdf:type	ns8:Source , skos:Concept ;
	skos:prefLabel	"Benchmarking deployment of eHealth among General Practitioners" ;
	foaf:page	ns10:benchmarking-deployment-ehealth-among-general-practitioners-2013-smart-20110033 ;
	skos:notation	"bench_gp" ;
	skos:definition	"Studies committed by DG Connect to monitor the adoption of eHealth technologies by General Practitioners: 2007, 2013" ;
	skos:topConceptOf	ns1:source .
ns6:berec_roam
	rdf:type	ns8:Source , skos:Concept ;
	skos:prefLabel	"International Roaming BEREC Benchmark Data Report" ;
	foaf:page	<http://berec.europa.eu/eng/document_register/subject_matter/berec/reports/1159-international-roaming-berec-benchmark-data-report-january-2012-8211-june-2012> ;
	skos:notation	"berec_roam" ;
	skos:definition	"International Roaming Benchmark Data Report by BEREC - The Body of European Regulators for Electronic Communications" ;
	skos:note	"Document date: 28.01.2013 (Document number: BoR (13) 05)." ;
	skos:topConceptOf	ns1:source .
ns6:biac
	rdf:type	ns8:Source , skos:Concept ;
	skos:prefLabel	"Broadband Internet Access Cost (BIAC) annual studies" ;
	foaf:page	ns10:study-retail-broadband-access-prices-2013-smart-20100038 ;
	skos:notation	"biac" ;
	skos:definition	"Broadband Internet Access Cost (BIAC), annual studies for the EC realised by Van Dijk, covering EU 28 Member States as well as Canada, Iceland, Japan, South Korea, Liechtenstein, FYROM, Norway, State of California, State of Colorado, State of New York, Switzerland and Turkey." ;
	skos:note	"update until feb 2012 data collection" ;
	skos:topConceptOf	ns1:source .
ns6:capgemini
	rdf:type	ns8:Source , skos:Concept ;
	skos:prefLabel	"eGovernment Benchmarking Reports 2001-2010" ;
	foaf:page	ns11:e-Government_Benchmarking_Reports ;
	skos:notation	"capgemini" ;
	skos:definition	"eGovernment Benchmarking Report, Study for the EC realised by Capgemini (2001-2010 data)" ;
	skos:note	"Extraction 20 May 2011" ;
	skos:topConceptOf	ns1:source .
ns6:cnect-estat
	rdf:type	ns8:Source , skos:Concept ;
	skos:prefLabel	"Pilot of new Digital Skills Indicators" ;
	foaf:page	<http://ec.europa.eu/information_society/newsroom/cf/dae/document.cfm?action=display&doc_id=5406> ;
	skos:notation	"cnect-estat" ;
	skos:definition	"Pilot work carried out by DG CONNECT/F4 in relation to action 62 of the Digital Agenda to propose \"EU-wide indicators of digital competence\". These indicators have been piloted on the 2012 microdata from the Eurostat community survey on ICT usage by Households/Individuals. It is proposed for regular implementation starting with the 2015 survey." ;
	skos:topConceptOf	ns1:source .
ns6:cocom
	rdf:type	ns8:Source , skos:Concept ;
	skos:prefLabel	"Communications Committee survey" ;
	foaf:page	ns12:about-fast-and-ultra-fast-internet-access ;
	skos:notation	"cocom" ;
	skos:definition	"Electronic communications market indicators collected by Commission services, through National Regulatory Authorities, for the Communications Committee (COCOM) - January and July reports." ;
	skos:note	"extraction 22 May 2013" ;
	skos:topConceptOf	ns1:source .
ns6:corda
	rdf:type	ns8:Source , skos:Concept ;
	skos:prefLabel	"CORDA " ;
	foaf:page	<http://webcorda.rtd.cec.eu.int/index.cfm?page=index> ;
	skos:notation	"corda" ;
	skos:definition	"Common Research Data Warehouse" ;
	skos:topConceptOf	ns1:source .
ns6:desi_1a1_fbbc
	rdf:type	ns8:Source , skos:Concept ;
	skos:prefLabel	"Broadband coverage in Europe Study" ;
	foaf:page	<http://digital-agenda-data.eu/charts/analyse-one-indicator-and-compare-countries#chart={\u0022indicator-group\u0022:\u0022any\u0022,\u0022indicator\u0022:\u0022bb_scov\u0022,\u0022breakdown\u0022:\u0022TOTAL_POPHH\u0022,\u0022unit-measure\u0022:\u0022pc_hh_all\u0022,\u0022ref-area\u0022:[\u0022BE\u0022,\u0022BG\u0022,\u0022CZ\u0022,\u0022DK\u0022,\u0022DE\u0022,\u0022EE\u0022,\u0022IE\u0022,\u0022EL\u0022,\u0022ES\u0022,\u0022FR\u0022,\u0022IT\u0022,\u0022CY\u0022,\u0022LV\u0022,\u0022LT\u0022,\u0022LU\u0022,\u0022HU\u0022,\u0022HR\u0022,\u0022MT\u0022,\u0022NL\u0022,\u0022AT\u0022,\u0022PL\u0022,\u0022PT\u0022,\u0022RO\u0022,\u0022SI\u0022,\u0022SK\u0022,\u0022FI\u0022,\u0022SE\u0022,\u0022UK\u0022,\u0022EU\u0022]}> ;
	skos:notation	"desi_1a1_fbbc" ;
	skos:definition	"Broadband coverage in Europe, studies for the EC by IHS and Valdani, Vicari & Associati (2013-2015, SMART 2013/0054) and by IHS and Point Topic (2016 onwards, SMART 2016/0045)" ;
	skos:topConceptOf	ns1:source .
ns6:desi_1a2_fbbtu
	rdf:type	ns8:Source , skos:Concept ;
	skos:prefLabel	"Eurostat Survey - ICT usage in Households and by People" ;
	foaf:page	<http://digital-agenda-data.eu/charts/analyse-one-indicator-and-compare-countries#chart={\u0022indicator-group\u0022:\u0022any\u0022,\u0022indicator\u0022:\u0022h_bbfix\u0022,\u0022breakdown\u0022:\u0022HH_total\u0022,\u0022unit-measure\u0022:\u0022pc_hh\u0022,\u0022ref-area\u0022:[\u0022BE\u0022,\u0022BG\u0022,\u0022CZ\u0022,\u0022DK\u0022,\u0022DE\u0022,\u0022EE\u0022,\u0022IE\u0022,\u0022EL\u0022,\u0022ES\u0022,\u0022FR\u0022,\u0022IT\u0022,\u0022CY\u0022,\u0022LV\u0022,\u0022LT\u0022,\u0022LU\u0022,\u0022HU\u0022,\u0022HR\u0022,\u0022MT\u0022,\u0022NL\u0022,\u0022AT\u0022,\u0022PL\u0022,\u0022PT\u0022,\u0022RO\u0022,\u0022SI\u0022,\u0022SK\u0022,\u0022FI\u0022,\u0022SE\u0022,\u0022UK\u0022,\u0022EU\u0022]}> ;
	skos:notation	"desi_1a2_fbbtu" ;
	skos:definition	"Eurostat - Community survey on ICT usage in Households and by People" ;
	skos:topConceptOf	ns1:source .
ns6:desi_1b1_4g
	rdf:type	ns8:Source , skos:Concept ;
	skos:prefLabel	"Broadband coverage in Europe Study" ;
	skos:notation	"desi_1b1_4g" ;
	skos:definition	"Broadband coverage in Europe, studies for the EC by IHS and Valdani, Vicari & Associati (2013-2015, SMART 2013/0054) and by IHS and Point Topic (2016 onwards, SMART 2016/0045)" ;
	skos:topConceptOf	ns1:source .
ns6:desi_1b2_mbbtu
	rdf:type	ns8:Source , skos:Concept ;
	skos:prefLabel	"Communications Committee survey" ;
	foaf:page	<http://digital-agenda-data.eu/charts/analyse-one-indicator-and-compare-countries#chart={\u0022indicator-group\u0022:\u0022any\u0022,\u0022indicator\u0022:\u0022mbb_penet\u0022,\u0022breakdown\u0022:\u0022TOTAL_MBB\u0022,\u0022unit-measure\u0022:\u0022subs_per_100_pop\u0022,\u0022ref-area\u0022:[\u0022BE\u0022,\u0022BG\u0022,\u0022CZ\u0022,\u0022DK\u0022,\u0022DE\u0022,\u0022EE\u0022,\u0022IE\u0022,\u0022EL\u0022,\u0022ES\u0022,\u0022FR\u0022,\u0022IT\u0022,\u0022CY\u0022,\u0022LV\u0022,\u0022LT\u0022,\u0022LU\u0022,\u0022HU\u0022,\u0022HR\u0022,\u0022MT\u0022,\u0022NL\u0022,\u0022AT\u0022,\u0022PL\u0022,\u0022PT\u0022,\u0022RO\u0022,\u0022SI\u0022,\u0022SK\u0022,\u0022FI\u0022,\u0022SE\u0022,\u0022UK\u0022,\u0022EU\u0022]}> ;
	skos:notation	"desi_1b2_mbbtu" ;
	skos:definition	"European Commission services, through the Communications Committee (COCOM)" ;
	skos:topConceptOf	ns1:source .
ns6:desi_1c1_ngac
	rdf:type	ns8:Source , skos:Concept ;
	skos:prefLabel	"Broadband coverage in Europe Study" ;
	foaf:page	<http://digital-agenda-data.eu/charts/analyse-one-indicator-and-compare-countries#chart={\u0022indicator-group\u0022:\u0022any\u0022,\u0022indicator\u0022:\u0022bb_ngacov\u0022,\u0022breakdown\u0022:\u0022TOTAL_POPHH\u0022,\u0022unit-measure\u0022:\u0022pc_hh_all\u0022,\u0022ref-area\u0022:[\u0022AT\u0022,\u0022BE\u0022,\u0022BG\u0022,\u0022HR\u0022,\u0022CY\u0022,\u0022CZ\u0022,\u0022DK\u0022,\u0022EE\u0022,\u0022EU\u0022,\u0022FI\u0022,\u0022FR\u0022,\u0022DE\u0022,\u0022EL\u0022,\u0022HU\u0022,\u0022IE\u0022,\u0022IT\u0022,\u0022LV\u0022,\u0022LT\u0022,\u0022LU\u0022,\u0022MT\u0022,\u0022NL\u0022,\u0022PL\u0022,\u0022PT\u0022,\u0022RO\u0022,\u0022SK\u0022,\u0022SI\u0022,\u0022ES\u0022,\u0022SE\u0022,\u0022UK\u0022]}> ;
	skos:notation	"desi_1c1_ngac" ;
	skos:definition	"Broadband coverage in Europe, studies for the EC by IHS and Valdani, Vicari & Associati (2013-2015, SMART 2013/0054) and by IHS and Point Topic (2016 onwards, SMART 2016/0045)" ;
	skos:topConceptOf	ns1:source .
ns6:desi_1c2_sfbb
	rdf:type	ns8:Source , skos:Concept ;
	skos:prefLabel	"Communications Committee Survey" ;
	foaf:page	<http://digital-agenda-data.eu/charts/analyse-one-indicator-and-compare-countries#chart={\u0022indicator-group\u0022:\u0022any\u0022,\u0022indicator\u0022:\u0022bb_speed30\u0022,\u0022breakdown\u0022:\u0022TOTAL_FBB\u0022,\u0022unit-measure\u0022:\u0022pc_lines\u0022,\u0022ref-area\u0022:[\u0022AT\u0022,\u0022BE\u0022,\u0022BG\u0022,\u0022HR\u0022,\u0022CY\u0022,\u0022CZ\u0022,\u0022DK\u0022,\u0022EE\u0022,\u0022EU\u0022,\u0022FI\u0022,\u0022FR\u0022,\u0022DE\u0022,\u0022EL\u0022,\u0022HU\u0022,\u0022IE\u0022,\u0022IT\u0022,\u0022LV\u0022,\u0022LT\u0022,\u0022LU\u0022,\u0022MT\u0022,\u0022NL\u0022,\u0022PL\u0022,\u0022PT\u0022,\u0022RO\u0022,\u0022SK\u0022,\u0022SI\u0022,\u0022ES\u0022,\u0022SE\u0022,\u0022UK\u0022]}> ;
	skos:notation	"desi_1c2_sfbb" ;
	skos:definition	"European  Commission services, through the Communications Committee (COCOM) and Eurostat Eurostat - Community survey on ICT usage in Households and by People" ;
	skos:topConceptOf	ns1:source .
ns6:desi_1d1_ubbc
	rdf:type	ns8:Source , skos:Concept ;
	skos:prefLabel	"Broadband coverage in Europe Study" ;
	skos:notation	"desi_1d1_ubbc" ;
	skos:definition	"Broadband coverage in Europe, studies for the EC by IHS and Valdani, Vicari & Associati (2013-2015, SMART 2013/0054) and by IHS and Point Topic (2016 onwards, SMART 2016/0045)" ;
	skos:topConceptOf	ns1:source .
ns6:desi_1d2_ubbta
	rdf:type	ns8:Source , skos:Concept ;
	skos:prefLabel	"Communications Committee Survey" ;
	skos:notation	"desi_1d2_ubbta" ;
	skos:definition	"European  Commission services, through the Communications Committee (COCOM) and Eurostat Eurostat - Community survey on ICT usage in Households and by People" ;
	skos:topConceptOf	ns1:source .
ns6:desi_1e1_bbpi
	rdf:type	ns8:Source , skos:Concept ;
	skos:prefLabel	"Broadband Price Index Study" ;
	skos:notation	"desi_1e1_bbpi" ;
	skos:definition	"Access cost: Broadband Internet Access Cost (BIAC), annual studies for the EC realised by Van Dijk (2013-2015) and by Empirica (2016 onwards). Income: Real adjusted gross disposable income of households per capita (Eurostat: tec00113)" ;
	skos:topConceptOf	ns1:source .
ns6:desi_2b1_ictspec
	rdf:type	ns8:Source , skos:Concept ;
	skos:prefLabel	"Eurostat - Labour force survey" ;
	skos:notation	"desi_2b1_ictspec" ;
	skos:definition	"Eurostat - Labour force survey" ;
	skos:topConceptOf	ns1:source .
ns6:desi_3c1_bank
	rdf:type	ns8:Source , skos:Concept ;
	skos:prefLabel	"Eurostat Survey - ICT usage in Households and by People" ;
	foaf:page	<http://digital-agenda-data.eu/charts/analyse-one-indicator-and-compare-countries#chart={\u0022indicator-group\u0022:\u0022any\u0022,\u0022indicator\u0022:\u0022i_iubk\u0022,\u0022breakdown\u0022:\u0022IND_TOTAL\u0022,\u0022unit-measure\u0022:\u0022pc_ind_iu3\u0022,\u0022ref-area\u0022:[\u0022AT\u0022,\u0022BE\u0022,\u0022BG\u0022,\u0022HR\u0022,\u0022CY\u0022,\u0022CZ\u0022,\u0022DK\u0022,\u0022EE\u0022,\u0022EU\u0022,\u0022FI\u0022,\u0022FR\u0022,\u0022DE\u0022,\u0022EL\u0022,\u0022HU\u0022,\u0022IE\u0022,\u0022IT\u0022,\u0022LV\u0022,\u0022LT\u0022,\u0022LU\u0022,\u0022MT\u0022,\u0022NL\u0022,\u0022PL\u0022,\u0022PT\u0022,\u0022RO\u0022,\u0022SK\u0022,\u0022SI\u0022,\u0022ES\u0022,\u0022SE\u0022,\u0022UK\u0022]}> ;
	skos:notation	"desi_3c1_bank" ;
	skos:definition	"Eurostat - Community survey on ICT usage in Households and by Individuals (I_IUBK)" ;
	skos:topConceptOf	ns1:source .
ns6:desi_3c2_shop
	rdf:type	ns8:Source , skos:Concept ;
	skos:prefLabel	"Eurostat Survey - ICT usage in Households and by People" ;
	foaf:page	<http://digital-agenda-data.eu/charts/analyse-one-indicator-and-compare-countries#chart={\u0022indicator-group\u0022:\u0022any\u0022,\u0022indicator\u0022:\u0022i_blt12\u0022,\u0022breakdown\u0022:\u0022IND_TOTAL\u0022,\u0022unit-measure\u0022:\u0022pc_ind_ilt12\u0022,\u0022ref-area\u0022:[\u0022AT\u0022,\u0022BE\u0022,\u0022BG\u0022,\u0022HR\u0022,\u0022CY\u0022,\u0022CZ\u0022,\u0022DK\u0022,\u0022EE\u0022,\u0022EU\u0022,\u0022FI\u0022,\u0022FR\u0022,\u0022DE\u0022,\u0022EL\u0022,\u0022HU\u0022,\u0022IE\u0022,\u0022IT\u0022,\u0022LV\u0022,\u0022LT\u0022,\u0022LU\u0022,\u0022MT\u0022,\u0022NL\u0022,\u0022PL\u0022,\u0022PT\u0022,\u0022RO\u0022,\u0022SK\u0022,\u0022SI\u0022,\u0022ES\u0022,\u0022SE\u0022,\u0022UK\u0022]}> ;
	skos:notation	"desi_3c2_shop" ;
	skos:definition	"Eurostat - Community survey on ICT usage in Households and by Individuals (I_BLT12)" ;
	skos:topConceptOf	ns1:source .
ns6:desi_4a1_eis
	rdf:type	ns8:Source , skos:Concept ;
	skos:prefLabel	"Eurostat - ICT Enterprises survey" ;
	foaf:page	<http://digital-agenda-data.eu/charts/analyse-one-indicator-and-compare-countries#chart={\u0022indicator-group\u0022:\u0022any\u0022,\u0022indicator\u0022:\u0022e_erp1\u0022,\u0022breakdown\u0022:\u0022ent_all_xfin\u0022,\u0022unit-measure\u0022:\u0022pc_ent\u0022,\u0022ref-area\u0022:[\u0022AT\u0022,\u0022BE\u0022,\u0022BG\u0022,\u0022HR\u0022,\u0022CY\u0022,\u0022CZ\u0022,\u0022DK\u0022,\u0022EE\u0022,\u0022EU\u0022,\u0022FI\u0022,\u0022FR\u0022,\u0022DE\u0022,\u0022EL\u0022,\u0022HU\u0022,\u0022IE\u0022,\u0022IT\u0022,\u0022LV\u0022,\u0022LT\u0022,\u0022LU\u0022,\u0022MT\u0022,\u0022NL\u0022,\u0022PL\u0022,\u0022PT\u0022,\u0022RO\u0022,\u0022SK\u0022,\u0022SI\u0022,\u0022ES\u0022,\u0022SE\u0022,\u0022UK\u0022]}> ;
	skos:notation	"desi_4a1_eis" ;
	skos:definition	"Eurostat - Community survey on ICT usage and eCommerce in Enterprises (E_ERP1)" ;
	skos:topConceptOf	ns1:source .
ns6:desi_4b1_smeso
	rdf:type	ns8:Source , skos:Concept ;
	skos:prefLabel	"Eurostat - ICT Enterprises survey" ;
	foaf:page	<http://digital-agenda-data.eu/charts/analyse-one-indicator-and-compare-countries#chart={\u0022indicator-group\u0022:\u0022any\u0022,\u0022indicator\u0022:\u0022e_esell\u0022,\u0022breakdown\u0022:\u0022ent_sm_xfin\u0022,\u0022unit-measure\u0022:\u0022pc_ent\u0022,\u0022ref-area\u0022:[\u0022AT\u0022,\u0022BE\u0022,\u0022BG\u0022,\u0022HR\u0022,\u0022CY\u0022,\u0022CZ\u0022,\u0022DK\u0022,\u0022EE\u0022,\u0022EU\u0022,\u0022FI\u0022,\u0022FR\u0022,\u0022DE\u0022,\u0022EL\u0022,\u0022HU\u0022,\u0022IE\u0022,\u0022IT\u0022,\u0022LV\u0022,\u0022LT\u0022,\u0022LU\u0022,\u0022MT\u0022,\u0022NL\u0022,\u0022PL\u0022,\u0022PT\u0022,\u0022RO\u0022,\u0022SK\u0022,\u0022SI\u0022,\u0022ES\u0022,\u0022SE\u0022,\u0022UK\u0022]}> ;
	skos:notation	"desi_4b1_smeso" ;
	skos:definition	"Eurostat - Community survey on ICT usage and eCommerce in Enterprises (E_ESELL)" ;
	skos:topConceptOf	ns1:source .
ns6:desi_4b2_ecomturn
	rdf:type	ns8:Source , skos:Concept ;
	skos:prefLabel	"Eurostat - ICT Enterprises survey" ;
	foaf:page	<http://digital-agenda-data.eu/charts/analyse-one-indicator-and-compare-countries#chart={\u0022indicator-group\u0022:\u0022any\u0022,\u0022indicator\u0022:\u0022e_eturn\u0022,\u0022breakdown\u0022:\u0022ent_sm_xfin\u0022,\u0022unit-measure\u0022:\u0022pc_turn\u0022,\u0022ref-area\u0022:[\u0022AT\u0022,\u0022BE\u0022,\u0022BG\u0022,\u0022HR\u0022,\u0022CY\u0022,\u0022CZ\u0022,\u0022DK\u0022,\u0022EE\u0022,\u0022EU\u0022,\u0022FR\u0022,\u0022DE\u0022,\u0022EL\u0022,\u0022HU\u0022,\u0022IE\u0022,\u0022IT\u0022,\u0022LV\u0022,\u0022LT\u0022,\u0022LU\u0022,\u0022MT\u0022,\u0022NL\u0022,\u0022PL\u0022,\u0022PT\u0022,\u0022RO\u0022,\u0022SK\u0022,\u0022ES\u0022,\u0022SE\u0022,\u0022UK\u0022]}> ;
	skos:notation	"desi_4b2_ecomturn" ;
	skos:definition	"Eurostat - Community survey on ICT usage and eCommerce in Enterprises (E_ETURN) " ;
	skos:topConceptOf	ns1:source .
ns6:desi_4b3_sellcb
	rdf:type	ns8:Source , skos:Concept ;
	skos:prefLabel	"Eurostat - ICT Enterprises survey" ;
	foaf:page	<http://digital-agenda-data.eu/charts/analyse-one-indicator-and-compare-countries#chart={\u0022indicator-group\u0022:\u0022any\u0022,\u0022indicator\u0022:\u0022e_aeseu\u0022,\u0022breakdown\u0022:\u0022ent_sm_xfin\u0022,\u0022unit-measure\u0022:\u0022pc_ent\u0022,\u0022ref-area\u0022:[\u0022AT\u0022,\u0022BE\u0022,\u0022BG\u0022,\u0022HR\u0022,\u0022CY\u0022,\u0022CZ\u0022,\u0022DK\u0022,\u0022EE\u0022,\u0022EU\u0022,\u0022FR\u0022,\u0022DE\u0022,\u0022EL\u0022,\u0022HU\u0022,\u0022IE\u0022,\u0022IT\u0022,\u0022LV\u0022,\u0022LT\u0022,\u0022LU\u0022,\u0022MT\u0022,\u0022NL\u0022,\u0022PL\u0022,\u0022PT\u0022,\u0022RO\u0022,\u0022SK\u0022,\u0022ES\u0022,\u0022SE\u0022,\u0022UK\u0022]}> ;
	skos:notation	"desi_4b3_sellcb" ;
	skos:definition	"Eurostat - Community survey on ICT usage and eCommerce in Enterprises (E_AESEU)" ;
	skos:topConceptOf	ns1:source .
ns6:desi_5a1_egovu
	rdf:type	ns8:Source , skos:Concept ;
	skos:prefLabel	"Eurostat Survey - ICT usage in Households and by People" ;
	foaf:page	<https://digital-agenda-data.eu/charts/analyse-one-indicator-and-compare-countries#chart={%22indicator-group%22:%22any%22,%22indicator%22:%22i_igov12rt%22,%22breakdown%22:%22IND_TOTAL%22,%22unit-measure%22:%22pc_ind_igov12nrt%22,%22ref-area%22:[%22AT%22,%22BE%22,%22BG%22,%22HR%22,%22CY%22,%22CZ%22,%22DK%22,%22EE%22,%22EU%22,%22FR%22,%22DE%22,%22EL%22,%22HU%22,%22IE%22,%22IT%22,%22LV%22,%22LT%22,%22LU%22,%22MT%22,%22NL%22,%22PL%22,%22PT%22,%22RO%22,%22SK%22,%22ES%22,%22SE%22,%22UK%22]}> ;
	skos:notation	"desi_5a1_egovu" ;
	skos:definition	"Eurostat - Community survey on ICT usage in Households and by Individuals (IGOV12RT)" ;
	skos:topConceptOf	ns1:source .
ns6:desi_5a2_prefform
	rdf:type	ns8:Source , skos:Concept ;
	skos:prefLabel	"eGovernment Benchmarking Report" ;
	foaf:page	ns13:egovernment-benchmark-2018-digital-efforts-european-countries-are-visibly-paying ;
	skos:notation	"desi_5a2_prefform" ;
	skos:definition	"eGovernment Benchmarking Report" ;
	skos:topConceptOf	ns1:source .
ns6:desi_5a3_osercomp
	rdf:type	ns8:Source , skos:Concept ;
	skos:prefLabel	"eGovernment Benchmarking Report" ;
	foaf:page	ns13:egovernment-benchmark-2018-digital-efforts-european-countries-are-visibly-paying ;
	skos:notation	"desi_5a3_osercomp" ;
	skos:definition	"eGovernment Benchmarking Report" ;
	skos:topConceptOf	ns1:source .
ns6:desi_5a4_psb
	rdf:type	ns8:Source , skos:Concept ;
	skos:prefLabel	"eGovernment Benchmarking Report" ;
	foaf:page	ns13:egovernment-benchmark-2018-digital-efforts-european-countries-are-visibly-paying ;
	skos:notation	"desi_5a4_psb" ;
	skos:definition	"eGovernment Benchmarking Report" ;
	skos:topConceptOf	ns1:source .
ns6:desi_5a5_opendata
	rdf:type	ns8:Source , skos:Concept ;
	skos:prefLabel	"European Data Portal" ;
	foaf:page	ns14:dashboard ;
	skos:notation	"desi_5a5_opendata" ;
	skos:definition	"European Data Portal" ;
	skos:topConceptOf	ns1:source .
ns6:desi_5b1_ehs
	rdf:type	ns8:Source , skos:Concept ;
	skos:prefLabel	"Eurobarometer 460: Attitudes towards the impact of digitisation and automation on daily life" ;
	foaf:page	ns13:attitudes-towards-impact-digitisation-and-automation-daily-life ;
	skos:notation	"desi_5b1_ehs" ;
	skos:definition	"Eurobarometer 460: Attitudes towards the impact of digitisation and automation on daily life" ;
	skos:topConceptOf	ns1:source .
ns6:eco_report_03_efis_comm
	rdf:type	ns8:Source , skos:Concept ;
	skos:prefLabel	"ECO Report 03" ;
	foaf:page	ns15:eco-reports ;
	skos:notation	"eco_report_03_efis_comm" ;
	skos:definition	"ECO Report 03, based on EFIS database, completed with direct communications between EU and Member States" ;
	skos:topConceptOf	ns1:source .
ns6:egov_bench12
	rdf:type	ns8:Source , skos:Concept ;
	skos:prefLabel	"eGovernment Benchmarking reports 2012-2014" ;
	foaf:page	<https://ec.europa.eu/digital-agenda/news-redirect/16475> ;
	skos:notation	"egov_bench12" ;
	skos:definition	"eGovernment Benchmarking Report, Studies for the EC peformed by Capgemini (2012-2014)" ;
	skos:topConceptOf	ns1:source .
ns6:egov_bench12_17
	rdf:type	ns8:Source , skos:Concept ;
	skos:prefLabel	"eGovernment Benchmarking Report, Studies for the EC performed by Capgemini (2012-2017)\u00A0" ;
	foaf:page	ns13:new-study-egovernment-services-europe-improving-cross-border-availability-services ;
	skos:notation	"egov_bench12_17" ;
	skos:definition	"eGovernment Benchmarking Report, Studies for the EC performed by Capgemini (2012-2017)\u00A0" ;
	skos:topConceptOf	ns1:source .
ns6:einfraegi
	rdf:type	ns8:Source , skos:Concept ;
	skos:prefLabel	"e-infrastructure project EGI" ;
	foaf:page	<http://www.egi.eu> ;
	skos:notation	"einfraegi" ;
	skos:definition	"e-infrastructure project EGI" ;
	skos:topConceptOf	ns1:source .
ns6:einfrageant
	rdf:type	ns8:Source , skos:Concept ;
	skos:prefLabel	"e-infrastructure project G\u00E9ant" ;
	foaf:page	<http://www.geant.net> ;
	skos:notation	"einfrageant" ;
	skos:definition	"e-infrastructure project G\u00E9ant" ;
	skos:topConceptOf	ns1:source .
ns6:einfraprace
	rdf:type	ns8:Source , skos:Concept ;
	skos:prefLabel	"e-infrastructure project PRACE" ;
	foaf:page	<http://www.prace-ri.eu> ;
	skos:notation	"einfraprace" ;
	skos:definition	"e-infrastructure project PRACE" ;
	skos:topConceptOf	ns1:source .
ns6:eoa_smart12-26
	rdf:type	ns8:Source , skos:Concept ;
	skos:prefLabel	"European Audiovisual Observatory - study \"On demand audiovisual markets in the EU\"" ;
	foaf:page	ns10:demand-audiovisual-markets-european-union-smart-20120028 ;
	skos:notation	"eoa_smart12-26" ;
	skos:definition	"European Audiovisual Observatory - study \"On demand audiovisual markets in the EU\", of April 2014 (smart 2012-0026)" ;
	skos:note	"page 20 table 4" ;
	skos:topConceptOf	ns1:source .
ns6:eoa_yearbook2014
	rdf:type	ns8:Source , skos:Concept ;
	skos:prefLabel	"European Audiovisual Observatory Yearbook 2014" ;
	foaf:page	ns16:premiumservice ;
	skos:notation	"eoa_yearbook2014" ;
	skos:definition	"European Audiovisual Observatory Yearbook 2014" ;
	skos:topConceptOf	ns1:source .
ns6:epsi
	rdf:type	ns8:Source , skos:Concept ;
	skos:prefLabel	"The PSI Scoreboard" ;
	foaf:page	ns17:european-psi-scoreboard ;
	skos:notation	"epsi" ;
	skos:definition	"The PSI Scoreboard is a \u2018crowdsourced\u2019 tool to measure the status of Open Data and PSI re-use throughout the EU." ;
	skos:topConceptOf	ns1:source .
ns6:epsiplatform
	rdf:type	ns8:Source , skos:Concept ;
	skos:prefLabel	"The PSI Scoreboard" ;
	foaf:page	ns17:european-psi-scoreboard ;
	skos:notation	"epsiplatform" ;
	skos:definition	"The PSI Scoreboard is a \u2018crowdsourced\u2019 tool to measure the status of Open Data and PSI re-use throughout the EU. It does NOT monitor government policies, but aims to assess the overall PSI re-use situation, which includes the open data community's activities." ;
	skos:topConceptOf	ns1:source .
ns6:estat-ent
	rdf:type	ns8:Source , skos:Concept ;
	skos:prefLabel	"Eurostat - ICT Enterprises survey" ;
	foaf:page	ns18:comprehensive-database ;
	skos:notation	"estat-ent" ;
	skos:definition	"Eurostat - Community survey on ICT usage and eCommerce in Enterprises <a href=\"http://ec.europa.eu/eurostat/web/digital-economy-and-society/data/comprehensive-database\">More information</a>." ;
	skos:note	"Extraction from ENT2 comprehensive database (NACE Rev 2 in ACCESS 133 MB) version 16 Apr 2013, and from ENT (NACE Rev 1.1 in ACCESS 104 MB) version 12 Dec 2011." ;
	skos:topConceptOf	ns1:source .
ns6:estat-hh
	rdf:type	ns8:Source , skos:Concept ;
	skos:prefLabel	"Eurostat - ICT Households survey" ;
	foaf:page	ns18:comprehensive-database ;
	skos:notation	"estat-hh" ;
	skos:definition	"Eurostat - Community survey on ICT usage in Households and by Individuals <a href=\"http://ec.europa.eu/eurostat/web/digital-economy-and-society/data/comprehensive-database\">More information</a>." ;
	skos:note	"Extraction from HH/Indiv comprehensive database (ACCESS) version\u00A029 April 2013" ;
	skos:topConceptOf	ns1:source .
ns6:estat-lfs
	rdf:type	ns8:Source , skos:Concept ;
	skos:prefLabel	"Eurostat - Labour Force Survey" ;
	foaf:page	ns19:database ;
	skos:notation	"estat-lfs" ;
	skos:definition	"Eurostat - Labour Force Survey" ;
	skos:note	"Extraction May 2013, ESTAT-G6" ;
	skos:topConceptOf	ns1:source .
ns6:estat-lfs-sks
	rdf:type	ns8:Source , skos:Concept ;
	skos:prefLabel	"Eurostat - ICT specialist statistics (derived from Labour Force Survey)" ;
	foaf:page	<http://ec.europa.eu/eurostat/cache/metadata/en/isoc_skslf_esms.htm> ;
	skos:notation	"estat-lfs-sks" ;
	skos:definition	"Eurostat - ICT specialist statistics (derived from Labour Force Survey)" ;
	skos:topConceptOf	ns1:source .
ns6:estat-trade
	rdf:type	ns8:Source , skos:Concept ;
	skos:prefLabel	"Eurostat - Trade statistics" ;
	foaf:page	ns20:database ;
	skos:notation	"estat-trade" ;
	skos:definition	"Eurostat - Trade statistics" ;
	skos:note	"Extraction May 2013, ESTAT-G6" ;
	skos:topConceptOf	ns1:source .
ns6:estat_gba_nabsfin07
	rdf:type	ns8:Source , skos:Concept ;
	skos:prefLabel	"Eurostat, Table gba_nabsfin07: Total GBAORD by NABS 2007 socio-economic objectives" ;
	foaf:page	ns21:gba_nabsfin07 ;
	skos:notation	"estat_gba_nabsfin07" ;
	skos:definition	"Eurostat, Table gba_nabsfin07: Total GBAORD by NABS 2007 socio-economic objectives" ;
	skos:note	"Double check? Predict?" ;
	skos:topConceptOf	ns1:source .
ns6:estat_isoc_bde15b_e
	rdf:type	ns8:Source , skos:Concept ;
	skos:prefLabel	"Eurostat, Table isoc_bde15b_e: Broadband and connectivity - enterprises" ;
	foaf:page	ns21:isoc_bde15b_e ;
	skos:notation	"estat_isoc_bde15b_e" ;
	skos:definition	"Eurostat, Table isoc_bde15b_e: Broadband and connectivity - enterprises" ;
	skos:topConceptOf	ns1:source .
ns6:estat_isoc_bde15b_h
	rdf:type	ns8:Source , skos:Concept ;
	skos:prefLabel	"Eurostat, Table isoc_bde15b_h: Broadband and connectivity - households" ;
	foaf:page	ns21:isoc_bde15b_h ;
	skos:notation	"estat_isoc_bde15b_h" ;
	skos:definition	"Eurostat, Table isoc_bde15b_h: Broadband and connectivity - households" ;
	skos:topConceptOf	ns1:source .
ns6:estat_isoc_bde15b_p
	rdf:type	ns8:Source , skos:Concept ;
	skos:prefLabel	"Eurostat, Table isoc_bde15b_p: Broadband and connectivity - persons employed" ;
	foaf:page	ns21:isoc_bde15b_p ;
	skos:notation	"estat_isoc_bde15b_p" ;
	skos:definition	"Eurostat, Table isoc_bde15b_p: Broadband and connectivity - persons employed" ;
	skos:topConceptOf	ns1:source .
ns6:estat_isoc_bde15cbc
	rdf:type	ns8:Source , skos:Concept ;
	skos:prefLabel	"Eurostat, Table isoc_bde15cbc: E-banking and e-commerce" ;
	foaf:page	ns21:isoc_bde15cbc ;
	skos:notation	"estat_isoc_bde15cbc" ;
	skos:definition	"Eurostat, Table isoc_bde15cbc: E-banking and e-commerce" ;
	skos:topConceptOf	ns1:source .
ns6:estat_isoc_bde15cua
	rdf:type	ns8:Source , skos:Concept ;
	skos:prefLabel	"Eurostat, Table isoc_bde15cua: Internet use and activities" ;
	foaf:page	ns21:isoc_bde15cua ;
	skos:notation	"estat_isoc_bde15cua" ;
	skos:definition	"Eurostat, Table isoc_bde15cua: Internet use and activities" ;
	skos:topConceptOf	ns1:source .
ns6:estat_isoc_bde15dec
	rdf:type	ns8:Source , skos:Concept ;
	skos:prefLabel	"Eurostat, Table estat_isoc_bde15dec: E-commerce, customer relation management (CRM) and secure transactions" ;
	foaf:page	ns21:isoc_bde15dec ;
	skos:notation	"estat_isoc_bde15dec" ;
	skos:definition	"Eurostat, Table estat_isoc_bde15dec: E-commerce, customer relation management (CRM) and secure transactions" ;
	skos:topConceptOf	ns1:source .
ns6:estat_isoc_bde15dip
	rdf:type	ns8:Source , skos:Concept ;
	skos:prefLabel	"Eurostat, Table isoc_bde15dip: Integration of internal processes" ;
	foaf:page	ns21:isoc_bde15dip ;
	skos:notation	"estat_isoc_bde15dip" ;
	skos:definition	"Eurostat, Table isoc_bde15dip: Integration of internal processes" ;
	skos:topConceptOf	ns1:source .
ns6:estat_isoc_bde15disc
	rdf:type	ns8:Source , skos:Concept ;
	skos:prefLabel	"Eurostat, Table isoc_bde15disc: Integration with customers/suppliers and SCM" ;
	foaf:page	ns21:isoc_bde15disc ;
	skos:notation	"estat_isoc_bde15disc" ;
	skos:definition	"Eurostat, Table isoc_bde15disc: Integration with customers/suppliers and SCM" ;
	skos:topConceptOf	ns1:source .
ns6:estat_isoc_bde15dth
	rdf:type	ns8:Source , skos:Concept ;
	skos:prefLabel	"Eurostat, Table isoc_bde15dth: Key technologies for the internet of things" ;
	foaf:page	ns21:isoc_bde15dth ;
	skos:notation	"estat_isoc_bde15dth" ;
	skos:definition	"Eurostat, Table isoc_bde15dth: Key technologies for the internet of things" ;
	skos:topConceptOf	ns1:source .
ns6:estat_isoc_bde15ee
	rdf:type	ns8:Source , skos:Concept ;
	skos:prefLabel	"Eurostat, Table isoc_bde15ee: Enterprises using the internet for interacting with public authorities" ;
	foaf:page	ns21:isoc_bde15ee ;
	skos:notation	"estat_isoc_bde15ee" ;
	skos:definition	"Eurostat, Table isoc_bde15ee: Enterprises using the internet for interacting with public authorities" ;
	skos:topConceptOf	ns1:source .
ns6:estat_isoc_ci_ac_i
	rdf:type	ns8:Source , skos:Concept ;
	skos:prefLabel	"Eurostat, Table isoc_ci_ac_i: Individuals - internet activities" , "Eurostat, Table isoc_ci_ac_i: Internet activities - individuals" ;
	foaf:page	ns21:isoc_ci_ac_i ;
	skos:notation	"estat_isoc_ci_ac_i" ;
	skos:definition	"Eurostat, Table isoc_pibi_ioa: Individuals doing specific online activities in the previous 3 months" , "Eurostat - Community survey on ICT usage in Households and by Individuals, Table: Internet activities - individuals" ;
	skos:topConceptOf	ns1:source .
ns6:estat_isoc_ci_eu_en2
	rdf:type	ns8:Source , skos:Concept ;
	skos:prefLabel	"Eurostat, Table isoc_ci_eu_en2: Computers and the internet: enterprises - summary of EU aggregates (NACE Rev. 2 activity) " , "Eurostat, Table isoc_ci_eu_en2: Computers and the internet: enterprises - summary of EU aggregates (NACE Rev. 2 activity)" ;
	foaf:page	ns21:isoc_ci_eu_en2 ;
	skos:notation	"estat_isoc_ci_eu_en2" ;
	skos:definition	"Eurostat, Table isoc_ci_eu_en2: Computers and the internet: enterprises - summary of EU aggregates (NACE Rev. 2 activity) " , "Eurostat, Table isoc_ci_eu_en2: Computers and the internet: enterprises - summary of EU aggregates (NACE Rev. 2 activity)" ;
	skos:topConceptOf	ns1:source .
ns6:estat_isoc_ci_eu_i
	rdf:type	ns8:Source , skos:Concept ;
	skos:prefLabel	"Eurostat, Table isoc_ci_eu_i: Computers and the internet: individuals - summary of EU aggregates" ;
	foaf:page	ns21:isoc_ci_eu_i ;
	skos:notation	"estat_isoc_ci_eu_i" ;
	skos:definition	"Eurostat, Table isoc_ci_eu_i: Computers and the internet: individuals - summary of EU aggregates" ;
	skos:topConceptOf	ns1:source .
ns6:estat_isoc_ci_ifp_fu
	rdf:type	ns8:Source , skos:Concept ;
	skos:prefLabel	"Eurostat, Table isoc_ci_ifp_fu: Frequency of internet use  - individuals" ;
	foaf:page	ns21:isoc_ci_ifp_fu ;
	skos:notation	"estat_isoc_ci_ifp_fu" ;
	skos:definition	"Eurostat, Table isoc_ci_ifp_fu: Frequency of internet use  - individuals" ;
	skos:topConceptOf	ns1:source .
ns6:estat_isoc_ci_ifp_iu
	rdf:type	ns8:Source , skos:Concept ;
	skos:prefLabel	"Eurostat, Table isoc_ci_ifp_iu: Internet use  - individuals" ;
	foaf:page	ns21:isoc_ci_ifp_iu ;
	skos:notation	"estat_isoc_ci_ifp_iu" ;
	skos:definition	"Eurostat, Table isoc_ci_ifp_iu: Internet use  - individuals" ;
	skos:topConceptOf	ns1:source .
ns6:estat_isoc_ci_im_i
	rdf:type	ns8:Source , skos:Concept ;
	skos:prefLabel	"Eurostat, Table isoc_ci_im_i: Mobile internet access  - individuals" ;
	foaf:page	ns21:isoc_ci_im_i ;
	skos:notation	"estat_isoc_ci_im_i" ;
	skos:definition	"Eurostat, Table isoc_ci_im_i: Mobile internet access  - individuals" ;
	skos:topConceptOf	ns1:source .
ns6:estat_isoc_cicce_use
	rdf:type	ns8:Source , skos:Concept ;
	skos:prefLabel	"Eurostat, Table isoc_cicce_use: Cloud computing services" ;
	foaf:page	ns21:isoc_cicce_use ;
	skos:notation	"estat_isoc_cicce_use" ;
	skos:definition	"Eurostat, Table isoc_cicce_use: Cloud computing services" ;
	skos:topConceptOf	ns1:source .
ns6:estat_isoc_cisci_ax
	rdf:type	ns8:Source , skos:Concept ;
	skos:prefLabel	"Eurostat, Table isoc_cisci_ax: Activities via internet not done because of security concerns" ;
	foaf:page	ns21:isoc_cisci_ax ;
	skos:notation	"estat_isoc_cisci_ax" ;
	skos:definition	"Eurostat, Table isoc_cisci_ax: Activities via internet not done because of security concerns" ;
	skos:topConceptOf	ns1:source .
ns6:estat_isoc_cisci_pb
	rdf:type	ns8:Source , skos:Concept ;
	skos:prefLabel	"Eurostat, Table isoc_cisci_pb: Security related problems experienced through using the internet for private purposes" ;
	foaf:page	ns21:isoc_cisci_pb ;
	skos:notation	"estat_isoc_cisci_pb" ;
	skos:definition	"Eurostat, Table isoc_cisci_pb: Security related problems experienced through using the internet for private purposes" ;
	skos:topConceptOf	ns1:source .
ns6:estat_isoc_cisci_prv
	rdf:type	ns8:Source , skos:Concept ;
	skos:prefLabel	"Eurostat, Table isoc_cisci_prv: Privacy and protection of personal information" ;
	foaf:page	ns21:isoc_cisci_prv ;
	skos:notation	"estat_isoc_cisci_prv" ;
	skos:definition	"Eurostat, Table isoc_cisci_prv: Privacy and protection of personal information" ;
	skos:topConceptOf	ns1:source .
ns6:estat_isoc_cismt
	rdf:type	ns8:Source , skos:Concept ;
	skos:prefLabel	"Eurostat, Table isoc_cismt: Social media use by type" ;
	foaf:page	ns21:isoc_cismt ;
	skos:notation	"estat_isoc_cismt" ;
	skos:definition	"Eurostat, Table isoc_cismt: Social media use by type" ;
	skos:topConceptOf	ns1:source .
ns6:estat_isoc_ec_eseln2
	rdf:type	ns8:Source , skos:Concept ;
	skos:prefLabel	"Eurostat, Table isoc_ec_eseln2: Enterprises selling via internet and/or networks other than internet (NACE Rev. 2 activity)" ;
	foaf:page	ns21:isoc_ec_eseln2 ;
	skos:notation	"estat_isoc_ec_eseln2" ;
	skos:definition	"Eurostat, Table isoc_ec_eseln2: Enterprises selling via internet and/or networks other than internet (NACE Rev. 2 activity)" ;
	skos:topConceptOf	ns1:source .
ns6:estat_isoc_ec_ibuy
	rdf:type	ns8:Source , skos:Concept ;
	skos:prefLabel	"Eurostat, Table isoc_ec_ibuy: Internet purchases by individuals" ;
	foaf:page	ns21:isoc_ec_ibuy ;
	skos:notation	"estat_isoc_ec_ibuy" ;
	skos:definition	"Eurostat, Table isoc_ec_ibuy: Internet purchases by individuals" ;
	skos:topConceptOf	ns1:source .
ns6:estat_isoc_ec_iprb
	rdf:type	ns8:Source , skos:Concept ;
	skos:prefLabel	"eurostat table isoc_ec_iprb " ;
	foaf:page	<http://appsso.eurostat.ec.europa.eu/nui/show.do?dataset=isoc_ec_iprb&lang=en> ;
	skos:notation	"estat_isoc_ec_iprb" ;
	skos:definition	"eurostat table isoc_ec_iprb Problems encountered by individuals when buying/ordering over the internet " ;
	skos:topConceptOf	ns1:source .
ns6:estat_isoc_pibi_ictbn2
	rdf:type	ns8:Source , skos:Concept ;
	skos:prefLabel	"Eurostat, Table isoc_pibi_ictbn2: Adoption of ICT by businesses (NACE Rev. 2 activity)" ;
	foaf:page	ns21:isoc_pibi_ictbn2 ;
	skos:notation	"estat_isoc_pibi_ictbn2" ;
	skos:definition	"Eurostat, Table isoc_pibi_ictbn2: Adoption of ICT by businesses (NACE Rev. 2 activity)" ;
	skos:topConceptOf	ns1:source .
ns6:estat_isoc_r_gov_i
	rdf:type	ns8:Source , skos:Concept ;
	skos:prefLabel	"Eurostat, Table isoc_r_gov_i: Individuals who used the internet for interaction with public authorities" ;
	foaf:page	ns21:isoc_r_gov_i ;
	skos:notation	"estat_isoc_r_gov_i" ;
	skos:definition	"Eurostat, Table isoc_r_gov_i: Individuals who used the internet for interaction with public authorities" ;
	skos:topConceptOf	ns1:source .
ns6:estat_isoc_r_iuse_i
	rdf:type	ns8:Source , skos:Concept ;
	skos:prefLabel	"Eurostat, Table isoc_r_iuse_i: Individuals who used the internet, frequency of use and activities" ;
	foaf:page	ns21:isoc_r_iuse_i ;
	skos:notation	"estat_isoc_r_iuse_i" ;
	skos:definition	"Eurostat, Table isoc_r_iuse_i: Individuals who used the internet, frequency of use and activities" ;
	skos:topConceptOf	ns1:source .
ns6:estat_isoc_sk_cskl_i
	rdf:type	ns8:Source , skos:Concept ;
	skos:prefLabel	"Eurostat, Table isoc_sk_cskl_i: Individuals' level of computer skills" ;
	foaf:page	ns21:isoc_sk_cskl_i ;
	skos:notation	"estat_isoc_sk_cskl_i" ;
	skos:definition	"Eurostat, Table isoc_sk_cskl_i: Individuals' level of computer skills" ;
	skos:topConceptOf	ns1:source .
ns6:estat_isoc_sk_dskl_i
	rdf:type	ns8:Source , skos:Concept ;
	skos:prefLabel	"Eurostat, Table isoc_sk_dskl_i: Individuals' level of digital skills" ;
	foaf:page	ns21:isoc_sk_dskl_i ;
	skos:notation	"estat_isoc_sk_dskl_i" ;
	skos:definition	"Eurostat, Table isoc_sk_dskl_i: Individuals' level of digital skills" ;
	skos:topConceptOf	ns1:source .
ns6:estat_isoc_sk_how_i
	rdf:type	ns8:Source , skos:Concept ;
	skos:prefLabel	"Eurostat, Table isoc_sk_how_i: Way of obtaining e-skills" ;
	foaf:page	ns21:isoc_sk_how_i ;
	skos:notation	"estat_isoc_sk_how_i" ;
	skos:definition	"Eurostat, Table isoc_sk_how_i: Way of obtaining e-skills" ;
	skos:topConceptOf	ns1:source .
ns6:estat_isoc_sk_iskl_i
	rdf:type	ns8:Source , skos:Concept ;
	skos:prefLabel	"Eurostat, Table isoc_sk_iskl_i:  Individuals' level of internet skills" ;
	foaf:page	ns21:isoc_sk_iskl_i ;
	skos:notation	"estat_isoc_sk_iskl_i" ;
	skos:definition	"Eurostat, Table isoc_sk_iskl_i:  Individuals' level of internet skills" ;
	skos:topConceptOf	ns1:source .
ns6:estat_isoc_ske_ittn2
	rdf:type	ns8:Source , skos:Concept ;
	skos:prefLabel	"Eurostat, Table isoc_ske_ittn2 : Enterprises that provided training to develop/upgrade ICT skills of their personnel (NACE Rev. 2 activity)" ;
	foaf:page	ns21:isoc_ske_ittn2 ;
	skos:notation	"estat_isoc_ske_ittn2" ;
	skos:definition	"Eurostat, Table isoc_ske_ittn2 : Enterprises that provided training to develop/upgrade ICT skills of their personnel (NACE Rev. 2 activity)" ;
	skos:topConceptOf	ns1:source .
ns6:estat_isoc_sks_itspt
	rdf:type	ns8:Source , skos:Concept ;
	skos:prefLabel	"Eurostat, Table isoc_sks_itspt: ICT specialists - total" ;
	foaf:page	ns21:isoc_sks_itspt ;
	skos:notation	"estat_isoc_sks_itspt" ;
	skos:definition	"Eurostat, Table isoc_sks_itspt: ICT specialists - total" ;
	skos:topConceptOf	ns1:source .
ns6:estat_lfst_hhnhwhtc
	rdf:type	ns8:Source , skos:Concept ;
	skos:prefLabel	"Eurostat, Table eurostat_lfst_hhnhwhtc: Number of private households by household composition, number of children and working status within households (1 000)" ;
	foaf:page	ns21:lfst_hhnhwhtc ;
	skos:notation	"estat_lfst_hhnhwhtc" ;
	skos:definition	"Eurostat, Table eurostat_lfst_hhnhwhtc: Number of private households by household composition, number of children and working status within households (1 000)" ;
	skos:topConceptOf	ns1:source .
ns6:estat_nama_gdp_c
	rdf:type	ns8:Source , skos:Concept ;
	skos:prefLabel	"Eurostat, Table estat_nama_gdp_c: GDP and main components - Current prices" ;
	foaf:page	ns21:nama_gdp_c ;
	skos:notation	"estat_nama_gdp_c" ;
	skos:definition	"Eurostat, Table estat_nama_gdp_c: GDP and main components - Current prices" ;
	skos:topConceptOf	ns1:source .
ns6:estat_randd
	rdf:type	ns8:Source , skos:Concept ;
	skos:prefLabel	"Eurostat\u2019s statistics on R&D expenditure" ;
	foaf:page	ns22:database ;
	skos:notation	"estat_randd" ;
	skos:definition	"Eurostat\u2019s statistics on R&D expenditure are compiled using guidelines laid out in the Frascati manual (http://www.oecd.org/document/6/0,3343,en_2649_34451_33828550_1_1_1_1,00.html)" ;
	skos:topConceptOf	ns1:source .
ns6:estat_tps00188
	rdf:type	ns8:Source , skos:Concept ;
	skos:prefLabel	"Eurostat, Table estat_tps00188: Science and technology graduates by sex" ;
	foaf:page	ns21:educ_uoe_grad04 ;
	skos:notation	"estat_tps00188" ;
	skos:definition	"Eurostat, Table estat_tps00188: Science and technology graduates by sex" ;
	skos:topConceptOf	ns1:source .
ns6:eun12
	rdf:type	ns8:Source , skos:Concept ;
	skos:prefLabel	"ESSIE Survey about ICT in Education - SMART 2010/0039" ;
	foaf:page	ns21:educ_uoe_grad02 ;
	skos:notation	"eun12" ;
	skos:definition	"The ESSIE Survey about ICT in Education - SMART 2010/0039 - is based on over 190,000 filled questionnaires from students, teachers and head teachers in 27 countries, collected during school-year 2011-12  (mainly between September and December 2011), with the purpose of benchmarking access, use and attitudes to IC Technologies in Europe's schools (Primary; Lower secondary; Upper secondary, both general and vocational)." ;
	skos:note	"Data for 2006 comes from a previous study for the EC by Empirica, only partially comparable." ;
	skos:topConceptOf	ns1:source .
ns6:euripidis-estat
	rdf:type	ns8:Source , skos:Concept ;
	skos:prefLabel	"JRC-IPTS Euripidis project based on Eurostat Business demography data" ;
	foaf:page	ns21:educ_uoe_grad03 ;
	skos:notation	"euripidis-estat" ;
	skos:definition	"Garry Gabison, (forthcoming) \u201CBirth, Survival, Growth, and Death of ICT Companies. How are ICT companies faring in the European Union: a Macroeconomic Analysis.\u201D JRC Scientific and Policy Reports. Seville: JRC-IPTS.  " ;
	skos:topConceptOf	ns1:source .
ns6:eurostat_ed
	rdf:type	ns8:Source , skos:Concept ;
	skos:prefLabel	"Eurostat education statistics (table educ_uoe_grad04 and tps00188) " ;
	foaf:page	ns21:educ_uoe_grad04 ;
	skos:notation	"eurostat_ed" ;
	skos:definition	"Eurostat education statistics (table educ_uoe_grad04 and tps00188) " ;
	skos:topConceptOf	ns1:source .
ns6:eurostat_nat_acc
	rdf:type	ns8:Source , skos:Concept ;
	skos:prefLabel	"Eurostat national accounts" ;
	foaf:page	ns23:database ;
	skos:notation	"eurostat_nat_acc" ;
	skos:definition	"Eurostat national accounts" ;
	skos:note	"extracted 21 may 2014" ;
	skos:topConceptOf	ns1:source .
ns6:eurostat_pop
	rdf:type	ns8:Source , skos:Concept ;
	skos:prefLabel	"Eurostat population statistics" ;
	foaf:page	ns24:database ;
	skos:notation	"eurostat_pop" ;
	skos:definition	"Eurostat population statistics" ;
	skos:note	"extracted 21 may 2013" ;
	skos:topConceptOf	ns1:source .
ns6:idate
	rdf:type	ns8:Source , skos:Concept ;
	skos:prefLabel	"IDATE - Broadband coverage studies (2005-2010)" ;
	foaf:page	ns25:broadband-coverage-eu-272-phase-iii-smart-20100037 ;
	skos:notation	"idate" ;
	skos:definition	"Broadband Coverage in Europe, Studies for the EC realised by IDATE (2005-2010 data), SMART 2010/037" ;
	skos:note	"extraction 4 May 2011" ;
	skos:topConceptOf	ns1:source .
ns6:ihs_tech
	rdf:type	ns8:Source , skos:Concept ;
	skos:prefLabel	"IHS TV Media Intelligence" ;
	foaf:page	<https://technology.ihs.com/account/login?returnUrl=> ;
	skos:notation	"ihs_tech" ;
	skos:definition	"IHS TV Media Intelligence" ;
	skos:topConceptOf	ns1:source .
ns6:ipv6obs
	rdf:type	ns8:Source , skos:Concept ;
	skos:prefLabel	"EC - IPv6 Observatory" ;
	foaf:page	<http://www.ipv6observatory.eu/the-study/> ;
	skos:notation	"ipv6obs" ;
	skos:definition	"IPv6 Observatory, Study for the EC realized by inno" ;
	skos:note	"extraction published 3 June 2012" ;
	skos:topConceptOf	ns1:source .
ns6:jrc-ictspec3
	rdf:type	ns8:Source , skos:Concept ;
	skos:prefLabel	"JRC report on ICT employment 2000-2012" ;
	foaf:page	ns26:definitions ;
	skos:notation	"jrc-ictspec3" ;
	skos:definition	"JRC (IPTS) \"The evolution of EU ICT employment 2000-2012\" Technical report (forthcoming) based on Eurostat - Labour Force Survey" ;
	skos:note	"(forthcoming)" ;
	skos:topConceptOf	ns1:source .
ns6:jrc_ict_randd
	rdf:type	ns8:Source , skos:Concept ;
	skos:prefLabel	"JRC-IPTS Reports on Public ICT R&D Expenditures" ;
	foaf:page	<http://is.jrc.ec.europa.eu/pages/ISG/PREDICT.html> ;
	skos:notation	"jrc_ict_randd" ;
	skos:definition	"JRC-IPTS Reports estimating Public ICT R&D Expenditures in the EU (PREDICT2 project)" ;
	skos:note	"2013 report" ;
	skos:topConceptOf	ns1:source .
ns6:mis
	rdf:type	ns8:Source , skos:Concept ;
	skos:prefLabel	"EC - FP7 ICT research projects" ;
	foaf:page	ns10:ict-research-projects-under-eus-seventh-framework-programme-fp7 ;
	skos:notation	"mis" ;
	skos:definition	"EC database of ICT research projects under the EU's Seventh Framework Programme (FP7) - Cooperation and Capacities (e-infrastructures) programs. Projects under the CIP ICT PSP are not included. More information on the Programmes at http://cordis.europa.eu/fp7/ict/home_en.html" ;
	skos:note	"Extraction January 2013" ;
	skos:topConceptOf	ns1:source .
ns6:nif_database
	rdf:type	ns8:Source , skos:Concept ;
	skos:prefLabel	"NIF_database" ;
	skos:notation	"nif_database" ;
	skos:definition	"NIF_database" ;
	skos:topConceptOf	ns1:source .
ns6:old_desi_1b3_spec
	rdf:type	ns8:Source , skos:Concept ;
	skos:prefLabel	"European Commission Services" ;
	foaf:page	<http://digital-agenda-data.eu/charts/analyse-one-indicator-and-compare-countries#chart={\u0022indicator-group\u0022:\u0022any\u0022,\u0022indicator\u0022:\u0022spectrum_WBB\u0022,\u0022breakdown\u0022:\u0022TOTAL\u0022,\u0022unit-measure\u0022:\u0022pc_spectrum_assigned\u0022,\u0022ref-area\u0022:[\u0022AT\u0022,\u0022BE\u0022,\u0022BG\u0022,\u0022HR\u0022,\u0022CY\u0022,\u0022CZ\u0022,\u0022DK\u0022,\u0022EE\u0022,\u0022EU\u0022,\u0022FI\u0022,\u0022FR\u0022,\u0022DE\u0022,\u0022EL\u0022,\u0022HU\u0022,\u0022IE\u0022,\u0022IT\u0022,\u0022LV\u0022,\u0022LT\u0022,\u0022LU\u0022,\u0022MT\u0022,\u0022NL\u0022,\u0022PL\u0022,\u0022PT\u0022,\u0022RO\u0022,\u0022SK\u0022,\u0022SI\u0022,\u0022ES\u0022,\u0022SE\u0022,\u0022UK\u0022]}> ;
	skos:notation	"old_desi_1b3_spec" ;
	skos:definition	"European Commission Services" ;
	skos:topConceptOf	ns1:source .
ns6:old_desi_1d1_fbbp
	rdf:type	ns8:Source , skos:Concept ;
	skos:prefLabel	"Broadband Internet Access Cost (BIAC) annual studies" ;
	foaf:page	<http://digital-agenda-data.eu/charts/analyse-one-indicator-and-compare-countries#chart={\u0022indicator-group\u0022:\u0022any\u0022,\u0022indicator\u0022:\u0022Price_Internet_only\u0022,\u0022breakdown\u0022:\u0022offer_12_30_Mbps\u0022,\u0022unit-measure\u0022:\u0022minimum_euro_PPP\u0022,\u0022ref-area\u0022:[\u0022AT\u0022,\u0022BE\u0022,\u0022BG\u0022,\u0022HR\u0022,\u0022CY\u0022,\u0022CZ\u0022,\u0022DK\u0022,\u0022EE\u0022,\u0022EU\u0022,\u0022FI\u0022,\u0022FR\u0022,\u0022DE\u0022,\u0022EL\u0022,\u0022HU\u0022,\u0022IE\u0022,\u0022IT\u0022,\u0022LV\u0022,\u0022LT\u0022,\u0022LU\u0022,\u0022MT\u0022,\u0022NL\u0022,\u0022PL\u0022,\u0022PT\u0022,\u0022RO\u0022,\u0022SK\u0022,\u0022SI\u0022,\u0022ES\u0022,\u0022SE\u0022,\u0022UK\u0022]}> ;
	skos:notation	"old_desi_1d1_fbbp" ;
	skos:definition	"Access cost: Broadband Internet Access Cost (BIAC), annual studies for the EC realised by Van Dijk (2013-2015) and by Empirica (2016 onwards). Income: Real adjusted gross disposable income of households per capita (Eurostat: tec00113)" ;
	skos:topConceptOf	ns1:source .
ns6:old_desi_5b1_mdataexch
	rdf:type	ns8:Source , skos:Concept ;
	skos:prefLabel	"eHealth Studies" ;
	foaf:page	<http://digital-agenda-data.eu/charts/analyse-one-indicator-and-compare-countries#chart={\u0022indicator-group\u0022:\u0022any\u0022,\u0022indicator\u0022:\u0022HIE_use_ex_admin\u0022,\u0022breakdown\u0022:\u0022TOTAL\u0022,\u0022unit-measure\u0022:\u0022pc_gp\u0022,\u0022ref-area\u0022:[\u0022AT\u0022,\u0022BE\u0022,\u0022BG\u0022,\u0022HR\u0022,\u0022CY\u0022,\u0022CZ\u0022,\u0022DK\u0022,\u0022EE\u0022,\u0022EU\u0022,\u0022FI\u0022,\u0022FR\u0022,\u0022DE\u0022,\u0022EL\u0022,\u0022HU\u0022,\u0022IE\u0022,\u0022IT\u0022,\u0022LV\u0022,\u0022LT\u0022,\u0022LU\u0022,\u0022MT\u0022,\u0022NL\u0022,\u0022PL\u0022,\u0022PT\u0022,\u0022RO\u0022,\u0022SK\u0022,\u0022SI\u0022,\u0022ES\u0022,\u0022SE\u0022,\u0022UK\u0022]}> ;
	skos:notation	"old_desi_5b1_mdataexch" ;
	skos:definition	"Benchmarking Deployment of eHealth among General Practitioners" ;
	skos:topConceptOf	ns1:source .
ns6:old_desi_5b2_epresc
	rdf:type	ns8:Source , skos:Concept ;
	skos:prefLabel	"eHealth Studies" ;
	foaf:page	<http://digital-agenda-data.eu/charts/analyse-one-indicator-and-compare-countries#chart={\u0022indicator-group\u0022:\u0022any\u0022,\u0022indicator\u0022:\u0022HIE_use_pharm\u0022,\u0022breakdown\u0022:\u0022TOTAL\u0022,\u0022unit-measure\u0022:\u0022pc_gp\u0022,\u0022ref-area\u0022:[\u0022AT\u0022,\u0022BE\u0022,\u0022BG\u0022,\u0022HR\u0022,\u0022CY\u0022,\u0022CZ\u0022,\u0022DK\u0022,\u0022EE\u0022,\u0022EU\u0022,\u0022FI\u0022,\u0022FR\u0022,\u0022DE\u0022,\u0022EL\u0022,\u0022HU\u0022,\u0022IE\u0022,\u0022IT\u0022,\u0022LV\u0022,\u0022LT\u0022,\u0022LU\u0022,\u0022MT\u0022,\u0022NL\u0022,\u0022PL\u0022,\u0022PT\u0022,\u0022RO\u0022,\u0022SK\u0022,\u0022SI\u0022,\u0022ES\u0022,\u0022SE\u0022,\u0022UK\u0022]}> ;
	skos:notation	"old_desi_5b2_epresc" ;
	skos:definition	"Benchmarking Deployment of eHealth among General Practitioners" ;
	skos:topConceptOf	ns1:source .
ns6:point_topic
	rdf:type	ns8:Source , skos:Concept ;
	skos:prefLabel	"Point Topic Study on broadband coverage" ;
	foaf:page	ns12:about-fast-and-ultra-fast-internet-access ;
	skos:notation	"point_topic" ;
	skos:definition	"Broadband coverage in Europe, studies for the EC by Point Topic (2011-2012 figures, SMART 2011/0027 and 2012/0035) and IHS and Valdani, Vicari & Associati (2013 figures, SMART 2013/0054)" ;
	skos:topConceptOf	ns1:source .
ns6:samknows
	rdf:type	ns8:Source , skos:Concept ;
	skos:prefLabel	"Study on \"Quality of Broadband Services in the EU\u201D SMART 2010/0036" ;
	foaf:page	ns25:quality-broadband-services-eu-samknows-study-internet-speeds ;
	skos:notation	"samknows" ;
	skos:definition	"Study on \"Quality of Broadband Services in the EU\u201D (SMART 2010/0036). For the purposes of this study 9,104 households across the European Union were given a specially configured hardware device (SamKnows Whitebox), which runs a series of purpose-built tests to measure every aspect of Internet performance. The sample is designed to represent tha main fixed broadband services, used by consumers and available all around the country." ;
	skos:note	"April 2013 Report" ;
	skos:topConceptOf	ns1:source .
ns6:smart11_39
	rdf:type	ns8:Source , skos:Concept ;
	skos:prefLabel	"Analysis of publications and patents of ICT research in FP7" ;
	foaf:page	ns27:our-studies-and-open-datasets ;
	skos:notation	"smart11_39" ;
	skos:definition	": Analysis conducted by DG CONNECT Unit F4, based on results of the study SMART 2011/0039 which main results are published in: Jacob, J., Sanditov, B., Smirnov, E., Wintjes, R., Surpatean, A., Notten, A., & Sasso, S. (Forthcoming). Analysis of publications and patents of ICT research in FP7. Brussels, European Commission. " ;
	skos:topConceptOf	ns1:source .
ns6:desi_1b3_5g
	rdf:type	ns8:Source , skos:Concept ;
	skos:prefLabel	"European Commission services" ;
	skos:notation	"desi_1b3_5g" ;
	skos:definition	"European Commission services" ;
	skos:topConceptOf	ns1:source .
ns6:desi_2a1_bds
	rdf:type	ns8:Source , skos:Concept ;
	skos:prefLabel	"Eurostat Survey - ICT usage in Households and by People" ;
	foaf:page	<https://digital-agenda-data.eu/charts/analyse-one-indicator-and-compare-countries#chart={%22indicator-group%22:%22any%22,%22indicator%22:%22i_dsk_bab%22,%22breakdown%22:%22IND_TOTAL%22,%22unit-measure%22:%22pc_ind%22,%22ref-area%22:[%22AT%22,%22BE%22,%22BG%22,%22HR%22,%22CY%22,%22CZ%22,%22DK%22,%22EE%22,%22EU%22,%22FI%22,%22FR%22,%22DE%22,%22EL%22,%22HU%22,%22IE%22,%22IT%22,%22LV%22,%22LT%22,%22LU%22,%22MT%22,%22NL%22,%22PL%22,%22PT%22,%22RO%22,%22SK%22,%22SI%22,%22ES%22,%22SE%22,%22UK%22]}> ;
	skos:notation	"desi_2a1_bds" ;
	skos:definition	"Eurostat - Community survey on ICT usage in Households and by Individuals " ;
	skos:topConceptOf	ns1:source .
ns6:desi_2a2_abds
	rdf:type	ns8:Source , skos:Concept ;
	skos:prefLabel	"Eurostat Survey - ICT usage in Households and by People" ;
	skos:notation	"desi_2a2_abds" ;
	skos:definition	"Eurostat - Community survey on ICT usage in Households and by Individuals " ;
	skos:topConceptOf	ns1:source .
ns6:desi_2a3_abss
	rdf:type	ns8:Source , skos:Concept ;
	skos:prefLabel	"Eurostat Survey - ICT usage in Households and by People" ;
	foaf:page	<https://digital-agenda-data.eu/charts/analyse-one-indicator-and-compare-countries#chart={%22indicator-group%22:%22any%22,%22indicator%22:%22i_dsk_s_bab%22,%22breakdown%22:%22IND_TOTAL%22,%22unit-measure%22:%22pc_ind%22,%22ref-area%22:[%22AT%22,%22BE%22,%22BG%22,%22HR%22,%22CY%22,%22CZ%22,%22DK%22,%22EE%22,%22EU%22,%22FI%22,%22FR%22,%22DE%22,%22EL%22,%22HU%22,%22IE%22,%22IT%22,%22LV%22,%22LT%22,%22LU%22,%22MT%22,%22NL%22,%22PL%22,%22PT%22,%22RO%22,%22SK%22,%22SI%22,%22ES%22,%22SE%22,%22UK%22]}> ;
	skos:notation	"desi_2a3_abss" ;
	skos:definition	"Eurostat - Community survey on ICT usage in Households and by Individuals " ;
	skos:topConceptOf	ns1:source .
ns6:desi_2b2_fictspec
	rdf:type	ns8:Source , skos:Concept ;
	skos:prefLabel	"Eurostat - Labour force survey" ;
	foaf:page	<https://digital-agenda-data.eu/charts/analyse-one-indicator-and-compare-countries#chart={%22indicator-group%22:%22any%22,%22indicator%22:%22wid_sse_icts%22,%22breakdown%22:%22F_Y16_74%22,%22unit-measure%22:%22pc_ind_emp%22,%22ref-area%22:[%22AT%22,%22BE%22,%22BG%22,%22HR%22,%22CY%22,%22CZ%22,%22DK%22,%22EE%22,%22EU%22,%22FI%22,%22FR%22,%22DE%22,%22EL%22,%22HU%22,%22IE%22,%22IT%22,%22LV%22,%22LT%22,%22LU%22,%22MT%22,%22NL%22,%22PL%22,%22PT%22,%22RO%22,%22SK%22,%22SI%22,%22ES%22,%22SE%22,%22UK%22]}> ;
	skos:notation	"desi_2b2_fictspec" ;
	skos:definition	"Eurostat - Labour force survey" ;
	skos:topConceptOf	ns1:source .
ns6:desi_2b3_ictg
	rdf:type	ns8:Source , skos:Concept ;
	skos:prefLabel	"Eurostat" ;
	skos:notation	"desi_2b3_ictg" ;
	skos:definition	"Eurostat (table educ_uoegrad04, using selection ISCED11=ED5-8)" ;
	skos:topConceptOf	ns1:source .
ns6:desi_3a1_notiu
	rdf:type	ns8:Source , skos:Concept ;
	skos:prefLabel	"Eurostat Survey - ICT usage in Households and by People" ;
	foaf:page	<https://digital-agenda-data.eu/charts/analyse-one-indicator-and-compare-countries#chart={%22indicator-group%22:%22any%22,%22indicator%22:%22i_iux%22,%22breakdown%22:%22IND_TOTAL%22,%22unit-measure%22:%22pc_ind%22,%22ref-area%22:[%22AT%22,%22BE%22,%22BG%22,%22HR%22,%22CY%22,%22CZ%22,%22DK%22,%22EE%22,%22EU%22,%22FI%22,%22FR%22,%22DE%22,%22EL%22,%22HU%22,%22IS%22,%22IE%22,%22IT%22,%22LV%22,%22LT%22,%22LU%22,%22MT%22,%22NL%22,%22NO%22,%22PL%22,%22PT%22,%22RO%22,%22SK%22,%22SI%22,%22ES%22,%22SE%22,%22UK%22]}> ;
	skos:notation	"desi_3a1_notiu" ;
	skos:definition	"Eurostat - Community survey on ICT usage in Households and by Individuals (I_IUX)" ;
	skos:topConceptOf	ns1:source .
ns6:desi_3a2_iu
	rdf:type	ns8:Source , skos:Concept ;
	skos:prefLabel	"Eurostat Survey - ICT usage in Households and by People" ;
	foaf:page	<https://digital-agenda-data.eu/charts/analyse-one-indicator-and-compare-countries#chart={%22indicator-group%22:%22any%22,%22indicator%22:%22i_iuse%22,%22breakdown%22:%22IND_TOTAL%22,%22unit-measure%22:%22pc_ind%22,%22ref-area%22:[%22AT%22,%22BE%22,%22BG%22,%22HR%22,%22CY%22,%22CZ%22,%22DK%22,%22EE%22,%22EU%22,%22FI%22,%22FR%22,%22DE%22,%22EL%22,%22HU%22,%22IS%22,%22IE%22,%22IT%22,%22LV%22,%22LT%22,%22LU%22,%22MT%22,%22NL%22,%22NO%22,%22PL%22,%22PT%22,%22RO%22,%22SK%22,%22SI%22,%22ES%22,%22SE%22,%22UK%22]}> ;
	skos:notation	"desi_3a2_iu" ;
	skos:definition	"Eurostat - Community survey on ICT usage in Households and by Individuals (I_IUSE)" ;
	skos:topConceptOf	ns1:source .
ns6:desi_3b1_news
	rdf:type	ns8:Source , skos:Concept ;
	skos:prefLabel	"Eurostat Survey - ICT usage in Households and by People" ;
	foaf:page	<http://digital-agenda-data.eu/charts/analyse-one-indicator-and-compare-countries#chart={\u0022indicator-group\u0022:\u0022any\u0022,\u0022indicator\u0022:\u0022i_iunw\u0022,\u0022breakdown\u0022:\u0022IND_TOTAL\u0022,\u0022unit-measure\u0022:\u0022pc_ind_iu3\u0022,\u0022ref-area\u0022:[\u0022AT\u0022,\u0022BE\u0022,\u0022BG\u0022,\u0022HR\u0022,\u0022CY\u0022,\u0022CZ\u0022,\u0022DK\u0022,\u0022EE\u0022,\u0022EU\u0022,\u0022FI\u0022,\u0022FR\u0022,\u0022DE\u0022,\u0022EL\u0022,\u0022HU\u0022,\u0022IE\u0022,\u0022IT\u0022,\u0022LV\u0022,\u0022LT\u0022,\u0022LU\u0022,\u0022MT\u0022,\u0022NL\u0022,\u0022PL\u0022,\u0022PT\u0022,\u0022RO\u0022,\u0022SK\u0022,\u0022SI\u0022,\u0022ES\u0022,\u0022SE\u0022,\u0022UK\u0022]}> ;
	skos:notation	"desi_3b1_news" ;
	skos:definition	"Eurostat - Community survey on ICT usage in Households and by Individuals (I_IUNW1)" ;
	skos:topConceptOf	ns1:source .
ns6:desi_3b2_mvg
	rdf:type	ns8:Source , skos:Concept ;
	skos:prefLabel	"Eurostat Survey - ICT usage in Households and by People" ;
	foaf:page	<http://digital-agenda-data.eu/charts/analyse-one-indicator-and-compare-countries#chart={\u0022indicator-group\u0022:\u0022any\u0022,\u0022indicator\u0022:\u0022i_iugm\u0022,\u0022breakdown\u0022:\u0022IND_TOTAL\u0022,\u0022unit-measure\u0022:\u0022pc_ind_iu3\u0022,\u0022ref-area\u0022:[\u0022AT\u0022,\u0022BE\u0022,\u0022BG\u0022,\u0022HR\u0022,\u0022CY\u0022,\u0022CZ\u0022,\u0022DK\u0022,\u0022EE\u0022,\u0022EU\u0022,\u0022FI\u0022,\u0022FR\u0022,\u0022DE\u0022,\u0022EL\u0022,\u0022HU\u0022,\u0022IE\u0022,\u0022IT\u0022,\u0022LV\u0022,\u0022LT\u0022,\u0022LU\u0022,\u0022MT\u0022,\u0022NL\u0022,\u0022PL\u0022,\u0022PT\u0022,\u0022RO\u0022,\u0022SK\u0022,\u0022SI\u0022,\u0022ES\u0022,\u0022SE\u0022,\u0022UK\u0022]}> ;
	skos:notation	"desi_3b2_mvg" ;
	skos:definition	"Eurostat - Community survey on ICT usage in Households and by Individuals" ;
	skos:topConceptOf	ns1:source .
ns6:desi_3b3_vod
	rdf:type	ns8:Source , skos:Concept ;
	skos:prefLabel	"Eurostat Survey - ICT usage in Households and by People" ;
	foaf:page	<http://digital-agenda-data.eu/charts/analyse-one-indicator-and-compare-countries#chart={\u0022indicator-group\u0022:\u0022any\u0022,\u0022indicator\u0022:\u0022vod\u0022,\u0022breakdown\u0022:\u0022HH_total\u0022,\u0022unit-measure\u0022:\u0022pc_EBhh_tv\u0022,\u0022ref-area\u0022:[\u0022AT\u0022,\u0022BE\u0022,\u0022CY\u0022,\u0022CZ\u0022,\u0022DK\u0022,\u0022EE\u0022,\u0022FI\u0022,\u0022FR\u0022,\u0022DE\u0022,\u0022EL\u0022,\u0022HU\u0022,\u0022IE\u0022,\u0022IT\u0022,\u0022LV\u0022,\u0022LT\u0022,\u0022LU\u0022,\u0022MT\u0022,\u0022NL\u0022,\u0022PL\u0022,\u0022PT\u0022,\u0022RO\u0022,\u0022SK\u0022,\u0022SI\u0022,\u0022ES\u0022,\u0022SE\u0022,\u0022UK\u0022]}> ;
	skos:notation	"desi_3b3_vod" ;
	skos:definition	"Eurostat - Community survey on ICT usage in Households and by Individuals" ;
	skos:topConceptOf	ns1:source .
ns6:desi_3b4_vidcall
	rdf:type	ns8:Source , skos:Concept ;
	skos:prefLabel	"Eurostat Survey - ICT usage in Households and by People" ;
	foaf:page	<http://digital-agenda-data.eu/charts/analyse-one-indicator-and-compare-countries#chart={\u0022indicator-group\u0022:\u0022any\u0022,\u0022indicator\u0022:\u0022i_iuph1\u0022,\u0022breakdown\u0022:\u0022IND_TOTAL\u0022,\u0022unit-measure\u0022:\u0022pc_ind_iu3\u0022,\u0022ref-area\u0022:[\u0022AT\u0022,\u0022BE\u0022,\u0022BG\u0022,\u0022HR\u0022,\u0022CY\u0022,\u0022CZ\u0022,\u0022DK\u0022,\u0022EE\u0022,\u0022EU\u0022,\u0022FI\u0022,\u0022FR\u0022,\u0022DE\u0022,\u0022EL\u0022,\u0022HU\u0022,\u0022IE\u0022,\u0022IT\u0022,\u0022LV\u0022,\u0022LT\u0022,\u0022LU\u0022,\u0022MT\u0022,\u0022NL\u0022,\u0022PL\u0022,\u0022PT\u0022,\u0022RO\u0022,\u0022SK\u0022,\u0022SI\u0022,\u0022ES\u0022,\u0022SE\u0022,\u0022UK\u0022]}> ;
	skos:notation	"desi_3b4_vidcall" ;
	skos:definition	"Eurostat - Community survey on ICT usage in Households and by Individuals (I_IUPH1)" ;
	skos:topConceptOf	ns1:source .
ns6:desi_3b5_socnet
	rdf:type	ns8:Source , skos:Concept ;
	skos:prefLabel	"Eurostat Survey - ICT usage in Households and by People" ;
	foaf:page	<http://digital-agenda-data.eu/charts/analyse-one-indicator-and-compare-countries#chart={\u0022indicator-group\u0022:\u0022any\u0022,\u0022indicator\u0022:\u0022i_iusnet\u0022,\u0022breakdown\u0022:\u0022IND_TOTAL\u0022,\u0022unit-measure\u0022:\u0022pc_ind_iu3\u0022,\u0022ref-area\u0022:[\u0022AT\u0022,\u0022BE\u0022,\u0022BG\u0022,\u0022HR\u0022,\u0022CY\u0022,\u0022CZ\u0022,\u0022DK\u0022,\u0022EE\u0022,\u0022EU\u0022,\u0022FI\u0022,\u0022FR\u0022,\u0022DE\u0022,\u0022EL\u0022,\u0022HU\u0022,\u0022IE\u0022,\u0022IT\u0022,\u0022LV\u0022,\u0022LT\u0022,\u0022LU\u0022,\u0022MT\u0022,\u0022NL\u0022,\u0022PL\u0022,\u0022PT\u0022,\u0022RO\u0022,\u0022SK\u0022,\u0022SI\u0022,\u0022ES\u0022,\u0022SE\u0022,\u0022UK\u0022]}> ;
	skos:notation	"desi_3b5_socnet" ;
	skos:definition	"Eurostat - Community survey on ICT usage in Households and by Individuals (I_IUSNET) " ;
	skos:topConceptOf	ns1:source .
ns6:desi_3b6_profsocnet
	rdf:type	ns8:Source , skos:Concept ;
	skos:prefLabel	"Eurostat Survey - ICT usage in Households and by People" ;
	skos:notation	"desi_3b6_profsocnet" ;
	skos:definition	"Eurostat - Community survey on ICT usage in Households and by Individuals (I_IUNET)" ;
	skos:topConceptOf	ns1:source .
ns6:desi_3b7_courseon
	rdf:type	ns8:Source , skos:Concept ;
	skos:prefLabel	"Eurostat Survey - ICT usage in Households and by People" ;
	foaf:page	<https://digital-agenda-data.eu/charts/analyse-one-indicator-and-compare-countries#chart={%22indicator-group%22:%22any%22,%22indicator%22:%22i_iuolc%22,%22breakdown%22:%22IND_TOTAL%22,%22unit-measure%22:%22pc_ind%22,%22ref-area%22:[%22AT%22,%22BE%22,%22BG%22,%22HR%22,%22CY%22,%22CZ%22,%22DK%22,%22EE%22,%22EU%22,%22FI%22,%22FR%22,%22DE%22,%22EL%22,%22HU%22,%22IS%22,%22IE%22,%22IT%22,%22LV%22,%22LT%22,%22LU%22,%22MT%22,%22NL%22,%22NO%22,%22PL%22,%22PT%22,%22RO%22,%22SK%22,%22SI%22,%22ES%22,%22SE%22,%22UK%22]}> ;
	skos:notation	"desi_3b7_courseon" ;
	skos:definition	"Eurostat - Community survey on ICT usage in Households and by Individuals (I_IUOLC) " ;
	skos:topConceptOf	ns1:source .
ns6:desi_3b8_convoton
	rdf:type	ns8:Source , skos:Concept ;
	skos:prefLabel	"Eurostat Survey - ICT usage in Households and by People" ;
	foaf:page	<https://digital-agenda-data.eu/charts/analyse-one-indicator-and-compare-countries#chart={%22indicator-group%22:%22any%22,%22indicator%22:%22i_iuvote%22,%22breakdown%22:%22IND_TOTAL%22,%22unit-measure%22:%22pc_ind%22,%22ref-area%22:[%22AT%22,%22BE%22,%22BG%22,%22HR%22,%22CY%22,%22CZ%22,%22DK%22,%22EE%22,%22EU%22,%22FI%22,%22FR%22,%22DE%22,%22EL%22,%22HU%22,%22IS%22,%22IE%22,%22IT%22,%22LV%22,%22LT%22,%22LU%22,%22MT%22,%22NL%22,%22NO%22,%22PL%22,%22PT%22,%22RO%22,%22SK%22,%22SI%22,%22ES%22,%22SE%22,%22UK%22]}> ;
	skos:notation	"desi_3b8_convoton" ;
	skos:definition	"Eurostat - Community survey on ICT usage in Households and by Individuals (I_IUVOTE) " ;
	skos:topConceptOf	ns1:source .
ns6:desi_3c3_sell
	rdf:type	ns8:Source , skos:Concept ;
	skos:prefLabel	"Eurostat Survey - ICT usage in Households and by People" ;
	foaf:page	<https://digital-agenda-data.eu/charts/analyse-one-indicator-and-compare-countries#chart={%22indicator-group%22:%22any%22,%22indicator%22:%22i_iusell%22,%22breakdown%22:%22IND_TOTAL%22,%22unit-measure%22:%22pc_ind_iu3%22,%22ref-area%22:[%22AT%22,%22BE%22,%22BG%22,%22HR%22,%22CY%22,%22CZ%22,%22DK%22,%22EE%22,%22EU%22,%22FI%22,%22FR%22,%22DE%22,%22EL%22,%22HU%22,%22IE%22,%22IT%22,%22LV%22,%22LT%22,%22LU%22,%22MT%22,%22NL%22,%22PL%22,%22PT%22,%22RO%22,%22SK%22,%22SI%22,%22ES%22,%22SE%22,%22UK%22]}> ;
	skos:notation	"desi_3c3_sell" ;
	skos:definition	"Eurostat - Community survey on ICT usage in Households and by Individuals (I_IUSELL)" ;
	skos:topConceptOf	ns1:source .
ns6:desi_4a2_socmed
	rdf:type	ns8:Source , skos:Concept ;
	skos:prefLabel	"Eurostat - ICT Enterprises survey" ;
	foaf:page	<http://digital-agenda-data.eu/charts/analyse-one-indicator-and-compare-countries#chart={\u0022indicator-group\u0022:\u0022any\u0022,\u0022indicator\u0022:\u0022e_sm_ge2\u0022,\u0022breakdown\u0022:\u0022ent_all_xfin\u0022,\u0022unit-measure\u0022:\u0022pc_ent\u0022,\u0022ref-area\u0022:[\u0022AT\u0022,\u0022BE\u0022,\u0022BG\u0022,\u0022HR\u0022,\u0022CY\u0022,\u0022CZ\u0022,\u0022DK\u0022,\u0022EE\u0022,\u0022EU\u0022,\u0022FI\u0022,\u0022FR\u0022,\u0022DE\u0022,\u0022EL\u0022,\u0022HU\u0022,\u0022IE\u0022,\u0022IT\u0022,\u0022LV\u0022,\u0022LT\u0022,\u0022LU\u0022,\u0022MT\u0022,\u0022NL\u0022,\u0022PL\u0022,\u0022PT\u0022,\u0022RO\u0022,\u0022SK\u0022,\u0022SI\u0022,\u0022ES\u0022,\u0022SE\u0022,\u0022UK\u0022]}> ;
	skos:notation	"desi_4a2_socmed" ;
	skos:definition	"Eurostat - Community survey on ICT usage and eCommerce in Enterprises (E_SM1_GE2)" ;
	skos:topConceptOf	ns1:source .
ns6:desi_4a3_bigdat
	rdf:type	ns8:Source , skos:Concept ;
	skos:prefLabel	"Eurostat - ICT Enterprises survey" ;
	foaf:page	<https://digital-agenda-data.eu/charts/analyse-one-indicator-and-compare-countries#chart={%22indicator-group%22:%22any%22,%22indicator%22:%22e_bd%22,%22breakdown%22:%22ent_all_xfin%22,%22unit-measure%22:%22pc_ent%22,%22ref-area%22:[%22AT%22,%22BE%22,%22BG%22,%22HR%22,%22CY%22,%22CZ%22,%22DK%22,%22EE%22,%22EU%22,%22FI%22,%22FR%22,%22DE%22,%22EL%22,%22HU%22,%22IS%22,%22IE%22,%22IT%22,%22LV%22,%22LT%22,%22LU%22,%22MT%22,%22NL%22,%22NO%22,%22PL%22,%22PT%22,%22RO%22,%22SK%22,%22SI%22,%22ES%22,%22SE%22,%22UK%22]}> ;
	skos:notation	"desi_4a3_bigdat" ;
	skos:definition	"Eurostat - Community survey on ICT usage and eCommerce in Enterprises (E_BD)" ;
	skos:topConceptOf	ns1:source .
ns6:desi_4a4_cloud
	rdf:type	ns8:Source , skos:Concept ;
	skos:prefLabel	"Eurostat - ICT Enterprises survey" ;
	foaf:page	<http://digital-agenda-data.eu/charts/analyse-one-indicator-and-compare-countries#chart={\u0022indicator-group\u0022:\u0022any\u0022,\u0022indicator\u0022:\u0022e_cc_ge_me\u0022,\u0022breakdown\u0022:\u0022ent_all_xfin\u0022,\u0022unit-measure\u0022:\u0022pc_ent\u0022,\u0022ref-area\u0022:[\u0022AT\u0022,\u0022BE\u0022,\u0022BG\u0022,\u0022HR\u0022,\u0022CY\u0022,\u0022CZ\u0022,\u0022DK\u0022,\u0022EE\u0022,\u0022EU\u0022,\u0022FI\u0022,\u0022FR\u0022,\u0022DE\u0022,\u0022EL\u0022,\u0022HU\u0022,\u0022IE\u0022,\u0022IT\u0022,\u0022LV\u0022,\u0022LT\u0022,\u0022LU\u0022,\u0022MT\u0022,\u0022NL\u0022,\u0022PL\u0022,\u0022PT\u0022,\u0022RO\u0022,\u0022SK\u0022,\u0022SI\u0022,\u0022ES\u0022,\u0022SE\u0022,\u0022UK\u0022]}> ;
	skos:notation	"desi_4a4_cloud" ;
	skos:definition	"Eurostat - Community survey on ICT usage and eCommerce in Enterprises" ;
	skos:topConceptOf	ns1:source .
ns6:desi_5b2_mdataexch
	rdf:type	ns8:Source , skos:Concept ;
	skos:prefLabel	"Benchmarking Deployment of eHealth among General Practitioners" ;
	skos:notation	"desi_5b2_mdataexch" ;
	skos:definition	"Benchmarking Deployment of eHealth among General Practitioners" ;
	skos:topConceptOf	ns1:source .
ns6:desi_5b3_epresc
	rdf:type	ns8:Source , skos:Concept ;
	skos:prefLabel	"Benchmarking Deployment of eHealth among General Practitioners" ;
	skos:notation	"desi_5b3_epresc" ;
	skos:definition	"Benchmarking Deployment of eHealth among General Practitioners" ;
	skos:topConceptOf	ns1:source .
ns6:old_desi_2a1_iu
	rdf:type	ns8:Source , skos:Concept ;
	skos:prefLabel	"Eurostat - ICT Households survey" ;
	foaf:page	<http://digital-agenda-data.eu/charts/analyse-one-indicator-and-compare-countries#chart={\u0022indicator-group\u0022:\u0022any\u0022,\u0022indicator\u0022:\u0022i_iuse\u0022,\u0022breakdown\u0022:\u0022IND_TOTAL\u0022,\u0022unit-measure\u0022:\u0022pc_ind\u0022,\u0022ref-area\u0022:[\u0022AT\u0022,\u0022BE\u0022,\u0022BG\u0022,\u0022HR\u0022,\u0022CY\u0022,\u0022CZ\u0022,\u0022DK\u0022,\u0022EE\u0022,\u0022EU\u0022,\u0022FI\u0022,\u0022FR\u0022,\u0022DE\u0022,\u0022EL\u0022,\u0022HU\u0022,\u0022IE\u0022,\u0022IT\u0022,\u0022LV\u0022,\u0022LT\u0022,\u0022LU\u0022,\u0022MT\u0022,\u0022NL\u0022,\u0022PL\u0022,\u0022PT\u0022,\u0022RO\u0022,\u0022SK\u0022,\u0022SI\u0022,\u0022ES\u0022,\u0022SE\u0022,\u0022UK\u0022]}> ;
	skos:notation	"old_desi_2a1_iu" ;
	skos:definition	"Eurostat - Community survey on ICT usage in Households and by Individuals" ;
	skos:topConceptOf	ns1:source .
ns6:old_desi_2a2_bds
	rdf:type	ns8:Source , skos:Concept ;
	skos:prefLabel	"Eurostat - ICT Households survey" ;
	foaf:page	<http://digital-agenda-data.eu/charts/analyse-one-indicator-and-compare-countries#chart={%22indicator-group%22:%22any%22,%22indicator%22:%22i_DSK_BAB%22,%22breakdown%22:%22IND_TOTAL%22,%22unit-measure%22:%22pc_ind%22,%22ref-area%22:[%22AT%22,%22BE%22,%22BG%22,%22HR%22,%22CY%22,%22CZ%22,%22DK%22,%22EE%22,%22EU%22,%22FI%22,%22FR%22,%22DE%22,%22EL%22,%22HU%22,%22IE%22,%22IT%22,%22LV%22,%22LT%22,%22LU%22,%22MT%22,%22NL%22,%22PL%22,%22PT%22,%22RO%22,%22SK%22,%22SI%22,%22ES%22,%22SE%22,%22UK%22]}> ;
	skos:notation	"old_desi_2a2_bds" ;
	skos:definition	"Eurostat - Community survey on ICT usage in Households and by Individuals" ;
	skos:topConceptOf	ns1:source .
ns6:old_desi_2b1_ictspec
	rdf:type	ns8:Source , skos:Concept ;
	skos:prefLabel	"Eurostat - Labour force survey" ;
	foaf:page	<http://digital-agenda-data.eu/charts/analyse-one-indicator-and-compare-countries#chart={\u0022indicator-group\u0022:\u0022any\u0022,\u0022indicator\u0022:\u0022ict_spec3_broad\u0022,\u0022breakdown\u0022:\u0022TOTAL\u0022,\u0022unit-measure\u0022:\u0022pc_ind_emp\u0022,\u0022ref-area\u0022:[\u0022AT\u0022,\u0022BE\u0022,\u0022BG\u0022,\u0022HR\u0022,\u0022CY\u0022,\u0022CZ\u0022,\u0022DK\u0022,\u0022EE\u0022,\u0022EU\u0022,\u0022FI\u0022,\u0022FR\u0022,\u0022DE\u0022,\u0022EL\u0022,\u0022HU\u0022,\u0022IE\u0022,\u0022IT\u0022,\u0022LV\u0022,\u0022LT\u0022,\u0022LU\u0022,\u0022MT\u0022,\u0022NL\u0022,\u0022PL\u0022,\u0022PT\u0022,\u0022RO\u0022,\u0022SK\u0022,\u0022SI\u0022,\u0022ES\u0022,\u0022SE\u0022,\u0022UK\u0022]}> ;
	skos:notation	"old_desi_2b1_ictspec" ;
	skos:definition	"Eurostat - Labour force survey" ;
	skos:topConceptOf	ns1:source .
ns6:old_desi_2b2_stemg
	rdf:type	ns8:Source , skos:Concept ;
	skos:prefLabel	"Eurostat education statistics" ;
	foaf:page	<http://digital-agenda-data.eu/charts/analyse-one-indicator-and-compare-countries#chart={\u0022indicator-group\u0022:\u0022any\u0022,\u0022indicator\u0022:\u0022st_grad\u0022,\u0022breakdown\u0022:\u0022TOTAL\u0022,\u0022unit-measure\u0022:\u0022nb_x1000inh_20_29\u0022,\u0022ref-area\u0022:[\u0022AT\u0022,\u0022BE\u0022,\u0022BG\u0022,\u0022HR\u0022,\u0022CY\u0022,\u0022CZ\u0022,\u0022DK\u0022,\u0022EE\u0022,\u0022EU\u0022,\u0022FI\u0022,\u0022FR\u0022,\u0022DE\u0022,\u0022EL\u0022,\u0022HU\u0022,\u0022IE\u0022,\u0022IT\u0022,\u0022LV\u0022,\u0022LT\u0022,\u0022LU\u0022,\u0022MT\u0022,\u0022NL\u0022,\u0022PL\u0022,\u0022PT\u0022,\u0022RO\u0022,\u0022SK\u0022,\u0022SI\u0022,\u0022ES\u0022,\u0022SE\u0022,\u0022UK\u0022]}> ;
	skos:notation	"old_desi_2b2_stemg" ;
	skos:definition	"Eurostat - Science and technology graduates by sex" ;
	skos:topConceptOf	ns1:source .
ns6:old_desi_3a1_news
	rdf:type	ns8:Source , skos:Concept ;
	skos:prefLabel	"Eurostat - ICT Households survey" ;
	foaf:page	<http://digital-agenda-data.eu/charts/analyse-one-indicator-and-compare-countries#chart={\u0022indicator-group\u0022:\u0022any\u0022,\u0022indicator\u0022:\u0022i_iunw\u0022,\u0022breakdown\u0022:\u0022IND_TOTAL\u0022,\u0022unit-measure\u0022:\u0022pc_ind_iu3\u0022,\u0022ref-area\u0022:[\u0022AT\u0022,\u0022BE\u0022,\u0022BG\u0022,\u0022HR\u0022,\u0022CY\u0022,\u0022CZ\u0022,\u0022DK\u0022,\u0022EE\u0022,\u0022EU\u0022,\u0022FI\u0022,\u0022FR\u0022,\u0022DE\u0022,\u0022EL\u0022,\u0022HU\u0022,\u0022IE\u0022,\u0022IT\u0022,\u0022LV\u0022,\u0022LT\u0022,\u0022LU\u0022,\u0022MT\u0022,\u0022NL\u0022,\u0022PL\u0022,\u0022PT\u0022,\u0022RO\u0022,\u0022SK\u0022,\u0022SI\u0022,\u0022ES\u0022,\u0022SE\u0022,\u0022UK\u0022]}> ;
	skos:notation	"old_desi_3a1_news" ;
	skos:definition	"Eurostat - Community survey on ICT usage in Households and by Individuals" ;
	skos:topConceptOf	ns1:source .
ns6:old_desi_3a2_mvg
	rdf:type	ns8:Source , skos:Concept ;
	skos:prefLabel	"Eurostat - ICT Households survey" ;
	foaf:page	<http://digital-agenda-data.eu/charts/analyse-one-indicator-and-compare-countries#chart={\u0022indicator-group\u0022:\u0022any\u0022,\u0022indicator\u0022:\u0022i_iugm\u0022,\u0022breakdown\u0022:\u0022IND_TOTAL\u0022,\u0022unit-measure\u0022:\u0022pc_ind_iu3\u0022,\u0022ref-area\u0022:[\u0022AT\u0022,\u0022BE\u0022,\u0022BG\u0022,\u0022HR\u0022,\u0022CY\u0022,\u0022CZ\u0022,\u0022DK\u0022,\u0022EE\u0022,\u0022EU\u0022,\u0022FI\u0022,\u0022FR\u0022,\u0022DE\u0022,\u0022EL\u0022,\u0022HU\u0022,\u0022IE\u0022,\u0022IT\u0022,\u0022LV\u0022,\u0022LT\u0022,\u0022LU\u0022,\u0022MT\u0022,\u0022NL\u0022,\u0022PL\u0022,\u0022PT\u0022,\u0022RO\u0022,\u0022SK\u0022,\u0022SI\u0022,\u0022ES\u0022,\u0022SE\u0022,\u0022UK\u0022]}> ;
	skos:notation	"old_desi_3a2_mvg" ;
	skos:definition	"Eurostat - Community survey on ICT usage in Households and by Individuals" ;
	skos:topConceptOf	ns1:source .
ns6:old_desi_3a3_vod
	rdf:type	ns8:Source , skos:Concept ;
	skos:prefLabel	"Eurostat - ICT Households survey" ;
	foaf:page	<http://digital-agenda-data.eu/charts/analyse-one-indicator-and-compare-countries#chart={\u0022indicator-group\u0022:\u0022any\u0022,\u0022indicator\u0022:\u0022vod\u0022,\u0022breakdown\u0022:\u0022HH_total\u0022,\u0022unit-measure\u0022:\u0022pc_EBhh_tv\u0022,\u0022ref-area\u0022:[\u0022AT\u0022,\u0022BE\u0022,\u0022CY\u0022,\u0022CZ\u0022,\u0022DK\u0022,\u0022EE\u0022,\u0022FI\u0022,\u0022FR\u0022,\u0022DE\u0022,\u0022EL\u0022,\u0022HU\u0022,\u0022IE\u0022,\u0022IT\u0022,\u0022LV\u0022,\u0022LT\u0022,\u0022LU\u0022,\u0022MT\u0022,\u0022NL\u0022,\u0022PL\u0022,\u0022PT\u0022,\u0022RO\u0022,\u0022SK\u0022,\u0022SI\u0022,\u0022ES\u0022,\u0022SE\u0022,\u0022UK\u0022]}> ;
	skos:notation	"old_desi_3a3_vod" ;
	skos:definition	"Eurostat - Community survey on ICT usage in Households and by Individuals" ;
	skos:topConceptOf	ns1:source .
ns6:old_desi_3a4_iptv
	rdf:type	ns8:Source , skos:Concept ;
	skos:prefLabel	"IHS TV Media Intelligence" ;
	foaf:page	<http://digital-agenda-data.eu/charts/analyse-one-indicator-and-compare-countries#chart={\u0022indicator-group\u0022:\u0022any\u0022,\u0022indicator\u0022:\u0022iptv\u0022,\u0022breakdown\u0022:\u0022HH_total\u0022,\u0022unit-measure\u0022:\u0022pc_EBhh_tv\u0022,\u0022ref-area\u0022:[\u0022AT\u0022,\u0022BE\u0022,\u0022BG\u0022,\u0022HR\u0022,\u0022CY\u0022,\u0022CZ\u0022,\u0022DK\u0022,\u0022EE\u0022,\u0022FI\u0022,\u0022FR\u0022,\u0022DE\u0022,\u0022EL\u0022,\u0022HU\u0022,\u0022IE\u0022,\u0022IT\u0022,\u0022LV\u0022,\u0022LT\u0022,\u0022LU\u0022,\u0022MT\u0022,\u0022NL\u0022,\u0022PL\u0022,\u0022PT\u0022,\u0022RO\u0022,\u0022SK\u0022,\u0022SI\u0022,\u0022ES\u0022,\u0022SE\u0022,\u0022UK\u0022]}> ;
	skos:notation	"old_desi_3a4_iptv" ;
	skos:definition	"IHS Technology databases - TV Media Intelligence Service - IPTV indicators" ;
	skos:topConceptOf	ns1:source .
ns6:old_desi_3b1_vidcall
	rdf:type	ns8:Source , skos:Concept ;
	skos:prefLabel	"Eurostat - ICT Households survey" ;
	foaf:page	<http://digital-agenda-data.eu/charts/analyse-one-indicator-and-compare-countries#chart={\u0022indicator-group\u0022:\u0022any\u0022,\u0022indicator\u0022:\u0022I_IUPH1\u0022,\u0022breakdown\u0022:\u0022IND_TOTAL\u0022,\u0022unit-measure\u0022:\u0022pc_ind_iu3\u0022,\u0022ref-area\u0022:[\u0022AT\u0022,\u0022BE\u0022,\u0022BG\u0022,\u0022HR\u0022,\u0022CY\u0022,\u0022CZ\u0022,\u0022DK\u0022,\u0022EE\u0022,\u0022EU\u0022,\u0022FI\u0022,\u0022FR\u0022,\u0022DE\u0022,\u0022EL\u0022,\u0022HU\u0022,\u0022IE\u0022,\u0022IT\u0022,\u0022LV\u0022,\u0022LT\u0022,\u0022LU\u0022,\u0022MT\u0022,\u0022NL\u0022,\u0022PL\u0022,\u0022PT\u0022,\u0022RO\u0022,\u0022SK\u0022,\u0022SI\u0022,\u0022ES\u0022,\u0022SE\u0022,\u0022UK\u0022]}> ;
	skos:notation	"old_desi_3b1_vidcall" ;
	skos:definition	"Eurostat - Community survey on ICT usage in Households and by Individuals" ;
	skos:topConceptOf	ns1:source .
ns6:old_desi_3b2_socnet
	rdf:type	ns8:Source , skos:Concept ;
	skos:prefLabel	"Eurostat - ICT Households survey" ;
	foaf:page	<http://digital-agenda-data.eu/charts/analyse-one-indicator-and-compare-countries#chart={\u0022indicator-group\u0022:\u0022any\u0022,\u0022indicator\u0022:\u0022i_iusnet\u0022,\u0022breakdown\u0022:\u0022IND_TOTAL\u0022,\u0022unit-measure\u0022:\u0022pc_ind_iu3\u0022,\u0022ref-area\u0022:[\u0022AT\u0022,\u0022BE\u0022,\u0022BG\u0022,\u0022HR\u0022,\u0022CY\u0022,\u0022CZ\u0022,\u0022DK\u0022,\u0022EE\u0022,\u0022EU\u0022,\u0022FI\u0022,\u0022FR\u0022,\u0022DE\u0022,\u0022EL\u0022,\u0022HU\u0022,\u0022IE\u0022,\u0022IT\u0022,\u0022LV\u0022,\u0022LT\u0022,\u0022LU\u0022,\u0022MT\u0022,\u0022NL\u0022,\u0022PL\u0022,\u0022PT\u0022,\u0022RO\u0022,\u0022SK\u0022,\u0022SI\u0022,\u0022ES\u0022,\u0022SE\u0022,\u0022UK\u0022]}> ;
	skos:notation	"old_desi_3b2_socnet" ;
	skos:definition	"Eurostat - Community survey on ICT usage in Households and by Individuals" ;
	skos:topConceptOf	ns1:source .
ns6:old_desi_4a1_eis
	rdf:type	ns8:Source , skos:Concept ;
	skos:prefLabel	"Eurostat - ICT Enterprises survey" ;
	foaf:page	<http://digital-agenda-data.eu/charts/analyse-one-indicator-and-compare-countries#chart={\u0022indicator-group\u0022:\u0022any\u0022,\u0022indicator\u0022:\u0022E_ERP1\u0022,\u0022breakdown\u0022:\u0022ent_all_xfin\u0022,\u0022unit-measure\u0022:\u0022pc_ent\u0022,\u0022ref-area\u0022:[\u0022AT\u0022,\u0022BE\u0022,\u0022BG\u0022,\u0022HR\u0022,\u0022CY\u0022,\u0022CZ\u0022,\u0022DK\u0022,\u0022EE\u0022,\u0022EU\u0022,\u0022FI\u0022,\u0022FR\u0022,\u0022DE\u0022,\u0022EL\u0022,\u0022HU\u0022,\u0022IE\u0022,\u0022IT\u0022,\u0022LV\u0022,\u0022LT\u0022,\u0022LU\u0022,\u0022MT\u0022,\u0022NL\u0022,\u0022PL\u0022,\u0022PT\u0022,\u0022RO\u0022,\u0022SK\u0022,\u0022SI\u0022,\u0022ES\u0022,\u0022SE\u0022,\u0022UK\u0022]}> ;
	skos:notation	"old_desi_4a1_eis" ;
	skos:definition	"Eurostat - Community survey on ICT usage and eCommerce in Enterprises" ;
	skos:topConceptOf	ns1:source .
ns6:old_desi_4a2_rfid
	rdf:type	ns8:Source , skos:Concept ;
	skos:prefLabel	"Eurostat - ICT Enterprises survey" ;
	foaf:page	<http://digital-agenda-data.eu/charts/analyse-one-indicator-and-compare-countries#chart={\u0022indicator-group\u0022:\u0022any\u0022,\u0022indicator\u0022:\u0022e_rfpsas\u0022,\u0022breakdown\u0022:\u0022ent_all_xfin\u0022,\u0022unit-measure\u0022:\u0022pc_ent\u0022,\u0022ref-area\u0022:[\u0022AT\u0022,\u0022BE\u0022,\u0022BG\u0022,\u0022HR\u0022,\u0022CY\u0022,\u0022CZ\u0022,\u0022DK\u0022,\u0022EE\u0022,\u0022EU\u0022,\u0022FI\u0022,\u0022FR\u0022,\u0022DE\u0022,\u0022EL\u0022,\u0022HU\u0022,\u0022IE\u0022,\u0022IT\u0022,\u0022LV\u0022,\u0022LT\u0022,\u0022LU\u0022,\u0022MT\u0022,\u0022NL\u0022,\u0022PL\u0022,\u0022PT\u0022,\u0022RO\u0022,\u0022SK\u0022,\u0022SI\u0022,\u0022ES\u0022,\u0022SE\u0022,\u0022UK\u0022]}> ;
	skos:notation	"old_desi_4a2_rfid" ;
	skos:definition	"Eurostat - Community survey on ICT usage and eCommerce in Enterprises" ;
	skos:topConceptOf	ns1:source .
ns6:old_desi_4a3_socmed
	rdf:type	ns8:Source , skos:Concept ;
	skos:prefLabel	"Eurostat - ICT Enterprises survey" ;
	foaf:page	<http://digital-agenda-data.eu/charts/analyse-one-indicator-and-compare-countries#chart={\u0022indicator-group\u0022:\u0022any\u0022,\u0022indicator\u0022:\u0022e_sm_ge2\u0022,\u0022breakdown\u0022:\u0022ent_all_xfin\u0022,\u0022unit-measure\u0022:\u0022pc_ent\u0022,\u0022ref-area\u0022:[\u0022AT\u0022,\u0022BE\u0022,\u0022BG\u0022,\u0022HR\u0022,\u0022CY\u0022,\u0022CZ\u0022,\u0022DK\u0022,\u0022EE\u0022,\u0022EU\u0022,\u0022FI\u0022,\u0022FR\u0022,\u0022DE\u0022,\u0022EL\u0022,\u0022HU\u0022,\u0022IE\u0022,\u0022IT\u0022,\u0022LV\u0022,\u0022LT\u0022,\u0022LU\u0022,\u0022MT\u0022,\u0022NL\u0022,\u0022PL\u0022,\u0022PT\u0022,\u0022RO\u0022,\u0022SK\u0022,\u0022SI\u0022,\u0022ES\u0022,\u0022SE\u0022,\u0022UK\u0022]}> ;
	skos:notation	"old_desi_4a3_socmed" ;
	skos:definition	"Eurostat - Community survey on ICT usage and eCommerce in Enterprises" ;
	skos:topConceptOf	ns1:source .
ns6:old_desi_4a4_einv
	rdf:type	ns8:Source , skos:Concept ;
	skos:prefLabel	"Eurostat - ICT Enterprises survey" ;
	foaf:page	<http://digital-agenda-data.eu/charts/analyse-one-indicator-and-compare-countries#chart={\u0022indicator-group\u0022:\u0022any\u0022,\u0022indicator\u0022:\u0022e_invsnd\u0022,\u0022breakdown\u0022:\u0022ent_all_xfin\u0022,\u0022unit-measure\u0022:\u0022pc_ent\u0022,\u0022ref-area\u0022:[\u0022AT\u0022,\u0022BE\u0022,\u0022BG\u0022,\u0022HR\u0022,\u0022CY\u0022,\u0022CZ\u0022,\u0022DK\u0022,\u0022EE\u0022,\u0022EU\u0022,\u0022FI\u0022,\u0022FR\u0022,\u0022DE\u0022,\u0022EL\u0022,\u0022HU\u0022,\u0022IE\u0022,\u0022IT\u0022,\u0022LV\u0022,\u0022LT\u0022,\u0022LU\u0022,\u0022MT\u0022,\u0022NL\u0022,\u0022PL\u0022,\u0022PT\u0022,\u0022RO\u0022,\u0022SK\u0022,\u0022SI\u0022,\u0022ES\u0022,\u0022SE\u0022,\u0022UK\u0022]}> ;
	skos:notation	"old_desi_4a4_einv" ;
	skos:definition	"Eurostat - Community survey on ICT usage and eCommerce in Enterprises" ;
	skos:topConceptOf	ns1:source .
ns6:old_desi_4a5_cloud
	rdf:type	ns8:Source , skos:Concept ;
	skos:prefLabel	"Eurostat - ICT Enterprises survey" ;
	foaf:page	<http://digital-agenda-data.eu/charts/analyse-one-indicator-and-compare-countries#chart={\u0022indicator-group\u0022:\u0022any\u0022,\u0022indicator\u0022:\u0022e_CC_GE_ME\u0022,\u0022breakdown\u0022:\u0022ent_all_xfin\u0022,\u0022unit-measure\u0022:\u0022pc_ent\u0022,\u0022ref-area\u0022:[\u0022AT\u0022,\u0022BE\u0022,\u0022BG\u0022,\u0022HR\u0022,\u0022CY\u0022,\u0022CZ\u0022,\u0022DK\u0022,\u0022EE\u0022,\u0022EU\u0022,\u0022FI\u0022,\u0022FR\u0022,\u0022DE\u0022,\u0022EL\u0022,\u0022HU\u0022,\u0022IE\u0022,\u0022IT\u0022,\u0022LV\u0022,\u0022LT\u0022,\u0022LU\u0022,\u0022MT\u0022,\u0022NL\u0022,\u0022PL\u0022,\u0022PT\u0022,\u0022RO\u0022,\u0022SK\u0022,\u0022SI\u0022,\u0022ES\u0022,\u0022SE\u0022,\u0022UK\u0022]}> ;
	skos:notation	"old_desi_4a5_cloud" ;
	skos:definition	"Eurostat - Community survey on ICT usage and eCommerce in Enterprises" ;
	skos:topConceptOf	ns1:source .
ns6:estathh_cocom
	rdf:type	ns8:Source , skos:Concept ;
	skos:prefLabel	"European Commission based on Eurostat - ICT Household survey and Communications Committee survey" ;
	skos:notation	"estathh_cocom" ;
	skos:definition	"European Commission based on Eurostat - Community survey on ICT usage in Households and by Individuals, and Electronic communications market indicators collected by Commission services, through National Regulatory Authorities, for the Communications Committee (COCOM) - January and July reports." ;
	skos:topConceptOf	ns1:source .
