@prefix rdf:	<http://www.w3.org/1999/02/22-rdf-syntax-ns#> .
@prefix ns1:	<http://semantic.digital-agenda-data.eu/codelist/indicator/> .
@prefix ns2:	<http://semantic.digital-agenda-data.eu/def/class/> .
ns1:e_di3_hi	rdf:type	ns2:Indicator .
@prefix skos:	<http://www.w3.org/2004/02/skos/core#> .
ns1:e_di3_hi	rdf:type	skos:Concept ;
	skos:prefLabel	"Enterprises with high digital intensity index (DII v3)" .
@prefix dct:	<http://purl.org/dc/terms/> .
@prefix ns5:	<http://semantic.digital-agenda-data.eu/codelist/source/> .
ns1:e_di3_hi	dct:source	ns5:estat-ent ;
	skos:notation	"e_di3_hi" ;
	skos:altLabel	"Enterprises with high digital intensity index (DII v3)" .
@prefix ns6:	<http://semantic.digital-agenda-data.eu/def/property/> .
@prefix ns7:	<http://semantic.digital-agenda-data.eu/codelist/indicator-group/ebusiness/> .
ns1:e_di3_hi	ns6:membership	ns7:e_di3_hi ;
	skos:definition	"Enterprises with high digital intensity index (DII v3)" .
@prefix ns8:	<http://semantic.digital-agenda-data.eu/codelist/> .
ns1:e_di3_hi	skos:topConceptOf	ns8:indicator .
ns1:e_di3_lo	rdf:type	ns2:Indicator ,
		skos:Concept ;
	skos:prefLabel	"Enterprises with low digital intensity index (DII v3)" ;
	dct:source	ns5:estat-ent ;
	skos:notation	"e_di3_lo" ;
	skos:altLabel	"Enterprises with low digital intensity index (DII v3)" ;
	ns6:membership	ns7:e_di3_lo ;
	skos:definition	"Enterprises with low digital intensity index (DII v3)" ;
	skos:topConceptOf	ns8:indicator .
ns1:e_di3_vhi	rdf:type	ns2:Indicator ,
		skos:Concept ;
	skos:prefLabel	"Enterprises with very high digital intensity index (DII v3)" ;
	dct:source	ns5:estat-ent ;
	skos:notation	"e_di3_vhi" ;
	skos:altLabel	"Enterprises with very high digital intensity index (DII v3)" ;
	ns6:membership	ns7:e_di3_vhi ;
	skos:definition	"Enterprises with very high digital intensity index (DII v3)" ;
	skos:topConceptOf	ns8:indicator .
ns1:e_di3_vlo	rdf:type	ns2:Indicator ,
		skos:Concept ;
	skos:prefLabel	"Enterprises with very low digital intensity index (DII v3)" ;
	dct:source	ns5:estat-ent ;
	skos:notation	"e_di3_vlo" ;
	skos:altLabel	"Enterprises with very low digital intensity index (DII v3)" ;
	ns6:membership	ns7:e_di3_vlo ;
	skos:definition	"Enterprises with very low digital intensity index (DII v3)" ;
	skos:topConceptOf	ns8:indicator .
ns1:e_ai_tany	rdf:type	ns2:Indicator ,
		skos:Concept ;
	skos:prefLabel	"Enterprises using AI technologies" ;
	dct:source	ns5:estat_isoc_eb_ai ;
	skos:notation	"e_ai_tany" ;
	skos:altLabel	"Enterprises using AI technologies" ;
	ns6:membership	ns7:e_ai_tany ;
	skos:definition	"Enterprises using at least one of the following AI technologies: analysis of written language, converting spoken language into machine-readable format, generating written or spoken language,  identifying objects or persons based on images,  machine learning (e.g. deep learning), automating different workflows or assisting in decision making or enabling physical movement of machines via autonomous decisions based on observation of surroundings" ;
	skos:topConceptOf	ns8:indicator .
ns1:e_cc1_si	rdf:type	ns2:Indicator ,
		skos:Concept ;
	skos:prefLabel	"Enterprises buying sophisticated or intermediate cloud computing services" ;
	dct:source	ns5:estat_isoc_cicce_use ;
	skos:notation	"e_cc1_si" ;
	skos:altLabel	"Enterprises buying sophisticated or intermediate cloud computing services" ;
	ns6:membership	ns7:e_cc1_si ;
	skos:definition	"Enterprises purchasing at least one of the following cloud computing services: accounting/finance/ERP software, CRM software, hosting for the enterprise's database, hosted environment for application development" ;
	skos:topConceptOf	ns8:indicator .
@prefix ns9:	<http://purl.org/linked-data/sdmx#> .
ns8:indicator	rdf:type	ns9:CodeList ,
		skos:ConceptScheme .
@prefix xsd:	<http://www.w3.org/2001/XMLSchema#> .
ns8:indicator	dct:modified	"2023-07-05T14:06:09"^^xsd:dateTime .
@prefix rdfs:	<http://www.w3.org/2000/01/rdf-schema#> .
ns8:indicator	rdfs:isDefinedBy	<http://digital-agenda-data.eu/> ;
	skos:prefLabel	"Code list for indicators used by Digital Agenda Scoreboard" ;
	skos:notation	"CL_INDICATOR" ;
	skos:hasTopConcept	ns1:e_gov_dpsc ,
		ns1:e_gov_od ,
		ns1:desi_dps_prefform ,
		ns1:desi_dps_pscit ,
		ns1:desi_idt_smedi ,
		ns1:e_bda ,
		ns1:e_inv4s_ap ,
		ns1:e_ai_tany ,
		ns1:e_cc1_si ,
		ns1:i_dsk2_na ,
		ns1:e_di3_hi ,
		ns1:e_di3_lo ,
		ns1:e_di3_vhi ,
		ns1:e_di3_vlo ,
		ns1:e_gov_4c_cb_eid ,
		ns1:e_gov_4d_cb_edoc ,
		ns1:mbb_5gcov ,
		ns1:mbb_r5gcov ,
		ns1:e_gov_3_ke ,
		ns1:e_gov_3a_ke_eid ,
		ns1:e_gov_3b_ke_edoc ,
		ns1:e_gov_3c_ke_as ,
		ns1:e_gov_3d_ke_dp ,
		ns1:e_gov_4_cb ,
		ns1:e_gov_4a_cb_oa ,
		ns1:e_gov_4b_cb_us ,
		ns1:e_gov_1a_uc_oa ,
		ns1:e_gov_1b_uc_mf ,
		ns1:e_gov_1c_uc_us ,
		ns1:e_gov_2_tr ,
		ns1:e_gov_2a_tr_sd ,
		ns1:e_gov_2x_tr_po ,
		<http://semantic.digital-agenda-data.eu/codelist/indicator/5g_read> ,
		ns1:bb_rvhcncov ,
		ns1:bb_vhcncov ,
		ns1:e_gov_1_uc ,
		ns1:i_dsk2_x ,
		ns1:i_dsk2_ps_b ,
		ns1:i_dsk2_ps_bab ,
		ns1:i_dsk2_sf_ab ,
		ns1:i_dsk2_sf_b ,
		ns1:i_dsk2_sf_bab ,
		ns1:i_dsk_ps_ab ,
		ns1:i_dsk_s_ab ,
		ns1:i_dsk_l ,
		ns1:edigint2022 ,
		ns1:e_gov_ebus ,
		ns1:edigint2018 ,
		ns1:edigint2021 ,
		ns1:h_fbbfix ,
		ns1:h_ubbfix ,
		ns1:i_dsk_x ,
		ns1:i_dsk_c_x ,
		ns1:i_dsk_s_x ,
		ns1:i_dsk_c_ab ,
		ns1:e_gov_0_score ,
		ns1:e_gov_2b_tr_pd ,
		ns1:e_gov_2c_tr_de ,
		ns1:rid_score ,
		ns1:rid_ui ,
		ns1:rid_ui_egov ,
		ns1:e_gov_4b_bm_us ,
		ns1:rid_ui_ib ,
		ns1:rid_ui_iu ,
		ns1:rid_ui_nui ,
		ns1:rid_ui_oc ,
		ns1:rid_ui_part ,
		ns1:rid_c_fttpc ,
		ns1:rid_c_mbbtu ,
		ns1:rid_c_vhcnc ,
		ns1:rid_ius ,
		ns1:rid_ius_abs ,
		ns1:rid_ius_bs ,
		ns1:rid_ius_icts ,
		ns1:rid_ius_ss ,
		ns1:desi_fttpc ,
		ns1:rid_c ,
		ns1:rid_c_5gc ,
		ns1:rid_c_fbbc ,
		ns1:rid_c_fbbtc ,
		<http://semantic.digital-agenda-data.eu/codelist/indicator/5g_cov_3400_3800> ,
		<http://semantic.digital-agenda-data.eu/codelist/indicator/5g_spectrum> ,
		ns1:sme_di_x_vlo ,
		ns1:wid_ui_ib ,
		ns1:e_di4_lo ,
		ns1:wid_ui_iu ,
		ns1:e_di4_vhi ,
		ns1:wid_ui_nui ,
		ns1:wid_ui_oc ,
		ns1:e_di4_vlo ,
		ns1:wid_ui_part ,
		ns1:wid_ius_ss ,
		ns1:wid_score ,
		ns1:wid_sse ,
		ns1:wid_sse_gpg ,
		ns1:wid_sse_icts ,
		ns1:wid_sse_stem ,
		ns1:wid_ui ,
		ns1:wid_ui_egov ,
		ns1:transparent_egov ,
		ns1:user_centric_egov ,
		ns1:val_add_ict ,
		ns1:wid_ius ,
		ns1:wid_ius_abs ,
		ns1:wid_ius_bs ,
		ns1:price_internet_fixed_tel_tv ,
		ns1:price_internet_only ,
		ns1:spectrum_wbb ,
		ns1:st_grad ,
		ns1:tel_ftr ,
		ns1:tel_inv ,
		ns1:tel_llu ,
		ns1:tel_rev ,
		ns1:mob_roam ,
		ns1:mob_subs ,
		ns1:p_empmd ,
		ns1:p_iuse ,
		ns1:population ,
		ns1:price_internet_fixed_tel ,
		ns1:mbb_penet ,
		ns1:mbb_rhspacov ,
		ns1:mbb_rltecov ,
		ns1:mob_arpm ,
		ns1:mob_arpu ,
		ns1:mob_ms ,
		ns1:mob_mtr ,
		ns1:mob_penet ,
		ns1:ict_hgc ,
		ns1:ict_imp ,
		ns1:ict_spec3_broad ,
		ns1:ict_specialists ,
		ns1:labour_prod_ict ,
		ns1:mbb_3gcov ,
		ns1:mbb_hspacov ,
		ns1:mbb_ltecov ,
		ns1:i_dsk_i_ab ,
		ns1:i_dsk_ab ,
		ns1:i_dsk_i_x ,
		ns1:i_dsk_ps_x ,
		ns1:e_gov_dpsc_new ,
		ns1:e_gov_ebus_new ,
		ns1:e_gov_pff_new ,
		ns1:desi_sliders ,
		ns1:c1_datatraffic ,
		ns1:desi ,
		ns1:e_gov_ke ,
		ns1:e_gov_opa ,
		ns1:e_gov_osc ,
		ns1:e_gov_pff ,
		ns1:e_igov ,
		ns1:e_igov2pr ,
		ns1:e_igovrt ,
		ns1:e_gov_5_ke ,
		ns1:e_gov_5a_ke_eid ,
		ns1:e_gov_5b_ke_edoc ,
		ns1:e_gov_5c_ke_as ,
		ns1:e_gov_5d_ke_dp ,
		ns1:e_gov_5e_ke_esafe ,
		ns1:e_gov_5f_ke_sso ,
		ns1:e_gov_3e_cm_eu ,
		ns1:e_gov_3f_cm_su ,
		ns1:e_gov_4_bm ,
		ns1:e_gov_4a_bm_oa ,
		ns1:e_gov_4c_bm_eidcb ,
		ns1:e_gov_4d_bm_edoccb ,
		ns1:e_gov_4e_bm_eu ,
		ns1:e_gov_4f_bm_su ,
		ns1:e_gov_2a_tg_sd ,
		ns1:e_gov_2b_tg_po ,
		ns1:e_gov_2c_tg_pd ,
		ns1:e_gov_3_cm ,
		ns1:e_gov_3a_cm_oa ,
		ns1:e_gov_3b_cm_us ,
		ns1:e_gov_3c_cm_eidcb ,
		ns1:e_gov_3d_cm_edoccb ,
		ns1:e_eturn ,
		ns1:e_gov_1_ucg ,
		ns1:e_gov_1a_ucg_oa ,
		ns1:e_gov_1b_ucg_us ,
		ns1:e_gov_1c_ucg_mf ,
		ns1:e_gov_1d_ucg_eu ,
		ns1:e_gov_1e_ucg_su ,
		ns1:e_gov_2_tg ,
		ns1:e_cc_pcpu ,
		ns1:e_crman ,
		ns1:e_di_hivhi ,
		ns1:e_di_vlo ,
		ns1:e_ebuy ,
		ns1:e_empmd_gt20 ,
		ns1:e_erp1 ,
		ns1:e_esell ,
		ns1:e_aws_cown ,
		ns1:e_aws_gt1_b2c_gt10ws ,
		ns1:e_awsval_cmp ,
		ns1:e_awsval_cown ,
		ns1:e_bd ,
		ns1:e_broad ,
		ns1:e_cc ,
		ns1:e_cc_ge_me ,
		ns1:e_ade ,
		ns1:e_ads ,
		ns1:e_ads_loc ,
		ns1:e_ads_trk ,
		ns1:e_aeseu ,
		ns1:e_aws ,
		ns1:e_aws_cmp ,
		ns1:h2020_totcost ,
		ns1:h2020ict_afxp ,
		ns1:h_bbfix ,
		ns1:h_broad ,
		ns1:h_iacc ,
		ns1:h_xcost ,
		ns1:hie_use_ex_admin ,
		ns1:hie_use_pharm ,
		ns1:gbaord ,
		ns1:gbaord_ict ,
		ns1:gdp ,
		ns1:h2020_cofin ,
		ns1:h2020_ec_funding ,
		ns1:h2020_newentry ,
		ns1:h2020_organisations ,
		ns1:h2020_particip ,
		ns1:fp7ict_ec_funding_prc ,
		ns1:fp7ict_ec_funding_smes ,
		ns1:fp7ict_newentry ,
		ns1:fp7ict_organisations ,
		ns1:fp7ict_particip ,
		ns1:fp7ict_particip_prc ,
		ns1:fp7ict_particip_smes ,
		ns1:fp7ict_totcost ,
		ns1:e_di4_hi ,
		ns1:foa_cit ,
		ns1:foa_ent ,
		ns1:fp7_ict_artic ,
		ns1:fp7_ict_pat ,
		ns1:fp7_ict_pub ,
		ns1:fp7ict_afxp ,
		ns1:fp7ict_cofin ,
		ns1:fp7ict_ec_funding ,
		ns1:edigint2015 ,
		ns1:employment_ict ,
		ns1:eoa_nn_films ,
		ns1:eoa_tvchannels_tarfor ,
		ns1:eoa_vod_estab_otheu ,
		ns1:epsi_score ,
		ns1:eun_computers ,
		ns1:eun_web ,
		ns1:e_sisc ,
		ns1:e_sisorp ,
		ns1:e_sm_any ,
		ns1:e_sm_ge2 ,
		ns1:e_web ,
		ns1:e_webf2 ,
		ns1:e_wsel25 ,
		ns1:e_wsel50 ,
		ns1:e_itt2 ,
		ns1:e_pmd ,
		ns1:e_pmd_app ,
		ns1:e_ra ,
		ns1:e_rfac ,
		ns1:e_rfid ,
		ns1:e_rfpsas ,
		ns1:e_secpol1 ,
		ns1:e_inv ,
		ns1:e_invsnd ,
		ns1:e_ispdf_ge30 ,
		ns1:e_ispdfokx ,
		ns1:e_ispdfokx_ge100 ,
		ns1:e_it_mext ,
		ns1:e_itsp2 ,
		ns1:e_itspvac2 ,
		ns1:i_piacadv ,
		ns1:i_sbgood ,
		ns1:i_secfl ,
		ns1:i_secpif1 ,
		ns1:i_secvir1 ,
		ns1:i_skedu ,
		ns1:ict_commit_in_trp ,
		ns1:ict_exp ,
		ns1:i_iuph1 ,
		ns1:i_iuse ,
		ns1:i_iusell ,
		ns1:i_iusnet ,
		ns1:i_iuupl ,
		ns1:i_iuvod ,
		ns1:i_iuvote ,
		ns1:i_iux ,
		ns1:i_iugov ,
		ns1:i_iugov12 ,
		ns1:i_iuif ,
		ns1:i_iujob ,
		ns1:i_iumapp ,
		ns1:i_iumc ,
		ns1:i_iunw ,
		ns1:i_iuolc ,
		ns1:i_ihif ,
		ns1:i_ilt12 ,
		ns1:i_isk_ge_me ,
		ns1:i_iu3 ,
		ns1:i_iu3g ,
		ns1:i_iubk ,
		ns1:i_iueduif ,
		ns1:i_iugm ,
		ns1:i_dsk_c_bab ,
		ns1:i_dsk_i_bab ,
		ns1:i_dsk_ps_bab ,
		ns1:i_dsk_s_bab ,
		ns1:i_iday ,
		ns1:i_igov12rt ,
		ns1:i_igovrt ,
		ns1:i_cc ,
		ns1:i_cisk_sfjob ,
		ns1:i_cisk_sfjobx ,
		ns1:i_cook ,
		ns1:i_cprg ,
		ns1:i_csk_ge_me ,
		ns1:i_cweb ,
		ns1:i_dsk_bab ,
		ns1:i_atsw ,
		ns1:i_barr1x ,
		ns1:i_bfeu ,
		ns1:i_bgood ,
		ns1:i_bgoodo ,
		ns1:i_blt12 ,
		ns1:i_bpgood ,
		ns1:i_bserv ,
		ns1:househ ,
		ns1:households ,
		ns1:desi_hc_entict ,
		ns1:desi_hc_fictspec ,
		ns1:desi_hc_ictg ,
		ns1:desi_hc_ictspec ,
		ns1:desi_idt ,
		ns1:desi_idt_ai ,
		ns1:desi_idt_bigdat ,
		ns1:desi_idt_cloud ,
		ns1:desi_fbbtc ,
		ns1:desi_gbpstc ,
		ns1:desi_hc ,
		ns1:desi_hc_abds ,
		ns1:desi_hc_abss ,
		ns1:desi_hc_asd ,
		ns1:desi_hc_bds ,
		ns1:desi_hc_bsu ,
		ns1:desi_c_mbb ,
		ns1:desi_conn ,
		ns1:desi_dps ,
		ns1:desi_dps_egov ,
		ns1:desi_dps_egovuser ,
		ns1:desi_dps_opendata ,
		ns1:desi_dps_psbiz ,
		ns1:desi_fbbc ,
		ns1:desi_5g ,
		ns1:desi_5gc ,
		ns1:desi_bbpi ,
		ns1:desi_c_bbpi ,
		ns1:desi_c_fbbc ,
		ns1:desi_c_fbbtc ,
		ns1:desi_idt_smeso ,
		ns1:desi_idt_socmed ,
		ns1:desi_mbbtu ,
		ns1:desi_total ,
		ns1:desi_ufbbtu ,
		ns1:desi_vhcnc ,
		ns1:desi_idt_di ,
		ns1:desi_idt_dtb ,
		ns1:desi_idt_ecomm ,
		ns1:desi_idt_ecomturn ,
		ns1:desi_idt_einv ,
		ns1:desi_idt_eis ,
		ns1:desi_idt_ictsust ,
		ns1:desi_idt_sellcb ,
		ns1:bb_speed100 ,
		ns1:bb_speed2 ,
		ns1:bb_speed30 ,
		ns1:bb_srcov ,
		ns1:bs_rd_expen_ict ,
		ns1:c1_bandwidth ,
		ns1:c1_compcyclesegi ,
		ns1:c1_compcyclesprace ,
		ns1:bb_lines ,
		ns1:bb_ne ,
		ns1:bb_ngacov ,
		ns1:bb_penet ,
		ns1:bb_rfttpcov ,
		ns1:bb_rngacov ,
		ns1:bb_scov ,
		ns1:bb_speed10 ,
		ns1:aaaa_cov ,
		ns1:actspeed ,
		ns1:afford_internet_only_minppp ,
		ns1:avg_ttg ,
		ns1:bb_dsl ,
		ns1:bb_fcov ,
		ns1:bb_fttpcov ,
		ns1:bb_hhi ,
		ns1:i_dsk2_dcc_b ,
		ns1:i_dsk2_dcc_bab ,
		ns1:i_dsk2_ic_s ,
		ns1:i_dsk2_il_ab ,
		ns1:i_dsk2_il_b ,
		ns1:i_dsk2_il_bab ,
		ns1:i_dsk2_lm ,
		ns1:i_dsk2_lw ,
		ns1:i_dsk2_ab ,
		ns1:i_dsk2_b ,
		ns1:i_dsk2_bab ,
		ns1:i_dsk2_cc_ab ,
		ns1:i_dsk2_cc_b ,
		ns1:i_dsk2_cc_bab ,
		ns1:i_dsk2_dcc_ab ,
		ns1:ict_grad ,
		ns1:i_dsk2_n ,
		ns1:i_dsk2_ps_ab .
@prefix ns12:	<http://semantic.digital-agenda-data.eu/def/> .
ns8:indicator	skos:inScheme	ns12:scheme .
@prefix ns13:	<http://semantic.digital-agenda-data.eu/codelist/indicator-group/audiovisual/> .
ns13:eoa_nn_films	rdf:type	ns2:IndicatorToGroupMembership ;
	rdfs:label	"audiovisual" .
@prefix ns14:	<http://semantic.digital-agenda-data.eu/codelist/indicator-group/> .
ns13:eoa_nn_films	ns6:member-of	ns14:audiovisual ;
	ns6:order	"3" .
ns13:eoa_tvchannels_tarfor	rdf:type	ns2:IndicatorToGroupMembership ;
	rdfs:label	"audiovisual" ;
	ns6:member-of	ns14:audiovisual ;
	ns6:order	"1" .
ns13:eoa_vod_estab_otheu	rdf:type	ns2:IndicatorToGroupMembership ;
	rdfs:label	"audiovisual" ;
	ns6:member-of	ns14:audiovisual ;
	ns6:order	"2" .
ns13:i_iugm	rdf:type	ns2:IndicatorToGroupMembership ;
	rdfs:label	"audiovisual" ;
	ns6:member-of	ns14:audiovisual ;
	ns6:order	"6" .
ns13:i_iunw	rdf:type	ns2:IndicatorToGroupMembership ;
	rdfs:label	"audiovisual" ;
	ns6:member-of	ns14:audiovisual ;
	ns6:order	"5" .
ns13:i_iuvod	rdf:type	ns2:IndicatorToGroupMembership ;
	rdfs:label	"audiovisual" ;
	ns6:member-of	ns14:audiovisual ;
	ns6:order	"12" .
@prefix ns15:	<http://semantic.digital-agenda-data.eu/codelist/indicator-group/back/> .
ns15:gdp	rdf:type	ns2:IndicatorToGroupMembership ;
	rdfs:label	"back" ;
	ns6:member-of	ns14:back ;
	ns6:order	"4" .
ns15:househ	rdf:type	ns2:IndicatorToGroupMembership ;
	rdfs:label	"back" ;
	ns6:member-of	ns14:back ;
	ns6:order	"1" .
ns15:households	rdf:type	ns2:IndicatorToGroupMembership ;
	rdfs:label	"back" ;
	ns6:member-of	ns14:back ;
	ns6:order	"5" .
ns15:population	rdf:type	ns2:IndicatorToGroupMembership ;
	rdfs:label	"back" ;
	ns6:member-of	ns14:back ;
	ns6:order	"3" .
@prefix ns16:	<http://semantic.digital-agenda-data.eu/codelist/indicator-group/bbquality/> .
ns16:actspeed	rdf:type	ns2:IndicatorToGroupMembership ;
	rdfs:label	"bbquality" ;
	ns6:member-of	ns14:bbquality ;
	ns6:order	"5" .
ns16:afford_internet_only_minppp	rdf:type	ns2:IndicatorToGroupMembership ;
	rdfs:label	"bbquality" ;
	ns6:member-of	ns14:bbquality ;
	ns6:order	"9" .
ns16:bb_speed10	rdf:type	ns2:IndicatorToGroupMembership ;
	rdfs:label	"bbquality" ;
	ns6:member-of	ns14:bbquality ;
	ns6:order	"2" .
ns16:bb_speed100	rdf:type	ns2:IndicatorToGroupMembership ;
	rdfs:label	"bbquality" ;
	ns6:member-of	ns14:bbquality ;
	ns6:order	"4" .
ns16:bb_speed2	rdf:type	ns2:IndicatorToGroupMembership ;
	rdfs:label	"bbquality" ;
	ns6:member-of	ns14:bbquality ;
	ns6:order	"1" .
ns16:bb_speed30	rdf:type	ns2:IndicatorToGroupMembership ;
	rdfs:label	"bbquality" ;
	ns6:member-of	ns14:bbquality ;
	ns6:order	"3" .
ns16:h_xcost	rdf:type	ns2:IndicatorToGroupMembership ;
	rdfs:label	"bbquality" ;
	ns6:member-of	ns14:bbquality ;
	ns6:order	"10" .
ns16:price_internet_fixed_tel	rdf:type	ns2:IndicatorToGroupMembership ;
	rdfs:label	"bbquality" ;
	ns6:member-of	ns14:bbquality ;
	ns6:order	"7" .
ns16:price_internet_fixed_tel_tv	rdf:type	ns2:IndicatorToGroupMembership ;
	rdfs:label	"bbquality" ;
	ns6:member-of	ns14:bbquality ;
	ns6:order	"8" .
ns16:price_internet_only	rdf:type	ns2:IndicatorToGroupMembership ;
	rdfs:label	"bbquality" ;
	ns6:member-of	ns14:bbquality ;
	ns6:order	"6" .
@prefix ns17:	<http://semantic.digital-agenda-data.eu/codelist/indicator-group/broadband/> .
ns17:bb_dsl	rdf:type	ns2:IndicatorToGroupMembership ;
	rdfs:label	"broadband" ;
	ns6:member-of	ns14:broadband ;
	ns6:order	"17" .
ns17:bb_fttpcov	rdf:type	ns2:IndicatorToGroupMembership ;
	rdfs:label	"broadband" ;
	ns6:member-of	ns14:broadband ;
	ns6:order	"7" .
ns17:bb_hhi	rdf:type	ns2:IndicatorToGroupMembership ;
	rdfs:label	"broadband" ;
	ns6:member-of	ns14:broadband .
ns17:bb_lines	rdf:type	ns2:IndicatorToGroupMembership ;
	rdfs:label	"broadband" ;
	ns6:member-of	ns14:broadband ;
	ns6:order	"16" .
ns17:bb_ne	rdf:type	ns2:IndicatorToGroupMembership ;
	rdfs:label	"broadband" ;
	ns6:member-of	ns14:broadband ;
	ns6:order	"18" .
ns17:bb_ngacov	rdf:type	ns2:IndicatorToGroupMembership ;
	rdfs:label	"broadband" ;
	ns6:member-of	ns14:broadband ;
	ns6:order	"3" .
ns17:bb_penet	rdf:type	ns2:IndicatorToGroupMembership ;
	rdfs:label	"broadband" ;
	ns6:member-of	ns14:broadband ;
	ns6:order	"15" .
ns17:bb_rfttpcov	rdf:type	ns2:IndicatorToGroupMembership ;
	rdfs:label	"broadband" ;
	ns6:member-of	ns14:broadband ;
	ns6:order	"8" .
ns17:bb_rngacov	rdf:type	ns2:IndicatorToGroupMembership ;
	rdfs:label	"broadband" ;
	ns6:member-of	ns14:broadband ;
	ns6:order	"4" .
ns17:bb_scov	rdf:type	ns2:IndicatorToGroupMembership ;
	rdfs:label	"broadband" ;
	ns6:member-of	ns14:broadband ;
	ns6:order	"5" .
ns17:bb_srcov	rdf:type	ns2:IndicatorToGroupMembership ;
	rdfs:label	"broadband" ;
	ns6:member-of	ns14:broadband ;
	ns6:order	"6" .
ns17:e_broad	rdf:type	ns2:IndicatorToGroupMembership ;
	rdfs:label	"broadband" ;
	ns6:member-of	ns14:broadband ;
	ns6:order	"13" .
ns17:e_ispdf_ge30	rdf:type	ns2:IndicatorToGroupMembership ;
	rdfs:label	"broadband" ;
	ns6:member-of	ns14:broadband ;
	ns6:order	"14" .
ns17:e_ispdfokx	rdf:type	ns2:IndicatorToGroupMembership ;
	rdfs:label	"broadband" ;
	ns6:member-of	ns14:broadband ;
	ns6:order	"19" .
ns17:e_ispdfokx_ge100	rdf:type	ns2:IndicatorToGroupMembership ;
	rdfs:label	"broadband" ;
	ns6:member-of	ns14:broadband ;
	ns6:order	"20" .
ns17:h_bbfix	rdf:type	ns2:IndicatorToGroupMembership ;
	rdfs:label	"broadband" ;
	ns6:member-of	ns14:broadband ;
	ns6:order	"10" .
ns17:h_broad	rdf:type	ns2:IndicatorToGroupMembership ;
	rdfs:label	"broadband" ;
	ns6:member-of	ns14:broadband ;
	ns6:order	"9" .
@prefix ns18:	<http://semantic.digital-agenda-data.eu/codelist/indicator-group/desi/> .
ns18:desi	rdf:type	ns2:IndicatorToGroupMembership ;
	rdfs:label	"desi" ;
	ns6:member-of	ns14:desi ;
	ns6:order	"2" .
@prefix ns19:	<http://semantic.digital-agenda-data.eu/codelist/indicator-group/desi_sliders/> .
ns19:desi_sliders	rdf:type	ns2:IndicatorToGroupMembership ;
	rdfs:label	"desi_sliders" ;
	ns6:member-of	ns14:desi_sliders ;
	ns6:order	"1" .
@prefix ns20:	<http://semantic.digital-agenda-data.eu/codelist/indicator-group/discontinued/> .
ns20:bb_fcov	rdf:type	ns2:IndicatorToGroupMembership ;
	rdfs:label	"discontinued" ;
	ns6:member-of	ns14:discontinued ;
	ns6:order	"16" .
ns20:e_ade	rdf:type	ns2:IndicatorToGroupMembership ;
	rdfs:label	"discontinued" ;
	ns6:member-of	ns14:discontinued ;
	ns6:order	"3" .
ns20:e_ebuy	rdf:type	ns2:IndicatorToGroupMembership ;
	rdfs:label	"discontinued" ;
	ns6:member-of	ns14:discontinued ;
	ns6:order	"5" .
ns20:e_igov	rdf:type	ns2:IndicatorToGroupMembership ;
	rdfs:label	"discontinued" ;
	ns6:member-of	ns14:discontinued ;
	ns6:order	"25" .
ns20:e_igov2pr	rdf:type	ns2:IndicatorToGroupMembership ;
	rdfs:label	"discontinued" ;
	ns6:member-of	ns14:discontinued ;
	ns6:order	"27" .
ns20:e_igovrt	rdf:type	ns2:IndicatorToGroupMembership ;
	rdfs:label	"discontinued" ;
	ns6:member-of	ns14:discontinued ;
	ns6:order	"26" .
ns20:e_inv	rdf:type	ns2:IndicatorToGroupMembership ;
	rdfs:label	"discontinued" ;
	ns6:member-of	ns14:discontinued ;
	ns6:order	"4" .
ns20:e_sisorp	rdf:type	ns2:IndicatorToGroupMembership ;
	rdfs:label	"discontinued" ;
	ns6:member-of	ns14:discontinued ;
	ns6:order	"2" .
ns20:foa_cit	rdf:type	ns2:IndicatorToGroupMembership ;
	rdfs:label	"discontinued" ;
	ns6:member-of	ns14:discontinued ;
	ns6:order	"19" .
ns20:foa_ent	rdf:type	ns2:IndicatorToGroupMembership ;
	rdfs:label	"discontinued" ;
	ns6:member-of	ns14:discontinued ;
	ns6:order	"20" .
ns20:i_cisk_sfjob	rdf:type	ns2:IndicatorToGroupMembership ;
	rdfs:label	"discontinued" ;
	ns6:member-of	ns14:discontinued ;
	ns6:order	"12" .
ns20:i_csk_ge_me	rdf:type	ns2:IndicatorToGroupMembership ;
	rdfs:label	"discontinued" ;
	ns6:member-of	ns14:discontinued ;
	ns6:order	"10" .
ns20:i_cweb	rdf:type	ns2:IndicatorToGroupMembership ;
	rdfs:label	"discontinued" ;
	ns6:member-of	ns14:discontinued ;
	ns6:order	"9" .
ns20:i_igovrt	rdf:type	ns2:IndicatorToGroupMembership ;
	rdfs:label	"discontinued" ;
	ns6:member-of	ns14:discontinued ;
	ns6:order	"24" .
ns20:i_isk_ge_me	rdf:type	ns2:IndicatorToGroupMembership ;
	rdfs:label	"discontinued" ;
	ns6:member-of	ns14:discontinued ;
	ns6:order	"11" .
ns20:i_iugov	rdf:type	ns2:IndicatorToGroupMembership ;
	rdfs:label	"discontinued" ;
	ns6:member-of	ns14:discontinued ;
	ns6:order	"23" .
ns20:ict_specialists	rdf:type	ns2:IndicatorToGroupMembership ;
	rdfs:label	"discontinued" ;
	ns6:member-of	ns14:discontinued ;
	ns6:order	"15" .
ns20:mbb_3gcov	rdf:type	ns2:IndicatorToGroupMembership ;
	rdfs:label	"discontinued" ;
	ns6:member-of	ns14:discontinued ;
	ns6:order	"17" .
ns20:mob_arpm	rdf:type	ns2:IndicatorToGroupMembership ;
	rdfs:label	"discontinued" ;
	ns6:member-of	ns14:discontinued ;
	ns6:order	"18" .
ns20:transparent_egov	rdf:type	ns2:IndicatorToGroupMembership ;
	rdfs:label	"discontinued" ;
	ns6:member-of	ns14:discontinued ;
	ns6:order	"22" .
ns20:user_centric_egov	rdf:type	ns2:IndicatorToGroupMembership ;
	rdfs:label	"discontinued" ;
	ns6:member-of	ns14:discontinued ;
	ns6:order	"21" .
ns7:e_ads	rdf:type	ns2:IndicatorToGroupMembership ;
	rdfs:label	"ebusiness" ;
	ns6:member-of	ns14:ebusiness ;
	ns6:order	"14" .
ns7:e_bd	rdf:type	ns2:IndicatorToGroupMembership ;
	rdfs:label	"ebusiness" ;
	ns6:member-of	ns14:ebusiness ;
	ns6:order	"30" .
ns7:e_cc	rdf:type	ns2:IndicatorToGroupMembership ;
	rdfs:label	"ebusiness" ;
	ns6:member-of	ns14:ebusiness ;
	ns6:order	"27" .
ns7:e_cc_ge_me	rdf:type	ns2:IndicatorToGroupMembership ;
	rdfs:label	"ebusiness" ;
	ns6:member-of	ns14:ebusiness ;
	ns6:order	"28" .
ns7:e_cc_pcpu	rdf:type	ns2:IndicatorToGroupMembership ;
	rdfs:label	"ebusiness" ;
	ns6:member-of	ns14:ebusiness ;
	ns6:order	"29" .
ns7:e_crman	rdf:type	ns2:IndicatorToGroupMembership ;
	rdfs:label	"ebusiness" ;
	ns6:member-of	ns14:ebusiness ;
	ns6:order	"3" .
ns7:e_di_hivhi	rdf:type	ns2:IndicatorToGroupMembership ;
	rdfs:label	"ebusiness" ;
	ns6:member-of	ns14:ebusiness ;
	ns6:order	"16" .
ns7:e_di_vlo	rdf:type	ns2:IndicatorToGroupMembership ;
	rdfs:label	"ebusiness" ;
	ns6:member-of	ns14:ebusiness ;
	ns6:order	"17" .
ns7:e_empmd_gt20	rdf:type	ns2:IndicatorToGroupMembership ;
	rdfs:label	"ebusiness" ;
	ns6:member-of	ns14:ebusiness ;
	ns6:order	"12" .
ns7:e_erp1	rdf:type	ns2:IndicatorToGroupMembership ;
	rdfs:label	"ebusiness" ;
	ns6:member-of	ns14:ebusiness ;
	ns6:order	"2" .
ns7:e_invsnd	rdf:type	ns2:IndicatorToGroupMembership ;
	rdfs:label	"ebusiness" ;
	ns6:member-of	ns14:ebusiness ;
	ns6:order	"6" .
ns7:e_pmd_app	rdf:type	ns2:IndicatorToGroupMembership ;
	rdfs:label	"ebusiness" ;
	ns6:member-of	ns14:ebusiness ;
	ns6:order	"13" .
ns7:e_ra	rdf:type	ns2:IndicatorToGroupMembership ;
	rdfs:label	"ebusiness" ;
	ns6:member-of	ns14:ebusiness ;
	ns6:order	"11" .
ns7:e_rfac	rdf:type	ns2:IndicatorToGroupMembership ;
	rdfs:label	"ebusiness" ;
	ns6:member-of	ns14:ebusiness ;
	ns6:order	"23" .
ns7:e_rfid	rdf:type	ns2:IndicatorToGroupMembership ;
	rdfs:label	"ebusiness" ;
	ns6:member-of	ns14:ebusiness ;
	ns6:order	"22" .
ns7:e_rfpsas	rdf:type	ns2:IndicatorToGroupMembership ;
	rdfs:label	"ebusiness" ;
	ns6:member-of	ns14:ebusiness ;
	ns6:order	"24" .
ns7:e_sisc	rdf:type	ns2:IndicatorToGroupMembership ;
	rdfs:label	"ebusiness" ;
	ns6:member-of	ns14:ebusiness ;
	ns6:order	"4" .
ns7:e_sm_any	rdf:type	ns2:IndicatorToGroupMembership ;
	rdfs:label	"ebusiness" ;
	ns6:member-of	ns14:ebusiness ;
	ns6:order	"25" .
ns7:e_sm_ge2	rdf:type	ns2:IndicatorToGroupMembership ;
	rdfs:label	"ebusiness" ;
	ns6:member-of	ns14:ebusiness ;
	ns6:order	"26" .
ns7:e_web	rdf:type	ns2:IndicatorToGroupMembership ;
	rdfs:label	"ebusiness" ;
	ns6:member-of	ns14:ebusiness ;
	ns6:order	"9" .
ns7:e_webf2	rdf:type	ns2:IndicatorToGroupMembership ;
	rdfs:label	"ebusiness" ;
	ns6:member-of	ns14:ebusiness ;
	ns6:order	"10" .
ns7:edigint2015	rdf:type	ns2:IndicatorToGroupMembership ;
	rdfs:label	"ebusiness" ;
	ns6:member-of	ns14:ebusiness ;
	ns6:order	"15" .
ns7:p_empmd	rdf:type	ns2:IndicatorToGroupMembership ;
	rdfs:label	"ebusiness" ;
	ns6:member-of	ns14:ebusiness ;
	ns6:order	"13" .
@prefix ns21:	<http://semantic.digital-agenda-data.eu/codelist/indicator-group/ecommerce/> .
ns21:e_aeseu	rdf:type	ns2:IndicatorToGroupMembership ;
	rdfs:label	"ecommerce" ;
	ns6:member-of	ns14:ecommerce ;
	ns6:order	"12" .
ns21:e_aws	rdf:type	ns2:IndicatorToGroupMembership ;
	rdfs:label	"ecommerce" ;
	ns6:member-of	ns14:ecommerce .
ns21:e_aws_cmp	rdf:type	ns2:IndicatorToGroupMembership ;
	rdfs:label	"ecommerce" ;
	ns6:member-of	ns14:ecommerce .
ns21:e_aws_cown	rdf:type	ns2:IndicatorToGroupMembership ;
	rdfs:label	"ecommerce" ;
	ns6:member-of	ns14:ecommerce .
ns21:e_aws_gt1_b2c_gt10ws	rdf:type	ns2:IndicatorToGroupMembership ;
	rdfs:label	"ecommerce" ;
	ns6:member-of	ns14:ecommerce ;
	ns6:order	"13" .
ns21:e_awsval_cmp	rdf:type	ns2:IndicatorToGroupMembership ;
	rdfs:label	"ecommerce" ;
	ns6:member-of	ns14:ecommerce .
ns21:e_awsval_cown	rdf:type	ns2:IndicatorToGroupMembership ;
	rdfs:label	"ecommerce" ;
	ns6:member-of	ns14:ecommerce .
ns21:e_esell	rdf:type	ns2:IndicatorToGroupMembership ;
	rdfs:label	"ecommerce" ;
	ns6:member-of	ns14:ecommerce ;
	ns6:order	"10" .
ns21:e_eturn	rdf:type	ns2:IndicatorToGroupMembership ;
	rdfs:label	"ecommerce" ;
	ns6:member-of	ns14:ecommerce ;
	ns6:order	"11" .
ns21:e_wsel25	rdf:type	ns2:IndicatorToGroupMembership ;
	rdfs:label	"ecommerce" ;
	ns6:member-of	ns14:ecommerce .
ns21:e_wsel50	rdf:type	ns2:IndicatorToGroupMembership ;
	rdfs:label	"ecommerce" ;
	ns6:member-of	ns14:ecommerce .
ns21:i_barr1x	rdf:type	ns2:IndicatorToGroupMembership ;
	rdfs:label	"ecommerce" ;
	ns6:member-of	ns14:ecommerce ;
	ns6:order	"9" .
ns21:i_bfeu	rdf:type	ns2:IndicatorToGroupMembership ;
	rdfs:label	"ecommerce" ;
	ns6:member-of	ns14:ecommerce ;
	ns6:order	"3" .
ns21:i_bgood	rdf:type	ns2:IndicatorToGroupMembership ;
	rdfs:label	"ecommerce" ;
	ns6:member-of	ns14:ecommerce ;
	ns6:order	"7" .
ns21:i_bgoodo	rdf:type	ns2:IndicatorToGroupMembership ;
	rdfs:label	"ecommerce" ;
	ns6:member-of	ns14:ecommerce ;
	ns6:order	"6" .
ns21:i_blt12	rdf:type	ns2:IndicatorToGroupMembership ;
	rdfs:label	"ecommerce" ;
	ns6:member-of	ns14:ecommerce ;
	ns6:order	"1" .
ns21:i_bpgood	rdf:type	ns2:IndicatorToGroupMembership ;
	rdfs:label	"ecommerce" ;
	ns6:member-of	ns14:ecommerce ;
	ns6:order	"4" .
ns21:i_bserv	rdf:type	ns2:IndicatorToGroupMembership ;
	rdfs:label	"ecommerce" ;
	ns6:member-of	ns14:ecommerce ;
	ns6:order	"5" .
ns21:i_iusell	rdf:type	ns2:IndicatorToGroupMembership ;
	rdfs:label	"ecommerce" ;
	ns6:member-of	ns14:ecommerce ;
	ns6:order	"8" .
@prefix ns22:	<http://semantic.digital-agenda-data.eu/codelist/indicator-group/egovernment/> .
ns22:e_gov_1_ucg	rdf:type	ns2:IndicatorToGroupMembership ;
	rdfs:label	"egovernment" ;
	ns6:member-of	ns14:egovernment ;
	ns6:order	"1111" .
ns22:e_gov_1a_ucg_oa	rdf:type	ns2:IndicatorToGroupMembership ;
	rdfs:label	"egovernment" ;
	ns6:member-of	ns14:egovernment ;
	ns6:order	"11111" .
ns22:e_gov_1b_ucg_us	rdf:type	ns2:IndicatorToGroupMembership ;
	rdfs:label	"egovernment" ;
	ns6:member-of	ns14:egovernment ;
	ns6:order	"11113" .
ns22:e_gov_1c_ucg_mf	rdf:type	ns2:IndicatorToGroupMembership ;
	rdfs:label	"egovernment" ;
	ns6:member-of	ns14:egovernment ;
	ns6:order	"11114" .
ns22:e_gov_1d_ucg_eu	rdf:type	ns2:IndicatorToGroupMembership ;
	rdfs:label	"egovernment" ;
	ns6:member-of	ns14:egovernment ;
	ns6:order	"11115" .
ns22:e_gov_1e_ucg_su	rdf:type	ns2:IndicatorToGroupMembership ;
	rdfs:label	"egovernment" ;
	ns6:member-of	ns14:egovernment ;
	ns6:order	"11116" .
ns22:e_gov_2_tg	rdf:type	ns2:IndicatorToGroupMembership ;
	rdfs:label	"egovernment" ;
	ns6:member-of	ns14:egovernment ;
	ns6:order	"1112" .
ns22:e_gov_2a_tg_sd	rdf:type	ns2:IndicatorToGroupMembership ;
	rdfs:label	"egovernment" ;
	ns6:member-of	ns14:egovernment ;
	ns6:order	"11121" .
ns22:e_gov_2b_tg_po	rdf:type	ns2:IndicatorToGroupMembership ;
	rdfs:label	"egovernment" ;
	ns6:member-of	ns14:egovernment ;
	ns6:order	"11122" .
ns22:e_gov_2c_tg_pd	rdf:type	ns2:IndicatorToGroupMembership ;
	rdfs:label	"egovernment" ;
	ns6:member-of	ns14:egovernment ;
	ns6:order	"11123" .
ns22:e_gov_3_cm	rdf:type	ns2:IndicatorToGroupMembership ;
	rdfs:label	"egovernment" ;
	ns6:member-of	ns14:egovernment ;
	ns6:order	"1113" .
ns22:e_gov_3a_cm_oa	rdf:type	ns2:IndicatorToGroupMembership ;
	rdfs:label	"egovernment" ;
	ns6:member-of	ns14:egovernment ;
	ns6:order	"11131" .
ns22:e_gov_3b_cm_us	rdf:type	ns2:IndicatorToGroupMembership ;
	rdfs:label	"egovernment" ;
	ns6:member-of	ns14:egovernment ;
	ns6:order	"11133" .
ns22:e_gov_3c_cm_eidcb	rdf:type	ns2:IndicatorToGroupMembership ;
	rdfs:label	"egovernment" ;
	ns6:member-of	ns14:egovernment ;
	ns6:order	"11135" .
ns22:e_gov_3d_cm_edoccb	rdf:type	ns2:IndicatorToGroupMembership ;
	rdfs:label	"egovernment" ;
	ns6:member-of	ns14:egovernment ;
	ns6:order	"11136" .
ns22:e_gov_3e_cm_eu	rdf:type	ns2:IndicatorToGroupMembership ;
	rdfs:label	"egovernment" ;
	ns6:member-of	ns14:egovernment ;
	ns6:order	"11137" .
ns22:e_gov_3f_cm_su	rdf:type	ns2:IndicatorToGroupMembership ;
	rdfs:label	"egovernment" ;
	ns6:member-of	ns14:egovernment ;
	ns6:order	"11138" .
ns22:e_gov_4_bm	rdf:type	ns2:IndicatorToGroupMembership ;
	rdfs:label	"egovernment" ;
	ns6:member-of	ns14:egovernment ;
	ns6:order	"1114" .
ns22:e_gov_4a_bm_oa	rdf:type	ns2:IndicatorToGroupMembership ;
	rdfs:label	"egovernment" ;
	ns6:member-of	ns14:egovernment ;
	ns6:order	"11141" .
ns22:e_gov_4b_bm_us	rdf:type	ns2:IndicatorToGroupMembership ;
	rdfs:label	"egovernment" ;
	ns6:member-of	ns14:egovernment ;
	ns6:order	"11143" .
ns22:e_gov_4c_bm_eidcb	rdf:type	ns2:IndicatorToGroupMembership ;
	rdfs:label	"egovernment" ;
	ns6:member-of	ns14:egovernment ;
	ns6:order	"11145" .
ns22:e_gov_4d_bm_edoccb	rdf:type	ns2:IndicatorToGroupMembership ;
	rdfs:label	"egovernment" ;
	ns6:member-of	ns14:egovernment ;
	ns6:order	"11146" .
ns22:e_gov_4e_bm_eu	rdf:type	ns2:IndicatorToGroupMembership ;
	rdfs:label	"egovernment" ;
	ns6:member-of	ns14:egovernment ;
	ns6:order	"11147" .
ns22:e_gov_4f_bm_su	rdf:type	ns2:IndicatorToGroupMembership ;
	rdfs:label	"egovernment" ;
	ns6:member-of	ns14:egovernment ;
	ns6:order	"11148" .
ns22:e_gov_5_ke	rdf:type	ns2:IndicatorToGroupMembership ;
	rdfs:label	"egovernment" ;
	ns6:member-of	ns14:egovernment ;
	ns6:order	"1115" .
ns22:e_gov_5a_ke_eid	rdf:type	ns2:IndicatorToGroupMembership ;
	rdfs:label	"egovernment" ;
	ns6:member-of	ns14:egovernment ;
	ns6:order	"11151" .
ns22:e_gov_5b_ke_edoc	rdf:type	ns2:IndicatorToGroupMembership ;
	rdfs:label	"egovernment" ;
	ns6:member-of	ns14:egovernment ;
	ns6:order	"11152" .
ns22:e_gov_5c_ke_as	rdf:type	ns2:IndicatorToGroupMembership ;
	rdfs:label	"egovernment" ;
	ns6:member-of	ns14:egovernment ;
	ns6:order	"11153" .
ns22:e_gov_5d_ke_dp	rdf:type	ns2:IndicatorToGroupMembership ;
	rdfs:label	"egovernment" ;
	ns6:member-of	ns14:egovernment ;
	ns6:order	"11154" .
ns22:e_gov_5e_ke_esafe	rdf:type	ns2:IndicatorToGroupMembership ;
	rdfs:label	"egovernment" ;
	ns6:member-of	ns14:egovernment ;
	ns6:order	"11155" .
ns22:e_gov_5f_ke_sso	rdf:type	ns2:IndicatorToGroupMembership ;
	rdfs:label	"egovernment" ;
	ns6:member-of	ns14:egovernment ;
	ns6:order	"11156" .
ns22:e_gov_ke	rdf:type	ns2:IndicatorToGroupMembership ;
	rdfs:label	"egovernment" ;
	ns6:member-of	ns14:egovernment ;
	ns6:order	"8" .
ns22:e_gov_opa	rdf:type	ns2:IndicatorToGroupMembership ;
	rdfs:label	"egovernment" ;
	ns6:member-of	ns14:egovernment ;
	ns6:order	"9" .
ns22:e_gov_osc	rdf:type	ns2:IndicatorToGroupMembership ;
	rdfs:label	"egovernment" ;
	ns6:member-of	ns14:egovernment ;
	ns6:order	"7" .
ns22:e_gov_pff	rdf:type	ns2:IndicatorToGroupMembership ;
	rdfs:label	"egovernment" ;
	ns6:member-of	ns14:egovernment ;
	ns6:order	"6" .
ns22:epsi_score	rdf:type	ns2:IndicatorToGroupMembership ;
	rdfs:label	"egovernment" ;
	ns6:member-of	ns14:egovernment ;
	ns6:order	"5" .
ns22:i_igov12rt	rdf:type	ns2:IndicatorToGroupMembership ;
	rdfs:label	"egovernment" ;
	ns6:member-of	ns14:egovernment ;
	ns6:order	"1" .
ns22:i_iugov12	rdf:type	ns2:IndicatorToGroupMembership ;
	rdfs:label	"egovernment" ;
	ns6:member-of	ns14:egovernment ;
	ns6:order	"6" .
@prefix ns23:	<http://semantic.digital-agenda-data.eu/codelist/indicator-group/ehealth/> .
ns23:hie_use_ex_admin	rdf:type	ns2:IndicatorToGroupMembership ;
	rdfs:label	"ehealth" ;
	ns6:member-of	ns14:ehealth ;
	ns6:order	"4" .
ns23:hie_use_pharm	rdf:type	ns2:IndicatorToGroupMembership ;
	rdfs:label	"ehealth" ;
	ns6:member-of	ns14:ehealth ;
	ns6:order	"3" .
ns23:i_ihif	rdf:type	ns2:IndicatorToGroupMembership ;
	rdfs:label	"ehealth" ;
	ns6:member-of	ns14:ehealth ;
	ns6:order	"1" .
ns23:i_iumapp	rdf:type	ns2:IndicatorToGroupMembership ;
	rdfs:label	"ehealth" ;
	ns6:member-of	ns14:ehealth ;
	ns6:order	"2" .
@prefix ns24:	<http://semantic.digital-agenda-data.eu/codelist/indicator-group/ict-edu/> .
ns24:eun_computers	rdf:type	ns2:IndicatorToGroupMembership ;
	rdfs:label	"ict-edu" ;
	ns6:member-of	ns14:ict-edu ;
	ns6:order	"1" .
ns24:eun_web	rdf:type	ns2:IndicatorToGroupMembership ;
	rdfs:label	"ict-edu" ;
	ns6:member-of	ns14:ict-edu ;
	ns6:order	"2" .
@prefix ns25:	<http://semantic.digital-agenda-data.eu/codelist/indicator-group/ict-sector/> .
ns25:bs_rd_expen_ict	rdf:type	ns2:IndicatorToGroupMembership ;
	rdfs:label	"ict-sector" ;
	ns6:member-of	ns14:ict-sector ;
	ns6:order	"6" .
ns25:employment_ict	rdf:type	ns2:IndicatorToGroupMembership ;
	rdfs:label	"ict-sector" ;
	ns6:member-of	ns14:ict-sector ;
	ns6:order	"4" .
ns25:ict_exp	rdf:type	ns2:IndicatorToGroupMembership ;
	rdfs:label	"ict-sector" ;
	ns6:member-of	ns14:ict-sector ;
	ns6:order	"1" .
ns25:ict_hgc	rdf:type	ns2:IndicatorToGroupMembership ;
	rdfs:label	"ict-sector" ;
	ns6:member-of	ns14:ict-sector ;
	ns6:order	"3" .
ns25:ict_imp	rdf:type	ns2:IndicatorToGroupMembership ;
	rdfs:label	"ict-sector" ;
	ns6:member-of	ns14:ict-sector ;
	ns6:order	"2" .
ns25:labour_prod_ict	rdf:type	ns2:IndicatorToGroupMembership ;
	rdfs:label	"ict-sector" ;
	ns6:member-of	ns14:ict-sector ;
	ns6:order	"7" .
ns25:val_add_ict	rdf:type	ns2:IndicatorToGroupMembership ;
	rdfs:label	"ict-sector" ;
	ns6:member-of	ns14:ict-sector ;
	ns6:order	"5" .
@prefix ns26:	<http://semantic.digital-agenda-data.eu/codelist/indicator-group/ict-skills/> .
ns26:i_dsk_bab	rdf:type	ns2:IndicatorToGroupMembership ;
	rdfs:label	"ict-skills" ;
	ns6:member-of	ns14:ict-skills ;
	ns6:order	"1112" .
ns26:i_dsk_c_bab	rdf:type	ns2:IndicatorToGroupMembership ;
	rdfs:label	"ict-skills" ;
	ns6:member-of	ns14:ict-skills ;
	ns6:order	"1115" .
ns26:i_dsk_i_bab	rdf:type	ns2:IndicatorToGroupMembership ;
	rdfs:label	"ict-skills" ;
	ns6:member-of	ns14:ict-skills ;
	ns6:order	"1118" .
ns26:i_dsk_ps_bab	rdf:type	ns2:IndicatorToGroupMembership ;
	rdfs:label	"ict-skills" ;
	ns6:member-of	ns14:ict-skills ;
	ns6:order	"1122" .
ns26:i_dsk_s_bab	rdf:type	ns2:IndicatorToGroupMembership ;
	rdfs:label	"ict-skills" ;
	ns6:member-of	ns14:ict-skills ;
	ns6:order	"1125" .
ns26:st_grad	rdf:type	ns2:IndicatorToGroupMembership ;
	rdfs:label	"ict-skills" ;
	ns6:member-of	ns14:ict-skills ;
	ns6:order	"30" .
@prefix ns27:	<http://semantic.digital-agenda-data.eu/codelist/indicator-group/ict-specialist/> .
ns27:e_it_mext	rdf:type	ns2:IndicatorToGroupMembership ;
	rdfs:label	"ict-specialist" ;
	ns6:member-of	ns14:ict-specialist ;
	ns6:order	"4" .
ns27:e_itsp2	rdf:type	ns2:IndicatorToGroupMembership ;
	rdfs:label	"ict-specialist" ;
	ns6:member-of	ns14:ict-specialist ;
	ns6:order	"1" .
ns27:e_itspvac2	rdf:type	ns2:IndicatorToGroupMembership ;
	rdfs:label	"ict-specialist" ;
	ns6:member-of	ns14:ict-specialist ;
	ns6:order	"2" .
ns27:e_itt2	rdf:type	ns2:IndicatorToGroupMembership ;
	rdfs:label	"ict-specialist" ;
	ns6:member-of	ns14:ict-specialist ;
	ns6:order	"5" .
ns27:ict_spec3_broad	rdf:type	ns2:IndicatorToGroupMembership ;
	rdfs:label	"ict-specialist" ;
	ns6:member-of	ns14:ict-specialist ;
	ns6:order	"3" .
@prefix ns28:	<http://semantic.digital-agenda-data.eu/codelist/indicator-group/internet-services/> .
ns28:i_cc	rdf:type	ns2:IndicatorToGroupMembership ;
	rdfs:label	"internet-services" ;
	ns6:member-of	ns14:internet-services ;
	ns6:order	"14" .
ns28:i_iubk	rdf:type	ns2:IndicatorToGroupMembership ;
	rdfs:label	"internet-services" ;
	ns6:member-of	ns14:internet-services ;
	ns6:order	"4" .
ns28:i_iueduif	rdf:type	ns2:IndicatorToGroupMembership ;
	rdfs:label	"internet-services" ;
	ns6:member-of	ns14:internet-services ;
	ns6:order	"10" .
ns28:i_iuif	rdf:type	ns2:IndicatorToGroupMembership ;
	rdfs:label	"internet-services" ;
	ns6:member-of	ns14:internet-services ;
	ns6:order	"1" .
ns28:i_iujob	rdf:type	ns2:IndicatorToGroupMembership ;
	rdfs:label	"internet-services" ;
	ns6:member-of	ns14:internet-services ;
	ns6:order	"8" .
ns28:i_iuolc	rdf:type	ns2:IndicatorToGroupMembership ;
	rdfs:label	"internet-services" ;
	ns6:member-of	ns14:internet-services ;
	ns6:order	"9" .
ns28:i_iuph1	rdf:type	ns2:IndicatorToGroupMembership ;
	rdfs:label	"internet-services" ;
	ns6:member-of	ns14:internet-services ;
	ns6:order	"5" .
ns28:i_iusnet	rdf:type	ns2:IndicatorToGroupMembership ;
	rdfs:label	"internet-services" ;
	ns6:member-of	ns14:internet-services ;
	ns6:order	"7" .
ns28:i_iuupl	rdf:type	ns2:IndicatorToGroupMembership ;
	rdfs:label	"internet-services" ;
	ns6:member-of	ns14:internet-services ;
	ns6:order	"6" .
ns28:i_iuvote	rdf:type	ns2:IndicatorToGroupMembership ;
	rdfs:label	"internet-services" ;
	ns6:member-of	ns14:internet-services ;
	ns6:order	"13" .
@prefix ns29:	<http://semantic.digital-agenda-data.eu/codelist/indicator-group/internet-usage/> .
ns29:aaaa_cov	rdf:type	ns2:IndicatorToGroupMembership ;
	rdfs:label	"internet-usage" ;
	ns6:member-of	ns14:internet-usage ;
	ns6:order	"9" .
ns29:h_iacc	rdf:type	ns2:IndicatorToGroupMembership ;
	rdfs:label	"internet-usage" ;
	ns6:member-of	ns14:internet-usage ;
	ns6:order	"1" .
ns29:i_iday	rdf:type	ns2:IndicatorToGroupMembership ;
	rdfs:label	"internet-usage" ;
	ns6:member-of	ns14:internet-usage ;
	ns6:order	"5" .
ns29:i_ilt12	rdf:type	ns2:IndicatorToGroupMembership ;
	rdfs:label	"internet-usage" ;
	ns6:member-of	ns14:internet-usage ;
	ns6:order	"3" .
ns29:i_iu3	rdf:type	ns2:IndicatorToGroupMembership ;
	rdfs:label	"internet-usage" ;
	ns6:member-of	ns14:internet-usage ;
	ns6:order	"2" .
ns29:i_iumc	rdf:type	ns2:IndicatorToGroupMembership ;
	rdfs:label	"internet-usage" ;
	ns6:member-of	ns14:internet-usage ;
	ns6:order	"6" .
ns29:i_iuse	rdf:type	ns2:IndicatorToGroupMembership ;
	rdfs:label	"internet-usage" ;
	ns6:member-of	ns14:internet-usage ;
	ns6:order	"4" .
ns29:i_iux	rdf:type	ns2:IndicatorToGroupMembership ;
	rdfs:label	"internet-usage" ;
	ns6:member-of	ns14:internet-usage ;
	ns6:order	"7" .
@prefix ns30:	<http://semantic.digital-agenda-data.eu/codelist/indicator-group/mobile/> .
ns30:e_pmd	rdf:type	ns2:IndicatorToGroupMembership ;
	rdfs:label	"mobile" ;
	ns6:member-of	ns14:mobile ;
	ns6:order	"12" .
ns30:i_iu3g	rdf:type	ns2:IndicatorToGroupMembership ;
	rdfs:label	"mobile" ;
	ns6:member-of	ns14:mobile ;
	ns6:order	"11" .
ns30:mbb_hspacov	rdf:type	ns2:IndicatorToGroupMembership ;
	rdfs:label	"mobile" ;
	ns6:member-of	ns14:mobile ;
	ns6:order	"6" .
ns30:mbb_ltecov	rdf:type	ns2:IndicatorToGroupMembership ;
	rdfs:label	"mobile" ;
	ns6:member-of	ns14:mobile ;
	ns6:order	"4" .
ns30:mbb_penet	rdf:type	ns2:IndicatorToGroupMembership ;
	rdfs:label	"mobile" ;
	ns6:member-of	ns14:mobile ;
	ns6:order	"10" .
ns30:mbb_rhspacov	rdf:type	ns2:IndicatorToGroupMembership ;
	rdfs:label	"mobile" ;
	ns6:member-of	ns14:mobile ;
	ns6:order	"7" .
ns30:mbb_rltecov	rdf:type	ns2:IndicatorToGroupMembership ;
	rdfs:label	"mobile" ;
	ns6:member-of	ns14:mobile ;
	ns6:order	"5" .
ns30:mob_arpu	rdf:type	ns2:IndicatorToGroupMembership ;
	rdfs:label	"mobile" ;
	ns6:member-of	ns14:mobile ;
	ns6:order	"14" .
ns30:mob_ms	rdf:type	ns2:IndicatorToGroupMembership ;
	rdfs:label	"mobile" ;
	ns6:member-of	ns14:mobile ;
	ns6:order	"13" .
ns30:mob_mtr	rdf:type	ns2:IndicatorToGroupMembership ;
	rdfs:label	"mobile" ;
	ns6:member-of	ns14:mobile ;
	ns6:order	"17" .
ns30:mob_penet	rdf:type	ns2:IndicatorToGroupMembership ;
	rdfs:label	"mobile" ;
	ns6:member-of	ns14:mobile ;
	ns6:order	"9" .
ns30:mob_roam	rdf:type	ns2:IndicatorToGroupMembership ;
	rdfs:label	"mobile" ;
	ns6:member-of	ns14:mobile ;
	ns6:order	"15" .
ns30:mob_subs	rdf:type	ns2:IndicatorToGroupMembership ;
	rdfs:label	"mobile" ;
	ns6:member-of	ns14:mobile ;
	ns6:order	"8" .
ns30:spectrum_wbb	rdf:type	ns2:IndicatorToGroupMembership ;
	rdfs:label	"mobile" ;
	ns6:member-of	ns14:mobile ;
	ns6:order	"16" .
@prefix ns31:	<http://semantic.digital-agenda-data.eu/codelist/indicator-group/research-and-development/> .
ns31:avg_ttg	rdf:type	ns2:IndicatorToGroupMembership ;
	rdfs:label	"research-and-development" ;
	ns6:member-of	ns14:research-and-development ;
	ns6:order	"21" .
ns31:fp7_ict_artic	rdf:type	ns2:IndicatorToGroupMembership ;
	rdfs:label	"research-and-development" ;
	ns6:member-of	ns14:research-and-development ;
	ns6:order	"32" .
ns31:fp7_ict_pat	rdf:type	ns2:IndicatorToGroupMembership ;
	rdfs:label	"research-and-development" ;
	ns6:member-of	ns14:research-and-development ;
	ns6:order	"30" .
ns31:fp7_ict_pub	rdf:type	ns2:IndicatorToGroupMembership ;
	rdfs:label	"research-and-development" ;
	ns6:member-of	ns14:research-and-development ;
	ns6:order	"31" .
ns31:fp7ict_afxp	rdf:type	ns2:IndicatorToGroupMembership ;
	rdfs:label	"research-and-development" ;
	ns6:member-of	ns14:research-and-development ;
	ns6:order	"17" .
ns31:fp7ict_cofin	rdf:type	ns2:IndicatorToGroupMembership ;
	rdfs:label	"research-and-development" ;
	ns6:member-of	ns14:research-and-development ;
	ns6:order	"15" .
ns31:fp7ict_ec_funding	rdf:type	ns2:IndicatorToGroupMembership ;
	rdfs:label	"research-and-development" ;
	ns6:member-of	ns14:research-and-development ;
	ns6:order	"13" .
ns31:fp7ict_ec_funding_prc	rdf:type	ns2:IndicatorToGroupMembership ;
	rdfs:label	"research-and-development" ;
	ns6:member-of	ns14:research-and-development ;
	ns6:order	"41" .
ns31:fp7ict_ec_funding_smes	rdf:type	ns2:IndicatorToGroupMembership ;
	rdfs:label	"research-and-development" ;
	ns6:member-of	ns14:research-and-development ;
	ns6:order	"42" .
ns31:fp7ict_newentry	rdf:type	ns2:IndicatorToGroupMembership ;
	rdfs:label	"research-and-development" ;
	ns6:member-of	ns14:research-and-development ;
	ns6:order	"18" .
ns31:fp7ict_organisations	rdf:type	ns2:IndicatorToGroupMembership ;
	rdfs:label	"research-and-development" ;
	ns6:member-of	ns14:research-and-development ;
	ns6:order	"19" .
ns31:fp7ict_particip	rdf:type	ns2:IndicatorToGroupMembership ;
	rdfs:label	"research-and-development" ;
	ns6:member-of	ns14:research-and-development ;
	ns6:order	"16" .
ns31:fp7ict_particip_prc	rdf:type	ns2:IndicatorToGroupMembership ;
	rdfs:label	"research-and-development" ;
	ns6:member-of	ns14:research-and-development ;
	ns6:order	"43" .
ns31:fp7ict_particip_smes	rdf:type	ns2:IndicatorToGroupMembership ;
	rdfs:label	"research-and-development" ;
	ns6:member-of	ns14:research-and-development ;
	ns6:order	"44" .
ns31:fp7ict_totcost	rdf:type	ns2:IndicatorToGroupMembership ;
	rdfs:label	"research-and-development" ;
	ns6:member-of	ns14:research-and-development ;
	ns6:order	"14" .
ns31:gbaord	rdf:type	ns2:IndicatorToGroupMembership ;
	rdfs:label	"research-and-development" ;
	ns6:member-of	ns14:research-and-development ;
	ns6:order	"1" .
ns31:gbaord_ict	rdf:type	ns2:IndicatorToGroupMembership ;
	rdfs:label	"research-and-development" ;
	ns6:member-of	ns14:research-and-development ;
	ns6:order	"2" .
ns31:h2020_cofin	rdf:type	ns2:IndicatorToGroupMembership ;
	rdfs:label	"research-and-development" ;
	ns6:member-of	ns14:research-and-development ;
	ns6:order	"5" .
ns31:h2020_ec_funding	rdf:type	ns2:IndicatorToGroupMembership ;
	rdfs:label	"research-and-development" ;
	ns6:member-of	ns14:research-and-development ;
	ns6:order	"3" .
ns31:h2020_newentry	rdf:type	ns2:IndicatorToGroupMembership ;
	rdfs:label	"research-and-development" ;
	ns6:member-of	ns14:research-and-development ;
	ns6:order	"9" .
ns31:h2020_organisations	rdf:type	ns2:IndicatorToGroupMembership ;
	rdfs:label	"research-and-development" ;
	ns6:member-of	ns14:research-and-development ;
	ns6:order	"8" .
ns31:h2020_particip	rdf:type	ns2:IndicatorToGroupMembership ;
	rdfs:label	"research-and-development" ;
	ns6:member-of	ns14:research-and-development ;
	ns6:order	"6" .
ns31:h2020_totcost	rdf:type	ns2:IndicatorToGroupMembership ;
	rdfs:label	"research-and-development" ;
	ns6:member-of	ns14:research-and-development ;
	ns6:order	"4" .
ns31:h2020ict_afxp	rdf:type	ns2:IndicatorToGroupMembership ;
	rdfs:label	"research-and-development" ;
	ns6:member-of	ns14:research-and-development ;
	ns6:order	"7" .
ns31:ict_commit_in_trp	rdf:type	ns2:IndicatorToGroupMembership ;
	rdfs:label	"research-and-development" ;
	ns6:member-of	ns14:research-and-development ;
	ns6:order	"20" .
@prefix ns32:	<http://semantic.digital-agenda-data.eu/codelist/indicator-group/research_einfra/> .
ns32:c1_bandwidth	rdf:type	ns2:IndicatorToGroupMembership ;
	rdfs:label	"research_einfra" ;
	ns6:member-of	ns14:research_einfra ;
	ns6:order	"3" .
ns32:c1_compcyclesegi	rdf:type	ns2:IndicatorToGroupMembership ;
	rdfs:label	"research_einfra" ;
	ns6:member-of	ns14:research_einfra ;
	ns6:order	"1" .
ns32:c1_compcyclesprace	rdf:type	ns2:IndicatorToGroupMembership ;
	rdfs:label	"research_einfra" ;
	ns6:member-of	ns14:research_einfra ;
	ns6:order	"2" .
ns32:c1_datatraffic	rdf:type	ns2:IndicatorToGroupMembership ;
	rdfs:label	"research_einfra" ;
	ns6:member-of	ns14:research_einfra ;
	ns6:order	"4" .
@prefix ns33:	<http://semantic.digital-agenda-data.eu/codelist/indicator-group/security-privacy/> .
ns33:e_ads_loc	rdf:type	ns2:IndicatorToGroupMembership ;
	rdfs:label	"security-privacy" ;
	ns6:member-of	ns14:security-privacy ;
	ns6:order	"9" .
ns33:e_ads_trk	rdf:type	ns2:IndicatorToGroupMembership ;
	rdfs:label	"security-privacy" ;
	ns6:member-of	ns14:security-privacy ;
	ns6:order	"10" .
ns33:e_secpol1	rdf:type	ns2:IndicatorToGroupMembership ;
	rdfs:label	"security-privacy" ;
	ns6:member-of	ns14:security-privacy ;
	ns6:order	"11" .
ns33:i_atsw	rdf:type	ns2:IndicatorToGroupMembership ;
	rdfs:label	"security-privacy" ;
	ns6:member-of	ns14:security-privacy ;
	ns6:order	"7" .
ns33:i_cook	rdf:type	ns2:IndicatorToGroupMembership ;
	rdfs:label	"security-privacy" ;
	ns6:member-of	ns14:security-privacy ;
	ns6:order	"6" .
ns33:i_piacadv	rdf:type	ns2:IndicatorToGroupMembership ;
	rdfs:label	"security-privacy" ;
	ns6:member-of	ns14:security-privacy ;
	ns6:order	"8" .
ns33:i_sbgood	rdf:type	ns2:IndicatorToGroupMembership ;
	rdfs:label	"security-privacy" ;
	ns6:member-of	ns14:security-privacy ;
	ns6:order	"5" .
ns33:i_secfl	rdf:type	ns2:IndicatorToGroupMembership ;
	rdfs:label	"security-privacy" ;
	ns6:member-of	ns14:security-privacy ;
	ns6:order	"2" .
ns33:i_secpif1	rdf:type	ns2:IndicatorToGroupMembership ;
	rdfs:label	"security-privacy" ;
	ns6:member-of	ns14:security-privacy ;
	ns6:order	"3" .
ns33:i_secvir1	rdf:type	ns2:IndicatorToGroupMembership ;
	rdfs:label	"security-privacy" ;
	ns6:member-of	ns14:security-privacy ;
	ns6:order	"4" .
@prefix ns34:	<http://semantic.digital-agenda-data.eu/codelist/indicator-group/telecom/> .
ns34:tel_ftr	rdf:type	ns2:IndicatorToGroupMembership ;
	rdfs:label	"telecom" ;
	ns6:member-of	ns14:telecom ;
	ns6:order	"3" .
ns34:tel_inv	rdf:type	ns2:IndicatorToGroupMembership ;
	rdfs:label	"telecom" ;
	ns6:member-of	ns14:telecom ;
	ns6:order	"2" .
ns34:tel_llu	rdf:type	ns2:IndicatorToGroupMembership ;
	rdfs:label	"telecom" ;
	ns6:member-of	ns14:telecom ;
	ns6:order	"4" .
ns34:tel_rev	rdf:type	ns2:IndicatorToGroupMembership ;
	rdfs:label	"telecom" ;
	ns6:member-of	ns14:telecom ;
	ns6:order	"1" .
@prefix ns35:	<http://semantic.digital-agenda-data.eu/codelist/indicator-group/wid/> .
ns35:wid_ius	rdf:type	ns2:IndicatorToGroupMembership ;
	rdfs:label	"wid" ;
	ns6:member-of	ns14:wid ;
	ns6:order	"10" .
ns35:wid_ius_abs	rdf:type	ns2:IndicatorToGroupMembership ;
	rdfs:label	"wid" ;
	ns6:member-of	ns14:wid ;
	ns6:order	"12" .
ns35:wid_ius_bs	rdf:type	ns2:IndicatorToGroupMembership ;
	rdfs:label	"wid" ;
	ns6:member-of	ns14:wid ;
	ns6:order	"11" .
ns35:wid_ius_ss	rdf:type	ns2:IndicatorToGroupMembership ;
	rdfs:label	"wid" ;
	ns6:member-of	ns14:wid ;
	ns6:order	"13" .
ns35:wid_score	rdf:type	ns2:IndicatorToGroupMembership ;
	rdfs:label	"wid" ;
	ns6:member-of	ns14:wid ;
	ns6:order	"1" .
ns35:wid_sse	rdf:type	ns2:IndicatorToGroupMembership ;
	rdfs:label	"wid" ;
	ns6:member-of	ns14:wid ;
	ns6:order	"14" .
ns35:wid_sse_gpg	rdf:type	ns2:IndicatorToGroupMembership ;
	rdfs:label	"wid" ;
	ns6:member-of	ns14:wid ;
	ns6:order	"17" .
ns35:wid_sse_icts	rdf:type	ns2:IndicatorToGroupMembership ;
	rdfs:label	"wid" ;
	ns6:member-of	ns14:wid ;
	ns6:order	"16" .
ns35:wid_sse_stem	rdf:type	ns2:IndicatorToGroupMembership ;
	rdfs:label	"wid" ;
	ns6:member-of	ns14:wid ;
	ns6:order	"15" .
ns35:wid_ui	rdf:type	ns2:IndicatorToGroupMembership ;
	rdfs:label	"wid" ;
	ns6:member-of	ns14:wid ;
	ns6:order	"2" .
ns35:wid_ui_egov	rdf:type	ns2:IndicatorToGroupMembership ;
	rdfs:label	"wid" ;
	ns6:member-of	ns14:wid ;
	ns6:order	"9" .
ns35:wid_ui_ib	rdf:type	ns2:IndicatorToGroupMembership ;
	rdfs:label	"wid" ;
	ns6:member-of	ns14:wid ;
	ns6:order	"5" .
ns35:wid_ui_iu	rdf:type	ns2:IndicatorToGroupMembership ;
	rdfs:label	"wid" ;
	ns6:member-of	ns14:wid ;
	ns6:order	"3" .
ns35:wid_ui_nui	rdf:type	ns2:IndicatorToGroupMembership ;
	rdfs:label	"wid" ;
	ns6:member-of	ns14:wid ;
	ns6:order	"4" .
ns35:wid_ui_oc	rdf:type	ns2:IndicatorToGroupMembership ;
	rdfs:label	"wid" ;
	ns6:member-of	ns14:wid ;
	ns6:order	"7" .
ns35:wid_ui_part	rdf:type	ns2:IndicatorToGroupMembership ;
	rdfs:label	"wid" ;
	ns6:member-of	ns14:wid ;
	ns6:order	"8" .
ns1:aaaa_cov	rdf:type	ns2:Indicator ,
		skos:Concept ;
	skos:prefLabel	"IPv6 readiness - websites having a AAAA coverage in DNS records (as % of most visited websites)" ;
	dct:source	ns5:ipv6obs ;
	skos:notation	"aaaa_cov" ;
	skos:altLabel	"IPv6 readiness of most visited websites" ;
	ns6:membership	ns29:aaaa_cov ;
	skos:definition	"IPv6 ready websites are those having at least one AAAA in their DNS records (means the website is visible/can reply to users having an IPv6 connectivity). Tests are done every trimester through a script run by the IPv6 Observatory study on the 1 million most visited websites list provided by Alexa. Websites are attributed to countries on the basis of their main operation location as provided by MaxMind GeoIP database." ;
	skos:topConceptOf	ns8:indicator .
ns1:actspeed	rdf:type	ns2:Indicator ,
		skos:Concept ;
	skos:prefLabel	"Actual download speed of fixed broadband subscriptions" ;
	dct:source	ns5:samknows ;
	skos:notation	"actspeed" ;
	skos:altLabel	"Actual fixed broadband download speed" ;
	ns6:membership	ns16:actspeed ;
	skos:definition	"Average Download Speed during peak periods (ACTSPEED), measured with a specially configured hardware device (SamKnows Whitebox), which runs a series of purpose-built tests to measure various aspect of Internet performance. The measured speed refers to a sample of subscriptions using a similar technology offered by internet service providers. Offers are not weigthed with market shares, so the measured speed cannot be interpreted as the average experienced by consumers." ;
	skos:topConceptOf	ns8:indicator .
ns1:afford_internet_only_minppp	rdf:type	ns2:Indicator ,
		skos:Concept ;
	skos:prefLabel	"Affordability of standalone Fixed Internet Access (minimum price offer)" ;
	dct:source	ns5:biac ;
	skos:notation	"afford_internet_only_minppp" ;
	skos:altLabel	"Affordability of Fixed Internet Access" ;
	ns6:membership	ns16:afford_internet_only_minppp ;
	skos:definition	"Affordability is defined as 12 times the monthly price divided by the \"real adjusted gross disposable income of households per capita\" of the previous year. Disposable income data come from  Eurostat table  <a href=\"http://ec.europa.eu/eurostat/tgm/table.do?tab=table&plugin=1&language=en&pcode=tec00113\">tec00113</a>. Monthly price of standalone Fixed Broadband Internet Access offers, include value added tax, exclude the additional cost of telephony or cable line (if any), and refers to the minimum price in the group of similar subscriptions offered by internet service providers (see the <a href=\"http://digital-agenda-data.eu/charts/see-the-evolution-of-an-indicator-and-compare-countries#chart={%22indicator-group%22:%22any%22,%22indicator%22:%22Price_Internet_only%22,%22breakdown%22:%22offer_12_30_Mbps%22,%22unit-measure%22:%22minimum_euro_PPP%22,%22ref-area%22:[%22EU27%22]}\">original indicator</a>). " ;
	skos:topConceptOf	ns8:indicator .
ns1:avg_ttg	rdf:type	ns2:Indicator ,
		skos:Concept ;
	skos:prefLabel	"Average time to grant" ;
	dct:source	ns5:corda ;
	skos:notation	"avg_ttg" ;
	skos:altLabel	"Average time to grant" ;
	ns6:membership	ns31:avg_ttg ;
	skos:definition	"The Time to Grant (TTG) is defined as the time lapsed from a call's closing date (deadline for submission of proposals) to that of a grant signature by the European Commission. In the case of two-stage calls for proposals, it is the second stage call deadline that is used in the calculation of the Time to Grant. Time to grant is expressed in calendar days. \nAverage time to grant is the arythmetic average for all grants within the defined scope." ;
	skos:topConceptOf	ns8:indicator .
ns1:bb_dsl	rdf:type	ns2:Indicator ,
		skos:Concept ;
	skos:prefLabel	"DSL subscriptions share in fixed broadband" ;
	dct:source	ns5:cocom ;
	skos:notation	"bb_dsl" ;
	skos:altLabel	"DSL subscriptions share in fixed broadband" ;
	ns6:membership	ns17:bb_dsl ;
	skos:definition	"Share of DSL (Digital Subscriber Line) in total fixed broadband subscriptions." ;
	skos:topConceptOf	ns8:indicator .
ns1:bb_fcov	rdf:type	ns2:Indicator ,
		skos:Concept ;
	skos:prefLabel	"Fixed broadband coverage (2005-2010)" ;
	dct:source	ns5:idate ;
	skos:notation	"bb_fcov" ;
	skos:altLabel	"Fixed broadband coverage (2005-2010)" ;
	ns6:membership	ns20:bb_fcov ;
	skos:definition	"Coverage is a supply indicator, defined as the percentage of total/rural population living in areas served by fixed broadband: either DSL or cable modem networks." ;
	skos:note	"Indicator collected until 2010. Then replaced with two different coverage indicators, for standard broadband and NGA respectively." ;
	skos:topConceptOf	ns8:indicator .
ns1:bb_fttpcov	rdf:type	ns2:Indicator ,
		skos:Concept ;
	skos:prefLabel	"Fibre to the Premises coverage/availability (as a % of households)" ;
	dct:source	ns5:bc2020 ;
	skos:notation	"bb_fttpcov" ;
	skos:altLabel	"Fibre to the Premises coverage" ;
	ns6:membership	ns17:bb_fttpcov ;
	skos:definition	"Coverage is a supply indicator defined as the percentage of Households living in areas served by FTTP" ;
	skos:topConceptOf	ns8:indicator .
ns1:bb_hhi	rdf:type	ns2:Indicator ,
		skos:Concept ;
	skos:prefLabel	"Herfindahl index on broadband competition" ;
	dct:source	ns5:cocom ;
	skos:notation	"bb_hhi" ;
	skos:altLabel	"Herfindahl index on broadband competition" ;
	ns6:membership	ns17:bb_hhi ;
	skos:definition	"Herfindahl index calculated for seven different connection technologies: xDSL, full or shared LLU, Cable, FTTH, FTTB, Other NGA, Other. Their respective market shares are expressed in percentage of all fixed broadband subscriptions. A small index indicates a competitive industry with no dominant technological platform. The index values raises with concentration over one or few platforms." ;
	skos:topConceptOf	ns8:indicator .
ns1:bb_lines	rdf:type	skos:Concept ,
		ns2:Indicator ;
	skos:prefLabel	"Fixed broadband subscriptions" ;
	dct:source	ns5:cocom ;
	skos:notation	"bb_lines" ;
	skos:altLabel	"Fixed broadband subscriptions" ;
	ns6:membership	ns17:bb_lines ;
	skos:definition	"Number of fixed broadband subscriptions (lines)." ;
	skos:topConceptOf	ns8:indicator .
ns1:bb_ne	rdf:type	skos:Concept ,
		ns2:Indicator ;
	skos:prefLabel	"New entrants' share in fixed broadband subscriptions" ;
	dct:source	ns5:cocom ;
	skos:notation	"bb_ne" ;
	skos:altLabel	"New entrants' share in fixed broadband subscriptions" ;
	ns6:membership	ns17:bb_ne ;
	skos:definition	"Market share based on fixed broadband subscriptions (lines). New entrants mean operators that did not enjoy special and exclusive rights or de facto monopoly for the provision of voice telephony services before the liberalisation." ;
	skos:topConceptOf	ns8:indicator .
ns1:bb_ngacov	rdf:type	skos:Concept ,
		ns2:Indicator ;
	skos:prefLabel	"NGA broadband coverage/availability (as a % of households)" ;
	dct:source	ns5:bc2020 ;
	skos:notation	"bb_ngacov" ;
	skos:altLabel	"NGA broadband coverage/availability" ;
	ns6:membership	ns17:bb_ngacov ;
	skos:definition	"Coverage is a supply indicator defined as the percentage of Households living in areas served by NGA. Next Generation Access includes the following technologies: FTTH, FTTB, Cable Docsis 3.0, VDSL and other superfast broadband (at least 30 Mbps download)" ;
	skos:topConceptOf	ns8:indicator .
ns1:bb_penet	rdf:type	skos:Concept ,
		ns2:Indicator ;
	skos:prefLabel	"Fixed broadband take-up (subscriptions/100 people)" ;
	dct:source	ns5:cocom ;
	skos:notation	"bb_penet" ;
	skos:altLabel	"Fixed broadband take-up (penetration rate)" ;
	ns6:membership	ns17:bb_penet ;
	skos:definition	"Number of fixed broadband subscriptions (lines) per 100 people. Penetration of fixed broadband." ;
	skos:topConceptOf	ns8:indicator .
ns1:bb_rfttpcov	rdf:type	skos:Concept ,
		ns2:Indicator ;
	skos:prefLabel	"Rural Fibre to the Premises coverage/availability (as a % of households)" ;
	dct:source	ns5:bc2020 ;
	skos:notation	"bb_rfttpcov" ;
	skos:altLabel	"Rural Fibre to the Premises coverage" ;
	ns6:membership	ns17:bb_rfttpcov ;
	skos:definition	"Coverage is a supply indicator defined as the percentage of Households living in areas served by FTTP. Rural areas are defined as those with less than 100 people per km2." ;
	skos:topConceptOf	ns8:indicator .
ns1:bb_rngacov	rdf:type	skos:Concept ,
		ns2:Indicator ;
	skos:prefLabel	"Rural NGA broadband coverage/availability (as a % of households)" ;
	dct:source	ns5:bc2020 ;
	skos:notation	"bb_rngacov" ;
	skos:altLabel	"Rural NGA broadband coverage" ;
	ns6:membership	ns17:bb_rngacov ;
	skos:definition	"Coverage is a supply indicator defined as the percentage of Households living in areas served by NGA. Next Generation Access includes the following technologies: FTTH, FTTB, Cable Docsis 3.0, VDSL and other superfast broadband (at least 30 Mbps download). Rural areas are defined as those with less than 100 people per km2." ;
	skos:topConceptOf	ns8:indicator .
ns1:bb_scov	rdf:type	skos:Concept ,
		ns2:Indicator ;
	skos:prefLabel	"Standard fixed broadband coverage/availability (as a % of households)" ;
	dct:source	ns5:bc2020 ;
	skos:notation	"bb_scov" ;
	skos:altLabel	"Standard fixed broadband coverage/availability" ;
	ns6:membership	ns17:bb_scov ;
	skos:definition	"Coverage is a supply indicator defined as the percentage of Households living in areas served by xDSL, cable (basic and NGA), FTTP or WiMax networks" ;
	skos:topConceptOf	ns8:indicator .
ns1:bb_speed10	rdf:type	skos:Concept ,
		ns2:Indicator ;
	skos:prefLabel	"Share of fixed broadband subscriptions >= 10 Mbps - Advertised download speed" ;
	dct:source	ns5:cocom ;
	skos:notation	"bb_speed10" ;
	skos:altLabel	"Share of fixed broadband subscriptions >= 10 Mbps" ;
	ns6:membership	ns16:bb_speed10 ;
	skos:definition	"Based on advertised download speeds." ;
	skos:topConceptOf	ns8:indicator .
ns1:bb_speed100	rdf:type	skos:Concept ,
		ns2:Indicator ;
	skos:prefLabel	"Share of fixed broadband subscriptions >= 100 Mbps - Advertised download speed" ;
	dct:source	ns5:cocom ;
	skos:notation	"bb_speed100" ;
	skos:altLabel	"Share of fixed broadband subscriptions >= 100 Mbps" ;
	ns6:membership	ns16:bb_speed100 ;
	skos:definition	"Based on advertised download speeds." ;
	skos:topConceptOf	ns8:indicator .
ns1:bb_speed2	rdf:type	skos:Concept ,
		ns2:Indicator ;
	skos:prefLabel	"Share of fixed broadband subscriptions >= 2 Mbps - Advertised download speed" ;
	dct:source	ns5:cocom ;
	skos:notation	"bb_speed2" ;
	skos:altLabel	"Share of fixed broadband subscriptions >= 2 Mbps" ;
	ns6:membership	ns16:bb_speed2 ;
	skos:definition	"Based on advertised download speeds." ;
	skos:topConceptOf	ns8:indicator .
ns1:bb_speed30	rdf:type	skos:Concept ,
		ns2:Indicator ;
	skos:prefLabel	"Share of fixed broadband subscriptions >= 30 Mbps - Advertised download speed" ;
	dct:source	ns5:cocom ;
	skos:notation	"bb_speed30" ;
	skos:altLabel	"Share of fixed broadband subscriptions >= 30 Mbps" ;
	ns6:membership	ns16:bb_speed30 ;
	skos:definition	"Based on advertised download speeds." ;
	skos:topConceptOf	ns8:indicator .
ns1:bb_srcov	rdf:type	skos:Concept ,
		ns2:Indicator ;
	skos:prefLabel	"Rural standard fixed broadband coverage (as a % of households)" ;
	dct:source	ns5:bc2020 ;
	skos:notation	"bb_srcov" ;
	skos:altLabel	"Rural standard fixed broadband coverage" ;
	ns6:membership	ns17:bb_srcov ;
	skos:definition	"Coverage is a supply indicator defined as the percentage of Households living in areas served by xDSL, cable (basic and NGA), FTTP or WiMax networks. Rural areas are defined as those with less than 100 people per km2." ;
	skos:topConceptOf	ns8:indicator .
ns1:bs_rd_expen_ict	rdf:type	skos:Concept ,
		ns2:Indicator ;
	skos:prefLabel	"Business R&D expenditure of the ICT sector" ;
	dct:source	ns5:jrc_ict_randd ;
	skos:notation	"bs_rd_expen_ict" ;
	skos:altLabel	"Business R&D expenditure of the ICT sector" ;
	ns6:membership	ns25:bs_rd_expen_ict ;
	skos:definition	"Intramural expenditures on R&D performed within business enterprise sector during a specific period, whatever the source of funds (Frascati Manual)." ;
	skos:topConceptOf	ns8:indicator .
ns1:c1_bandwidth	rdf:type	skos:Concept ,
		ns2:Indicator ;
	skos:prefLabel	"Total bandwidth available in G\u00E9ant" ;
	dct:source	ns5:einfrageant ;
	skos:notation	"c1_bandwidth" ;
	skos:altLabel	"Total bandwidth available in G\u00E9ant" ;
	ns6:membership	ns32:c1_bandwidth ;
	skos:definition	"This is measured as total bandwidth available in the European G\u00C9ANT footprint (Gbpskms)  ( European dark fibre + European leased capacity excluding the connections to interconnections such as Internet2)" ;
	skos:note	"As of June 2014 the revamping of the networking was achieved and due to a technology optimisation there are less lightened backup routes explaining the decrease in capacity." ;
	skos:topConceptOf	ns8:indicator .
ns1:c1_compcyclesegi	rdf:type	skos:Concept ,
		ns2:Indicator ;
	skos:prefLabel	"Computing cycles available for open transnational access in EGI" ;
	dct:source	ns5:einfraegi ;
	skos:notation	"c1_compcyclesegi" ;
	skos:altLabel	"Computing cycles EGI" ;
	ns6:membership	ns32:c1_compcyclesegi ;
	skos:definition	"Computing cycles made available by EGI - the European Grid Infrastructure -, a federation of over 350 resource centres coordinated by a not-for-profit foundation which delivers integrated computing services to European researchers, co-funded by the European Commission." ;
	skos:topConceptOf	ns8:indicator .
ns1:c1_compcyclesprace	rdf:type	skos:Concept ,
		ns2:Indicator ;
	skos:prefLabel	"Computing cycles available for open transnational access in PRACE" ;
	dct:source	ns5:einfraprace ;
	skos:notation	"c1_compcyclesprace" ;
	skos:altLabel	"Computing cycles PRACE" ;
	ns6:membership	ns32:c1_compcyclesprace ;
	skos:definition	"Computing cycles allocated by PRACE - Partnership for Advanced Computing in Europe -, a project which delivers pan-European supercomputing infrastructure to European researchers, co-funded by the European Commission." ;
	skos:topConceptOf	ns8:indicator .
ns1:c1_datatraffic	rdf:type	ns2:Indicator ,
		skos:Concept ;
	skos:prefLabel	"Cross border Data traffic over the research networks" ;
	dct:source	ns5:einfrageant ;
	skos:notation	"c1_datatraffic" ;
	skos:altLabel	"Cross border Data traffic" ;
	ns6:membership	ns32:c1_datatraffic ;
	skos:definition	"This is the total monthly volume of traffic transiting G\u00C9ANT. As reported in the G\u00C9ANT MSR, measured as the aggregated traffic over a month to and from the European NRENs and all world regions." ;
	skos:note	"As of 01/01/2015 the indicator is reset to integrate traffic that was not counted (Layer 1 & 2)." ;
	skos:topConceptOf	ns8:indicator .
ns1:desi	rdf:type	ns2:Indicator ,
		skos:Concept ;
	skos:prefLabel	"Digital Economy and Society Index" ;
	dct:source	ns5: ;
	skos:notation	"desi" ;
	skos:altLabel	"DESI Stacked" ;
	ns6:membership	ns18:desi ;
	skos:definition	"DESI overall index, calculated as the weighted average of the four main DESI dimensions." ;
	skos:topConceptOf	ns8:indicator .
ns1:desi_sliders	rdf:type	skos:Concept ,
		ns2:Indicator ;
	skos:prefLabel	"Digital Economy and Society Index" ;
	dct:source	ns5: ;
	skos:notation	"desi_sliders" ;
	skos:altLabel	"DESI" ;
	ns6:membership	ns19:desi_sliders ;
	skos:definition	"DESI overall index, calculated as the weighted average of the four main DESI dimensions with the weights selected by the user." ;
	skos:topConceptOf	ns8:indicator .
ns1:e_ade	rdf:type	ns2:Indicator ,
		skos:Concept ;
	skos:prefLabel	"Enterprises exchanging business documents suitable for automatic processing" ;
	dct:source	ns5:estat_isoc_bde15disc ;
	skos:notation	"e_ade" ;
	skos:altLabel	"Automatic exchange of business documents" ;
	ns6:membership	ns20:e_ade ;
	skos:definition	"The indicator refers to sending/receiving of messages (orders, invoices, payment transactions, transport documents, tax declarations, etc.) to/from other enterprises, public authorities or financial institutions in an agreed or standard format (as EDIFACT, XML, etc) which allows their automatic processing without the individual message being manually typed." ;
	skos:note	"Enterprises with 10 or more persons employed. All manufacturing and service sectors, excluding the financial sector. Breaks in series because until 2008 economic activities according to NACE Rev 1.1 and from 2009 data are based on NACE Rev.2. Since 2010 data include also sector S 95.1-Repair of computers and communication equipment." ;
	skos:topConceptOf	ns8:indicator .
ns1:e_ads	rdf:type	ns2:Indicator ,
		skos:Concept ;
	skos:prefLabel	"Enterprises paying to advertise on the internet\n" ;
	dct:source	ns5:estat_isoc_cismt ;
	skos:notation	"e_ads" ;
	skos:altLabel	"Enterprises paying to advertise on the internet\n" ;
	ns6:membership	ns7:e_ads ;
	skos:definition	"Enterprises paying to advertise on the internet\n" ;
	skos:note	"Enterprises with 10 or more persons employed. All manufacturing and service sectors, excluding the financial sector. Breaks in series because until 2008 economic activities according to NACE Rev 1.1 and from 2009 data are based on NACE Rev.2. Since 2010 data include also sector S 95.1-Repair of computers and communication equipment." ;
	skos:topConceptOf	ns8:indicator .
ns1:e_ads_loc	rdf:type	ns2:Indicator ,
		skos:Concept ;
	skos:prefLabel	"Enterprises advertising online based on the geolocation of internet users " ;
	dct:source	ns5:estat_isoc_cismt ;
	skos:notation	"e_ads_loc" ;
	skos:altLabel	"Enterprises advertising online based on the geolocation of internet users " ;
	ns6:membership	ns33:e_ads_loc ;
	skos:definition	"Pay to advertise on the internet, based on the geolocation of internet users " ;
	skos:topConceptOf	ns8:indicator .
ns1:e_ads_trk	rdf:type	ns2:Indicator ,
		skos:Concept ;
	skos:prefLabel	"Enterprises tracking internet users for targeted advertising " ;
	dct:source	ns5:estat_isoc_cismt ;
	skos:notation	"e_ads_trk" ;
	skos:altLabel	"Enterprises tracking internet users for targeted advertising " ;
	ns6:membership	ns33:e_ads_trk ;
	skos:definition	"Pay to advertise on the internet, based on the tracking of internet users' past activities or profile " ;
	skos:topConceptOf	ns8:indicator .
ns1:e_aeseu	rdf:type	ns2:Indicator ,
		skos:Concept ;
	skos:prefLabel	"Enterprises having done electronic sales to other EU countries in the last calender year" ;
	dct:source	ns5:estat_isoc_ec_eseln2 ;
	skos:notation	"e_aeseu" ;
	skos:altLabel	"Enterprises selling cross-border to other EU countries" ;
	ns6:membership	ns21:e_aeseu ;
	skos:definition	"The sales have been realised, during the previous calendar year, via any computer networks (in monetary terms, excluding VAT). Computer networks include websites, EDI-type systems and other means of electronic data transfer, excluding manually typed e-mails." ;
	skos:note	"Enterprises with 10 or more persons employed. All manufacturing and service sectors, excluding the financial sector. Breaks in series because until 2008 economic activities according to NACE Rev 1.1 and from 2009 data are based on NACE Rev.2. Since 2010 data include also sector S 95.1-Repair of computers and communication equipment." ;
	skos:topConceptOf	ns8:indicator .
ns1:e_aws	rdf:type	ns2:Indicator ,
		skos:Concept ;
	skos:prefLabel	"Enterprises selling via a website or apps by geographical location of the costumer" ;
	dct:source	ns5: ;
	skos:notation	"e_aws" ;
	skos:altLabel	"Enterprises selling via a website or apps by geographical location " ;
	ns6:membership	ns21:e_aws ;
	skos:definition	"Share of the enterprises that, during the previous calendar year, received orders by costumers located in the own country, other EU countries or the rest of the world" ;
	skos:note	"Enterprises with 10 or more persons employed. All manufacturing and service sectors, excluding the financial sector. Breaks in series because until 2008 economic activities according to NACE Rev 1.1 and from 2009 data are based on NACE Rev.2. Since 2010 data include also sector S 95.1-Repair of computers and communication equipment." ;
	skos:topConceptOf	ns8:indicator .
ns1:e_aws_cmp	rdf:type	ns2:Indicator ,
		skos:Concept ;
	skos:prefLabel	"Enterprises using e-Commerce marketplace for sales" ;
	dct:source	ns5: ;
	skos:notation	"e_aws_cmp" ;
	skos:altLabel	"Enterprises selling via e-Commerce marketplace" ;
	ns6:membership	ns21:e_aws_cmp ;
	skos:definition	"Share of enterprises that, during the previous calendar year, received orders for goods or services via an e-Commerce marketplace" ;
	skos:note	"Enterprises with 10 or more persons employed. All manufacturing and service sectors, excluding the financial sector. Breaks in series because until 2008 economic activities according to NACE Rev 1.1 and from 2009 data are based on NACE Rev.2. Since 2010 data include also sector S 95.1-Repair of computers and communication equipment." ;
	skos:topConceptOf	ns8:indicator .
ns1:e_aws_cown	rdf:type	ns2:Indicator ,
		skos:Concept ;
	skos:prefLabel	"Enterprises using  their own website or apps for sales" ;
	dct:source	ns5: ;
	skos:notation	"e_aws_cown" ;
	skos:altLabel	"Enterprises selling via own website or apps" ;
	ns6:membership	ns21:e_aws_cown ;
	skos:definition	"Share of enterprises that, during the previous calendar year, received orders for goods or services via their own website or apps." ;
	skos:note	"Enterprises with 10 or more persons employed. All manufacturing and service sectors, excluding the financial sector. Breaks in series because until 2008 economic activities according to NACE Rev 1.1 and from 2009 data are based on NACE Rev.2. Since 2010 data include also sector S 95.1-Repair of computers and communication equipment." ;
	skos:topConceptOf	ns8:indicator .
ns1:e_aws_gt1_b2c_gt10ws	rdf:type	ns2:Indicator ,
		skos:Concept ;
	skos:prefLabel	"Enterprises exploiting the \"Business to Consumers\" opportunities of web sales" ;
	dct:source	ns5:estat_isoc_ec_eseln2 ;
	skos:notation	"e_aws_gt1_b2c_gt10ws" ;
	skos:altLabel	"Enterprises exploiting B2C opportunities of web sales " ;
	ns6:membership	ns21:e_aws_gt1_b2c_gt10ws ;
	skos:definition	"Enterprises where web sales are more than 1% of total turnover and B2C web sales more than 10% of the web sales" ;
	skos:note	"Enterprises with 10 or more persons employed. All manufacturing and service sectors, excluding the financial sector. Breaks in series because since 2010 data include also sector S 95.1-Repair of computers and communication equipment." ;
	skos:topConceptOf	ns8:indicator .
ns1:e_awsval_cmp	rdf:type	ns2:Indicator ,
		skos:Concept ;
	skos:prefLabel	"Sells via marketplace  as a pecentage of turnover" ;
	dct:source	ns5: ;
	skos:notation	"e_awsval_cmp" ;
	skos:altLabel	"Sells via marketplace" ;
	ns6:membership	ns21:e_awsval_cmp ;
	skos:definition	"The value of sales made during the previous calendar year, via an e-Commerce marketplace in % of the total turnover value (in monetary terms, excluding VAT)." ;
	skos:note	"Enterprises with 10 or more persons employed. All manufacturing and service sectors, excluding the financial sector. Breaks in series because until 2008 economic activities according to NACE Rev 1.1 and from 2009 data are based on NACE Rev.2. Since 2010 data include also sector S 95.1-Repair of computers and communication equipment." ;
	skos:topConceptOf	ns8:indicator .
ns1:e_awsval_cown	rdf:type	ns2:Indicator ,
		skos:Concept ;
	skos:prefLabel	"Sells via own website or apps as a pecentage of turnover" ;
	dct:source	ns5: ;
	skos:notation	"e_awsval_cown" ;
	skos:altLabel	"Sells via own website or apps " ;
	ns6:membership	ns21:e_awsval_cown ;
	skos:definition	"The value of sales made during the previous calendar year, via their own website or apps in % of the total turnover value (in monetary terms, excluding VAT)." ;
	skos:note	"Enterprises with 10 or more persons employed. All manufacturing and service sectors, excluding the financial sector. Breaks in series because until 2008 economic activities according to NACE Rev 1.1 and from 2009 data are based on NACE Rev.2. Since 2010 data include also sector S 95.1-Repair of computers and communication equipment." ;
	skos:topConceptOf	ns8:indicator .
ns1:e_bd	rdf:type	ns2:Indicator ,
		skos:Concept ;
	skos:prefLabel	"Enterprises analysing big data from any data source" ;
	dct:source	ns5:estat-ent ;
	skos:notation	"e_bd" ;
	skos:altLabel	"Enterprises analysing big data from any data source (until 2018)" ;
	ns6:membership	ns7:e_bd ;
	skos:definition	"Analyse big data from any data source" ;
	skos:topConceptOf	ns8:indicator .
ns1:e_broad	rdf:type	ns2:Indicator ,
		skos:Concept ;
	skos:prefLabel	"Enterprises having a fixed broadband connection" ;
	dct:source	ns5:estat_isoc_ci_eu_en2 ;
	skos:notation	"e_broad" ;
	skos:altLabel	"Enterprises with a fixed broadband connection" ;
	ns6:membership	ns17:e_broad ;
	skos:definition	"Fixed broadband connections include DSL, xDSL, cable leased lines, Frame Relay, Metro-Ethernet, PLC-Powerline communications, fixed wireless connections, etc." ;
	skos:note	"Enterprises with 10 or more persons employed. All manufacturing and service sectors, excluding the financial sector. Breaks in series because until 2008 economic activities according to NACE Rev 1.1 and from 2009 data are based on NACE Rev.2. Since 2010 data include also sector S 95.1-Repair of computers and communication equipment." ;
	skos:topConceptOf	ns8:indicator .
ns1:e_cc	rdf:type	ns2:Indicator ,
		skos:Concept ;
	skos:prefLabel	"Buy Cloud Computing services used over the internet" ;
	dct:source	ns5:estat_isoc_cicce_use ;
	skos:notation	"e_cc" ;
	skos:altLabel	"Cloud computing services (any)" ;
	ns6:membership	ns7:e_cc ;
	skos:definition	"Cloud computing refers to purchased ICT services that have all of the following characteristics: are delivered from servers of service providers; can be easily scaled up or down; can be used on-demand by the user without human interaction with the service provider; are paid for, either per user, by capacity used, or they are pre-paid.Eurostat variable e_cc_ge_me" ;
	skos:note	"Cloud computing may include connections via Virtual Private Networks (VPN). Optional question in 2015, not all countries have collected the indicator." ;
	skos:topConceptOf	ns8:indicator .
ns1:e_cc_ge_me	rdf:type	ns2:Indicator ,
		skos:Concept ;
	skos:prefLabel	"Buy Cloud Computing services of medium-high sophistication" ;
	dct:source	ns5:estat_isoc_cicce_use ;
	skos:notation	"e_cc_ge_me" ;
	skos:altLabel	"Cloud computing services (medium-high sophistication)" ;
	ns6:membership	ns7:e_cc_ge_me ;
	skos:definition	"Enterprises purchasing at least one of the following cloud computing services: hosting of the enterprise's database, accounting software applications, CRM software, computing power." ;
	skos:note	"Computed from Eurostat database with the following formula = (e_cc_me) - (e_cc_lo) + (e_cc_hi). Optional question in 2015, not all countries have collected the indicator." ;
	skos:topConceptOf	ns8:indicator .
ns1:e_cc_pcpu	rdf:type	skos:Concept ,
		ns2:Indicator ;
	skos:prefLabel	"Enterprises buying computing power in the Cloud" ;
	dct:source	ns5:estat_isoc_ci_eu_en2 ;
	skos:notation	"e_cc_pcpu" ;
	skos:altLabel	"Enterprises buying computing power to run own software in the Cloud" ;
	ns6:membership	ns7:e_cc_pcpu ;
	skos:definition	"Cloud computing refers to purchased ICT services that have all of the following characteristics: are delivered from servers of service providers; can be easily scaled up or down; can be used on-demand by the user without human interaction with the service provider; are paid for, either per user, by capacity used, or they are pre-paid." ;
	skos:note	"Optional question in 2015, not all countries have collected the indicator." ;
	skos:topConceptOf	ns8:indicator .
ns1:e_crman	rdf:type	skos:Concept ,
		ns2:Indicator ;
	skos:prefLabel	"Enterprises using Customer Relationship Management (CRM) software" ;
	dct:source	ns5:estat_isoc_bde15dec ;
	skos:notation	"e_crman" ;
	skos:altLabel	"Use of analytical CRM software" ;
	ns6:membership	ns7:e_crman ;
	skos:definition	"CRM refers to the use of any software application used for the analysis of information about clients for marketing purposes." ;
	skos:note	"Enterprises with 10 or more persons employed. All manufacturing and service sectors, excluding the financial sector. Breaks in series because until 2008 economic activities according to NACE Rev 1.1 and from 2009 data are based on NACE Rev.2. Since 2010 data include also sector S 95.1-Repair of computers and communication equipment." ;
	skos:topConceptOf	ns8:indicator .
ns1:e_di_hivhi	rdf:type	skos:Concept ,
		ns2:Indicator ;
	skos:prefLabel	"Enterprises with High levels of Digital Intensity" ;
	dct:source	ns5:estat-ent ;
	skos:notation	"e_di_hivhi" ;
	skos:altLabel	"Enterprises with High levels of Digital Intensity" ;
	ns6:membership	ns7:e_di_hivhi ;
	skos:definition	"The Digital Intensity score is based on counting how many out of 12 technologies are used by each enterprise. High levels are attributed to those enterprises using at least 7 of the listed digital technologies." ;
	skos:note	"The 2015 list of technologies includes: usage of internet by a majority of the workers; access to ICT specialist skills; fixed broadband speed > 30 Mbps; mobile devices used by more than 20% of employed persons; has a website; has some sophisticated functions on the website; presence on social media; does e-sales for at least 1% of turnover; exploit the B2C opportunities of web sales; use an ERP software; use a CRM software; share electronically supply chain management information.\r\nIn 2016 the last 3 indicators have been replaced with: pay to advertise on the internet; purchase cloud computing advanced services; send eInvoices. There is thus a break in series with in general a reduction of the digital intensity scores." ;
	skos:topConceptOf	ns8:indicator .
ns1:e_di_vlo	rdf:type	skos:Concept ,
		ns2:Indicator ;
	skos:prefLabel	"Enterprises with Very Low level of Digital Intensity" ;
	dct:source	ns5:estat-ent ;
	skos:notation	"e_di_vlo" ;
	skos:altLabel	"Enterprises with Very Low level of Digital Intensity" ;
	ns6:membership	ns7:e_di_vlo ;
	skos:definition	"The Digital Intensity score is based on counting how many out of 12 technologies are used by each enterprise. Very Low levels are attributed to those enterprises using no more than 3 of the listed digital technologies." ;
	skos:note	"The 2015 list of technologies includes: usage of internet by a majority of the workers; access to ICT specialist skills; fixed broadband speed > 30 Mbps; mobile devices used by more than 20% of employed persons; has a website; has some sophisticated functions on the website; presence on social media; does e-sales for at least 1% of turnover; exploit the B2C opportunities of web sales; use an ERP software; use a CRM software; share electronically supply chain management information.\r\nIn 2016 the last 3 indicators have been replaced with: pay to advertise on the internet; purchase cloud computing advanced services; send eInvoices. There is thus a break in series with in general a reduction of the digital intensity scores." ;
	skos:topConceptOf	ns8:indicator .
ns1:e_ebuy	rdf:type	skos:Concept ,
		ns2:Indicator ;
	skos:prefLabel	"Enterprises using any computer network for purchases (at least 1%)" ;
	dct:source	ns5:estat_isoc_bde15dec ;
	skos:notation	"e_ebuy" ;
	skos:altLabel	"Enterprises purchasing online" ;
	ns6:membership	ns20:e_ebuy ;
	skos:definition	"The purchases realised, during the previous calendar year, via any computer networks should represent at least 1% of the total purchases value (in monetary terms, excluding VAT). Computer networks include websites, EDI-type systems and other means of electronic data transfer, excluding manually typed e-mails." ;
	skos:note	"Since 2011 the indicator is optional, so EU27 estimates cover less countries and are not comparable with previous years. Enterprises with 10 or more persons employed. All manufacturing and service sectors, excluding the financial sector. Breaks in series because until 2008 economic activities according to NACE Rev 1.1 and from 2009 data are based on NACE Rev.2. Since 2010 data include also sector S 95.1-Repair of computers and communication equipment." ;
	skos:topConceptOf	ns8:indicator .
ns1:e_empmd_gt20	rdf:type	skos:Concept ,
		ns2:Indicator ;
	skos:prefLabel	"Enterprises providing portable devices to more than 20% of their employed persons" ;
	dct:source	ns5:estat_isoc_bde15b_e ;
	skos:notation	"e_empmd_gt20" ;
	skos:altLabel	"Enterprises providing portable devices to > 20% of their employed persons" ;
	ns6:membership	ns7:e_empmd_gt20 ;
	skos:definition	"The devices (portable computers, tablets, smartphones, PDA phones, etc.) should be provided for business use and the enterprises pay for all or at least up to a limit the subscription and the use costs." ;
	skos:note	"Only the 2011 question was limited to portable devices using at least 3G technology to connect to the internet. Enterprises with 10 or more persons employed. All manufacturing and service sectors, excluding the financial sector." ;
	skos:topConceptOf	ns8:indicator .
ns1:e_erp1	rdf:type	skos:Concept ,
		ns2:Indicator ;
	skos:prefLabel	"Enterprises that share internally electronic information with an ERP" ;
	dct:source	ns5:estat_isoc_bde15dip ;
	skos:notation	"e_erp1" ;
	skos:altLabel	"Integration of internal processes (with an ERP)" ;
	ns6:membership	ns7:e_erp1 ;
	skos:definition	"Have in use an ERP-Enterprise resource planning software package, to share information between different functional areas (e.g. accounting, planning, production, marketing)." ;
	skos:note	"Enterprises with 10 or more persons employed. All manufacturing and service sectors, excluding the financial sector. Breaks in series because until 2008 economic activities according to NACE Rev 1.1 and from 2009 data are based on NACE Rev.2. Since 2010 data include also sector S 95.1-Repair of computers and communication equipment. Break in series in 2012 due to different wording of the question." ;
	skos:topConceptOf	ns8:indicator .
ns1:e_esell	rdf:type	skos:Concept ,
		ns2:Indicator ;
	skos:prefLabel	"Enterprises using any computer network for sales (at least 1%)" ;
	dct:source	ns5:estat_isoc_ec_eseln2 ;
	skos:notation	"e_esell" ;
	skos:altLabel	"Enterprises selling online" ;
	ns6:membership	ns21:e_esell ;
	skos:definition	"The sales realised, during the previous calendar year, via any computer networks should represent at least 1% of the total turnover value (in monetary terms, excluding VAT). Computer networks include websites, EDI-type systems and other means of electronic data transfer, excluding manually typed e-mails." ;
	skos:note	"Enterprises with 10 or more persons employed. All manufacturing and service sectors, excluding the financial sector. Breaks in series because until 2008 economic activities according to NACE Rev 1.1 and from 2009 data are based on NACE Rev.2. Since 2010 data include also sector S 95.1-Repair of computers and communication equipment." ;
	skos:topConceptOf	ns8:indicator .
ns1:e_eturn	rdf:type	skos:Concept ,
		ns2:Indicator ;
	skos:prefLabel	"Total electronic sales by enterprises, as a % of their total turnover" ;
	dct:source	ns5:estat_isoc_ci_eu_en2 ;
	skos:notation	"e_eturn" ;
	skos:altLabel	"Turnover from eCommerce" ;
	ns6:membership	ns21:e_eturn ;
	skos:definition	"The value of sales realised, during the previous calendar year, via any computer networks in % of the total turnover value (in monetary terms, excluding VAT). Computer networks include websites, EDI-type systems and other means of electronic data transfer, excluding manually typed e-mails." ;
	skos:note	"Enterprises with 10 or more persons employed. All manufacturing and service sectors, excluding the financial sector. Breaks in series because until 2008 economic activities according to NACE Rev 1.1 and from 2009 data are based on NACE Rev.2. Since 2010 data include also sector S 95.1-Repair of computers and communication equipment." ;
	skos:topConceptOf	ns8:indicator .
ns1:e_gov_1_ucg	rdf:type	skos:Concept ,
		ns2:Indicator ;
	skos:prefLabel	"1 User Centricity" ;
	dct:source	ns5:egov_bench12_17 ;
	skos:notation	"e_gov_1_ucg" ;
	skos:altLabel	"1 User Centricity" ;
	ns6:membership	ns22:e_gov_1_ucg ;
	skos:definition	"The extent to which (information about) a public service is provided online, how the online journey is supported and if public websites are mobile friendly." ;
	skos:note	"Composite indicator:\n(2016-2017) weighted average of Online availability (67%), Usability (22%) and Mobile Friendliness (11%).\n(2012-2015) weighted average of Online availability (67%), Usability (17%), Ease of Use (8%) and Speed of Use (8%)\nBreak in series in 2016 (no data displayed for breakdown:Total 2016)." ;
	skos:topConceptOf	ns8:indicator .
ns1:e_gov_1a_ucg_oa	rdf:type	skos:Concept ,
		ns2:Indicator ;
	skos:prefLabel	"1a User Centricity - Online availability" ;
	dct:source	ns5:egov_bench12_17 ;
	skos:notation	"e_gov_1a_ucg_oa" ;
	skos:altLabel	"1a User Centricity - Online availability" ;
	ns6:membership	ns22:e_gov_1a_ucg_oa ;
	skos:definition	"The extent to which a Public Service or information concerning the public service is provided online, and via a portal." ;
	skos:topConceptOf	ns8:indicator .
ns1:e_gov_1b_ucg_us	rdf:type	skos:Concept ,
		ns2:Indicator ;
	skos:prefLabel	"1b User Centricity - Usability" ;
	dct:source	ns5:egov_bench12_17 ;
	skos:notation	"e_gov_1b_ucg_us" ;
	skos:altLabel	"1b User Centricity - Usability" ;
	ns6:membership	ns22:e_gov_1b_ucg_us ;
	skos:definition	"Indicates if support, help and (interactive) feedback functionalities for the online public service are available." ;
	skos:topConceptOf	ns8:indicator .
ns1:e_gov_1c_ucg_mf	rdf:type	skos:Concept ,
		ns2:Indicator ;
	skos:prefLabel	"1c User Centricity - Mobile Friendliness" ;
	dct:source	ns5:egov_bench12_17 ;
	skos:notation	"e_gov_1c_ucg_mf" ;
	skos:altLabel	"1c User Centricity - Mobile Friendliness" ;
	ns6:membership	ns22:e_gov_1c_ucg_mf ;
	skos:definition	"The ability to provide public services through a mobile-friendly interface; an interface that is \u2018adapted\u2019 to the mobile device. The data collection for this indicator is done via an automated tool. " ;
	skos:note	"The new key enabler \u201CMobile Friendliness\u201D was introduced in 2016. Mobile friendliness was also measured in 2014 and 2015 as proof-of-concept indicator. It was not part of the calculation of the User Centricity Benchmark in those years, but presented as separate index. In 2016, mobile friendliness of both individual services\u2019 websites as well as generic portals is integrated as a component of the Online Usability and User Centricity composite indicators." ;
	skos:topConceptOf	ns8:indicator .
ns1:e_gov_1d_ucg_eu	rdf:type	skos:Concept ,
		ns2:Indicator ;
	skos:prefLabel	"1d User Centricity - Ease of Use" ;
	dct:source	ns5:egov_bench12_17 ;
	skos:notation	"e_gov_1d_ucg_eu" ;
	skos:altLabel	"1d User Centricity - Ease of Use" ;
	ns6:membership	ns22:e_gov_1d_ucg_eu ;
	skos:definition	"Quality assessment by researchers indicating how intuitively and smoothly the online process steps for obtaining a public service can be completed.  It assesses  the extent to which the user achieved his/her goal, understood what he/she was supposed to do for obtaining the service, he/she found the succession of the process steps logical and he/she was actively engaged to improve the service." ;
	skos:note	"This indicator has been discontinued starting from 2016" ;
	skos:topConceptOf	ns8:indicator .
ns1:e_gov_1e_ucg_su	rdf:type	skos:Concept ,
		ns2:Indicator ;
	skos:prefLabel	"1e User Centricity - Speed of Use" ;
	dct:source	ns5:egov_bench12_17 ;
	skos:notation	"e_gov_1e_ucg_su" ;
	skos:altLabel	"1e User Centricity - Speed of Use" ;
	ns6:membership	ns22:e_gov_1e_ucg_su ;
	skos:definition	"Quality assessment researchers indicating if  the online process steps for obtaining a public service could be completed within reasonable amount of time. It assesses the extent to which citizens or businesses are able to submit information to the authority (or information was pre-filled), the time needed to obtain the service and the extent to which the services were structured efficiently.  " ;
	skos:note	"This indicator has been discontinued starting from 2016" ;
	skos:topConceptOf	ns8:indicator .
ns1:e_gov_2_tg	rdf:type	skos:Concept ,
		ns2:Indicator ;
	skos:prefLabel	"2 Transparency" ;
	dct:source	ns5:egov_bench12_17 ;
	skos:notation	"e_gov_2_tg" ;
	skos:altLabel	"2 Transparency" ;
	ns6:membership	ns22:e_gov_2_tg ;
	skos:definition	"The extent to which governments are transparent with regard to:\na) the process of public service delivery\nb) their own responsibilities and performance\nc) the personal data involved in service delivery\nThis top-level benchmark evaluates the transparency of government authorities\u2019 operations, service delivery procedures as well as with regard to the consultation of personal data by public administrations." ;
	skos:note	"Composite indicator: simple average of (Transparency) Service Delivery, Public Organisations and Personal Data" ;
	skos:topConceptOf	ns8:indicator .
ns1:e_gov_2a_tg_sd	rdf:type	ns2:Indicator ,
		skos:Concept ;
	skos:prefLabel	"2a Transparency - Service delivery" ;
	dct:source	ns5:egov_bench12_17 ;
	skos:notation	"e_gov_2a_tg_sd" ;
	skos:altLabel	"2a Transparency - Service delivery" ;
	ns6:membership	ns22:e_gov_2a_tg_sd ;
	skos:definition	"The extent to which public administrations inform users about the public service itself, setting expectations on timeliness, process and delivery for citizens and entrepreneurs from the moment a user request a service until the service is delivered." ;
	skos:topConceptOf	ns8:indicator .
ns1:e_gov_2b_tg_po	rdf:type	ns2:Indicator ,
		skos:Concept ;
	skos:prefLabel	"2b Transparency - Public organisations" ;
	dct:source	ns5:egov_bench12_17 ;
	skos:notation	"e_gov_2b_tg_po" ;
	skos:altLabel	"2b Transparency - Public organisations" ;
	ns6:membership	ns22:e_gov_2b_tg_po ;
	skos:definition	"The extent to which public administrations publish information about their organisations (e.g. finance, organisational structure and responsibilities), and about their activities (e.g. the decision-making processes and regulations). " ;
	skos:topConceptOf	ns8:indicator .
ns1:e_gov_2c_tg_pd	rdf:type	ns2:Indicator ,
		skos:Concept ;
	skos:prefLabel	"2c Transparency - Personal data" ;
	dct:source	ns5:egov_bench12_17 ;
	skos:notation	"e_gov_2c_tg_pd" ;
	skos:altLabel	"2c Transparency - Personal data" ;
	ns6:membership	ns22:e_gov_2c_tg_pd ;
	skos:definition	"The extent to which governments proactively inform users about how, when, and by whom their personal data is being processed" ;
	skos:note	"In 2016, an additional question was added to the questionnaire for this indicator." ;
	skos:topConceptOf	ns8:indicator .
ns1:e_gov_3_cm	rdf:type	ns2:Indicator ,
		skos:Concept ;
	skos:prefLabel	"3 Citizen Mobility" ;
	dct:source	ns5:egov_bench12_17 ;
	skos:notation	"e_gov_3_cm" ;
	skos:altLabel	"3 Citizen Mobility" ;
	ns6:membership	ns22:e_gov_3_cm ;
	skos:definition	"The extent to which public services that are aimed at foreign  citizens are available online, usable, and implement eID and eDocument capabilities" ;
	skos:note	"Composite indicator:\n(2016-2017) weighted average of (Citizen Mobility) Online Availability (50%), Usability (25%), eID Cross Borders (12%) and eDocuments Cross Borders (12%).\n(2012-2015) weighted average of (Citizen Mobility) Online Availability (67%), Usability (17%), Ease of Use (8%) and Speed of Use (8%)\nBreak in series in 2016 (no data displayed for breakdown:Total 2016)." ;
	skos:topConceptOf	ns8:indicator .
ns1:e_gov_3a_cm_oa	rdf:type	ns2:Indicator ,
		skos:Concept ;
	skos:prefLabel	"3a Citizen Mobility - Online availability" ;
	dct:source	ns5:egov_bench12_17 ;
	skos:notation	"e_gov_3a_cm_oa" ;
	skos:altLabel	"3a Citizen Mobility - Online availability" ;
	ns6:membership	ns22:e_gov_3a_cm_oa ;
	skos:definition	"The extent to which a public service (or information concerning the service) aimed at foreign citizens  is available online." ;
	skos:topConceptOf	ns8:indicator .
ns1:e_gov_3b_cm_us	rdf:type	ns2:Indicator ,
		skos:Concept ;
	skos:prefLabel	"3b Citizen Mobility - Usability" ;
	dct:source	ns5:egov_bench12_17 ;
	skos:notation	"e_gov_3b_cm_us" ;
	skos:altLabel	"3b Citizen Mobility - Usability" ;
	ns6:membership	ns22:e_gov_3b_cm_us ;
	skos:definition	"Online support and help features on services aimed at foreign citizens." ;
	skos:topConceptOf	ns8:indicator .
ns1:e_gov_3c_cm_eidcb	rdf:type	ns2:Indicator ,
		skos:Concept ;
	skos:prefLabel	"3c Citizen Mobility - eID Cross Borders" ;
	dct:source	ns5:egov_bench12_17 ;
	skos:notation	"e_gov_3c_cm_eidcb" ;
	skos:altLabel	"3c Citizen Mobility - eID Cross Borders" ;
	ns6:membership	ns22:e_gov_3c_cm_eidcb ;
	skos:definition	"The possibility of using a foreign eID for accessing citizen services." ;
	skos:note	"New indicator, introduced in 2016." ;
	skos:topConceptOf	ns8:indicator .
ns1:e_gov_3d_cm_edoccb	rdf:type	ns2:Indicator ,
		skos:Concept ;
	skos:prefLabel	"3d Citizen Mobility - eDocuments Cross Borders" ;
	dct:source	ns5:egov_bench12_17 ;
	skos:notation	"e_gov_3d_cm_edoccb" ;
	skos:altLabel	"3d Citizen Mobility - eDocuments Cross Borders" ;
	ns6:membership	ns22:e_gov_3d_cm_edoccb ;
	skos:definition	"The possibility of sending/receiving eDocuments for a foreigner using citizen services" ;
	skos:note	"New indicator, introduced in 2016." ;
	skos:topConceptOf	ns8:indicator .
ns1:e_gov_3e_cm_eu	rdf:type	ns2:Indicator ,
		skos:Concept ;
	skos:prefLabel	"3e Citizen Mobility - Ease of Use" ;
	dct:source	ns5:egov_bench12_17 ;
	skos:notation	"e_gov_3e_cm_eu" ;
	skos:altLabel	"3e Citizen Mobility - Ease of Use" ;
	ns6:membership	ns22:e_gov_3e_cm_eu ;
	skos:definition	"Quality assessment by researchers indicating how intuitively and smoothly the online process steps for obtaining a public service can be completed by a foreign citizen.  It assesses  the extent to which the user achieved his/her goal, understood what he/she was supposed to do for obtaining the service, he/she found the succession of the process steps logical and he/she was actively engaged to improve the service." ;
	skos:note	"This indicator has been discontinued starting from 2016" ;
	skos:topConceptOf	ns8:indicator .
ns1:e_gov_3f_cm_su	rdf:type	ns2:Indicator ,
		skos:Concept ;
	skos:prefLabel	"3f Citizen Mobility - Speed of Use" ;
	dct:source	ns5:egov_bench12_17 ;
	skos:notation	"e_gov_3f_cm_su" ;
	skos:altLabel	"3f Citizen Mobility - Speed of Use" ;
	ns6:membership	ns22:e_gov_3f_cm_su ;
	skos:definition	"Quality assessment researchers indicating if  the online process steps for obtaining a public service could be completed within reasonable amount of time by a foreign citizen. It assesses the extent to which (foreign) citizens are able to submit information to the authority (or information was pre-filled), the time needed to obtain the service and the extent to which the services were structured efficiently.  " ;
	skos:note	"This indicator has been discontinued starting from 2016" ;
	skos:topConceptOf	ns8:indicator .
ns1:e_gov_4_bm	rdf:type	ns2:Indicator ,
		skos:Concept ;
	skos:prefLabel	"4 Business Mobility" ;
	dct:source	ns5:egov_bench12_17 ;
	skos:notation	"e_gov_4_bm" ;
	skos:altLabel	"4 Business Mobility" ;
	ns6:membership	ns22:e_gov_4_bm ;
	skos:definition	"The extent to which public services that are aimed at foreign  businesses are available online, usable, and implement eID and eDocument capabilities" ;
	skos:note	"Composite indicator:\n(2016-2017) weighted average of (Business Mobility) Online Availability (50%), Usability (25%), eID Cross Borders (12%) and eDocuments Cross Borders (12%).\n(2012-2015) weighted average of (Business Mobility) Online Availability (67%), Usability (17%), Ease of Use (8%) and Speed of Use (8%)\nBreak in series in 2016 (no data displayed for breakdown:Total 2016)." ;
	skos:topConceptOf	ns8:indicator .
ns1:e_gov_4a_bm_oa	rdf:type	ns2:Indicator ,
		skos:Concept ;
	skos:prefLabel	"4a Business Mobility - Online availability" ;
	dct:source	ns5:egov_bench12_17 ;
	skos:notation	"e_gov_4a_bm_oa" ;
	skos:altLabel	"4a Business Mobility - Online availability" ;
	ns6:membership	ns22:e_gov_4a_bm_oa ;
	skos:definition	"The extent to which a public service (or information concerning the service) aimed at foreign businesses  is available online." ;
	skos:topConceptOf	ns8:indicator .
ns1:e_gov_4c_bm_eidcb	rdf:type	ns2:Indicator ,
		skos:Concept ;
	skos:prefLabel	"4c Business Mobility - eID Cross Borders" ;
	dct:source	ns5:egov_bench12_17 ;
	skos:notation	"e_gov_4c_bm_eidcb" ;
	skos:altLabel	"4e Business Mobility - eID Cross Borders" ;
	ns6:membership	ns22:e_gov_4c_bm_eidcb ;
	skos:definition	"The possibility of using a foreign eID for accessing business services." ;
	skos:note	"New indicator, introduced in 2016." ;
	skos:topConceptOf	ns8:indicator .
ns1:e_gov_4d_bm_edoccb	rdf:type	ns2:Indicator ,
		skos:Concept ;
	skos:prefLabel	"4d Business Mobility - eDocuments Cross Borders" ;
	dct:source	ns5:egov_bench12_17 ;
	skos:notation	"e_gov_4d_bm_edoccb" ;
	skos:altLabel	"4f Business Mobility - eDocuments Cross Borders" ;
	ns6:membership	ns22:e_gov_4d_bm_edoccb ;
	skos:definition	"The possibility of sending/receiving eDocuments for a foreigner using business services" ;
	skos:note	"New indicator, introduced in 2016." ;
	skos:topConceptOf	ns8:indicator .
ns1:e_gov_4e_bm_eu	rdf:type	ns2:Indicator ,
		skos:Concept ;
	skos:prefLabel	"4e Business Mobility - Ease of Use" ;
	dct:source	ns5:egov_bench12_17 ;
	skos:notation	"e_gov_4e_bm_eu" ;
	skos:altLabel	"4g Business Mobility - Ease of Use" ;
	ns6:membership	ns22:e_gov_4e_bm_eu ;
	skos:definition	"Quality assessment by researchers indicating how intuitively and smoothly the online process steps for obtaining a public service can be completed by a foreign business.  It assesses  the extent to which the user achieved his/her goal, understood what he/she was supposed to do for obtaining the service, he/she found the succession of the process steps logical and he/she was actively engaged to improve the service." ;
	skos:note	"This indicator has been discontinued starting from 2016" ;
	skos:topConceptOf	ns8:indicator .
ns1:e_gov_4f_bm_su	rdf:type	ns2:Indicator ,
		skos:Concept ;
	skos:prefLabel	"4f Business Mobility - Speed of Use" ;
	dct:source	ns5:egov_bench12_17 ;
	skos:notation	"e_gov_4f_bm_su" ;
	skos:altLabel	"4h Business Mobility - Speed of Use" ;
	ns6:membership	ns22:e_gov_4f_bm_su ;
	skos:definition	"Quality assessment researchers indicating if  the online process steps for obtaining a public service could be completed within reasonable amount of time by a foreign business. It assesses the extent to which (foreign) businesses are able to submit information to the authority (or information was pre-filled), the time needed to obtain the service and the extent to which the services were structured efficiently.  " ;
	skos:note	"This indicator has been discontinued starting from 2016" ;
	skos:topConceptOf	ns8:indicator .
ns1:e_gov_5_ke	rdf:type	skos:Concept ,
		ns2:Indicator ;
	skos:prefLabel	"5 Key Enablers" ;
	dct:source	ns5:egov_bench12_17 ;
	skos:notation	"e_gov_5_ke" ;
	skos:altLabel	"5 Key Enablers" ;
	ns6:membership	ns22:e_gov_5_ke ;
	skos:definition	"The extent to which technical pre-conditions for eGovernment service provision are used. The key enablers used for measuring the quality of the services to businesses and citizens are:\na) Electronic Identification (eID)\nb) Electronic Documents (eDocuments)\nc) Authentic Sources\nd) Digital Post\ne) eSafe (now discontinued)\nf) Single Sign On (SSO) (now discontinued)" ;
	skos:note	"Composite indicator:\n(2016-2017) simple average of eID, eDocuments, Authentic Sources and Digital Post.\n(2012-2015) simple average of eID, eDocuments, Authentic Sources, eSafe and Single Sign On.\nBreak in series in 2016 as the  eSafe and Single Sign On are discontinued and Digital Post is added." ;
	skos:topConceptOf	ns8:indicator .
ns1:e_gov_5a_ke_eid	rdf:type	skos:Concept ,
		ns2:Indicator ;
	skos:prefLabel	"5a Key Enablers - eID" ;
	dct:source	ns5:egov_bench12_17 ;
	skos:notation	"e_gov_5a_ke_eid" ;
	skos:altLabel	"5a Key Enablers - eID" ;
	ns6:membership	ns22:e_gov_5a_ke_eid ;
	skos:definition	"Electronic Identification (eID) is a government-issued document for online identification, and authentication." ;
	skos:topConceptOf	ns8:indicator .
ns1:e_gov_5b_ke_edoc	rdf:type	skos:Concept ,
		ns2:Indicator ;
	skos:prefLabel	"5b Key Enablers - eDocuments" ;
	dct:source	ns5:egov_bench12_17 ;
	skos:notation	"e_gov_5b_ke_edoc" ;
	skos:altLabel	"5b Key Enablers - eDocuments" ;
	ns6:membership	ns22:e_gov_5b_ke_edoc ;
	skos:definition	"A document which has been authenticated by its issuer using any means recognised under applicable national law, specifically through the use of electronic signatures, e.g. not a regular pdf or word document." ;
	skos:topConceptOf	ns8:indicator .
ns1:e_gov_5c_ke_as	rdf:type	skos:Concept ,
		ns2:Indicator ;
	skos:prefLabel	"5c Key Enablers - Authentic sources" ;
	dct:source	ns5:egov_bench12_17 ;
	skos:notation	"e_gov_5c_ke_as" ;
	skos:altLabel	"5c Key Enablers - Authentic sources" ;
	ns6:membership	ns22:e_gov_5c_ke_as ;
	skos:definition	"Authentic Sources are base registries used by governments to automatically validate or fetch data relating to citizens or businesses." ;
	skos:topConceptOf	ns8:indicator .
ns1:e_gov_5d_ke_dp	rdf:type	skos:Concept ,
		ns2:Indicator ;
	skos:prefLabel	"5d Key Enablers - Digital Post" ;
	dct:source	ns5:egov_bench12_17 ;
	skos:notation	"e_gov_5d_ke_dp" ;
	skos:altLabel	"5d Key Enablers - Digital Post" ;
	ns6:membership	ns22:e_gov_5d_ke_dp ;
	skos:definition	"Assesses whether public authorities allow citizens to receive communications digitally only, and hence reducing paper mailings. Digital Post refers to the possibility that governments communicate electronically-only with citizens or entrepreneurs through e.g. personal mailboxes or other digital post solutions." ;
	skos:note	"New indicator, introduced in 2016." ;
	skos:topConceptOf	ns8:indicator .
ns1:e_gov_5e_ke_esafe	rdf:type	skos:Concept ,
		ns2:Indicator ;
	skos:prefLabel	"5e Key Enablers - eSafe" ;
	dct:source	ns5:egov_bench12_17 ;
	skos:notation	"e_gov_5e_ke_esafe" ;
	skos:altLabel	"5e Key Enablers - eSafe" ;
	ns6:membership	ns22:e_gov_5e_ke_esafe ;
	skos:definition	"A virtual repository for storing, administering and sharing personal electronic data and documents. It can be used to securely store personal documents in public service processes." ;
	skos:note	"This indicator has been discontinued starting from 2016" ;
	skos:topConceptOf	ns8:indicator .
ns1:e_gov_5f_ke_sso	rdf:type	skos:Concept ,
		ns2:Indicator ;
	skos:prefLabel	"5f Key Enablers - Single Sign On (SSO)" ;
	dct:source	ns5:egov_bench12_17 ;
	skos:notation	"e_gov_5f_ke_sso" ;
	skos:altLabel	"5f Key Enablers - Single Sign On (SSO)" ;
	ns6:membership	ns22:e_gov_5f_ke_sso ;
	skos:definition	"A functionality that allows users to get access to multiple websites without the need to log in multiple times." ;
	skos:note	"This indicator has been discontinued starting from 2016" ;
	skos:topConceptOf	ns8:indicator .
ns1:e_gov_ke	rdf:type	skos:Concept ,
		ns2:Indicator ;
	skos:prefLabel	"Key Enablers" ;
	dct:source	ns5:egov_bench14 ;
	skos:notation	"e_gov_ke" ;
	skos:altLabel	"Key Enablers" ;
	ns6:membership	ns22:e_gov_ke ;
	skos:definition	"Availability of Key Enablers such as electronic Identification (eID), electronic Documents, Authentic Sources as well as Digital Post (newly introduced in 2017)" ;
	skos:note	"The degree to which key enablers (eID, eDocuments. Authentic sources, Digital Post) are available for interaction with public administration for the life events (Business, Family, Job, Studying)" ;
	skos:topConceptOf	ns8:indicator .
ns1:e_gov_opa	rdf:type	skos:Concept ,
		ns2:Indicator ;
	skos:prefLabel	"Openness of Public Administrations" ;
	dct:source	ns5:egov_bench15 ;
	skos:notation	"e_gov_opa" ;
	skos:altLabel	"Openness of Public Administrations" ;
	ns6:membership	ns22:e_gov_opa ;
	skos:definition	"Openness of Member States in regards to Open Data, freedom of expression, free media and freedom of association." ;
	skos:note	"Composed indicator made of open data (DESI) and voice and accountability (World Bank indicator)" ;
	skos:topConceptOf	ns8:indicator .
ns1:e_gov_osc	rdf:type	skos:Concept ,
		ns2:Indicator ;
	skos:prefLabel	"Online Service Completion" ;
	dct:source	ns5:e_gov_bench ;
	skos:notation	"e_gov_osc" ;
	skos:altLabel	"Online Service Completion" ;
	ns6:membership	ns22:e_gov_osc ;
	skos:definition	"Share of the steps in a Public Service life event that can be completed online (Online availability sub-indicator for User centricity of the eGovernment benchmark)" ;
	skos:note	"The indicator was measuring: Basic and Extended services for National services only till 2019. From 2020 the new indicator, \"Digital Public Services for Citizens\", was introduced. Together with the \"Digital Public Services for Business' they are fully covering the spectrum of online services. \nThe data was recalculated to include EU27 Average." ;
	skos:topConceptOf	ns8:indicator .
ns1:e_gov_pff	rdf:type	skos:Concept ,
		ns2:Indicator ;
	skos:prefLabel	"Pre-filled forms (up to 2020)" ;
	dct:source	ns5:e_gov_bench ;
	skos:notation	"e_gov_pff" ;
	skos:altLabel	"Pre-filled forms (up to 2020)" ;
	ns6:membership	ns22:e_gov_pff ;
	skos:definition	"Amount of data that is pre-filled in Public Services' online forms (Authentic sources Key Enabler indicator of eGovernment benchmark)" ;
	skos:topConceptOf	ns8:indicator .
ns1:e_igov	rdf:type	skos:Concept ,
		ns2:Indicator ;
	skos:prefLabel	"Enterprises interacting online with public authorities" ;
	dct:source	ns5:estat_isoc_bde15dec ;
	skos:notation	"e_igov" ;
	skos:altLabel	"Use of eGovernment services - enterprises" ;
	ns6:membership	ns20:e_igov ;
	skos:definition	"Use of internet for interaction with public authorities, in the last calendar year before the survey, includes: obtaining information or forms from websites, returning filled in forms, following administrative procedures completely electronically or offering products in public authorities' electronic procurement sustems (eTendering)." ;
	skos:note	"Enterprises with 10 or more persons employed, all manufacturing and service sectors, excluding the financial sector. Break in series in 2011 and 2012 because the structure of the question has changed. Breaks in series because until 2008 sectors follow economic activities according to NACE Rev 1.1 and from 2009 data are based on NACE Rev.2. Since 2010 data include also sector S 95.1-Repair of computers and communication equipment." ;
	skos:topConceptOf	ns8:indicator .
ns1:e_igov2pr	rdf:type	skos:Concept ,
		ns2:Indicator ;
	skos:prefLabel	"Enterprises submitting a proposal in a public electronic tender system (eProcurement)" ;
	dct:source	ns5:estat_isoc_bde15dec ;
	skos:notation	"e_igov2pr" ;
	skos:altLabel	"Use of eProcurement services - enterprises" ;
	ns6:membership	ns20:e_igov2pr ;
	skos:definition	" Tender proposals should have been submitted in the system itself and not by email, in the last calendar year before the survey. " ;
	skos:note	"Data from previous years are not comparable because the structure of the question has changed. Enterprises with 10 or more persons employed, carrying out this activity over the internet in the last calendar year before the survey. All manufacturing and service sectors, excluding the financial sector. " ;
	skos:topConceptOf	ns8:indicator .
ns1:e_igovrt	rdf:type	skos:Concept ,
		ns2:Indicator ;
	skos:prefLabel	"Enterprises returning filled in forms to public authorities, over the internet" ;
	dct:source	ns5:estat_isoc_bde15dec ;
	skos:notation	"e_igovrt" ;
	skos:altLabel	"Returning filled forms to eGov services - enterprises" ;
	ns6:membership	ns20:e_igovrt ;
	skos:definition	"Activity carried out over the internet, in the last calendar year before the survey." ;
	skos:note	"Enterprises with 10 or more persons employed. Break in series in 2011 and 2012 because the question has changed. All manufacturing and service sectors, excluding the financial sector. Breaks in series because until 2008 economic activities according to NACE Rev 1.1 and from 2009 data are based on NACE Rev.2. Since Since 2010 data include also sector S 95.1-Repair of computers and communication equipment." ;
	skos:topConceptOf	ns8:indicator .
ns1:e_inv	rdf:type	ns2:Indicator ,
		skos:Concept ;
	skos:prefLabel	"Enterprises sending or receiving e-invoices in a format suitable for automatic processing" ;
	dct:source	ns5:estat_isoc_bde15disc ;
	skos:notation	"e_inv" ;
	skos:altLabel	"Sending or receiving of e-Invoices" ;
	ns6:membership	ns20:e_inv ;
	skos:definition	"The indicator refers to sending/receiving invoices in an agreed standard format (as EDIFACT, XML, etc) which allows their automatic processing, without the individual message being manually typed" ;
	skos:note	"Important break in series due to a more detailed question since 2011. Enterprises with 10 or more persons employed. All manufacturing and service sectors, excluding the financial sector. Breaks in series because until 2008 economic activities according to NACE Rev 1.1 and from 2009 data are based on NACE Rev.2. Since 2010 data include also sector S 95.1-Repair of computers and communication equipment." ;
	skos:topConceptOf	ns8:indicator .
ns1:e_invsnd	rdf:type	ns2:Indicator ,
		skos:Concept ;
	skos:prefLabel	"Enterprises sending e-invoices (derived indicator, until 2017)" ;
	dct:source	ns5:estat_isoc_bde15disc ;
	skos:notation	"e_invsnd" ;
	skos:altLabel	"Enterprises sending e-invoices (until 2017)" ;
	ns6:membership	ns7:e_invsnd ;
	skos:definition	"The indicator refers to sending invoices in an agreed standard format (as EDIFACT, XML, etc) which allows their automatic processing, without the individual message being manually typed. Eurostat variable e_inv3sbg_ap_gt0" ;
	skos:note	"Break in series in 2011 because of a new more precise question. Break in series in 2014 because of introduction of a limitation to invoices sent to business or public organisations." ;
	skos:topConceptOf	ns8:indicator .
ns1:e_ispdf_ge30	rdf:type	ns2:Indicator ,
		skos:Concept ;
	skos:prefLabel	"Enterprises having a fast fixed broadband connection" ;
	dct:source	ns5:estat_isoc_ci_eu_en2 ;
	skos:notation	"e_ispdf_ge30" ;
	skos:altLabel	"Enterprises having a fast fixed broadband connection" ;
	ns6:membership	ns17:e_ispdf_ge30 ;
	skos:definition	"The maximum contracted download speed of the fastest fixed internet connection is at least 30 Mb/s" ;
	skos:topConceptOf	ns8:indicator .
ns1:e_ispdfokx	rdf:type	ns2:Indicator ,
		skos:Concept ;
	skos:prefLabel	"The speed of the fixed connection to internet  is not sufficient for the actual needs of the enterprise" ;
	dct:source	ns5: ;
	skos:notation	"e_ispdfokx" ;
	skos:altLabel	"Internet fixed connection speed is not sufficient" ;
	ns6:membership	ns17:e_ispdfokx ;
	skos:definition	"Number of enterprises reporting that the speed of the fixed connection(s) to the internet is usually not sufficient for the actual  needs of the enterprise " ;
	skos:note	"Enterprises with 10 or more persons employed. All manufacturing and service sectors, excluding the financial sector. Breaks in series because until 2008 economic activities according to NACE Rev 1.1 and from 2009 data are based on NACE Rev.2. Since 2010 data include also sector S 95.1-Repair of computers and communication equipment." ;
	skos:topConceptOf	ns8:indicator .
ns1:e_ispdfokx_ge100	rdf:type	ns2:Indicator ,
		skos:Concept ;
	skos:prefLabel	"The speed of the fixed connection to internet (at least 100 Mb/s) is not sufficient for the actual needs of the enterprise" ;
	dct:source	ns5: ;
	skos:notation	"e_ispdfokx_ge100" ;
	skos:altLabel	"Internet fixed connection speed of 100Mb/s is not sufficient" ;
	ns6:membership	ns17:e_ispdfokx_ge100 ;
	skos:definition	"Number of enterprises reporting that the speed of the fixed connection(s) to the internet (at least 100 Mb/s) is usually not sufficient for the actual  needs of the enterprise " ;
	skos:note	"Enterprises with 10 or more persons employed. All manufacturing and service sectors, excluding the financial sector. Breaks in series because until 2008 economic activities according to NACE Rev 1.1 and from 2009 data are based on NACE Rev.2. Since 2010 data include also sector S 95.1-Repair of computers and communication equipment." ;
	skos:topConceptOf	ns8:indicator .
ns1:e_it_mext	rdf:type	ns2:Indicator ,
		skos:Concept ;
	skos:prefLabel	"Enterprises where ICT functions are mainly performed by external suppliers" ;
	dct:source	ns5:estat_isoc_ci_eu_en2 ;
	skos:notation	"e_it_mext" ;
	skos:altLabel	"Enterprises where ICT functions are mainly performed by external suppliers" ;
	ns6:membership	ns27:e_it_mext ;
	skos:definition	"The majority of ICT functions, out of a list of seven, are mainly performed by external suppliers and not by own employees or by ICT specialist in parent or affiliate enterprises. The functions include: maintenance of ICT infrastructures, support for office software, development and support for web solutions or business management software/systems (e.g. ERP, CRM, HR, databases), security and data protection." ;
	skos:note	"Detailed results are available in the Eurostat table <a href=\"http://appsso.eurostat.ec.europa.eu/nui/show.do?dataset=isoc_ci_eu_en2&lang=en\">ISOC_CI_EU_EN2</a>." ;
	skos:topConceptOf	ns8:indicator .
ns1:e_itsp2	rdf:type	ns2:Indicator ,
		skos:Concept ;
	skos:prefLabel	"Enterprises employing ICT specialists" ;
	dct:source	ns5:estat_isoc_ci_eu_en2 ;
	skos:notation	"e_itsp2" ;
	skos:altLabel	"Enterprises employing ICT specialists" ;
	ns6:membership	ns27:e_itsp2 ;
	skos:definition	"ICT specialists are employees for whom ICT is the main job. For example, to develop, operate or maintain ICT systems or applications." ;
	skos:note	"Limited comparability between 2007 and 2012 because of changes in the wording of the question. Enterprises with 10 or more persons employed. All manufacturing and service sectors, excluding the financial sector." ;
	skos:topConceptOf	ns8:indicator .
ns1:e_itspvac2	rdf:type	ns2:Indicator ,
		skos:Concept ;
	skos:prefLabel	"Enterprises reporting hard-to-fill vacancies for jobs requiring ICT specialist skills" ;
	dct:source	ns5:estat_isoc_ci_eu_en2 ;
	skos:notation	"e_itspvac2" ;
	skos:altLabel	"Enterprises reporting hard-to-fill vacancies for ICT specialist" ;
	ns6:membership	ns27:e_itspvac2 ;
	skos:definition	" Hard-to-fill vacancies during the previous calendar year refer to a range of situations in which enterprises find it difficult to find persons with particular skills (hard-to-fill vacancies due to skills shortage)." ;
	skos:note	"Limited comparability between 2007 and 2012 because of changes in the wording of the question. Enterprises with 10 or more persons employed. All manufacturing and service sectors, excluding the financial sector." ;
	skos:topConceptOf	ns8:indicator .
ns1:e_itt2	rdf:type	ns2:Indicator ,
		skos:Concept ;
	skos:prefLabel	"Enterprise provided training to their personnel to develop/upgrade their ICT skills" ;
	dct:source	ns5:estat_isoc_ske_ittn2 ;
	skos:notation	"e_itt2" ;
	skos:altLabel	"Enterprise provided training to their personnel to develop/upgrade their ICT skills" ;
	ns6:membership	ns27:e_itt2 ;
	skos:definition	"Detailed results are available in the Eurostat table <a href=\"http://appsso.eurostat.ec.europa.eu/nui/show.do?dataset=isoc_ske_ittn2&lang=en\">ISOC_SKE_ITTN2</a>." ;
	skos:topConceptOf	ns8:indicator .
ns1:e_pmd	rdf:type	ns2:Indicator ,
		skos:Concept ;
	skos:prefLabel	"Enterprises providing portable devices to some of their persons employed" ;
	dct:source	ns5:estat_isoc_bde15b_e ;
	skos:notation	"e_pmd" ;
	skos:altLabel	"Enterprises providing portable devices to persons employed" ;
	ns6:membership	ns30:e_pmd ;
	skos:definition	"The devices (portable computers, tablets, smartphones, PDA phones, etc.) should be provided for business use and the enterprises pay for all or at least up to a limit the subscription and the use costs." ;
	skos:note	"The 2011 question was limited to portable devices using at least 3G technology to connect to the internet. Enterprises with 10 or more persons employed. All manufacturing and service sectors, excluding the financial sector." ;
	skos:topConceptOf	ns8:indicator .
ns1:e_pmd_app	rdf:type	ns2:Indicator ,
		skos:Concept ;
	skos:prefLabel	"Enterprises using mobile Internet to run business applications" ;
	dct:source	ns5:estat-ent ;
	skos:notation	"e_pmd_app" ;
	skos:altLabel	"Enterprises using mobile Internet to run business applications" ;
	ns6:membership	ns7:e_pmd_app ;
	skos:definition	"Mobile connection to the Internet for business use to use dedicated business software applications" ;
	skos:topConceptOf	ns8:indicator .
ns1:e_ra	rdf:type	ns2:Indicator ,
		skos:Concept ;
	skos:prefLabel	"Enterprises providing persons employed a remote access to the enterprise's e-mail system, documents or applications" ;
	dct:source	ns5:estat-ent ;
	skos:notation	"e_ra" ;
	skos:altLabel	"Enterprises providing persons employed a remote access to the IT system" ;
	ns6:membership	ns7:e_ra ;
	skos:note	"Enterprises with 10 or more persons employed. All manufacturing and service sectors, excluding the financial sector." ;
	skos:topConceptOf	ns8:indicator .
ns1:e_rfac	rdf:type	ns2:Indicator ,
		skos:Concept ;
	skos:prefLabel	"Enterprises using RFID technologies for person identification or access control" ;
	dct:source	ns5:estat_isoc_bde15dth ;
	skos:notation	"e_rfac" ;
	skos:altLabel	"Enterprises using RFID for person identification or access control" ;
	ns6:membership	ns7:e_rfac ;
	skos:definition	"RFID tags or transponders are devices that can be applied to or incorporated into a product or object and transmits data via radiowaves." ;
	skos:topConceptOf	ns8:indicator .
ns1:e_rfid	rdf:type	ns2:Indicator ,
		skos:Concept ;
	skos:prefLabel	"Enterprises using Radio Frequency Identification (RFID) technologies" ;
	dct:source	ns5:estat_isoc_bde15dth ;
	skos:notation	"e_rfid" ;
	skos:altLabel	"Use of Radio Frequency Identification (RFID) technologies" ;
	ns6:membership	ns7:e_rfid ;
	skos:definition	"RFID tags or transponders are devices that can be applied to or incorporated into a product or object and transmits data via radiowaves. The indicator includes their use for person identification, for tracking of supply chain and inventory or for after-sales product identification." ;
	skos:note	"Enterprises with 10 or more persons employed. All manufacturing and service sectors, excluding the financial sector. Since 2010 data include also sector S95.1-Repair of computers and communication equipment. Biennial indicator not collected in 2010." ;
	skos:topConceptOf	ns8:indicator .
ns1:e_rfpsas	rdf:type	ns2:Indicator ,
		skos:Concept ;
	skos:prefLabel	"Enterprises using RFID for product identification" ;
	dct:source	ns5:estat_isoc_bde15dth ;
	skos:notation	"e_rfpsas" ;
	skos:altLabel	"Enterprises using RFID for product identification" ;
	ns6:membership	ns7:e_rfpsas ;
	skos:definition	"RFID tags or transponders are devices that can be applied to or incorporated into a product or object and transmits data via radiowaves. The indicator includes their use for tracking of supply chain and inventory or for after-sales product identification." ;
	skos:topConceptOf	ns8:indicator .
ns1:e_secpol1	rdf:type	ns2:Indicator ,
		skos:Concept ;
	skos:prefLabel	"Enterprises with a formally defined ICT security policy" ;
	dct:source	ns5:estat_isoc_ci_eu_en2 ;
	skos:notation	"e_secpol1" ;
	skos:altLabel	"Enterprises with a formally defined ICT security policy" ;
	ns6:membership	ns33:e_secpol1 ;
	skos:topConceptOf	ns8:indicator .
ns1:e_sisc	rdf:type	skos:Concept ,
		ns2:Indicator ;
	skos:prefLabel	"Enterprises sharing electronic information on the supply chain" ;
	dct:source	ns5:estat_isoc_bde15disc ;
	skos:notation	"e_sisc" ;
	skos:altLabel	"Electronic Supply Chain Management" ;
	ns6:membership	ns7:e_sisc ;
	skos:definition	"The indicator refers to sending/receiving all type of information on the supply chain (e.g. inventory levels, production plans, forecasts, progress of delivery) via computer networks or via websites, but excluding manually typed e-mail messages. " ;
	skos:note	"Enterprises with 10 or more persons employed. All manufacturing and service sectors, excluding the financial sector. Breaks in series because untill 2008 economic activities according to NACE Rev 1.1 and from 2009 data are based on NACE Rev.2. Since 2010 data include also sector 95.1-Repair of computers and communication equipment. Biennial indicator not collected in 2011." ;
	skos:topConceptOf	ns8:indicator .
ns1:e_sisorp	rdf:type	skos:Concept ,
		ns2:Indicator ;
	skos:prefLabel	"Enterprises that share internally electronic information on sales/purchases" ;
	dct:source	ns5:estat_isoc_bde15dec ;
	skos:notation	"e_sisorp" ;
	skos:altLabel	"Integration of internal processes (orders)" ;
	ns6:membership	ns20:e_sisorp ;
	skos:definition	"Information on sales/purchases is shared electronically and automatically with the software used for any internal function as: the management of inventory levels, the accounting system, the production management or the distribution management. " ;
	skos:note	"Enterprises with 10 or more persons employed. All manufacturing and service sectors, excluding the financial sector. Breaks in series because until 2008 economic activities according to NACE Rev 1.1 and from 2009 data are based on NACE Rev.2. Since 2010 data include also sector S 95.1-Repair of computers and communication equipment." ;
	skos:topConceptOf	ns8:indicator .
ns1:e_sm_any	rdf:type	skos:Concept ,
		ns2:Indicator ;
	skos:prefLabel	"Enterprises using social media" ;
	dct:source	ns5:estat_isoc_ci_eu_en2 ;
	skos:notation	"e_sm_any" ;
	skos:altLabel	"Enterprises using social media" ;
	ns6:membership	ns7:e_sm_any ;
	skos:definition	"Enterprises using at least one of the following social media: social networks, enterprise's blog or microblog, multimedia content sharing websites, wiki based knowledge sharing tools. Using social media means that the enterprise have a user profile, an account or a user license depending on the requirements and the type of the social media." ;
	skos:topConceptOf	ns8:indicator .
ns1:e_sm_ge2	rdf:type	skos:Concept ,
		ns2:Indicator ;
	skos:prefLabel	"Use two or more social media" ;
	dct:source	ns5:estat_isoc_ci_eu_en2 ;
	skos:notation	"e_sm_ge2" ;
	skos:altLabel	"Enterprises using two or more social media" ;
	ns6:membership	ns7:e_sm_ge2 ;
	skos:definition	"Enterprises using two or more of the following social media: social networks, enterprise's blog or microblog, multimedia content sharing websites, wiki based knowledge sharing tools. Using social media means that the enterprise have a user profile, an account or a user license depending on the requirements and the type of the social media." ;
	skos:topConceptOf	ns8:indicator .
ns1:e_web	rdf:type	skos:Concept ,
		ns2:Indicator ;
	skos:prefLabel	"Enterprises having a web site or homepage" ;
	dct:source	ns5:estat_isoc_ci_eu_en2 ;
	skos:notation	"e_web" ;
	skos:altLabel	"Enterprises having a web site or homepage" ;
	ns6:membership	ns7:e_web ;
	skos:note	"Enterprises with 10 or more persons employed. All manufacturing and service sectors, excluding the financial sector. Breaks in series because until 2008 economic activities according to NACE Rev 1.1 and from 2009 data are based on NACE Rev.2. Since 2010 data include also sector S95.1-Repair of computers and communication equipment." ;
	skos:topConceptOf	ns8:indicator .
ns1:e_webf2	rdf:type	skos:Concept ,
		ns2:Indicator ;
	skos:prefLabel	"Enterprises having a website with some sophisticated functionalities" ;
	dct:source	ns5:estat_isoc_ci_eu_en2 ;
	skos:notation	"e_webf2" ;
	skos:altLabel	"Enterprises having a website with some sophisticated functionalities" ;
	ns6:membership	ns7:e_webf2 ;
	skos:definition	"Website having at least one of the following four functionalities : product catalogues or price lists (webacc), possibilities for visitors to customise or design the products (webctm), order tracking available online (webot) or personalised content in the website for regular/repeated visitors (webper)." ;
	skos:note	"Enterprises with 10 or more persons employed. All manufacturing and service sectors, excluding the financial sector. Breaks in series because until 2008 economic activities according to NACE Rev 1.1 and from 2009 data are based on NACE Rev.2. Since 2010 data include also sector S95.1-Repair of computers and communication equipment." ;
	skos:topConceptOf	ns8:indicator .
ns1:e_wsel25	rdf:type	skos:Concept ,
		ns2:Indicator ;
	skos:prefLabel	"Enterprises selling over 25% via a website or apps" ;
	dct:source	ns5: ;
	skos:notation	"e_wsel25" ;
	skos:altLabel	"Enterprises selling over 25% via a website or apps" ;
	ns6:membership	ns21:e_wsel25 ;
	skos:definition	"The sales made via website or apps, during the previous calendar year, should represent at least 25% of the total turnover value (in monetary terms, excluding VAT)." ;
	skos:note	"Enterprises with 10 or more persons employed. All manufacturing and service sectors, excluding the financial sector. Breaks in series because until 2008 economic activities according to NACE Rev 1.1 and from 2009 data are based on NACE Rev.2. Since 2010 data include also sector S 95.1-Repair of computers and communication equipment." ;
	skos:topConceptOf	ns8:indicator .
ns1:e_wsel50	rdf:type	skos:Concept ,
		ns2:Indicator ;
	skos:prefLabel	"Enterprises selling over 50% via a website or apps" ;
	dct:source	ns5: ;
	skos:notation	"e_wsel50" ;
	skos:altLabel	"Enterprises selling over 50% via a website or apps" ;
	ns6:membership	ns21:e_wsel50 ;
	skos:definition	"The sales made via website or apps, during the previous calendar year, should represent at least 50% of the total turnover value (in monetary terms, excluding VAT)." ;
	skos:note	"Enterprises with 10 or more persons employed. All manufacturing and service sectors, excluding the financial sector. Breaks in series because until 2008 economic activities according to NACE Rev 1.1 and from 2009 data are based on NACE Rev.2. Since 2010 data include also sector S 95.1-Repair of computers and communication equipment." ;
	skos:topConceptOf	ns8:indicator .
ns1:edigint2015	rdf:type	skos:Concept ,
		ns2:Indicator ;
	skos:prefLabel	"Digital Intensity score for Enterprises (DII v1)" ;
	dct:source	ns5:estat-ent ;
	skos:notation	"edigint2015" ;
	skos:altLabel	"Digital Intensity score for Enterprises (DII v1)" ;
	ns6:membership	ns7:edigint2015 ;
	skos:definition	"The Digital Intensity score is based on counting how many out of 12 technologies are used by each enterprise. Then they are divided into four clusters of digital intensity: Very Low (scores 0-3), Low (score 4-6), High (score 7-9), Very High (score 10-12)." ;
	skos:note	"The DII composition varies between different survey years, depending on the questions included in the survey. The exact composition for the different survey years can be found at https://circabc.europa.eu/ui/group/89577311-0f9b-4fc0-b8c2-2aaa7d3ccb91/library/30b83b9c-3d0c-4086-bf52-77905e19b4eb/details." ;
	skos:topConceptOf	ns8:indicator .
ns1:employment_ict	rdf:type	skos:Concept ,
		ns2:Indicator ;
	skos:prefLabel	"Employment of the ICT sector" ;
	dct:source	ns5:jrc_ict_randd ;
	skos:notation	"employment_ict" ;
	skos:altLabel	"Employment of the ICT sector" ;
	ns6:membership	ns25:employment_ict ;
	skos:definition	"Number of persons employed. In the System of National Accounts (SNA) this is defined as all persons, both employees and self-employed, engaged in some productive activity that falls within the production boundary of the SNA and that is undertaken by a resident institutional unit." ;
	skos:topConceptOf	ns8:indicator .
ns1:eoa_nn_films	rdf:type	skos:Concept ,
		ns2:Indicator ;
	skos:prefLabel	"Non-national European films in cinemas" ;
	dct:source	ns5:eoa_yearbook2014 ;
	skos:notation	"eoa_nn_films" ;
	skos:altLabel	"Non-national European Films market share in EU cinemas" ;
	ns6:membership	ns13:eoa_nn_films ;
	skos:topConceptOf	ns8:indicator .
ns1:eoa_tvchannels_tarfor	rdf:type	skos:Concept ,
		ns2:Indicator ;
	skos:prefLabel	"Linear TV channels established in a Member State and targeting foreign countries" ;
	dct:source	ns5:eoa_yearbook2014 ;
	skos:notation	"eoa_tvchannels_tarfor" ;
	skos:altLabel	"Linear TV channels targeting foreign countries" ;
	ns6:membership	ns13:eoa_tvchannels_tarfor ;
	skos:note	"page 125" ;
	skos:topConceptOf	ns8:indicator .
ns1:eoa_vod_estab_otheu	rdf:type	skos:Concept ,
		ns2:Indicator ;
	skos:prefLabel	"Video on Demand services available in the country but established in another EU country" ;
	dct:source	ns5:eoa_smart12-26 ;
	skos:notation	"eoa_vod_estab_otheu" ;
	skos:altLabel	"VoD services available, established in another EU country" ;
	ns6:membership	ns13:eoa_vod_estab_otheu ;
	skos:definition	"Video on demand (VoD) services (all genre except adult) available in a Member State, but established in another EU country" ;
	skos:topConceptOf	ns8:indicator .
ns1:epsi_score	rdf:type	skos:Concept ,
		ns2:Indicator ;
	skos:prefLabel	"Public Sector Information scoreboard" ;
	dct:source	ns5:epsiplatform ;
	skos:notation	"epsi_score" ;
	skos:altLabel	"Public Sector Information scoreboard" ;
	ns6:membership	ns22:epsi_score ;
	skos:definition	"The PSI Scoreboard is a \u2018crowdsourced\u2019 tool to measure the status of Open Data and PSI re-use throughout the EU. It does NOT monitor government policies, but aims to assess the overall PSI re-use situation, which includes the open data community's activities." ;
	skos:topConceptOf	ns8:indicator .
ns1:eun_computers	rdf:type	skos:Concept ,
		ns2:Indicator ;
	skos:prefLabel	"Computers for educational purposes" ;
	dct:source	ns5:eun12 ;
	skos:notation	"eun_computers" ;
	skos:altLabel	"Computers for educational purposes" ;
	ns6:membership	ns24:eun_computers ;
	skos:definition	"Computers used for educational purposes include desktop, laptop, netbook or tablet computer, whether or not connected to the internet" ;
	skos:topConceptOf	ns8:indicator .
ns1:eun_web	rdf:type	skos:Concept ,
		ns2:Indicator ;
	skos:prefLabel	"Schools having a website" ;
	dct:source	ns5:eun12 ;
	skos:notation	"eun_web" ;
	skos:altLabel	"Schools having a website" ;
	ns6:membership	ns24:eun_web ;
	skos:definition	"Own home page or web site available at school." ;
	skos:topConceptOf	ns8:indicator .
ns1:foa_cit	rdf:type	ns2:Indicator ,
		skos:Concept ;
	skos:prefLabel	"Basic public services for citizens, which are fully available online" ;
	dct:source	ns5:capgemini ;
	skos:notation	"foa_cit" ;
	skos:altLabel	"Availability of eGovernment services - citizens" ;
	ns6:membership	ns20:foa_cit ;
	skos:definition	"Percentage of public services for citizens out of a basket of 12 basic services (income taxes, job search, social security benefits, personal documents, car registration, building permissions, declaration to police, public libraries, certificates, enrolment in higher education, announcement of moving, health-related services) for which the entire procedure can be completed online" ;
	skos:note	"Collected until 2010." ;
	skos:topConceptOf	ns8:indicator .
ns1:foa_ent	rdf:type	ns2:Indicator ,
		skos:Concept ;
	skos:prefLabel	"Basic public services for enterprises, which are fully available online" ;
	dct:source	ns5:capgemini ;
	skos:notation	"foa_ent" ;
	skos:altLabel	"Availability of eGovernment services - enterprises" ;
	ns6:membership	ns20:foa_ent ;
	skos:definition	"Percentage of public services for enterprises out of a basket of 8 basic services (social contributions, corporate tax, VAT, company registration, statistical data, customs declaration, environment-related permits, public procurement) for which the entire procedure can be completed online" ;
	skos:note	"Collected until 2010." ;
	skos:topConceptOf	ns8:indicator .
ns1:fp7_ict_artic	rdf:type	ns2:Indicator ,
		skos:Concept ;
	skos:prefLabel	"Articles resulting from FP7 funded projects in ICT" ;
	dct:source	ns5:smart11_39 ;
	skos:notation	"fp7_ict_artic" ;
	skos:altLabel	"Articles from FP7 ICT projects" ;
	ns6:membership	ns31:fp7_ict_artic ;
	skos:definition	"Articles in journals reported through annual surveys of ongoing ICT research projects carried out by the European Commission - DG CONNECT. Outputs reported by participants have been validated in Elsevier\u2019s Scopus databases by UNU-MERIT \u2013 Maastricht University under the service contract SMART 2011/0039 funded by the European Commission - DG CONNECT" ;
	skos:note	"It covers FP7 ICT projects started before October 2013. The indicator is not expected to evolve regularly year by year, due to the coverage of thematic areas by calls which may differ from one year to another. Annual figures should therefore be interpreted with caution." ;
	skos:topConceptOf	ns8:indicator .
ns1:fp7_ict_pat	rdf:type	ns2:Indicator ,
		skos:Concept ;
	skos:prefLabel	"Patents resulting from FP7 funded projects in ICT" ;
	dct:source	ns5:smart11_39 ;
	skos:notation	"fp7_ict_pat" ;
	skos:altLabel	"Patents from FP7 ICT projects" ;
	ns6:membership	ns31:fp7_ict_pat ;
	skos:definition	"Patents reported through annual surveys of ongoing ICT research projects carried out by the European Commission - DG CONNECT. Outputs reported by participants have been validated in EPO PATSTAT and Espacenet databases by UNU-MERIT \u2013 Maastricht University under the service contract SMART 2011/0039 funded by the European Commission - DG CONNECT" ;
	skos:note	"It covers FP7 ICT projects started before October 2013. The indicator is not expected to evolve regularly year by year, due to the coverage of thematic areas by calls which may differ from one year to another. Annual figures should therefore be interpreted with caution." ;
	skos:topConceptOf	ns8:indicator .
ns1:fp7_ict_pub	rdf:type	ns2:Indicator ,
		skos:Concept ;
	skos:prefLabel	"Publications resulting from FP7 funded projects in ICT" ;
	dct:source	ns5:smart11_39 ;
	skos:notation	"fp7_ict_pub" ;
	skos:altLabel	"Publications from FP7 ICT projects" ;
	ns6:membership	ns31:fp7_ict_pub ;
	skos:definition	"Publications reported through annual surveys of ongoing ICT research projects carried out by the European Commission - DG CONNECT. Outputs reported by participants have been validated in Elsevier\u2019s Scopus databases by UNU-MERIT \u2013 Maastricht University under the service contract SMART 2011/0039 funded by the European Commission - DG CONNECT. \n* It includes articles in journals and trade journals, conference proceedings, books, book series" ;
	skos:note	"It covers FP7 ICT projects started before October 2013. The indicator is not expected to evolve regularly year by year, due to the coverage of thematic areas by calls which may differ from one year to another. Annual figures should therefore be interpreted with caution." ;
	skos:topConceptOf	ns8:indicator .
ns1:fp7ict_afxp	rdf:type	ns2:Indicator ,
		skos:Concept ;
	skos:prefLabel	"Average EC funding per participation in FP7-ICT projects" ;
	dct:source	ns5:mis ;
	skos:notation	"fp7ict_afxp" ;
	skos:altLabel	"FP7 Average EC funding per participation" ;
	ns6:membership	ns31:fp7ict_afxp ;
	skos:definition	"EC funding is the funding committed by the European Commission through grant agreements signed during the reference year. The indicator measure the average EC funding attributed to each partner participation in a specific project." ;
	skos:topConceptOf	ns8:indicator .
ns1:fp7ict_cofin	rdf:type	ns2:Indicator ,
		skos:Concept ;
	skos:prefLabel	"FP7 EC effective cofinancing rate" ;
	dct:source	ns5:mis ;
	skos:notation	"fp7ict_cofin" ;
	skos:altLabel	"FP7 EC cofinancing rate" ;
	ns6:membership	ns31:fp7ict_cofin ;
	skos:definition	"The cofinancing rate is the % of projects total costs which are covered by EC funding grants. Figures include all partners and third parties (as subcontractors)." ;
	skos:topConceptOf	ns8:indicator .
ns1:fp7ict_ec_funding	rdf:type	ns2:Indicator ,
		skos:Concept ;
	skos:prefLabel	"EC funding to participants in FP7-ICT projects" ;
	dct:source	ns5:mis ;
	skos:notation	"fp7ict_ec_funding" ;
	skos:altLabel	"EC funding to FP7-ICT projects" ;
	ns6:membership	ns31:fp7ict_ec_funding ;
	skos:definition	"Value of European Commission funding committed through grant agreements signed, during the reference year, with participants in ICT research projects under the EU's Seventh Framework Programme (FP7). Projects under negotiation are not included." ;
	skos:topConceptOf	ns8:indicator .
ns1:fp7ict_ec_funding_prc	rdf:type	ns2:Indicator ,
		skos:Concept ;
	skos:prefLabel	"EC funding to private commercial organisations in FP7-ICT projects" ;
	dct:source	ns5:mis ;
	skos:notation	"fp7ict_ec_funding_prc" ;
	skos:altLabel	"EC funding to private commercial organisations in FP7-ICT projects" ;
	ns6:membership	ns31:fp7ict_ec_funding_prc ;
	skos:definition	"Value of European Commission funding committed through grant agreements signed, during the reference year, with private commercial organisations (SMEs and large enterprises) participating in ICT research projects under the EU's Seventh Framework Programme (FP7) - Cooperation and Capacities (e-infrastructures). " ;
	skos:topConceptOf	ns8:indicator .
ns1:fp7ict_ec_funding_smes	rdf:type	ns2:Indicator ,
		skos:Concept ;
	skos:prefLabel	"EC funding granted to SMEs in FP7-ICT projects" ;
	dct:source	ns5:mis ;
	skos:notation	"fp7ict_ec_funding_smes" ;
	skos:altLabel	"EC funding to SMEs in FP7-ICT projects" ;
	ns6:membership	ns31:fp7ict_ec_funding_smes ;
	skos:definition	"Value of European Commission funding committed through grant agreements signed, during the reference year, with SMEs participating in ICT research projects under the EU's Seventh Framework Programme (FP7) - Cooperation and Capacities (e-infrastructures). " ;
	skos:topConceptOf	ns8:indicator .
ns1:fp7ict_newentry	rdf:type	ns2:Indicator ,
		skos:Concept ;
	skos:prefLabel	"Number of distinct organisations participating in FP7-ICT projects for the first time" ;
	dct:source	ns5:mis ;
	skos:notation	"fp7ict_newentry" ;
	skos:altLabel	"Number of NEW organisations in FP7-ICT projects" ;
	ns6:membership	ns31:fp7ict_newentry ;
	skos:definition	"The first call of FP7 ICT was in 2007 and all participants are considered as new ones. For each of the following years are counted only the organisations participating for the first time in FP7 ICT calls." ;
	skos:topConceptOf	ns8:indicator .
ns1:fp7ict_organisations	rdf:type	ns2:Indicator ,
		skos:Concept ;
	skos:prefLabel	"Number of distinct organisations participating in FP7-ICT projects" ;
	dct:source	ns5:mis ;
	skos:notation	"fp7ict_organisations" ;
	skos:altLabel	"Number of participants in FP7-ICT projects" ;
	ns6:membership	ns31:fp7ict_organisations ;
	skos:definition	"Organisations participating in FP7 ICT calls for research projects (Cooperation and Capacities and e-infrastructures programs) during the reference year." ;
	skos:topConceptOf	ns8:indicator .
ns1:fp7ict_particip	rdf:type	ns2:Indicator ,
		skos:Concept ;
	skos:prefLabel	"Total number of participations in FP7-ICT projects" ;
	dct:source	ns5:mis ;
	skos:notation	"fp7ict_particip" ;
	skos:altLabel	"FP7 Total number of participations" ;
	ns6:membership	ns31:fp7ict_particip ;
	skos:definition	"Each project has multiple partners participating and each partner can participate in multiple projects. For each participation there could be an EC funding (some participations do not receive EC funding). Third parties are included as partners, receiveing or not EU funding." ;
	skos:topConceptOf	ns8:indicator .
ns1:fp7ict_particip_prc	rdf:type	ns2:Indicator ,
		skos:Concept ;
	skos:prefLabel	"Total number of participations  by private commercial organisations in FP7-ICT projects" ;
	dct:source	ns5:mis ;
	skos:notation	"fp7ict_particip_prc" ;
	skos:altLabel	"Total number of private commercial organisations'participations in FP7-ICT projects" ;
	ns6:membership	ns31:fp7ict_particip_prc ;
	skos:definition	"Total number of participations by private commercial organisations (SMEs and large enterprises)in ICT research projects under the EU's Seventh Framework Programme (FP7) - Cooperation and Capacities (e-infrastructures). Each project has multiple partners participating and each partner can participate in multiple projects. " ;
	skos:topConceptOf	ns8:indicator .
ns1:fp7ict_particip_smes	rdf:type	ns2:Indicator ,
		skos:Concept ;
	skos:prefLabel	"Total number of participations by SMEs in FP7-ICT projects" ;
	dct:source	ns5:mis ;
	skos:notation	"fp7ict_particip_smes" ;
	skos:altLabel	"Total number of SMEs' participations in FP7-ICT projects" ;
	ns6:membership	ns31:fp7ict_particip_smes ;
	skos:definition	"Total number by participations of SMEs in ICT research projects under the EU's Seventh Framework Programme (FP7) - Cooperation and Capacities (e-infrastructures). Each project has multiple partners participating and each partner can participate in multiple projects. " ;
	skos:topConceptOf	ns8:indicator .
ns1:fp7ict_totcost	rdf:type	ns2:Indicator ,
		skos:Concept ;
	skos:prefLabel	"Total cost of FP7-ICT projects" ;
	dct:source	ns5:mis ;
	skos:notation	"fp7ict_totcost" ;
	skos:altLabel	"Total cost of FP7-ICT projects" ;
	ns6:membership	ns31:fp7ict_totcost ;
	skos:definition	"Value of the total cost of the ICT research projects for which a grant agreement was signed in the reference year, under the EU's Seventh Framework Programme (FP7). Total cost of the project is the sum of participants' total costs." ;
	skos:topConceptOf	ns8:indicator .
ns1:gbaord	rdf:type	skos:Concept ,
		ns2:Indicator ;
	skos:prefLabel	"GBAORD - Government budget appropriations or outlays for research and development" ;
	dct:source	ns5:jrc_ict_randd ;
	skos:notation	"gbaord" ;
	skos:altLabel	"Public R&D expediture (GBAORD)" ;
	ns6:membership	ns31:gbaord ;
	skos:definition	"GBAORD include all appropriations (government spending) given to R&D in central (or federal) government budgets. Provincial (or State) government posts are only included if the contribution is significant. Local government funds are excluded" ;
	skos:note	"From 2006 onwards figures were revised and updated by PREDICT 2 project" ;
	skos:topConceptOf	ns8:indicator .
ns1:gbaord_ict	rdf:type	skos:Concept ,
		ns2:Indicator ;
	skos:prefLabel	"Public ICT R&D spending (GBAORD in the field of ICT)" ;
	dct:source	ns5:jrc_ict_randd ;
	skos:notation	"gbaord_ict" ;
	skos:altLabel	"Public ICT R&D spending " ;
	ns6:membership	ns31:gbaord_ict ;
	skos:definition	"Estimate of the ICT share in existing disaggregated GBAORD data, based on the assumption that the share of research in the ICT field in GBAORD expenditure is proportional to the share of ICT specialists in the R&D labour cost. Methodology developped and implemented by JRC-IPTS." ;
	skos:note	"From 2006 onwards figures were revised and updated by PREDICT 2 project" ;
	skos:topConceptOf	ns8:indicator .
ns1:gdp	rdf:type	skos:Concept ,
		ns2:Indicator ;
	skos:prefLabel	"GDP - Gross domestic product at market prices" ;
	dct:source	ns5:estat_nama_gdp_c ;
	skos:notation	"gdp" ;
	skos:altLabel	"GDP at market prices" ;
	ns6:membership	ns15:gdp ;
	skos:definition	"Eurostat estimation of GDP and main components - Current prices [nama_gdp_c]" ;
	skos:topConceptOf	ns8:indicator .
ns1:h2020_cofin	rdf:type	skos:Concept ,
		ns2:Indicator ;
	skos:prefLabel	"H2020 effective cofinancing rate" ;
	dct:source	ns5:corda ;
	skos:notation	"h2020_cofin" ;
	skos:altLabel	"H2020 cofinancing rate" ;
	ns6:membership	ns31:h2020_cofin ;
	skos:definition	"The cofinancing rate is the % of projects total costs which are covered by EC funding grants. " ;
	skos:topConceptOf	ns8:indicator .
ns1:h2020_ec_funding	rdf:type	skos:Concept ,
		ns2:Indicator ;
	skos:prefLabel	"Total EC funding to participants in H2020 ICT projects" ;
	dct:source	ns5:corda ;
	skos:notation	"h2020_ec_funding" ;
	skos:altLabel	"Total EC funding to H2020 ICT projects" ;
	ns6:membership	ns31:h2020_ec_funding ;
	skos:definition	"Value of European Commission funding committed through grant agreements signed, during the reference year, with participants in ICT research projects under Horizon 2020 (LEIT ICT, Excellent Science, Societal Challenges 1, 6 and 7). Projects under negotiation are not included." ;
	skos:topConceptOf	ns8:indicator .
ns1:h2020_newentry	rdf:type	skos:Concept ,
		ns2:Indicator ;
	skos:prefLabel	"Number of distinct organisations participating in H2020 ICT projects for the first time" ;
	dct:source	ns5:corda ;
	skos:notation	"h2020_newentry" ;
	skos:altLabel	"Number of new organisations in H2020 projects" ;
	ns6:membership	ns31:h2020_newentry ;
	skos:definition	"Organisations participating for the first time in H2020 ICT calls, and which have not participated in FP7 ICT calls during 2007-2013 period." ;
	skos:topConceptOf	ns8:indicator .
ns1:h2020_organisations	rdf:type	skos:Concept ,
		ns2:Indicator ;
	skos:prefLabel	"Number of distinct organisations participating in H2020 ICT projects" ;
	dct:source	ns5:corda ;
	skos:notation	"h2020_organisations" ;
	skos:altLabel	"H2020 Total number of organisations" ;
	ns6:membership	ns31:h2020_organisations ;
	skos:definition	"Organisations participating in H2020 ICT projects during the reference year." ;
	skos:topConceptOf	ns8:indicator .
ns1:h2020_particip	rdf:type	skos:Concept ,
		ns2:Indicator ;
	skos:prefLabel	"Total number of participations in H2020 ICT projects" ;
	dct:source	ns5:corda ;
	skos:notation	"h2020_particip" ;
	skos:altLabel	"H2020 Total number of participations" ;
	ns6:membership	ns31:h2020_particip ;
	skos:definition	"Each project has multiple partners participating and each partner can participate in multiple projects. For each participation there could be an EC funding (some participations do not receive EC funding). " ;
	skos:topConceptOf	ns8:indicator .
ns1:h2020_totcost	rdf:type	skos:Concept ,
		ns2:Indicator ;
	skos:prefLabel	"Total cost of H2020 ICT projects" ;
	dct:source	ns5:corda ;
	skos:notation	"h2020_totcost" ;
	skos:altLabel	"Total cost of H2020 ICT projects" ;
	ns6:membership	ns31:h2020_totcost ;
	skos:definition	"Value of the total cost of the ICT research projects for which a grant agreement was signed in the reference year, under the Horizon 2020 LEIT ICT, Excellent Science, Societal Challenges 1, 6 and 7). Total cost of the project is the sum of participants' total costs." ;
	skos:topConceptOf	ns8:indicator .
ns1:h2020ict_afxp	rdf:type	skos:Concept ,
		ns2:Indicator ;
	skos:prefLabel	"Average EC funding per participation in H2020 ICT projects" ;
	dct:source	ns5:corda ;
	skos:notation	"h2020ict_afxp" ;
	skos:altLabel	"H2020 Average EC funding per participation" ;
	ns6:membership	ns31:h2020ict_afxp ;
	skos:definition	"EC funding is the funding committed by the European Commission through grant agreements signed during the reference year. The indicator measures the average EC funding attributed to each partner participation in a specific project." ;
	skos:topConceptOf	ns8:indicator .
ns1:h_bbfix	rdf:type	skos:Concept ,
		ns2:Indicator ;
	skos:prefLabel	"Households with fixed broadband connection" ;
	dct:source	ns5:estat_isoc_bde15b_h ;
	skos:notation	"h_bbfix" ;
	skos:altLabel	"Households with fixed broadband connection" ;
	ns6:membership	ns17:h_bbfix ;
	skos:definition	"Household internet connection type: fixed broadband" ;
	skos:topConceptOf	ns8:indicator .
ns1:h_broad	rdf:type	skos:Concept ,
		ns2:Indicator ;
	skos:prefLabel	"Households having a broadband connection" ;
	dct:source	ns5:estat_isoc_bde15b_h ;
	skos:notation	"h_broad" ;
	skos:altLabel	"Households with a broadband connection" ;
	ns6:membership	ns17:h_broad ;
	skos:definition	"Broadband connection used by the household includes: DSL, wired fixed (cable, fiber, Ethernet, PLC), fixed wireless (satellite, WiFi, WiMax) and mobile wireless (3G/UMTS)." ;
	skos:note	"Scope includes Households with at least one member aged 16-74. " ;
	skos:topConceptOf	ns8:indicator .
ns1:h_iacc	rdf:type	skos:Concept ,
		ns2:Indicator ;
	skos:prefLabel	"Households with access to the Internet at home" ;
	dct:source	ns5:estat_isoc_bde15b_h ;
	skos:notation	"h_iacc" ;
	skos:altLabel	"Households with access to the Internet at home" ;
	ns6:membership	ns29:h_iacc ;
	skos:definition	"Any member of the household has access to the Internet at home" ;
	skos:note	"Scope includes Households with at least one member aged 16-74." ;
	skos:topConceptOf	ns8:indicator .
ns1:h_xcost	rdf:type	skos:Concept ,
		ns2:Indicator ;
	skos:prefLabel	"Households that have no access to Internet at home, because the costs are too high" ;
	dct:source	ns5:estat-hh ;
	skos:notation	"h_xcost" ;
	skos:altLabel	"Households with no access to Internet at home, because the costs are too high" ;
	ns6:membership	ns16:h_xcost ;
	skos:definition	"Households that have no access to Internet at home, because the costs are too high" ;
	skos:topConceptOf	ns8:indicator .
ns1:hie_use_ex_admin	rdf:type	skos:Concept ,
		ns2:Indicator ;
	skos:prefLabel	"GPs exchanging medical patient data with other healthcare providers and professionals" ;
	dct:source	ns5:bench_gp ;
	skos:notation	"hie_use_ex_admin" ;
	skos:altLabel	"GPs exchanging medical patient data with other healthcare providers and professionals" ;
	ns6:membership	ns23:hie_use_ex_admin ;
	skos:definition	"Percentatge of general practitioners using electronic networks to exchange medical patient data with other healthcare providers and professionals" ;
	skos:topConceptOf	ns8:indicator .
ns1:hie_use_pharm	rdf:type	skos:Concept ,
		ns2:Indicator ;
	skos:prefLabel	"GPs using electronic networks to transfer prescriptions to pharmacists" ;
	dct:source	ns5:bench_gp ;
	skos:notation	"hie_use_pharm" ;
	skos:altLabel	"GPs using electronic networks to transfer prescriptions to pharmacists" ;
	ns6:membership	ns23:hie_use_pharm ;
	skos:definition	"Percentatge of general practitioners using electronic networks to transfer prescriptions to pharmacists" ;
	skos:topConceptOf	ns8:indicator .
ns1:househ	rdf:type	ns2:Indicator ,
		skos:Concept ;
	skos:prefLabel	"Number of households" ;
	dct:source	ns5:estat-hh ;
	skos:notation	"househ" ;
	skos:altLabel	"Number of households" ;
	ns6:membership	ns15:househ ;
	skos:definition	"Estimation of the number of Households with at least one member aged 16-74, for the purpose of the survey on ICT usage by individuals and households." ;
	skos:topConceptOf	ns8:indicator .
ns1:households	rdf:type	ns2:Indicator ,
		skos:Concept ;
	skos:prefLabel	"Number of private Households" ;
	dct:source	ns5:estat_lfst_hhnhwhtc ;
	skos:notation	"households" ;
	skos:altLabel	"Number of private Households" ;
	ns6:membership	ns15:households ;
	skos:definition	"Number of private households (Eurostat table lfst_hhnhwhtc)" ;
	skos:topConceptOf	ns8:indicator .
ns1:i_atsw	rdf:type	ns2:Indicator ,
		skos:Concept ;
	skos:prefLabel	"Individuals using anti-tracking software" ;
	dct:source	ns5:estat_isoc_cisci_prv ;
	skos:notation	"i_atsw" ;
	skos:altLabel	"Individuals using anti-tracking software" ;
	ns6:membership	ns33:i_atsw ;
	skos:definition	"Individuals using anti-tracking software" ;
	skos:topConceptOf	ns8:indicator .
ns1:i_barr1x	rdf:type	ns2:Indicator ,
		skos:Concept ;
	skos:prefLabel	"Individuals who did not encounter problems when buying/ordering goods or services over the internet for private use" ;
	dct:source	ns5:estat_isoc_ec_iprb ;
	skos:notation	"i_barr1x" ;
	skos:altLabel	"Individuals who had no problems buying/ordering goods or services over the internet for private use" ;
	ns6:membership	ns21:i_barr1x ;
	skos:definition	"Individuals who had no problems buying/ordering goods or services over the internet for private use" ;
	skos:topConceptOf	ns8:indicator .
ns1:i_bfeu	rdf:type	ns2:Indicator ,
		skos:Concept ;
	skos:prefLabel	"Individuals ordering goods or services online, from sellers from other EU countries" ;
	dct:source	ns5:estat_isoc_bde15cbc ;
	skos:notation	"i_bfeu" ;
	skos:altLabel	"Cross-border eCommerce" ;
	ns6:membership	ns21:i_bfeu ;
	skos:definition	"Individuals that ordered goods or services for private use over the Internet in the last 12 months from sellers from other EU countries" ;
	skos:topConceptOf	ns8:indicator .
ns1:i_bgood	rdf:type	ns2:Indicator ,
		skos:Concept ;
	skos:prefLabel	"Individuals ordering content or software delivered online or offline" ;
	dct:source	ns5:estat_isoc_ec_ibuy ;
	skos:notation	"i_bgood" ;
	skos:altLabel	"Buying: content (any delivery mode)" ;
	ns6:membership	ns21:i_bgood ;
	skos:definition	"Online purchases: films/music or books/magazines/e-learning material or computer software" ;
	skos:topConceptOf	ns8:indicator .
ns1:i_bgoodo	rdf:type	ns2:Indicator ,
		skos:Concept ;
	skos:prefLabel	"Individuals ordering content or software that were delivered or upgraded online" ;
	dct:source	ns5:estat_isoc_ec_ibuy ;
	skos:notation	"i_bgoodo" ;
	skos:altLabel	"Buying : online content" ;
	ns6:membership	ns21:i_bgoodo ;
	skos:definition	"The online content and software include: films, music, books, magazines, e-learning material, computer software, video games, that were ordered/bought over the Internet in the last 12 months, for non-work use." ;
	skos:topConceptOf	ns8:indicator .
ns1:i_blt12	rdf:type	ns2:Indicator ,
		skos:Concept ;
	skos:prefLabel	"Individuals ordering goods or services online" ;
	dct:source	ns5:estat_isoc_ec_ibuy ;
	skos:notation	"i_blt12" ;
	skos:altLabel	"Ordering goods or services online" ;
	ns6:membership	ns21:i_blt12 ;
	skos:definition	"Individuals carrying out this activity over the internet in the last 12 months, for private use." ;
	skos:topConceptOf	ns8:indicator .
ns1:i_bpgood	rdf:type	ns2:Indicator ,
		skos:Concept ;
	skos:prefLabel	"Individuals ordering physical goods online" ;
	dct:source	ns5:estat_isoc_ec_ibuy ;
	skos:notation	"i_bpgood" ;
	skos:altLabel	"Buying : physical goods online" ;
	ns6:membership	ns21:i_bpgood ;
	skos:definition	"Individuals that have ordered online any of the following physical goods: food/groceries, household goods, medicine, clothes/sports, computer hardware, electronic equipment." ;
	skos:topConceptOf	ns8:indicator .
ns1:i_bserv	rdf:type	ns2:Indicator ,
		skos:Concept ;
	skos:prefLabel	"Individuals ordering services online" ;
	dct:source	ns5:estat_isoc_ec_ibuy ;
	skos:notation	"i_bserv" ;
	skos:altLabel	"Buying : services online" ;
	ns6:membership	ns21:i_bserv ;
	skos:definition	"Individuals that have ordered online any of the following services: telecommunications services, share/insurance/financial, holiday accomodation, travel arrangements, tickets for events." ;
	skos:topConceptOf	ns8:indicator .
ns1:i_cc	rdf:type	skos:Concept ,
		ns2:Indicator ;
	skos:prefLabel	"Used internet storage space to save documents, pictures, music, video or other files" ;
	dct:source	ns5:estat_isoc_cicce_use ;
	skos:notation	"i_cc" ;
	skos:altLabel	"Used internet storage space" ;
	ns6:membership	ns28:i_cc ;
	skos:definition	"Used internet storage space to save documents, pictures, music, video or other files" ;
	skos:topConceptOf	ns8:indicator .
ns1:i_cisk_sfjob	rdf:type	skos:Concept ,
		ns2:Indicator ;
	skos:prefLabel	"workers who judge their current ICT skills sufficient for changing job within a year" ;
	dct:source	ns5:estat_isoc_sk_cskl_i ;
	skos:notation	"i_cisk_sfjob" ;
	skos:altLabel	"ICT skills perceived as sufficient for the labour market" ;
	ns6:membership	ns20:i_cisk_sfjob ;
	skos:definition	"Individuals with an occupation as employees, self-employed or family workers, were asked if they judge their current computer or Internet skills to be sufficient (yes/not) if they were to look for a job or change job within a year." ;
	skos:topConceptOf	ns8:indicator .
ns1:i_cisk_sfjobx	rdf:type	skos:Concept ,
		ns2:Indicator ;
	skos:prefLabel	"workers who judge their current ICT skills insufficient for changing job within a year" ;
	dct:source	ns5:estat_isoc_sk_cskl_i ;
	skos:notation	"i_cisk_sfjobx" ;
	skos:altLabel	"ICT skills perceived as insufficient for the labour market" ;
	ns6:membership	ns27:i_cisk_sfjobx ;
	skos:definition	"Individuals with an occupation as employees, self-employed or family workers, were asked if they judge their current computer or Internet skills to be sufficient (yes/not) if they were to look for a job or change job within a year." ;
	skos:topConceptOf	ns8:indicator .
ns1:i_cook	rdf:type	skos:Concept ,
		ns2:Indicator ;
	skos:prefLabel	"Individuals who know that cookies can be used to trace movements of people on the internet" ;
	dct:source	ns5:estat_isoc_cisci_prv ;
	skos:notation	"i_cook" ;
	skos:altLabel	"Awareness about cookies" ;
	ns6:membership	ns33:i_cook ;
	skos:definition	"Individuals who know that cookies can be used to trace movements of people on the internet" ;
	skos:topConceptOf	ns8:indicator .
ns1:i_cprg	rdf:type	skos:Concept ,
		ns2:Indicator ;
	skos:prefLabel	"Individuals who have written a computer program using a specialised programming language" ;
	dct:source	ns5:estat_isoc_sk_cskl_i ;
	skos:notation	"i_cprg" ;
	skos:altLabel	"Have written a computer program" ;
	ns6:membership	ns27:i_cprg ;
	skos:definition	"Individuals who have written a computer program using a specialised programming language. " ;
	skos:note	"Break in series because before 2015 the activity could have been carried out ever, but since 2015 it refers to the last 12 months ." ;
	skos:topConceptOf	ns8:indicator .
ns1:i_csk_ge_me	rdf:type	skos:Concept ,
		ns2:Indicator ;
	skos:prefLabel	"Individuals with medium or high computer skills (3 or more of 6 computer activities)" ;
	dct:source	ns5:estat_isoc_sk_cskl_i ;
	skos:notation	"i_csk_ge_me" ;
	skos:altLabel	"Individuals with medium or high computer skills" ;
	ns6:membership	ns20:i_csk_ge_me ;
	skos:definition	"The indicator counts individuals having ever carried out at least 3 of the following 6 activities: coping or moving a file or folder, using copy and paste tools, using basic arithmetic formula in a spreadsheet, compressing (or zipping) files, connecting and installing new devices, writing a computer program using a specialised programming language. Only those having ever used a computer were proposed the question." ;
	skos:topConceptOf	ns8:indicator .
ns1:i_cweb	rdf:type	skos:Concept ,
		ns2:Indicator ;
	skos:prefLabel	"Individuals who have created a Web page" ;
	dct:source	ns5:estat_isoc_sk_iskl_i ;
	skos:notation	"i_cweb" ;
	skos:altLabel	"Have created a Web page" ;
	ns6:membership	ns20:i_cweb ;
	skos:definition	"The activity could have been carried out ever. Only those having ever used the internet were proposed the question." ;
	skos:topConceptOf	ns8:indicator .
ns1:i_dsk_bab	rdf:type	skos:Concept ,
		ns2:Indicator ;
	skos:prefLabel	"DSI 2015-2019 Individuals with at least basic digital skills" ;
	dct:source	ns5:estat_isoc_sk_dskl_i ;
	skos:notation	"i_dsk_bab" ;
	skos:altLabel	"DSI 2015-2019 - At least basic digital skills" ;
	ns6:membership	ns26:i_dsk_bab ;
	skos:definition	"Persons that have been using internet during last 3 months are attributed a score on four digital competence domains: information, communication, content-creation and problem-solving, depending the activities they have been able to do. The scores in each domain are basic, above basic and below basic. Individuals not using internet are classified without digital skills. To be classified \"basic or above basic\" on the overall indicator an individual has to have basic or above basic skills in all the four Digital Competence domains included in the index: information, communication, content-creation and problem-solving." ;
	skos:note	"Detailed results are available in the Eurostat table <a href=\"http://appsso.eurostat.ec.europa.eu/nui/show.do?dataset=isoc_sk_dskl_i&lang=en\">ISOC_SK_DSKL_I</a>. Consult the <a href=\"https://ec.europa.eu/digital-agenda/en/news/new-comprehensive-digital-skills-indicator\"> methodological note</a> on DG CONNECT newsroom." ;
	skos:topConceptOf	ns8:indicator .
ns1:i_dsk_c_bab	rdf:type	skos:Concept ,
		ns2:Indicator ;
	skos:prefLabel	"DSI 2015-2019 Individuals with at least basic digital skills in Communication domain" ;
	dct:source	ns5:estat_isoc_sk_dskl_i ;
	skos:notation	"i_dsk_c_bab" ;
	skos:altLabel	"DSI 2015-2019 - Communication Domain - At least Basic  Skills" ;
	ns6:membership	ns26:i_dsk_c_bab ;
	skos:definition	"These skills refer to the ability to communicate in digital environments, share resources through online tools, link with others and collaborate through digital tools, interact with and participate in communities and networks, cross-cultural awareness. The indicator is based on four activities internet users have been able to do online during previous 3 months. The scores are basic, above basic and none. Individuals not using internet are classified without digital skills." ;
	skos:note	"Detailed results are available in the Eurostat table <a href=\"http://appsso.eurostat.ec.europa.eu/nui/show.do?dataset=isoc_sk_dskl_i&lang=en\">ISOC_SK_DSKL_I</a>. Consult the <a href=\"https://ec.europa.eu/digital-agenda/en/news/new-comprehensive-digital-skills-indicator\"> methodological note</a> on DG CONNECT newsroom." ;
	skos:topConceptOf	ns8:indicator .
ns1:i_dsk_i_bab	rdf:type	skos:Concept ,
		ns2:Indicator ;
	skos:prefLabel	"DSI 2015-2019 Individuals with at least basic digital skills in Information domain" ;
	dct:source	ns5:estat_isoc_sk_dskl_i ;
	skos:notation	"i_dsk_i_bab" ;
	skos:altLabel	"DSI 2015-2019 - Information Domain - At least Basic  Skills" ;
	ns6:membership	ns26:i_dsk_i_bab ;
	skos:definition	"Information processing skills refers to the ability to identify, locate, retrieve, store, organise and analyse digital information, judging its relevance and purpose. The indicator is based on five activities internet users have been able to do online during previous 3 months. The scores are basic, above basic and none. Individuals not using internet are classified without digital skills." ;
	skos:note	"Detailed results are available in the Eurostat table <a href=\"http://appsso.eurostat.ec.europa.eu/nui/show.do?dataset=isoc_sk_dskl_i&lang=en\">ISOC_SK_DSKL_I</a>. Consult the <a href=\"https://ec.europa.eu/digital-agenda/en/news/new-comprehensive-digital-skills-indicator\"> methodological note</a> on DG CONNECT newsroom." ;
	skos:topConceptOf	ns8:indicator .
ns1:i_dsk_ps_bab	rdf:type	skos:Concept ,
		ns2:Indicator ;
	skos:prefLabel	"DSI 2015-2019 Individuals with at least basic digital skills in Problem solving domain" ;
	dct:source	ns5:estat_isoc_sk_dskl_i ;
	skos:notation	"i_dsk_ps_bab" ;
	skos:altLabel	"DSI 2015-2019 - Problem Solving Domain - At least Basic  Skills" ;
	ns6:membership	ns26:i_dsk_ps_bab ;
	skos:definition	"Problem solving skills refers to the ability to identify digital needs and resources, make informed decisions as to which are the most appropriate digital tools according to the purpose or need, solve conceptual problems through digital means, creatively use technologies, solve technical problems, update one's own and others' competences. The indicator is based on three basic digital problems and familiarity with four online services internet users have been able to do during previous 3 months. The scores are basic, above basic and none. Individuals not using internet are classified without digital skills." ;
	skos:note	"Detailed results are available in the Eurostat table <a href=\"http://appsso.eurostat.ec.europa.eu/nui/show.do?dataset=isoc_sk_dskl_i&lang=en\">ISOC_SK_DSKL_I</a>. Consult the <a href=\"https://ec.europa.eu/digital-agenda/en/news/new-comprehensive-digital-skills-indicator\"> methodological note</a> on DG CONNECT newsroom." ;
	skos:topConceptOf	ns8:indicator .
ns1:i_dsk_s_bab	rdf:type	skos:Concept ,
		ns2:Indicator ;
	skos:prefLabel	"DSI 2015-2019 Individuals with at least basic digital skills in Software domain" ;
	dct:source	ns5:estat_isoc_sk_dskl_i ;
	skos:notation	"i_dsk_s_bab" ;
	skos:altLabel	"DSI 2015-2019 - Software Domain - At least Basic  Skills" ;
	ns6:membership	ns26:i_dsk_s_bab ;
	skos:definition	"Software skills for content manipulation refer to the ability to create and edit new content (from word processing to images and video); integrate and re-elaborate previous knowledge and content; produce creative expressions, media outputs and programming; deal with and apply intellectual property rights and licences. The indicator is based on six activities internet users have been able to do during previous 3 months. The scores are basic, above basic and none. Individuals not using internet are classified without digital skills." ;
	skos:note	"Detailed results are available in the Eurostat table <a href=\"http://appsso.eurostat.ec.europa.eu/nui/show.do?dataset=isoc_sk_dskl_i&lang=en\">ISOC_SK_DSKL_I</a>. Consult the <a href=\"https://ec.europa.eu/digital-agenda/en/news/new-comprehensive-digital-skills-indicator\"> methodological note</a> on DG CONNECT newsroom." ;
	skos:topConceptOf	ns8:indicator .
ns1:i_iday	rdf:type	skos:Concept ,
		ns2:Indicator ;
	skos:prefLabel	"Individuals who are frequent internet users (every day or almost every day)" ;
	dct:source	ns5:estat_isoc_bde15cua ;
	skos:notation	"i_iday" ;
	skos:altLabel	"Frequent internet users" ;
	ns6:membership	ns29:i_iday ;
	skos:definition	"Individuals using the internet every day or almost every day, in the last 3 months." ;
	skos:topConceptOf	ns8:indicator .
ns1:i_igov12rt	rdf:type	skos:Concept ,
		ns2:Indicator ;
	skos:prefLabel	"Individuals submitting completed forms to public authorities, over the internet, last 12 months" ;
	dct:source	ns5:estat_isoc_r_gov_i ;
	skos:notation	"i_igov12rt" ;
	skos:altLabel	"Citizens submitting filled forms to eGov services, last 12 months" ;
	ns6:membership	ns22:i_igov12rt ;
	skos:topConceptOf	ns8:indicator .
ns1:i_igovrt	rdf:type	skos:Concept ,
		ns2:Indicator ;
	skos:prefLabel	"sending filled forms to public authorities, over the internet, last 3 months" ;
	dct:source	ns5:estat_isoc_ci_ac_i ;
	skos:notation	"i_igovrt" ;
	skos:altLabel	"Sending filled forms to eGov services, last 3 months" ;
	ns6:membership	ns20:i_igovrt ;
	skos:note	"Indicator collected until 2010." ;
	skos:topConceptOf	ns8:indicator .
ns1:i_ihif	rdf:type	ns2:Indicator ,
		skos:Concept ;
	skos:prefLabel	"seeking online information about health" ;
	dct:source	ns5:estat_isoc_bde15cua ;
	skos:notation	"i_ihif" ;
	skos:altLabel	"Seeking health information" ;
	ns6:membership	ns23:i_ihif ;
	skos:definition	"Individuals using internet in the last 3 months, seeking information about health: injury, disease, nutrition, improving health, etc." ;
	skos:topConceptOf	ns8:indicator .
ns1:i_ilt12	rdf:type	ns2:Indicator ,
		skos:Concept ;
	skos:prefLabel	"Individuals who have used internet in the last 12 months" ;
	dct:source	ns5:estat_isoc_ci_ifp_iu ;
	skos:notation	"i_ilt12" ;
	skos:altLabel	"Internet used in the last 12 months" ;
	ns6:membership	ns29:i_ilt12 ;
	skos:topConceptOf	ns8:indicator .
ns1:i_isk_ge_me	rdf:type	ns2:Indicator ,
		skos:Concept ;
	skos:prefLabel	"Individuals with medium or high internet skills (3 or more of 6 internet activities)" ;
	dct:source	ns5:estat_isoc_sk_iskl_i ;
	skos:notation	"i_isk_ge_me" ;
	skos:altLabel	"Individuals with medium or high internet skills" ;
	ns6:membership	ns20:i_isk_ge_me ;
	skos:definition	"The indicator counts individuals having ever carried out at least 3 of the following 6 activities: using a search engine to find information, sending e-mails with attached files, posting messages to chatrooms, newsgroups or an online discussion forum, using the internet to make telephone calls, using peer-to-peer file sharing for exchanging movies or music, creating a webpage. Only those having ever used the internet were proposed the question." ;
	skos:topConceptOf	ns8:indicator .
ns1:i_iu3	rdf:type	ns2:Indicator ,
		skos:Concept ;
	skos:prefLabel	"Individuals who have used internet in the last 3 months" ;
	dct:source	ns5:estat_isoc_ci_ifp_iu ;
	skos:notation	"i_iu3" ;
	skos:altLabel	"Internet used in the last 3 months" ;
	ns6:membership	ns29:i_iu3 ;
	skos:topConceptOf	ns8:indicator .
ns1:i_iu3g	rdf:type	ns2:Indicator ,
		skos:Concept ;
	skos:prefLabel	"Individuals accessing the Internet through a mobile phone via UMTS (3G)" ;
	dct:source	ns5:estat_isoc_ci_im_i ;
	skos:notation	"i_iu3g" ;
	skos:altLabel	"Use of mobile phones to access the Internet" ;
	ns6:membership	ns30:i_iu3g ;
	skos:definition	"Individuals using a mobile phone or smart phone to access the internet, in the last 3 months. Since 2011 the question specify \"away from home or work\". Until 2012  the question was limited to \"via UMTS, HSDPA (3G or 3G+) connections\"." ;
	skos:note	"Break in series in 2011 and 2012 as the structure of the question has changed. Reconstructed time series using Eurostat variables: i_iu3g, i_iu3G1, i_iuhd_mph, i_iump_mph" ;
	skos:topConceptOf	ns8:indicator .
ns1:i_iubk	rdf:type	ns2:Indicator ,
		skos:Concept ;
	skos:prefLabel	"using online banking" ;
	dct:source	ns5:estat_isoc_ci_ac_i ;
	skos:notation	"i_iubk" ;
	skos:altLabel	"Online banking" ;
	ns6:membership	ns28:i_iubk ;
	skos:definition	"Individuals have used Internet, in the last 3 months, for Internet banking" ;
	skos:topConceptOf	ns8:indicator .
ns1:i_iueduif	rdf:type	ns2:Indicator ,
		skos:Concept ;
	skos:prefLabel	"looking online for information about education, training or course offers" ;
	dct:source	ns5:estat_isoc_ci_ac_i ;
	skos:notation	"i_iueduif" ;
	skos:altLabel	"Information about education & training" ;
	ns6:membership	ns28:i_iueduif ;
	skos:definition	"Individuals have used Internet, in the last 3 months, for looking for information about education, training or course offers" ;
	skos:topConceptOf	ns8:indicator .
ns1:i_iugm	rdf:type	ns2:Indicator ,
		skos:Concept ;
	skos:prefLabel	"playing or downloading games, images, films or music" ;
	dct:source	ns5:estat_isoc_bde15cua ;
	skos:notation	"i_iugm" ;
	skos:altLabel	"Games, images, films or music" ;
	ns6:membership	ns13:i_iugm ;
	skos:definition	"Individuals have used Internet, in the last 3 months, for playing or downloading games, images films or music" ;
	skos:note	"Biennial indicator not collected in 2011" ;
	skos:topConceptOf	ns8:indicator .
ns1:i_iugov	rdf:type	ns2:Indicator ,
		skos:Concept ;
	skos:prefLabel	"interacting online with public authorities, last 3 months" ;
	dct:source	ns5:estat_isoc_ci_ac_i ;
	skos:notation	"i_iugov" ;
	skos:altLabel	"Use of eGovernment services, last 3 months" ;
	ns6:membership	ns20:i_iugov ;
	skos:definition	"Individuals have used Internet, in the last 3 months, for interaction with public authorities. It includes obtaining information from public authorities web sites, downloading official forms and sending filled in forms." ;
	skos:topConceptOf	ns8:indicator .
ns1:i_iugov12	rdf:type	ns2:Indicator ,
		skos:Concept ;
	skos:prefLabel	"Individuals interacting online with public authorities, last 12 months" ;
	dct:source	ns5:estat_isoc_r_gov_i ;
	skos:notation	"i_iugov12" ;
	skos:altLabel	"Citizens' use of eGovernment services, last 12 months" ;
	ns6:membership	ns22:i_iugov12 ;
	skos:definition	"Individuals have used Internet, in the last 12 months, for interaction with public authorities. It includes obtaining information from public authorities web sites, OR downloading official forms OR sending filled in forms." ;
	skos:topConceptOf	ns8:indicator .
ns1:i_iuif	rdf:type	ns2:Indicator ,
		skos:Concept ;
	skos:prefLabel	"looking for information about goods and services online" ;
	dct:source	ns5:estat_isoc_ci_ac_i ;
	skos:notation	"i_iuif" ;
	skos:altLabel	"Information about goods and services" ;
	ns6:membership	ns28:i_iuif ;
	skos:definition	"Individuals have used Internet, in the last 3 months, for finding information about goods and services" ;
	skos:topConceptOf	ns8:indicator .
ns1:i_iujob	rdf:type	ns2:Indicator ,
		skos:Concept ;
	skos:prefLabel	"looking online for a job or sending a job application" ;
	dct:source	ns5:estat_isoc_bde15cua ;
	skos:notation	"i_iujob" ;
	skos:altLabel	"Looking for a job, sending a job application" ;
	ns6:membership	ns28:i_iujob ;
	skos:definition	"Individuals have used Internet, in the last 3 months, for looking for a job or sending a job application" ;
	skos:topConceptOf	ns8:indicator .
ns1:i_iumapp	rdf:type	ns2:Indicator ,
		skos:Concept ;
	skos:prefLabel	"making an appointment with a practitioner via a website" ;
	dct:source	ns5:estat_isoc_bde15cua ;
	skos:notation	"i_iumapp" ;
	skos:altLabel	"Appointment with a practitioner via a website" ;
	ns6:membership	ns23:i_iumapp ;
	skos:definition	"Individuals have used Internet, in the last 3 months, for making an appointment with a practitioner via a website (e.g. of a hospital or a health care centre)" ;
	skos:note	"Biennial indicator" ;
	skos:topConceptOf	ns8:indicator .
ns1:i_iumc	rdf:type	ns2:Indicator ,
		skos:Concept ;
	skos:prefLabel	"Individuals using a laptop/tablet to access the internet, away from home or work " ;
	dct:source	ns5:estat_isoc_ci_im_i ;
	skos:notation	"i_iumc" ;
	skos:altLabel	"Nomadic use of laptop/tablet to access the Internet" ;
	ns6:membership	ns29:i_iumc ;
	skos:definition	"Individuals using a portable computer (laptop) to access the internet away from home or work via any wireless connection (WiFi or cellular networks), in the last 3 months. Since 2012 the question explicitly mention also tablet computer (with touch screen)." ;
	skos:note	"Break in series in 2011 and 2012 as the structure of the question has changed. Reconstructed time series using Eurostat varibales: i_iuport, i_iuport1, i_iumc" ;
	skos:topConceptOf	ns8:indicator .
ns1:i_iunw	rdf:type	ns2:Indicator ,
		skos:Concept ;
	skos:prefLabel	"reading / downloading online newspapers / news magazines" ;
	dct:source	ns5:estat_isoc_bde15cua ;
	skos:notation	"i_iunw" ;
	skos:altLabel	"Reading online newspapers/magazines" ;
	ns6:membership	ns13:i_iunw ;
	skos:definition	"Individuals have used Internet, in the last 3 months, for reading / downloading online newspapers / news magazines" ;
	skos:topConceptOf	ns8:indicator .
ns1:i_iuolc	rdf:type	ns2:Indicator ,
		skos:Concept ;
	skos:prefLabel	"doing an online course (in any subject)" ;
	dct:source	ns5:estat_isoc_bde15cua ;
	skos:notation	"i_iuolc" ;
	skos:altLabel	"Doing an online course" ;
	ns6:membership	ns28:i_iuolc ;
	skos:definition	"Individuals have used Internet, in the last 3 months, for doing an online course (of any subject)" ;
	skos:topConceptOf	ns8:indicator .
ns1:i_iuph1	rdf:type	skos:Concept ,
		ns2:Indicator ;
	skos:prefLabel	"telephoning or video calls (via webcam) over the internet" ;
	dct:source	ns5:estat_isoc_bde15cua ;
	skos:notation	"i_iuph1" ;
	skos:altLabel	"Telephoning or video calls" ;
	ns6:membership	ns28:i_iuph1 ;
	skos:note	"Biennial indicator. Break in time series between 2007 and 2008 because of new wording. Reconstructed time series using Eurostat varibales: i_iuph and i_iuph1." ;
	skos:topConceptOf	ns8:indicator .
ns1:i_iuse	rdf:type	skos:Concept ,
		ns2:Indicator ;
	skos:prefLabel	"Individuals who are regular internet users (at least once a week)" ;
	dct:source	ns5:estat_isoc_ci_ifp_fu ;
	skos:notation	"i_iuse" ;
	skos:altLabel	"Regular internet users" ;
	ns6:membership	ns29:i_iuse ;
	skos:definition	"Individuals using the internet at least once a week in the last 3 months." ;
	skos:topConceptOf	ns8:indicator .
ns1:i_iusell	rdf:type	skos:Concept ,
		ns2:Indicator ;
	skos:prefLabel	"Individuals selling goods or services online (e.g. via auctions)" ;
	dct:source	ns5:estat_isoc_r_iuse_i ;
	skos:notation	"i_iusell" ;
	skos:altLabel	"Selling online (e.g. via auctions)" ;
	ns6:membership	ns21:i_iusell ;
	skos:definition	"Individuals have used Internet, in the last 3 months, for selling goods and services (e.g. via auctions)" ;
	skos:topConceptOf	ns8:indicator .
ns1:i_iusnet	rdf:type	skos:Concept ,
		ns2:Indicator ;
	skos:prefLabel	"participating in social networks, over the internet, last 3 months" ;
	dct:source	ns5:estat_isoc_bde15cua ;
	skos:notation	"i_iusnet" ;
	skos:altLabel	"Participating in social networks" ;
	ns6:membership	ns28:i_iusnet ;
	skos:definition	"Individuals have used Internet, in the last 3 months, for participating in social networks (creating user profile, posting messages or other contributions to facebook, twitter, etc.)" ;
	skos:topConceptOf	ns8:indicator .
ns1:i_iuupl	rdf:type	skos:Concept ,
		ns2:Indicator ;
	skos:prefLabel	"uploading self-created content to be shared" ;
	dct:source	ns5:estat_isoc_bde15cua ;
	skos:notation	"i_iuupl" ;
	skos:altLabel	"Uploading self-created content" ;
	ns6:membership	ns28:i_iuupl ;
	skos:definition	"Individuals have used Internet, in the last 3 months, for uploading self-created content (text, images, photos, videos, music, etc.)" ;
	skos:note	"Biennial indicator not collected in 2011." ;
	skos:topConceptOf	ns8:indicator .
ns1:i_iuvod	rdf:type	skos:Concept ,
		ns2:Indicator ;
	skos:prefLabel	"Individuals watching video on demand from commercial services" ;
	dct:source	ns5:estat_isoc_ci_ac_i ;
	skos:notation	"i_iuvod" ;
	skos:altLabel	"Individuals watching video on demand from commercial services" ;
	ns6:membership	ns13:i_iuvod ;
	skos:definition	"Individuals watching video on demand from commercial services" ;
	skos:topConceptOf	ns8:indicator .
ns1:i_iuvote	rdf:type	skos:Concept ,
		ns2:Indicator ;
	skos:prefLabel	"taking part in on-line consultations or voting to define civic or political issues" ;
	dct:source	ns5:estat_isoc_bde15cua ;
	skos:notation	"i_iuvote" ;
	skos:altLabel	"Taking part in on-line consultations or voting" ;
	ns6:membership	ns28:i_iuvote ;
	skos:definition	"Individuals have used Internet, in the last 3 months, for taking part in on-line consultations or voting to define civic or political issues (e.g. urban planning, signing a petition)" ;
	skos:note	"Biennial indicator not collected in 2012." ;
	skos:topConceptOf	ns8:indicator .
ns1:i_iux	rdf:type	skos:Concept ,
		ns2:Indicator ;
	skos:prefLabel	"Individuals who have never used the internet" ;
	dct:source	ns5:estat_isoc_ci_ifp_iu ;
	skos:notation	"i_iux" ;
	skos:altLabel	"Individuals who have never used the internet" ;
	ns6:membership	ns29:i_iux ;
	skos:topConceptOf	ns8:indicator .
ns1:i_piacadv	rdf:type	skos:Concept ,
		ns2:Indicator ;
	skos:prefLabel	"Individuals not allowing use of personal information for advertising" ;
	dct:source	ns5:estat_isoc_cisci_prv ;
	skos:notation	"i_piacadv" ;
	skos:altLabel	"Individuals not allowing use of personal information for advertising" ;
	ns6:membership	ns33:i_piacadv ;
	skos:definition	"Individuals not allowing use of personal information for advertising" ;
	skos:topConceptOf	ns8:indicator .
ns1:i_sbgood	rdf:type	skos:Concept ,
		ns2:Indicator ;
	skos:prefLabel	"Security concerns kept individual from ordering or buying online" ;
	dct:source	ns5:estat_isoc_cisci_ax ;
	skos:notation	"i_sbgood" ;
	skos:altLabel	"Security concerns kept individual from buying online" ;
	ns6:membership	ns33:i_sbgood ;
	skos:definition	"Security concerns kept individual from ordering or buying goods or services for private use" ;
	skos:topConceptOf	ns8:indicator .
ns1:i_secfl	rdf:type	skos:Concept ,
		ns2:Indicator ;
	skos:prefLabel	"Individuals experienced financial loss" ;
	dct:source	ns5:estat_isoc_cisci_pb ;
	skos:notation	"i_secfl" ;
	skos:altLabel	"Individuals experienced financial loss" ;
	ns6:membership	ns33:i_secfl ;
	skos:definition	"Individuals experienced financial loss due to fraudulent payment (credit or debit) card use OR as a result of receiving fraudulent messages ('phishing') or getting redirected to fake websites asking for personal information ('pharming')." ;
	skos:topConceptOf	ns8:indicator .
ns1:i_secpif1	rdf:type	skos:Concept ,
		ns2:Indicator ;
	skos:prefLabel	"Individuals experienced abuse of personal information and/or other privacy violations" ;
	dct:source	ns5:estat_isoc_cisci_pb ;
	skos:notation	"i_secpif1" ;
	skos:altLabel	"Individuals experienced abuse of personal information/privacy violations " ;
	ns6:membership	ns33:i_secpif1 ;
	skos:definition	"Individuals experienced abuse of personal information sent on the Internet and/or other privacy violations (e.g. abuse of pictures, videos, personal data uploaded on community websites)" ;
	skos:topConceptOf	ns8:indicator .
ns1:i_secvir1	rdf:type	skos:Concept ,
		ns2:Indicator ;
	skos:prefLabel	"Individuals caught a virus or other computer infection resulting in loss of information or time" ;
	dct:source	ns5:estat_isoc_cisci_pb ;
	skos:notation	"i_secvir1" ;
	skos:altLabel	"Individuals caught a virus/computer infection" ;
	ns6:membership	ns33:i_secvir1 ;
	skos:definition	"Individuals caught a virus or other computer infection (e.g. worm or Trojan horse) resulting in loss of information or time" ;
	skos:topConceptOf	ns8:indicator .
ns1:i_skedu	rdf:type	skos:Concept ,
		ns2:Indicator ;
	skos:prefLabel	"Individuals who have obtained ICT skills through formal educational institutions" ;
	dct:source	ns5:estat_isoc_sk_how_i ;
	skos:notation	"i_skedu" ;
	skos:altLabel	"ICT skills obtained through formal educational institutions" ;
	ns6:membership	ns27:i_skedu ;
	skos:definition	"Individuals who have obtained ICT skills through formal educational institutions (school, college, university, etc.)" ;
	skos:topConceptOf	ns8:indicator .
ns1:ict_commit_in_trp	rdf:type	skos:Concept ,
		ns2:Indicator ;
	skos:prefLabel	"EU R&I committed funding for ICT" ;
	dct:source	ns5:abac ;
	skos:notation	"ict_commit_in_trp" ;
	skos:altLabel	"EU R&I committed funding for ICT" ;
	ns6:membership	ns31:ict_commit_in_trp ;
	skos:definition	"Credit commitments for ICT Research and Innovation, during the reference year." ;
	skos:topConceptOf	ns8:indicator .
ns1:ict_exp	rdf:type	skos:Concept ,
		ns2:Indicator ;
	skos:prefLabel	"Export of ICT goods and services" ;
	dct:source	ns5:estat-trade ;
	skos:notation	"ict_exp" ;
	skos:altLabel	"Export of ICT goods and services" ;
	ns6:membership	ns25:ict_exp ;
	skos:definition	"ICT goods include: Computers and peripheral equipment, Communication equipment, Consumer electronic equipment, Electronic components and Miscellaneous. ICT services include: Communications services, Computer and information services. The value of exports cover both intra- and extra- EU.\n\n" ;
	skos:note	"The HS classifications used over time (HS1997, HS2002, HS2007) are bridged using the method described in the OECD document DSTI/ICCP/IIS(2010)5." ;
	skos:topConceptOf	ns8:indicator .
ns1:ict_hgc	rdf:type	ns2:Indicator ,
		skos:Concept ;
	skos:prefLabel	"High Growth Companies in the ICT sector" ;
	dct:source	ns5:euripidis-estat ;
	skos:notation	"ict_hgc" ;
	skos:altLabel	"High Growth ICT Companies" ;
	ns6:membership	ns25:ict_hgc ;
	skos:definition	"High growth companies are companies, with more than 10 employees during the reference year, that grows in employent on average by 10% or more over the last 3 year" ;
	skos:topConceptOf	ns8:indicator .
ns1:ict_imp	rdf:type	ns2:Indicator ,
		skos:Concept ;
	skos:prefLabel	"Import of ICT goods and services" ;
	dct:source	ns5:estat-trade ;
	skos:notation	"ict_imp" ;
	skos:altLabel	"Import of ICT goods and services" ;
	ns6:membership	ns25:ict_imp ;
	skos:definition	"ICT goods include: Computers and peripheral equipment, Communication equipment, Consumer electronic equipment, Electronic components and Miscellaneous. ICT services include: Communications services, Computer and information services. The value of import cover both intra- and extra- EU.\n\n" ;
	skos:note	"The HS classifications used over time (HS1997, HS2002, HS2007) are bridged using the method described in the OECD document DSTI/ICCP/IIS(2010)5." ;
	skos:topConceptOf	ns8:indicator .
ns1:ict_spec3_broad	rdf:type	ns2:Indicator ,
		skos:Concept ;
	skos:prefLabel	"Persons Employed with ICT Specialist Skills (broad measure)" ;
	dct:source	ns5:estat_isoc_sks_itspt ;
	skos:notation	"ict_spec3_broad" ;
	skos:altLabel	"Persons Employed with ICT Specialist Skills (broad measure)" ;
	ns6:membership	ns27:ict_spec3_broad ;
	skos:definition	"The definition of the ICT Specialists' occupations is based on the new ISCO-08 classification. It includes ICT service managers (code 133), ICT professionals (25), ICT technicians (35) and some other groups, from electronic and telecomunnications engineers (215*) up to ICT installers and servicers (7422). Where 4-digit data was not available, the share of computing graduates in the corresponding 3-digit data was estimated. See <a href=\"http://ec.europa.eu/eurostat/cache/metadata/en/isoc_sks_esms.htm\">metadata fiche</a> for a complete explanation of the methodology  (Eurostat table isoc_sks_itspt)" ;
	skos:note	"The definition of the ICT Specialists' occupations before 2010 is based on ISCO-88. It includes codes 213, 312, 313, 1236, 2144, 2359, 3114, 7242, 7243. Due to change of the classification and the related definition, the data on ICT Specialists for 2011 and later are not fully comparable with previous years." ;
	skos:topConceptOf	ns8:indicator .
ns1:ict_specialists	rdf:type	ns2:Indicator ,
		skos:Concept ;
	skos:prefLabel	"Persons Employed with ICT Specialist Skills" ;
	dct:source	ns5:cnect-estat ;
	skos:notation	"ict_specialists" ;
	skos:altLabel	"Persons Employed with ICT Specialist Skills" ;
	ns6:membership	ns20:ict_specialists ;
	skos:definition	" The definition of the ICT Specialists' occupations is based on the new ISCO-08 classification. It includes ICT service managers (code 133), ICT professionals (25), ICT technicians (35) and ICT installers and servicers (7422). " ;
	skos:note	"New ISCO-08 classification of occupations is used from 2011 reference period, replacing the former ISCO-88. Due to change of the classification and the related definition, the data on ICT Specialists for 2011 and later are not fully comparable with previous years. " ;
	skos:topConceptOf	ns8:indicator .
ns1:labour_prod_ict	rdf:type	ns2:Indicator ,
		skos:Concept ;
	skos:prefLabel	"Labour productivity of the ICT sector (per person)" ;
	dct:source	ns5:jrc_ict_randd ;
	skos:notation	"labour_prod_ict" ;
	skos:altLabel	"Labour productivity of the ICT sector (per person)" ;
	ns6:membership	ns25:labour_prod_ict ;
	skos:definition	"Is defined as value added per unit of labour input (persons employed)." ;
	skos:topConceptOf	ns8:indicator .
ns1:mbb_3gcov	rdf:type	ns2:Indicator ,
		skos:Concept ;
	skos:prefLabel	"3G coverage (2005-2010)" ;
	dct:source	ns5:idate ;
	skos:notation	"mbb_3gcov" ;
	skos:altLabel	"3G coverage (2005-2010)" ;
	ns6:membership	ns20:mbb_3gcov ;
	skos:definition	"Coverage is a supply indicator defined as the percentage of population living in areas covered by 3G - third generation mobile networks." ;
	skos:note	"Indicator collected until 2010. Then replaced with a more specific one on advanced 3G mobile broadband (HSPA)." ;
	skos:topConceptOf	ns8:indicator .
ns1:mbb_hspacov	rdf:type	ns2:Indicator ,
		skos:Concept ;
	skos:prefLabel	"Advanced 3G mobile broadband (HSPA) coverage (as a % of households)" ;
	dct:source	ns5:point_topic ;
	skos:notation	"mbb_hspacov" ;
	skos:altLabel	"Advanced 3G mobile broadband coverage" ;
	ns6:membership	ns30:mbb_hspacov ;
	skos:definition	"Coverage is a supply indicator defined as the percentage of Households living in areas covered by advanced third generation mobile broadband (HSPA protocol)" ;
	skos:topConceptOf	ns8:indicator .
ns1:mbb_ltecov	rdf:type	ns2:Indicator ,
		skos:Concept ;
	skos:prefLabel	"4G mobile broadband (LTE) coverage (as a % of households)" ;
	dct:source	ns5:bc2020 ;
	skos:notation	"mbb_ltecov" ;
	skos:altLabel	"4G mobile broadband coverage" ;
	ns6:membership	ns30:mbb_ltecov ;
	skos:definition	"Coverage is a supply indicator defined as the percentage of Households living in areas covered by advanced fourth generation mobile broadband (LTE protocol)" ;
	skos:topConceptOf	ns8:indicator .
ns1:mbb_penet	rdf:type	ns2:Indicator ,
		skos:Concept ;
	skos:prefLabel	"Take-up of mobile broadband (subscriptions/100 people)" ;
	dct:source	ns5:cocom ;
	skos:notation	"mbb_penet" ;
	skos:altLabel	"Mobile broadband take-up  (penetration rate)" ;
	ns6:membership	ns30:mbb_penet ;
	skos:definition	"Mobile Broadband penetration is defined as the number of active mobile broadband SIM cards per 100 people. " ;
	skos:topConceptOf	ns8:indicator .
ns1:mbb_rhspacov	rdf:type	ns2:Indicator ,
		skos:Concept ;
	skos:prefLabel	"Rural advanced 3G mobile broadband (HSPA) coverage (as a % of households)" ;
	dct:source	ns5:point_topic ;
	skos:notation	"mbb_rhspacov" ;
	skos:altLabel	"Rural Advanced 3G mobile broadband coverage" ;
	ns6:membership	ns30:mbb_rhspacov ;
	skos:definition	"Coverage is a supply indicator defined as the percentage of Households living in areas covered by advanced third generation mobile broadband (HSPA protocol). Rural areas are defined as those with less than 100 people per km2." ;
	skos:topConceptOf	ns8:indicator .
ns1:mbb_rltecov	rdf:type	ns2:Indicator ,
		skos:Concept ;
	skos:prefLabel	"Rural 4G mobile broadband (LTE) coverage (as a % of households)" ;
	dct:source	ns5:bc2020 ;
	skos:notation	"mbb_rltecov" ;
	skos:altLabel	"Rural 4G mobile broadband coverage" ;
	ns6:membership	ns30:mbb_rltecov ;
	skos:definition	"Coverage is a supply indicator defined as the percentage of Households living in areas covered by advanced fourth generation mobile broadband (LTE protocol). Rural areas are defined as those with less than 100 people per km2." ;
	skos:topConceptOf	ns8:indicator .
ns1:mob_arpm	rdf:type	ns2:Indicator ,
		skos:Concept ;
	skos:prefLabel	"Average Revenue per Minute in Retail Mobile Voice Communications " ;
	dct:source	ns5:cocom ;
	skos:notation	"mob_arpm" ;
	skos:altLabel	"Average Revenue per Minute in Retail Mobile Voice Communications " ;
	ns6:membership	ns20:mob_arpm ;
	skos:definition	"Total voice related retail revenues divided by total voice minutes" ;
	skos:topConceptOf	ns8:indicator .
ns1:mob_arpu	rdf:type	ns2:Indicator ,
		skos:Concept ;
	skos:prefLabel	"Average Revenue per User (ARPU) in the Retail Mobile Market" ;
	dct:source	ns5:cocom ;
	skos:notation	"mob_arpu" ;
	skos:altLabel	"Average Revenue per User (ARPU) in the Retail Mobile Market" ;
	ns6:membership	ns30:mob_arpu ;
	skos:definition	"Total retail mobile revenues divided by number of active SIM cards" ;
	skos:topConceptOf	ns8:indicator .
ns1:mob_ms	rdf:type	ns2:Indicator ,
		skos:Concept ;
	skos:prefLabel	"Market share of leading operator (in % of active SIM cards)" ;
	dct:source	ns5:cocom ;
	skos:notation	"mob_ms" ;
	skos:altLabel	"Market share of mobile leading operator" ;
	ns6:membership	ns30:mob_ms ;
	skos:definition	"Market share of the market leader based on the number of active SIM cards" ;
	skos:topConceptOf	ns8:indicator .
ns1:mob_mtr	rdf:type	ns2:Indicator ,
		skos:Concept ;
	skos:prefLabel	"Mobile voice termination rate" ;
	dct:source	ns5:cocom ;
	skos:notation	"mob_mtr" ;
	skos:altLabel	"Mobile voice termination rate" ;
	ns6:membership	ns30:mob_mtr ;
	skos:definition	"Wholesale call termination charges in mobile voice tecephony" ;
	skos:topConceptOf	ns8:indicator .
ns1:mob_penet	rdf:type	ns2:Indicator ,
		skos:Concept ;
	skos:prefLabel	"Take-up of mobile  - active SIM cards for voice or data" ;
	dct:source	ns5:cocom ;
	skos:notation	"mob_penet" ;
	skos:altLabel	"Mobile take-up (voice or data)" ;
	ns6:membership	ns30:mob_penet ;
	skos:definition	"Number of active SIM cards divided by population. It includes both voice and data services, installed in telephones, modem, usb keys or other devices." ;
	skos:topConceptOf	ns8:indicator .
ns1:mob_roam	rdf:type	skos:Concept ,
		ns2:Indicator ;
	skos:prefLabel	"Mobile roaming price per minute" ;
	dct:source	ns5:berec_roam ;
	skos:notation	"mob_roam" ;
	skos:altLabel	"Mobile roaming price per minute" ;
	ns6:membership	ns30:mob_roam ;
	skos:definition	"Average retail price per minute (in \u20AC-cents) on Eurotariff for intra-EEA roaming voice calls made" ;
	skos:topConceptOf	ns8:indicator .
ns1:mob_subs	rdf:type	skos:Concept ,
		ns2:Indicator ;
	skos:prefLabel	"Total number of subscriptions (SIM cards)" ;
	dct:source	ns5:cocom ;
	skos:notation	"mob_subs" ;
	skos:altLabel	"Number of mobile subscriptions" ;
	ns6:membership	ns30:mob_subs ;
	skos:definition	"Mobile subscriptions are defined as the number of active SIM cards. It includes both voice and data services, installed in telephones, modem, usb keys or other devices." ;
	skos:topConceptOf	ns8:indicator .
ns1:p_empmd	rdf:type	skos:Concept ,
		ns2:Indicator ;
	skos:prefLabel	"Persons employed which were provided a portable device by their employer (business sector)" ;
	dct:source	ns5:estat_isoc_ci_eu_en2 ;
	skos:notation	"p_empmd" ;
	skos:altLabel	"Persons employed provided with a portable device by their enterprise" ;
	ns6:membership	ns7:p_empmd ;
	skos:definition	"The devices (portable computers, tablets, smartphones, PDA phones, etc.) should be provided for business use and the enterprises pay for all or at least up to a limit the subscription and the use costs. Are included only the enterprises with 10 or more persons employed, from all manufacturing and service sectors, excluding the financial sector." ;
	skos:note	"The 2011 question was limited to portable devices using at least 3G technology to connect to the internet." ;
	skos:topConceptOf	ns8:indicator .
ns1:p_iuse	rdf:type	skos:Concept ,
		ns2:Indicator ;
	skos:prefLabel	"Persons employed using computers with access to the Web at work (business sector)" ;
	dct:source	ns5:estat_isoc_bde15b_p ;
	skos:notation	"p_iuse" ;
	skos:altLabel	"Persons employed using computers at work" ;
	ns6:membership	ns27:p_iuse ;
	skos:definition	"The computers (desktop, laptop, smartphones, etc.) should have access to the World Wide Web and be used at least once a week. Are included only the enterprises with 10 or more persons employed, from all manufacturing and service sectors, excluding the financial sector." ;
	skos:note	"Only the business sector is included in the scope: NACEv2 sectors from C10 to N82 (withouk financial services K) + S951." ;
	skos:topConceptOf	ns8:indicator .
ns1:population	rdf:type	skos:Concept ,
		ns2:Indicator ;
	skos:prefLabel	"Total population" ;
	dct:source	ns5:eurostat_pop ;
	skos:notation	"population" ;
	skos:altLabel	"Total population" ;
	ns6:membership	ns15:population ;
	skos:definition	"Total population estimate 1st of January of the same year (Eurostat table demo_pjan)" ;
	skos:topConceptOf	ns8:indicator .
ns1:price_internet_fixed_tel	rdf:type	skos:Concept ,
		ns2:Indicator ;
	skos:prefLabel	"Monthly price of  Fixed Broadband Internet Access offers including Fixed Telephony" ;
	dct:source	ns5:biac ;
	skos:notation	"price_internet_fixed_tel" ;
	skos:altLabel	"Monthly price of  Internet + Fixed Telephony" ;
	ns6:membership	ns16:price_internet_fixed_tel ;
	skos:definition	"Monthly price of Fixed Broadband Internet Access offers including Fixed Telephony, including value added tax, excluding the aditional cost of telephony or cable line (if any). The minimum and median prices refer to the group of similar subscriptions offered by internet service providers. Offers are not weigthed with market shares, so the offers' median price cannot be interpreted as the median price paid by consumers." ;
	skos:note	"If no data is present for a country, it is because no corresponding offers have been found on the national market." ;
	skos:topConceptOf	ns8:indicator .
ns1:price_internet_fixed_tel_tv	rdf:type	skos:Concept ,
		ns2:Indicator ;
	skos:prefLabel	"Monthly price of Internet Acccess + Fixed Telephony + TV bundles" ;
	dct:source	ns5:biac ;
	skos:notation	"price_internet_fixed_tel_tv" ;
	skos:altLabel	"Monthly price of Internet + Fixed Telephony + TV" ;
	ns6:membership	ns16:price_internet_fixed_tel_tv ;
	skos:definition	"Monthly price of Fixed Broadband Internet Access offers including Fixed Telephony and TV (analogue or digital television service), including value added tax, excluding the aditional cost of telephony or cable line (if any). The minimum and median prices refer to the group of similar subscriptions offered by internet service providers. Offers are not weigthed with market shares, so the offers' median price cannot be interpreted as the median price paid by consumers." ;
	skos:note	"If no data is present for a country, it is because no corresponding offers have been found on the national market." ;
	skos:topConceptOf	ns8:indicator .
ns1:price_internet_only	rdf:type	skos:Concept ,
		ns2:Indicator ;
	skos:prefLabel	"Monthly price of standalone internet access" ;
	dct:source	ns5:biac ;
	skos:notation	"price_internet_only" ;
	skos:altLabel	"Monthly price of Internet Access only" ;
	ns6:membership	ns16:price_internet_only ;
	skos:definition	"Monthly price of standalone Fixed Broadband Internet Access offers, including value added tax, excluding the additional cost of telephony or cable line (if any). The minimum and median prices refer to the group of similar subscriptions offered by internet service providers. Offers are not weigthed with market shares, so the offers' median price cannot be interpreted as the median price paid by consumers." ;
	skos:note	"If no data is present for a country, it is because no corresponding offers have been found on the national market." ;
	skos:topConceptOf	ns8:indicator .
ns1:spectrum_wbb	rdf:type	skos:Concept ,
		ns2:Indicator ;
	skos:prefLabel	"Spectrum assigned for wireless broadband in EU harmonised bands" ;
	dct:source	ns5:eco_report_03_efis_comm ;
	skos:notation	"spectrum_wbb" ;
	skos:altLabel	"Assigned spectrum WBB (EU harmonised bands)" ;
	ns6:membership	ns30:spectrum_wbb ;
	skos:definition	"Amount of spectrum assigned by Member States for wireless mobile broadband comunications (WBB) within the ranges harmonised by the European Union. Charts allow to compare with the total value of EU HARMONISED bands and with a simple EU AVERAGE of countries assignements. The policy target is to harmonise and assign 1200 MHz to WBB." ;
	skos:topConceptOf	ns8:indicator .
ns1:st_grad	rdf:type	skos:Concept ,
		ns2:Indicator ;
	skos:prefLabel	"Science and technology graduates" ;
	dct:source	ns5:estat_tps00188 ;
	skos:notation	"st_grad" ;
	skos:altLabel	"Science and technology graduates" ;
	ns6:membership	ns26:st_grad ;
	skos:definition	"Tertiary graduates in science and technology per 1 000 inhabitants aged 20-29 years includes new tertiary graduates in a calendar year from both public and private institutions completing graduate and post graduate studies compared to an age group that corresponds to the typical graduation age in most countries." ;
	skos:topConceptOf	ns8:indicator .
ns1:tel_ftr	rdf:type	skos:Concept ,
		ns2:Indicator ;
	skos:prefLabel	"Fixed voice termination rate" ;
	dct:source	ns5:cocom ;
	skos:notation	"tel_ftr" ;
	skos:altLabel	"Fixed voice termination rate" ;
	ns6:membership	ns34:tel_ftr ;
	skos:definition	"Wholesale call termination charges of the incumbent operator in fixed voice tecephony for local calls" ;
	skos:topConceptOf	ns8:indicator .
ns1:tel_inv	rdf:type	skos:Concept ,
		ns2:Indicator ;
	skos:prefLabel	"Total investment in networks by the electronic communications sector" ;
	dct:source	ns5:cocom ;
	skos:notation	"tel_inv" ;
	skos:altLabel	"Total investment in networks by the electronic communications sector" ;
	ns6:membership	ns34:tel_inv ;
	skos:definition	"Total investment includes both tangible and intangible investment in telecommunication networks (without license fees) by all telecom operators" ;
	skos:topConceptOf	ns8:indicator .
ns1:tel_llu	rdf:type	skos:Concept ,
		ns2:Indicator ;
	skos:prefLabel	"Local Loop Unbundling: total monthly charge" ;
	dct:source	ns5:cocom ;
	skos:notation	"tel_llu" ;
	skos:altLabel	"Local Loop Unbundling: total monthly charge" ;
	ns6:membership	ns34:tel_llu ;
	skos:definition	"The monthly total wholesale cost for Local Loop Unbundling charged by incumbent operators, Calculated as the sum of the monthly charge and 1/36  of the conncetion fee " ;
	skos:topConceptOf	ns8:indicator .
ns1:tel_rev	rdf:type	skos:Concept ,
		ns2:Indicator ;
	skos:prefLabel	"Total revenues of the electronic communications sector" ;
	dct:source	ns5:cocom ;
	skos:notation	"tel_rev" ;
	skos:altLabel	"Total revenues of the electronic communications sector" ;
	ns6:membership	ns34:tel_rev ;
	skos:definition	"Total includes wholesale and retail revenues from electronic communications perceived in the reference year by all telecom operators (VAT excluded)" ;
	skos:topConceptOf	ns8:indicator .
ns1:transparent_egov	rdf:type	ns2:Indicator ,
		skos:Concept ;
	skos:prefLabel	"Transparency Score of eGovernment Services" ;
	dct:source	ns5:egov_bench12 ;
	skos:notation	"transparent_egov" ;
	skos:altLabel	"Transparency Score" ;
	ns6:membership	ns20:transparent_egov ;
	skos:definition	"The Transparency score indicates to what extent eGovernment services are transparent. It assesses three aspects of transparency: to what extent public authorities are transparent regarding their own responsibilities and performance, to what extent they are transparent regarding the process of service delivery, and to what extent they are transparent regarding the personal data involved in service delivery." ;
	skos:topConceptOf	ns8:indicator .
ns1:user_centric_egov	rdf:type	ns2:Indicator ,
		skos:Concept ;
	skos:prefLabel	"User Centricity Score of eGovernment services" ;
	dct:source	ns5:egov_bench12 ;
	skos:notation	"user_centric_egov" ;
	skos:altLabel	"User Centricity Score" ;
	ns6:membership	ns20:user_centric_egov ;
	skos:definition	"The User centricity score indicates to what extent (information about) a service is provided online and how usable it is (e.g., if support, help and feedback functionality exist online), as well as quality assessments by researchers on the service's ease and speed of use." ;
	skos:topConceptOf	ns8:indicator .
ns1:val_add_ict	rdf:type	ns2:Indicator ,
		skos:Concept ;
	skos:prefLabel	"Value added of the ICT sector" ;
	dct:source	ns5:jrc_ict_randd ;
	skos:notation	"val_add_ict" ;
	skos:altLabel	"Value added of the ICT sector" ;
	ns6:membership	ns25:val_add_ict ;
	skos:definition	"Value added. In the System of National Accounts it is defined as the value of output less the value of intermediate consumption; it is a measure of the contribution to GDP made by an individual producer, industry or sector." ;
	skos:topConceptOf	ns8:indicator .
ns1:wid_ius	rdf:type	ns2:Indicator ,
		skos:Concept ;
	skos:prefLabel	"2 Internet user skills" ;
	dct:source	ns5: ;
	skos:notation	"wid_ius" ;
	skos:altLabel	"2 Internet user skills" ;
	ns6:membership	ns35:wid_ius ;
	skos:definition	"WID Internet user skills dimension calculated as the weighted average of the three indicators: 2.1 At least basic digital skills  (33.3%), 2.2 Above basic digital skills (33.3%), 2.3 At least basic digital content creation skills (33.3%)." ;
	skos:topConceptOf	ns8:indicator .
ns1:wid_ius_abs	rdf:type	ns2:Indicator ,
		skos:Concept ;
	skos:prefLabel	"2.2 Above basic digital skills" ;
	dct:source	ns5: ;
	skos:notation	"wid_ius_abs" ;
	skos:altLabel	"2.2 Above basic digital skills" ;
	ns6:membership	ns35:wid_ius_abs ;
	skos:definition	"Individuals with \u2018above basic\u2019 digital skills in each of the following five dimensions: information, communication, problem solving, software for content creation and safety" ;
	skos:topConceptOf	ns8:indicator .
ns1:wid_ius_bs	rdf:type	ns2:Indicator ,
		skos:Concept ;
	skos:prefLabel	"2.1 At least basic digital skills" ;
	dct:source	ns5: ;
	skos:notation	"wid_ius_bs" ;
	skos:altLabel	"2.1 At least basic digital skills" ;
	ns6:membership	ns35:wid_ius_bs ;
	skos:definition	"Individuals with \u2018basic\u2019 or \u2018above basic\u2019 digital skills in each of the following five dimensions: information, communication, problem solving, software for content creation and safety" ;
	skos:topConceptOf	ns8:indicator .
ns1:wid_ius_ss	rdf:type	ns2:Indicator ,
		skos:Concept ;
	skos:prefLabel	"2.3 At least basic digital content creation skills" ;
	dct:source	ns5: ;
	skos:notation	"wid_ius_ss" ;
	skos:altLabel	"2.3 At least basic digital content creation skills" ;
	ns6:membership	ns35:wid_ius_ss ;
	skos:definition	"Individuals with a basic level in using software for digital content creation" ;
	skos:topConceptOf	ns8:indicator .
ns1:wid_score	rdf:type	ns2:Indicator ,
		skos:Concept ;
	skos:prefLabel	"Women in Digital (WID) score" ;
	dct:source	ns5: ;
	skos:notation	"wid_score" ;
	skos:altLabel	"Women in Digital (WID) score" ;
	ns6:membership	ns35:wid_score ;
	skos:definition	"Women in digital score calculated as the weighted average of the three sub-dimensions: 1 Use of internet  (33.3%), 2 Internet users skills (33.3%), 3 Specialist skills and employment (33.3%).\n\n" ;
	skos:topConceptOf	ns8:indicator .
ns1:wid_sse	rdf:type	ns2:Indicator ,
		skos:Concept ;
	skos:prefLabel	"3 Specialist skills and employment" ;
	dct:source	ns5: ;
	skos:notation	"wid_sse" ;
	skos:altLabel	"3 Specialist skills and employment" ;
	ns6:membership	ns35:wid_sse ;
	skos:definition	"WID Use of Internet Dimension calculated as the weighted average of the three indicators: \n3.1 STEM graduates (33.3%), 3.2 ICT specialists (33.3%), 3.3 Gender pay gap  (33.3%)." ;
	skos:topConceptOf	ns8:indicator .
ns1:wid_sse_gpg	rdf:type	ns2:Indicator ,
		skos:Concept ;
	skos:prefLabel	"3.3 Gender pay gap" ;
	dct:source	ns5: ;
	skos:notation	"wid_sse_gpg" ;
	skos:altLabel	"3.3 Unadjusted gender pay gap" ;
	ns6:membership	ns35:wid_sse_gpg ;
	skos:definition	"Gender pay gap in unadjusted form, measured as the difference between average gross hourly earnings of male paid employees and  female paid employees as a percentage of average gross hourly earnings of male paid employees. The indicator has been defined as unadjusted, because it gives an overall picture of gender inequalities in terms of pay and measures a concept which is broader than the concept of equal pay for equal work. All employees working in firms with ten or more employees, without restrictions for age and hours worked, are included." ;
	skos:topConceptOf	ns8:indicator .
ns1:wid_sse_icts	rdf:type	ns2:Indicator ,
		skos:Concept ;
	skos:prefLabel	"3.2 ICT specialists" ;
	dct:source	ns5: ;
	skos:notation	"wid_sse_icts" ;
	skos:altLabel	"3.2 ICT specialists" ;
	ns6:membership	ns35:wid_sse_icts ;
	skos:definition	"Employed ICT specialists. Broad definition based on the ISCO-08 classification and including jobs like ICT service managers, ICT professionals, ICT technicians, ICT installers and servicers." ;
	skos:topConceptOf	ns8:indicator .
ns1:wid_sse_stem	rdf:type	ns2:Indicator ,
		skos:Concept ;
	skos:prefLabel	"3.1 STEM graduates" ;
	dct:source	ns5: ;
	skos:notation	"wid_sse_stem" ;
	skos:altLabel	"3.1 STEM graduates" ;
	ns6:membership	ns35:wid_sse_stem ;
	skos:definition	"People with a degree in a science, technology, maths or engineering-related subject" ;
	skos:topConceptOf	ns8:indicator .
ns1:wid_ui	rdf:type	ns2:Indicator ,
		skos:Concept ;
	skos:prefLabel	"1 Use of internet" ;
	dct:source	ns5: ;
	skos:notation	"wid_ui" ;
	skos:altLabel	"1 Use of internet" ;
	ns6:membership	ns35:wid_ui ;
	skos:definition	"WID Use of internet dimension calculated as the weighted average of the six indicators: \r\n1.1 Regular internet use (16.67%), 1.2 People who never used the internet (16.67%), 1.3 Online banking (16.67%), 1.4 Doing an online course (16.67%), 1.5 Online consultations or voting (16.67%), 1.6 eGovernment users (16.67%)." ;
	skos:topConceptOf	ns8:indicator .
ns1:wid_ui_egov	rdf:type	ns2:Indicator ,
		skos:Concept ;
	skos:prefLabel	"1.6 eGovernment users " ;
	dct:source	ns5: ;
	skos:notation	"wid_ui_egov" ;
	skos:altLabel	"1.6 eGovernment users " ;
	ns6:membership	ns35:wid_ui_egov ;
	skos:definition	"Individuals that have used Internet, in the last 12 months, for interaction with public authorities. It includes obtaining information from public authorities web sites, OR downloading official forms OR sending filled in forms. Unit of measure: Percentage of individuals who used Internet within the last 12 months" ;
	skos:topConceptOf	ns8:indicator .
ns1:wid_ui_ib	rdf:type	skos:Concept ,
		ns2:Indicator ;
	skos:prefLabel	"1.3 Online banking" ;
	dct:source	ns5: ;
	skos:notation	"wid_ui_ib" ;
	skos:altLabel	"1.3 Online banking" ;
	ns6:membership	ns35:wid_ui_ib ;
	skos:definition	"People who used the Internet to use online banking " ;
	skos:topConceptOf	ns8:indicator .
ns1:wid_ui_iu	rdf:type	skos:Concept ,
		ns2:Indicator ;
	skos:prefLabel	"1.1 Regular internet use" ;
	dct:source	ns5: ;
	skos:notation	"wid_ui_iu" ;
	skos:altLabel	"1.1 Regular internet use" ;
	ns6:membership	ns35:wid_ui_iu ;
	skos:definition	"People who used the Internet at least once a week" ;
	skos:topConceptOf	ns8:indicator .
ns1:wid_ui_nui	rdf:type	skos:Concept ,
		ns2:Indicator ;
	skos:prefLabel	"1.2 People who never used the internet" ;
	dct:source	ns5: ;
	skos:notation	"wid_ui_nui" ;
	skos:altLabel	"1.2 People who never used the internet" ;
	ns6:membership	ns35:wid_ui_nui ;
	skos:definition	"People who never used the Internet" ;
	skos:topConceptOf	ns8:indicator .
ns1:wid_ui_oc	rdf:type	skos:Concept ,
		ns2:Indicator ;
	skos:prefLabel	"1.4 Doing an online course" ;
	dct:source	ns5: ;
	skos:notation	"wid_ui_oc" ;
	skos:altLabel	"1.4 Doing an online course" ;
	ns6:membership	ns35:wid_ui_oc ;
	skos:definition	"People who used the Internet for doing an online course (on any subject)" ;
	skos:topConceptOf	ns8:indicator .
ns1:wid_ui_part	rdf:type	skos:Concept ,
		ns2:Indicator ;
	skos:prefLabel	"1.5 Online consultations or voting" ;
	dct:source	ns5: ;
	skos:notation	"wid_ui_part" ;
	skos:altLabel	"1.5 Online consultations or voting" ;
	ns6:membership	ns35:wid_ui_part ;
	skos:definition	"People who took part in on-line consultations or voting to define civic or political issues (e.g. urban planning, signing a petition)" ;
	skos:topConceptOf	ns8:indicator .
ns22:e_gov_0_score	rdf:type	ns2:IndicatorToGroupMembership ;
	rdfs:label	"egovernment" ;
	ns6:member-of	ns14:egovernment ;
	ns6:order	"1110" .
ns22:e_gov_2b_tr_pd	rdf:type	ns2:IndicatorToGroupMembership ;
	rdfs:label	"egovernment" ;
	ns6:member-of	ns14:egovernment ;
	ns6:order	"11122" .
ns22:e_gov_2c_tr_de	rdf:type	ns2:IndicatorToGroupMembership ;
	rdfs:label	"egovernment" ;
	ns6:member-of	ns14:egovernment ;
	ns6:order	"11123" .
ns1:e_gov_0_score	rdf:type	ns2:Indicator ,
		skos:Concept ;
	skos:prefLabel	"0 Overall Score" ;
	dct:source	ns5:egov_bench ;
	skos:notation	"e_gov_0_score" ;
	skos:altLabel	"0 Overall Score" ;
	ns6:membership	ns22:e_gov_0_score ;
	skos:definition	"The overall eGovernment maturity score that captures the scores of all four dimensions, which consist of 14 underlying indicators, broken down into 48 survey questions" ;
	skos:topConceptOf	ns8:indicator .
ns1:e_gov_2b_tr_pd	rdf:type	ns2:Indicator ,
		skos:Concept ;
	skos:prefLabel	"2.2 Transparency - Transparency of personal data" ;
	dct:source	ns5:egov_bench ;
	skos:notation	"e_gov_2b_tr_pd" ;
	skos:altLabel	"2.2 Transparency - Transparency of personal data" ;
	ns6:membership	ns22:e_gov_2b_tr_pd ;
	skos:definition	"The extent to which user can manage their personal data held by government organisations." ;
	skos:topConceptOf	ns8:indicator .
ns1:e_gov_2c_tr_de	rdf:type	ns2:Indicator ,
		skos:Concept ;
	skos:prefLabel	"2.3 Transparency - Transparency of service design" ;
	dct:source	ns5:egov_bench ;
	skos:notation	"e_gov_2c_tr_de" ;
	skos:altLabel	"2.3 Transparency - Transparency of service design" ;
	ns6:membership	ns22:e_gov_2c_tr_de ;
	skos:definition	"The extent to which user are informed on and involved in policy and service design processes." ;
	skos:topConceptOf	ns8:indicator .
ns7:edigint2018	rdf:type	ns2:IndicatorToGroupMembership ;
	rdfs:label	"ebusiness" ;
	ns6:member-of	ns14:ebusiness ;
	ns6:order	"15" .
ns7:edigint2021	rdf:type	ns2:IndicatorToGroupMembership ;
	rdfs:label	"ebusiness" ;
	ns6:member-of	ns14:ebusiness ;
	ns6:order	"15" .
ns7:edigint2022	rdf:type	ns2:IndicatorToGroupMembership ;
	rdfs:label	"ebusiness" ;
	ns6:member-of	ns14:ebusiness ;
	ns6:order	"15" .
ns1:edigint2018	rdf:type	ns2:Indicator ,
		skos:Concept ;
	skos:prefLabel	"Digital Intensity score for Enterprises (DII v2)" ;
	dct:source	ns5:estat-ent ;
	skos:notation	"edigint2018" ;
	skos:altLabel	"Digital Intensity score for Enterprises (DII v2)" ;
	ns6:membership	ns7:edigint2018 ;
	skos:definition	"The Digital Intensity score is based on counting how many out of 12 technologies are used by each enterprise. Then they are divided into four clusters of digital intensity: Very Low (scores 0-3), Low (score 4-6), High (score 7-9), Very High (score 10-12)." ;
	skos:note	"The DII composition varies between different survey years, depending on the questions included in the survey. The exact composition for the different survey years can be found at https://circabc.europa.eu/ui/group/89577311-0f9b-4fc0-b8c2-2aaa7d3ccb91/library/30b83b9c-3d0c-4086-bf52-77905e19b4eb/details." ;
	skos:topConceptOf	ns8:indicator .
ns1:edigint2021	rdf:type	ns2:Indicator ,
		skos:Concept ;
	skos:prefLabel	"Digital Intensity score for Enterprises (DII v3)" ;
	dct:source	ns5:estat-ent ;
	skos:notation	"edigint2021" ;
	skos:altLabel	"Digital Intensity score for Enterprises (DII v3)" ;
	ns6:membership	ns7:edigint2021 ;
	skos:definition	"The Digital Intensity score is based on counting how many out of 12 technologies are used by each enterprise. Then they are divided into four clusters of digital intensity: Very Low (scores 0-3), Low (score 4-6), High (score 7-9), Very High (score 10-12)." ;
	skos:note	"The DII composition varies between different survey years, depending on the questions included in the survey. The exact composition for the different survey years can be found at https://circabc.europa.eu/ui/group/89577311-0f9b-4fc0-b8c2-2aaa7d3ccb91/library/30b83b9c-3d0c-4086-bf52-77905e19b4eb/details." ;
	skos:topConceptOf	ns8:indicator .
ns1:edigint2022	rdf:type	skos:Concept ,
		ns2:Indicator ;
	skos:prefLabel	"Digital Intensity score for Enterprises (DII v4)" ;
	dct:source	ns5:estat-ent ;
	skos:notation	"edigint2022" ;
	skos:altLabel	"Digital Intensity score for Enterprises (DII v4)" ;
	ns6:membership	ns7:edigint2022 ;
	skos:definition	"The Digital Intensity score is based on counting how many out of 12 technologies are used by each enterprise. Then they are divided into four clusters of digital intensity: Very Low (scores 0-3), Low (score 4-6), High (score 7-9), Very High (score 10-12)." ;
	skos:note	"The DII composition varies between different survey years, depending on the questions included in the survey. The exact composition for the different survey years can be found at https://circabc.europa.eu/ui/group/89577311-0f9b-4fc0-b8c2-2aaa7d3ccb91/library/30b83b9c-3d0c-4086-bf52-77905e19b4eb/details." ;
	skos:topConceptOf	ns8:indicator .
ns7:sme_di_x_vlo	rdf:type	ns2:IndicatorToGroupMembership ;
	rdfs:label	"ebusiness" ;
	ns6:member-of	ns14:ebusiness ;
	ns6:order	"16" .
<http://semantic.digital-agenda-data.eu/codelist/indicator-group/mobile/5g_cov_3400_3800>	rdf:type	ns2:IndicatorToGroupMembership ;
	rdfs:label	"mobile" ;
	ns6:member-of	ns14:mobile ;
	ns6:order	"2" .
<http://semantic.digital-agenda-data.eu/codelist/indicator-group/mobile/5g_spectrum>	rdf:type	ns2:IndicatorToGroupMembership ;
	rdfs:label	"mobile" ;
	ns6:member-of	ns14:mobile ;
	ns6:order	"3" .
<http://semantic.digital-agenda-data.eu/codelist/indicator/5g_cov_3400_3800>	rdf:type	skos:Concept ,
		ns2:Indicator ;
	skos:prefLabel	"5G coverage on the 3.4-3.8 GHz spectrum band" ;
	dct:source	ns5:point_topic ;
	skos:notation	"5g_cov_3400_3800" ;
	skos:altLabel	"5G coverage on the 3.4-3.8 GHz spectrum band" ;
	ns6:membership	<http://semantic.digital-agenda-data.eu/codelist/indicator-group/mobile/5g_cov_3400_3800> ;
	skos:definition	"% of populated areas with coverage by 5G using the 3.4-3.8GHz spectrum band" ;
	skos:topConceptOf	ns8:indicator .
<http://semantic.digital-agenda-data.eu/codelist/indicator/5g_spectrum>	rdf:type	skos:Concept ,
		ns2:Indicator ;
	skos:prefLabel	"5G spectrum" ;
	dct:source	ns5:cocom_new ;
	skos:notation	"5g_spectrum" ;
	skos:altLabel	"5G spectrum" ;
	ns6:membership	<http://semantic.digital-agenda-data.eu/codelist/indicator-group/mobile/5g_spectrum> ;
	skos:definition	"The amount of spectrum assigned and ready for 5G use within the so-called 5G pioneer bands. These bands are 700 MHz (703-733 MHz and 758-788 MHz), 3.6 GHz (3400-3800 MHz) and 26 GHz (1000 MHz within 24250-27500 MHz). All three spectrum bands have an equal weight." ;
	skos:topConceptOf	ns8:indicator .
ns1:sme_di_x_vlo	rdf:type	skos:Concept ,
		ns2:Indicator ;
	skos:prefLabel	"SMEs with at least a basic level of digital intensity (2022)" ;
	dct:source	ns5:estat_isoc_e_dii ;
	skos:notation	"sme_di_x_vlo" ;
	skos:altLabel	"SMEs with at least a basic level of digital intensity" ;
	ns6:membership	ns7:sme_di_x_vlo ;
	skos:definition	"SMEs with low, high or very high digital intensity" ;
	skos:note	"Enterprises with 10-250 persons employed. All manufacturing and service sectors, excluding the financial sector. " ;
	skos:topConceptOf	ns8:indicator .
ns1:e_gov_4b_bm_us	rdf:type	ns2:Indicator ,
		skos:Concept ;
	skos:prefLabel	"4b Business Mobility - Usability" ;
	dct:source	ns5:egov_bench12_17 ;
	skos:notation	"e_gov_4b_bm_us" ;
	skos:altLabel	"4c Business Mobility - Usability" ;
	ns6:membership	ns22:e_gov_4b_bm_us ;
	skos:definition	"Online support and help features on services aimed at foreign businesses." ;
	skos:topConceptOf	ns8:indicator .
ns26:ict_grad	rdf:type	ns2:IndicatorToGroupMembership ;
	rdfs:label	"ict-skills" ;
	ns6:member-of	ns14:ict-skills ;
	ns6:order	"31" .
ns1:ict_grad	rdf:type	skos:Concept ,
		ns2:Indicator ;
	skos:prefLabel	"ICT graduates" ;
	dct:source	ns5:estat_educ_uoe_grad03 ;
	skos:notation	"ict_grad" ;
	skos:altLabel	"ICT graduates" ;
	ns6:membership	ns26:ict_grad ;
	skos:definition	"Individuals with a degree in ICT" ;
	skos:topConceptOf	ns8:indicator .
ns22:e_gov_dpsc_new	rdf:type	ns2:IndicatorToGroupMembership ;
	rdfs:label	"egovernment" ;
	ns6:member-of	ns14:egovernment ;
	ns6:order	"3" .
ns22:e_gov_ebus_new	rdf:type	ns2:IndicatorToGroupMembership ;
	rdfs:label	"egovernment" ;
	ns6:member-of	ns14:egovernment ;
	ns6:order	"4" .
ns22:e_gov_pff_new	rdf:type	ns2:IndicatorToGroupMembership ;
	rdfs:label	"egovernment" ;
	ns6:member-of	ns14:egovernment ;
	ns6:order	"2" .
ns1:e_gov_dpsc_new	rdf:type	skos:Concept ,
		ns2:Indicator ;
	skos:prefLabel	"Digital Public Services for Citizens (from 2021)" ;
	dct:source	ns5: ;
	skos:notation	"e_gov_dpsc_new" ;
	skos:altLabel	"Digital Public Services for Citizens (from 2021)" ;
	ns6:membership	ns22:e_gov_dpsc_new ;
	skos:definition	"The extent to which a service or information concerning service for citizens is provided online, and via a portal. Services that are offered fully, partially or not at all online. " ;
	skos:topConceptOf	ns8:indicator .
ns1:e_gov_ebus_new	rdf:type	skos:Concept ,
		ns2:Indicator ;
	skos:prefLabel	"Digital Public Services for Businesses (from 2021)" ;
	dct:source	ns5: ;
	skos:notation	"e_gov_ebus_new" ;
	skos:altLabel	"Digital Public Services for Businesses (from 2021)" ;
	ns6:membership	ns22:e_gov_ebus_new ;
	skos:definition	"The extent to which a service or information concerning service for businesses is provided online and via a portal. Services that are offered fully, partially or not at all online. " ;
	skos:topConceptOf	ns8:indicator .
ns1:e_gov_pff_new	rdf:type	skos:Concept ,
		ns2:Indicator ;
	skos:prefLabel	"Pre-filled forms (from 2021)" ;
	dct:source	ns5: ;
	skos:notation	"e_gov_pff_new" ;
	skos:altLabel	"Pre-filled forms (from 2021)" ;
	ns6:membership	ns22:e_gov_pff_new ;
	skos:definition	"Amount of data that is pre-filled in Public Services' online forms (Authentic sources Key Enabler indicator of eGovernment benchmark)" ;
	skos:topConceptOf	ns8:indicator .
@prefix ns36:	<http://semantic.digital-agenda-data.eu/codelist/indicator-group/desi_ind/> .
ns36:desi_fttpc	rdf:type	ns2:IndicatorToGroupMembership ;
	rdfs:label	"desi_ind" ;
	ns6:member-of	ns14:desi_ind ;
	ns6:order	"231" .
@prefix ns37:	<http://semantic.digital-agenda-data.eu/codelist/indicator-group/rid/> .
ns37:rid_c	rdf:type	ns2:IndicatorToGroupMembership ;
	rdfs:label	"rid" ;
	ns6:member-of	ns14:rid ;
	ns6:order	"15" .
ns37:rid_c_5gc	rdf:type	ns2:IndicatorToGroupMembership ;
	rdfs:label	"rid" ;
	ns6:member-of	ns14:rid ;
	ns6:order	"21" .
ns37:rid_c_fbbc	rdf:type	ns2:IndicatorToGroupMembership ;
	rdfs:label	"rid" ;
	ns6:member-of	ns14:rid ;
	ns6:order	"18" .
ns37:rid_c_fbbtc	rdf:type	ns2:IndicatorToGroupMembership ;
	rdfs:label	"rid" ;
	ns6:member-of	ns14:rid ;
	ns6:order	"16" .
ns37:rid_c_fttpc	rdf:type	ns2:IndicatorToGroupMembership ;
	rdfs:label	"rid" ;
	ns6:member-of	ns14:rid ;
	ns6:order	"20" .
ns37:rid_c_mbbtu	rdf:type	ns2:IndicatorToGroupMembership ;
	rdfs:label	"rid" ;
	ns6:member-of	ns14:rid ;
	ns6:order	"17" .
ns37:rid_c_vhcnc	rdf:type	ns2:IndicatorToGroupMembership ;
	rdfs:label	"rid" ;
	ns6:member-of	ns14:rid ;
	ns6:order	"19" .
ns37:rid_ius	rdf:type	ns2:IndicatorToGroupMembership ;
	rdfs:label	"rid" ;
	ns6:member-of	ns14:rid ;
	ns6:order	"10" .
ns37:rid_ius_abs	rdf:type	ns2:IndicatorToGroupMembership ;
	rdfs:label	"rid" ;
	ns6:member-of	ns14:rid ;
	ns6:order	"12" .
ns37:rid_ius_bs	rdf:type	ns2:IndicatorToGroupMembership ;
	rdfs:label	"rid" ;
	ns6:member-of	ns14:rid ;
	ns6:order	"11" .
ns37:rid_ius_icts	rdf:type	ns2:IndicatorToGroupMembership ;
	rdfs:label	"rid" ;
	ns6:member-of	ns14:rid ;
	ns6:order	"14" .
ns37:rid_ius_ss	rdf:type	ns2:IndicatorToGroupMembership ;
	rdfs:label	"rid" ;
	ns6:member-of	ns14:rid ;
	ns6:order	"13" .
ns37:rid_score	rdf:type	ns2:IndicatorToGroupMembership ;
	rdfs:label	"rid" ;
	ns6:member-of	ns14:rid ;
	ns6:order	"1" .
ns37:rid_ui_egov	rdf:type	ns2:IndicatorToGroupMembership ;
	rdfs:label	"rid" ;
	ns6:member-of	ns14:rid ;
	ns6:order	"9" .
ns37:rid_ui_ib	rdf:type	ns2:IndicatorToGroupMembership ;
	rdfs:label	"rid" ;
	ns6:member-of	ns14:rid ;
	ns6:order	"5" .
ns37:rid_ui_iu	rdf:type	ns2:IndicatorToGroupMembership ;
	rdfs:label	"rid" ;
	ns6:member-of	ns14:rid ;
	ns6:order	"3" .
ns37:rid_ui_nui	rdf:type	ns2:IndicatorToGroupMembership ;
	rdfs:label	"rid" ;
	ns6:member-of	ns14:rid ;
	ns6:order	"4" .
ns37:rid_ui_oc	rdf:type	ns2:IndicatorToGroupMembership ;
	rdfs:label	"rid" ;
	ns6:member-of	ns14:rid ;
	ns6:order	"7" .
ns37:rid_ui_part	rdf:type	ns2:IndicatorToGroupMembership ;
	rdfs:label	"rid" ;
	ns6:member-of	ns14:rid ;
	ns6:order	"8" .
ns1:desi_fttpc	rdf:type	ns2:Indicator ,
		skos:Concept ;
	skos:prefLabel	"Fibre to the Premises (FTTP) coverage" ;
	dct:source	ns5:desi_fttpc ;
	skos:notation	"desi_fttpc" ;
	skos:altLabel	"Fibre to the Premises (FTTP) coverage" ;
	ns6:membership	ns36:desi_fttpc ;
	skos:definition	"Percentage of households covered by FTTH and FTTB " ;
	skos:topConceptOf	ns8:indicator .
ns1:rid_c	rdf:type	ns2:Indicator ,
		skos:Concept ;
	skos:prefLabel	"3 Connectivity" ;
	dct:source	ns5: ;
	skos:notation	"rid_c" ;
	skos:altLabel	"3 Connectivity" ;
	ns6:membership	ns37:rid_c ;
	skos:definition	"Connectivity dimension calculated as the weighted average of the six indicators: 3.1 Overall fixed broadband take-up (12.5%), 3.2 Mobile broadband take-up (12.5%), 3.3 Fast broadband (NGA) coverage (12.5%%), 3.4 Fixed Very High Capacity Network (VHCN) coverage (25%), 3.5 Fibre to the Premises (FTTP) coverage (12.5%) and 3.6 5G coverage (25%)" ;
	skos:topConceptOf	ns8:indicator .
ns1:rid_c_5gc	rdf:type	ns2:Indicator ,
		skos:Concept ;
	skos:prefLabel	"3.6 5G coverage" ;
	dct:source	ns5: ;
	skos:notation	"rid_c_5gc" ;
	skos:altLabel	"3.6 5G coverage" ;
	ns6:membership	ns37:rid_c_5gc ;
	skos:definition	"Percentage of populated areas with coverage by 5G" ;
	skos:topConceptOf	ns8:indicator .
ns1:rid_c_fbbc	rdf:type	ns2:Indicator ,
		skos:Concept ;
	skos:prefLabel	"3.3 Fast broadband (NGA) coverage" ;
	dct:source	ns5: ;
	skos:notation	"rid_c_fbbc" ;
	skos:altLabel	"3.3 Fast broadband (NGA) coverage" ;
	ns6:membership	ns37:rid_c_fbbc ;
	skos:definition	"Percentage of households covered by fixed broadband of at least 30 Mbps download. The technologies considered are FTTH, FTTB, Cable Docsis 3.0 and VDSL" ;
	skos:topConceptOf	ns8:indicator .
ns1:rid_c_fbbtc	rdf:type	ns2:Indicator ,
		skos:Concept ;
	skos:prefLabel	"3.1 Overall fixed broadband take-up" ;
	dct:source	ns5: ;
	skos:notation	"rid_c_fbbtc" ;
	skos:altLabel	"3.1 Overall fixed broadband take-up" ;
	ns6:membership	ns37:rid_c_fbbtc ;
	skos:definition	"Percentage of households subscribing to fixed broadband" ;
	skos:topConceptOf	ns8:indicator .
ns1:rid_c_fttpc	rdf:type	skos:Concept ,
		ns2:Indicator ;
	skos:prefLabel	"3.5 Fibre to the Premises (FTTP) coverage" ;
	dct:source	ns5: ;
	skos:notation	"rid_c_fttpc" ;
	skos:altLabel	"3.5 Fibre to the Premises (FTTP) coverage" ;
	ns6:membership	ns37:rid_c_fttpc ;
	skos:definition	"Percentage of households covered by FTTH and FTTB " ;
	skos:topConceptOf	ns8:indicator .
ns1:rid_c_mbbtu	rdf:type	skos:Concept ,
		ns2:Indicator ;
	skos:prefLabel	"3.2 Mobile broadband take-up" ;
	dct:source	ns5: ;
	skos:notation	"rid_c_mbbtu" ;
	skos:altLabel	"3.2 Mobile broadband take-up" ;
	ns6:membership	ns37:rid_c_mbbtu ;
	skos:definition	"Individuals who used the internet on a mobile device" ;
	skos:topConceptOf	ns8:indicator .
ns1:rid_c_vhcnc	rdf:type	skos:Concept ,
		ns2:Indicator ;
	skos:prefLabel	"3.4 Fixed Very High Capacity Network (VHCN) coverage" ;
	dct:source	ns5: ;
	skos:notation	"rid_c_vhcnc" ;
	skos:altLabel	"3.4 Fixed Very High Capacity Network (VHCN) coverage" ;
	ns6:membership	ns37:rid_c_vhcnc ;
	skos:definition	"Percentage of households covered by any fixed VHCN. The technologies considered are FTTH, FTTB and Cable Docsis 3.1" ;
	skos:topConceptOf	ns8:indicator .
ns1:rid_ius	rdf:type	skos:Concept ,
		ns2:Indicator ;
	skos:prefLabel	"2 Human capital" ;
	dct:source	ns5: ;
	skos:notation	"rid_ius" ;
	skos:altLabel	"2 Human capital" ;
	ns6:membership	ns37:rid_ius ;
	skos:definition	"Human Capital dimension calculated as the weighted average of the four indicators: 2.1 At least basic digital skills  (33%), 2.2 Above basic digital skills (17%), 2.3 At least basic digital content creation skills (17%), 2.4 ICT specialists (33%)" ;
	skos:topConceptOf	ns8:indicator .
ns1:rid_ius_abs	rdf:type	skos:Concept ,
		ns2:Indicator ;
	skos:prefLabel	"2.2 Above basic digital skills" ;
	dct:source	ns5: ;
	skos:notation	"rid_ius_abs" ;
	skos:altLabel	"2.2 Above basic digital skills" ;
	ns6:membership	ns37:rid_ius_abs ;
	skos:definition	"Individuals with \u2018above basic\u2019 digital skills in each of the following five dimensions: information, communication, problem solving, software for content creation and safety" ;
	skos:topConceptOf	ns8:indicator .
ns1:rid_ius_bs	rdf:type	skos:Concept ,
		ns2:Indicator ;
	skos:prefLabel	"2.1 At least basic digital skills" ;
	dct:source	ns5: ;
	skos:notation	"rid_ius_bs" ;
	skos:altLabel	"2.1 At least basic digital skills" ;
	ns6:membership	ns37:rid_ius_bs ;
	skos:definition	"Individuals with \u2018basic\u2019 or \u2018above basic\u2019 digital skills in each of the following five dimensions: information, communication, problem solving, software for content creation and safety" ;
	skos:topConceptOf	ns8:indicator .
ns1:rid_ius_icts	rdf:type	skos:Concept ,
		ns2:Indicator ;
	skos:prefLabel	"2.4 ICT specialists" ;
	dct:source	ns5: ;
	skos:notation	"rid_ius_icts" ;
	skos:altLabel	"2.4 ICT specialists" ;
	ns6:membership	ns37:rid_ius_icts ;
	skos:definition	"Employed ICT specialists. Broad definition based on the ISCO-08 classification and including jobs like ICT service managers, ICT professionals, ICT technicians, ICT installers and servicers." ;
	skos:topConceptOf	ns8:indicator .
ns1:rid_ius_ss	rdf:type	skos:Concept ,
		ns2:Indicator ;
	skos:prefLabel	"2.3 At least basic digital content creation skills" ;
	dct:source	ns5: ;
	skos:notation	"rid_ius_ss" ;
	skos:altLabel	"2.3 At least basic digital content creation skills" ;
	ns6:membership	ns37:rid_ius_ss ;
	skos:definition	"Individuals with a basic level in using software for digital content creation" ;
	skos:topConceptOf	ns8:indicator .
ns1:rid_score	rdf:type	skos:Concept ,
		ns2:Indicator ;
	skos:prefLabel	"Rural Digital Index" ;
	dct:source	ns5: ;
	skos:notation	"rid_score" ;
	skos:altLabel	"Rural Digital Index" ;
	ns6:membership	ns37:rid_score ;
	skos:definition	"Rural Digital Index score calculated as the weighted average of the three sub-dimensions: 1 Use of internet  (33.3%), 2 Human Capital (33.3%), 3 Connectivity (33.3%).\n\n" ;
	skos:topConceptOf	ns8:indicator .
ns1:rid_ui	rdf:type	skos:Concept ,
		ns2:Indicator ;
	skos:prefLabel	"1 Use of internet" ;
	dct:source	ns5: ;
	skos:notation	"rid_ui" ;
	skos:altLabel	"1 Use of internet" ;
	ns6:membership	ns37:rid_ui ;
	skos:definition	"Use of internet dimension calculated as the weighted average of the six indicators: \r\n1.1 Regular internet use (16.67%), 1.2 People who never used the internet (16.67%), 1.3 Online banking (16.67%), 1.4 Doing an online course (16.67%), 1.5 Online consultations or voting (16.67%), 1.6 eGovernment users (16.67%)." ;
	skos:topConceptOf	ns8:indicator .
ns1:rid_ui_egov	rdf:type	skos:Concept ,
		ns2:Indicator ;
	skos:prefLabel	"1.6 eGovernment users " ;
	dct:source	ns5: ;
	skos:notation	"rid_ui_egov" ;
	skos:altLabel	"1.6 eGovernment users " ;
	ns6:membership	ns37:rid_ui_egov ;
	skos:definition	"Individuals that have used Internet, in the last 12 months, for interaction with public authorities. It includes obtaining information from public authorities web sites, OR downloading official forms OR sending filled in forms. Unit of measure: Percentage of individuals who used Internet within the last 12 months" ;
	skos:topConceptOf	ns8:indicator .
ns1:rid_ui_ib	rdf:type	skos:Concept ,
		ns2:Indicator ;
	skos:prefLabel	"1.3 Online banking" ;
	dct:source	ns5: ;
	skos:notation	"rid_ui_ib" ;
	skos:altLabel	"1.3 Online banking" ;
	ns6:membership	ns37:rid_ui_ib ;
	skos:definition	"People who used the Internet to use online banking " ;
	skos:topConceptOf	ns8:indicator .
ns1:rid_ui_iu	rdf:type	skos:Concept ,
		ns2:Indicator ;
	skos:prefLabel	"1.1 Regular internet use" ;
	dct:source	ns5: ;
	skos:notation	"rid_ui_iu" ;
	skos:altLabel	"1.1 Regular internet use" ;
	ns6:membership	ns37:rid_ui_iu ;
	skos:definition	"People who used the Internet at least once a week" ;
	skos:topConceptOf	ns8:indicator .
ns1:rid_ui_nui	rdf:type	skos:Concept ,
		ns2:Indicator ;
	skos:prefLabel	"1.2 People who never used the internet" ;
	dct:source	ns5: ;
	skos:notation	"rid_ui_nui" ;
	skos:altLabel	"1.2 People who never used the internet" ;
	ns6:membership	ns37:rid_ui_nui ;
	skos:definition	"People who never used the Internet" ;
	skos:topConceptOf	ns8:indicator .
ns1:rid_ui_oc	rdf:type	skos:Concept ,
		ns2:Indicator ;
	skos:prefLabel	"1.4 Doing an online course" ;
	dct:source	ns5: ;
	skos:notation	"rid_ui_oc" ;
	skos:altLabel	"1.4 Doing an online course" ;
	ns6:membership	ns37:rid_ui_oc ;
	skos:definition	"People who used the Internet for doing an online course (on any subject)" ;
	skos:topConceptOf	ns8:indicator .
ns1:rid_ui_part	rdf:type	skos:Concept ,
		ns2:Indicator ;
	skos:prefLabel	"1.5 Online consultations or voting" ;
	dct:source	ns5: ;
	skos:notation	"rid_ui_part" ;
	skos:altLabel	"1.5 Online consultations or voting" ;
	ns6:membership	ns37:rid_ui_part ;
	skos:definition	"People who took part in on-line consultations or voting to define civic or political issues (e.g. urban planning, signing a petition)" ;
	skos:topConceptOf	ns8:indicator .
ns37:rid_ui	rdf:type	ns2:IndicatorToGroupMembership ;
	rdfs:label	"rid" ;
	ns6:member-of	ns14:rid ;
	ns6:order	"2" .
ns1:e_di4_hi	rdf:type	skos:Concept ,
		ns2:Indicator ;
	skos:prefLabel	"Enterprises with high digital intensity index (DII v4)" ;
	dct:source	ns5:estat-ent ;
	skos:notation	"e_di4_hi" ;
	skos:altLabel	"Enterprises with high digital intensity index (DII v4)" ;
	ns6:membership	ns7:e_di4_hi ;
	skos:definition	"Enterprises with high digital intensity index (DII v4)" ;
	skos:topConceptOf	ns8:indicator .
ns1:e_di4_lo	rdf:type	ns2:Indicator ,
		skos:Concept ;
	skos:prefLabel	"Enterprises with low digital intensity index (DII v4)" ;
	dct:source	ns5:estat-ent ;
	skos:notation	"e_di4_lo" ;
	skos:altLabel	"Enterprises with low digital intensity index (DII v4)" ;
	ns6:membership	ns7:e_di4_lo ;
	skos:definition	"Enterprises with low digital intensity index (DII v4)" ;
	skos:topConceptOf	ns8:indicator .
ns1:e_di4_vhi	rdf:type	ns2:Indicator ,
		skos:Concept ;
	skos:prefLabel	"Enterprises with very high digital intensity index (DII v4)" ;
	dct:source	ns5:estat-ent ;
	skos:notation	"e_di4_vhi" ;
	skos:altLabel	"Enterprises with very high digital intensity index (DII v4)" ;
	ns6:membership	ns7:e_di4_vhi ;
	skos:definition	"Enterprises with very high digital intensity index (DII v4)" ;
	skos:topConceptOf	ns8:indicator .
ns1:e_di4_vlo	rdf:type	ns2:Indicator ,
		skos:Concept ;
	skos:prefLabel	"Enterprises with very low digital intensity index (DII v4)" ;
	dct:source	ns5:estat-ent ;
	skos:notation	"e_di4_vlo" ;
	skos:altLabel	"Enterprises with very low digital intensity index (DII v4)" ;
	ns6:membership	ns7:e_di4_vlo ;
	skos:definition	"Enterprises with very low digital intensity index (DII v4)" ;
	skos:topConceptOf	ns8:indicator .
ns17:bb_rvhcncov	rdf:type	ns2:IndicatorToGroupMembership ;
	rdfs:label	"broadband" ;
	ns6:member-of	ns14:broadband ;
	ns6:order	"2" .
ns17:bb_vhcncov	rdf:type	ns2:IndicatorToGroupMembership ;
	rdfs:label	"broadband" ;
	ns6:member-of	ns14:broadband ;
	ns6:order	"1" .
ns22:e_gov_1_uc	rdf:type	ns2:IndicatorToGroupMembership ;
	rdfs:label	"egovernment" ;
	ns6:member-of	ns14:egovernment ;
	ns6:order	"1111" .
ns22:e_gov_1a_uc_oa	rdf:type	ns2:IndicatorToGroupMembership ;
	rdfs:label	"egovernment" ;
	ns6:member-of	ns14:egovernment ;
	ns6:order	"11111" .
ns22:e_gov_1b_uc_mf	rdf:type	ns2:IndicatorToGroupMembership ;
	rdfs:label	"egovernment" ;
	ns6:member-of	ns14:egovernment ;
	ns6:order	"11112" .
ns22:e_gov_1c_uc_us	rdf:type	ns2:IndicatorToGroupMembership ;
	rdfs:label	"egovernment" ;
	ns6:member-of	ns14:egovernment ;
	ns6:order	"11113" .
ns22:e_gov_2_tr	rdf:type	ns2:IndicatorToGroupMembership ;
	rdfs:label	"egovernment" ;
	ns6:member-of	ns14:egovernment ;
	ns6:order	"1112" .
ns22:e_gov_2a_tr_sd	rdf:type	ns2:IndicatorToGroupMembership ;
	rdfs:label	"egovernment" ;
	ns6:member-of	ns14:egovernment ;
	ns6:order	"11121" .
ns22:e_gov_2x_tr_po	rdf:type	ns2:IndicatorToGroupMembership ;
	rdfs:label	"egovernment" ;
	ns6:member-of	ns14:egovernment ;
	ns6:order	"11124" .
ns22:e_gov_3_ke	rdf:type	ns2:IndicatorToGroupMembership ;
	rdfs:label	"egovernment" ;
	ns6:member-of	ns14:egovernment ;
	ns6:order	"1113" .
ns22:e_gov_3a_ke_eid	rdf:type	ns2:IndicatorToGroupMembership ;
	rdfs:label	"egovernment" ;
	ns6:member-of	ns14:egovernment ;
	ns6:order	"11131" .
ns22:e_gov_3b_ke_edoc	rdf:type	ns2:IndicatorToGroupMembership ;
	rdfs:label	"egovernment" ;
	ns6:member-of	ns14:egovernment ;
	ns6:order	"11132" .
ns22:e_gov_3c_ke_as	rdf:type	ns2:IndicatorToGroupMembership ;
	rdfs:label	"egovernment" ;
	ns6:member-of	ns14:egovernment ;
	ns6:order	"11133" .
ns22:e_gov_3d_ke_dp	rdf:type	ns2:IndicatorToGroupMembership ;
	rdfs:label	"egovernment" ;
	ns6:member-of	ns14:egovernment ;
	ns6:order	"11134" .
ns22:e_gov_4_cb	rdf:type	ns2:IndicatorToGroupMembership ;
	rdfs:label	"egovernment" ;
	ns6:member-of	ns14:egovernment ;
	ns6:order	"1114" .
ns22:e_gov_4a_cb_oa	rdf:type	ns2:IndicatorToGroupMembership ;
	rdfs:label	"egovernment" ;
	ns6:member-of	ns14:egovernment ;
	ns6:order	"11141" .
ns22:e_gov_4b_cb_us	rdf:type	ns2:IndicatorToGroupMembership ;
	rdfs:label	"egovernment" ;
	ns6:member-of	ns14:egovernment ;
	ns6:order	"11142" .
ns22:e_gov_4c_cb_eid	rdf:type	ns2:IndicatorToGroupMembership ;
	rdfs:label	"egovernment" ;
	ns6:member-of	ns14:egovernment ;
	ns6:order	"11143" .
ns22:e_gov_4d_cb_edoc	rdf:type	ns2:IndicatorToGroupMembership ;
	rdfs:label	"egovernment" ;
	ns6:member-of	ns14:egovernment ;
	ns6:order	"11144" .
ns22:e_gov_dpsc	rdf:type	ns2:IndicatorToGroupMembership ;
	rdfs:label	"egovernment" ;
	ns6:member-of	ns14:egovernment ;
	ns6:order	"7" .
ns22:e_gov_od	rdf:type	ns2:IndicatorToGroupMembership ;
	rdfs:label	"egovernment" ;
	ns6:member-of	ns14:egovernment ;
	ns6:order	"5" .
<http://semantic.digital-agenda-data.eu/codelist/indicator-group/mobile/5g_read>	rdf:type	ns2:IndicatorToGroupMembership ;
	rdfs:label	"mobile" ;
	ns6:member-of	ns14:mobile ;
	ns6:order	"3" .
ns30:mbb_5gcov	rdf:type	ns2:IndicatorToGroupMembership ;
	rdfs:label	"mobile" ;
	ns6:member-of	ns14:mobile ;
	ns6:order	"1" .
ns30:mbb_r5gcov	rdf:type	ns2:IndicatorToGroupMembership ;
	rdfs:label	"mobile" ;
	ns6:member-of	ns14:mobile ;
	ns6:order	"2" .
<http://semantic.digital-agenda-data.eu/codelist/indicator/5g_read>	rdf:type	ns2:Indicator ,
		skos:Concept ;
	skos:prefLabel	"5G spectrum" ;
	dct:source	ns5:cocom_new ;
	skos:notation	"5g_read" ;
	skos:altLabel	"5G spectrum" ;
	ns6:membership	<http://semantic.digital-agenda-data.eu/codelist/indicator-group/mobile/5g_read> ;
	skos:definition	"The amount of spectrum assigned and ready for 5G use within the so-called 5G pioneer bands. These bands are 700 MHz (703-733 MHz and 758-788 MHz), 3.6 GHz (3400-3800 MHz) and 26 GHz (1000 MHz within 24250-27500 MHz). All three spectrum bands have an equal weight." ;
	skos:topConceptOf	ns8:indicator .
ns1:bb_rvhcncov	rdf:type	ns2:Indicator ,
		skos:Concept ;
	skos:prefLabel	"Rural Fixed Very High Capacity Network (VHCN) coverage" ;
	dct:source	ns5:bc2020 ;
	skos:notation	"bb_rvhcncov" ;
	skos:altLabel	"Rural Fixed Very High Capacity Network (VHCN) coverage" ;
	ns6:membership	ns17:bb_rvhcncov ;
	skos:definition	"Percentage of households covered by any fixed VHCN. The technologies considered are FTTH and FTTB for 2015-2018 and FTTH, FTTB and Cable Docsis 3.1 for 2019 onwards." ;
	skos:topConceptOf	ns8:indicator .
ns1:bb_vhcncov	rdf:type	ns2:Indicator ,
		skos:Concept ;
	skos:prefLabel	"Fixed Very High Capacity Network (VHCN) coverage" ;
	dct:source	ns5:bc2020 ;
	skos:notation	"bb_vhcncov" ;
	skos:altLabel	"Fixed Very High Capacity Network (VHCN) coverage" ;
	ns6:membership	ns17:bb_vhcncov ;
	skos:definition	"Percentage of households covered by any fixed VHCN. The technologies considered are FTTH and FTTB for 2015-2018 and FTTH, FTTB and Cable Docsis 3.1 for 2019 onwards.\nRural areas are defined as those with less than 100 people per km2." ;
	skos:topConceptOf	ns8:indicator .
ns1:e_gov_1_uc	rdf:type	ns2:Indicator ,
		skos:Concept ;
	skos:prefLabel	"1 User centricity" ;
	dct:source	ns5: ;
	skos:notation	"e_gov_1_uc" ;
	skos:altLabel	"1 User centricity" ;
	ns6:membership	ns22:e_gov_1_uc ;
	skos:definition	"The extent to which information and services are available online, supported online and compatible with mobile devices.D362" ;
	skos:topConceptOf	ns8:indicator .
ns1:e_gov_1a_uc_oa	rdf:type	ns2:Indicator ,
		skos:Concept ;
	skos:prefLabel	"1.1 User centricity - Online availability" ;
	dct:source	ns5:egov_bench ;
	skos:notation	"e_gov_1a_uc_oa" ;
	skos:altLabel	"1.1 User centricity - Online availability" ;
	ns6:membership	ns22:e_gov_1a_uc_oa ;
	skos:definition	"The extent to which informational and transactional services and information concerning these services is provided online, and can be reached via a portal website." ;
	skos:topConceptOf	ns8:indicator .
ns1:e_gov_1b_uc_mf	rdf:type	ns2:Indicator ,
		skos:Concept ;
	skos:prefLabel	"1.2 User centricity - Mobile friendliness" ;
	dct:source	ns5:egov_bench ;
	skos:notation	"e_gov_1b_uc_mf" ;
	skos:altLabel	"1.2 User centricity - Mobile friendliness" ;
	ns6:membership	ns22:e_gov_1b_uc_mf ;
	skos:definition	"The extent to which services are provided through a mobile-friendly interface, an interface that is responsive to the mobile device." ;
	skos:topConceptOf	ns8:indicator .
ns1:e_gov_1c_uc_us	rdf:type	ns2:Indicator ,
		skos:Concept ;
	skos:prefLabel	"1.3 User centricity - User support" ;
	dct:source	ns5:egov_bench ;
	skos:notation	"e_gov_1c_uc_us" ;
	skos:altLabel	"1.3 User centricity - User support" ;
	ns6:membership	ns22:e_gov_1c_uc_us ;
	skos:definition	"The extent to which online support, help features, and feedback mechanisms are available." ;
	skos:topConceptOf	ns8:indicator .
ns1:e_gov_2_tr	rdf:type	ns2:Indicator ,
		skos:Concept ;
	skos:prefLabel	"2 Transparency" ;
	dct:source	ns5:egov_bench ;
	skos:notation	"e_gov_2_tr" ;
	skos:altLabel	"2 Transparency" ;
	ns6:membership	ns22:e_gov_2_tr ;
	skos:definition	"The extent to which service processes are transparent, services are designed with user involvement and users can manage their personal data." ;
	skos:topConceptOf	ns8:indicator .
ns1:e_gov_2a_tr_sd	rdf:type	ns2:Indicator ,
		skos:Concept ;
	skos:prefLabel	"2.1 Transparency - Transparency of service delivery" ;
	dct:source	ns5:egov_bench ;
	skos:notation	"e_gov_2a_tr_sd" ;
	skos:altLabel	"2.1 Transparency - Transparency of service delivery" ;
	ns6:membership	ns22:e_gov_2a_tr_sd ;
	skos:definition	"The extent to which the service process and expectations are clarified." ;
	skos:topConceptOf	ns8:indicator .
ns1:e_gov_2x_tr_po	rdf:type	ns2:Indicator ,
		skos:Concept ;
	skos:prefLabel	"2.X Transparency - Transparency of public organisations (old indicator)" ;
	dct:source	ns5:egov_bench ;
	skos:notation	"e_gov_2x_tr_po" ;
	skos:altLabel	"2.X Transparency - Transparency of public organisations (old indicator)" ;
	ns6:membership	ns22:e_gov_2x_tr_po ;
	skos:definition	"The extent to which public administrations publish information about their organisations (e.g. finance, organisational structure and responsibilities), and about their activities (e.g. the decision-making processes and regulations). " ;
	skos:note	"This indicator has been discontinued starting from 2020" ;
	skos:topConceptOf	ns8:indicator .
ns1:e_gov_3_ke	rdf:type	skos:Concept ,
		ns2:Indicator ;
	skos:prefLabel	"3 Key Enablers" ;
	dct:source	ns5:egov_bench ;
	skos:notation	"e_gov_3_ke" ;
	skos:altLabel	"3 Key Enablers" ;
	ns6:membership	ns22:e_gov_3_ke ;
	skos:definition	"The extent to which main IT enablers (eIDs, eDocuments, Authentic sources, Digital post and security) are available during services processes, which can be used to assess the presence of the technical pre-conditions of the efficient and effective use of online services." ;
	skos:topConceptOf	ns8:indicator .
ns1:e_gov_3a_ke_eid	rdf:type	skos:Concept ,
		ns2:Indicator ;
	skos:prefLabel	"3.1 Key enablers - eID" ;
	dct:source	ns5:egov_bench ;
	skos:notation	"e_gov_3a_ke_eid" ;
	skos:altLabel	"3.1 Key enablers - eID" ;
	ns6:membership	ns22:e_gov_3a_ke_eid ;
	skos:definition	"The extent to which electronic Identification (eID), any means accepted by eGovernment services (e.g. smartcards, username and password) for online identification, can be used during service processes." ;
	skos:topConceptOf	ns8:indicator .
ns1:e_gov_3b_ke_edoc	rdf:type	skos:Concept ,
		ns2:Indicator ;
	skos:prefLabel	"3.2 Key enabler - eDocuments" ;
	dct:source	ns5:egov_bench ;
	skos:notation	"e_gov_3b_ke_edoc" ;
	skos:altLabel	"3.2 Key enabler - eDocuments" ;
	ns6:membership	ns22:e_gov_3b_ke_edoc ;
	skos:definition	"The extent to which electronic documents (eDocuments), any document in digital form that the user needs to submit/upload in order to complete an eGovernment service, or that the user obtains as a proof or a result of the service (e.g. certificate, diploma, proof of registration) can be used during service processes. " ;
	skos:topConceptOf	ns8:indicator .
ns1:e_gov_3c_ke_as	rdf:type	skos:Concept ,
		ns2:Indicator ;
	skos:prefLabel	"3.3 Key enabler - Authentic sources" ;
	dct:source	ns5:egov_bench ;
	skos:notation	"e_gov_3c_ke_as" ;
	skos:altLabel	"3.3 Key enabler - Authentic sources" ;
	ns6:membership	ns22:e_gov_3c_ke_as ;
	skos:definition	"The extent to which Authentic Sources, base registries used by governments to automatically validate or fetch data relating to citizens or businesses, can be used during the service process." ;
	skos:topConceptOf	ns8:indicator .
ns1:e_gov_3d_ke_dp	rdf:type	skos:Concept ,
		ns2:Indicator ;
	skos:prefLabel	"3.4 Key enabler - Digital Post" ;
	dct:source	ns5:egov_bench ;
	skos:notation	"e_gov_3d_ke_dp" ;
	skos:altLabel	"3.4 Key enabler - Digital Post" ;
	ns6:membership	ns22:e_gov_3d_ke_dp ;
	skos:definition	"The extent to which public authorities allow citizens to receive communications digitally only and opt-out for paper mailings. Digital Post refers to the possibility that governments communicate electronically-only with citizens or entrepreneurs through e.g. personal mailboxes or other digital postal solutions." ;
	skos:topConceptOf	ns8:indicator .
ns1:e_gov_4_cb	rdf:type	skos:Concept ,
		ns2:Indicator ;
	skos:prefLabel	"4 Cross-border services" ;
	dct:source	ns5:egov_bench ;
	skos:notation	"e_gov_4_cb" ;
	skos:altLabel	"4 Cross-border services" ;
	ns6:membership	ns22:e_gov_4_cb ;
	skos:definition	"The extent to which information and services are available online, usable, and integrated with eIDs and eDocuments for users from other European countries." ;
	skos:topConceptOf	ns8:indicator .
ns1:e_gov_4a_cb_oa	rdf:type	skos:Concept ,
		ns2:Indicator ;
	skos:prefLabel	"4.1 Cross-border services - Cross-border online availability" ;
	dct:source	ns5:egov_bench ;
	skos:notation	"e_gov_4a_cb_oa" ;
	skos:altLabel	"4.1 Cross-border services - Cross-border online availability" ;
	ns6:membership	ns22:e_gov_4a_cb_oa ;
	skos:definition	"The extent to which informational and transactional services and information concerning these services is provided online for users from other European countries." ;
	skos:topConceptOf	ns8:indicator .
ns1:e_gov_4b_cb_us	rdf:type	skos:Concept ,
		ns2:Indicator ;
	skos:prefLabel	"4.2 Cross-border services - Cross-border user support" ;
	dct:source	ns5:egov_bench ;
	skos:notation	"e_gov_4b_cb_us" ;
	skos:altLabel	"4.2 Cross-border services - Cross-border user support" ;
	ns6:membership	ns22:e_gov_4b_cb_us ;
	skos:definition	"The extent to which online support, help features, and feedback mechanisms are available for users from other European countries." ;
	skos:topConceptOf	ns8:indicator .
ns1:e_gov_4c_cb_eid	rdf:type	skos:Concept ,
		ns2:Indicator ;
	skos:prefLabel	"4.3 Cross-border services - Cross-border eID" ;
	dct:source	ns5:egov_bench ;
	skos:notation	"e_gov_4c_cb_eid" ;
	skos:altLabel	"4.3 Cross-border services - Cross-border eID" ;
	ns6:membership	ns22:e_gov_4c_cb_eid ;
	skos:definition	"The extent to which electronic Identification (eID) can be used during service processes by users from other European countries, a government-issued document for online identification, and authentication." ;
	skos:topConceptOf	ns8:indicator .
ns1:e_gov_4d_cb_edoc	rdf:type	skos:Concept ,
		ns2:Indicator ;
	skos:prefLabel	"4.4 Cross-border services - Cross-border eDocuments" ;
	dct:source	ns5:egov_bench ;
	skos:notation	"e_gov_4d_cb_edoc" ;
	skos:altLabel	"4.4 Cross-border services - Cross-border eDocuments" ;
	ns6:membership	ns22:e_gov_4d_cb_edoc ;
	skos:definition	"The extent to which electronic documents (eDocuments) can be used during service processes by users from other European countries, documents that have been authenticated by its issuer using any means recognised under applicable national law, specifically through the use of electronic signatures, e.g. not a regular PDF or Word file." ;
	skos:topConceptOf	ns8:indicator .
ns1:mbb_5gcov	rdf:type	skos:Concept ,
		ns2:Indicator ;
	skos:prefLabel	"5G mobile broadband coverage (as a % of households)" ;
	dct:source	ns5:bc2020 ;
	skos:notation	"mbb_5gcov" ;
	skos:altLabel	"5G mobile broadband coverage" ;
	ns6:membership	ns30:mbb_5gcov ;
	skos:definition	"Coverage is a supply indicator defined as the percentage of Households living in areas covered by fifth generation mobile broadband. " ;
	skos:topConceptOf	ns8:indicator .
ns1:mbb_r5gcov	rdf:type	skos:Concept ,
		ns2:Indicator ;
	skos:prefLabel	"Rural 5G mobile broadband coverage (as a % of households)" ;
	dct:source	ns5:bc2020 ;
	skos:notation	"mbb_r5gcov" ;
	skos:altLabel	"Rural 5G mobile broadband coverage" ;
	ns6:membership	ns30:mbb_r5gcov ;
	skos:definition	"Coverage is a supply indicator defined as the percentage of Households living in areas covered by fifth generation mobile broadband. \nRural areas are defined as those with less than 100 people per km2." ;
	skos:topConceptOf	ns8:indicator .
ns1:desi_5g	rdf:type	ns2:Indicator ,
		skos:Concept ;
	skos:prefLabel	"5G spectrum" ;
	dct:source	ns5:desi_5g ;
	skos:notation	"desi_5g" ;
	skos:altLabel	"5G spectrum" ;
	ns6:membership	ns36:desi_5g ;
	skos:definition	"The amount of spectrum assigned and ready for 5G use by the end of 2020 within the so-called 5G pioneer bands. These bands are 700 MHz (703-733 MHz and 758-788 MHz), 3.6 GHz (3400-3800 MHz) and 26 GHz (1000 MHz within 24250-27500 MHz). All three spectrum bands have an equal weight" ;
	skos:topConceptOf	ns8:indicator .
ns1:desi_5gc	rdf:type	ns2:Indicator ,
		skos:Concept ;
	skos:prefLabel	"5G coverage" ;
	dct:source	ns5:desi_5gc ;
	skos:notation	"desi_5gc" ;
	skos:altLabel	"5G coverage" ;
	ns6:membership	ns36:desi_5gc ;
	skos:definition	"Percentage of populated areas with coverage by 5G" ;
	skos:topConceptOf	ns8:indicator .
ns1:desi_bbpi	rdf:type	ns2:Indicator ,
		skos:Concept ;
	skos:prefLabel	"Broadband price index" ;
	dct:source	ns5:desi_bbpi ;
	skos:notation	"desi_bbpi" ;
	skos:altLabel	"Broadband price index" ;
	ns6:membership	ns36:desi_bbpi ;
	skos:definition	"The broadband price index measures the prices of representative baskets of fixed, mobile and converged broadband offers" ;
	skos:topConceptOf	ns8:indicator .
ns1:desi_c_bbpi	rdf:type	ns2:Indicator ,
		skos:Concept ;
	skos:prefLabel	"Broadband price index" ;
	dct:source	ns5: ;
	skos:notation	"desi_c_bbpi" ;
	skos:altLabel	"Broadband price index" .
@prefix ns38:	<http://semantic.digital-agenda-data.eu/codelist/indicator-group/desi_subdim/> .
ns1:desi_c_bbpi	ns6:membership	ns38:desi_c_bbpi ;
	skos:topConceptOf	ns8:indicator .
ns1:desi_c_fbbc	rdf:type	ns2:Indicator ,
		skos:Concept ;
	skos:prefLabel	"Fixed broadband coverage" ;
	dct:source	ns5: ;
	skos:notation	"desi_c_fbbc" ;
	skos:altLabel	"Fixed broadband coverage" ;
	ns6:membership	ns38:desi_c_fbbc ;
	skos:topConceptOf	ns8:indicator .
ns1:desi_c_fbbtc	rdf:type	ns2:Indicator ,
		skos:Concept ;
	skos:prefLabel	"Fixed broadband take-up" ;
	dct:source	ns5: ;
	skos:notation	"desi_c_fbbtc" ;
	skos:altLabel	"Fixed broadband take-up" ;
	ns6:membership	ns38:desi_c_fbbtc ;
	skos:topConceptOf	ns8:indicator .
ns1:desi_c_mbb	rdf:type	ns2:Indicator ,
		skos:Concept ;
	skos:prefLabel	"Mobile broadband" ;
	dct:source	ns5: ;
	skos:notation	"desi_c_mbb" ;
	skos:altLabel	"Mobile broadband" ;
	ns6:membership	ns38:desi_c_mbb ;
	skos:topConceptOf	ns8:indicator .
ns1:desi_conn	rdf:type	ns2:Indicator ,
		skos:Concept ;
	skos:prefLabel	"Connectivity" ;
	dct:source	ns5: ;
	skos:notation	"desi_conn" ;
	skos:altLabel	"Connectivity" .
@prefix ns39:	<http://semantic.digital-agenda-data.eu/codelist/indicator-group/desi_dim/> .
ns1:desi_conn	ns6:membership	ns39:desi_conn ;
	skos:topConceptOf	ns8:indicator .
ns1:desi_dps	rdf:type	ns2:Indicator ,
		skos:Concept ;
	skos:prefLabel	"Digital Public Services" ;
	dct:source	ns5: ;
	skos:notation	"desi_dps" ;
	skos:altLabel	"Digital Public Services" ;
	ns6:membership	ns39:desi_dps ;
	skos:topConceptOf	ns8:indicator .
ns1:desi_dps_egov	rdf:type	ns2:Indicator ,
		skos:Concept ;
	skos:prefLabel	"e-Government" ;
	dct:source	ns5: ;
	skos:notation	"desi_dps_egov" ;
	skos:altLabel	"e-Government" ;
	ns6:membership	ns38:desi_dps_egov ;
	skos:topConceptOf	ns8:indicator .
ns1:desi_dps_egovuser	rdf:type	ns2:Indicator ,
		skos:Concept ;
	skos:prefLabel	"e-Government Users" ;
	dct:source	ns5:desi_dps_egovuser ;
	skos:notation	"desi_dps_egovuser" ;
	skos:altLabel	"e-Government Users" ;
	ns6:membership	ns36:desi_dps_egovuser ;
	skos:definition	"Individuals who used the Internet, in the last 12 months, for interaction with public authorities" ;
	skos:topConceptOf	ns8:indicator .
ns1:desi_dps_opendata	rdf:type	ns2:Indicator ,
		skos:Concept ;
	skos:prefLabel	"Open Data" ;
	dct:source	ns5:desi_dps_opendata ;
	skos:notation	"desi_dps_opendata" ;
	skos:altLabel	"Open Data" ;
	ns6:membership	ns36:desi_dps_opendata ;
	skos:definition	"This composite indicator measures to what extent countries have an open data policy in place (including the transposition of the revised PSI Directive), the estimated political, social and economic impact of open data and the characteristics (functionalities, data availability and usage) of the national data portal." ;
	skos:topConceptOf	ns8:indicator .
ns1:desi_dps_psbiz	rdf:type	ns2:Indicator ,
		skos:Concept ;
	skos:prefLabel	"Digital public services for businesses" ;
	dct:source	ns5:desi_dps_psbiz ;
	skos:notation	"desi_dps_psbiz" ;
	skos:altLabel	"Digital public services for businesses" ;
	ns6:membership	ns36:desi_dps_psbiz ;
	skos:definition	"The indicator broadly reflects the share of public services needed for starting a business and conducting regular business operations that are available online for domestic as well as foreign users. Services provided through a portal receive a higher score, services which provide only information (but have to be completed offline) receive a more limited score." ;
	skos:topConceptOf	ns8:indicator .
ns1:desi_fbbc	rdf:type	ns2:Indicator ,
		skos:Concept ;
	skos:prefLabel	"Fast BB (NGA) coverage" ;
	dct:source	ns5:desi_fbbc ;
	skos:notation	"desi_fbbc" ;
	skos:altLabel	"Fast broadband (NGA) coverage" ;
	ns6:membership	ns36:desi_fbbc ;
	skos:definition	"Percentage of households covered by fixed broadband of at least 30 Mbps download. The technologies considered are FTTH, FTTB, Cable Docsis 3.0 and VDS" ;
	skos:topConceptOf	ns8:indicator .
ns1:desi_fbbtc	rdf:type	skos:Concept ,
		ns2:Indicator ;
	skos:prefLabel	"Overall fixed BB take-up" ;
	dct:source	ns5:desi_fbbtc ;
	skos:notation	"desi_fbbtc" ;
	skos:altLabel	"Overall fixed broadband take-up" ;
	ns6:membership	ns36:desi_fbbtc ;
	skos:definition	"Percentage of households subscribing to fixed broadband" ;
	skos:topConceptOf	ns8:indicator .
ns1:desi_gbpstc	rdf:type	skos:Concept ,
		ns2:Indicator ;
	skos:prefLabel	"At least 1 Gbps take-up" ;
	dct:source	ns5:desi_gbpstc ;
	skos:notation	"desi_gbpstc" ;
	skos:altLabel	"At least 1 Gbps take-up" ;
	ns6:membership	ns36:desi_gbpstc ;
	skos:definition	"Percentage of households subscribing to fixed broadband of at least 1 Gbps, calculated as overall fixed broadband take-up " ;
	skos:topConceptOf	ns8:indicator .
ns1:desi_hc	rdf:type	skos:Concept ,
		ns2:Indicator ;
	skos:prefLabel	"Human Capital" ;
	dct:source	ns5: ;
	skos:notation	"desi_hc" ;
	skos:altLabel	"Human Capital" ;
	ns6:membership	ns39:desi_hc ;
	skos:topConceptOf	ns8:indicator .
ns1:desi_hc_abds	rdf:type	skos:Concept ,
		ns2:Indicator ;
	skos:prefLabel	"Above basic digital skills" ;
	dct:source	ns5:desi_hc_abds ;
	skos:notation	"desi_hc_abds" ;
	skos:altLabel	"Above basic digital skills" ;
	ns6:membership	ns36:desi_hc_abds ;
	skos:definition	"Individuals with \u2018above basic\u2019 digital skills in each of the following five dimensions: information, communication, problem solving, software for content creation and safety" ;
	skos:topConceptOf	ns8:indicator .
ns1:desi_hc_abss	rdf:type	skos:Concept ,
		ns2:Indicator ;
	skos:prefLabel	"At least basic digital content creation skills" ;
	dct:source	ns5:desi_hc_abss ;
	skos:notation	"desi_hc_abss" ;
	skos:altLabel	"At least basic digital content creation skills" ;
	ns6:membership	ns36:desi_hc_abss ;
	skos:definition	"Individuals with a basic level in using software for digital content creation" ;
	skos:topConceptOf	ns8:indicator .
ns1:desi_hc_asd	rdf:type	skos:Concept ,
		ns2:Indicator ;
	skos:prefLabel	"Advanced Skills and Development" ;
	dct:source	ns5: ;
	skos:notation	"desi_hc_asd" ;
	skos:altLabel	"Advanced Skills and Development" ;
	ns6:membership	ns38:desi_hc_asd ;
	skos:topConceptOf	ns8:indicator .
ns1:desi_hc_bds	rdf:type	skos:Concept ,
		ns2:Indicator ;
	skos:prefLabel	"At least Basic Digital Skills" ;
	dct:source	ns5:desi_hc_bds ;
	skos:notation	"desi_hc_bds" ;
	skos:altLabel	"At least Basic Digital Skills" ;
	ns6:membership	ns36:desi_hc_bds ;
	skos:definition	"Individuals with \u2018basic\u2019 or \u2018above basic\u2019 digital skills in each of the following five dimensions: information, communication, problem solving, software for content creation and safety" ;
	skos:topConceptOf	ns8:indicator .
ns1:desi_hc_bsu	rdf:type	skos:Concept ,
		ns2:Indicator ;
	skos:prefLabel	"Internet User Skills" ;
	dct:source	ns5: ;
	skos:notation	"desi_hc_bsu" ;
	skos:altLabel	"Internet User Skills" ;
	ns6:membership	ns38:desi_hc_bsu ;
	skos:topConceptOf	ns8:indicator .
ns1:desi_hc_entict	rdf:type	skos:Concept ,
		ns2:Indicator ;
	skos:prefLabel	"Enterprises providing ICT training " ;
	dct:source	ns5:desi_hc_entict ;
	skos:notation	"desi_hc_entict" ;
	skos:altLabel	"Enterprises providing ICT training " ;
	ns6:membership	ns36:desi_hc_entict ;
	skos:definition	"Enterprises who provided training in ICT to their personnel" ;
	skos:topConceptOf	ns8:indicator .
ns1:desi_hc_fictspec	rdf:type	skos:Concept ,
		ns2:Indicator ;
	skos:prefLabel	"Female ICT specialists" ;
	dct:source	ns5:desi_hc_fictspec ;
	skos:notation	"desi_hc_fictspec" ;
	skos:altLabel	"Female ICT specialists" ;
	ns6:membership	ns36:desi_hc_fictspec ;
	skos:definition	"Employed female ICT specialists. Broad definition based on the ISCO-08 classification and including jobs like ICT service managers, ICT professionals, ICT technicians, ICT installers and servicers." ;
	skos:topConceptOf	ns8:indicator .
ns1:desi_hc_ictg	rdf:type	skos:Concept ,
		ns2:Indicator ;
	skos:prefLabel	"ICT graduates" ;
	dct:source	ns5:desi_hc_ictg ;
	skos:notation	"desi_hc_ictg" ;
	skos:altLabel	"ICT graduates" ;
	ns6:membership	ns36:desi_hc_ictg ;
	skos:definition	"Individuals with a degree in ICT" ;
	skos:topConceptOf	ns8:indicator .
ns1:desi_hc_ictspec	rdf:type	skos:Concept ,
		ns2:Indicator ;
	skos:prefLabel	"ICT Specialists" ;
	dct:source	ns5:desi_hc_ictspec ;
	skos:notation	"desi_hc_ictspec" ;
	skos:altLabel	"ICT Specialists" ;
	ns6:membership	ns36:desi_hc_ictspec ;
	skos:definition	"Employed ICT specialists. Broad definition based on the ISCO-08 classification and including jobs like ICT service managers, ICT professionals, ICT technicians, ICT installers and servicers." ;
	skos:topConceptOf	ns8:indicator .
ns1:desi_idt	rdf:type	skos:Concept ,
		ns2:Indicator ;
	skos:prefLabel	"Integration of Digital Technology" ;
	dct:source	ns5: ;
	skos:notation	"desi_idt" ;
	skos:altLabel	"Integration of Digital Technology" ;
	ns6:membership	ns39:desi_idt ;
	skos:topConceptOf	ns8:indicator .
ns1:desi_idt_ai	rdf:type	skos:Concept ,
		ns2:Indicator ;
	skos:prefLabel	"Artificial intelligence" ;
	dct:source	ns5:desi_idt_ai ;
	skos:notation	"desi_idt_ai" ;
	skos:altLabel	"AI" ;
	ns6:membership	ns36:desi_idt_ai ;
	skos:definition	"Enterprises using any AI technology" ;
	skos:topConceptOf	ns8:indicator .
ns1:desi_idt_bigdat	rdf:type	skos:Concept ,
		ns2:Indicator ;
	skos:prefLabel	"Big data" ;
	dct:source	ns5:desi_idt_bigdat ;
	skos:notation	"desi_idt_bigdat" ;
	skos:altLabel	"Big data" ;
	ns6:membership	ns36:desi_idt_bigdat ;
	skos:definition	"Enterprises analysing big data from any data source" ;
	skos:topConceptOf	ns8:indicator .
ns1:desi_idt_cloud	rdf:type	skos:Concept ,
		ns2:Indicator ;
	skos:prefLabel	"Cloud" ;
	dct:source	ns5:desi_idt_cloud ;
	skos:notation	"desi_idt_cloud" ;
	skos:altLabel	"Cloud" ;
	ns6:membership	ns36:desi_idt_cloud ;
	skos:definition	"Enterprises purchasing at least one of the following cloud computing services: hosting of the enterprise's database, accounting software applications, CRM software, computing power" ;
	skos:topConceptOf	ns8:indicator .
ns1:desi_idt_di	rdf:type	ns2:Indicator ,
		skos:Concept ;
	skos:prefLabel	"Digital intensity" ;
	dct:source	ns5: ;
	skos:notation	"desi_idt_di" ;
	skos:altLabel	"Digital intensity" ;
	ns6:membership	ns38:desi_idt_di ;
	skos:topConceptOf	ns8:indicator .
ns1:desi_idt_dtb	rdf:type	ns2:Indicator ,
		skos:Concept ;
	skos:prefLabel	"Digital technologies for businesses" ;
	dct:source	ns5: ;
	skos:notation	"desi_idt_dtb" ;
	skos:altLabel	"Digital technologies for businesses" ;
	ns6:membership	ns38:desi_idt_dtb ;
	skos:topConceptOf	ns8:indicator .
ns1:desi_idt_ecomm	rdf:type	ns2:Indicator ,
		skos:Concept ;
	skos:prefLabel	"e-Commerce" ;
	dct:source	ns5: ;
	skos:notation	"desi_idt_ecomm" ;
	skos:altLabel	"e-Commerce" ;
	ns6:membership	ns38:desi_idt_ecomm ;
	skos:topConceptOf	ns8:indicator .
ns1:desi_idt_ecomturn	rdf:type	ns2:Indicator ,
		skos:Concept ;
	skos:prefLabel	"e-Commerce turnover" ;
	dct:source	ns5:desi_idt_ecomturn ;
	skos:notation	"desi_idt_ecomturn" ;
	skos:altLabel	"e-Commerce turnover" ;
	ns6:membership	ns36:desi_idt_ecomturn ;
	skos:definition	"SMEs total turnover from e-commerce" ;
	skos:topConceptOf	ns8:indicator .
ns1:desi_idt_einv	rdf:type	ns2:Indicator ,
		skos:Concept ;
	skos:prefLabel	"e-Invoices" ;
	dct:source	ns5:desi_idt_einv ;
	skos:notation	"desi_idt_einv" ;
	skos:altLabel	"e-Invoices" ;
	ns6:membership	ns36:desi_idt_einv ;
	skos:definition	"Enterprises sending e-invoices, suitable for automated processing" ;
	skos:topConceptOf	ns8:indicator .
ns1:desi_idt_eis	rdf:type	ns2:Indicator ,
		skos:Concept ;
	skos:prefLabel	"Electronic Information Sharing" ;
	dct:source	ns5:desi_idt_eis ;
	skos:notation	"desi_idt_eis" ;
	skos:altLabel	"Electronic Information Sharing" ;
	ns6:membership	ns36:desi_idt_eis ;
	skos:definition	"Enterprises who have in use an ERP (enterprise resource planning) software package to share information between different functional areas (e.g. accounting, planning, production, marketing)" ;
	skos:topConceptOf	ns8:indicator .
ns1:desi_idt_ictsust	rdf:type	ns2:Indicator ,
		skos:Concept ;
	skos:prefLabel	"ICT for environmental sustainability" ;
	dct:source	ns5:desi_idt_ictsust ;
	skos:notation	"desi_idt_ictsust" ;
	skos:altLabel	"ICT for environmental sustainability" ;
	ns6:membership	ns36:desi_idt_ictsust ;
	skos:definition	"The indicator measures the level of support that adopted ICT technologies offered to enterprises to engage in more environmentally-friendly actions. The level of intensity is measured based on the number of environmental actions (maximum 10) reported by enterprises to have been facilitated by the use of ICT. The following categorisation was achieved: low intensity (0 to 4 actions), medium intensity (5 to 7 actions) and high intensity (8 to 10 actions)." ;
	skos:topConceptOf	ns8:indicator .
ns1:desi_idt_sellcb	rdf:type	ns2:Indicator ,
		skos:Concept ;
	skos:prefLabel	"Selling online cross-border" ;
	dct:source	ns5:desi_idt_sellcb ;
	skos:notation	"desi_idt_sellcb" ;
	skos:altLabel	"Selling online cross-border" ;
	ns6:membership	ns36:desi_idt_sellcb ;
	skos:definition	"SMEs that carried out electronic sales to other EU countries" ;
	skos:topConceptOf	ns8:indicator .
ns1:desi_idt_smeso	rdf:type	ns2:Indicator ,
		skos:Concept ;
	skos:prefLabel	"SMEs selling online" ;
	dct:source	ns5:desi_idt_smeso ;
	skos:notation	"desi_idt_smeso" ;
	skos:altLabel	"SMEs selling online" ;
	ns6:membership	ns36:desi_idt_smeso ;
	skos:definition	"SMEs selling online (at least 1% of turnover)" ;
	skos:topConceptOf	ns8:indicator .
ns1:desi_idt_socmed	rdf:type	ns2:Indicator ,
		skos:Concept ;
	skos:prefLabel	"Social media" ;
	dct:source	ns5:desi_idt_socmed ;
	skos:notation	"desi_idt_socmed" ;
	skos:altLabel	"Social media" ;
	ns6:membership	ns36:desi_idt_socmed ;
	skos:definition	"Enterprises using two or more of the following social media: social networks, enterprise's blog or microblog, multimedia content sharing websites, wiki-based knowledge sharing tools. Using social media means that the enterprise has a user profile, an account or a user license depending on the requirements and the type of the social media. " ;
	skos:topConceptOf	ns8:indicator .
ns1:desi_mbbtu	rdf:type	ns2:Indicator ,
		skos:Concept ;
	skos:prefLabel	"Mobile BB take-up" ;
	dct:source	ns5:desi_mbbtu ;
	skos:notation	"desi_mbbtu" ;
	skos:altLabel	"Mobile broadband take-up" ;
	ns6:membership	ns36:desi_mbbtu ;
	skos:definition	"Number of mobile data subscriptions per 100 people" ;
	skos:topConceptOf	ns8:indicator .
ns1:desi_total	rdf:type	ns2:Indicator ,
		skos:Concept ;
	skos:prefLabel	"Digital Economy and Society Index" ;
	dct:source	ns5: ;
	skos:notation	"desi_total" ;
	skos:altLabel	"DESI Total " .
@prefix ns40:	<http://semantic.digital-agenda-data.eu/codelist/indicator-group/desi_total/> .
ns1:desi_total	ns6:membership	ns40:desi_total ;
	skos:definition	"DESI overall index score per country" ;
	skos:topConceptOf	ns8:indicator .
ns1:desi_ufbbtu	rdf:type	ns2:Indicator ,
		skos:Concept ;
	skos:prefLabel	"At least 100 Mbps fixed BB take-up" ;
	dct:source	ns5:desi_ufbbtu ;
	skos:notation	"desi_ufbbtu" ;
	skos:altLabel	"At least 100 Mbps fixed broadband take-up" ;
	ns6:membership	ns36:desi_ufbbtu ;
	skos:definition	"Percentage of households subscribing to fixed broadband of at least 100 Mbps, calculated as overall fixed broadband take-up" ;
	skos:topConceptOf	ns8:indicator .
ns1:desi_vhcnc	rdf:type	ns2:Indicator ,
		skos:Concept ;
	skos:prefLabel	"Fixed Very High Capacity Network (VHCN) coverage" ;
	dct:source	ns5:desi_vhcnc ;
	skos:notation	"desi_vhcnc" ;
	skos:altLabel	"Fixed Very High Capacity Network (VHCN) coverage" ;
	ns6:membership	ns36:desi_vhcnc ;
	skos:definition	"Percentage of households covered by any fixed VHCN. The technologies considered are FTTH and FTTB for 2015-2018 and FTTH, FTTB and Cable Docsis 3.1 for 201" ;
	skos:topConceptOf	ns8:indicator .
ns1:desi_dps_prefform	rdf:type	ns2:Indicator ,
		skos:Concept ;
	skos:prefLabel	"Pre-filled Forms" ;
	dct:source	ns5:desi_dps_prefform ;
	skos:notation	"desi_dps_prefform" ;
	skos:altLabel	"Pre-filled Forms" ;
	ns6:membership	ns36:desi_dps_prefform ;
	skos:definition	"Amount of data that is pre-filled in public services' online forms" ;
	skos:topConceptOf	ns8:indicator .
ns1:desi_dps_pscit	rdf:type	ns2:Indicator ,
		skos:Concept ;
	skos:prefLabel	"Digital public services for citizens" ;
	dct:source	ns5:desi_dps_pscit ;
	skos:notation	"desi_dps_pscit" ;
	skos:altLabel	"Digital public services for citizens" ;
	ns6:membership	ns36:desi_dps_pscit ;
	skos:definition	"The share of administrative steps that can be done online for major life events (birth of a child, new residence, etc.) for citizens" ;
	skos:topConceptOf	ns8:indicator .
ns1:desi_idt_smedi	rdf:type	ns2:Indicator ,
		skos:Concept ;
	skos:prefLabel	"SMEs with at least a basic level of digital intensity" ;
	dct:source	ns5:desi_idt_smedi ;
	skos:notation	"desi_idt_smedi" ;
	skos:altLabel	"SMEs with at least a basic level of digital intensity" ;
	ns6:membership	ns36:desi_idt_smedi ;
	skos:definition	"The digital intensity score is based on counting how many out of 12 selected technologies are used by enterprises. A basic level requires usage of at least 4 technologies. " ;
	skos:topConceptOf	ns8:indicator .
ns7:e_ai_tany	rdf:type	ns2:IndicatorToGroupMembership ;
	rdfs:label	"ebusiness" ;
	ns6:member-of	ns14:ebusiness ;
	ns6:order	"31" .
ns7:e_cc1_si	rdf:type	ns2:IndicatorToGroupMembership ;
	rdfs:label	"ebusiness" ;
	ns6:member-of	ns14:ebusiness ;
	ns6:order	"27" .
ns1:i_dsk2_ab	rdf:type	skos:Concept ,
		ns2:Indicator ;
	skos:prefLabel	"DSI 2.0 - Individuals with above basic overall digital skills" ;
	dct:source	ns5:estat_isoc_sk_dskl_i21 ;
	skos:notation	"i_dsk2_ab" ;
	skos:altLabel	"DSI 2.0 -  Above basic overall digital skills (from 2021)" ;
	ns6:membership	ns26:i_dsk2_ab ;
	skos:definition	"Individuals with  \u201Cabove basic digital skills\u201D in all 5 areas." ;
	skos:topConceptOf	ns8:indicator .
ns1:i_dsk2_b	rdf:type	skos:Concept ,
		ns2:Indicator ;
	skos:prefLabel	"DSI 2.0 - Individuals with basic overall digital skills" ;
	dct:source	ns5:estat_isoc_sk_dskl_i21 ;
	skos:notation	"i_dsk2_b" ;
	skos:altLabel	"DSI 2.0 - Basic overall digital skills (from 2021)" ;
	ns6:membership	ns26:i_dsk2_b ;
	skos:definition	" The skills in 5 areas are at 'at least basic level' (some can be \u201Cbasic\u201D and some can be \u201Cabove basic\u201D, but not all 5 areas are \u201Cabove basic\u201D." ;
	skos:topConceptOf	ns8:indicator .
ns1:i_dsk2_bab	rdf:type	skos:Concept ,
		ns2:Indicator ;
	skos:prefLabel	"DSI 2.0 - Individuals with at least basic overall digital skills" ;
	dct:source	ns5:estat_isoc_sk_dskl_i21 ;
	skos:notation	"i_dsk2_bab" ;
	skos:altLabel	"DSI 2.0 - At least basic overall digital skills (from 2021)" ;
	ns6:membership	ns26:i_dsk2_bab ;
	skos:definition	"The sum of basic and above basic skills." ;
	skos:topConceptOf	ns8:indicator .
ns1:i_dsk2_cc_ab	rdf:type	skos:Concept ,
		ns2:Indicator ;
	skos:prefLabel	"DSI 2.0 - Individuals with above basic communication and collaboration\u00A0 skills" ;
	dct:source	ns5:estat_isoc_sk_dskl_i21 ;
	skos:notation	"i_dsk2_cc_ab" ;
	skos:altLabel	"DSI 2.0 - Communication and collaboration - Above basic skills (from 2021)" ;
	ns6:membership	ns26:i_dsk2_cc_ab ;
	skos:definition	"Above basic: more than one activity from activities used for calculating the communication and collaboration skills" ;
	skos:note	"Definition in Digital Competence Framework 2.0: To interact, communicate and collaborate through digital technologies while being aware of cultural and generational diversity. To participate in society through public and private digital services and participatory citizenship. To manage one\u2019s digital identity and reputation.\n\nSending/receiving emails (IUEM);\nTelephoning/video calls over the internet (IUPH1);\nInstant messaging (IUCHAT1);\nParticipating in social networks (IUSNET);\nExpressing opinions on civic or political issues on websites or in social media (IUPOL2);\nTaking part in online consultations or voting to define civic or political issues (IUVOTE)." ;
	skos:topConceptOf	ns8:indicator .
ns1:i_dsk2_cc_b	rdf:type	skos:Concept ,
		ns2:Indicator ;
	skos:prefLabel	"DSI 2.0 - Individuals with basic communication and collaboration\u00A0 skills" ;
	dct:source	ns5:estat_isoc_sk_dskl_i21 ;
	skos:notation	"i_dsk2_cc_b" ;
	skos:altLabel	"DSI 2.0 - Communication and collaboration - Basic\u00A0skills (from 2021)" ;
	ns6:membership	ns26:i_dsk2_cc_b ;
	skos:definition	"Basic: one activity from activities used for calculating the communication and collaboration skills" ;
	skos:note	"Definition in Digital Competence Framework 2.0: To interact, communicate and collaborate through digital technologies while being aware of cultural and generational diversity. To participate in society through public and private digital services and participatory citizenship. To manage one\u2019s digital identity and reputation.\n\nSending/receiving emails (IUEM);\nTelephoning/video calls over the internet (IUPH1);\nInstant messaging (IUCHAT1);\nParticipating in social networks (IUSNET);\nExpressing opinions on civic or political issues on websites or in social media (IUPOL2);\nTaking part in online consultations or voting to define civic or political issues (IUVOTE)." ;
	skos:topConceptOf	ns8:indicator .
ns1:i_dsk2_cc_bab	rdf:type	skos:Concept ,
		ns2:Indicator ;
	skos:prefLabel	"DSI 2.0 - Individuals with basic or above basic communication and collaboration skills" ;
	dct:source	ns5:estat_isoc_sk_dskl_i21 ;
	skos:notation	"i_dsk2_cc_bab" ;
	skos:altLabel	"DSI 2.0 - Communication and collaboration - Basic or above basic skills (from 2021)" ;
	ns6:membership	ns26:i_dsk2_cc_bab ;
	skos:definition	"At least basic skills - sum of basic and above basic skills. " ;
	skos:note	"Definition in Digital Competence Framework 2.0: To interact, communicate and collaborate through digital technologies while being aware of cultural and generational diversity. To participate in society through public and private digital services and participatory citizenship. To manage one\u2019s digital identity and reputation." ;
	skos:topConceptOf	ns8:indicator .
ns1:i_dsk2_dcc_ab	rdf:type	skos:Concept ,
		ns2:Indicator ;
	skos:prefLabel	"DSI 2.0 - Individuals with above basic digital content creation\u00A0 skills" ;
	dct:source	ns5:estat_isoc_sk_dskl_i21 ;
	skos:notation	"i_dsk2_dcc_ab" ;
	skos:altLabel	"DSI 2.0 - Digital content creation - Above basic\u00A0skills (from 2021)" ;
	ns6:membership	ns26:i_dsk2_dcc_ab ;
	skos:definition	"Above basic: 3 or more activities from activities used for calculating the digital content creation\u00A0skills" ;
	skos:note	"Definition in Digital Competence Framework 2.0: To create and edit digital content. To improve and integrate information and content into an existing body of knowledge while understanding how copyright and licences are to be applied. To know how to give understandable instructions for a computer system.\n\nUsing word processing software (CWRD1);\nUsing spreadsheet software (CXLS1);\nEditing photos, video or audio files (CEPVA1);\nCopying or moving files (such as documents, data, images, video) between folders, devices (via e-mail, instant messaging, USB, cable) or on the cloud (CXFER1);\nCreating files (such as documents, image, videos) incorporating several elements such as text, picture, table, chart, animation or sound (CPRES2);\nUsing advanced features of spreadsheet software (functions, formulas, macros and other developer functions) to organize, analyse, structure or modify data (CXLSADV1);\nWriting code in a programming language (CPRG2)." ;
	skos:topConceptOf	ns8:indicator .
ns1:i_dsk2_dcc_b	rdf:type	skos:Concept ,
		ns2:Indicator ;
	skos:prefLabel	"DSI 2.0 - Individuals with basic digital content creation\u00A0skills" ;
	dct:source	ns5:estat_isoc_sk_dskl_i21 ;
	skos:notation	"i_dsk2_dcc_b" ;
	skos:altLabel	"DSI 2.0 - Digital content creation - Basic skills (from 2021)" ;
	ns6:membership	ns26:i_dsk2_dcc_b ;
	skos:definition	"Basic: one or two activities from activities used for calculating the digital content creation skills" ;
	skos:note	"Definition in Digital Competence Framework 2.0: To create and edit digital content. To improve and integrate information and content into an existing body of knowledge while understanding how copyright and licences are to be applied. To know how to give understandable instructions for a computer system.\n\nUsing word processing software (CWRD1);\nUsing spreadsheet software (CXLS1);\nEditing photos, video or audio files (CEPVA1);\nCopying or moving files (such as documents, data, images, video) between folders, devices (via e-mail, instant messaging, USB, cable) or on the cloud (CXFER1);\nCreating files (such as documents, image, videos) incorporating several elements such as text, picture, table, chart, animation or sound (CPRES2);\nUsing advanced features of spreadsheet software (functions, formulas, macros and other developer functions) to organize, analyse, structure or modify data (CXLSADV1);\nWriting code in a programming language (CPRG2)." ;
	skos:topConceptOf	ns8:indicator .
ns1:i_dsk2_dcc_bab	rdf:type	skos:Concept ,
		ns2:Indicator ;
	skos:prefLabel	"DSI 2.0 - Individuals with basic or above basic digital content creation skills" ;
	dct:source	ns5:estat_isoc_sk_dskl_i21 ;
	skos:notation	"i_dsk2_dcc_bab" ;
	skos:altLabel	"DSI 2.0 - Digital content creation - Basic or above basic skills (from 2021)" ;
	ns6:membership	ns26:i_dsk2_dcc_bab ;
	skos:definition	"At least basic skills - sum of basic and above basic skills. " ;
	skos:note	"Definition in Digital Competence Framework 2.0: To create and edit digital content. To improve and integrate information and content into an existing body of knowledge while understanding how copyright and licences are to be applied. To know how to give understandable instructions for a computer system.\n\nUsing word processing software (CWRD1);\nUsing spreadsheet software (CXLS1);\nEditing photos, video or audio files (CEPVA1);\nCopying or moving files (such as documents, data, images, video) between folders, devices (via e-mail, instant messaging, USB, cable) or on the cloud (CXFER1);\nCreating files (such as documents, image, videos) incorporating several elements such as text, picture, table, chart, animation or sound (CPRES2);\nUsing advanced features of spreadsheet software (functions, formulas, macros and other developer functions) to organize, analyse, structure or modify data (CXLSADV1);\nWriting code in a programming language (CPRG2)." ;
	skos:topConceptOf	ns8:indicator .
ns1:i_dsk2_ic_s	rdf:type	skos:Concept ,
		ns2:Indicator ;
	skos:prefLabel	"DSI 2.0 - Individuals with online information and communication skills" ;
	dct:source	ns5:estat_isoc_sk_dskl_i21 ;
	skos:notation	"i_dsk2_ic_s" ;
	skos:altLabel	"DSI 2.0 - Online information and communication skills (from 2021)" ;
	ns6:membership	ns26:i_dsk2_ic_s ;
	skos:definition	"Individuals with online information and communication skills (at \u201Cbasic\u201D or \u201Cabove basic\u201D level) and have \u201Cno skills\u201D in 3 remaining areas (Digital content creation, Safety, and Problem solving)\n" ;
	skos:note	"At least one variable from the following list (Information and data literacy skills):\nFinding information about goods or services (IUIF);\nSeeking health-related information (IHIF);\nReading online news sites, newspapers or news magazines (IUNW1);\nActivities related to fact-checking online information and its sources (TICCSFOI, TICIDIS, TICNIDIS, TICXND).\nAND\n\nAt least one variable from the following list (Communication and collaboration skills):\nSending/receiving emails (IUEM);\nTelephoning/video calls over the internet (IUPH1);\nInstant messaging (IUCHAT1);\nParticipating in social networks (IUSNET);\nExpressing opinions on civic or political issues on websites or in social media (IUPOL2);\nTaking part in online consultations or voting to define civic or political issues (IUVOTE).\n \nAND individuals have \u201Cno skills\u201D in 3 remaining areas (Digital content creation, Safety, and Problem solving)" ;
	skos:topConceptOf	ns8:indicator .
ns1:i_dsk2_il_ab	rdf:type	skos:Concept ,
		ns2:Indicator ;
	skos:prefLabel	"DSI 2.0 - Individuals with above basic information and data literacy\u00A0 skills" ;
	dct:source	ns5:estat_isoc_sk_dskl_i21 ;
	skos:notation	"i_dsk2_il_ab" ;
	skos:altLabel	"DSI 2.0 - Information and data literacy- Above basic\u00A0skills (from 2021)" ;
	ns6:membership	ns26:i_dsk2_il_ab ;
	skos:definition	"Above basic: more than one activity from activities used for calculating the information and data literacy skills." ;
	skos:note	"Definition in Digital Competence Framework 2.0:\u00A0\u00A0To articulate information needs, to locate and retrieve digital data, information and content. To judge the relevance of the source and its content. To store, manage, organize digital data, information and content.\n\nFinding information about goods or services (IUIF);\nSeeking health-related information (IHIF);\nReading online news sites, newspapers or news magazines (IUNW1);\nActivities related to fact-checking online information and its sources (TICCSFOI, TICIDIS, TICNIDIS, TICXND)." ;
	skos:topConceptOf	ns8:indicator .
ns1:i_dsk2_il_b	rdf:type	skos:Concept ,
		ns2:Indicator ;
	skos:prefLabel	"DSI 2.0 - Individuals with basic information and data literacy\u00A0 skills" ;
	dct:source	ns5:estat_isoc_sk_dskl_i21 ;
	skos:notation	"i_dsk2_il_b" ;
	skos:altLabel	"DSI 2.0 - Information and data literacy - Basic skills (from 2021)" ;
	ns6:membership	ns26:i_dsk2_il_b ;
	skos:definition	"Basic: one activity from activities used for calculating the information and data literacy skills." ;
	skos:note	"Definition in Digital Competence Framework 2.0:\u00A0\u00A0To articulate information needs, to locate and retrieve digital data, information and content. To judge the relevance of the source and its content. To store, manage, organize digital data, information and content.\n\nFinding information about goods or services (IUIF);\nSeeking health-related information (IHIF);\nReading online news sites, newspapers or news magazines (IUNW1);\nActivities related to fact-checking online information and its sources (TICCSFOI, TICIDIS, TICNIDIS, TICXND)." ;
	skos:topConceptOf	ns8:indicator .
ns1:i_dsk2_il_bab	rdf:type	skos:Concept ,
		ns2:Indicator ;
	skos:prefLabel	"DSI 2.0 - Individuals with basic or above basic information and data literacy\u00A0 skills" ;
	dct:source	ns5:estat_isoc_sk_dskl_i21 ;
	skos:notation	"i_dsk2_il_bab" ;
	skos:altLabel	"DSI 2.0 - Information and data literacy - Basic or above basic\u00A0skills (from 2021)" ;
	ns6:membership	ns26:i_dsk2_il_bab ;
	skos:definition	"At least basic skills - sum of basic and above basic skills. " ;
	skos:note	"Definition in Digital Competence Framework 2.0:\u00A0\u00A0To articulate information needs, to locate and retrieve digital data, information and content. To judge the relevance of the source and its content. To store, manage, organize digital data, information and content.\n" ;
	skos:topConceptOf	ns8:indicator .
ns1:i_dsk2_lm	rdf:type	skos:Concept ,
		ns2:Indicator ;
	skos:prefLabel	"DSI 2.0 - Individuals with limited overall digital skills (2 out of 5)" ;
	dct:source	ns5:estat_isoc_sk_dskl_i21 ;
	skos:notation	"i_dsk2_lm" ;
	skos:altLabel	"DSI 2.0 - Limited overall digital skills (2 out of 5) - (from 2021)" ;
	ns6:membership	ns26:i_dsk2_lm ;
	skos:definition	"Individuals have \u201Cbasic\u201D or \u201Cabove basic\u201D level in 2 areas and \u201Cno skills\u201D in 3 areas (2 out of 5)." ;
	skos:topConceptOf	ns8:indicator .
ns1:i_dsk2_lw	rdf:type	skos:Concept ,
		ns2:Indicator ;
	skos:prefLabel	"DSI 2.0 - Individuals with low overall digital skills (4 out of 5)" ;
	dct:source	ns5:estat_isoc_sk_dskl_i21 ;
	skos:notation	"i_dsk2_lw" ;
	skos:altLabel	"DSI 2.0 - Low overall digital skills (4 out of 5) - (from 2021)" ;
	ns6:membership	ns26:i_dsk2_lw ;
	skos:definition	"Individuals have \u201Cbasic\u201D or \u201Cabove basic\u201D level in 4 areas and \u201Cno skills\u201D in 1 area (4 out of 5)." ;
	skos:topConceptOf	ns8:indicator .
ns1:i_dsk2_n	rdf:type	ns2:Indicator ,
		skos:Concept ;
	skos:prefLabel	"DSI 2.0 - Individuals with narrow overall digital skills (3 out of 5)" ;
	dct:source	ns5:estat_isoc_sk_dskl_i21 ;
	skos:notation	"i_dsk2_n" ;
	skos:altLabel	"DSI 2.0 - Narrow overall digital skills (3 out of 5) - (from 2021)" ;
	ns6:membership	ns26:i_dsk2_n ;
	skos:definition	"Individuals have \u201Cbasic\u201D or \u201Cabove basic\u201D level in 3 areas and \u201Cno skills\u201D in 2 areas (3 out of 5)." ;
	skos:topConceptOf	ns8:indicator .
ns1:i_dsk2_ps_ab	rdf:type	ns2:Indicator ,
		skos:Concept ;
	skos:prefLabel	"DSI 2.0 - Individuals with above basic problem solving\u00A0 skills" ;
	dct:source	ns5:estat_isoc_sk_dskl_i21 ;
	skos:notation	"i_dsk2_ps_ab" ;
	skos:altLabel	"DSI 2.0 - Problem solving- Above basic skills (from 2021)" ;
	ns6:membership	ns26:i_dsk2_ps_ab ;
	skos:definition	"Above basic: 3 or more activities from activities used for calculating the problem solving\u00A0 skills" ;
	skos:note	"Definition in Digital Competence Framework 2.0: To identify needs and problems, and to resolve conceptual problems and problem situations in digital environments. To use digital tools to innovate processes and products. To keep up-to-date with the digital evolution.\n\nDownloading or installing software or apps (CINSAPP1);\nChanging settings of software, app or device (CCONF1);\nOnline purchases (in the last 12 months) (IBUY=1 or IBUY=2);\nSelling online (IUSELL);\nUsed online learning resources (IUOLC or IUOLM);\nInternet banking (IUBK);\nLooking for a job or sending a job application (IUJOB)" ;
	skos:topConceptOf	ns8:indicator .
ns1:i_dsk2_ps_b	rdf:type	skos:Concept ,
		ns2:Indicator ;
	skos:prefLabel	"DSI 2.0 - Individuals with basic problem solving skills" ;
	dct:source	ns5:estat_isoc_sk_dskl_i21 ;
	skos:notation	"i_dsk2_ps_b" ;
	skos:altLabel	"DSI 2.0 - Problem solving- Basic skills (from 2021)" ;
	ns6:membership	ns26:i_dsk2_ps_b ;
	skos:definition	"Basic: one or two activities from activities used for calculating the problem solving\u00A0 skills" ;
	skos:note	"Definition in Digital Competence Framework 2.0: To identify needs and problems, and to resolve conceptual problems and problem situations in digital environments. To use digital tools to innovate processes and products. To keep up-to-date with the digital evolution.\n\nDownloading or installing software or apps (CINSAPP1);\nChanging settings of software, app or device (CCONF1);\nOnline purchases (in the last 12 months) (IBUY=1 or IBUY=2);\nSelling online (IUSELL);\nUsed online learning resources (IUOLC or IUOLM);\nInternet banking (IUBK);\nLooking for a job or sending a job application (IUJOB)" ;
	skos:topConceptOf	ns8:indicator .
ns1:i_dsk2_ps_bab	rdf:type	skos:Concept ,
		ns2:Indicator ;
	skos:prefLabel	"DSI 2.0 - Individuals with basic or above basic problem solving skills" ;
	dct:source	ns5:estat_isoc_sk_dskl_i21 ;
	skos:notation	"i_dsk2_ps_bab" ;
	skos:altLabel	"DSI 2.0 - Problem solving - Basic or above basic skills (from 2021)" ;
	ns6:membership	ns26:i_dsk2_ps_bab ;
	skos:definition	"At least basic skills - sum of basic and above basic skills. " ;
	skos:note	"Definition in Digital Competence Framework 2.0: To identify needs and problems, and to resolve conceptual problems and problem situations in digital environments. To use digital tools to innovate processes and products. To keep up-to-date with the digital evolution.\n\nDownloading or installing software or apps (CINSAPP1);\nChanging settings of software, app or device (CCONF1);\nOnline purchases (in the last 12 months) (IBUY=1 or IBUY=2);\nSelling online (IUSELL);\nUsed online learning resources (IUOLC or IUOLM);\nInternet banking (IUBK);\nLooking for a job or sending a job application (IUJOB)" ;
	skos:topConceptOf	ns8:indicator .
ns1:i_dsk2_sf_ab	rdf:type	skos:Concept ,
		ns2:Indicator ;
	skos:prefLabel	"DSI 2.0 - Individuals with above basic safety\u00A0 skills" ;
	dct:source	ns5:estat_isoc_sk_dskl_i21 ;
	skos:notation	"i_dsk2_sf_ab" ;
	skos:altLabel	"DSI 2.0 - Safety - Above basic\u00A0skills (from 2021)" ;
	ns6:membership	ns26:i_dsk2_sf_ab ;
	skos:definition	"Above basic: 3 or more activities from activities used for calculating the safety skills" ;
	skos:note	"Definition in Digital Competence Framework 2.0: To protect devices, content, personal data and privacy in digital environments. To protect physical and psychological health, and to be aware of digital technologies for social well-being and social inclusion. To be aware of the environmental impact of digital technologies and their use.\n\nManaging access to own personal data by checking that the website where the respondent provided personal data was secure (MAPS_CWSC);\nManaging access to own personal data by reading privacy statements before providing personal data (MAPS_RPS);\nManaging access to own personal data by restricting or refusing access to own geographical location (MAPS_RRGL);\nManaging access to own personal data by limiting access to profile or content on social networking sites or shared online storage (MAPS_LAP);\nManaging access to own personal data by refusing allowing use of personal data for advertising purposes (MAPS_RAAD);\nChanging settings in own internet browser to prevent or limit cookies on any of the respondent devices (PCOOK1)." ;
	skos:topConceptOf	ns8:indicator .
ns1:i_dsk2_sf_b	rdf:type	skos:Concept ,
		ns2:Indicator ;
	skos:prefLabel	"DSI 2.0 - Individuals with basic safety skills" ;
	dct:source	ns5:estat_isoc_sk_dskl_i21 ;
	skos:notation	"i_dsk2_sf_b" ;
	skos:altLabel	"DSI 2.0 - Safety - Basic skills (from 2021)" ;
	ns6:membership	ns26:i_dsk2_sf_b ;
	skos:definition	"Basic: one or two activities from activities used for calculating the safety skills" ;
	skos:note	"Definition in Digital Competence Framework 2.0: To protect devices, content, personal data and privacy in digital environments. To protect physical and psychological health, and to be aware of digital technologies for social well-being and social inclusion. To be aware of the environmental impact of digital technologies and their use.\n\nManaging access to own personal data by checking that the website where the respondent provided personal data was secure (MAPS_CWSC);\nManaging access to own personal data by reading privacy statements before providing personal data (MAPS_RPS);\nManaging access to own personal data by restricting or refusing access to own geographical location (MAPS_RRGL);\nManaging access to own personal data by limiting access to profile or content on social networking sites or shared online storage (MAPS_LAP);\nManaging access to own personal data by refusing allowing use of personal data for advertising purposes (MAPS_RAAD);\nChanging settings in own internet browser to prevent or limit cookies on any of the respondent devices (PCOOK1)." ;
	skos:topConceptOf	ns8:indicator .
ns1:i_dsk2_sf_bab	rdf:type	skos:Concept ,
		ns2:Indicator ;
	skos:prefLabel	"DSI 2.0 - Individuals with basic or above basic safety skills" ;
	dct:source	ns5:estat_isoc_sk_dskl_i21 ;
	skos:notation	"i_dsk2_sf_bab" ;
	skos:altLabel	"DSI 2.0 - Safety - Basic or above basic skills (from 2021)" ;
	ns6:membership	ns26:i_dsk2_sf_bab ;
	skos:definition	"At least basic skills - sum of basic and above basic skills. " ;
	skos:note	"Definition in Digital Competence Framework 2.0: To protect devices, content, personal data and privacy in digital environments. To protect physical and psychological health, and to be aware of digital technologies for social well-being and social inclusion. To be aware of the environmental impact of digital technologies and their use.\n\nManaging access to own personal data by checking that the website where the respondent provided personal data was secure (MAPS_CWSC);\nManaging access to own personal data by reading privacy statements before providing personal data (MAPS_RPS);\nManaging access to own personal data by restricting or refusing access to own geographical location (MAPS_RRGL);\nManaging access to own personal data by limiting access to profile or content on social networking sites or shared online storage (MAPS_LAP);\nManaging access to own personal data by refusing allowing use of personal data for advertising purposes (MAPS_RAAD);\nChanging settings in own internet browser to prevent or limit cookies on any of the respondent devices (PCOOK1)." ;
	skos:topConceptOf	ns8:indicator .
ns1:i_dsk2_x	rdf:type	skos:Concept ,
		ns2:Indicator ;
	skos:prefLabel	"DSI 2.0 - Individuals with no overall digital skills" ;
	dct:source	ns5:estat_isoc_sk_dskl_i21 ;
	skos:notation	"i_dsk2_x" ;
	skos:altLabel	"DSI 2.0 - No overall digital skills (from 2021)" ;
	ns6:membership	ns26:i_dsk2_x ;
	skos:definition	"Individuals have \u201Cno skills\u201D in 4 areas or \u201Cno skills\u201D in all 5 areas despite declaring having used the internet at least once during last 3 months." ;
	skos:topConceptOf	ns8:indicator .
ns26:i_dsk2_ab	rdf:type	ns2:IndicatorToGroupMembership ;
	rdfs:label	"ict-skills" ;
	ns6:member-of	ns14:ict-skills ;
	ns6:order	"2" .
ns26:i_dsk2_b	rdf:type	ns2:IndicatorToGroupMembership ;
	rdfs:label	"ict-skills" ;
	ns6:member-of	ns14:ict-skills ;
	ns6:order	"1" .
ns26:i_dsk2_bab	rdf:type	ns2:IndicatorToGroupMembership ;
	rdfs:label	"ict-skills" ;
	ns6:member-of	ns14:ict-skills ;
	ns6:order	"3" .
ns26:i_dsk2_cc_ab	rdf:type	ns2:IndicatorToGroupMembership ;
	rdfs:label	"ict-skills" ;
	ns6:member-of	ns14:ict-skills ;
	ns6:order	"14" .
ns26:i_dsk2_cc_b	rdf:type	ns2:IndicatorToGroupMembership ;
	rdfs:label	"ict-skills" ;
	ns6:member-of	ns14:ict-skills ;
	ns6:order	"13" .
ns26:i_dsk2_cc_bab	rdf:type	ns2:IndicatorToGroupMembership ;
	rdfs:label	"ict-skills" ;
	ns6:member-of	ns14:ict-skills ;
	ns6:order	"15" .
ns26:i_dsk2_dcc_ab	rdf:type	ns2:IndicatorToGroupMembership ;
	rdfs:label	"ict-skills" ;
	ns6:member-of	ns14:ict-skills ;
	ns6:order	"17" .
ns26:i_dsk2_dcc_b	rdf:type	ns2:IndicatorToGroupMembership ;
	rdfs:label	"ict-skills" ;
	ns6:member-of	ns14:ict-skills ;
	ns6:order	"16" .
ns26:i_dsk2_dcc_bab	rdf:type	ns2:IndicatorToGroupMembership ;
	rdfs:label	"ict-skills" ;
	ns6:member-of	ns14:ict-skills ;
	ns6:order	"18" .
ns26:i_dsk2_ic_s	rdf:type	ns2:IndicatorToGroupMembership ;
	rdfs:label	"ict-skills" ;
	ns6:member-of	ns14:ict-skills ;
	ns6:order	"9" .
ns26:i_dsk2_il_ab	rdf:type	ns2:IndicatorToGroupMembership ;
	rdfs:label	"ict-skills" ;
	ns6:member-of	ns14:ict-skills ;
	ns6:order	"11" .
ns26:i_dsk2_il_b	rdf:type	ns2:IndicatorToGroupMembership ;
	rdfs:label	"ict-skills" ;
	ns6:member-of	ns14:ict-skills ;
	ns6:order	"10" .
ns26:i_dsk2_il_bab	rdf:type	ns2:IndicatorToGroupMembership ;
	rdfs:label	"ict-skills" ;
	ns6:member-of	ns14:ict-skills ;
	ns6:order	"12" .
ns26:i_dsk2_lm	rdf:type	ns2:IndicatorToGroupMembership ;
	rdfs:label	"ict-skills" ;
	ns6:member-of	ns14:ict-skills ;
	ns6:order	"6" .
ns26:i_dsk2_lw	rdf:type	ns2:IndicatorToGroupMembership ;
	rdfs:label	"ict-skills" ;
	ns6:member-of	ns14:ict-skills ;
	ns6:order	"4" .
ns26:i_dsk2_n	rdf:type	ns2:IndicatorToGroupMembership ;
	rdfs:label	"ict-skills" ;
	ns6:member-of	ns14:ict-skills ;
	ns6:order	"5" .
ns26:i_dsk2_na	rdf:type	ns2:IndicatorToGroupMembership ;
	rdfs:label	"ict-skills" ;
	ns6:member-of	ns14:ict-skills ;
	ns6:order	"8" .
ns26:i_dsk2_ps_ab	rdf:type	ns2:IndicatorToGroupMembership ;
	rdfs:label	"ict-skills" ;
	ns6:member-of	ns14:ict-skills ;
	ns6:order	"23" .
ns26:i_dsk2_ps_b	rdf:type	ns2:IndicatorToGroupMembership ;
	rdfs:label	"ict-skills" ;
	ns6:member-of	ns14:ict-skills ;
	ns6:order	"22" .
ns26:i_dsk2_ps_bab	rdf:type	ns2:IndicatorToGroupMembership ;
	rdfs:label	"ict-skills" ;
	ns6:member-of	ns14:ict-skills ;
	ns6:order	"24" .
ns26:i_dsk2_sf_ab	rdf:type	ns2:IndicatorToGroupMembership ;
	rdfs:label	"ict-skills" ;
	ns6:member-of	ns14:ict-skills ;
	ns6:order	"20" .
ns26:i_dsk2_sf_b	rdf:type	ns2:IndicatorToGroupMembership ;
	rdfs:label	"ict-skills" ;
	ns6:member-of	ns14:ict-skills ;
	ns6:order	"19" .
ns26:i_dsk2_sf_bab	rdf:type	ns2:IndicatorToGroupMembership ;
	rdfs:label	"ict-skills" ;
	ns6:member-of	ns14:ict-skills ;
	ns6:order	"21" .
ns26:i_dsk2_x	rdf:type	ns2:IndicatorToGroupMembership ;
	rdfs:label	"ict-skills" ;
	ns6:member-of	ns14:ict-skills ;
	ns6:order	"7" .
ns7:e_di4_hi	rdf:type	ns2:IndicatorToGroupMembership ;
	rdfs:label	"ebusiness" ;
	ns6:member-of	ns14:ebusiness ;
	ns6:order	"19" .
ns7:e_di4_lo	rdf:type	ns2:IndicatorToGroupMembership ;
	rdfs:label	"ebusiness" ;
	ns6:member-of	ns14:ebusiness ;
	ns6:order	"20" .
ns7:e_di4_vhi	rdf:type	ns2:IndicatorToGroupMembership ;
	rdfs:label	"ebusiness" ;
	ns6:member-of	ns14:ebusiness ;
	ns6:order	"18" .
ns7:e_di4_vlo	rdf:type	ns2:IndicatorToGroupMembership ;
	rdfs:label	"ebusiness" ;
	ns6:member-of	ns14:ebusiness ;
	ns6:order	"21" .
ns1:e_gov_dpsc	rdf:type	skos:Concept ,
		ns2:Indicator ;
	skos:prefLabel	"Digital Public Services for Citizens (up to 2020)" ;
	dct:source	ns5:e_gov_bench ;
	skos:notation	"e_gov_dpsc" ;
	skos:altLabel	"Digital Public Services for Citizens (up to 2020)" ;
	ns6:membership	ns22:e_gov_dpsc ;
	skos:definition	"The extent to which a service or information concerning service for citizens is provided online, and via a portal. Services that are offered fully, partially or not at all online. " ;
	skos:topConceptOf	ns8:indicator .
ns1:e_gov_od	rdf:type	skos:Concept ,
		ns2:Indicator ;
	skos:prefLabel	"Open Data" ;
	dct:source	ns5:european_data_portal ;
	skos:notation	"e_gov_od" ;
	skos:altLabel	"Open Data" ;
	ns6:membership	ns22:e_gov_od ;
	skos:definition	"A series of indicators have been selected to measure Open Data maturity across Europe. These indicators cover the level of development of national policies promoting Open Data, an assessment of the features made available on national data portals as well as the expected impact and quality of Open Data." ;
	skos:note	"This composite indicator comprises 4 dimensions:\ni)Open Data Policy that focuses on the presence of specific  olicies and strategies to foster open data at national level; \nii) Open Data Impact that looks at the activities performed to monitor and measure open re-use and the impact derived by such re-use; \niii) Open Data Portal that focuses on advanced portal  unctions that enable both versed and less versed users to access open data via the national portal and features that enhance the interaction between publishers and re-users (via forum and discussion boards); and \niv) Open Data Quality that focuses on the measures  dopted by portal managers to ensure the systematic harvesting of metadata from sources across the country, as well as the  urrency of the available metadata and where possible the actual data, the monitoring of the compliance with the DCAT-AP metadata standard as well as the quality of  eployment of the published data.\nBreak in series in 2020 due to methodological changes.\nThe data was recalculated to include EU27 Average.\nFor more information please consult: https://www.europeandataportal.eu/en/impact-studies/open-data-maturity" ;
	skos:topConceptOf	ns8:indicator .
ns1:i_dsk_x	rdf:type	skos:Concept ,
		ns2:Indicator ;
	skos:prefLabel	"DSI 2015-2019 Individuals with no digital skills" ;
	dct:source	ns5:estat_isoc_sk_dskl_i ;
	skos:notation	"i_dsk_x" ;
	skos:altLabel	"DSI 2015-2019 - No overall digital skills" ;
	ns6:membership	ns26:i_dsk_x ;
	skos:definition	"Persons that have been using internet during last 3 months are attributed a score on four digital competence domains: information, communication, content-creation and problem-solving, depending the activities they have been able to do. The scores in each domain are basic, above basic and below basic. Individuals not using internet are classified without digital skills. To be classified \"basic or above basic\" on the overall indicator an individual has to have basic or above basic skills in all the four Digital Competence domains included in the index: information, communication, content-creation and problem-solving." ;
	skos:note	"Detailed results are available in the Eurostat table <a href=\"http://appsso.eurostat.ec.europa.eu/nui/show.do?dataset=isoc_sk_dskl_i&lang=en\">ISOC_SK_DSKL_I</a>. Consult the <a href=\"https://ec.europa.eu/digital-agenda/en/news/new-comprehensive-digital-skills-indicator\"> methodological note</a> on DG CONNECT newsroom." ;
	skos:topConceptOf	ns8:indicator .
ns1:i_dsk_c_x	rdf:type	ns2:Indicator ,
		skos:Concept ;
	skos:prefLabel	"DSI 2015-2019 Individuals with no digital skills in Communication domain" ;
	dct:source	ns5:estat_isoc_sk_dskl_i ;
	skos:notation	"i_dsk_c_x" ;
	skos:altLabel	"DSI 2015-2019 - Communication Domain - No Skills" ;
	ns6:membership	ns26:i_dsk_c_x ;
	skos:definition	"These skills refer to the ability to communicate in digital environments, share resources through online tools, link with others and collaborate through digital tools, interact with and participate in communities and networks, cross-cultural awareness. The indicator is based on four activities internet users have been able to do online during previous 3 months. The scores are basic, above basic and none. Individuals not using internet are classified without digital skills." ;
	skos:note	"Detailed results are available in the Eurostat table <a href=\"http://appsso.eurostat.ec.europa.eu/nui/show.do?dataset=isoc_sk_dskl_i&lang=en\">ISOC_SK_DSKL_I</a>. Consult the <a href=\"https://ec.europa.eu/digital-agenda/en/news/new-comprehensive-digital-skills-indicator\"> methodological note</a> on DG CONNECT newsroom." ;
	skos:topConceptOf	ns8:indicator .
ns1:i_dsk2_na	rdf:type	skos:Concept ,
		ns2:Indicator ;
	skos:prefLabel	"DSI 2.0 - Digital skills could not be assessed because the individual has not used the internet in the last 3 months" ;
	dct:source	ns5:estat_isoc_sk_dskl_i21 ;
	skos:notation	"i_dsk2_na" ;
	skos:altLabel	"DSI 2.0 - Digital skills could not be assessed because the individual has not used the internet in the last 3 months (from 2021)" ;
	ns6:membership	ns26:i_dsk2_na ;
	skos:definition	"Individuals that have not used the internet in the last 3 months and skills could have not been assessed." ;
	skos:topConceptOf	ns8:indicator .
ns7:e_bda	rdf:type	ns2:IndicatorToGroupMembership ;
	rdfs:label	"ebusiness" ;
	ns6:member-of	ns14:ebusiness ;
	ns6:order	"30" .
ns7:e_di3_hi	rdf:type	ns2:IndicatorToGroupMembership ;
	rdfs:label	"ebusiness" ;
	ns6:member-of	ns14:ebusiness ;
	ns6:order	"19" .
ns7:e_di3_lo	rdf:type	ns2:IndicatorToGroupMembership ;
	rdfs:label	"ebusiness" ;
	ns6:member-of	ns14:ebusiness ;
	ns6:order	"20" .
ns7:e_di3_vhi	rdf:type	ns2:IndicatorToGroupMembership ;
	rdfs:label	"ebusiness" ;
	ns6:member-of	ns14:ebusiness ;
	ns6:order	"18" .
ns7:e_di3_vlo	rdf:type	ns2:IndicatorToGroupMembership ;
	rdfs:label	"ebusiness" ;
	ns6:member-of	ns14:ebusiness ;
	ns6:order	"21" .
ns7:e_inv4s_ap	rdf:type	ns2:IndicatorToGroupMembership ;
	rdfs:label	"ebusiness" ;
	ns6:member-of	ns14:ebusiness ;
	ns6:order	"5" .
ns1:e_bda	rdf:type	ns2:Indicator ,
		skos:Concept ;
	skos:prefLabel	"Enterprises analysing big data (2020)" ;
	dct:source	ns5:estat_isoc_eb_bd ;
	skos:notation	"e_bda" ;
	skos:altLabel	"Enterprises analysing big data from any data source" ;
	ns6:membership	ns7:e_bda ;
	skos:definition	"Analyse big data internally from any data source or externally" ;
	skos:topConceptOf	ns8:indicator .
ns1:e_inv4s_ap	rdf:type	ns2:Indicator ,
		skos:Concept ;
	skos:prefLabel	"Enterprises sending e-invoices" ;
	dct:source	ns5:estat_isoc_bde15disc ;
	skos:notation	"e_inv4s_ap" ;
	skos:altLabel	"Enterprises sending e-invoices" ;
	ns6:membership	ns7:e_inv4s_ap ;
	skos:definition	"Enterprises sending eInvoices, suitable for automatic processing" ;
	skos:topConceptOf	ns8:indicator .
ns1:i_dsk_l	rdf:type	skos:Concept ,
		ns2:Indicator ;
	skos:prefLabel	"DSI 2015-2019 Individuals with low level of digital skills (missing some type of basic skills)" ;
	dct:source	ns5:estat_isoc_sk_dskl_i ;
	skos:notation	"i_dsk_l" ;
	skos:altLabel	"DSI 2015-2019 - Individuals with \"low\" level of skills " ;
	ns6:membership	ns26:i_dsk_l ;
	skos:definition	"Persons that have been using internet during last 3 months are attributed a score on four digital competence domains: information, communication, content-creation and problem-solving, depending the activities they have been able to do. The scores in each domain are basic, above basic and below basic. Individuals not using internet are classified without digital skills. To be classified \"basic or above basic\" on the overall indicator an individual has to have basic or above basic skills in all the four Digital Competence domains included in the index: information, communication, content-creation and problem-solving." ;
	skos:note	"Detailed results are available in the Eurostat table <a href=\"http://appsso.eurostat.ec.europa.eu/nui/show.do?dataset=isoc_sk_dskl_i&lang=en\">ISOC_SK_DSKL_I</a>. Consult the <a href=\"https://ec.europa.eu/digital-agenda/en/news/new-comprehensive-digital-skills-indicator\"> methodological note</a> on DG CONNECT newsroom." ;
	skos:topConceptOf	ns8:indicator .
ns1:i_dsk_s_ab	rdf:type	ns2:Indicator ,
		skos:Concept ;
	skos:prefLabel	"DSI 2015-2019 Individuals with above basic level of digital skills in Software domain" ;
	dct:source	ns5:estat_isoc_sk_dskl_i ;
	skos:notation	"i_dsk_s_ab" ;
	skos:altLabel	"DSI 2015-2019 - Software Domain - Above Basic Skills" ;
	ns6:membership	ns26:i_dsk_s_ab ;
	skos:definition	"Software skills for content manipulation refer to the ability to create and edit new content (from word processing to images and video); integrate and re-elaborate previous knowledge and content; produce creative expressions, media outputs and programming; deal with and apply intellectual property rights and licences. The indicator is based on six activities internet users have been able to do during previous 3 months. The scores are basic, above basic and none. Individuals not using internet are classified without digital skills." ;
	skos:note	"Detailed results are available in the Eurostat table <a href=\"http://appsso.eurostat.ec.europa.eu/nui/show.do?dataset=isoc_sk_dskl_i&lang=en\">ISOC_SK_DSKL_I</a>. Consult the <a href=\"https://ec.europa.eu/digital-agenda/en/news/new-comprehensive-digital-skills-indicator\"> methodological note</a> on DG CONNECT newsroom." ;
	skos:topConceptOf	ns8:indicator .
ns1:i_dsk_ps_ab	rdf:type	ns2:Indicator ,
		skos:Concept ;
	skos:prefLabel	"DSI 2015-2019 Individuals with above basic level of digital skills in Problem solving domain" ;
	dct:source	ns5:estat_isoc_sk_dskl_i ;
	skos:notation	"i_dsk_ps_ab" ;
	skos:altLabel	"DSI 2015-2019 - Problem Solving Domain - Above Basic Skills" ;
	ns6:membership	ns26:i_dsk_ps_ab ;
	skos:definition	"Problem solving skills refers to the ability to identify digital needs and resources, make informed decisions as to which are the most appropriate digital tools according to the purpose or need, solve conceptual problems through digital means, creatively use technologies, solve technical problems, update one's own and others' competences. The indicator is based on three basic digital problems and familiarity with four online services internet users have been able to do during previous 3 months. The scores are basic, above basic and none. Individuals not using internet are classified without digital skills." ;
	skos:note	"Detailed results are available in the Eurostat table <a href=\"http://appsso.eurostat.ec.europa.eu/nui/show.do?dataset=isoc_sk_dskl_i&lang=en\">ISOC_SK_DSKL_I</a>. Consult the <a href=\"https://ec.europa.eu/digital-agenda/en/news/new-comprehensive-digital-skills-indicator\"> methodological note</a> on DG CONNECT newsroom." ;
	skos:topConceptOf	ns8:indicator .
ns1:i_dsk_ab	rdf:type	skos:Concept ,
		ns2:Indicator ;
	skos:prefLabel	"DSI 2015-2019 Individuals with above basic level of digital skills" ;
	dct:source	ns5:estat_isoc_sk_dskl_i ;
	skos:notation	"i_dsk_ab" ;
	skos:altLabel	"DSI 2015-2019 - Above basic level of skills" ;
	ns6:membership	ns26:i_dsk_ab ;
	skos:definition	"Persons that have been using internet during last 3 months are attributed a score on four digital competence domains: information, communication, content-creation and problem-solving, depending the activities they have been able to do. The scores in each domain are basic, above basic and below basic. Individuals not using internet are classified without digital skills. To be classified \"basic or above basic\" on the overall indicator an individual has to have basic or above basic skills in all the four Digital Competence domains included in the index: information, communication, content-creation and problem-solving." ;
	skos:note	"Detailed results are available in the Eurostat table <a href=\"http://appsso.eurostat.ec.europa.eu/nui/show.do?dataset=isoc_sk_dskl_i&lang=en\">ISOC_SK_DSKL_I</a>. Consult the <a href=\"https://ec.europa.eu/digital-agenda/en/news/new-comprehensive-digital-skills-indicator\"> methodological note</a> on DG CONNECT newsroom." ;
	skos:topConceptOf	ns8:indicator .
ns1:i_dsk_i_x	rdf:type	skos:Concept ,
		ns2:Indicator ;
	skos:prefLabel	"DSI 2015-2019 Individuals with no digital skills in Information domain" ;
	dct:source	ns5:estat_isoc_sk_dskl_i ;
	skos:notation	"i_dsk_i_x" ;
	skos:altLabel	"DSI 2015-2019 - Information Domain - No Skills" ;
	ns6:membership	ns26:i_dsk_i_x ;
	skos:definition	"Information processing skills refers to the ability to identify, locate, retrieve, store, organise and analyse digital information, judging its relevance and purpose. The indicator is based on five activities internet users have been able to do online during previous 3 months. The scores are basic, above basic and none. Individuals not using internet are classified without digital skills." ;
	skos:note	"Detailed results are available in the Eurostat table <a href=\"http://appsso.eurostat.ec.europa.eu/nui/show.do?dataset=isoc_sk_dskl_i&lang=en\">ISOC_SK_DSKL_I</a>. Consult the <a href=\"https://ec.europa.eu/digital-agenda/en/news/new-comprehensive-digital-skills-indicator\"> methodological note</a> on DG CONNECT newsroom." ;
	skos:topConceptOf	ns8:indicator .
ns1:i_dsk_ps_x	rdf:type	skos:Concept ,
		ns2:Indicator ;
	skos:prefLabel	"DSI 2015-2019 Individuals with no digital skills in Problem solving domain" ;
	dct:source	ns5:estat_isoc_sk_dskl_i ;
	skos:notation	"i_dsk_ps_x" ;
	skos:altLabel	"DSI 2015-2019 - Problem Solving Domain - No Skills" ;
	ns6:membership	ns26:i_dsk_ps_x ;
	skos:definition	"Problem solving skills refers to the ability to identify digital needs and resources, make informed decisions as to which are the most appropriate digital tools according to the purpose or need, solve conceptual problems through digital means, creatively use technologies, solve technical problems, update one's own and others' competences. The indicator is based on three basic digital problems and familiarity with four online services internet users have been able to do during previous 3 months. The scores are basic, above basic and none. Individuals not using internet are classified without digital skills." ;
	skos:note	"Detailed results are available in the Eurostat table <a href=\"http://appsso.eurostat.ec.europa.eu/nui/show.do?dataset=isoc_sk_dskl_i&lang=en\">ISOC_SK_DSKL_I</a>. Consult the <a href=\"https://ec.europa.eu/digital-agenda/en/news/new-comprehensive-digital-skills-indicator\"> methodological note</a> on DG CONNECT newsroom." ;
	skos:topConceptOf	ns8:indicator .
ns1:i_dsk_i_ab	rdf:type	ns2:Indicator ,
		skos:Concept ;
	skos:prefLabel	"DSI 2015-2019 Individuals with above basic level of digital skills in Information domain" ;
	dct:source	ns5:estat_isoc_sk_dskl_i ;
	skos:notation	"i_dsk_i_ab" ;
	skos:altLabel	"DSI 2015-2019 - Information Domain - Above Basic Skills" ;
	ns6:membership	ns26:i_dsk_i_ab ;
	skos:definition	"Information processing skills refers to the ability to identify, locate, retrieve, store, organise and analyse digital information, judging its relevance and purpose. The indicator is based on five activities internet users have been able to do online during previous 3 months. The scores are basic, above basic and none. Individuals not using internet are classified without digital skills." ;
	skos:note	"Detailed results are available in the Eurostat table <a href=\"http://appsso.eurostat.ec.europa.eu/nui/show.do?dataset=isoc_sk_dskl_i&lang=en\">ISOC_SK_DSKL_I</a>. Consult the <a href=\"https://ec.europa.eu/digital-agenda/en/news/new-comprehensive-digital-skills-indicator\"> methodological note</a> on DG CONNECT newsroom." ;
	skos:topConceptOf	ns8:indicator .
ns26:i_dsk_ab	rdf:type	ns2:IndicatorToGroupMembership ;
	rdfs:label	"ict-skills" ;
	ns6:member-of	ns14:ict-skills ;
	ns6:order	"1111" .
ns26:i_dsk_c_ab	rdf:type	ns2:IndicatorToGroupMembership ;
	rdfs:label	"ict-skills" ;
	ns6:member-of	ns14:ict-skills ;
	ns6:order	"1114" .
ns26:i_dsk_c_x	rdf:type	ns2:IndicatorToGroupMembership ;
	rdfs:label	"ict-skills" ;
	ns6:member-of	ns14:ict-skills ;
	ns6:order	"1116" .
ns26:i_dsk_i_ab	rdf:type	ns2:IndicatorToGroupMembership ;
	rdfs:label	"ict-skills" ;
	ns6:member-of	ns14:ict-skills ;
	ns6:order	"1117" .
ns26:i_dsk_i_x	rdf:type	ns2:IndicatorToGroupMembership ;
	rdfs:label	"ict-skills" ;
	ns6:member-of	ns14:ict-skills ;
	ns6:order	"1119" .
ns26:i_dsk_l	rdf:type	ns2:IndicatorToGroupMembership ;
	rdfs:label	"ict-skills" ;
	ns6:member-of	ns14:ict-skills ;
	ns6:order	"1120" .
ns26:i_dsk_ps_ab	rdf:type	ns2:IndicatorToGroupMembership ;
	rdfs:label	"ict-skills" ;
	ns6:member-of	ns14:ict-skills ;
	ns6:order	"1121" .
ns26:i_dsk_ps_x	rdf:type	ns2:IndicatorToGroupMembership ;
	rdfs:label	"ict-skills" ;
	ns6:member-of	ns14:ict-skills ;
	ns6:order	"1123" .
ns26:i_dsk_s_ab	rdf:type	ns2:IndicatorToGroupMembership ;
	rdfs:label	"ict-skills" ;
	ns6:member-of	ns14:ict-skills ;
	ns6:order	"1124" .
ns26:i_dsk_s_x	rdf:type	ns2:IndicatorToGroupMembership ;
	rdfs:label	"ict-skills" ;
	ns6:member-of	ns14:ict-skills ;
	ns6:order	"1126" .
ns26:i_dsk_x	rdf:type	ns2:IndicatorToGroupMembership ;
	rdfs:label	"ict-skills" ;
	ns6:member-of	ns14:ict-skills ;
	ns6:order	"1113" .
ns27:i_cisk_sfjobx	rdf:type	ns2:IndicatorToGroupMembership ;
	rdfs:label	"ict-specialist" ;
	ns6:member-of	ns14:ict-specialist ;
	ns6:order	"6" .
ns27:i_cprg	rdf:type	ns2:IndicatorToGroupMembership ;
	rdfs:label	"ict-specialist" ;
	ns6:member-of	ns14:ict-specialist ;
	ns6:order	"9" .
ns27:i_skedu	rdf:type	ns2:IndicatorToGroupMembership ;
	rdfs:label	"ict-specialist" ;
	ns6:member-of	ns14:ict-specialist ;
	ns6:order	"7" .
ns27:p_iuse	rdf:type	ns2:IndicatorToGroupMembership ;
	rdfs:label	"ict-specialist" ;
	ns6:member-of	ns14:ict-specialist ;
	ns6:order	"8" .
ns17:h_fbbfix	rdf:type	ns2:IndicatorToGroupMembership ;
	rdfs:label	"broadband" ;
	ns6:member-of	ns14:broadband ;
	ns6:order	"11" .
ns17:h_ubbfix	rdf:type	ns2:IndicatorToGroupMembership ;
	rdfs:label	"broadband" ;
	ns6:member-of	ns14:broadband ;
	ns6:order	"12" .
ns1:h_fbbfix	rdf:type	ns2:Indicator ,
		skos:Concept ;
	skos:prefLabel	"Households with fast fixed broadband connection" ;
	dct:source	ns5:estathh_cocom ;
	skos:notation	"h_fbbfix" ;
	skos:altLabel	"Households with fast fixed broadband connection" ;
	ns6:membership	ns17:h_fbbfix ;
	skos:definition	"Households with fast fixed broadband connection" ;
	skos:topConceptOf	ns8:indicator .
ns1:h_ubbfix	rdf:type	ns2:Indicator ,
		skos:Concept ;
	skos:prefLabel	"Households with ultrafast fixed broadband connection" ;
	dct:source	ns5:estathh_cocom ;
	skos:notation	"h_ubbfix" ;
	skos:altLabel	"Households with ultrafast fixed broadband connection" ;
	ns6:membership	ns17:h_ubbfix ;
	skos:definition	"Households with ultrafast fixed broadband connection" ;
	skos:topConceptOf	ns8:indicator .
ns22:e_gov_ebus	rdf:type	ns2:IndicatorToGroupMembership ;
	rdfs:label	"egovernment" ;
	ns6:member-of	ns14:egovernment ;
	ns6:order	"8" .
ns1:e_gov_ebus	rdf:type	ns2:Indicator ,
		skos:Concept ;
	skos:prefLabel	"Digital Public Services for Businesses (up to 2020)" ;
	dct:source	ns5:egov_bench ;
	skos:notation	"e_gov_ebus" ;
	skos:altLabel	"Digital Public Services for Businesses (up to 2020)" ;
	ns6:membership	ns22:e_gov_ebus ;
	skos:definition	"The extent to which a service or information concerning service for businesses is provided online and via a portal. Services that are offered fully, partially or not at all online. " ;
	skos:topConceptOf	ns8:indicator .
ns1:i_dsk_s_x	rdf:type	ns2:Indicator ,
		skos:Concept ;
	skos:prefLabel	"DSI 2015-2019 Individuals with no digital skills in Software domain" ;
	dct:source	ns5:estat_isoc_sk_dskl_i ;
	skos:notation	"i_dsk_s_x" ;
	skos:altLabel	"DSI 2015-2019 - Software Domain - No Skills" ;
	ns6:membership	ns26:i_dsk_s_x ;
	skos:definition	"Software skills for content manipulation refer to the ability to create and edit new content (from word processing to images and video); integrate and re-elaborate previous knowledge and content; produce creative expressions, media outputs and programming; deal with and apply intellectual property rights and licences. The indicator is based on six activities internet users have been able to do during previous 3 months. The scores are basic, above basic and none. Individuals not using internet are classified without digital skills." ;
	skos:note	"Detailed results are available in the Eurostat table <a href=\"http://appsso.eurostat.ec.europa.eu/nui/show.do?dataset=isoc_sk_dskl_i&lang=en\">ISOC_SK_DSKL_I</a>. Consult the <a href=\"https://ec.europa.eu/digital-agenda/en/news/new-comprehensive-digital-skills-indicator\"> methodological note</a> on DG CONNECT newsroom." ;
	skos:topConceptOf	ns8:indicator .
ns1:i_dsk_c_ab	rdf:type	ns2:Indicator ,
		skos:Concept ;
	skos:prefLabel	"DSI 2015-2019 Individuals with above basic level of digital skills in Communication domain" ;
	dct:source	ns5:estat_isoc_sk_dskl_i ;
	skos:notation	"i_dsk_c_ab" ;
	skos:altLabel	"DSI 2015-2019 - Communication Domain - Above Basic Skills" ;
	ns6:membership	ns26:i_dsk_c_ab ;
	skos:definition	"These skills refer to the ability to communicate in digital environments, share resources through online tools, link with others and collaborate through digital tools, interact with and participate in communities and networks, cross-cultural awareness. The indicator is based on four activities internet users have been able to do online during previous 3 months. The scores are basic, above basic and none. Individuals not using internet are classified without digital skills." ;
	skos:note	"Detailed results are available in the Eurostat table <a href=\"http://appsso.eurostat.ec.europa.eu/nui/show.do?dataset=isoc_sk_dskl_i&lang=en\">ISOC_SK_DSKL_I</a>. Consult the <a href=\"https://ec.europa.eu/digital-agenda/en/news/new-comprehensive-digital-skills-indicator\"> methodological note</a> on DG CONNECT newsroom." ;
	skos:topConceptOf	ns8:indicator .
ns39:desi_conn	rdf:type	ns2:IndicatorToGroupMembership ;
	rdfs:label	"desi_dim" ;
	ns6:member-of	ns14:desi_dim ;
	ns6:order	"2" .
ns39:desi_dps	rdf:type	ns2:IndicatorToGroupMembership ;
	rdfs:label	"desi_dim" ;
	ns6:member-of	ns14:desi_dim ;
	ns6:order	"4" .
ns39:desi_hc	rdf:type	ns2:IndicatorToGroupMembership ;
	rdfs:label	"desi_dim" ;
	ns6:member-of	ns14:desi_dim ;
	ns6:order	"1" .
ns39:desi_idt	rdf:type	ns2:IndicatorToGroupMembership ;
	rdfs:label	"desi_dim" ;
	ns6:member-of	ns14:desi_dim ;
	ns6:order	"3" .
ns36:desi_5g	rdf:type	ns2:IndicatorToGroupMembership ;
	rdfs:label	"desi_ind" ;
	ns6:member-of	ns14:desi_ind ;
	ns6:order	"232" .
ns36:desi_5gc	rdf:type	ns2:IndicatorToGroupMembership ;
	rdfs:label	"desi_ind" ;
	ns6:member-of	ns14:desi_ind ;
	ns6:order	"233" .
ns36:desi_bbpi	rdf:type	ns2:IndicatorToGroupMembership ;
	rdfs:label	"desi_ind" ;
	ns6:member-of	ns14:desi_ind ;
	ns6:order	"241" .
ns36:desi_dps_egovuser	rdf:type	ns2:IndicatorToGroupMembership ;
	rdfs:label	"desi_ind" ;
	ns6:member-of	ns14:desi_ind ;
	ns6:order	"411" .
ns36:desi_dps_opendata	rdf:type	ns2:IndicatorToGroupMembership ;
	rdfs:label	"desi_ind" ;
	ns6:member-of	ns14:desi_ind ;
	ns6:order	"415" .
ns36:desi_dps_prefform	rdf:type	ns2:IndicatorToGroupMembership ;
	rdfs:label	"desi_ind" ;
	ns6:member-of	ns14:desi_ind ;
	ns6:order	"412" .
ns36:desi_dps_psbiz	rdf:type	ns2:IndicatorToGroupMembership ;
	rdfs:label	"desi_ind" ;
	ns6:member-of	ns14:desi_ind ;
	ns6:order	"414" .
ns36:desi_dps_pscit	rdf:type	ns2:IndicatorToGroupMembership ;
	rdfs:label	"desi_ind" ;
	ns6:member-of	ns14:desi_ind ;
	ns6:order	"413" .
ns36:desi_fbbc	rdf:type	ns2:IndicatorToGroupMembership ;
	rdfs:label	"desi_ind" ;
	ns6:member-of	ns14:desi_ind ;
	ns6:order	"221" .
ns36:desi_fbbtc	rdf:type	ns2:IndicatorToGroupMembership ;
	rdfs:label	"desi_ind" ;
	ns6:member-of	ns14:desi_ind ;
	ns6:order	"211" .
ns36:desi_gbpstc	rdf:type	ns2:IndicatorToGroupMembership ;
	rdfs:label	"desi_ind" ;
	ns6:member-of	ns14:desi_ind ;
	ns6:order	"213" .
ns36:desi_hc_abds	rdf:type	ns2:IndicatorToGroupMembership ;
	rdfs:label	"desi_ind" ;
	ns6:member-of	ns14:desi_ind ;
	ns6:order	"112" .
ns36:desi_hc_abss	rdf:type	ns2:IndicatorToGroupMembership ;
	rdfs:label	"desi_ind" ;
	ns6:member-of	ns14:desi_ind ;
	ns6:order	"113" .
ns36:desi_hc_bds	rdf:type	ns2:IndicatorToGroupMembership ;
	rdfs:label	"desi_ind" ;
	ns6:member-of	ns14:desi_ind ;
	ns6:order	"111" .
ns36:desi_hc_entict	rdf:type	ns2:IndicatorToGroupMembership ;
	rdfs:label	"desi_ind" ;
	ns6:member-of	ns14:desi_ind ;
	ns6:order	"123" .
ns36:desi_hc_fictspec	rdf:type	ns2:IndicatorToGroupMembership ;
	rdfs:label	"desi_ind" ;
	ns6:member-of	ns14:desi_ind ;
	ns6:order	"122" .
ns36:desi_hc_ictg	rdf:type	ns2:IndicatorToGroupMembership ;
	rdfs:label	"desi_ind" ;
	ns6:member-of	ns14:desi_ind ;
	ns6:order	"124" .
ns36:desi_hc_ictspec	rdf:type	ns2:IndicatorToGroupMembership ;
	rdfs:label	"desi_ind" ;
	ns6:member-of	ns14:desi_ind ;
	ns6:order	"121" .
ns36:desi_idt_ai	rdf:type	ns2:IndicatorToGroupMembership ;
	rdfs:label	"desi_ind" ;
	ns6:member-of	ns14:desi_ind ;
	ns6:order	"325" .
ns36:desi_idt_bigdat	rdf:type	ns2:IndicatorToGroupMembership ;
	rdfs:label	"desi_ind" ;
	ns6:member-of	ns14:desi_ind ;
	ns6:order	"323" .
ns36:desi_idt_cloud	rdf:type	ns2:IndicatorToGroupMembership ;
	rdfs:label	"desi_ind" ;
	ns6:member-of	ns14:desi_ind ;
	ns6:order	"324" .
ns36:desi_idt_ecomturn	rdf:type	ns2:IndicatorToGroupMembership ;
	rdfs:label	"desi_ind" ;
	ns6:member-of	ns14:desi_ind ;
	ns6:order	"332" .
ns36:desi_idt_einv	rdf:type	ns2:IndicatorToGroupMembership ;
	rdfs:label	"desi_ind" ;
	ns6:member-of	ns14:desi_ind ;
	ns6:order	"327" .
ns36:desi_idt_eis	rdf:type	ns2:IndicatorToGroupMembership ;
	rdfs:label	"desi_ind" ;
	ns6:member-of	ns14:desi_ind ;
	ns6:order	"321" .
ns36:desi_idt_ictsust	rdf:type	ns2:IndicatorToGroupMembership ;
	rdfs:label	"desi_ind" ;
	ns6:member-of	ns14:desi_ind ;
	ns6:order	"326" .
ns36:desi_idt_sellcb	rdf:type	ns2:IndicatorToGroupMembership ;
	rdfs:label	"desi_ind" ;
	ns6:member-of	ns14:desi_ind ;
	ns6:order	"333" .
ns36:desi_idt_smedi	rdf:type	ns2:IndicatorToGroupMembership ;
	rdfs:label	"desi_ind" ;
	ns6:member-of	ns14:desi_ind ;
	ns6:order	"311" .
ns36:desi_idt_smeso	rdf:type	ns2:IndicatorToGroupMembership ;
	rdfs:label	"desi_ind" ;
	ns6:member-of	ns14:desi_ind ;
	ns6:order	"331" .
ns36:desi_idt_socmed	rdf:type	ns2:IndicatorToGroupMembership ;
	rdfs:label	"desi_ind" ;
	ns6:member-of	ns14:desi_ind ;
	ns6:order	"322" .
ns36:desi_mbbtu	rdf:type	ns2:IndicatorToGroupMembership ;
	rdfs:label	"desi_ind" ;
	ns6:member-of	ns14:desi_ind ;
	ns6:order	"234" .
ns36:desi_ufbbtu	rdf:type	ns2:IndicatorToGroupMembership ;
	rdfs:label	"desi_ind" ;
	ns6:member-of	ns14:desi_ind ;
	ns6:order	"212" .
ns36:desi_vhcnc	rdf:type	ns2:IndicatorToGroupMembership ;
	rdfs:label	"desi_ind" ;
	ns6:member-of	ns14:desi_ind ;
	ns6:order	"222" .
ns38:desi_c_bbpi	rdf:type	ns2:IndicatorToGroupMembership ;
	rdfs:label	"desi_subdim" ;
	ns6:member-of	ns14:desi_subdim ;
	ns6:order	"24" .
ns38:desi_c_fbbc	rdf:type	ns2:IndicatorToGroupMembership ;
	rdfs:label	"desi_subdim" ;
	ns6:member-of	ns14:desi_subdim ;
	ns6:order	"22" .
ns38:desi_c_fbbtc	rdf:type	ns2:IndicatorToGroupMembership ;
	rdfs:label	"desi_subdim" ;
	ns6:member-of	ns14:desi_subdim ;
	ns6:order	"21" .
ns38:desi_c_mbb	rdf:type	ns2:IndicatorToGroupMembership ;
	rdfs:label	"desi_subdim" ;
	ns6:member-of	ns14:desi_subdim ;
	ns6:order	"23" .
ns38:desi_dps_egov	rdf:type	ns2:IndicatorToGroupMembership ;
	rdfs:label	"desi_subdim" ;
	ns6:member-of	ns14:desi_subdim ;
	ns6:order	"41" .
ns38:desi_hc_asd	rdf:type	ns2:IndicatorToGroupMembership ;
	rdfs:label	"desi_subdim" ;
	ns6:member-of	ns14:desi_subdim ;
	ns6:order	"12" .
ns38:desi_hc_bsu	rdf:type	ns2:IndicatorToGroupMembership ;
	rdfs:label	"desi_subdim" ;
	ns6:member-of	ns14:desi_subdim ;
	ns6:order	"11" .
ns38:desi_idt_di	rdf:type	ns2:IndicatorToGroupMembership ;
	rdfs:label	"desi_subdim" ;
	ns6:member-of	ns14:desi_subdim ;
	ns6:order	"31" .
ns38:desi_idt_dtb	rdf:type	ns2:IndicatorToGroupMembership ;
	rdfs:label	"desi_subdim" ;
	ns6:member-of	ns14:desi_subdim ;
	ns6:order	"32" .
ns38:desi_idt_ecomm	rdf:type	ns2:IndicatorToGroupMembership ;
	rdfs:label	"desi_subdim" ;
	ns6:member-of	ns14:desi_subdim ;
	ns6:order	"33" .
ns40:desi_total	rdf:type	ns2:IndicatorToGroupMembership ;
	rdfs:label	"desi_total" ;
	ns6:member-of	ns14:desi_total ;
	ns6:order	"1" .