@prefix rdf:	<http://www.w3.org/1999/02/22-rdf-syntax-ns#> .
@prefix ns1:	<http://semantic.digital-agenda-data.eu/codelist/> .
@prefix skos:	<http://www.w3.org/2004/02/skos/core#> .
@prefix ns3:	<http://purl.org/linked-data/sdmx#> .
@prefix xsd:	<http://www.w3.org/2001/XMLSchema#> .
@prefix dct:	<http://purl.org/dc/terms/> .
@prefix rdfs:	<http://www.w3.org/2000/01/rdf-schema#> .
@prefix ns7:	<http://semantic.digital-agenda-data.eu/codelist/breakdown-group/> .
@prefix ns8:	<http://semantic.digital-agenda-data.eu/def/> .
@prefix ns9:	<http://semantic.digital-agenda-data.eu/def/class/> .
@prefix ns10:	<http://semantic.digital-agenda-data.eu/def/property/> .
@prefix ns11:	<http://eurostat.linked-statistics.org/dic/> .
@prefix ns12:	<https://ec.europa.eu/digital-agenda/en/news/> .

ns1:breakdown-group
	rdf:type	skos:ConceptScheme , ns3:CodeList ;
	dct:modified	"2020-06-11T11:23:24"^^xsd:dateTime ;
	rdfs:isDefinedBy	<http://digital-agenda-data.eu/> ;
	skos:prefLabel	"Breakdown groups used by Digital Agenda Scoreboard" ;
	skos:notation	"CL_BREAKDOWN_GROUP" ;
	skos:hasTopConcept	ns7:by_location , ns7:byage3classes , ns7:byage6classes , ns7:bycbirth , ns7:byccitizen , ns7:byccsophistication , ns7:bydensity , ns7:bydigint2015 , ns7:bydownloadspeed , ns7:bydownloadspeed4 , ns7:byedu , ns7:byedugrade , ns7:byemp , ns7:byentsize , ns7:byentsize_s_m_l , ns7:byfbbtech , ns7:bygender , ns7:byictsector2subsec , ns7:byictsector6subsec , ns7:bynaceeu , ns7:bynacenat , ns7:byorganizationclass , ns7:byregion , ns7:byrisk , ns7:byskills , ns7:bytypeproduct , ns7:cnect_directorates , ns7:desi , ns7:desi_1_conn , ns7:desi_2_hc , ns7:desi_2a_bsu , ns7:desi_2b_asd , ns7:desi_3_ui , ns7:desi_3c_trans , ns7:desi_4_idt , ns7:desi_4a_bd , ns7:desi_4b_ecomm , ns7:desi_5_dps , ns7:desi_5a_egov , ns7:desi_totals , ns7:digskill_level , ns7:e_gov_1_ucg , ns7:e_gov_2_tg , ns7:e_gov_3_cm , ns7:e_gov_4_bm , ns7:e_gov_5_ke , ns7:e_gov_events , ns7:econsector , ns7:econsector_size , ns7:egov_le , ns7:epsi_dimensions , ns7:hhbyiq , ns7:hhbytype , ns7:infso_directorates , ns7:labour_force , ns7:manuf , ns7:mhz_bands , ns7:others , ns7:rural_pop , ns7:sos_agg , ns7:total , ns7:wid_score , ns7:desi_1a_fbbtc , ns7:desi_1b_fbbc , ns7:desi_1c_mbb , ns7:desi_1d_bbpi , ns7:childrenhh , ns7:ictproffession , ns7:workingscheme , ns7:desi_3a_ui , ns7:desi_3b_acton ;
	skos:inScheme	ns8:scheme .
ns7:by_location
	rdf:type	ns9:BreakdownGroup , skos:Concept ;
	skos:prefLabel	"Geographical area" ;
	skos:notation	"by_location" ;
	skos:altLabel	"Geographical area" ;
	ns10:order	"100" ;
	skos:definition	"The following breakdown is considered: Own country, Other EU countries, Rest of the world" ;
	skos:topConceptOf	ns1:breakdown-group .
ns7:byage3classes
	rdf:type	ns9:BreakdownGroup , skos:Concept ;
	rdfs:seeAlso	ns11:ind_type ;
	skos:prefLabel	"Age (3 groups)" ;
	skos:notation	"byage3classes" ;
	skos:altLabel	"Age (3 groups)" ;
	ns10:order	"2" ;
	skos:definition	"breakdown by 3 age groups: 16-24, 25-54 and 55-74 years" ;
	skos:topConceptOf	ns1:breakdown-group .
ns7:byage6classes
	rdf:type	ns9:BreakdownGroup , skos:Concept ;
	rdfs:seeAlso	ns11:ind_type ;
	skos:prefLabel	"Age (6 groups)" ;
	skos:notation	"byage6classes" ;
	skos:altLabel	"Age (6 groups)" ;
	ns10:order	"3" ;
	skos:definition	"breakdown by 6 age groups: 16-24, 25-34,35-44, 45-54, 55-64 and 65-74 years" ;
	skos:topConceptOf	ns1:breakdown-group .
ns7:bycbirth
	rdf:type	ns9:BreakdownGroup , skos:Concept ;
	rdfs:seeAlso	ns11:ind_type ;
	skos:prefLabel	"Country of birth" ;
	skos:notation	"bycbirth" ;
	skos:altLabel	"Country of birth" ;
	ns10:order	"7" ;
	skos:definition	"breakdown by country of birth (native, EU country, other non-EU country)" ;
	skos:topConceptOf	ns1:breakdown-group .
ns7:byccitizen
	rdf:type	ns9:BreakdownGroup , skos:Concept ;
	rdfs:seeAlso	ns11:ind_type ;
	skos:prefLabel	"Citizenship" ;
	skos:notation	"byccitizen" ;
	skos:altLabel	"Citizenship" ;
	ns10:order	"8" ;
	skos:definition	"breakdown by citizenship (nationals, other EU country nationals, non EU nationals)" ;
	skos:topConceptOf	ns1:breakdown-group .
ns7:byccsophistication
	rdf:type	ns9:BreakdownGroup , skos:Concept ;
	skos:prefLabel	"CC services sophistication" ;
	skos:notation	"byccsophistication" ;
	skos:altLabel	"CC services sophistication" ;
	skos:definition	"The seven types of cloud computing services proposed in Eurostat questionnaire are attributed a low-medium-high degree of sophistication which somehow reflect also the degree of enterprise's dependence or trust running more or less vital data-services in the cloud." ;
	skos:topConceptOf	ns1:breakdown-group .
ns7:bydensity
	rdf:type	ns9:BreakdownGroup , skos:Concept ;
	skos:prefLabel	"Urban-rural density of the living area" ;
	skos:notation	"bydensity" ;
	skos:altLabel	"Urban-rural density of the living area" ;
	ns10:order	"12" ;
	skos:definition	"breakdown by 3 type of living areas: densely-populated with at least 500 inhabitants/Km2, sparsely populated area with less than 100 inhabitants/Km2, and intermediate." ;
	skos:topConceptOf	ns1:breakdown-group .
ns7:bydigint2015
	rdf:type	ns9:BreakdownGroup , skos:Concept ;
	skos:prefLabel	"Level of digital intensity" ;
	skos:notation	"bydigint2015" ;
	skos:altLabel	"Level of digital intensity" ;
	ns10:order	"10" ;
	skos:definition	"The Digital Intensity score is based on counting how many out of 12 technologies are used by each enterprise. Then they are divided into four clusters of digital intensity: Very Low (scores 0-3), Low (score 4-6), High (score 7-9), Very High (score 10-12)." ;
	skos:topConceptOf	ns1:breakdown-group .
ns7:bydownloadspeed
	rdf:type	ns9:BreakdownGroup , skos:Concept ;
	skos:prefLabel	"Maximum advertised download speed 3 categories" ;
	skos:notation	"bydownloadspeed" ;
	skos:altLabel	"Max. adv. download speed 3 cat." ;
	ns10:order	"29" ;
	skos:definition	"breakdown by the maximum advertised download speed of internet access offers, in Mbps (above 8 and up to 12;  above 12 and up to 30; above 30)." ;
	skos:topConceptOf	ns1:breakdown-group .
ns7:bydownloadspeed4
	rdf:type	ns9:BreakdownGroup , skos:Concept ;
	skos:prefLabel	"Maximum advertised download speed 4 categories" ;
	skos:notation	"bydownloadspeed4" ;
	skos:altLabel	"Max. adv. download speed 4 cat." ;
	ns10:order	"30" ;
	skos:definition	"breakdown by the maximum advertised download speed of internet access offers, in Mbps (above 8 and up to 12;  above 12 and up to 30; above 30 and up to 100; above 100)." ;
	skos:topConceptOf	ns1:breakdown-group .
ns7:byedu
	rdf:type	ns9:BreakdownGroup , skos:Concept ;
	rdfs:seeAlso	ns11:ind_type ;
	skos:prefLabel	"Education level" ;
	skos:notation	"byedu" ;
	skos:altLabel	"Education level" ;
	ns10:order	"4" ;
	skos:definition	"brekadown by education level (low, medium, high, based on ISCED 0-2, 3-4, 5-6)" ;
	skos:topConceptOf	ns1:breakdown-group .
ns7:byedugrade
	rdf:type	ns9:BreakdownGroup , skos:Concept ;
	skos:prefLabel	"Education grade (years of schooling)" ;
	skos:notation	"byedugrade" ;
	skos:altLabel	"Education grade (years of schooling)" ;
	ns10:order	"21" ;
	skos:definition	"breakdown by education grade is based on the years of schooling, counting from the first year of Primary - ISCED level 1." ;
	skos:topConceptOf	ns1:breakdown-group .
ns7:byemp
	rdf:type	ns9:BreakdownGroup , skos:Concept ;
	rdfs:seeAlso	ns11:ind_type ;
	skos:prefLabel	"Employment status" ;
	skos:notation	"byemp" ;
	skos:altLabel	"Employment status" ;
	ns10:order	"5" ;
	skos:definition	"breakdown by employment status (employee or self-employed, unemployed, student, retired and other inactive)" ;
	skos:topConceptOf	ns1:breakdown-group .
ns7:byentsize
	rdf:type	ns9:BreakdownGroup , skos:Concept ;
	rdfs:seeAlso	ns11:sizen_r2 ;
	skos:prefLabel	"Enterprise size (SMEs, Large)" ;
	skos:notation	"byentsize" ;
	skos:altLabel	"Enterprise size (SMEs, Large)" ;
	ns10:order	"15" ;
	skos:definition	"breakdown by company size (SMEs with 10-249 persons employed, Large enterprises with 250 or more)" ;
	skos:topConceptOf	ns1:breakdown-group .
ns7:byentsize_s_m_l
	rdf:type	ns9:BreakdownGroup , skos:Concept ;
	rdfs:seeAlso	ns11:sizen_r2 ;
	skos:prefLabel	"Enterprise size (Small, Medium, Large)" ;
	skos:notation	"byentsize_s_m_l" ;
	skos:altLabel	"Enterprise size (Small, Medium, Large)" ;
	ns10:order	"16" ;
	skos:definition	"breakdown by company size (Small enterprises (10-49 persons employed),Medium enterprises (50-249 persons employed), Large enterprises with 250 or more))" ;
	skos:topConceptOf	ns1:breakdown-group .
ns7:byfbbtech
	rdf:type	ns9:BreakdownGroup , skos:Concept ;
	skos:prefLabel	"Fixed broadband technology" ;
	skos:notation	"byfbbtech" ;
	skos:altLabel	"Fixed broadband technology" ;
	ns10:order	"19" ;
	skos:definition	"breakdown by type of fixed broadband technology: xDSL, cable modem, Fiber to the x." ;
	skos:topConceptOf	ns1:breakdown-group .
ns7:bygender
	rdf:type	ns9:BreakdownGroup , skos:Concept ;
	rdfs:seeAlso	ns11:ind_type ;
	skos:prefLabel	"Gender" ;
	skos:notation	"bygender" ;
	skos:altLabel	"Gender" ;
	ns10:order	"6" ;
	skos:definition	"breakdown by gender (male, female)" ;
	skos:topConceptOf	ns1:breakdown-group .
ns7:byictsector2subsec
	rdf:type	ns9:BreakdownGroup , skos:Concept ;
	skos:prefLabel	"ICT Sectors (2 sub-sectors)" ;
	skos:notation	"byictsector2subsec" ;
	skos:altLabel	"ICT Sectors (2 sub-sectors)" ;
	skos:definition	"breakdown by 2 operational ICT sub sectors (Manufacturing NACE2 261 to 264, Services NACE2 582,61, 62, 631, 951)" ;
	skos:topConceptOf	ns1:breakdown-group .
ns7:byictsector6subsec
	rdf:type	ns9:BreakdownGroup , skos:Concept ;
	skos:prefLabel	"ICT Sectors (6 sub-sectors)" ;
	skos:notation	"byictsector6subsec" ;
	skos:altLabel	"ICT Sectors (6 sub-sectors)" ;
	skos:definition	"breakdown by 6 operational ICT sectors: NACE2 261 to 264, 582,61, 62, 631, 951 " ;
	skos:topConceptOf	ns1:breakdown-group .
ns7:bynaceeu
	rdf:type	ns9:BreakdownGroup , skos:Concept ;
	skos:prefLabel	"NACE EU" ;
	skos:notation	"bynaceeu" ;
	skos:altLabel	"NACE EU" ;
	ns10:order	"16" ;
	skos:definition	"breakdown by NACE EU" ;
	skos:topConceptOf	ns1:breakdown-group .
ns7:bynacenat
	rdf:type	ns9:BreakdownGroup , skos:Concept ;
	skos:prefLabel	"NACE NAT" ;
	skos:notation	"bynacenat" ;
	skos:altLabel	"NACE NAT" ;
	ns10:order	"17" ;
	skos:definition	"breakdown by NACE NAT" ;
	skos:topConceptOf	ns1:breakdown-group .
ns7:byorganizationclass
	rdf:type	ns9:BreakdownGroup , skos:Concept ;
	skos:prefLabel	"Type of organization" ;
	skos:notation	"byorganizationclass" ;
	skos:altLabel	"Type of organization" ;
	ns10:order	"20" ;
	skos:definition	"Partner organisations are divided into four main classes: \nSME = Small and medium individual private enterprises with less than 250 employed persons and a turnover \u2264 50 millions euro or a balance sheet total \u2264 43 millions euro. \nLarge = all other enterprises. \nHES/REC = includes public or private higher education institutions and not for profit research organisations. \nNIL = includes all other types of organisations (i.e. public administrations, NGO, public sector enterprises, etc.)." ;
	skos:topConceptOf	ns1:breakdown-group .
ns7:byregion
	rdf:type	ns9:BreakdownGroup , skos:Concept ;
	skos:prefLabel	"Objective1-Convergence regions" ;
	skos:notation	"byregion" ;
	skos:altLabel	"Objective1-Convergence regions" ;
	ns10:order	"13" ;
	skos:definition	"breakdown by regions inside/outsisde Objective 1 - Convergence regions, as defined by Structural Funds regulations" ;
	skos:topConceptOf	ns1:breakdown-group .
ns7:byrisk
	rdf:type	ns9:BreakdownGroup , skos:Concept ;
	rdfs:seeAlso	ns11:ind_type ;
	skos:prefLabel	"Disadvantage factors" ;
	skos:notation	"byrisk" ;
	skos:altLabel	"Disadvantage factors" ;
	ns10:order	"9" ;
	skos:definition	"breakdown by disadvantage factors defined as one of the 3 following characteristics: 55 to 74 years old; low education; unemployed or inactive or retired." ;
	skos:topConceptOf	ns1:breakdown-group .
ns7:byskills
	rdf:type	ns9:BreakdownGroup , skos:Concept ;
	rdfs:seeAlso	ns11:indic_is ;
	skos:prefLabel	"Computer skills" ;
	skos:notation	"byskills" ;
	skos:altLabel	"Computer skills" ;
	ns10:order	"10" ;
	skos:definition	"breakdown by computer skills: High (5-6), Medium (3-4), Low (1-2), None(0), but have ever used a computer. The indicator is based on the count of how many of the following 6 activities individuals have ever carried out: coping or moving a file or folder, using copy and paste tools, using basic arithmetic formula in a spreadsheet, compressing (or zipping) files, connecting and installing new devices, writing a computer program using a specialised programming language. Only those having ever used a computer were proposed the question." ;
	skos:topConceptOf	ns1:breakdown-group .
ns7:bytypeproduct
	rdf:type	ns9:BreakdownGroup , skos:Concept ;
	skos:prefLabel	"Type of products" ;
	skos:notation	"bytypeproduct" ;
	skos:altLabel	"Type of products" ;
	ns10:order	"22" ;
	skos:definition	"breakdown by type of products: goods or services" ;
	skos:topConceptOf	ns1:breakdown-group .
ns7:cnect_directorates
	rdf:type	ns9:BreakdownGroup , skos:Concept ;
	skos:prefLabel	"DG CONNECT Directorates" ;
	skos:notation	"cnect_directorates" ;
	skos:altLabel	"DG CONNECT Directorates" ;
	skos:definition	"Organisation chart since 2012. See: http://ec.europa.eu/dgs/connect/who-we-are" ;
	skos:topConceptOf	ns1:breakdown-group .
ns7:desi
	rdf:type	ns9:BreakdownGroup , skos:Concept ;
	skos:prefLabel	"Main Dimensions of the DESI" ;
	skos:notation	"desi" ;
	ns10:order	"2" ;
	skos:topConceptOf	ns1:breakdown-group .
ns7:desi_1_conn
	rdf:type	ns9:BreakdownGroup , skos:Concept ;
	skos:prefLabel	"Sub-dimensions of 1 Connectivity" ;
	skos:notation	"desi_1_conn" ;
	ns10:order	"3" ;
	skos:topConceptOf	ns1:breakdown-group .
ns7:desi_2_hc
	rdf:type	ns9:BreakdownGroup , skos:Concept ;
	skos:prefLabel	"Sub-dimensions of 2 Human Capital" ;
	skos:notation	"desi_2_hc" ;
	ns10:order	"4" ;
	skos:topConceptOf	ns1:breakdown-group .
ns7:desi_2a_bsu
	rdf:type	ns9:BreakdownGroup , skos:Concept ;
	skos:prefLabel	"Indicators under 2a Internet User Skills" ;
	skos:notation	"desi_2a_bsu" ;
	ns10:order	"13" ;
	skos:topConceptOf	ns1:breakdown-group .
ns7:desi_2b_asd
	rdf:type	ns9:BreakdownGroup , skos:Concept ;
	skos:prefLabel	"Indicators under 2b Advanced Skills and Development" ;
	skos:notation	"desi_2b_asd" ;
	ns10:order	"14" ;
	skos:topConceptOf	ns1:breakdown-group .
ns7:desi_3_ui
	rdf:type	ns9:BreakdownGroup , skos:Concept ;
	skos:prefLabel	"Sub-dimensions of 3 Use of Internet Services" ;
	skos:notation	"desi_3_ui" ;
	ns10:order	"5" ;
	skos:topConceptOf	ns1:breakdown-group .
ns7:desi_3c_trans
	rdf:type	ns9:BreakdownGroup , skos:Concept ;
	skos:prefLabel	"Indicators under 3c Transactions" ;
	skos:notation	"desi_3c_trans" ;
	ns10:order	"17" ;
	skos:topConceptOf	ns1:breakdown-group .
ns7:desi_4_idt
	rdf:type	ns9:BreakdownGroup , skos:Concept ;
	skos:prefLabel	"Sub-dimensions of 4 Integration of Digital Technology" ;
	skos:notation	"desi_4_idt" ;
	ns10:order	"6" ;
	skos:topConceptOf	ns1:breakdown-group .
ns7:desi_4a_bd
	rdf:type	ns9:BreakdownGroup , skos:Concept ;
	skos:prefLabel	"Indicators under 4a Business digitization" ;
	skos:notation	"desi_4a_bd" ;
	ns10:order	"18" ;
	skos:topConceptOf	ns1:breakdown-group .
ns7:desi_4b_ecomm
	rdf:type	ns9:BreakdownGroup , skos:Concept ;
	skos:prefLabel	"Indicators under 4b e-Commerce" ;
	skos:notation	"desi_4b_ecomm" ;
	ns10:order	"19" ;
	skos:topConceptOf	ns1:breakdown-group .
ns7:desi_5_dps
	rdf:type	ns9:BreakdownGroup , skos:Concept ;
	skos:prefLabel	"Sub-dimensions of 5 Digital Public Services" ;
	skos:notation	"desi_5_dps" ;
	ns10:order	"7" ;
	skos:topConceptOf	ns1:breakdown-group .
ns7:desi_5a_egov
	rdf:type	ns9:BreakdownGroup , skos:Concept ;
	skos:prefLabel	"Indicators under 5a e-Government" ;
	skos:notation	"desi_5a_egov" ;
	ns10:order	"20" ;
	skos:topConceptOf	ns1:breakdown-group .
ns7:desi_totals
	rdf:type	ns9:BreakdownGroup , skos:Concept ;
	skos:prefLabel	"Aggregate scores" ;
	skos:notation	"desi_totals" ;
	ns10:order	"1" ;
	skos:topConceptOf	ns1:breakdown-group .
ns7:digskill_level
	rdf:type	ns9:BreakdownGroup , skos:Concept ;
	skos:prefLabel	"Digital skills level" ;
	skos:notation	"digskill_level" ;
	skos:altLabel	"Digital skills level" ;
	ns10:order	"25" ;
	skos:topConceptOf	ns1:breakdown-group .
ns7:e_gov_1_ucg
	rdf:type	ns9:BreakdownGroup , skos:Concept ;
	skos:prefLabel	"User Centric Government" ;
	skos:notation	"e_gov_1_ucg" ;
	skos:altLabel	"User Centric Government" ;
	ns10:order	"108" ;
	skos:definition	"Breakdown by User Centric Government" ;
	skos:topConceptOf	ns1:breakdown-group .
ns7:e_gov_2_tg
	rdf:type	ns9:BreakdownGroup , skos:Concept ;
	skos:prefLabel	"Transparent Government" ;
	skos:notation	"e_gov_2_tg" ;
	skos:altLabel	"Transparent Government" ;
	ns10:order	"109" ;
	skos:definition	"Breakdown by Transparent Government" ;
	skos:topConceptOf	ns1:breakdown-group .
ns7:e_gov_3_cm
	rdf:type	ns9:BreakdownGroup , skos:Concept ;
	skos:prefLabel	"Citizen Mobility" ;
	skos:notation	"e_gov_3_cm" ;
	skos:altLabel	"Citizen Mobility" ;
	ns10:order	"110" ;
	skos:definition	"Breakdown by Citizen Mobility" ;
	skos:topConceptOf	ns1:breakdown-group .
ns7:e_gov_4_bm
	rdf:type	ns9:BreakdownGroup , skos:Concept ;
	skos:prefLabel	"Business Mobility" ;
	skos:notation	"e_gov_4_bm" ;
	skos:altLabel	"Business Mobility" ;
	ns10:order	"111" ;
	skos:definition	"Breakdown by Business Mobility" ;
	skos:topConceptOf	ns1:breakdown-group .
ns7:e_gov_5_ke
	rdf:type	ns9:BreakdownGroup , skos:Concept ;
	skos:prefLabel	"Key Enablers" ;
	skos:notation	"e_gov_5_ke" ;
	skos:altLabel	"Key Enablers" ;
	ns10:order	"112" ;
	skos:definition	"Breakdown by Key Enablers" ;
	skos:topConceptOf	ns1:breakdown-group .
ns7:e_gov_events
	rdf:type	ns9:BreakdownGroup , skos:Concept ;
	skos:prefLabel	"Life Events for eGovernment" ;
	skos:notation	"e_gov_events" ;
	skos:altLabel	"Life Events for eGovernment" ;
	ns10:order	"107" ;
	skos:definition	"Breakdown by 8 life events for eGovernment" ;
	skos:topConceptOf	ns1:breakdown-group .
ns7:econsector
	rdf:type	ns9:BreakdownGroup , skos:Concept ;
	skos:prefLabel	"Economic sectors (17 Nace groups)" ;
	skos:notation	"econsector" ;
	skos:altLabel	"Economic sectors (17 Nace groups)" ;
	ns10:order	"40" ;
	skos:definition	"Breakdown by 17 economic sectors (Nace rev.2)" ;
	skos:topConceptOf	ns1:breakdown-group .
ns7:econsector_size
	rdf:type	ns9:BreakdownGroup , skos:Concept ;
	skos:prefLabel	"Economic sector and size (6 groups)" ;
	skos:notation	"econsector_size" ;
	skos:altLabel	"Economic sector and size (6 groups)" ;
	ns10:order	"41" ;
	skos:definition	"Breakdown by economic sector and size (6 groups)" ;
	skos:topConceptOf	ns1:breakdown-group .
ns7:egov_le
	rdf:type	ns9:BreakdownGroup , skos:Concept ;
	skos:prefLabel	"Life Events for eGovernment benchmarking" ;
	skos:notation	"egov_le" ;
	skos:altLabel	"Life Events for eGovernment benchmarking" ;
	ns10:order	"24" ;
	skos:definition	"Life Events constitute situations in which a citizen or business needs to interact with with Public Authorities. The eGovernment benchmarking defines a set of Life Events and assesses how well different countries perform in supporting all the necessary interactions between the citizen and the public administration when going through each of those Life Events." ;
	skos:topConceptOf	ns1:breakdown-group .
ns7:epsi_dimensions
	rdf:type	ns9:BreakdownGroup , skos:Concept ;
	skos:prefLabel	"PSI sub-dimensions" ;
	skos:notation	"epsi_dimensions" ;
	skos:altLabel	"PSI sub-dimensions" ;
	skos:topConceptOf	ns1:breakdown-group .
ns7:hhbyiq
	rdf:type	ns9:BreakdownGroup , skos:Concept ;
	rdfs:seeAlso	ns11:ind_type ;
	skos:prefLabel	"Household Income in quartiles" ;
	skos:notation	"hhbyiq" ;
	skos:altLabel	"Household Income in quartiles" ;
	ns10:order	"11" ;
	skos:definition	"breakdown by income quartile of the household: from 25% lowest to 25% highest among incomes observed (after grossing up)" ;
	skos:topConceptOf	ns1:breakdown-group .
ns7:hhbytype
	rdf:type	ns9:BreakdownGroup , skos:Concept ;
	skos:prefLabel	"Presence of dependent childrens" ;
	skos:notation	"hhbytype" ;
	skos:altLabel	"Dependent childrens" ;
	ns10:order	"14" ;
	skos:definition	"breakdown by presence of dependent childrens (under 16) in the household" ;
	skos:topConceptOf	ns1:breakdown-group .
ns7:infso_directorates
	rdf:type	ns9:BreakdownGroup , skos:Concept ;
	skos:prefLabel	"DG INFSO Directorates" ;
	skos:notation	"infso_directorates" ;
	skos:altLabel	"DG INFSO Directorates" ;
	skos:definition	"Organisation chart for the period 2007-2011" ;
	skos:topConceptOf	ns1:breakdown-group .
ns7:labour_force
	rdf:type	ns9:BreakdownGroup , skos:Concept ;
	skos:prefLabel	"Labour force" ;
	skos:notation	"labour_force" ;
	skos:altLabel	"Labour force" ;
	ns10:order	"26" ;
	skos:topConceptOf	ns1:breakdown-group .
ns7:manuf
	rdf:type	ns9:BreakdownGroup , skos:Concept ;
	skos:prefLabel	"Manufacturing sub-sectors" ;
	skos:notation	"manuf" ;
	skos:altLabel	"Manufacturing sub-sectors" ;
	skos:definition	"Manufacturing sector (NACE rev.2 group C) divided into 9 sub-sectors" ;
	skos:topConceptOf	ns1:breakdown-group .
ns7:mhz_bands
	rdf:type	ns9:BreakdownGroup , skos:Concept ;
	skos:prefLabel	"Spectrum Bands " ;
	skos:notation	"mhz_bands" ;
	skos:altLabel	"Spectrum Bands " ;
	skos:definition	"Spectrum assigned for wireless broadband in accordance to EU level harmonisation measures" ;
	skos:topConceptOf	ns1:breakdown-group .
ns7:others
	rdf:type	ns9:BreakdownGroup , skos:Concept ;
	skos:prefLabel	"others" ;
	skos:notation	"others" ;
	skos:altLabel	"others" ;
	ns10:order	"99" ;
	skos:definition	"Particular subgroups of cases (slices) which partially overlap with other complete groups of breakdown modalities." ;
	skos:topConceptOf	ns1:breakdown-group .
ns7:rural_pop
	rdf:type	ns9:BreakdownGroup , skos:Concept ;
	skos:prefLabel	"Rural population" ;
	skos:notation	"rural_pop" ;
	skos:altLabel	"Rural population" ;
	ns10:order	"23" ;
	skos:topConceptOf	ns1:breakdown-group .
ns7:sos_agg
	rdf:type	ns9:BreakdownGroup , skos:Concept ;
	rdfs:seeAlso	ns12:ict-research-projects-under-eus-seventh-framework-programme-fp7 ;
	skos:prefLabel	"Strategic Objectives Aggregated" ;
	skos:notation	"sos_agg" ;
	skos:altLabel	"Strategic Objectives (27)" ;
	skos:definition	"The research strategic objectives within FP7 ICT (Cooperation theme) are aggregated into 26 thematic research areas. In addition, there is one thematic area for projects funded under Capacities Programme for eInfrastructures" ;
	skos:topConceptOf	ns1:breakdown-group .
ns7:total
	rdf:type	ns9:BreakdownGroup , skos:Concept ;
	skos:prefLabel	"Total" ;
	skos:notation	"total" ;
	skos:altLabel	"Total" ;
	ns10:order	"1" ;
	skos:definition	"Total (no breakdown)" ;
	skos:topConceptOf	ns1:breakdown-group .
ns7:wid_score
	rdf:type	ns9:BreakdownGroup , skos:Concept ;
	skos:prefLabel	"Women in Digital score" ;
	skos:notation	"wid_score" ;
	skos:altLabel	"Women in digital score" ;
	ns10:order	"114" ;
	skos:topConceptOf	ns1:breakdown-group .
ns7:desi_1a_fbbtc
	rdf:type	ns9:BreakdownGroup , skos:Concept ;
	skos:prefLabel	"Indicators under 1a Fixed broadband take-up" ;
	skos:notation	"desi_1a_fbbtc" ;
	ns10:order	"8" ;
	skos:topConceptOf	ns1:breakdown-group .
ns7:desi_1b_fbbc
	rdf:type	ns9:BreakdownGroup , skos:Concept ;
	skos:prefLabel	"Indicators under 1b Fixed broadband coverage" ;
	skos:notation	"desi_1b_fbbc" ;
	ns10:order	"9" ;
	skos:topConceptOf	ns1:breakdown-group .
ns7:desi_1c_mbb
	rdf:type	ns9:BreakdownGroup , skos:Concept ;
	skos:prefLabel	"Indicators under 1c Mobile broadband" ;
	skos:notation	"desi_1c_mbb" ;
	ns10:order	"10" ;
	skos:topConceptOf	ns1:breakdown-group .
ns7:desi_1d_bbpi
	rdf:type	ns9:BreakdownGroup , skos:Concept ;
	skos:prefLabel	"Indicators under 1d Broadband price index" ;
	skos:notation	"desi_1d_bbpi" ;
	ns10:order	"11" ;
	skos:topConceptOf	ns1:breakdown-group .
ns7:childrenhh
	rdf:type	ns9:BreakdownGroup , skos:Concept ;
	skos:prefLabel	"Household with or without  children" ;
	skos:notation	"childrenhh" ;
	skos:altLabel	"Household with or without  children" ;
	ns10:order	"28" ;
	skos:definition	"Breakdown by Individuals living in the household with or without  children" ;
	skos:topConceptOf	ns1:breakdown-group .
ns7:ictproffession
	rdf:type	ns9:BreakdownGroup , skos:Concept ;
	skos:prefLabel	"ICT and non-ICT profession" ;
	skos:notation	"ictproffession" ;
	skos:altLabel	"ICT and non-ICT profession" ;
	ns10:order	"27" ;
	skos:definition	"Breakdown by ICT and non-ICT profession" ;
	skos:topConceptOf	ns1:breakdown-group .
ns7:workingscheme
	rdf:type	ns9:BreakdownGroup , skos:Concept ;
	skos:prefLabel	"Working patterns and conditions" ;
	skos:notation	"workingscheme" ;
	skos:altLabel	"Working patterns and conditions" ;
	ns10:order	"29" ;
	skos:definition	"Breakdown by Working patterns(full/ part time) and conditions (contract duration)" ;
	skos:topConceptOf	ns1:breakdown-group .
ns7:desi_3a_ui
	rdf:type	ns9:BreakdownGroup , skos:Concept ;
	skos:prefLabel	"Indicators under 3a Internet use" ;
	skos:notation	"desi_3a_ui" ;
	ns10:order	"15" ;
	skos:topConceptOf	ns1:breakdown-group .
ns7:desi_3b_acton
	rdf:type	ns9:BreakdownGroup , skos:Concept ;
	skos:prefLabel	"Indicators under 3b Activities online" ;
	skos:notation	"desi_3b_acton" ;
	ns10:order	"16" ;
	skos:topConceptOf	ns1:breakdown-group .
