@prefix rdf:	<http://www.w3.org/1999/02/22-rdf-syntax-ns#> .
@prefix ns1:	<http://semantic.digital-agenda-data.eu/codelist/> .
@prefix ns2:	<http://purl.org/linked-data/sdmx#> .
ns1:indicator	rdf:type	ns2:CodeList .
@prefix skos:	<http://www.w3.org/2004/02/skos/core#> .
ns1:indicator	rdf:type	skos:ConceptScheme .
@prefix xsd:	<http://www.w3.org/2001/XMLSchema#> .
@prefix dct:	<http://purl.org/dc/terms/> .
ns1:indicator	dct:modified	"2021-11-12T10:34:12"^^xsd:dateTime .
@prefix rdfs:	<http://www.w3.org/2000/01/rdf-schema#> .
ns1:indicator	rdfs:isDefinedBy	<http://digital-agenda-data.eu/> ;
	skos:prefLabel	"Code list for indicators used by Digital Agenda Scoreboard" ;
	skos:notation	"CL_INDICATOR" .
@prefix ns7:	<http://semantic.digital-agenda-data.eu/codelist/indicator/> .
ns1:indicator	skos:hasTopConcept	ns7:e_gov_dpsc ,
		ns7:e_gov_od ,
		ns7:old_i_dsk_i_b ,
		ns7:old_i_dsk_ps_b ,
		ns7:old_i_dsk_s_b ,
		ns7:old_digskillindex ,
		ns7:old_digskillindex_basicandabove ,
		ns7:old_i_dsk_b ,
		ns7:old_i_dsk_c_b ,
		ns7:old_wid_ui_ps ,
		ns7:desi_dps_prefform ,
		ns7:desi_dps_pscit ,
		ns7:desi_idt_smedi ,
		ns7:e_gov_4c_cb_eid ,
		ns7:e_gov_4d_cb_edoc ,
		ns7:mbb_5gcov ,
		ns7:mbb_r5gcov ,
		ns7:e_gov_3_ke ,
		ns7:e_gov_3a_ke_eid ,
		ns7:e_gov_3b_ke_edoc ,
		ns7:e_gov_3c_ke_as ,
		ns7:e_gov_3d_ke_dp ,
		ns7:e_gov_4_cb ,
		ns7:e_gov_4a_cb_oa ,
		ns7:e_gov_4b_cb_us ,
		ns7:e_gov_1a_uc_oa ,
		ns7:e_gov_1b_uc_mf ,
		ns7:e_gov_1c_uc_us ,
		ns7:e_gov_2_tr ,
		ns7:e_gov_2a_tr_sd ,
		ns7:e_gov_2c_tr_pd ,
		ns7:e_gov_2c_tr_sd ,
		ns7:e_gov_2x_tr_po ,
		<http://semantic.digital-agenda-data.eu/codelist/indicator/5g_read> ,
		ns7:bb_rvhcncov ,
		ns7:bb_vhcncov ,
		ns7:e_gov_1_uc ,
		ns7:i_dsk_ps_ab ,
		ns7:i_dsk_s_ab ,
		ns7:i_dsk_l ,
		ns7:e_gov_ebus ,
		ns7:h_fbbfix ,
		ns7:h_ubbfix ,
		ns7:i_dsk_x ,
		ns7:i_dsk_c_x ,
		ns7:i_dsk_s_x ,
		ns7:i_dsk_c_ab ,
		ns7:e_gov_4b_bm_us ,
		ns7:wid_ui_ib ,
		ns7:wid_ui_iu ,
		ns7:wid_ui_nui ,
		ns7:wid_ui_oc ,
		ns7:wid_ui_part ,
		ns7:wid_ius_ss ,
		ns7:wid_score ,
		ns7:wid_sse ,
		ns7:wid_sse_gpg ,
		ns7:wid_sse_icts ,
		ns7:wid_sse_stem ,
		ns7:wid_ui ,
		ns7:wid_ui_egov ,
		ns7:transparent_egov ,
		ns7:ttg_in_scope ,
		ns7:user_centric_egov ,
		ns7:val_add_ict ,
		ns7:vod ,
		ns7:wid_ius ,
		ns7:wid_ius_abs ,
		ns7:wid_ius_bs ,
		ns7:price_internet_fixed_tel_tv ,
		ns7:price_internet_only ,
		ns7:spectrum_wbb ,
		ns7:st_grad ,
		ns7:tel_ftr ,
		ns7:tel_inv ,
		ns7:tel_llu ,
		ns7:tel_rev ,
		ns7:mob_roam ,
		ns7:mob_subs ,
		ns7:p_empmd ,
		ns7:p_iuse ,
		ns7:pay_on_time_projects ,
		ns7:pop ,
		ns7:population ,
		ns7:price_internet_fixed_tel ,
		ns7:mbb_penet ,
		ns7:mbb_rhspacov ,
		ns7:mbb_rltecov ,
		ns7:mob_arpm ,
		ns7:mob_arpu ,
		ns7:mob_ms ,
		ns7:mob_mtr ,
		ns7:mob_penet ,
		ns7:ict_hgc ,
		ns7:ict_imp ,
		ns7:ict_spec3_broad ,
		ns7:ict_specialists ,
		ns7:labour_prod_ict ,
		ns7:mbb_3gcov ,
		ns7:mbb_hspacov ,
		ns7:mbb_ltecov ,
		ns7:i_dsk_i_ab ,
		ns7:i_dsk_ab ,
		ns7:i_dsk_i_x ,
		ns7:i_dsk_ps_x ,
		ns7:desi_sliders ,
		ns7:c1_datatraffic ,
		ns7:desi ,
		ns7:e_gov_ke ,
		ns7:e_gov_opa ,
		ns7:e_gov_osc ,
		ns7:e_gov_pff ,
		ns7:e_igov ,
		ns7:e_igov2pr ,
		ns7:e_igovrt ,
		ns7:e_gov_5_ke ,
		ns7:e_gov_5a_ke_eid ,
		ns7:e_gov_5b_ke_edoc ,
		ns7:e_gov_5c_ke_as ,
		ns7:e_gov_5d_ke_dp ,
		ns7:e_gov_5e_ke_esafe ,
		ns7:e_gov_5f_ke_sso ,
		ns7:e_gov_3e_cm_eu ,
		ns7:e_gov_3f_cm_su ,
		ns7:e_gov_4_bm ,
		ns7:e_gov_4a_bm_oa ,
		ns7:e_gov_4c_bm_eidcb ,
		ns7:e_gov_4d_bm_edoccb ,
		ns7:e_gov_4e_bm_eu ,
		ns7:e_gov_4f_bm_su ,
		ns7:e_gov_2a_tg_sd ,
		ns7:e_gov_2b_tg_po ,
		ns7:e_gov_2c_tg_pd ,
		ns7:e_gov_3_cm ,
		ns7:e_gov_3a_cm_oa ,
		ns7:e_gov_3b_cm_us ,
		ns7:e_gov_3c_cm_eidcb ,
		ns7:e_gov_3d_cm_edoccb ,
		ns7:e_eturn ,
		ns7:e_gov_1_ucg ,
		ns7:e_gov_1a_ucg_oa ,
		ns7:e_gov_1b_ucg_us ,
		ns7:e_gov_1c_ucg_mf ,
		ns7:e_gov_1d_ucg_eu ,
		ns7:e_gov_1e_ucg_su ,
		ns7:e_gov_2_tg ,
		ns7:e_cc_pcpu ,
		ns7:e_crman ,
		ns7:e_di_hivhi ,
		ns7:e_di_vlo ,
		ns7:e_ebuy ,
		ns7:e_empmd_gt20 ,
		ns7:e_erp1 ,
		ns7:e_esell ,
		ns7:e_aws_cown ,
		ns7:e_aws_gt1_b2c_gt10ws ,
		ns7:e_awsval_cmp ,
		ns7:e_awsval_cown ,
		ns7:e_bd ,
		ns7:e_broad ,
		ns7:e_cc ,
		ns7:e_cc_ge_me ,
		ns7:e_ade ,
		ns7:e_ads ,
		ns7:e_ads_loc ,
		ns7:e_ads_trk ,
		ns7:e_aeseu ,
		ns7:e_aws ,
		ns7:e_aws_cmp ,
		ns7:h2020_totcost ,
		ns7:h2020ict_afxp ,
		ns7:h_bbfix ,
		ns7:h_broad ,
		ns7:h_iacc ,
		ns7:h_xcost ,
		ns7:hie_use_ex_admin ,
		ns7:hie_use_pharm ,
		ns7:gbaord ,
		ns7:gbaord_ict ,
		ns7:gdp ,
		ns7:h2020_cofin ,
		ns7:h2020_ec_funding ,
		ns7:h2020_newentry ,
		ns7:h2020_organisations ,
		ns7:h2020_particip ,
		ns7:fp7ict_ec_funding_prc ,
		ns7:fp7ict_ec_funding_smes ,
		ns7:fp7ict_newentry ,
		ns7:fp7ict_organisations ,
		ns7:fp7ict_particip ,
		ns7:fp7ict_particip_prc ,
		ns7:fp7ict_particip_smes ,
		ns7:fp7ict_totcost ,
		ns7:foa_cit ,
		ns7:foa_ent ,
		ns7:fp7_ict_artic ,
		ns7:fp7_ict_pat ,
		ns7:fp7_ict_pub ,
		ns7:fp7ict_afxp ,
		ns7:fp7ict_cofin ,
		ns7:fp7ict_ec_funding ,
		ns7:edigint2015 ,
		ns7:employment_ict ,
		ns7:eoa_nn_films ,
		ns7:eoa_tvchannels_tarfor ,
		ns7:eoa_vod_estab_otheu ,
		ns7:epsi_score ,
		ns7:eun_computers ,
		ns7:eun_web ,
		ns7:e_sisc ,
		ns7:e_sisorp ,
		ns7:e_sm_any ,
		ns7:e_sm_ge2 ,
		ns7:e_web ,
		ns7:e_webf2 ,
		ns7:e_wsel25 ,
		ns7:e_wsel50 ,
		ns7:e_itt2 ,
		ns7:e_pmd ,
		ns7:e_pmd_app ,
		ns7:e_ra ,
		ns7:e_rfac ,
		ns7:e_rfid ,
		ns7:e_rfpsas ,
		ns7:e_secpol1 ,
		ns7:e_inv ,
		ns7:e_invsnd ,
		ns7:e_ispdf_ge30 ,
		ns7:e_ispdfokx ,
		ns7:e_ispdfokx_ge100 ,
		ns7:e_it_mext ,
		ns7:e_itsp2 ,
		ns7:e_itspvac2 ,
		ns7:i_piacadv ,
		ns7:i_sbgood ,
		ns7:i_secfl ,
		ns7:i_secpif1 ,
		ns7:i_secvir1 ,
		ns7:i_skedu ,
		ns7:ict_commit_in_trp ,
		ns7:ict_exp ,
		ns7:i_iuph1 ,
		ns7:i_iuse ,
		ns7:i_iusell ,
		ns7:i_iusnet ,
		ns7:i_iuupl ,
		ns7:i_iuvod ,
		ns7:i_iuvote ,
		ns7:i_iux ,
		ns7:i_iugov ,
		ns7:i_iugov12 ,
		ns7:i_iuif ,
		ns7:i_iujob ,
		ns7:i_iumapp ,
		ns7:i_iumc ,
		ns7:i_iunw ,
		ns7:i_iuolc ,
		ns7:i_ihif ,
		ns7:i_ilt12 ,
		ns7:i_isk_ge_me ,
		ns7:i_iu3 ,
		ns7:i_iu3g ,
		ns7:i_iubk ,
		ns7:i_iueduif ,
		ns7:i_iugm ,
		ns7:i_dsk_c_bab ,
		ns7:i_dsk_i_bab ,
		ns7:i_dsk_ps_bab ,
		ns7:i_dsk_s_bab ,
		ns7:i_ia12ave ,
		ns7:i_iday ,
		ns7:i_igov12rt ,
		ns7:i_igovrt ,
		ns7:i_cc ,
		ns7:i_cisk_sfjob ,
		ns7:i_cisk_sfjobx ,
		ns7:i_cook ,
		ns7:i_cprg ,
		ns7:i_csk_ge_me ,
		ns7:i_cweb ,
		ns7:i_dsk_bab ,
		ns7:i_atsw ,
		ns7:i_barr1x ,
		ns7:i_bfeu ,
		ns7:i_bgood ,
		ns7:i_bgoodo ,
		ns7:i_blt12 ,
		ns7:i_bpgood ,
		ns7:i_bserv ,
		ns7:househ ,
		ns7:households ,
		ns7:desi_hc_entict ,
		ns7:desi_hc_fictspec ,
		ns7:desi_hc_ictg ,
		ns7:desi_hc_ictspec ,
		ns7:desi_idt ,
		ns7:desi_idt_ai ,
		ns7:desi_idt_bigdat ,
		ns7:desi_idt_cloud ,
		ns7:desi_fbbtc ,
		ns7:desi_gbpstc ,
		ns7:desi_hc ,
		ns7:desi_hc_abds ,
		ns7:desi_hc_abss ,
		ns7:desi_hc_asd ,
		ns7:desi_hc_bds ,
		ns7:desi_hc_bsu ,
		ns7:desi_c_mbb ,
		ns7:desi_conn ,
		ns7:desi_dps ,
		ns7:desi_dps_egov ,
		ns7:desi_dps_egovuser ,
		ns7:desi_dps_opendata ,
		ns7:desi_dps_psbiz ,
		ns7:desi_fbbc ,
		ns7:desi_4g ,
		ns7:desi_5g ,
		ns7:desi_5gc ,
		ns7:desi_bbpi ,
		ns7:desi_c_bbpi ,
		ns7:desi_c_fbbc ,
		ns7:desi_c_fbbtc ,
		ns7:desi_idt_smeso ,
		ns7:desi_idt_socmed ,
		ns7:desi_mbbtu ,
		ns7:desi_total ,
		ns7:desi_ufbbtu ,
		ns7:desi_vhcnc ,
		ns7:desi_idt_di ,
		ns7:desi_idt_dtb ,
		ns7:desi_idt_ecomm ,
		ns7:desi_idt_ecomturn ,
		ns7:desi_idt_einv ,
		ns7:desi_idt_eis ,
		ns7:desi_idt_ictsust ,
		ns7:desi_idt_sellcb ,
		ns7:bb_speed100 ,
		ns7:bb_speed2 ,
		ns7:bb_speed30 ,
		ns7:bb_srcov ,
		ns7:bs_rd_expen_ict ,
		ns7:c1_bandwidth ,
		ns7:c1_compcyclesegi ,
		ns7:c1_compcyclesprace ,
		ns7:bb_lines ,
		ns7:bb_ne ,
		ns7:bb_ngacov ,
		ns7:bb_penet ,
		ns7:bb_rfttpcov ,
		ns7:bb_rngacov ,
		ns7:bb_scov ,
		ns7:bb_speed10 ,
		ns7:aaaa_cov ,
		ns7:actspeed ,
		ns7:afford_internet_only_minppp ,
		ns7:avg_ttg ,
		ns7:bb_dsl ,
		ns7:bb_fcov ,
		ns7:bb_fttpcov ,
		ns7:bb_hhi .
@prefix ns8:	<http://semantic.digital-agenda-data.eu/def/> .
ns1:indicator	skos:inScheme	ns8:scheme .
@prefix ns9:	<http://semantic.digital-agenda-data.eu/codelist/indicator-group/audiovisual/> .
@prefix ns10:	<http://semantic.digital-agenda-data.eu/def/class/> .
ns9:eoa_nn_films	rdf:type	ns10:IndicatorToGroupMembership ;
	rdfs:label	"audiovisual" .
@prefix ns11:	<http://semantic.digital-agenda-data.eu/def/property/> .
@prefix ns12:	<http://semantic.digital-agenda-data.eu/codelist/indicator-group/> .
ns9:eoa_nn_films	ns11:member-of	ns12:audiovisual ;
	ns11:order	"3" .
ns9:eoa_tvchannels_tarfor	rdf:type	ns10:IndicatorToGroupMembership ;
	rdfs:label	"audiovisual" ;
	ns11:member-of	ns12:audiovisual ;
	ns11:order	"1" .
ns9:eoa_vod_estab_otheu	rdf:type	ns10:IndicatorToGroupMembership ;
	rdfs:label	"audiovisual" ;
	ns11:member-of	ns12:audiovisual ;
	ns11:order	"2" .
ns9:i_iugm	rdf:type	ns10:IndicatorToGroupMembership ;
	rdfs:label	"audiovisual" ;
	ns11:member-of	ns12:audiovisual ;
	ns11:order	"6" .
ns9:i_iunw	rdf:type	ns10:IndicatorToGroupMembership ;
	rdfs:label	"audiovisual" ;
	ns11:member-of	ns12:audiovisual ;
	ns11:order	"5" .
ns9:i_iuvod	rdf:type	ns10:IndicatorToGroupMembership ;
	rdfs:label	"audiovisual" ;
	ns11:member-of	ns12:audiovisual ;
	ns11:order	"12" .
ns9:vod	rdf:type	ns10:IndicatorToGroupMembership ;
	rdfs:label	"audiovisual" ;
	ns11:member-of	ns12:audiovisual ;
	ns11:order	"11" .
@prefix ns13:	<http://semantic.digital-agenda-data.eu/codelist/indicator-group/back/> .
ns13:gdp	rdf:type	ns10:IndicatorToGroupMembership ;
	rdfs:label	"back" ;
	ns11:member-of	ns12:back ;
	ns11:order	"4" .
ns13:househ	rdf:type	ns10:IndicatorToGroupMembership ;
	rdfs:label	"back" ;
	ns11:member-of	ns12:back ;
	ns11:order	"1" .
ns13:households	rdf:type	ns10:IndicatorToGroupMembership ;
	rdfs:label	"back" ;
	ns11:member-of	ns12:back ;
	ns11:order	"5" .
ns13:pop	rdf:type	ns10:IndicatorToGroupMembership ;
	rdfs:label	"back" ;
	ns11:member-of	ns12:back ;
	ns11:order	"2" .
ns13:population	rdf:type	ns10:IndicatorToGroupMembership ;
	rdfs:label	"back" ;
	ns11:member-of	ns12:back ;
	ns11:order	"3" .
@prefix ns14:	<http://semantic.digital-agenda-data.eu/codelist/indicator-group/bbquality/> .
ns14:actspeed	rdf:type	ns10:IndicatorToGroupMembership ;
	rdfs:label	"bbquality" ;
	ns11:member-of	ns12:bbquality ;
	ns11:order	"5" .
ns14:afford_internet_only_minppp	rdf:type	ns10:IndicatorToGroupMembership ;
	rdfs:label	"bbquality" ;
	ns11:member-of	ns12:bbquality ;
	ns11:order	"9" .
ns14:bb_speed10	rdf:type	ns10:IndicatorToGroupMembership ;
	rdfs:label	"bbquality" ;
	ns11:member-of	ns12:bbquality ;
	ns11:order	"2" .
ns14:bb_speed100	rdf:type	ns10:IndicatorToGroupMembership ;
	rdfs:label	"bbquality" ;
	ns11:member-of	ns12:bbquality ;
	ns11:order	"4" .
ns14:bb_speed2	rdf:type	ns10:IndicatorToGroupMembership ;
	rdfs:label	"bbquality" ;
	ns11:member-of	ns12:bbquality ;
	ns11:order	"1" .
ns14:bb_speed30	rdf:type	ns10:IndicatorToGroupMembership ;
	rdfs:label	"bbquality" ;
	ns11:member-of	ns12:bbquality ;
	ns11:order	"3" .
ns14:h_xcost	rdf:type	ns10:IndicatorToGroupMembership ;
	rdfs:label	"bbquality" ;
	ns11:member-of	ns12:bbquality ;
	ns11:order	"10" .
ns14:price_internet_fixed_tel	rdf:type	ns10:IndicatorToGroupMembership ;
	rdfs:label	"bbquality" ;
	ns11:member-of	ns12:bbquality ;
	ns11:order	"7" .
ns14:price_internet_fixed_tel_tv	rdf:type	ns10:IndicatorToGroupMembership ;
	rdfs:label	"bbquality" ;
	ns11:member-of	ns12:bbquality ;
	ns11:order	"8" .
ns14:price_internet_only	rdf:type	ns10:IndicatorToGroupMembership ;
	rdfs:label	"bbquality" ;
	ns11:member-of	ns12:bbquality ;
	ns11:order	"6" .
@prefix ns15:	<http://semantic.digital-agenda-data.eu/codelist/indicator-group/broadband/> .
ns15:bb_dsl	rdf:type	ns10:IndicatorToGroupMembership ;
	rdfs:label	"broadband" ;
	ns11:member-of	ns12:broadband ;
	ns11:order	"17" .
ns15:bb_fttpcov	rdf:type	ns10:IndicatorToGroupMembership ;
	rdfs:label	"broadband" ;
	ns11:member-of	ns12:broadband ;
	ns11:order	"7" .
ns15:bb_hhi	rdf:type	ns10:IndicatorToGroupMembership ;
	rdfs:label	"broadband" ;
	ns11:member-of	ns12:broadband .
ns15:bb_lines	rdf:type	ns10:IndicatorToGroupMembership ;
	rdfs:label	"broadband" ;
	ns11:member-of	ns12:broadband ;
	ns11:order	"16" .
ns15:bb_ne	rdf:type	ns10:IndicatorToGroupMembership ;
	rdfs:label	"broadband" ;
	ns11:member-of	ns12:broadband ;
	ns11:order	"18" .
ns15:bb_ngacov	rdf:type	ns10:IndicatorToGroupMembership ;
	rdfs:label	"broadband" ;
	ns11:member-of	ns12:broadband ;
	ns11:order	"3" .
ns15:bb_penet	rdf:type	ns10:IndicatorToGroupMembership ;
	rdfs:label	"broadband" ;
	ns11:member-of	ns12:broadband ;
	ns11:order	"15" .
ns15:bb_rfttpcov	rdf:type	ns10:IndicatorToGroupMembership ;
	rdfs:label	"broadband" ;
	ns11:member-of	ns12:broadband ;
	ns11:order	"8" .
ns15:bb_rngacov	rdf:type	ns10:IndicatorToGroupMembership ;
	rdfs:label	"broadband" ;
	ns11:member-of	ns12:broadband ;
	ns11:order	"4" .
ns15:bb_scov	rdf:type	ns10:IndicatorToGroupMembership ;
	rdfs:label	"broadband" ;
	ns11:member-of	ns12:broadband ;
	ns11:order	"5" .
ns15:bb_srcov	rdf:type	ns10:IndicatorToGroupMembership ;
	rdfs:label	"broadband" ;
	ns11:member-of	ns12:broadband ;
	ns11:order	"6" .
ns15:e_broad	rdf:type	ns10:IndicatorToGroupMembership ;
	rdfs:label	"broadband" ;
	ns11:member-of	ns12:broadband ;
	ns11:order	"13" .
ns15:e_ispdf_ge30	rdf:type	ns10:IndicatorToGroupMembership ;
	rdfs:label	"broadband" ;
	ns11:member-of	ns12:broadband ;
	ns11:order	"14" .
ns15:e_ispdfokx	rdf:type	ns10:IndicatorToGroupMembership ;
	rdfs:label	"broadband" ;
	ns11:member-of	ns12:broadband ;
	ns11:order	"19" .
ns15:e_ispdfokx_ge100	rdf:type	ns10:IndicatorToGroupMembership ;
	rdfs:label	"broadband" ;
	ns11:member-of	ns12:broadband ;
	ns11:order	"20" .
ns15:h_bbfix	rdf:type	ns10:IndicatorToGroupMembership ;
	rdfs:label	"broadband" ;
	ns11:member-of	ns12:broadband ;
	ns11:order	"10" .
ns15:h_broad	rdf:type	ns10:IndicatorToGroupMembership ;
	rdfs:label	"broadband" ;
	ns11:member-of	ns12:broadband ;
	ns11:order	"9" .
@prefix ns16:	<http://semantic.digital-agenda-data.eu/codelist/indicator-group/desi/> .
ns16:desi	rdf:type	ns10:IndicatorToGroupMembership ;
	rdfs:label	"desi" ;
	ns11:member-of	ns12:desi ;
	ns11:order	"2" .
@prefix ns17:	<http://semantic.digital-agenda-data.eu/codelist/indicator-group/desi_sliders/> .
ns17:desi_sliders	rdf:type	ns10:IndicatorToGroupMembership ;
	rdfs:label	"desi_sliders" ;
	ns11:member-of	ns12:desi_sliders ;
	ns11:order	"1" .
@prefix ns18:	<http://semantic.digital-agenda-data.eu/codelist/indicator-group/discontinued/> .
ns18:bb_fcov	rdf:type	ns10:IndicatorToGroupMembership ;
	rdfs:label	"discontinued" ;
	ns11:member-of	ns12:discontinued ;
	ns11:order	"16" .
ns18:e_ade	rdf:type	ns10:IndicatorToGroupMembership ;
	rdfs:label	"discontinued" ;
	ns11:member-of	ns12:discontinued ;
	ns11:order	"3" .
ns18:e_ebuy	rdf:type	ns10:IndicatorToGroupMembership ;
	rdfs:label	"discontinued" ;
	ns11:member-of	ns12:discontinued ;
	ns11:order	"5" .
ns18:e_igov	rdf:type	ns10:IndicatorToGroupMembership ;
	rdfs:label	"discontinued" ;
	ns11:member-of	ns12:discontinued ;
	ns11:order	"25" .
ns18:e_igov2pr	rdf:type	ns10:IndicatorToGroupMembership ;
	rdfs:label	"discontinued" ;
	ns11:member-of	ns12:discontinued ;
	ns11:order	"27" .
ns18:e_igovrt	rdf:type	ns10:IndicatorToGroupMembership ;
	rdfs:label	"discontinued" ;
	ns11:member-of	ns12:discontinued ;
	ns11:order	"26" .
ns18:e_inv	rdf:type	ns10:IndicatorToGroupMembership ;
	rdfs:label	"discontinued" ;
	ns11:member-of	ns12:discontinued ;
	ns11:order	"4" .
ns18:e_sisorp	rdf:type	ns10:IndicatorToGroupMembership ;
	rdfs:label	"discontinued" ;
	ns11:member-of	ns12:discontinued ;
	ns11:order	"2" .
ns18:foa_cit	rdf:type	ns10:IndicatorToGroupMembership ;
	rdfs:label	"discontinued" ;
	ns11:member-of	ns12:discontinued ;
	ns11:order	"19" .
ns18:foa_ent	rdf:type	ns10:IndicatorToGroupMembership ;
	rdfs:label	"discontinued" ;
	ns11:member-of	ns12:discontinued ;
	ns11:order	"20" .
ns18:i_cisk_sfjob	rdf:type	ns10:IndicatorToGroupMembership ;
	rdfs:label	"discontinued" ;
	ns11:member-of	ns12:discontinued ;
	ns11:order	"12" .
ns18:i_csk_ge_me	rdf:type	ns10:IndicatorToGroupMembership ;
	rdfs:label	"discontinued" ;
	ns11:member-of	ns12:discontinued ;
	ns11:order	"10" .
ns18:i_cweb	rdf:type	ns10:IndicatorToGroupMembership ;
	rdfs:label	"discontinued" ;
	ns11:member-of	ns12:discontinued ;
	ns11:order	"9" .
ns18:i_igovrt	rdf:type	ns10:IndicatorToGroupMembership ;
	rdfs:label	"discontinued" ;
	ns11:member-of	ns12:discontinued ;
	ns11:order	"24" .
ns18:i_isk_ge_me	rdf:type	ns10:IndicatorToGroupMembership ;
	rdfs:label	"discontinued" ;
	ns11:member-of	ns12:discontinued ;
	ns11:order	"11" .
ns18:i_iugov	rdf:type	ns10:IndicatorToGroupMembership ;
	rdfs:label	"discontinued" ;
	ns11:member-of	ns12:discontinued ;
	ns11:order	"23" .
ns18:ict_specialists	rdf:type	ns10:IndicatorToGroupMembership ;
	rdfs:label	"discontinued" ;
	ns11:member-of	ns12:discontinued ;
	ns11:order	"15" .
ns18:mbb_3gcov	rdf:type	ns10:IndicatorToGroupMembership ;
	rdfs:label	"discontinued" ;
	ns11:member-of	ns12:discontinued ;
	ns11:order	"17" .
ns18:mob_arpm	rdf:type	ns10:IndicatorToGroupMembership ;
	rdfs:label	"discontinued" ;
	ns11:member-of	ns12:discontinued ;
	ns11:order	"18" .
ns18:transparent_egov	rdf:type	ns10:IndicatorToGroupMembership ;
	rdfs:label	"discontinued" ;
	ns11:member-of	ns12:discontinued ;
	ns11:order	"22" .
ns18:user_centric_egov	rdf:type	ns10:IndicatorToGroupMembership ;
	rdfs:label	"discontinued" ;
	ns11:member-of	ns12:discontinued ;
	ns11:order	"21" .
@prefix ns19:	<http://semantic.digital-agenda-data.eu/codelist/indicator-group/ebusiness/> .
ns19:e_ads	rdf:type	ns10:IndicatorToGroupMembership ;
	rdfs:label	"ebusiness" ;
	ns11:member-of	ns12:ebusiness ;
	ns11:order	"15" .
ns19:e_bd	rdf:type	ns10:IndicatorToGroupMembership ;
	rdfs:label	"ebusiness" ;
	ns11:member-of	ns12:ebusiness ;
	ns11:order	"30" .
ns19:e_cc	rdf:type	ns10:IndicatorToGroupMembership ;
	rdfs:label	"ebusiness" ;
	ns11:member-of	ns12:ebusiness ;
	ns11:order	"27" .
ns19:e_cc_ge_me	rdf:type	ns10:IndicatorToGroupMembership ;
	rdfs:label	"ebusiness" ;
	ns11:member-of	ns12:ebusiness ;
	ns11:order	"28" .
ns19:e_cc_pcpu	rdf:type	ns10:IndicatorToGroupMembership ;
	rdfs:label	"ebusiness" ;
	ns11:member-of	ns12:ebusiness ;
	ns11:order	"29" .
ns19:e_crman	rdf:type	ns10:IndicatorToGroupMembership ;
	rdfs:label	"ebusiness" ;
	ns11:member-of	ns12:ebusiness ;
	ns11:order	"3" .
ns19:e_di_hivhi	rdf:type	ns10:IndicatorToGroupMembership ;
	rdfs:label	"ebusiness" ;
	ns11:member-of	ns12:ebusiness ;
	ns11:order	"16" .
ns19:e_di_vlo	rdf:type	ns10:IndicatorToGroupMembership ;
	rdfs:label	"ebusiness" ;
	ns11:member-of	ns12:ebusiness ;
	ns11:order	"17" .
ns19:e_empmd_gt20	rdf:type	ns10:IndicatorToGroupMembership ;
	rdfs:label	"ebusiness" ;
	ns11:member-of	ns12:ebusiness ;
	ns11:order	"12" .
ns19:e_erp1	rdf:type	ns10:IndicatorToGroupMembership ;
	rdfs:label	"ebusiness" ;
	ns11:member-of	ns12:ebusiness ;
	ns11:order	"2" .
ns19:e_invsnd	rdf:type	ns10:IndicatorToGroupMembership ;
	rdfs:label	"ebusiness" ;
	ns11:member-of	ns12:ebusiness ;
	ns11:order	"8" .
ns19:e_pmd_app	rdf:type	ns10:IndicatorToGroupMembership ;
	rdfs:label	"ebusiness" ;
	ns11:member-of	ns12:ebusiness ;
	ns11:order	"14" .
ns19:e_ra	rdf:type	ns10:IndicatorToGroupMembership ;
	rdfs:label	"ebusiness" ;
	ns11:member-of	ns12:ebusiness ;
	ns11:order	"11" .
ns19:e_rfac	rdf:type	ns10:IndicatorToGroupMembership ;
	rdfs:label	"ebusiness" ;
	ns11:member-of	ns12:ebusiness ;
	ns11:order	"21" .
ns19:e_rfid	rdf:type	ns10:IndicatorToGroupMembership ;
	rdfs:label	"ebusiness" ;
	ns11:member-of	ns12:ebusiness ;
	ns11:order	"20" .
ns19:e_rfpsas	rdf:type	ns10:IndicatorToGroupMembership ;
	rdfs:label	"ebusiness" ;
	ns11:member-of	ns12:ebusiness ;
	ns11:order	"22" .
ns19:e_sisc	rdf:type	ns10:IndicatorToGroupMembership ;
	rdfs:label	"ebusiness" ;
	ns11:member-of	ns12:ebusiness ;
	ns11:order	"7" .
ns19:e_sm_any	rdf:type	ns10:IndicatorToGroupMembership ;
	rdfs:label	"ebusiness" ;
	ns11:member-of	ns12:ebusiness ;
	ns11:order	"25" .
ns19:e_sm_ge2	rdf:type	ns10:IndicatorToGroupMembership ;
	rdfs:label	"ebusiness" ;
	ns11:member-of	ns12:ebusiness ;
	ns11:order	"26" .
ns19:e_web	rdf:type	ns10:IndicatorToGroupMembership ;
	rdfs:label	"ebusiness" ;
	ns11:member-of	ns12:ebusiness ;
	ns11:order	"9" .
ns19:e_webf2	rdf:type	ns10:IndicatorToGroupMembership ;
	rdfs:label	"ebusiness" ;
	ns11:member-of	ns12:ebusiness ;
	ns11:order	"10" .
ns19:edigint2015	rdf:type	ns10:IndicatorToGroupMembership ;
	rdfs:label	"ebusiness" ;
	ns11:member-of	ns12:ebusiness ;
	ns11:order	"18" .
ns19:p_empmd	rdf:type	ns10:IndicatorToGroupMembership ;
	rdfs:label	"ebusiness" ;
	ns11:member-of	ns12:ebusiness ;
	ns11:order	"13" .
@prefix ns20:	<http://semantic.digital-agenda-data.eu/codelist/indicator-group/ecommerce/> .
ns20:e_aeseu	rdf:type	ns10:IndicatorToGroupMembership ;
	rdfs:label	"ecommerce" ;
	ns11:member-of	ns12:ecommerce ;
	ns11:order	"12" .
ns20:e_aws	rdf:type	ns10:IndicatorToGroupMembership ;
	rdfs:label	"ecommerce" ;
	ns11:member-of	ns12:ecommerce .
ns20:e_aws_cmp	rdf:type	ns10:IndicatorToGroupMembership ;
	rdfs:label	"ecommerce" ;
	ns11:member-of	ns12:ecommerce .
ns20:e_aws_cown	rdf:type	ns10:IndicatorToGroupMembership ;
	rdfs:label	"ecommerce" ;
	ns11:member-of	ns12:ecommerce .
ns20:e_aws_gt1_b2c_gt10ws	rdf:type	ns10:IndicatorToGroupMembership ;
	rdfs:label	"ecommerce" ;
	ns11:member-of	ns12:ecommerce ;
	ns11:order	"13" .
ns20:e_awsval_cmp	rdf:type	ns10:IndicatorToGroupMembership ;
	rdfs:label	"ecommerce" ;
	ns11:member-of	ns12:ecommerce .
ns20:e_awsval_cown	rdf:type	ns10:IndicatorToGroupMembership ;
	rdfs:label	"ecommerce" ;
	ns11:member-of	ns12:ecommerce .
ns20:e_esell	rdf:type	ns10:IndicatorToGroupMembership ;
	rdfs:label	"ecommerce" ;
	ns11:member-of	ns12:ecommerce ;
	ns11:order	"10" .
ns20:e_eturn	rdf:type	ns10:IndicatorToGroupMembership ;
	rdfs:label	"ecommerce" ;
	ns11:member-of	ns12:ecommerce ;
	ns11:order	"11" .
ns20:e_wsel25	rdf:type	ns10:IndicatorToGroupMembership ;
	rdfs:label	"ecommerce" ;
	ns11:member-of	ns12:ecommerce .
ns20:e_wsel50	rdf:type	ns10:IndicatorToGroupMembership ;
	rdfs:label	"ecommerce" ;
	ns11:member-of	ns12:ecommerce .
ns20:i_barr1x	rdf:type	ns10:IndicatorToGroupMembership ;
	rdfs:label	"ecommerce" ;
	ns11:member-of	ns12:ecommerce ;
	ns11:order	"9" .
ns20:i_bfeu	rdf:type	ns10:IndicatorToGroupMembership ;
	rdfs:label	"ecommerce" ;
	ns11:member-of	ns12:ecommerce ;
	ns11:order	"3" .
ns20:i_bgood	rdf:type	ns10:IndicatorToGroupMembership ;
	rdfs:label	"ecommerce" ;
	ns11:member-of	ns12:ecommerce ;
	ns11:order	"7" .
ns20:i_bgoodo	rdf:type	ns10:IndicatorToGroupMembership ;
	rdfs:label	"ecommerce" ;
	ns11:member-of	ns12:ecommerce ;
	ns11:order	"6" .
ns20:i_blt12	rdf:type	ns10:IndicatorToGroupMembership ;
	rdfs:label	"ecommerce" ;
	ns11:member-of	ns12:ecommerce ;
	ns11:order	"1" .
ns20:i_bpgood	rdf:type	ns10:IndicatorToGroupMembership ;
	rdfs:label	"ecommerce" ;
	ns11:member-of	ns12:ecommerce ;
	ns11:order	"4" .
ns20:i_bserv	rdf:type	ns10:IndicatorToGroupMembership ;
	rdfs:label	"ecommerce" ;
	ns11:member-of	ns12:ecommerce ;
	ns11:order	"5" .
ns20:i_iusell	rdf:type	ns10:IndicatorToGroupMembership ;
	rdfs:label	"ecommerce" ;
	ns11:member-of	ns12:ecommerce ;
	ns11:order	"8" .
@prefix ns21:	<http://semantic.digital-agenda-data.eu/codelist/indicator-group/egovernment/> .
ns21:e_gov_1_ucg	rdf:type	ns10:IndicatorToGroupMembership ;
	rdfs:label	"egovernment" ;
	ns11:member-of	ns12:egovernment ;
	ns11:order	"1111" .
ns21:e_gov_1a_ucg_oa	rdf:type	ns10:IndicatorToGroupMembership ;
	rdfs:label	"egovernment" ;
	ns11:member-of	ns12:egovernment ;
	ns11:order	"11111" .
ns21:e_gov_1b_ucg_us	rdf:type	ns10:IndicatorToGroupMembership ;
	rdfs:label	"egovernment" ;
	ns11:member-of	ns12:egovernment ;
	ns11:order	"11113" .
ns21:e_gov_1c_ucg_mf	rdf:type	ns10:IndicatorToGroupMembership ;
	rdfs:label	"egovernment" ;
	ns11:member-of	ns12:egovernment ;
	ns11:order	"11114" .
ns21:e_gov_1d_ucg_eu	rdf:type	ns10:IndicatorToGroupMembership ;
	rdfs:label	"egovernment" ;
	ns11:member-of	ns12:egovernment ;
	ns11:order	"11115" .
ns21:e_gov_1e_ucg_su	rdf:type	ns10:IndicatorToGroupMembership ;
	rdfs:label	"egovernment" ;
	ns11:member-of	ns12:egovernment ;
	ns11:order	"11116" .
ns21:e_gov_2_tg	rdf:type	ns10:IndicatorToGroupMembership ;
	rdfs:label	"egovernment" ;
	ns11:member-of	ns12:egovernment ;
	ns11:order	"1112" .
ns21:e_gov_2a_tg_sd	rdf:type	ns10:IndicatorToGroupMembership ;
	rdfs:label	"egovernment" ;
	ns11:member-of	ns12:egovernment ;
	ns11:order	"11121" .
ns21:e_gov_2b_tg_po	rdf:type	ns10:IndicatorToGroupMembership ;
	rdfs:label	"egovernment" ;
	ns11:member-of	ns12:egovernment ;
	ns11:order	"11122" .
ns21:e_gov_2c_tg_pd	rdf:type	ns10:IndicatorToGroupMembership ;
	rdfs:label	"egovernment" ;
	ns11:member-of	ns12:egovernment ;
	ns11:order	"11123" .
ns21:e_gov_3_cm	rdf:type	ns10:IndicatorToGroupMembership ;
	rdfs:label	"egovernment" ;
	ns11:member-of	ns12:egovernment ;
	ns11:order	"1113" .
ns21:e_gov_3a_cm_oa	rdf:type	ns10:IndicatorToGroupMembership ;
	rdfs:label	"egovernment" ;
	ns11:member-of	ns12:egovernment ;
	ns11:order	"11131" .
ns21:e_gov_3b_cm_us	rdf:type	ns10:IndicatorToGroupMembership ;
	rdfs:label	"egovernment" ;
	ns11:member-of	ns12:egovernment ;
	ns11:order	"11133" .
ns21:e_gov_3c_cm_eidcb	rdf:type	ns10:IndicatorToGroupMembership ;
	rdfs:label	"egovernment" ;
	ns11:member-of	ns12:egovernment ;
	ns11:order	"11135" .
ns21:e_gov_3d_cm_edoccb	rdf:type	ns10:IndicatorToGroupMembership ;
	rdfs:label	"egovernment" ;
	ns11:member-of	ns12:egovernment ;
	ns11:order	"11136" .
ns21:e_gov_3e_cm_eu	rdf:type	ns10:IndicatorToGroupMembership ;
	rdfs:label	"egovernment" ;
	ns11:member-of	ns12:egovernment ;
	ns11:order	"11137" .
ns21:e_gov_3f_cm_su	rdf:type	ns10:IndicatorToGroupMembership ;
	rdfs:label	"egovernment" ;
	ns11:member-of	ns12:egovernment ;
	ns11:order	"11138" .
ns21:e_gov_4_bm	rdf:type	ns10:IndicatorToGroupMembership ;
	rdfs:label	"egovernment" ;
	ns11:member-of	ns12:egovernment ;
	ns11:order	"1114" .
ns21:e_gov_4a_bm_oa	rdf:type	ns10:IndicatorToGroupMembership ;
	rdfs:label	"egovernment" ;
	ns11:member-of	ns12:egovernment ;
	ns11:order	"11141" .
ns21:e_gov_4b_bm_us	rdf:type	ns10:IndicatorToGroupMembership ;
	rdfs:label	"egovernment" ;
	ns11:member-of	ns12:egovernment ;
	ns11:order	"11143" .
ns21:e_gov_4c_bm_eidcb	rdf:type	ns10:IndicatorToGroupMembership ;
	rdfs:label	"egovernment" ;
	ns11:member-of	ns12:egovernment ;
	ns11:order	"11145" .
ns21:e_gov_4d_bm_edoccb	rdf:type	ns10:IndicatorToGroupMembership ;
	rdfs:label	"egovernment" ;
	ns11:member-of	ns12:egovernment ;
	ns11:order	"11146" .
ns21:e_gov_4e_bm_eu	rdf:type	ns10:IndicatorToGroupMembership ;
	rdfs:label	"egovernment" ;
	ns11:member-of	ns12:egovernment ;
	ns11:order	"11147" .
ns21:e_gov_4f_bm_su	rdf:type	ns10:IndicatorToGroupMembership ;
	rdfs:label	"egovernment" ;
	ns11:member-of	ns12:egovernment ;
	ns11:order	"11148" .
ns21:e_gov_5_ke	rdf:type	ns10:IndicatorToGroupMembership ;
	rdfs:label	"egovernment" ;
	ns11:member-of	ns12:egovernment ;
	ns11:order	"1115" .
ns21:e_gov_5a_ke_eid	rdf:type	ns10:IndicatorToGroupMembership ;
	rdfs:label	"egovernment" ;
	ns11:member-of	ns12:egovernment ;
	ns11:order	"11151" .
ns21:e_gov_5b_ke_edoc	rdf:type	ns10:IndicatorToGroupMembership ;
	rdfs:label	"egovernment" ;
	ns11:member-of	ns12:egovernment ;
	ns11:order	"11152" .
ns21:e_gov_5c_ke_as	rdf:type	ns10:IndicatorToGroupMembership ;
	rdfs:label	"egovernment" ;
	ns11:member-of	ns12:egovernment ;
	ns11:order	"11153" .
ns21:e_gov_5d_ke_dp	rdf:type	ns10:IndicatorToGroupMembership ;
	rdfs:label	"egovernment" ;
	ns11:member-of	ns12:egovernment ;
	ns11:order	"11154" .
ns21:e_gov_5e_ke_esafe	rdf:type	ns10:IndicatorToGroupMembership ;
	rdfs:label	"egovernment" ;
	ns11:member-of	ns12:egovernment ;
	ns11:order	"11155" .
ns21:e_gov_5f_ke_sso	rdf:type	ns10:IndicatorToGroupMembership ;
	rdfs:label	"egovernment" ;
	ns11:member-of	ns12:egovernment ;
	ns11:order	"11156" .
ns21:e_gov_ke	rdf:type	ns10:IndicatorToGroupMembership ;
	rdfs:label	"egovernment" ;
	ns11:member-of	ns12:egovernment ;
	ns11:order	"8" .
ns21:e_gov_opa	rdf:type	ns10:IndicatorToGroupMembership ;
	rdfs:label	"egovernment" ;
	ns11:member-of	ns12:egovernment ;
	ns11:order	"9" .
ns21:e_gov_osc	rdf:type	ns10:IndicatorToGroupMembership ;
	rdfs:label	"egovernment" ;
	ns11:member-of	ns12:egovernment ;
	ns11:order	"7" .
ns21:e_gov_pff	rdf:type	ns10:IndicatorToGroupMembership ;
	rdfs:label	"egovernment" ;
	ns11:member-of	ns12:egovernment ;
	ns11:order	"2" .
ns21:epsi_score	rdf:type	ns10:IndicatorToGroupMembership ;
	rdfs:label	"egovernment" ;
	ns11:member-of	ns12:egovernment ;
	ns11:order	"5" .
ns21:i_igov12rt	rdf:type	ns10:IndicatorToGroupMembership ;
	rdfs:label	"egovernment" ;
	ns11:member-of	ns12:egovernment ;
	ns11:order	"1" .
ns21:i_iugov12	rdf:type	ns10:IndicatorToGroupMembership ;
	rdfs:label	"egovernment" ;
	ns11:member-of	ns12:egovernment ;
	ns11:order	"6" .
@prefix ns22:	<http://semantic.digital-agenda-data.eu/codelist/indicator-group/ehealth/> .
ns22:hie_use_ex_admin	rdf:type	ns10:IndicatorToGroupMembership ;
	rdfs:label	"ehealth" ;
	ns11:member-of	ns12:ehealth ;
	ns11:order	"4" .
ns22:hie_use_pharm	rdf:type	ns10:IndicatorToGroupMembership ;
	rdfs:label	"ehealth" ;
	ns11:member-of	ns12:ehealth ;
	ns11:order	"3" .
ns22:i_ihif	rdf:type	ns10:IndicatorToGroupMembership ;
	rdfs:label	"ehealth" ;
	ns11:member-of	ns12:ehealth ;
	ns11:order	"1" .
ns22:i_iumapp	rdf:type	ns10:IndicatorToGroupMembership ;
	rdfs:label	"ehealth" ;
	ns11:member-of	ns12:ehealth ;
	ns11:order	"2" .
@prefix ns23:	<http://semantic.digital-agenda-data.eu/codelist/indicator-group/ict-edu/> .
ns23:eun_computers	rdf:type	ns10:IndicatorToGroupMembership ;
	rdfs:label	"ict-edu" ;
	ns11:member-of	ns12:ict-edu ;
	ns11:order	"1" .
ns23:eun_web	rdf:type	ns10:IndicatorToGroupMembership ;
	rdfs:label	"ict-edu" ;
	ns11:member-of	ns12:ict-edu ;
	ns11:order	"2" .
@prefix ns24:	<http://semantic.digital-agenda-data.eu/codelist/indicator-group/ict-sector/> .
ns24:bs_rd_expen_ict	rdf:type	ns10:IndicatorToGroupMembership ;
	rdfs:label	"ict-sector" ;
	ns11:member-of	ns12:ict-sector ;
	ns11:order	"6" .
ns24:employment_ict	rdf:type	ns10:IndicatorToGroupMembership ;
	rdfs:label	"ict-sector" ;
	ns11:member-of	ns12:ict-sector ;
	ns11:order	"4" .
ns24:ict_exp	rdf:type	ns10:IndicatorToGroupMembership ;
	rdfs:label	"ict-sector" ;
	ns11:member-of	ns12:ict-sector ;
	ns11:order	"1" .
ns24:ict_hgc	rdf:type	ns10:IndicatorToGroupMembership ;
	rdfs:label	"ict-sector" ;
	ns11:member-of	ns12:ict-sector ;
	ns11:order	"3" .
ns24:ict_imp	rdf:type	ns10:IndicatorToGroupMembership ;
	rdfs:label	"ict-sector" ;
	ns11:member-of	ns12:ict-sector ;
	ns11:order	"2" .
ns24:labour_prod_ict	rdf:type	ns10:IndicatorToGroupMembership ;
	rdfs:label	"ict-sector" ;
	ns11:member-of	ns12:ict-sector ;
	ns11:order	"7" .
ns24:val_add_ict	rdf:type	ns10:IndicatorToGroupMembership ;
	rdfs:label	"ict-sector" ;
	ns11:member-of	ns12:ict-sector ;
	ns11:order	"5" .
@prefix ns25:	<http://semantic.digital-agenda-data.eu/codelist/indicator-group/ict-skills/> .
ns25:i_dsk_bab	rdf:type	ns10:IndicatorToGroupMembership ;
	rdfs:label	"ict-skills" ;
	ns11:member-of	ns12:ict-skills ;
	ns11:order	"13" .
ns25:i_dsk_c_bab	rdf:type	ns10:IndicatorToGroupMembership ;
	rdfs:label	"ict-skills" ;
	ns11:member-of	ns12:ict-skills ;
	ns11:order	"22" .
ns25:i_dsk_i_bab	rdf:type	ns10:IndicatorToGroupMembership ;
	rdfs:label	"ict-skills" ;
	ns11:member-of	ns12:ict-skills ;
	ns11:order	"18" .
ns25:i_dsk_ps_bab	rdf:type	ns10:IndicatorToGroupMembership ;
	rdfs:label	"ict-skills" ;
	ns11:member-of	ns12:ict-skills ;
	ns11:order	"26" .
ns25:i_dsk_s_bab	rdf:type	ns10:IndicatorToGroupMembership ;
	rdfs:label	"ict-skills" ;
	ns11:member-of	ns12:ict-skills ;
	ns11:order	"32" .
ns25:st_grad	rdf:type	ns10:IndicatorToGroupMembership ;
	rdfs:label	"ict-skills" ;
	ns11:member-of	ns12:ict-skills ;
	ns11:order	"91" .
@prefix ns26:	<http://semantic.digital-agenda-data.eu/codelist/indicator-group/ict-specialist/> .
ns26:e_it_mext	rdf:type	ns10:IndicatorToGroupMembership ;
	rdfs:label	"ict-specialist" ;
	ns11:member-of	ns12:ict-specialist ;
	ns11:order	"4" .
ns26:e_itsp2	rdf:type	ns10:IndicatorToGroupMembership ;
	rdfs:label	"ict-specialist" ;
	ns11:member-of	ns12:ict-specialist ;
	ns11:order	"1" .
ns26:e_itspvac2	rdf:type	ns10:IndicatorToGroupMembership ;
	rdfs:label	"ict-specialist" ;
	ns11:member-of	ns12:ict-specialist ;
	ns11:order	"2" .
ns26:e_itt2	rdf:type	ns10:IndicatorToGroupMembership ;
	rdfs:label	"ict-specialist" ;
	ns11:member-of	ns12:ict-specialist ;
	ns11:order	"5" .
ns26:ict_spec3_broad	rdf:type	ns10:IndicatorToGroupMembership ;
	rdfs:label	"ict-specialist" ;
	ns11:member-of	ns12:ict-specialist ;
	ns11:order	"3" .
@prefix ns27:	<http://semantic.digital-agenda-data.eu/codelist/indicator-group/internet-services/> .
ns27:i_cc	rdf:type	ns10:IndicatorToGroupMembership ;
	rdfs:label	"internet-services" ;
	ns11:member-of	ns12:internet-services ;
	ns11:order	"14" .
ns27:i_iubk	rdf:type	ns10:IndicatorToGroupMembership ;
	rdfs:label	"internet-services" ;
	ns11:member-of	ns12:internet-services ;
	ns11:order	"4" .
ns27:i_iueduif	rdf:type	ns10:IndicatorToGroupMembership ;
	rdfs:label	"internet-services" ;
	ns11:member-of	ns12:internet-services ;
	ns11:order	"10" .
ns27:i_iuif	rdf:type	ns10:IndicatorToGroupMembership ;
	rdfs:label	"internet-services" ;
	ns11:member-of	ns12:internet-services ;
	ns11:order	"1" .
ns27:i_iujob	rdf:type	ns10:IndicatorToGroupMembership ;
	rdfs:label	"internet-services" ;
	ns11:member-of	ns12:internet-services ;
	ns11:order	"8" .
ns27:i_iuolc	rdf:type	ns10:IndicatorToGroupMembership ;
	rdfs:label	"internet-services" ;
	ns11:member-of	ns12:internet-services ;
	ns11:order	"9" .
ns27:i_iuph1	rdf:type	ns10:IndicatorToGroupMembership ;
	rdfs:label	"internet-services" ;
	ns11:member-of	ns12:internet-services ;
	ns11:order	"5" .
ns27:i_iusnet	rdf:type	ns10:IndicatorToGroupMembership ;
	rdfs:label	"internet-services" ;
	ns11:member-of	ns12:internet-services ;
	ns11:order	"7" .
ns27:i_iuupl	rdf:type	ns10:IndicatorToGroupMembership ;
	rdfs:label	"internet-services" ;
	ns11:member-of	ns12:internet-services ;
	ns11:order	"6" .
ns27:i_iuvote	rdf:type	ns10:IndicatorToGroupMembership ;
	rdfs:label	"internet-services" ;
	ns11:member-of	ns12:internet-services ;
	ns11:order	"13" .
@prefix ns28:	<http://semantic.digital-agenda-data.eu/codelist/indicator-group/internet-usage/> .
ns28:aaaa_cov	rdf:type	ns10:IndicatorToGroupMembership ;
	rdfs:label	"internet-usage" ;
	ns11:member-of	ns12:internet-usage ;
	ns11:order	"9" .
ns28:h_iacc	rdf:type	ns10:IndicatorToGroupMembership ;
	rdfs:label	"internet-usage" ;
	ns11:member-of	ns12:internet-usage ;
	ns11:order	"1" .
ns28:i_ia12ave	rdf:type	ns10:IndicatorToGroupMembership ;
	rdfs:label	"internet-usage" ;
	ns11:member-of	ns12:internet-usage ;
	ns11:order	"8" .
ns28:i_iday	rdf:type	ns10:IndicatorToGroupMembership ;
	rdfs:label	"internet-usage" ;
	ns11:member-of	ns12:internet-usage ;
	ns11:order	"5" .
ns28:i_ilt12	rdf:type	ns10:IndicatorToGroupMembership ;
	rdfs:label	"internet-usage" ;
	ns11:member-of	ns12:internet-usage ;
	ns11:order	"3" .
ns28:i_iu3	rdf:type	ns10:IndicatorToGroupMembership ;
	rdfs:label	"internet-usage" ;
	ns11:member-of	ns12:internet-usage ;
	ns11:order	"2" .
ns28:i_iumc	rdf:type	ns10:IndicatorToGroupMembership ;
	rdfs:label	"internet-usage" ;
	ns11:member-of	ns12:internet-usage ;
	ns11:order	"6" .
ns28:i_iuse	rdf:type	ns10:IndicatorToGroupMembership ;
	rdfs:label	"internet-usage" ;
	ns11:member-of	ns12:internet-usage ;
	ns11:order	"4" .
ns28:i_iux	rdf:type	ns10:IndicatorToGroupMembership ;
	rdfs:label	"internet-usage" ;
	ns11:member-of	ns12:internet-usage ;
	ns11:order	"7" .
@prefix ns29:	<http://semantic.digital-agenda-data.eu/codelist/indicator-group/mobile/> .
ns29:e_pmd	rdf:type	ns10:IndicatorToGroupMembership ;
	rdfs:label	"mobile" ;
	ns11:member-of	ns12:mobile ;
	ns11:order	"12" .
ns29:i_iu3g	rdf:type	ns10:IndicatorToGroupMembership ;
	rdfs:label	"mobile" ;
	ns11:member-of	ns12:mobile ;
	ns11:order	"11" .
ns29:mbb_hspacov	rdf:type	ns10:IndicatorToGroupMembership ;
	rdfs:label	"mobile" ;
	ns11:member-of	ns12:mobile ;
	ns11:order	"6" .
ns29:mbb_ltecov	rdf:type	ns10:IndicatorToGroupMembership ;
	rdfs:label	"mobile" ;
	ns11:member-of	ns12:mobile ;
	ns11:order	"4" .
ns29:mbb_penet	rdf:type	ns10:IndicatorToGroupMembership ;
	rdfs:label	"mobile" ;
	ns11:member-of	ns12:mobile ;
	ns11:order	"10" .
ns29:mbb_rhspacov	rdf:type	ns10:IndicatorToGroupMembership ;
	rdfs:label	"mobile" ;
	ns11:member-of	ns12:mobile ;
	ns11:order	"7" .
ns29:mbb_rltecov	rdf:type	ns10:IndicatorToGroupMembership ;
	rdfs:label	"mobile" ;
	ns11:member-of	ns12:mobile ;
	ns11:order	"5" .
ns29:mob_arpu	rdf:type	ns10:IndicatorToGroupMembership ;
	rdfs:label	"mobile" ;
	ns11:member-of	ns12:mobile ;
	ns11:order	"14" .
ns29:mob_ms	rdf:type	ns10:IndicatorToGroupMembership ;
	rdfs:label	"mobile" ;
	ns11:member-of	ns12:mobile ;
	ns11:order	"13" .
ns29:mob_mtr	rdf:type	ns10:IndicatorToGroupMembership ;
	rdfs:label	"mobile" ;
	ns11:member-of	ns12:mobile ;
	ns11:order	"17" .
ns29:mob_penet	rdf:type	ns10:IndicatorToGroupMembership ;
	rdfs:label	"mobile" ;
	ns11:member-of	ns12:mobile ;
	ns11:order	"9" .
ns29:mob_roam	rdf:type	ns10:IndicatorToGroupMembership ;
	rdfs:label	"mobile" ;
	ns11:member-of	ns12:mobile ;
	ns11:order	"15" .
ns29:mob_subs	rdf:type	ns10:IndicatorToGroupMembership ;
	rdfs:label	"mobile" ;
	ns11:member-of	ns12:mobile ;
	ns11:order	"8" .
ns29:spectrum_wbb	rdf:type	ns10:IndicatorToGroupMembership ;
	rdfs:label	"mobile" ;
	ns11:member-of	ns12:mobile ;
	ns11:order	"16" .
@prefix ns30:	<http://semantic.digital-agenda-data.eu/codelist/indicator-group/research-and-development/> .
ns30:avg_ttg	rdf:type	ns10:IndicatorToGroupMembership ;
	rdfs:label	"research-and-development" ;
	ns11:member-of	ns12:research-and-development ;
	ns11:order	"21" .
ns30:fp7_ict_artic	rdf:type	ns10:IndicatorToGroupMembership ;
	rdfs:label	"research-and-development" ;
	ns11:member-of	ns12:research-and-development ;
	ns11:order	"32" .
ns30:fp7_ict_pat	rdf:type	ns10:IndicatorToGroupMembership ;
	rdfs:label	"research-and-development" ;
	ns11:member-of	ns12:research-and-development ;
	ns11:order	"30" .
ns30:fp7_ict_pub	rdf:type	ns10:IndicatorToGroupMembership ;
	rdfs:label	"research-and-development" ;
	ns11:member-of	ns12:research-and-development ;
	ns11:order	"31" .
ns30:fp7ict_afxp	rdf:type	ns10:IndicatorToGroupMembership ;
	rdfs:label	"research-and-development" ;
	ns11:member-of	ns12:research-and-development ;
	ns11:order	"17" .
ns30:fp7ict_cofin	rdf:type	ns10:IndicatorToGroupMembership ;
	rdfs:label	"research-and-development" ;
	ns11:member-of	ns12:research-and-development ;
	ns11:order	"15" .
ns30:fp7ict_ec_funding	rdf:type	ns10:IndicatorToGroupMembership ;
	rdfs:label	"research-and-development" ;
	ns11:member-of	ns12:research-and-development ;
	ns11:order	"13" .
ns30:fp7ict_ec_funding_prc	rdf:type	ns10:IndicatorToGroupMembership ;
	rdfs:label	"research-and-development" ;
	ns11:member-of	ns12:research-and-development ;
	ns11:order	"41" .
ns30:fp7ict_ec_funding_smes	rdf:type	ns10:IndicatorToGroupMembership ;
	rdfs:label	"research-and-development" ;
	ns11:member-of	ns12:research-and-development ;
	ns11:order	"42" .
ns30:fp7ict_newentry	rdf:type	ns10:IndicatorToGroupMembership ;
	rdfs:label	"research-and-development" ;
	ns11:member-of	ns12:research-and-development ;
	ns11:order	"18" .
ns30:fp7ict_organisations	rdf:type	ns10:IndicatorToGroupMembership ;
	rdfs:label	"research-and-development" ;
	ns11:member-of	ns12:research-and-development ;
	ns11:order	"19" .
ns30:fp7ict_particip	rdf:type	ns10:IndicatorToGroupMembership ;
	rdfs:label	"research-and-development" ;
	ns11:member-of	ns12:research-and-development ;
	ns11:order	"16" .
ns30:fp7ict_particip_prc	rdf:type	ns10:IndicatorToGroupMembership ;
	rdfs:label	"research-and-development" ;
	ns11:member-of	ns12:research-and-development ;
	ns11:order	"43" .
ns30:fp7ict_particip_smes	rdf:type	ns10:IndicatorToGroupMembership ;
	rdfs:label	"research-and-development" ;
	ns11:member-of	ns12:research-and-development ;
	ns11:order	"44" .
ns30:fp7ict_totcost	rdf:type	ns10:IndicatorToGroupMembership ;
	rdfs:label	"research-and-development" ;
	ns11:member-of	ns12:research-and-development ;
	ns11:order	"14" .
ns30:gbaord	rdf:type	ns10:IndicatorToGroupMembership ;
	rdfs:label	"research-and-development" ;
	ns11:member-of	ns12:research-and-development ;
	ns11:order	"1" .
ns30:gbaord_ict	rdf:type	ns10:IndicatorToGroupMembership ;
	rdfs:label	"research-and-development" ;
	ns11:member-of	ns12:research-and-development ;
	ns11:order	"2" .
ns30:h2020_cofin	rdf:type	ns10:IndicatorToGroupMembership ;
	rdfs:label	"research-and-development" ;
	ns11:member-of	ns12:research-and-development ;
	ns11:order	"5" .
ns30:h2020_ec_funding	rdf:type	ns10:IndicatorToGroupMembership ;
	rdfs:label	"research-and-development" ;
	ns11:member-of	ns12:research-and-development ;
	ns11:order	"3" .
ns30:h2020_newentry	rdf:type	ns10:IndicatorToGroupMembership ;
	rdfs:label	"research-and-development" ;
	ns11:member-of	ns12:research-and-development ;
	ns11:order	"9" .
ns30:h2020_organisations	rdf:type	ns10:IndicatorToGroupMembership ;
	rdfs:label	"research-and-development" ;
	ns11:member-of	ns12:research-and-development ;
	ns11:order	"8" .
ns30:h2020_particip	rdf:type	ns10:IndicatorToGroupMembership ;
	rdfs:label	"research-and-development" ;
	ns11:member-of	ns12:research-and-development ;
	ns11:order	"6" .
ns30:h2020_totcost	rdf:type	ns10:IndicatorToGroupMembership ;
	rdfs:label	"research-and-development" ;
	ns11:member-of	ns12:research-and-development ;
	ns11:order	"4" .
ns30:h2020ict_afxp	rdf:type	ns10:IndicatorToGroupMembership ;
	rdfs:label	"research-and-development" ;
	ns11:member-of	ns12:research-and-development ;
	ns11:order	"7" .
ns30:ict_commit_in_trp	rdf:type	ns10:IndicatorToGroupMembership ;
	rdfs:label	"research-and-development" ;
	ns11:member-of	ns12:research-and-development ;
	ns11:order	"20" .
ns30:pay_on_time_projects	rdf:type	ns10:IndicatorToGroupMembership ;
	rdfs:label	"research-and-development" ;
	ns11:member-of	ns12:research-and-development ;
	ns11:order	"23" .
ns30:ttg_in_scope	rdf:type	ns10:IndicatorToGroupMembership ;
	rdfs:label	"research-and-development" ;
	ns11:member-of	ns12:research-and-development ;
	ns11:order	"22" .
@prefix ns31:	<http://semantic.digital-agenda-data.eu/codelist/indicator-group/research_einfra/> .
ns31:c1_bandwidth	rdf:type	ns10:IndicatorToGroupMembership ;
	rdfs:label	"research_einfra" ;
	ns11:member-of	ns12:research_einfra ;
	ns11:order	"3" .
ns31:c1_compcyclesegi	rdf:type	ns10:IndicatorToGroupMembership ;
	rdfs:label	"research_einfra" ;
	ns11:member-of	ns12:research_einfra ;
	ns11:order	"1" .
ns31:c1_compcyclesprace	rdf:type	ns10:IndicatorToGroupMembership ;
	rdfs:label	"research_einfra" ;
	ns11:member-of	ns12:research_einfra ;
	ns11:order	"2" .
ns31:c1_datatraffic	rdf:type	ns10:IndicatorToGroupMembership ;
	rdfs:label	"research_einfra" ;
	ns11:member-of	ns12:research_einfra ;
	ns11:order	"4" .
@prefix ns32:	<http://semantic.digital-agenda-data.eu/codelist/indicator-group/security-privacy/> .
ns32:e_ads_loc	rdf:type	ns10:IndicatorToGroupMembership ;
	rdfs:label	"security-privacy" ;
	ns11:member-of	ns12:security-privacy ;
	ns11:order	"9" .
ns32:e_ads_trk	rdf:type	ns10:IndicatorToGroupMembership ;
	rdfs:label	"security-privacy" ;
	ns11:member-of	ns12:security-privacy ;
	ns11:order	"10" .
ns32:e_secpol1	rdf:type	ns10:IndicatorToGroupMembership ;
	rdfs:label	"security-privacy" ;
	ns11:member-of	ns12:security-privacy ;
	ns11:order	"11" .
ns32:i_atsw	rdf:type	ns10:IndicatorToGroupMembership ;
	rdfs:label	"security-privacy" ;
	ns11:member-of	ns12:security-privacy ;
	ns11:order	"7" .
ns32:i_cook	rdf:type	ns10:IndicatorToGroupMembership ;
	rdfs:label	"security-privacy" ;
	ns11:member-of	ns12:security-privacy ;
	ns11:order	"6" .
ns32:i_piacadv	rdf:type	ns10:IndicatorToGroupMembership ;
	rdfs:label	"security-privacy" ;
	ns11:member-of	ns12:security-privacy ;
	ns11:order	"8" .
ns32:i_sbgood	rdf:type	ns10:IndicatorToGroupMembership ;
	rdfs:label	"security-privacy" ;
	ns11:member-of	ns12:security-privacy ;
	ns11:order	"5" .
ns32:i_secfl	rdf:type	ns10:IndicatorToGroupMembership ;
	rdfs:label	"security-privacy" ;
	ns11:member-of	ns12:security-privacy ;
	ns11:order	"2" .
ns32:i_secpif1	rdf:type	ns10:IndicatorToGroupMembership ;
	rdfs:label	"security-privacy" ;
	ns11:member-of	ns12:security-privacy ;
	ns11:order	"3" .
ns32:i_secvir1	rdf:type	ns10:IndicatorToGroupMembership ;
	rdfs:label	"security-privacy" ;
	ns11:member-of	ns12:security-privacy ;
	ns11:order	"4" .
@prefix ns33:	<http://semantic.digital-agenda-data.eu/codelist/indicator-group/telecom/> .
ns33:tel_ftr	rdf:type	ns10:IndicatorToGroupMembership ;
	rdfs:label	"telecom" ;
	ns11:member-of	ns12:telecom ;
	ns11:order	"3" .
ns33:tel_inv	rdf:type	ns10:IndicatorToGroupMembership ;
	rdfs:label	"telecom" ;
	ns11:member-of	ns12:telecom ;
	ns11:order	"2" .
ns33:tel_llu	rdf:type	ns10:IndicatorToGroupMembership ;
	rdfs:label	"telecom" ;
	ns11:member-of	ns12:telecom ;
	ns11:order	"4" .
ns33:tel_rev	rdf:type	ns10:IndicatorToGroupMembership ;
	rdfs:label	"telecom" ;
	ns11:member-of	ns12:telecom ;
	ns11:order	"1" .
@prefix ns34:	<http://semantic.digital-agenda-data.eu/codelist/indicator-group/wid/> .
ns34:wid_ius	rdf:type	ns10:IndicatorToGroupMembership ;
	rdfs:label	"wid" ;
	ns11:member-of	ns12:wid ;
	ns11:order	"10" .
ns34:wid_ius_abs	rdf:type	ns10:IndicatorToGroupMembership ;
	rdfs:label	"wid" ;
	ns11:member-of	ns12:wid ;
	ns11:order	"12" .
ns34:wid_ius_bs	rdf:type	ns10:IndicatorToGroupMembership ;
	rdfs:label	"wid" ;
	ns11:member-of	ns12:wid ;
	ns11:order	"11" .
ns34:wid_ius_ss	rdf:type	ns10:IndicatorToGroupMembership ;
	rdfs:label	"wid" ;
	ns11:member-of	ns12:wid ;
	ns11:order	"13" .
ns34:wid_score	rdf:type	ns10:IndicatorToGroupMembership ;
	rdfs:label	"wid" ;
	ns11:member-of	ns12:wid ;
	ns11:order	"1" .
ns34:wid_sse	rdf:type	ns10:IndicatorToGroupMembership ;
	rdfs:label	"wid" ;
	ns11:member-of	ns12:wid ;
	ns11:order	"14" .
ns34:wid_sse_gpg	rdf:type	ns10:IndicatorToGroupMembership ;
	rdfs:label	"wid" ;
	ns11:member-of	ns12:wid ;
	ns11:order	"17" .
ns34:wid_sse_icts	rdf:type	ns10:IndicatorToGroupMembership ;
	rdfs:label	"wid" ;
	ns11:member-of	ns12:wid ;
	ns11:order	"16" .
ns34:wid_sse_stem	rdf:type	ns10:IndicatorToGroupMembership ;
	rdfs:label	"wid" ;
	ns11:member-of	ns12:wid ;
	ns11:order	"15" .
ns34:wid_ui	rdf:type	ns10:IndicatorToGroupMembership ;
	rdfs:label	"wid" ;
	ns11:member-of	ns12:wid ;
	ns11:order	"2" .
ns34:wid_ui_egov	rdf:type	ns10:IndicatorToGroupMembership ;
	rdfs:label	"wid" ;
	ns11:member-of	ns12:wid ;
	ns11:order	"9" .
ns34:wid_ui_ib	rdf:type	ns10:IndicatorToGroupMembership ;
	rdfs:label	"wid" ;
	ns11:member-of	ns12:wid ;
	ns11:order	"5" .
ns34:wid_ui_iu	rdf:type	ns10:IndicatorToGroupMembership ;
	rdfs:label	"wid" ;
	ns11:member-of	ns12:wid ;
	ns11:order	"3" .
ns34:wid_ui_nui	rdf:type	ns10:IndicatorToGroupMembership ;
	rdfs:label	"wid" ;
	ns11:member-of	ns12:wid ;
	ns11:order	"4" .
ns34:wid_ui_oc	rdf:type	ns10:IndicatorToGroupMembership ;
	rdfs:label	"wid" ;
	ns11:member-of	ns12:wid ;
	ns11:order	"7" .
ns34:wid_ui_part	rdf:type	ns10:IndicatorToGroupMembership ;
	rdfs:label	"wid" ;
	ns11:member-of	ns12:wid ;
	ns11:order	"8" .
ns7:aaaa_cov	rdf:type	ns10:Indicator ,
		skos:Concept ;
	skos:prefLabel	"IPv6 readiness - websites having a AAAA coverage in DNS records (as % of most visited websites)" .
@prefix ns35:	<http://semantic.digital-agenda-data.eu/codelist/source/> .
ns7:aaaa_cov	dct:source	ns35:ipv6obs ;
	skos:notation	"aaaa_cov" ;
	skos:altLabel	"IPv6 readiness of most visited websites" ;
	ns11:membership	ns28:aaaa_cov ;
	skos:definition	"IPv6 ready websites are those having at least one AAAA in their DNS records (means the website is visible/can reply to users having an IPv6 connectivity). Tests are done every trimester through a script run by the IPv6 Observatory study on the 1 million most visited websites list provided by Alexa. Websites are attributed to countries on the basis of their main operation location as provided by MaxMind GeoIP database." ;
	skos:topConceptOf	ns1:indicator .
ns7:actspeed	rdf:type	ns10:Indicator ,
		skos:Concept ;
	skos:prefLabel	"Actual download speed of fixed broadband subscriptions" ;
	dct:source	ns35:samknows ;
	skos:notation	"actspeed" ;
	skos:altLabel	"Actual fixed broadband download speed" ;
	ns11:membership	ns14:actspeed ;
	skos:definition	"Average Download Speed during peak periods (ACTSPEED), measured with a specially configured hardware device (SamKnows Whitebox), which runs a series of purpose-built tests to measure various aspect of Internet performance. The measured speed refers to a sample of subscriptions using a similar technology offered by internet service providers. Offers are not weigthed with market shares, so the measured speed cannot be interpreted as the average experienced by consumers." ;
	skos:topConceptOf	ns1:indicator .
ns7:afford_internet_only_minppp	rdf:type	ns10:Indicator ,
		skos:Concept ;
	skos:prefLabel	"Affordability of standalone Fixed Internet Access (minimum price offer)" ;
	dct:source	ns35:biac ;
	skos:notation	"afford_internet_only_minppp" ;
	skos:altLabel	"Affordability of Fixed Internet Access" ;
	ns11:membership	ns14:afford_internet_only_minppp ;
	skos:definition	"Affordability is defined as 12 times the monthly price divided by the \"real adjusted gross disposable income of households per capita\" of the previous year. Disposable income data come from  Eurostat table  <a href=\"http://ec.europa.eu/eurostat/tgm/table.do?tab=table&plugin=1&language=en&pcode=tec00113\">tec00113</a>. Monthly price of standalone Fixed Broadband Internet Access offers, include value added tax, exclude the additional cost of telephony or cable line (if any), and refers to the minimum price in the group of similar subscriptions offered by internet service providers (see the <a href=\"http://digital-agenda-data.eu/charts/see-the-evolution-of-an-indicator-and-compare-countries#chart={%22indicator-group%22:%22any%22,%22indicator%22:%22Price_Internet_only%22,%22breakdown%22:%22offer_12_30_Mbps%22,%22unit-measure%22:%22minimum_euro_PPP%22,%22ref-area%22:[%22EU27%22]}\">original indicator</a>). " ;
	skos:topConceptOf	ns1:indicator .
ns7:avg_ttg	rdf:type	ns10:Indicator ,
		skos:Concept ;
	skos:prefLabel	"Average time to grant" ;
	dct:source	ns35:corda ;
	skos:notation	"avg_ttg" ;
	skos:altLabel	"Average time to grant" ;
	ns11:membership	ns30:avg_ttg ;
	skos:definition	"The Time to Grant (TTG) is defined as the time lapsed from a call's closing date (deadline for submission of proposals) to that of a grant signature by the European Commission. In the case of two-stage calls for proposals, it is the second stage call deadline that is used in the calculation of the Time to Grant. Time to grant is expressed in calendar days. \nAverage time to grant is the arythmetic average for all grants within the defined scope." ;
	skos:topConceptOf	ns1:indicator .
ns7:bb_dsl	rdf:type	ns10:Indicator ,
		skos:Concept ;
	skos:prefLabel	"DSL subscriptions share in fixed broadband" ;
	dct:source	ns35:cocom ;
	skos:notation	"bb_dsl" ;
	skos:altLabel	"DSL subscriptions share in fixed broadband" ;
	ns11:membership	ns15:bb_dsl ;
	skos:definition	"Share of DSL (Digital Subscriber Line) in total fixed broadband subscriptions." ;
	skos:topConceptOf	ns1:indicator .
ns7:bb_fcov	rdf:type	ns10:Indicator ,
		skos:Concept ;
	skos:prefLabel	"Fixed broadband coverage (2005-2010)" ;
	dct:source	ns35:idate ;
	skos:notation	"bb_fcov" ;
	skos:altLabel	"Fixed broadband coverage (2005-2010)" ;
	ns11:membership	ns18:bb_fcov ;
	skos:definition	"Coverage is a supply indicator, defined as the percentage of total/rural population living in areas served by fixed broadband: either DSL or cable modem networks." ;
	skos:note	"Indicator collected until 2010. Then replaced with two different coverage indicators, for standard broadband and NGA respectively." ;
	skos:topConceptOf	ns1:indicator .
ns7:bb_fttpcov	rdf:type	ns10:Indicator ,
		skos:Concept ;
	skos:prefLabel	"Fibre to the Premises coverage/availability (as a % of households)" ;
	dct:source	ns35:bc2020 ;
	skos:notation	"bb_fttpcov" ;
	skos:altLabel	"Fibre to the Premises coverage" ;
	ns11:membership	ns15:bb_fttpcov ;
	skos:definition	"Coverage is a supply indicator defined as the percentage of Households living in areas served by FTTP" ;
	skos:topConceptOf	ns1:indicator .
ns7:bb_hhi	rdf:type	ns10:Indicator ,
		skos:Concept ;
	skos:prefLabel	"Herfindahl index on broadband competition" ;
	dct:source	ns35:cocom ;
	skos:notation	"bb_hhi" ;
	skos:altLabel	"Herfindahl index on broadband competition" ;
	ns11:membership	ns15:bb_hhi ;
	skos:definition	"Herfindahl index calculated for seven different connection technologies: xDSL, full or shared LLU, Cable, FTTH, FTTB, Other NGA, Other. Their respective market shares are expressed in percentage of all fixed broadband subscriptions. A small index indicates a competitive industry with no dominant technological platform. The index values raises with concentration over one or few platforms." ;
	skos:topConceptOf	ns1:indicator .
ns7:bb_lines	rdf:type	skos:Concept ,
		ns10:Indicator ;
	skos:prefLabel	"Fixed broadband subscriptions" ;
	dct:source	ns35:cocom ;
	skos:notation	"bb_lines" ;
	skos:altLabel	"Fixed broadband subscriptions" ;
	ns11:membership	ns15:bb_lines ;
	skos:definition	"Number of fixed broadband subscriptions (lines)." ;
	skos:topConceptOf	ns1:indicator .
ns7:bb_ne	rdf:type	skos:Concept ,
		ns10:Indicator ;
	skos:prefLabel	"New entrants' share in fixed broadband subscriptions" ;
	dct:source	ns35:cocom ;
	skos:notation	"bb_ne" ;
	skos:altLabel	"New entrants' share in fixed broadband subscriptions" ;
	ns11:membership	ns15:bb_ne ;
	skos:definition	"Market share based on fixed broadband subscriptions (lines). New entrants mean operators that did not enjoy special and exclusive rights or de facto monopoly for the provision of voice telephony services before the liberalisation." ;
	skos:topConceptOf	ns1:indicator .
ns7:bb_ngacov	rdf:type	skos:Concept ,
		ns10:Indicator ;
	skos:prefLabel	"NGA broadband coverage/availability (as a % of households)" ;
	dct:source	ns35:bc2020 ;
	skos:notation	"bb_ngacov" ;
	skos:altLabel	"NGA broadband coverage/availability" ;
	ns11:membership	ns15:bb_ngacov ;
	skos:definition	"Coverage is a supply indicator defined as the percentage of Households living in areas served by NGA. Next Generation Access includes the following technologies: FTTH, FTTB, Cable Docsis 3.0, VDSL and other superfast broadband (at least 30 Mbps download)" ;
	skos:topConceptOf	ns1:indicator .
ns7:bb_penet	rdf:type	skos:Concept ,
		ns10:Indicator ;
	skos:prefLabel	"Fixed broadband take-up (subscriptions/100 people)" ;
	dct:source	ns35:cocom ;
	skos:notation	"bb_penet" ;
	skos:altLabel	"Fixed broadband take-up (penetration rate)" ;
	ns11:membership	ns15:bb_penet ;
	skos:definition	"Number of fixed broadband subscriptions (lines) per 100 people. Penetration of fixed broadband." ;
	skos:topConceptOf	ns1:indicator .
ns7:bb_rfttpcov	rdf:type	skos:Concept ,
		ns10:Indicator ;
	skos:prefLabel	"Rural Fibre to the Premises coverage/availability (as a % of households)" ;
	dct:source	ns35:bc2020 ;
	skos:notation	"bb_rfttpcov" ;
	skos:altLabel	"Rural Fibre to the Premises coverage" ;
	ns11:membership	ns15:bb_rfttpcov ;
	skos:definition	"Coverage is a supply indicator defined as the percentage of Households living in areas served by FTTP. Rural areas are defined as those with less than 100 people per km2." ;
	skos:topConceptOf	ns1:indicator .
ns7:bb_rngacov	rdf:type	skos:Concept ,
		ns10:Indicator ;
	skos:prefLabel	"Rural NGA broadband coverage/availability (as a % of households)" ;
	dct:source	ns35:bc2020 ;
	skos:notation	"bb_rngacov" ;
	skos:altLabel	"Rural NGA broadband coverage" ;
	ns11:membership	ns15:bb_rngacov ;
	skos:definition	"Coverage is a supply indicator defined as the percentage of Households living in areas served by NGA. Next Generation Access includes the following technologies: FTTH, FTTB, Cable Docsis 3.0, VDSL and other superfast broadband (at least 30 Mbps download). Rural areas are defined as those with less than 100 people per km2." ;
	skos:topConceptOf	ns1:indicator .
ns7:bb_scov	rdf:type	skos:Concept ,
		ns10:Indicator ;
	skos:prefLabel	"Standard fixed broadband coverage/availability (as a % of households)" ;
	dct:source	ns35:bc2020 ;
	skos:notation	"bb_scov" ;
	skos:altLabel	"Standard fixed broadband coverage/availability" ;
	ns11:membership	ns15:bb_scov ;
	skos:definition	"Coverage is a supply indicator defined as the percentage of Households living in areas served by xDSL, cable (basic and NGA), FTTP or WiMax networks" ;
	skos:topConceptOf	ns1:indicator .
ns7:bb_speed10	rdf:type	skos:Concept ,
		ns10:Indicator ;
	skos:prefLabel	"Share of fixed broadband subscriptions >= 10 Mbps - Advertised download speed" ;
	dct:source	ns35:cocom ;
	skos:notation	"bb_speed10" ;
	skos:altLabel	"Share of fixed broadband subscriptions >= 10 Mbps" ;
	ns11:membership	ns14:bb_speed10 ;
	skos:definition	"Based on advertised download speeds." ;
	skos:topConceptOf	ns1:indicator .
ns7:bb_speed100	rdf:type	skos:Concept ,
		ns10:Indicator ;
	skos:prefLabel	"Share of fixed broadband subscriptions >= 100 Mbps - Advertised download speed" ;
	dct:source	ns35:cocom ;
	skos:notation	"bb_speed100" ;
	skos:altLabel	"Share of fixed broadband subscriptions >= 100 Mbps" ;
	ns11:membership	ns14:bb_speed100 ;
	skos:definition	"Based on advertised download speeds." ;
	skos:topConceptOf	ns1:indicator .
ns7:bb_speed2	rdf:type	skos:Concept ,
		ns10:Indicator ;
	skos:prefLabel	"Share of fixed broadband subscriptions >= 2 Mbps - Advertised download speed" ;
	dct:source	ns35:cocom ;
	skos:notation	"bb_speed2" ;
	skos:altLabel	"Share of fixed broadband subscriptions >= 2 Mbps" ;
	ns11:membership	ns14:bb_speed2 ;
	skos:definition	"Based on advertised download speeds." ;
	skos:topConceptOf	ns1:indicator .
ns7:bb_speed30	rdf:type	skos:Concept ,
		ns10:Indicator ;
	skos:prefLabel	"Share of fixed broadband subscriptions >= 30 Mbps - Advertised download speed" ;
	dct:source	ns35:cocom ;
	skos:notation	"bb_speed30" ;
	skos:altLabel	"Share of fixed broadband subscriptions >= 30 Mbps" ;
	ns11:membership	ns14:bb_speed30 ;
	skos:definition	"Based on advertised download speeds." ;
	skos:topConceptOf	ns1:indicator .
ns7:bb_srcov	rdf:type	skos:Concept ,
		ns10:Indicator ;
	skos:prefLabel	"Rural standard fixed broadband coverage (as a % of households)" ;
	dct:source	ns35:bc2020 ;
	skos:notation	"bb_srcov" ;
	skos:altLabel	"Rural standard fixed broadband coverage" ;
	ns11:membership	ns15:bb_srcov ;
	skos:definition	"Coverage is a supply indicator defined as the percentage of Households living in areas served by xDSL, cable (basic and NGA), FTTP or WiMax networks. Rural areas are defined as those with less than 100 people per km2." ;
	skos:topConceptOf	ns1:indicator .
ns7:bs_rd_expen_ict	rdf:type	skos:Concept ,
		ns10:Indicator ;
	skos:prefLabel	"Business R&D expenditure of the ICT sector" ;
	dct:source	ns35:jrc_ict_randd ;
	skos:notation	"bs_rd_expen_ict" ;
	skos:altLabel	"Business R&D expenditure of the ICT sector" ;
	ns11:membership	ns24:bs_rd_expen_ict ;
	skos:definition	"Intramural expenditures on R&D performed within business enterprise sector during a specific period, whatever the source of funds (Frascati Manual)." ;
	skos:topConceptOf	ns1:indicator .
ns7:c1_bandwidth	rdf:type	skos:Concept ,
		ns10:Indicator ;
	skos:prefLabel	"Total bandwidth available in G\u00E9ant" ;
	dct:source	ns35:einfrageant ;
	skos:notation	"c1_bandwidth" ;
	skos:altLabel	"Total bandwidth available in G\u00E9ant" ;
	ns11:membership	ns31:c1_bandwidth ;
	skos:definition	"This is measured as total bandwidth available in the European G\u00C9ANT footprint (Gbpskms)  ( European dark fibre + European leased capacity excluding the connections to interconnections such as Internet2)" ;
	skos:note	"As of June 2014 the revamping of the networking was achieved and due to a technology optimisation there are less lightened backup routes explaining the decrease in capacity." ;
	skos:topConceptOf	ns1:indicator .
ns7:c1_compcyclesegi	rdf:type	skos:Concept ,
		ns10:Indicator ;
	skos:prefLabel	"Computing cycles available for open transnational access in EGI" ;
	dct:source	ns35:einfraegi ;
	skos:notation	"c1_compcyclesegi" ;
	skos:altLabel	"Computing cycles EGI" ;
	ns11:membership	ns31:c1_compcyclesegi ;
	skos:definition	"Computing cycles made available by EGI - the European Grid Infrastructure -, a federation of over 350 resource centres coordinated by a not-for-profit foundation which delivers integrated computing services to European researchers, co-funded by the European Commission." ;
	skos:topConceptOf	ns1:indicator .
ns7:c1_compcyclesprace	rdf:type	skos:Concept ,
		ns10:Indicator ;
	skos:prefLabel	"Computing cycles available for open transnational access in PRACE" ;
	dct:source	ns35:einfraprace ;
	skos:notation	"c1_compcyclesprace" ;
	skos:altLabel	"Computing cycles PRACE" ;
	ns11:membership	ns31:c1_compcyclesprace ;
	skos:definition	"Computing cycles allocated by PRACE - Partnership for Advanced Computing in Europe -, a project which delivers pan-European supercomputing infrastructure to European researchers, co-funded by the European Commission." ;
	skos:topConceptOf	ns1:indicator .
ns7:c1_datatraffic	rdf:type	ns10:Indicator ,
		skos:Concept ;
	skos:prefLabel	"Cross border Data traffic over the research networks" ;
	dct:source	ns35:einfrageant ;
	skos:notation	"c1_datatraffic" ;
	skos:altLabel	"Cross border Data traffic" ;
	ns11:membership	ns31:c1_datatraffic ;
	skos:definition	"This is the total monthly volume of traffic transiting G\u00C9ANT. As reported in the G\u00C9ANT MSR, measured as the aggregated traffic over a month to and from the European NRENs and all world regions." ;
	skos:note	"As of 01/01/2015 the indicator is reset to integrate traffic that was not counted (Layer 1 & 2)." ;
	skos:topConceptOf	ns1:indicator .
ns7:desi	rdf:type	ns10:Indicator ,
		skos:Concept ;
	skos:prefLabel	"Digital Economy and Society Index" ;
	dct:source	ns35: ;
	skos:notation	"desi" ;
	skos:altLabel	"DESI Stacked" ;
	ns11:membership	ns16:desi ;
	skos:definition	"DESI overall index, calculated as the weighted average of the four main DESI dimensions." ;
	skos:topConceptOf	ns1:indicator .
ns7:desi_sliders	rdf:type	skos:Concept ,
		ns10:Indicator ;
	skos:prefLabel	"Digital Economy and Society Index" ;
	dct:source	ns35: ;
	skos:notation	"desi_sliders" ;
	skos:altLabel	"DESI" ;
	ns11:membership	ns17:desi_sliders ;
	skos:definition	"DESI overall index, calculated as the weighted average of the four main DESI dimensions with the weights selected by the user." ;
	skos:topConceptOf	ns1:indicator .
ns7:e_ade	rdf:type	ns10:Indicator ,
		skos:Concept ;
	skos:prefLabel	"Enterprises exchanging business documents suitable for automatic processing" ;
	dct:source	ns35:estat_isoc_bde15disc ;
	skos:notation	"e_ade" ;
	skos:altLabel	"Automatic exchange of business documents" ;
	ns11:membership	ns18:e_ade ;
	skos:definition	"The indicator refers to sending/receiving of messages (orders, invoices, payment transactions, transport documents, tax declarations, etc.) to/from other enterprises, public authorities or financial institutions in an agreed or standard format (as EDIFACT, XML, etc) which allows their automatic processing without the individual message being manually typed." ;
	skos:note	"Enterprises with 10 or more persons employed. All manufacturing and service sectors, excluding the financial sector. Breaks in series because until 2008 economic activities according to NACE Rev 1.1 and from 2009 data are based on NACE Rev.2. Since 2010 data include also sector S 95.1-Repair of computers and communication equipment." ;
	skos:topConceptOf	ns1:indicator .
ns7:e_ads	rdf:type	ns10:Indicator ,
		skos:Concept ;
	skos:prefLabel	"Enterprises paying to advertise on the internet\n" ;
	dct:source	ns35:estat_isoc_cismt ;
	skos:notation	"e_ads" ;
	skos:altLabel	"Enterprises paying to advertise on the internet\n" ;
	ns11:membership	ns19:e_ads ;
	skos:definition	"Enterprises paying to advertise on the internet\n" ;
	skos:note	"Enterprises with 10 or more persons employed. All manufacturing and service sectors, excluding the financial sector. Breaks in series because until 2008 economic activities according to NACE Rev 1.1 and from 2009 data are based on NACE Rev.2. Since 2010 data include also sector S 95.1-Repair of computers and communication equipment." ;
	skos:topConceptOf	ns1:indicator .
ns7:e_ads_loc	rdf:type	ns10:Indicator ,
		skos:Concept ;
	skos:prefLabel	"Enterprises advertising online based on the geolocation of internet users " ;
	dct:source	ns35:estat_isoc_cismt ;
	skos:notation	"e_ads_loc" ;
	skos:altLabel	"Enterprises advertising online based on the geolocation of internet users " ;
	ns11:membership	ns32:e_ads_loc ;
	skos:definition	"Pay to advertise on the internet, based on the geolocation of internet users " ;
	skos:topConceptOf	ns1:indicator .
ns7:e_ads_trk	rdf:type	ns10:Indicator ,
		skos:Concept ;
	skos:prefLabel	"Enterprises tracking internet users for targeted advertising " ;
	dct:source	ns35:estat_isoc_cismt ;
	skos:notation	"e_ads_trk" ;
	skos:altLabel	"Enterprises tracking internet users for targeted advertising " ;
	ns11:membership	ns32:e_ads_trk ;
	skos:definition	"Pay to advertise on the internet, based on the tracking of internet users' past activities or profile " ;
	skos:topConceptOf	ns1:indicator .
ns7:e_aeseu	rdf:type	ns10:Indicator ,
		skos:Concept ;
	skos:prefLabel	"Enterprises having done electronic sales to other EU countries in the last calender year" ;
	dct:source	ns35:estat_isoc_ec_eseln2 ;
	skos:notation	"e_aeseu" ;
	skos:altLabel	"Enterprises selling cross-border to other EU countries" ;
	ns11:membership	ns20:e_aeseu ;
	skos:definition	"The sales have been realised, during the previous calendar year, via any computer networks (in monetary terms, excluding VAT). Computer networks include websites, EDI-type systems and other means of electronic data transfer, excluding manually typed e-mails." ;
	skos:note	"Enterprises with 10 or more persons employed. All manufacturing and service sectors, excluding the financial sector. Breaks in series because until 2008 economic activities according to NACE Rev 1.1 and from 2009 data are based on NACE Rev.2. Since 2010 data include also sector S 95.1-Repair of computers and communication equipment." ;
	skos:topConceptOf	ns1:indicator .
ns7:e_aws	rdf:type	ns10:Indicator ,
		skos:Concept ;
	skos:prefLabel	"Enterprises selling via a website or apps by geographical location of the costumer" ;
	dct:source	ns35: ;
	skos:notation	"e_aws" ;
	skos:altLabel	"Enterprises selling via a website or apps by geographical location " ;
	ns11:membership	ns20:e_aws ;
	skos:definition	"Share of the enterprises that, during the previous calendar year, received orders by costumers located in the own country, other EU countries or the rest of the world" ;
	skos:note	"Enterprises with 10 or more persons employed. All manufacturing and service sectors, excluding the financial sector. Breaks in series because until 2008 economic activities according to NACE Rev 1.1 and from 2009 data are based on NACE Rev.2. Since 2010 data include also sector S 95.1-Repair of computers and communication equipment." ;
	skos:topConceptOf	ns1:indicator .
ns7:e_aws_cmp	rdf:type	ns10:Indicator ,
		skos:Concept ;
	skos:prefLabel	"Enterprises using e-Commerce marketplace for sales" ;
	dct:source	ns35: ;
	skos:notation	"e_aws_cmp" ;
	skos:altLabel	"Enterprises selling via e-Commerce marketplace" ;
	ns11:membership	ns20:e_aws_cmp ;
	skos:definition	"Share of enterprises that, during the previous calendar year, received orders for goods or services via an e-Commerce marketplace" ;
	skos:note	"Enterprises with 10 or more persons employed. All manufacturing and service sectors, excluding the financial sector. Breaks in series because until 2008 economic activities according to NACE Rev 1.1 and from 2009 data are based on NACE Rev.2. Since 2010 data include also sector S 95.1-Repair of computers and communication equipment." ;
	skos:topConceptOf	ns1:indicator .
ns7:e_aws_cown	rdf:type	ns10:Indicator ,
		skos:Concept ;
	skos:prefLabel	"Enterprises using  their own website or apps for sales" ;
	dct:source	ns35: ;
	skos:notation	"e_aws_cown" ;
	skos:altLabel	"Enterprises selling via own website or apps" ;
	ns11:membership	ns20:e_aws_cown ;
	skos:definition	"Share of enterprises that, during the previous calendar year, received orders for goods or services via their own website or apps." ;
	skos:note	"Enterprises with 10 or more persons employed. All manufacturing and service sectors, excluding the financial sector. Breaks in series because until 2008 economic activities according to NACE Rev 1.1 and from 2009 data are based on NACE Rev.2. Since 2010 data include also sector S 95.1-Repair of computers and communication equipment." ;
	skos:topConceptOf	ns1:indicator .
ns7:e_aws_gt1_b2c_gt10ws	rdf:type	ns10:Indicator ,
		skos:Concept ;
	skos:prefLabel	"Enterprises exploiting the \"Business to Consumers\" opportunities of web sales" ;
	dct:source	ns35:estat_isoc_ec_eseln2 ;
	skos:notation	"e_aws_gt1_b2c_gt10ws" ;
	skos:altLabel	"Enterprises exploiting B2C opportunities of web sales " ;
	ns11:membership	ns20:e_aws_gt1_b2c_gt10ws ;
	skos:definition	"Enterprises where web sales are more than 1% of total turnover and B2C web sales more than 10% of the web sales" ;
	skos:note	"Enterprises with 10 or more persons employed. All manufacturing and service sectors, excluding the financial sector. Breaks in series because since 2010 data include also sector S 95.1-Repair of computers and communication equipment." ;
	skos:topConceptOf	ns1:indicator .
ns7:e_awsval_cmp	rdf:type	ns10:Indicator ,
		skos:Concept ;
	skos:prefLabel	"Sells via marketplace  as a pecentage of turnover" ;
	dct:source	ns35: ;
	skos:notation	"e_awsval_cmp" ;
	skos:altLabel	"Sells via marketplace" ;
	ns11:membership	ns20:e_awsval_cmp ;
	skos:definition	"The value of sales made during the previous calendar year, via an e-Commerce marketplace in % of the total turnover value (in monetary terms, excluding VAT)." ;
	skos:note	"Enterprises with 10 or more persons employed. All manufacturing and service sectors, excluding the financial sector. Breaks in series because until 2008 economic activities according to NACE Rev 1.1 and from 2009 data are based on NACE Rev.2. Since 2010 data include also sector S 95.1-Repair of computers and communication equipment." ;
	skos:topConceptOf	ns1:indicator .
ns7:e_awsval_cown	rdf:type	ns10:Indicator ,
		skos:Concept ;
	skos:prefLabel	"Sells via own website or apps as a pecentage of turnover" ;
	dct:source	ns35: ;
	skos:notation	"e_awsval_cown" ;
	skos:altLabel	"Sells via own website or apps " ;
	ns11:membership	ns20:e_awsval_cown ;
	skos:definition	"The value of sales made during the previous calendar year, via their own website or apps in % of the total turnover value (in monetary terms, excluding VAT)." ;
	skos:note	"Enterprises with 10 or more persons employed. All manufacturing and service sectors, excluding the financial sector. Breaks in series because until 2008 economic activities according to NACE Rev 1.1 and from 2009 data are based on NACE Rev.2. Since 2010 data include also sector S 95.1-Repair of computers and communication equipment." ;
	skos:topConceptOf	ns1:indicator .
ns7:e_bd	rdf:type	ns10:Indicator ,
		skos:Concept ;
	skos:prefLabel	"Enterprises analysing big data from any data source" ;
	dct:source	ns35:estat-ent ;
	skos:notation	"e_bd" ;
	skos:altLabel	"Enterprises analysing big data from any data source" ;
	ns11:membership	ns19:e_bd ;
	skos:definition	"Analyse big data from any data source" ;
	skos:topConceptOf	ns1:indicator .
ns7:e_broad	rdf:type	ns10:Indicator ,
		skos:Concept ;
	skos:prefLabel	"Enterprises having a fixed broadband connection" ;
	dct:source	ns35:estat_isoc_ci_eu_en2 ;
	skos:notation	"e_broad" ;
	skos:altLabel	"Enterprises with a fixed broadband connection" ;
	ns11:membership	ns15:e_broad ;
	skos:definition	"Fixed broadband connections include DSL, xDSL, cable leased lines, Frame Relay, Metro-Ethernet, PLC-Powerline communications, fixed wireless connections, etc." ;
	skos:note	"Enterprises with 10 or more persons employed. All manufacturing and service sectors, excluding the financial sector. Breaks in series because until 2008 economic activities according to NACE Rev 1.1 and from 2009 data are based on NACE Rev.2. Since 2010 data include also sector S 95.1-Repair of computers and communication equipment." ;
	skos:topConceptOf	ns1:indicator .
ns7:e_cc	rdf:type	ns10:Indicator ,
		skos:Concept ;
	skos:prefLabel	"Buy Cloud Computing services used over the internet" ;
	dct:source	ns35:estat_isoc_cicce_use ;
	skos:notation	"e_cc" ;
	skos:altLabel	"Cloud computing services (any)" ;
	ns11:membership	ns19:e_cc ;
	skos:definition	"Cloud computing refers to purchased ICT services that have all of the following characteristics: are delivered from servers of service providers; can be easily scaled up or down; can be used on-demand by the user without human interaction with the service provider; are paid for, either per user, by capacity used, or they are pre-paid.Eurostat variable e_cc_ge_me" ;
	skos:note	"Cloud computing may include connections via Virtual Private Networks (VPN). Optional question in 2015, not all countries have collected the indicator." ;
	skos:topConceptOf	ns1:indicator .
ns7:e_cc_ge_me	rdf:type	ns10:Indicator ,
		skos:Concept ;
	skos:prefLabel	"Buy Cloud Computing services of medium-high sophistication" ;
	dct:source	ns35:estat_isoc_cicce_use ;
	skos:notation	"e_cc_ge_me" ;
	skos:altLabel	"Cloud computing services (medium-high sophistication)" ;
	ns11:membership	ns19:e_cc_ge_me ;
	skos:definition	"Enterprises purchasing at least one of the following cloud computing services: hosting of the enterprise's database, accounting software applications, CRM software, computing power." ;
	skos:note	"Computed from Eurostat database with the following formula = (e_cc_me) - (e_cc_lo) + (e_cc_hi). Optional question in 2015, not all countries have collected the indicator." ;
	skos:topConceptOf	ns1:indicator .
ns7:e_cc_pcpu	rdf:type	skos:Concept ,
		ns10:Indicator ;
	skos:prefLabel	"Enterprises buying computing power in the Cloud" ;
	dct:source	ns35:estat_isoc_ci_eu_en2 ;
	skos:notation	"e_cc_pcpu" ;
	skos:altLabel	"Enterprises buying computing power to run own software in the Cloud" ;
	ns11:membership	ns19:e_cc_pcpu ;
	skos:definition	"Cloud computing refers to purchased ICT services that have all of the following characteristics: are delivered from servers of service providers; can be easily scaled up or down; can be used on-demand by the user without human interaction with the service provider; are paid for, either per user, by capacity used, or they are pre-paid." ;
	skos:note	"Optional question in 2015, not all countries have collected the indicator." ;
	skos:topConceptOf	ns1:indicator .
ns7:e_crman	rdf:type	skos:Concept ,
		ns10:Indicator ;
	skos:prefLabel	"Enterprises using Customer Relationship Management (CRM) software" ;
	dct:source	ns35:estat_isoc_bde15dec ;
	skos:notation	"e_crman" ;
	skos:altLabel	"Use of analytical CRM software" ;
	ns11:membership	ns19:e_crman ;
	skos:definition	"CRM refers to the use of any software application used for the analysis of information about clients for marketing purposes." ;
	skos:note	"Enterprises with 10 or more persons employed. All manufacturing and service sectors, excluding the financial sector. Breaks in series because until 2008 economic activities according to NACE Rev 1.1 and from 2009 data are based on NACE Rev.2. Since 2010 data include also sector S 95.1-Repair of computers and communication equipment." ;
	skos:topConceptOf	ns1:indicator .
ns7:e_di_hivhi	rdf:type	skos:Concept ,
		ns10:Indicator ;
	skos:prefLabel	"Enterprises with High levels of Digital Intensity" ;
	dct:source	ns35:estat-ent ;
	skos:notation	"e_di_hivhi" ;
	skos:altLabel	"Enterprises with High levels of Digital Intensity" ;
	ns11:membership	ns19:e_di_hivhi ;
	skos:definition	"The Digital Intensity score is based on counting how many out of 12 technologies are used by each enterprise. High levels are attributed to those enterprises using at least 7 of the listed digital technologies." ;
	skos:note	"The 2015 list of technologies includes: usage of internet by a majority of the workers; access to ICT specialist skills; fixed broadband speed > 30 Mbps; mobile devices used by more than 20% of employed persons; has a website; has some sophisticated functions on the website; presence on social media; does e-sales for at least 1% of turnover; exploit the B2C opportunities of web sales; use an ERP software; use a CRM software; share electronically supply chain management information.\r\nIn 2016 the last 3 indicators have been replaced with: pay to advertise on the internet; purchase cloud computing advanced services; send eInvoices. There is thus a break in series with in general a reduction of the digital intensity scores." ;
	skos:topConceptOf	ns1:indicator .
ns7:e_di_vlo	rdf:type	skos:Concept ,
		ns10:Indicator ;
	skos:prefLabel	"Enterprises with Very Low level of Digital Intensity" ;
	dct:source	ns35:estat-ent ;
	skos:notation	"e_di_vlo" ;
	skos:altLabel	"Enterprises with Very Low level of Digital Intensity" ;
	ns11:membership	ns19:e_di_vlo ;
	skos:definition	"The Digital Intensity score is based on counting how many out of 12 technologies are used by each enterprise. Very Low levels are attributed to those enterprises using no more than 3 of the listed digital technologies." ;
	skos:note	"The 2015 list of technologies includes: usage of internet by a majority of the workers; access to ICT specialist skills; fixed broadband speed > 30 Mbps; mobile devices used by more than 20% of employed persons; has a website; has some sophisticated functions on the website; presence on social media; does e-sales for at least 1% of turnover; exploit the B2C opportunities of web sales; use an ERP software; use a CRM software; share electronically supply chain management information.\r\nIn 2016 the last 3 indicators have been replaced with: pay to advertise on the internet; purchase cloud computing advanced services; send eInvoices. There is thus a break in series with in general a reduction of the digital intensity scores." ;
	skos:topConceptOf	ns1:indicator .
ns7:e_ebuy	rdf:type	skos:Concept ,
		ns10:Indicator ;
	skos:prefLabel	"Enterprises using any computer network for purchases (at least 1%)" ;
	dct:source	ns35:estat_isoc_bde15dec ;
	skos:notation	"e_ebuy" ;
	skos:altLabel	"Enterprises purchasing online" ;
	ns11:membership	ns18:e_ebuy ;
	skos:definition	"The purchases realised, during the previous calendar year, via any computer networks should represent at least 1% of the total purchases value (in monetary terms, excluding VAT). Computer networks include websites, EDI-type systems and other means of electronic data transfer, excluding manually typed e-mails." ;
	skos:note	"Since 2011 the indicator is optional, so EU27 estimates cover less countries and are not comparable with previous years. Enterprises with 10 or more persons employed. All manufacturing and service sectors, excluding the financial sector. Breaks in series because until 2008 economic activities according to NACE Rev 1.1 and from 2009 data are based on NACE Rev.2. Since 2010 data include also sector S 95.1-Repair of computers and communication equipment." ;
	skos:topConceptOf	ns1:indicator .
ns7:e_empmd_gt20	rdf:type	skos:Concept ,
		ns10:Indicator ;
	skos:prefLabel	"Enterprises providing portable devices to more than 20% of their employed persons" ;
	dct:source	ns35:estat_isoc_bde15b_e ;
	skos:notation	"e_empmd_gt20" ;
	skos:altLabel	"Enterprises providing portable devices to > 20% of their employed persons" ;
	ns11:membership	ns19:e_empmd_gt20 ;
	skos:definition	"The devices (portable computers, tablets, smartphones, PDA phones, etc.) should be provided for business use and the enterprises pay for all or at least up to a limit the subscription and the use costs." ;
	skos:note	"Only the 2011 question was limited to portable devices using at least 3G technology to connect to the internet. Enterprises with 10 or more persons employed. All manufacturing and service sectors, excluding the financial sector." ;
	skos:topConceptOf	ns1:indicator .
ns7:e_erp1	rdf:type	skos:Concept ,
		ns10:Indicator ;
	skos:prefLabel	"Enterprises that share internally electronic information with an ERP" ;
	dct:source	ns35:estat_isoc_bde15dip ;
	skos:notation	"e_erp1" ;
	skos:altLabel	"Integration of internal processes (with an ERP)" ;
	ns11:membership	ns19:e_erp1 ;
	skos:definition	"Have in use an ERP-Enterprise resource planning software package, to share information between different functional areas (e.g. accounting, planning, production, marketing)." ;
	skos:note	"Enterprises with 10 or more persons employed. All manufacturing and service sectors, excluding the financial sector. Breaks in series because until 2008 economic activities according to NACE Rev 1.1 and from 2009 data are based on NACE Rev.2. Since 2010 data include also sector S 95.1-Repair of computers and communication equipment. Break in series in 2012 due to different wording of the question." ;
	skos:topConceptOf	ns1:indicator .
ns7:e_esell	rdf:type	skos:Concept ,
		ns10:Indicator ;
	skos:prefLabel	"Enterprises using any computer network for sales (at least 1%)" ;
	dct:source	ns35:estat_isoc_ec_eseln2 ;
	skos:notation	"e_esell" ;
	skos:altLabel	"Enterprises selling online" ;
	ns11:membership	ns20:e_esell ;
	skos:definition	"The sales realised, during the previous calendar year, via any computer networks should represent at least 1% of the total turnover value (in monetary terms, excluding VAT). Computer networks include websites, EDI-type systems and other means of electronic data transfer, excluding manually typed e-mails." ;
	skos:note	"Enterprises with 10 or more persons employed. All manufacturing and service sectors, excluding the financial sector. Breaks in series because until 2008 economic activities according to NACE Rev 1.1 and from 2009 data are based on NACE Rev.2. Since 2010 data include also sector S 95.1-Repair of computers and communication equipment." ;
	skos:topConceptOf	ns1:indicator .
ns7:e_eturn	rdf:type	skos:Concept ,
		ns10:Indicator ;
	skos:prefLabel	"Total electronic sales by enterprises, as a % of their total turnover" ;
	dct:source	ns35:estat_isoc_ci_eu_en2 ;
	skos:notation	"e_eturn" ;
	skos:altLabel	"Turnover from eCommerce" ;
	ns11:membership	ns20:e_eturn ;
	skos:definition	"The value of sales realised, during the previous calendar year, via any computer networks in % of the total turnover value (in monetary terms, excluding VAT). Computer networks include websites, EDI-type systems and other means of electronic data transfer, excluding manually typed e-mails." ;
	skos:note	"Enterprises with 10 or more persons employed. All manufacturing and service sectors, excluding the financial sector. Breaks in series because until 2008 economic activities according to NACE Rev 1.1 and from 2009 data are based on NACE Rev.2. Since 2010 data include also sector S 95.1-Repair of computers and communication equipment." ;
	skos:topConceptOf	ns1:indicator .
ns7:e_gov_1_ucg	rdf:type	skos:Concept ,
		ns10:Indicator ;
	skos:prefLabel	"1 User Centricity" ;
	dct:source	ns35:egov_bench12_17 ;
	skos:notation	"e_gov_1_ucg" ;
	skos:altLabel	"1 User Centricity" ;
	ns11:membership	ns21:e_gov_1_ucg ;
	skos:definition	"The extent to which (information about) a public service is provided online, how the online journey is supported and if public websites are mobile friendly." ;
	skos:note	"Composite indicator:\n(2016-2017) weighted average of Online availability (67%), Usability (22%) and Mobile Friendliness (11%).\n(2012-2015) weighted average of Online availability (67%), Usability (17%), Ease of Use (8%) and Speed of Use (8%)\nBreak in series in 2016 (no data displayed for breakdown:Total 2016)." ;
	skos:topConceptOf	ns1:indicator .
ns7:e_gov_1a_ucg_oa	rdf:type	skos:Concept ,
		ns10:Indicator ;
	skos:prefLabel	"1a User Centricity - Online availability" ;
	dct:source	ns35:egov_bench12_17 ;
	skos:notation	"e_gov_1a_ucg_oa" ;
	skos:altLabel	"1a User Centricity - Online availability" ;
	ns11:membership	ns21:e_gov_1a_ucg_oa ;
	skos:definition	"The extent to which a Public Service or information concerning the public service is provided online, and via a portal." ;
	skos:topConceptOf	ns1:indicator .
ns7:e_gov_1b_ucg_us	rdf:type	skos:Concept ,
		ns10:Indicator ;
	skos:prefLabel	"1b User Centricity - Usability" ;
	dct:source	ns35:egov_bench12_17 ;
	skos:notation	"e_gov_1b_ucg_us" ;
	skos:altLabel	"1b User Centricity - Usability" ;
	ns11:membership	ns21:e_gov_1b_ucg_us ;
	skos:definition	"Indicates if support, help and (interactive) feedback functionalities for the online public service are available." ;
	skos:topConceptOf	ns1:indicator .
ns7:e_gov_1c_ucg_mf	rdf:type	skos:Concept ,
		ns10:Indicator ;
	skos:prefLabel	"1c User Centricity - Mobile Friendliness" ;
	dct:source	ns35:egov_bench12_17 ;
	skos:notation	"e_gov_1c_ucg_mf" ;
	skos:altLabel	"1c User Centricity - Mobile Friendliness" ;
	ns11:membership	ns21:e_gov_1c_ucg_mf ;
	skos:definition	"The ability to provide public services through a mobile-friendly interface; an interface that is \u2018adapted\u2019 to the mobile device. The data collection for this indicator is done via an automated tool. " ;
	skos:note	"The new key enabler \u201CMobile Friendliness\u201D was introduced in 2016. Mobile friendliness was also measured in 2014 and 2015 as proof-of-concept indicator. It was not part of the calculation of the User Centricity Benchmark in those years, but presented as separate index. In 2016, mobile friendliness of both individual services\u2019 websites as well as generic portals is integrated as a component of the Online Usability and User Centricity composite indicators." ;
	skos:topConceptOf	ns1:indicator .
ns7:e_gov_1d_ucg_eu	rdf:type	skos:Concept ,
		ns10:Indicator ;
	skos:prefLabel	"1d User Centricity - Ease of Use" ;
	dct:source	ns35:egov_bench12_17 ;
	skos:notation	"e_gov_1d_ucg_eu" ;
	skos:altLabel	"1d User Centricity - Ease of Use" ;
	ns11:membership	ns21:e_gov_1d_ucg_eu ;
	skos:definition	"Quality assessment by researchers indicating how intuitively and smoothly the online process steps for obtaining a public service can be completed.  It assesses  the extent to which the user achieved his/her goal, understood what he/she was supposed to do for obtaining the service, he/she found the succession of the process steps logical and he/she was actively engaged to improve the service." ;
	skos:note	"This indicator has been discontinued starting from 2016" ;
	skos:topConceptOf	ns1:indicator .
ns7:e_gov_1e_ucg_su	rdf:type	skos:Concept ,
		ns10:Indicator ;
	skos:prefLabel	"1e User Centricity - Speed of Use" ;
	dct:source	ns35:egov_bench12_17 ;
	skos:notation	"e_gov_1e_ucg_su" ;
	skos:altLabel	"1e User Centricity - Speed of Use" ;
	ns11:membership	ns21:e_gov_1e_ucg_su ;
	skos:definition	"Quality assessment researchers indicating if  the online process steps for obtaining a public service could be completed within reasonable amount of time. It assesses the extent to which citizens or businesses are able to submit information to the authority (or information was pre-filled), the time needed to obtain the service and the extent to which the services were structured efficiently.  " ;
	skos:note	"This indicator has been discontinued starting from 2016" ;
	skos:topConceptOf	ns1:indicator .
ns7:e_gov_2_tg	rdf:type	skos:Concept ,
		ns10:Indicator ;
	skos:prefLabel	"2 Transparency" ;
	dct:source	ns35:egov_bench12_17 ;
	skos:notation	"e_gov_2_tg" ;
	skos:altLabel	"2 Transparency" ;
	ns11:membership	ns21:e_gov_2_tg ;
	skos:definition	"The extent to which governments are transparent with regard to:\na) the process of public service delivery\nb) their own responsibilities and performance\nc) the personal data involved in service delivery\nThis top-level benchmark evaluates the transparency of government authorities\u2019 operations, service delivery procedures as well as with regard to the consultation of personal data by public administrations." ;
	skos:note	"Composite indicator: simple average of (Transparency) Service Delivery, Public Organisations and Personal Data" ;
	skos:topConceptOf	ns1:indicator .
ns7:e_gov_2a_tg_sd	rdf:type	ns10:Indicator ,
		skos:Concept ;
	skos:prefLabel	"2a Transparency - Service delivery" ;
	dct:source	ns35:egov_bench12_17 ;
	skos:notation	"e_gov_2a_tg_sd" ;
	skos:altLabel	"2a Transparency - Service delivery" ;
	ns11:membership	ns21:e_gov_2a_tg_sd ;
	skos:definition	"The extent to which public administrations inform users about the public service itself, setting expectations on timeliness, process and delivery for citizens and entrepreneurs from the moment a user request a service until the service is delivered." ;
	skos:topConceptOf	ns1:indicator .
ns7:e_gov_2b_tg_po	rdf:type	ns10:Indicator ,
		skos:Concept ;
	skos:prefLabel	"2b Transparency - Public organisations" ;
	dct:source	ns35:egov_bench12_17 ;
	skos:notation	"e_gov_2b_tg_po" ;
	skos:altLabel	"2b Transparency - Public organisations" ;
	ns11:membership	ns21:e_gov_2b_tg_po ;
	skos:definition	"The extent to which public administrations publish information about their organisations (e.g. finance, organisational structure and responsibilities), and about their activities (e.g. the decision-making processes and regulations). " ;
	skos:topConceptOf	ns1:indicator .
ns7:e_gov_2c_tg_pd	rdf:type	ns10:Indicator ,
		skos:Concept ;
	skos:prefLabel	"2c Transparency - Personal data" ;
	dct:source	ns35:egov_bench12_17 ;
	skos:notation	"e_gov_2c_tg_pd" ;
	skos:altLabel	"2c Transparency - Personal data" ;
	ns11:membership	ns21:e_gov_2c_tg_pd ;
	skos:definition	"The extent to which governments proactively inform users about how, when, and by whom their personal data is being processed" ;
	skos:note	"In 2016, an additional question was added to the questionnaire for this indicator." ;
	skos:topConceptOf	ns1:indicator .
ns7:e_gov_3_cm	rdf:type	ns10:Indicator ,
		skos:Concept ;
	skos:prefLabel	"3 Citizen Mobility" ;
	dct:source	ns35:egov_bench12_17 ;
	skos:notation	"e_gov_3_cm" ;
	skos:altLabel	"3 Citizen Mobility" ;
	ns11:membership	ns21:e_gov_3_cm ;
	skos:definition	"The extent to which public services that are aimed at foreign  citizens are available online, usable, and implement eID and eDocument capabilities" ;
	skos:note	"Composite indicator:\n(2016-2017) weighted average of (Citizen Mobility) Online Availability (50%), Usability (25%), eID Cross Borders (12%) and eDocuments Cross Borders (12%).\n(2012-2015) weighted average of (Citizen Mobility) Online Availability (67%), Usability (17%), Ease of Use (8%) and Speed of Use (8%)\nBreak in series in 2016 (no data displayed for breakdown:Total 2016)." ;
	skos:topConceptOf	ns1:indicator .
ns7:e_gov_3a_cm_oa	rdf:type	ns10:Indicator ,
		skos:Concept ;
	skos:prefLabel	"3a Citizen Mobility - Online availability" ;
	dct:source	ns35:egov_bench12_17 ;
	skos:notation	"e_gov_3a_cm_oa" ;
	skos:altLabel	"3a Citizen Mobility - Online availability" ;
	ns11:membership	ns21:e_gov_3a_cm_oa ;
	skos:definition	"The extent to which a public service (or information concerning the service) aimed at foreign citizens  is available online." ;
	skos:topConceptOf	ns1:indicator .
ns7:e_gov_3b_cm_us	rdf:type	ns10:Indicator ,
		skos:Concept ;
	skos:prefLabel	"3b Citizen Mobility - Usability" ;
	dct:source	ns35:egov_bench12_17 ;
	skos:notation	"e_gov_3b_cm_us" ;
	skos:altLabel	"3b Citizen Mobility - Usability" ;
	ns11:membership	ns21:e_gov_3b_cm_us ;
	skos:definition	"Online support and help features on services aimed at foreign citizens." ;
	skos:topConceptOf	ns1:indicator .
ns7:e_gov_3c_cm_eidcb	rdf:type	ns10:Indicator ,
		skos:Concept ;
	skos:prefLabel	"3c Citizen Mobility - eID Cross Borders" ;
	dct:source	ns35:egov_bench12_17 ;
	skos:notation	"e_gov_3c_cm_eidcb" ;
	skos:altLabel	"3c Citizen Mobility - eID Cross Borders" ;
	ns11:membership	ns21:e_gov_3c_cm_eidcb ;
	skos:definition	"The possibility of using a foreign eID for accessing citizen services." ;
	skos:note	"New indicator, introduced in 2016." ;
	skos:topConceptOf	ns1:indicator .
ns7:e_gov_3d_cm_edoccb	rdf:type	ns10:Indicator ,
		skos:Concept ;
	skos:prefLabel	"3d Citizen Mobility - eDocuments Cross Borders" ;
	dct:source	ns35:egov_bench12_17 ;
	skos:notation	"e_gov_3d_cm_edoccb" ;
	skos:altLabel	"3d Citizen Mobility - eDocuments Cross Borders" ;
	ns11:membership	ns21:e_gov_3d_cm_edoccb ;
	skos:definition	"The possibility of sending/receiving eDocuments for a foreigner using citizen services" ;
	skos:note	"New indicator, introduced in 2016." ;
	skos:topConceptOf	ns1:indicator .
ns7:e_gov_3e_cm_eu	rdf:type	ns10:Indicator ,
		skos:Concept ;
	skos:prefLabel	"3e Citizen Mobility - Ease of Use" ;
	dct:source	ns35:egov_bench12_17 ;
	skos:notation	"e_gov_3e_cm_eu" ;
	skos:altLabel	"3e Citizen Mobility - Ease of Use" ;
	ns11:membership	ns21:e_gov_3e_cm_eu ;
	skos:definition	"Quality assessment by researchers indicating how intuitively and smoothly the online process steps for obtaining a public service can be completed by a foreign citizen.  It assesses  the extent to which the user achieved his/her goal, understood what he/she was supposed to do for obtaining the service, he/she found the succession of the process steps logical and he/she was actively engaged to improve the service." ;
	skos:note	"This indicator has been discontinued starting from 2016" ;
	skos:topConceptOf	ns1:indicator .
ns7:e_gov_3f_cm_su	rdf:type	ns10:Indicator ,
		skos:Concept ;
	skos:prefLabel	"3f Citizen Mobility - Speed of Use" ;
	dct:source	ns35:egov_bench12_17 ;
	skos:notation	"e_gov_3f_cm_su" ;
	skos:altLabel	"3f Citizen Mobility - Speed of Use" ;
	ns11:membership	ns21:e_gov_3f_cm_su ;
	skos:definition	"Quality assessment researchers indicating if  the online process steps for obtaining a public service could be completed within reasonable amount of time by a foreign citizen. It assesses the extent to which (foreign) citizens are able to submit information to the authority (or information was pre-filled), the time needed to obtain the service and the extent to which the services were structured efficiently.  " ;
	skos:note	"This indicator has been discontinued starting from 2016" ;
	skos:topConceptOf	ns1:indicator .
ns7:e_gov_4_bm	rdf:type	ns10:Indicator ,
		skos:Concept ;
	skos:prefLabel	"4 Business Mobility" ;
	dct:source	ns35:egov_bench12_17 ;
	skos:notation	"e_gov_4_bm" ;
	skos:altLabel	"4 Business Mobility" ;
	ns11:membership	ns21:e_gov_4_bm ;
	skos:definition	"The extent to which public services that are aimed at foreign  businesses are available online, usable, and implement eID and eDocument capabilities" ;
	skos:note	"Composite indicator:\n(2016-2017) weighted average of (Business Mobility) Online Availability (50%), Usability (25%), eID Cross Borders (12%) and eDocuments Cross Borders (12%).\n(2012-2015) weighted average of (Business Mobility) Online Availability (67%), Usability (17%), Ease of Use (8%) and Speed of Use (8%)\nBreak in series in 2016 (no data displayed for breakdown:Total 2016)." ;
	skos:topConceptOf	ns1:indicator .
ns7:e_gov_4a_bm_oa	rdf:type	ns10:Indicator ,
		skos:Concept ;
	skos:prefLabel	"4a Business Mobility - Online availability" ;
	dct:source	ns35:egov_bench12_17 ;
	skos:notation	"e_gov_4a_bm_oa" ;
	skos:altLabel	"4a Business Mobility - Online availability" ;
	ns11:membership	ns21:e_gov_4a_bm_oa ;
	skos:definition	"The extent to which a public service (or information concerning the service) aimed at foreign businesses  is available online." ;
	skos:topConceptOf	ns1:indicator .
ns7:e_gov_4c_bm_eidcb	rdf:type	ns10:Indicator ,
		skos:Concept ;
	skos:prefLabel	"4c Business Mobility - eID Cross Borders" ;
	dct:source	ns35:egov_bench12_17 ;
	skos:notation	"e_gov_4c_bm_eidcb" ;
	skos:altLabel	"4e Business Mobility - eID Cross Borders" ;
	ns11:membership	ns21:e_gov_4c_bm_eidcb ;
	skos:definition	"The possibility of using a foreign eID for accessing business services." ;
	skos:note	"New indicator, introduced in 2016." ;
	skos:topConceptOf	ns1:indicator .
ns7:e_gov_4d_bm_edoccb	rdf:type	ns10:Indicator ,
		skos:Concept ;
	skos:prefLabel	"4d Business Mobility - eDocuments Cross Borders" ;
	dct:source	ns35:egov_bench12_17 ;
	skos:notation	"e_gov_4d_bm_edoccb" ;
	skos:altLabel	"4f Business Mobility - eDocuments Cross Borders" ;
	ns11:membership	ns21:e_gov_4d_bm_edoccb ;
	skos:definition	"The possibility of sending/receiving eDocuments for a foreigner using business services" ;
	skos:note	"New indicator, introduced in 2016." ;
	skos:topConceptOf	ns1:indicator .
ns7:e_gov_4e_bm_eu	rdf:type	ns10:Indicator ,
		skos:Concept ;
	skos:prefLabel	"4e Business Mobility - Ease of Use" ;
	dct:source	ns35:egov_bench12_17 ;
	skos:notation	"e_gov_4e_bm_eu" ;
	skos:altLabel	"4g Business Mobility - Ease of Use" ;
	ns11:membership	ns21:e_gov_4e_bm_eu ;
	skos:definition	"Quality assessment by researchers indicating how intuitively and smoothly the online process steps for obtaining a public service can be completed by a foreign business.  It assesses  the extent to which the user achieved his/her goal, understood what he/she was supposed to do for obtaining the service, he/she found the succession of the process steps logical and he/she was actively engaged to improve the service." ;
	skos:note	"This indicator has been discontinued starting from 2016" ;
	skos:topConceptOf	ns1:indicator .
ns7:e_gov_4f_bm_su	rdf:type	ns10:Indicator ,
		skos:Concept ;
	skos:prefLabel	"4f Business Mobility - Speed of Use" ;
	dct:source	ns35:egov_bench12_17 ;
	skos:notation	"e_gov_4f_bm_su" ;
	skos:altLabel	"4h Business Mobility - Speed of Use" ;
	ns11:membership	ns21:e_gov_4f_bm_su ;
	skos:definition	"Quality assessment researchers indicating if  the online process steps for obtaining a public service could be completed within reasonable amount of time by a foreign business. It assesses the extent to which (foreign) businesses are able to submit information to the authority (or information was pre-filled), the time needed to obtain the service and the extent to which the services were structured efficiently.  " ;
	skos:note	"This indicator has been discontinued starting from 2016" ;
	skos:topConceptOf	ns1:indicator .
ns7:e_gov_5_ke	rdf:type	skos:Concept ,
		ns10:Indicator ;
	skos:prefLabel	"5 Key Enablers" ;
	dct:source	ns35:egov_bench12_17 ;
	skos:notation	"e_gov_5_ke" ;
	skos:altLabel	"5 Key Enablers" ;
	ns11:membership	ns21:e_gov_5_ke ;
	skos:definition	"The extent to which technical pre-conditions for eGovernment service provision are used. The key enablers used for measuring the quality of the services to businesses and citizens are:\na) Electronic Identification (eID)\nb) Electronic Documents (eDocuments)\nc) Authentic Sources\nd) Digital Post\ne) eSafe (now discontinued)\nf) Single Sign On (SSO) (now discontinued)" ;
	skos:note	"Composite indicator:\n(2016-2017) simple average of eID, eDocuments, Authentic Sources and Digital Post.\n(2012-2015) simple average of eID, eDocuments, Authentic Sources, eSafe and Single Sign On.\nBreak in series in 2016 as the  eSafe and Single Sign On are discontinued and Digital Post is added." ;
	skos:topConceptOf	ns1:indicator .
ns7:e_gov_5a_ke_eid	rdf:type	skos:Concept ,
		ns10:Indicator ;
	skos:prefLabel	"5a Key Enablers - eID" ;
	dct:source	ns35:egov_bench12_17 ;
	skos:notation	"e_gov_5a_ke_eid" ;
	skos:altLabel	"5a Key Enablers - eID" ;
	ns11:membership	ns21:e_gov_5a_ke_eid ;
	skos:definition	"Electronic Identification (eID) is a government-issued document for online identification, and authentication." ;
	skos:topConceptOf	ns1:indicator .
ns7:e_gov_5b_ke_edoc	rdf:type	skos:Concept ,
		ns10:Indicator ;
	skos:prefLabel	"5b Key Enablers - eDocuments" ;
	dct:source	ns35:egov_bench12_17 ;
	skos:notation	"e_gov_5b_ke_edoc" ;
	skos:altLabel	"5b Key Enablers - eDocuments" ;
	ns11:membership	ns21:e_gov_5b_ke_edoc ;
	skos:definition	"A document which has been authenticated by its issuer using any means recognised under applicable national law, specifically through the use of electronic signatures, e.g. not a regular pdf or word document." ;
	skos:topConceptOf	ns1:indicator .
ns7:e_gov_5c_ke_as	rdf:type	skos:Concept ,
		ns10:Indicator ;
	skos:prefLabel	"5c Key Enablers - Authentic sources" ;
	dct:source	ns35:egov_bench12_17 ;
	skos:notation	"e_gov_5c_ke_as" ;
	skos:altLabel	"5c Key Enablers - Authentic sources" ;
	ns11:membership	ns21:e_gov_5c_ke_as ;
	skos:definition	"Authentic Sources are base registries used by governments to automatically validate or fetch data relating to citizens or businesses." ;
	skos:topConceptOf	ns1:indicator .
ns7:e_gov_5d_ke_dp	rdf:type	skos:Concept ,
		ns10:Indicator ;
	skos:prefLabel	"5d Key Enablers - Digital Post" ;
	dct:source	ns35:egov_bench12_17 ;
	skos:notation	"e_gov_5d_ke_dp" ;
	skos:altLabel	"5d Key Enablers - Digital Post" ;
	ns11:membership	ns21:e_gov_5d_ke_dp ;
	skos:definition	"Assesses whether public authorities allow citizens to receive communications digitally only, and hence reducing paper mailings. Digital Post refers to the possibility that governments communicate electronically-only with citizens or entrepreneurs through e.g. personal mailboxes or other digital post solutions." ;
	skos:note	"New indicator, introduced in 2016." ;
	skos:topConceptOf	ns1:indicator .
ns7:e_gov_5e_ke_esafe	rdf:type	skos:Concept ,
		ns10:Indicator ;
	skos:prefLabel	"5e Key Enablers - eSafe" ;
	dct:source	ns35:egov_bench12_17 ;
	skos:notation	"e_gov_5e_ke_esafe" ;
	skos:altLabel	"5e Key Enablers - eSafe" ;
	ns11:membership	ns21:e_gov_5e_ke_esafe ;
	skos:definition	"A virtual repository for storing, administering and sharing personal electronic data and documents. It can be used to securely store personal documents in public service processes." ;
	skos:note	"This indicator has been discontinued starting from 2016" ;
	skos:topConceptOf	ns1:indicator .
ns7:e_gov_5f_ke_sso	rdf:type	skos:Concept ,
		ns10:Indicator ;
	skos:prefLabel	"5f Key Enablers - Single Sign On (SSO)" ;
	dct:source	ns35:egov_bench12_17 ;
	skos:notation	"e_gov_5f_ke_sso" ;
	skos:altLabel	"5f Key Enablers - Single Sign On (SSO)" ;
	ns11:membership	ns21:e_gov_5f_ke_sso ;
	skos:definition	"A functionality that allows users to get access to multiple websites without the need to log in multiple times." ;
	skos:note	"This indicator has been discontinued starting from 2016" ;
	skos:topConceptOf	ns1:indicator .
ns7:e_gov_ke	rdf:type	skos:Concept ,
		ns10:Indicator ;
	skos:prefLabel	"Key Enablers" ;
	dct:source	ns35:egov_bench14 ;
	skos:notation	"e_gov_ke" ;
	skos:altLabel	"Key Enablers" ;
	ns11:membership	ns21:e_gov_ke ;
	skos:definition	"Availability of Key Enablers such as electronic Identification (eID), electronic Documents, Authentic Sources as well as Digital Post (newly introduced in 2017)" ;
	skos:note	"The degree to which key enablers (eID, eDocuments. Authentic sources, Digital Post) are available for interaction with public administration for the life events (Business, Family, Job, Studying)" ;
	skos:topConceptOf	ns1:indicator .
ns7:e_gov_opa	rdf:type	skos:Concept ,
		ns10:Indicator ;
	skos:prefLabel	"Openness of Public Administrations" ;
	dct:source	ns35:egov_bench15 ;
	skos:notation	"e_gov_opa" ;
	skos:altLabel	"Openness of Public Administrations" ;
	ns11:membership	ns21:e_gov_opa ;
	skos:definition	"Openness of Member States in regards to Open Data, freedom of expression, free media and freedom of association." ;
	skos:note	"Composed indicator made of open data (DESI) and voice and accountability (World Bank indicator)" ;
	skos:topConceptOf	ns1:indicator .
ns7:e_gov_osc	rdf:type	skos:Concept ,
		ns10:Indicator ;
	skos:prefLabel	"Online Service Completion" ;
	dct:source	ns35:e_gov_bench ;
	skos:notation	"e_gov_osc" ;
	skos:altLabel	"Online Service Completion" ;
	ns11:membership	ns21:e_gov_osc ;
	skos:definition	"Share of the steps in a Public Service life event that can be completed online (Online availability sub-indicator for User centricity of the eGovernment benchmark)" ;
	skos:note	"The indicator was measuring: Basic and Extended services for National services only till 2019. From 2020 the new indicator, \"Digital Public Services for Citizens\", was introduced. Together with the \"Digital Public Services for Business' they are fully covering the spectrum of online services. \nThe data was recalculated to include EU27 Average." ;
	skos:topConceptOf	ns1:indicator .
ns7:e_gov_pff	rdf:type	skos:Concept ,
		ns10:Indicator ;
	skos:prefLabel	"Pre-filled forms" ;
	dct:source	ns35:e_gov_bench ;
	skos:notation	"e_gov_pff" ;
	skos:altLabel	"Pre-filled forms" ;
	ns11:membership	ns21:e_gov_pff ;
	skos:definition	"Amount of data that is pre-filled in Public Services' online forms (Authentic sources Key Enabler indicator of eGovernment benchmark)" ;
	skos:note	"The data was recalculated to include EU27 Average." ;
	skos:topConceptOf	ns1:indicator .
ns7:e_igov	rdf:type	skos:Concept ,
		ns10:Indicator ;
	skos:prefLabel	"Enterprises interacting online with public authorities" ;
	dct:source	ns35:estat_isoc_bde15dec ;
	skos:notation	"e_igov" ;
	skos:altLabel	"Use of eGovernment services - enterprises" ;
	ns11:membership	ns18:e_igov ;
	skos:definition	"Use of internet for interaction with public authorities, in the last calendar year before the survey, includes: obtaining information or forms from websites, returning filled in forms, following administrative procedures completely electronically or offering products in public authorities' electronic procurement sustems (eTendering)." ;
	skos:note	"Enterprises with 10 or more persons employed, all manufacturing and service sectors, excluding the financial sector. Break in series in 2011 and 2012 because the structure of the question has changed. Breaks in series because until 2008 sectors follow economic activities according to NACE Rev 1.1 and from 2009 data are based on NACE Rev.2. Since 2010 data include also sector S 95.1-Repair of computers and communication equipment." ;
	skos:topConceptOf	ns1:indicator .
ns7:e_igov2pr	rdf:type	skos:Concept ,
		ns10:Indicator ;
	skos:prefLabel	"Enterprises submitting a proposal in a public electronic tender system (eProcurement)" ;
	dct:source	ns35:estat_isoc_bde15dec ;
	skos:notation	"e_igov2pr" ;
	skos:altLabel	"Use of eProcurement services - enterprises" ;
	ns11:membership	ns18:e_igov2pr ;
	skos:definition	" Tender proposals should have been submitted in the system itself and not by email, in the last calendar year before the survey. " ;
	skos:note	"Data from previous years are not comparable because the structure of the question has changed. Enterprises with 10 or more persons employed, carrying out this activity over the internet in the last calendar year before the survey. All manufacturing and service sectors, excluding the financial sector. " ;
	skos:topConceptOf	ns1:indicator .
ns7:e_igovrt	rdf:type	skos:Concept ,
		ns10:Indicator ;
	skos:prefLabel	"Enterprises returning filled in forms to public authorities, over the internet" ;
	dct:source	ns35:estat_isoc_bde15dec ;
	skos:notation	"e_igovrt" ;
	skos:altLabel	"Returning filled forms to eGov services - enterprises" ;
	ns11:membership	ns18:e_igovrt ;
	skos:definition	"Activity carried out over the internet, in the last calendar year before the survey." ;
	skos:note	"Enterprises with 10 or more persons employed. Break in series in 2011 and 2012 because the question has changed. All manufacturing and service sectors, excluding the financial sector. Breaks in series because until 2008 economic activities according to NACE Rev 1.1 and from 2009 data are based on NACE Rev.2. Since Since 2010 data include also sector S 95.1-Repair of computers and communication equipment." ;
	skos:topConceptOf	ns1:indicator .
ns7:e_inv	rdf:type	ns10:Indicator ,
		skos:Concept ;
	skos:prefLabel	"Enterprises sending or receiving e-invoices in a format suitable for automatic processing" ;
	dct:source	ns35:estat_isoc_bde15disc ;
	skos:notation	"e_inv" ;
	skos:altLabel	"Sending or receiving of e-Invoices" ;
	ns11:membership	ns18:e_inv ;
	skos:definition	"The indicator refers to sending/receiving invoices in an agreed standard format (as EDIFACT, XML, etc) which allows their automatic processing, without the individual message being manually typed" ;
	skos:note	"Important break in series due to a more detailed question since 2011. Enterprises with 10 or more persons employed. All manufacturing and service sectors, excluding the financial sector. Breaks in series because until 2008 economic activities according to NACE Rev 1.1 and from 2009 data are based on NACE Rev.2. Since 2010 data include also sector S 95.1-Repair of computers and communication equipment." ;
	skos:topConceptOf	ns1:indicator .
ns7:e_invsnd	rdf:type	ns10:Indicator ,
		skos:Concept ;
	skos:prefLabel	"Enterprises sending e-invoices (derived indicator)" ;
	dct:source	ns35:estat_isoc_bde15disc ;
	skos:notation	"e_invsnd" ;
	skos:altLabel	"Enterprises sending e-invoices" ;
	ns11:membership	ns19:e_invsnd ;
	skos:definition	"The indicator refers to sending invoices in an agreed standard format (as EDIFACT, XML, etc) which allows their automatic processing, without the individual message being manually typed. Eurostat variable e_inv3sbg_ap_gt0" ;
	skos:note	"Break in series in 2011 because of a new more precise question. Break in series in 2014 because of introduction of a limitation to invoices sent to business or public organisations." ;
	skos:topConceptOf	ns1:indicator .
ns7:e_ispdf_ge30	rdf:type	ns10:Indicator ,
		skos:Concept ;
	skos:prefLabel	"Enterprises having a fast fixed broadband connection" ;
	dct:source	ns35:estat_isoc_ci_eu_en2 ;
	skos:notation	"e_ispdf_ge30" ;
	skos:altLabel	"Enterprises having a fast fixed broadband connection" ;
	ns11:membership	ns15:e_ispdf_ge30 ;
	skos:definition	"The maximum contracted download speed of the fastest fixed internet connection is at least 30 Mb/s" ;
	skos:topConceptOf	ns1:indicator .
ns7:e_ispdfokx	rdf:type	ns10:Indicator ,
		skos:Concept ;
	skos:prefLabel	"The speed of the fixed connection to internet  is not sufficient for the actual needs of the enterprise" ;
	dct:source	ns35: ;
	skos:notation	"e_ispdfokx" ;
	skos:altLabel	"Internet fixed connection speed is not sufficient" ;
	ns11:membership	ns15:e_ispdfokx ;
	skos:definition	"Number of enterprises reporting that the speed of the fixed connection(s) to the internet is usually not sufficient for the actual  needs of the enterprise " ;
	skos:note	"Enterprises with 10 or more persons employed. All manufacturing and service sectors, excluding the financial sector. Breaks in series because until 2008 economic activities according to NACE Rev 1.1 and from 2009 data are based on NACE Rev.2. Since 2010 data include also sector S 95.1-Repair of computers and communication equipment." ;
	skos:topConceptOf	ns1:indicator .
ns7:e_ispdfokx_ge100	rdf:type	ns10:Indicator ,
		skos:Concept ;
	skos:prefLabel	"The speed of the fixed connection to internet (at least 100 Mb/s) is not sufficient for the actual needs of the enterprise" ;
	dct:source	ns35: ;
	skos:notation	"e_ispdfokx_ge100" ;
	skos:altLabel	"Internet fixed connection speed of 100Mb/s is not sufficient" ;
	ns11:membership	ns15:e_ispdfokx_ge100 ;
	skos:definition	"Number of enterprises reporting that the speed of the fixed connection(s) to the internet (at least 100 Mb/s) is usually not sufficient for the actual  needs of the enterprise " ;
	skos:note	"Enterprises with 10 or more persons employed. All manufacturing and service sectors, excluding the financial sector. Breaks in series because until 2008 economic activities according to NACE Rev 1.1 and from 2009 data are based on NACE Rev.2. Since 2010 data include also sector S 95.1-Repair of computers and communication equipment." ;
	skos:topConceptOf	ns1:indicator .
ns7:e_it_mext	rdf:type	ns10:Indicator ,
		skos:Concept ;
	skos:prefLabel	"Enterprises where ICT functions are mainly performed by external suppliers" ;
	dct:source	ns35:estat_isoc_ci_eu_en2 ;
	skos:notation	"e_it_mext" ;
	skos:altLabel	"Enterprises where ICT functions are mainly performed by external suppliers" ;
	ns11:membership	ns26:e_it_mext ;
	skos:definition	"The majority of ICT functions, out of a list of seven, are mainly performed by external suppliers and not by own employees or by ICT specialist in parent or affiliate enterprises. The functions include: maintenance of ICT infrastructures, support for office software, development and support for web solutions or business management software/systems (e.g. ERP, CRM, HR, databases), security and data protection." ;
	skos:note	"Detailed results are available in the Eurostat table <a href=\"http://appsso.eurostat.ec.europa.eu/nui/show.do?dataset=isoc_ci_eu_en2&lang=en\">ISOC_CI_EU_EN2</a>." ;
	skos:topConceptOf	ns1:indicator .
ns7:e_itsp2	rdf:type	ns10:Indicator ,
		skos:Concept ;
	skos:prefLabel	"Enterprises employing ICT specialists" ;
	dct:source	ns35:estat_isoc_ci_eu_en2 ;
	skos:notation	"e_itsp2" ;
	skos:altLabel	"Enterprises employing ICT specialists" ;
	ns11:membership	ns26:e_itsp2 ;
	skos:definition	"ICT specialists are employees for whom ICT is the main job. For example, to develop, operate or maintain ICT systems or applications." ;
	skos:note	"Limited comparability between 2007 and 2012 because of changes in the wording of the question. Enterprises with 10 or more persons employed. All manufacturing and service sectors, excluding the financial sector." ;
	skos:topConceptOf	ns1:indicator .
ns7:e_itspvac2	rdf:type	ns10:Indicator ,
		skos:Concept ;
	skos:prefLabel	"Enterprises reporting hard-to-fill vacancies for jobs requiring ICT specialist skills" ;
	dct:source	ns35:estat_isoc_ci_eu_en2 ;
	skos:notation	"e_itspvac2" ;
	skos:altLabel	"Enterprises reporting hard-to-fill vacancies for ICT specialist" ;
	ns11:membership	ns26:e_itspvac2 ;
	skos:definition	" Hard-to-fill vacancies during the previous calendar year refer to a range of situations in which enterprises find it difficult to find persons with particular skills (hard-to-fill vacancies due to skills shortage)." ;
	skos:note	"Limited comparability between 2007 and 2012 because of changes in the wording of the question. Enterprises with 10 or more persons employed. All manufacturing and service sectors, excluding the financial sector." ;
	skos:topConceptOf	ns1:indicator .
ns7:e_itt2	rdf:type	ns10:Indicator ,
		skos:Concept ;
	skos:prefLabel	"Enterprise provided training to their personnel to develop/upgrade their ICT skills" ;
	dct:source	ns35:estat_isoc_ske_ittn2 ;
	skos:notation	"e_itt2" ;
	skos:altLabel	"Enterprise provided training to their personnel to develop/upgrade their ICT skills" ;
	ns11:membership	ns26:e_itt2 ;
	skos:definition	"Detailed results are available in the Eurostat table <a href=\"http://appsso.eurostat.ec.europa.eu/nui/show.do?dataset=isoc_ske_ittn2&lang=en\">ISOC_SKE_ITTN2</a>." ;
	skos:topConceptOf	ns1:indicator .
ns7:e_pmd	rdf:type	ns10:Indicator ,
		skos:Concept ;
	skos:prefLabel	"Enterprises providing portable devices to some of their persons employed" ;
	dct:source	ns35:estat_isoc_bde15b_e ;
	skos:notation	"e_pmd" ;
	skos:altLabel	"Enterprises providing portable devices to persons employed" ;
	ns11:membership	ns29:e_pmd ;
	skos:definition	"The devices (portable computers, tablets, smartphones, PDA phones, etc.) should be provided for business use and the enterprises pay for all or at least up to a limit the subscription and the use costs." ;
	skos:note	"The 2011 question was limited to portable devices using at least 3G technology to connect to the internet. Enterprises with 10 or more persons employed. All manufacturing and service sectors, excluding the financial sector." ;
	skos:topConceptOf	ns1:indicator .
ns7:e_pmd_app	rdf:type	ns10:Indicator ,
		skos:Concept ;
	skos:prefLabel	"Enterprises using mobile Internet to run business applications" ;
	dct:source	ns35:estat-ent ;
	skos:notation	"e_pmd_app" ;
	skos:altLabel	"Enterprises using mobile Internet to run business applications" ;
	ns11:membership	ns19:e_pmd_app ;
	skos:definition	"Mobile connection to the Internet for business use to use dedicated business software applications" ;
	skos:topConceptOf	ns1:indicator .
ns7:e_ra	rdf:type	ns10:Indicator ,
		skos:Concept ;
	skos:prefLabel	"Enterprises providing persons employed a remote access to the enterprise's e-mail system, documents or applications" ;
	dct:source	ns35:estat-ent ;
	skos:notation	"e_ra" ;
	skos:altLabel	"Enterprises providing persons employed a remote access to the IT system" ;
	ns11:membership	ns19:e_ra ;
	skos:note	"Enterprises with 10 or more persons employed. All manufacturing and service sectors, excluding the financial sector." ;
	skos:topConceptOf	ns1:indicator .
ns7:e_rfac	rdf:type	ns10:Indicator ,
		skos:Concept ;
	skos:prefLabel	"Enterprises using RFID technologies for person identification or access control" ;
	dct:source	ns35:estat_isoc_bde15dth ;
	skos:notation	"e_rfac" ;
	skos:altLabel	"Enterprises using RFID for person identification or access control" ;
	ns11:membership	ns19:e_rfac ;
	skos:definition	"RFID tags or transponders are devices that can be applied to or incorporated into a product or object and transmits data via radiowaves." ;
	skos:topConceptOf	ns1:indicator .
ns7:e_rfid	rdf:type	ns10:Indicator ,
		skos:Concept ;
	skos:prefLabel	"Enterprises using Radio Frequency Identification (RFID) technologies" ;
	dct:source	ns35:estat_isoc_bde15dth ;
	skos:notation	"e_rfid" ;
	skos:altLabel	"Use of Radio Frequency Identification (RFID) technologies" ;
	ns11:membership	ns19:e_rfid ;
	skos:definition	"RFID tags or transponders are devices that can be applied to or incorporated into a product or object and transmits data via radiowaves. The indicator includes their use for person identification, for tracking of supply chain and inventory or for after-sales product identification." ;
	skos:note	"Enterprises with 10 or more persons employed. All manufacturing and service sectors, excluding the financial sector. Since 2010 data include also sector S95.1-Repair of computers and communication equipment. Biennial indicator not collected in 2010." ;
	skos:topConceptOf	ns1:indicator .
ns7:e_rfpsas	rdf:type	ns10:Indicator ,
		skos:Concept ;
	skos:prefLabel	"Enterprises using RFID for product identification" ;
	dct:source	ns35:estat_isoc_bde15dth ;
	skos:notation	"e_rfpsas" ;
	skos:altLabel	"Enterprises using RFID for product identification" ;
	ns11:membership	ns19:e_rfpsas ;
	skos:definition	"RFID tags or transponders are devices that can be applied to or incorporated into a product or object and transmits data via radiowaves. The indicator includes their use for tracking of supply chain and inventory or for after-sales product identification." ;
	skos:topConceptOf	ns1:indicator .
ns7:e_secpol1	rdf:type	ns10:Indicator ,
		skos:Concept ;
	skos:prefLabel	"Enterprises with a formally defined ICT security policy" ;
	dct:source	ns35:estat_isoc_ci_eu_en2 ;
	skos:notation	"e_secpol1" ;
	skos:altLabel	"Enterprises with a formally defined ICT security policy" ;
	ns11:membership	ns32:e_secpol1 ;
	skos:topConceptOf	ns1:indicator .
ns7:e_sisc	rdf:type	skos:Concept ,
		ns10:Indicator ;
	skos:prefLabel	"Enterprises sharing electronic information on the supply chain" ;
	dct:source	ns35:estat_isoc_bde15disc ;
	skos:notation	"e_sisc" ;
	skos:altLabel	"Electronic Supply Chain Management" ;
	ns11:membership	ns19:e_sisc ;
	skos:definition	"The indicator refers to sending/receiving all type of information on the supply chain (e.g. inventory levels, production plans, forecasts, progress of delivery) via computer networks or via websites, but excluding manually typed e-mail messages. " ;
	skos:note	"Enterprises with 10 or more persons employed. All manufacturing and service sectors, excluding the financial sector. Breaks in series because untill 2008 economic activities according to NACE Rev 1.1 and from 2009 data are based on NACE Rev.2. Since 2010 data include also sector 95.1-Repair of computers and communication equipment. Biennial indicator not collected in 2011." ;
	skos:topConceptOf	ns1:indicator .
ns7:e_sisorp	rdf:type	skos:Concept ,
		ns10:Indicator ;
	skos:prefLabel	"Enterprises that share internally electronic information on sales/purchases" ;
	dct:source	ns35:estat_isoc_bde15dec ;
	skos:notation	"e_sisorp" ;
	skos:altLabel	"Integration of internal processes (orders)" ;
	ns11:membership	ns18:e_sisorp ;
	skos:definition	"Information on sales/purchases is shared electronically and automatically with the software used for any internal function as: the management of inventory levels, the accounting system, the production management or the distribution management. " ;
	skos:note	"Enterprises with 10 or more persons employed. All manufacturing and service sectors, excluding the financial sector. Breaks in series because until 2008 economic activities according to NACE Rev 1.1 and from 2009 data are based on NACE Rev.2. Since 2010 data include also sector S 95.1-Repair of computers and communication equipment." ;
	skos:topConceptOf	ns1:indicator .
ns7:e_sm_any	rdf:type	skos:Concept ,
		ns10:Indicator ;
	skos:prefLabel	"Enterprises using social media" ;
	dct:source	ns35:estat_isoc_ci_eu_en2 ;
	skos:notation	"e_sm_any" ;
	skos:altLabel	"Enterprises using social media" ;
	ns11:membership	ns19:e_sm_any ;
	skos:definition	"Enterprises using at least one of the following social media: social networks, enterprise's blog or microblog, multimedia content sharing websites, wiki based knowledge sharing tools. Using social media means that the enterprise have a user profile, an account or a user license depending on the requirements and the type of the social media." ;
	skos:topConceptOf	ns1:indicator .
ns7:e_sm_ge2	rdf:type	skos:Concept ,
		ns10:Indicator ;
	skos:prefLabel	"Use two or more social media" ;
	dct:source	ns35:estat_isoc_ci_eu_en2 ;
	skos:notation	"e_sm_ge2" ;
	skos:altLabel	"Enterprises using two or more social media" ;
	ns11:membership	ns19:e_sm_ge2 ;
	skos:definition	"Enterprises using two or more of the following social media: social networks, enterprise's blog or microblog, multimedia content sharing websites, wiki based knowledge sharing tools. Using social media means that the enterprise have a user profile, an account or a user license depending on the requirements and the type of the social media." ;
	skos:topConceptOf	ns1:indicator .
ns7:e_web	rdf:type	skos:Concept ,
		ns10:Indicator ;
	skos:prefLabel	"Enterprises having a web site or homepage" ;
	dct:source	ns35:estat_isoc_ci_eu_en2 ;
	skos:notation	"e_web" ;
	skos:altLabel	"Enterprises having a web site or homepage" ;
	ns11:membership	ns19:e_web ;
	skos:note	"Enterprises with 10 or more persons employed. All manufacturing and service sectors, excluding the financial sector. Breaks in series because until 2008 economic activities according to NACE Rev 1.1 and from 2009 data are based on NACE Rev.2. Since 2010 data include also sector S95.1-Repair of computers and communication equipment." ;
	skos:topConceptOf	ns1:indicator .
ns7:e_webf2	rdf:type	skos:Concept ,
		ns10:Indicator ;
	skos:prefLabel	"Enterprises having a website with some sofisticated functionalities" ;
	dct:source	ns35:estat_isoc_ci_eu_en2 ;
	skos:notation	"e_webf2" ;
	skos:altLabel	"Enterprises having a website with some sofisticated functionalities" ;
	ns11:membership	ns19:e_webf2 ;
	skos:definition	"Website having at least one of the following four functionalities : product catalogues or price lists (webacc), possibilities for visitors to customise or design the products (webctm), order tracking available online (webot) or personalised content in the website for regular/repeated visitors (webper)." ;
	skos:note	"Enterprises with 10 or more persons employed. All manufacturing and service sectors, excluding the financial sector. Breaks in series because until 2008 economic activities according to NACE Rev 1.1 and from 2009 data are based on NACE Rev.2. Since 2010 data include also sector S95.1-Repair of computers and communication equipment." ;
	skos:topConceptOf	ns1:indicator .
ns7:e_wsel25	rdf:type	skos:Concept ,
		ns10:Indicator ;
	skos:prefLabel	"Enterprises selling over 25% via a website or apps" ;
	dct:source	ns35: ;
	skos:notation	"e_wsel25" ;
	skos:altLabel	"Enterprises selling over 25% via a website or apps" ;
	ns11:membership	ns20:e_wsel25 ;
	skos:definition	"The sales made via website or apps, during the previous calendar year, should represent at least 25% of the total turnover value (in monetary terms, excluding VAT)." ;
	skos:note	"Enterprises with 10 or more persons employed. All manufacturing and service sectors, excluding the financial sector. Breaks in series because until 2008 economic activities according to NACE Rev 1.1 and from 2009 data are based on NACE Rev.2. Since 2010 data include also sector S 95.1-Repair of computers and communication equipment." ;
	skos:topConceptOf	ns1:indicator .
ns7:e_wsel50	rdf:type	skos:Concept ,
		ns10:Indicator ;
	skos:prefLabel	"Enterprises selling over 50% via a website or apps" ;
	dct:source	ns35: ;
	skos:notation	"e_wsel50" ;
	skos:altLabel	"Enterprises selling over 50% via a website or apps" ;
	ns11:membership	ns20:e_wsel50 ;
	skos:definition	"The sales made via website or apps, during the previous calendar year, should represent at least 50% of the total turnover value (in monetary terms, excluding VAT)." ;
	skos:note	"Enterprises with 10 or more persons employed. All manufacturing and service sectors, excluding the financial sector. Breaks in series because until 2008 economic activities according to NACE Rev 1.1 and from 2009 data are based on NACE Rev.2. Since 2010 data include also sector S 95.1-Repair of computers and communication equipment." ;
	skos:topConceptOf	ns1:indicator .
ns7:edigint2015	rdf:type	skos:Concept ,
		ns10:Indicator ;
	skos:prefLabel	"Digital Intensity score for Enterprises" ;
	dct:source	ns35:estat-ent ;
	skos:notation	"edigint2015" ;
	skos:altLabel	"Digital Intensity score for Enterprises" ;
	ns11:membership	ns19:edigint2015 ;
	skos:definition	"The Digital Intensity score is based on counting how many out of 12 technologies are used by each enterprise. Then they are divided into four clusters of digital intensity: Very Low (scores 0-3), Low (score 4-6), High (score 7-9), Very High (score 10-12)." ;
	skos:note	"The 2015 list of technologies includes: usage of internet by a majority of the workers; access to ICT specialist skills; fixed broadband speed > 30 Mbps; mobile devices used by more than 20% of employed persons; has a website; has some sophisticated functions on the website; presence on social media; does e-sales for at least 1% of turnover; exploit the B2C opportunities of web sales; use an ERP software; use a CRM software; share electronically supply chain management information.\r\nIn 2016 the last 3 indicators have been replaced with: pay to advertise on the internet; purchase cloud computing advanced services; send eInvoices. There is thus a break in series with in general a reduction of the digital intensity scores." ;
	skos:topConceptOf	ns1:indicator .
ns7:employment_ict	rdf:type	skos:Concept ,
		ns10:Indicator ;
	skos:prefLabel	"Employment of the ICT sector" ;
	dct:source	ns35:jrc_ict_randd ;
	skos:notation	"employment_ict" ;
	skos:altLabel	"Employment of the ICT sector" ;
	ns11:membership	ns24:employment_ict ;
	skos:definition	"Number of persons employed. In the System of National Accounts (SNA) this is defined as all persons, both employees and self-employed, engaged in some productive activity that falls within the production boundary of the SNA and that is undertaken by a resident institutional unit." ;
	skos:topConceptOf	ns1:indicator .
ns7:eoa_nn_films	rdf:type	skos:Concept ,
		ns10:Indicator ;
	skos:prefLabel	"Non-national European films in cinemas" ;
	dct:source	ns35:eoa_yearbook2014 ;
	skos:notation	"eoa_nn_films" ;
	skos:altLabel	"Non-national European Films market share in EU cinemas" ;
	ns11:membership	ns9:eoa_nn_films ;
	skos:topConceptOf	ns1:indicator .
ns7:eoa_tvchannels_tarfor	rdf:type	skos:Concept ,
		ns10:Indicator ;
	skos:prefLabel	"Linear TV channels established in a Member State and targeting foreign countries" ;
	dct:source	ns35:eoa_yearbook2014 ;
	skos:notation	"eoa_tvchannels_tarfor" ;
	skos:altLabel	"Linear TV channels targeting foreign countries" ;
	ns11:membership	ns9:eoa_tvchannels_tarfor ;
	skos:note	"page 125" ;
	skos:topConceptOf	ns1:indicator .
ns7:eoa_vod_estab_otheu	rdf:type	skos:Concept ,
		ns10:Indicator ;
	skos:prefLabel	"Video on Demand services available in the country but established in another EU country" ;
	dct:source	ns35:eoa_smart12-26 ;
	skos:notation	"eoa_vod_estab_otheu" ;
	skos:altLabel	"VoD services available, established in another EU country" ;
	ns11:membership	ns9:eoa_vod_estab_otheu ;
	skos:definition	"Video on demand (VoD) services (all genre except adult) available in a Member State, but established in another EU country" ;
	skos:topConceptOf	ns1:indicator .
ns7:epsi_score	rdf:type	skos:Concept ,
		ns10:Indicator ;
	skos:prefLabel	"Public Sector Information scoreboard" ;
	dct:source	ns35:epsiplatform ;
	skos:notation	"epsi_score" ;
	skos:altLabel	"Public Sector Information scoreboard" ;
	ns11:membership	ns21:epsi_score ;
	skos:definition	"The PSI Scoreboard is a \u2018crowdsourced\u2019 tool to measure the status of Open Data and PSI re-use throughout the EU. It does NOT monitor government policies, but aims to assess the overall PSI re-use situation, which includes the open data community's activities." ;
	skos:topConceptOf	ns1:indicator .
ns7:eun_computers	rdf:type	skos:Concept ,
		ns10:Indicator ;
	skos:prefLabel	"Computers for educational purposes" ;
	dct:source	ns35:eun12 ;
	skos:notation	"eun_computers" ;
	skos:altLabel	"Computers for educational purposes" ;
	ns11:membership	ns23:eun_computers ;
	skos:definition	"Computers used for educational purposes include desktop, laptop, netbook or tablet computer, whether or not connected to the internet" ;
	skos:topConceptOf	ns1:indicator .
ns7:eun_web	rdf:type	skos:Concept ,
		ns10:Indicator ;
	skos:prefLabel	"Schools having a website" ;
	dct:source	ns35:eun12 ;
	skos:notation	"eun_web" ;
	skos:altLabel	"Schools having a website" ;
	ns11:membership	ns23:eun_web ;
	skos:definition	"Own home page or web site available at school." ;
	skos:topConceptOf	ns1:indicator .
ns7:foa_cit	rdf:type	ns10:Indicator ,
		skos:Concept ;
	skos:prefLabel	"Basic public services for citizens, which are fully available online" ;
	dct:source	ns35:capgemini ;
	skos:notation	"foa_cit" ;
	skos:altLabel	"Availability of eGovernment services - citizens" ;
	ns11:membership	ns18:foa_cit ;
	skos:definition	"Percentage of public services for citizens out of a basket of 12 basic services (income taxes, job search, social security benefits, personal documents, car registration, building permissions, declaration to police, public libraries, certificates, enrolment in higher education, announcement of moving, health-related services) for which the entire procedure can be completed online" ;
	skos:note	"Collected until 2010." ;
	skos:topConceptOf	ns1:indicator .
ns7:foa_ent	rdf:type	ns10:Indicator ,
		skos:Concept ;
	skos:prefLabel	"Basic public services for enterprises, which are fully available online" ;
	dct:source	ns35:capgemini ;
	skos:notation	"foa_ent" ;
	skos:altLabel	"Availability of eGovernment services - enterprises" ;
	ns11:membership	ns18:foa_ent ;
	skos:definition	"Percentage of public services for enterprises out of a basket of 8 basic services (social contributions, corporate tax, VAT, company registration, statistical data, customs declaration, environment-related permits, public procurement) for which the entire procedure can be completed online" ;
	skos:note	"Collected until 2010." ;
	skos:topConceptOf	ns1:indicator .
ns7:fp7_ict_artic	rdf:type	ns10:Indicator ,
		skos:Concept ;
	skos:prefLabel	"Articles resulting from FP7 funded projects in ICT" ;
	dct:source	ns35:smart11_39 ;
	skos:notation	"fp7_ict_artic" ;
	skos:altLabel	"Articles from FP7 ICT projects" ;
	ns11:membership	ns30:fp7_ict_artic ;
	skos:definition	"Articles in journals reported through annual surveys of ongoing ICT research projects carried out by the European Commission - DG CONNECT. Outputs reported by participants have been validated in Elsevier\u2019s Scopus databases by UNU-MERIT \u2013 Maastricht University under the service contract SMART 2011/0039 funded by the European Commission - DG CONNECT" ;
	skos:note	"It covers FP7 ICT projects started before October 2013. The indicator is not expected to evolve regularly year by year, due to the coverage of thematic areas by calls which may differ from one year to another. Annual figures should therefore be interpreted with caution." ;
	skos:topConceptOf	ns1:indicator .
ns7:fp7_ict_pat	rdf:type	ns10:Indicator ,
		skos:Concept ;
	skos:prefLabel	"Patents resulting from FP7 funded projects in ICT" ;
	dct:source	ns35:smart11_39 ;
	skos:notation	"fp7_ict_pat" ;
	skos:altLabel	"Patents from FP7 ICT projects" ;
	ns11:membership	ns30:fp7_ict_pat ;
	skos:definition	"Patents reported through annual surveys of ongoing ICT research projects carried out by the European Commission - DG CONNECT. Outputs reported by participants have been validated in EPO PATSTAT and Espacenet databases by UNU-MERIT \u2013 Maastricht University under the service contract SMART 2011/0039 funded by the European Commission - DG CONNECT" ;
	skos:note	"It covers FP7 ICT projects started before October 2013. The indicator is not expected to evolve regularly year by year, due to the coverage of thematic areas by calls which may differ from one year to another. Annual figures should therefore be interpreted with caution." ;
	skos:topConceptOf	ns1:indicator .
ns7:fp7_ict_pub	rdf:type	ns10:Indicator ,
		skos:Concept ;
	skos:prefLabel	"Publications resulting from FP7 funded projects in ICT" ;
	dct:source	ns35:smart11_39 ;
	skos:notation	"fp7_ict_pub" ;
	skos:altLabel	"Publications from FP7 ICT projects" ;
	ns11:membership	ns30:fp7_ict_pub ;
	skos:definition	"Publications reported through annual surveys of ongoing ICT research projects carried out by the European Commission - DG CONNECT. Outputs reported by participants have been validated in Elsevier\u2019s Scopus databases by UNU-MERIT \u2013 Maastricht University under the service contract SMART 2011/0039 funded by the European Commission - DG CONNECT. \n* It includes articles in journals and trade journals, conference proceedings, books, book series" ;
	skos:note	"It covers FP7 ICT projects started before October 2013. The indicator is not expected to evolve regularly year by year, due to the coverage of thematic areas by calls which may differ from one year to another. Annual figures should therefore be interpreted with caution." ;
	skos:topConceptOf	ns1:indicator .
ns7:fp7ict_afxp	rdf:type	ns10:Indicator ,
		skos:Concept ;
	skos:prefLabel	"Average EC funding per participation in FP7-ICT projects" ;
	dct:source	ns35:mis ;
	skos:notation	"fp7ict_afxp" ;
	skos:altLabel	"FP7 Average EC funding per participation" ;
	ns11:membership	ns30:fp7ict_afxp ;
	skos:definition	"EC funding is the funding committed by the European Commission through grant agreements signed during the reference year. The indicator measure the average EC funding attributed to each partner participation in a specific project." ;
	skos:topConceptOf	ns1:indicator .
ns7:fp7ict_cofin	rdf:type	ns10:Indicator ,
		skos:Concept ;
	skos:prefLabel	"FP7 EC effective cofinancing rate" ;
	dct:source	ns35:mis ;
	skos:notation	"fp7ict_cofin" ;
	skos:altLabel	"FP7 EC cofinancing rate" ;
	ns11:membership	ns30:fp7ict_cofin ;
	skos:definition	"The cofinancing rate is the % of projects total costs which are covered by EC funding grants. Figures include all partners and third parties (as subcontractors)." ;
	skos:topConceptOf	ns1:indicator .
ns7:fp7ict_ec_funding	rdf:type	ns10:Indicator ,
		skos:Concept ;
	skos:prefLabel	"EC funding to participants in FP7-ICT projects" ;
	dct:source	ns35:mis ;
	skos:notation	"fp7ict_ec_funding" ;
	skos:altLabel	"EC funding to FP7-ICT projects" ;
	ns11:membership	ns30:fp7ict_ec_funding ;
	skos:definition	"Value of European Commission funding committed through grant agreements signed, during the reference year, with participants in ICT research projects under the EU's Seventh Framework Programme (FP7). Projects under negotiation are not included." ;
	skos:topConceptOf	ns1:indicator .
ns7:fp7ict_ec_funding_prc	rdf:type	ns10:Indicator ,
		skos:Concept ;
	skos:prefLabel	"EC funding to private commercial organisations in FP7-ICT projects" ;
	dct:source	ns35:mis ;
	skos:notation	"fp7ict_ec_funding_prc" ;
	skos:altLabel	"EC funding to private commercial organisations in FP7-ICT projects" ;
	ns11:membership	ns30:fp7ict_ec_funding_prc ;
	skos:definition	"Value of European Commission funding committed through grant agreements signed, during the reference year, with private commercial organisations (SMEs and large enterprises) participating in ICT research projects under the EU's Seventh Framework Programme (FP7) - Cooperation and Capacities (e-infrastructures). " ;
	skos:topConceptOf	ns1:indicator .
ns7:fp7ict_ec_funding_smes	rdf:type	ns10:Indicator ,
		skos:Concept ;
	skos:prefLabel	"EC funding granted to SMEs in FP7-ICT projects" ;
	dct:source	ns35:mis ;
	skos:notation	"fp7ict_ec_funding_smes" ;
	skos:altLabel	"EC funding to SMEs in FP7-ICT projects" ;
	ns11:membership	ns30:fp7ict_ec_funding_smes ;
	skos:definition	"Value of European Commission funding committed through grant agreements signed, during the reference year, with SMEs participating in ICT research projects under the EU's Seventh Framework Programme (FP7) - Cooperation and Capacities (e-infrastructures). " ;
	skos:topConceptOf	ns1:indicator .
ns7:fp7ict_newentry	rdf:type	ns10:Indicator ,
		skos:Concept ;
	skos:prefLabel	"Number of distinct organisations participating in FP7-ICT projects for the first time" ;
	dct:source	ns35:mis ;
	skos:notation	"fp7ict_newentry" ;
	skos:altLabel	"Number of NEW organisations in FP7-ICT projects" ;
	ns11:membership	ns30:fp7ict_newentry ;
	skos:definition	"The first call of FP7 ICT was in 2007 and all participants are considered as new ones. For each of the following years are counted only the organisations participating for the first time in FP7 ICT calls." ;
	skos:topConceptOf	ns1:indicator .
ns7:fp7ict_organisations	rdf:type	ns10:Indicator ,
		skos:Concept ;
	skos:prefLabel	"Number of distinct organisations participating in FP7-ICT projects" ;
	dct:source	ns35:mis ;
	skos:notation	"fp7ict_organisations" ;
	skos:altLabel	"Number of participants in FP7-ICT projects" ;
	ns11:membership	ns30:fp7ict_organisations ;
	skos:definition	"Organisations participating in FP7 ICT calls for research projects (Cooperation and Capacities and e-infrastructures programs) during the reference year." ;
	skos:topConceptOf	ns1:indicator .
ns7:fp7ict_particip	rdf:type	ns10:Indicator ,
		skos:Concept ;
	skos:prefLabel	"Total number of participations in FP7-ICT projects" ;
	dct:source	ns35:mis ;
	skos:notation	"fp7ict_particip" ;
	skos:altLabel	"FP7 Total number of participations" ;
	ns11:membership	ns30:fp7ict_particip ;
	skos:definition	"Each project has multiple partners participating and each partner can participate in multiple projects. For each participation there could be an EC funding (some participations do not receive EC funding). Third parties are included as partners, receiveing or not EU funding." ;
	skos:topConceptOf	ns1:indicator .
ns7:fp7ict_particip_prc	rdf:type	ns10:Indicator ,
		skos:Concept ;
	skos:prefLabel	"Total number of participations  by private commercial organisations in FP7-ICT projects" ;
	dct:source	ns35:mis ;
	skos:notation	"fp7ict_particip_prc" ;
	skos:altLabel	"Total number of private commercial organisations'participations in FP7-ICT projects" ;
	ns11:membership	ns30:fp7ict_particip_prc ;
	skos:definition	"Total number of participations by private commercial organisations (SMEs and large enterprises)in ICT research projects under the EU's Seventh Framework Programme (FP7) - Cooperation and Capacities (e-infrastructures). Each project has multiple partners participating and each partner can participate in multiple projects. " ;
	skos:topConceptOf	ns1:indicator .
ns7:fp7ict_particip_smes	rdf:type	ns10:Indicator ,
		skos:Concept ;
	skos:prefLabel	"Total number of participations by SMEs in FP7-ICT projects" ;
	dct:source	ns35:mis ;
	skos:notation	"fp7ict_particip_smes" ;
	skos:altLabel	"Total number of SMEs' participations in FP7-ICT projects" ;
	ns11:membership	ns30:fp7ict_particip_smes ;
	skos:definition	"Total number by participations of SMEs in ICT research projects under the EU's Seventh Framework Programme (FP7) - Cooperation and Capacities (e-infrastructures). Each project has multiple partners participating and each partner can participate in multiple projects. " ;
	skos:topConceptOf	ns1:indicator .
ns7:fp7ict_totcost	rdf:type	ns10:Indicator ,
		skos:Concept ;
	skos:prefLabel	"Total cost of FP7-ICT projects" ;
	dct:source	ns35:mis ;
	skos:notation	"fp7ict_totcost" ;
	skos:altLabel	"Total cost of FP7-ICT projects" ;
	ns11:membership	ns30:fp7ict_totcost ;
	skos:definition	"Value of the total cost of the ICT research projects for which a grant agreement was signed in the reference year, under the EU's Seventh Framework Programme (FP7). Total cost of the project is the sum of participants' total costs." ;
	skos:topConceptOf	ns1:indicator .
ns7:gbaord	rdf:type	skos:Concept ,
		ns10:Indicator ;
	skos:prefLabel	"GBAORD - Government budget appropriations or outlays for research and development" ;
	dct:source	ns35:jrc_ict_randd ;
	skos:notation	"gbaord" ;
	skos:altLabel	"Public R&D expediture (GBAORD)" ;
	ns11:membership	ns30:gbaord ;
	skos:definition	"GBAORD include all appropriations (government spending) given to R&D in central (or federal) government budgets. Provincial (or State) government posts are only included if the contribution is significant. Local government funds are excluded" ;
	skos:note	"From 2006 onwards figures were revised and updated by PREDICT 2 project" ;
	skos:topConceptOf	ns1:indicator .
ns7:gbaord_ict	rdf:type	skos:Concept ,
		ns10:Indicator ;
	skos:prefLabel	"Public ICT R&D spending (GBAORD in the field of ICT)" ;
	dct:source	ns35:jrc_ict_randd ;
	skos:notation	"gbaord_ict" ;
	skos:altLabel	"Public ICT R&D spending " ;
	ns11:membership	ns30:gbaord_ict ;
	skos:definition	"Estimate of the ICT share in existing disaggregated GBAORD data, based on the assumption that the share of research in the ICT field in GBAORD expenditure is proportional to the share of ICT specialists in the R&D labour cost. Methodology developped and implemented by JRC-IPTS." ;
	skos:note	"From 2006 onwards figures were revised and updated by PREDICT 2 project" ;
	skos:topConceptOf	ns1:indicator .
ns7:gdp	rdf:type	skos:Concept ,
		ns10:Indicator ;
	skos:prefLabel	"GDP - Gross domestic product at market prices" ;
	dct:source	ns35:estat_nama_gdp_c ;
	skos:notation	"gdp" ;
	skos:altLabel	"GDP at market prices" ;
	ns11:membership	ns13:gdp ;
	skos:definition	"Eurostat estimation of GDP and main components - Current prices [nama_gdp_c]" ;
	skos:topConceptOf	ns1:indicator .
ns7:h2020_cofin	rdf:type	skos:Concept ,
		ns10:Indicator ;
	skos:prefLabel	"H2020 effective cofinancing rate" ;
	dct:source	ns35:corda ;
	skos:notation	"h2020_cofin" ;
	skos:altLabel	"H2020 cofinancing rate" ;
	ns11:membership	ns30:h2020_cofin ;
	skos:definition	"The cofinancing rate is the % of projects total costs which are covered by EC funding grants. " ;
	skos:topConceptOf	ns1:indicator .
ns7:h2020_ec_funding	rdf:type	skos:Concept ,
		ns10:Indicator ;
	skos:prefLabel	"Total EC funding to participants in H2020 ICT projects" ;
	dct:source	ns35:corda ;
	skos:notation	"h2020_ec_funding" ;
	skos:altLabel	"Total EC funding to H2020 ICT projects" ;
	ns11:membership	ns30:h2020_ec_funding ;
	skos:definition	"Value of European Commission funding committed through grant agreements signed, during the reference year, with participants in ICT research projects under Horizon 2020 (LEIT ICT, Excellent Science, Societal Challenges 1, 6 and 7). Projects under negotiation are not included." ;
	skos:topConceptOf	ns1:indicator .
ns7:h2020_newentry	rdf:type	skos:Concept ,
		ns10:Indicator ;
	skos:prefLabel	"Number of distinct organisations participating in H2020 ICT projects for the first time" ;
	dct:source	ns35:corda ;
	skos:notation	"h2020_newentry" ;
	skos:altLabel	"Number of new organisations in H2020 projects" ;
	ns11:membership	ns30:h2020_newentry ;
	skos:definition	"Organisations participating for the first time in H2020 ICT calls, and which have not participated in FP7 ICT calls during 2007-2013 period." ;
	skos:topConceptOf	ns1:indicator .
ns7:h2020_organisations	rdf:type	skos:Concept ,
		ns10:Indicator ;
	skos:prefLabel	"Number of distinct organisations participating in H2020 ICT projects" ;
	dct:source	ns35:corda ;
	skos:notation	"h2020_organisations" ;
	skos:altLabel	"H2020 Total number of organisations" ;
	ns11:membership	ns30:h2020_organisations ;
	skos:definition	"Organisations participating in H2020 ICT projects during the reference year." ;
	skos:topConceptOf	ns1:indicator .
ns7:h2020_particip	rdf:type	skos:Concept ,
		ns10:Indicator ;
	skos:prefLabel	"Total number of participations in H2020 ICT projects" ;
	dct:source	ns35:corda ;
	skos:notation	"h2020_particip" ;
	skos:altLabel	"H2020 Total number of participations" ;
	ns11:membership	ns30:h2020_particip ;
	skos:definition	"Each project has multiple partners participating and each partner can participate in multiple projects. For each participation there could be an EC funding (some participations do not receive EC funding). " ;
	skos:topConceptOf	ns1:indicator .
ns7:h2020_totcost	rdf:type	skos:Concept ,
		ns10:Indicator ;
	skos:prefLabel	"Total cost of H2020 ICT projects" ;
	dct:source	ns35:corda ;
	skos:notation	"h2020_totcost" ;
	skos:altLabel	"Total cost of H2020 ICT projects" ;
	ns11:membership	ns30:h2020_totcost ;
	skos:definition	"Value of the total cost of the ICT research projects for which a grant agreement was signed in the reference year, under the Horizon 2020 LEIT ICT, Excellent Science, Societal Challenges 1, 6 and 7). Total cost of the project is the sum of participants' total costs." ;
	skos:topConceptOf	ns1:indicator .
ns7:h2020ict_afxp	rdf:type	skos:Concept ,
		ns10:Indicator ;
	skos:prefLabel	"Average EC funding per participation in H2020 ICT projects" ;
	dct:source	ns35:corda ;
	skos:notation	"h2020ict_afxp" ;
	skos:altLabel	"H2020 Average EC funding per participation" ;
	ns11:membership	ns30:h2020ict_afxp ;
	skos:definition	"EC funding is the funding committed by the European Commission through grant agreements signed during the reference year. The indicator measures the average EC funding attributed to each partner participation in a specific project." ;
	skos:topConceptOf	ns1:indicator .
ns7:h_bbfix	rdf:type	skos:Concept ,
		ns10:Indicator ;
	skos:prefLabel	"Households with fixed broadband connection" ;
	dct:source	ns35:estat_isoc_bde15b_h ;
	skos:notation	"h_bbfix" ;
	skos:altLabel	"Households with fixed broadband connection" ;
	ns11:membership	ns15:h_bbfix ;
	skos:definition	"Household internet connection type: fixed broadband" ;
	skos:topConceptOf	ns1:indicator .
ns7:h_broad	rdf:type	skos:Concept ,
		ns10:Indicator ;
	skos:prefLabel	"Households having a broadband connection" ;
	dct:source	ns35:estat_isoc_bde15b_h ;
	skos:notation	"h_broad" ;
	skos:altLabel	"Households with a broadband connection" ;
	ns11:membership	ns15:h_broad ;
	skos:definition	"Broadband connection used by the household includes: DSL, wired fixed (cable, fiber, Ethernet, PLC), fixed wireless (satellite, WiFi, WiMax) and mobile wireless (3G/UMTS)." ;
	skos:note	"Scope includes Households with at least one member aged 16-74. " ;
	skos:topConceptOf	ns1:indicator .
ns7:h_iacc	rdf:type	skos:Concept ,
		ns10:Indicator ;
	skos:prefLabel	"Households with access to the Internet at home" ;
	dct:source	ns35:estat_isoc_bde15b_h ;
	skos:notation	"h_iacc" ;
	skos:altLabel	"Households with access to the Internet at home" ;
	ns11:membership	ns28:h_iacc ;
	skos:definition	"Any member of the household has access to the Internet at home" ;
	skos:note	"Scope includes Households with at least one member aged 16-74." ;
	skos:topConceptOf	ns1:indicator .
ns7:h_xcost	rdf:type	skos:Concept ,
		ns10:Indicator ;
	skos:prefLabel	"Households that have no access to Internet at home, because the costs are too high" ;
	dct:source	ns35:estat-hh ;
	skos:notation	"h_xcost" ;
	skos:altLabel	"Households with no access to Internet at home, because the costs are too high" ;
	ns11:membership	ns14:h_xcost ;
	skos:definition	"Households that have no access to Internet at home, because the costs are too high" ;
	skos:topConceptOf	ns1:indicator .
ns7:hie_use_ex_admin	rdf:type	skos:Concept ,
		ns10:Indicator ;
	skos:prefLabel	"GPs exchanging medical patient data with other healthcare providers and professionals" ;
	dct:source	ns35:bench_gp ;
	skos:notation	"hie_use_ex_admin" ;
	skos:altLabel	"GPs exchanging medical patient data with other healthcare providers and professionals" ;
	ns11:membership	ns22:hie_use_ex_admin ;
	skos:definition	"Percentatge of general practitioners using electronic networks to exchange medical patient data with other healthcare providers and professionals" ;
	skos:topConceptOf	ns1:indicator .
ns7:hie_use_pharm	rdf:type	skos:Concept ,
		ns10:Indicator ;
	skos:prefLabel	"GPs using electronic networks to transfer prescriptions to pharmacists" ;
	dct:source	ns35:bench_gp ;
	skos:notation	"hie_use_pharm" ;
	skos:altLabel	"GPs using electronic networks to transfer prescriptions to pharmacists" ;
	ns11:membership	ns22:hie_use_pharm ;
	skos:definition	"Percentatge of general practitioners using electronic networks to transfer prescriptions to pharmacists" ;
	skos:topConceptOf	ns1:indicator .
ns7:househ	rdf:type	ns10:Indicator ,
		skos:Concept ;
	skos:prefLabel	"Number of households" ;
	dct:source	ns35:estat-hh ;
	skos:notation	"househ" ;
	skos:altLabel	"Number of households" ;
	ns11:membership	ns13:househ ;
	skos:definition	"Estimation of the number of Households with at least one member aged 16-74, for the purpose of the survey on ICT usage by individuals and households." ;
	skos:topConceptOf	ns1:indicator .
ns7:households	rdf:type	ns10:Indicator ,
		skos:Concept ;
	skos:prefLabel	"Number of private Households" ;
	dct:source	ns35:estat_lfst_hhnhwhtc ;
	skos:notation	"households" ;
	skos:altLabel	"Number of private Households" ;
	ns11:membership	ns13:households ;
	skos:definition	"Number of private households (Eurostat table lfst_hhnhwhtc)" ;
	skos:topConceptOf	ns1:indicator .
ns7:i_atsw	rdf:type	ns10:Indicator ,
		skos:Concept ;
	skos:prefLabel	"Individuals using anti-tracking software" ;
	dct:source	ns35:estat_isoc_cisci_prv ;
	skos:notation	"i_atsw" ;
	skos:altLabel	"Individuals using anti-tracking software" ;
	ns11:membership	ns32:i_atsw ;
	skos:definition	"Individuals using anti-tracking software" ;
	skos:topConceptOf	ns1:indicator .
ns7:i_barr1x	rdf:type	ns10:Indicator ,
		skos:Concept ;
	skos:prefLabel	"Individuals who did not encounter problems when buying/ordering goods or services over the internet for private use" ;
	dct:source	ns35:estat_isoc_ec_iprb ;
	skos:notation	"i_barr1x" ;
	skos:altLabel	"Individuals who had no problems buying/ordering goods or services over the internet for private use" ;
	ns11:membership	ns20:i_barr1x ;
	skos:definition	"Individuals who had no problems buying/ordering goods or services over the internet for private use" ;
	skos:topConceptOf	ns1:indicator .
ns7:i_bfeu	rdf:type	ns10:Indicator ,
		skos:Concept ;
	skos:prefLabel	"Individuals ordering goods or services online, from sellers from other EU countries" ;
	dct:source	ns35:estat_isoc_bde15cbc ;
	skos:notation	"i_bfeu" ;
	skos:altLabel	"Cross-border eCommerce" ;
	ns11:membership	ns20:i_bfeu ;
	skos:definition	"Individuals that ordered goods or services for private use over the Internet in the last 12 months from sellers from other EU countries" ;
	skos:topConceptOf	ns1:indicator .
ns7:i_bgood	rdf:type	ns10:Indicator ,
		skos:Concept ;
	skos:prefLabel	"Individuals ordering content or software delivered online or offline" ;
	dct:source	ns35:estat_isoc_ec_ibuy ;
	skos:notation	"i_bgood" ;
	skos:altLabel	"Buying: content (any delivery mode)" ;
	ns11:membership	ns20:i_bgood ;
	skos:definition	"Online purchases: films/music or books/magazines/e-learning material or computer software" ;
	skos:topConceptOf	ns1:indicator .
ns7:i_bgoodo	rdf:type	ns10:Indicator ,
		skos:Concept ;
	skos:prefLabel	"Individuals ordering content or software that were delivered or upgraded online" ;
	dct:source	ns35:estat_isoc_ec_ibuy ;
	skos:notation	"i_bgoodo" ;
	skos:altLabel	"Buying : online content" ;
	ns11:membership	ns20:i_bgoodo ;
	skos:definition	"The online content and software include: films, music, books, magazines, e-learning material, computer software, video games, that were ordered/bought over the Internet in the last 12 months, for non-work use." ;
	skos:topConceptOf	ns1:indicator .
ns7:i_blt12	rdf:type	ns10:Indicator ,
		skos:Concept ;
	skos:prefLabel	"Individuals ordering goods or services online" ;
	dct:source	ns35:estat_isoc_ec_ibuy ;
	skos:notation	"i_blt12" ;
	skos:altLabel	"Ordering goods or services online" ;
	ns11:membership	ns20:i_blt12 ;
	skos:definition	"Individuals carrying out this activity over the internet in the last 12 months, for private use." ;
	skos:topConceptOf	ns1:indicator .
ns7:i_bpgood	rdf:type	ns10:Indicator ,
		skos:Concept ;
	skos:prefLabel	"Individuals ordering physical goods online" ;
	dct:source	ns35:estat_isoc_ec_ibuy ;
	skos:notation	"i_bpgood" ;
	skos:altLabel	"Buying : physical goods online" ;
	ns11:membership	ns20:i_bpgood ;
	skos:definition	"Individuals that have ordered online any of the following physical goods: food/groceries, household goods, medicine, clothes/sports, computer hardware, electronic equipment." ;
	skos:topConceptOf	ns1:indicator .
ns7:i_bserv	rdf:type	ns10:Indicator ,
		skos:Concept ;
	skos:prefLabel	"Individuals ordering services online" ;
	dct:source	ns35:estat_isoc_ec_ibuy ;
	skos:notation	"i_bserv" ;
	skos:altLabel	"Buying : services online" ;
	ns11:membership	ns20:i_bserv ;
	skos:definition	"Individuals that have ordered online any of the following services: telecommunications services, share/insurance/financial, holiday accomodation, travel arrangements, tickets for events." ;
	skos:topConceptOf	ns1:indicator .
ns7:i_cc	rdf:type	skos:Concept ,
		ns10:Indicator ;
	skos:prefLabel	"Used internet storage space to save documents, pictures, music, video or other files" ;
	dct:source	ns35:estat_isoc_cicce_use ;
	skos:notation	"i_cc" ;
	skos:altLabel	"Used internet storage space" ;
	ns11:membership	ns27:i_cc ;
	skos:definition	"Used internet storage space to save documents, pictures, music, video or other files" ;
	skos:topConceptOf	ns1:indicator .
ns7:i_cisk_sfjob	rdf:type	skos:Concept ,
		ns10:Indicator ;
	skos:prefLabel	"workers who judge their current ICT skills sufficient for changing job within a year" ;
	dct:source	ns35:estat_isoc_sk_cskl_i ;
	skos:notation	"i_cisk_sfjob" ;
	skos:altLabel	"ICT skills perceived as sufficient for the labour market" ;
	ns11:membership	ns18:i_cisk_sfjob ;
	skos:definition	"Individuals with an occupation as employees, self-employed or family workers, were asked if they judge their current computer or Internet skills to be sufficient (yes/not) if they were to look for a job or change job within a year." ;
	skos:topConceptOf	ns1:indicator .
ns7:i_cisk_sfjobx	rdf:type	skos:Concept ,
		ns10:Indicator ;
	skos:prefLabel	"workers who judge their current ICT skills insufficient for changing job within a year" ;
	dct:source	ns35:estat_isoc_sk_cskl_i ;
	skos:notation	"i_cisk_sfjobx" ;
	skos:altLabel	"ICT skills perceived as insufficient for the labour market" ;
	ns11:membership	ns26:i_cisk_sfjobx ;
	skos:definition	"Individuals with an occupation as employees, self-employed or family workers, were asked if they judge their current computer or Internet skills to be sufficient (yes/not) if they were to look for a job or change job within a year." ;
	skos:topConceptOf	ns1:indicator .
ns7:i_cook	rdf:type	skos:Concept ,
		ns10:Indicator ;
	skos:prefLabel	"Individuals who know that cookies can be used to trace movements of people on the internet" ;
	dct:source	ns35:estat_isoc_cisci_prv ;
	skos:notation	"i_cook" ;
	skos:altLabel	"Awareness about cookies" ;
	ns11:membership	ns32:i_cook ;
	skos:definition	"Individuals who know that cookies can be used to trace movements of people on the internet" ;
	skos:topConceptOf	ns1:indicator .
ns7:i_cprg	rdf:type	skos:Concept ,
		ns10:Indicator ;
	skos:prefLabel	"Individuals who have written a computer program using a specialised programming language" ;
	dct:source	ns35:estat_isoc_sk_cskl_i ;
	skos:notation	"i_cprg" ;
	skos:altLabel	"Have written a computer program" ;
	ns11:membership	ns26:i_cprg ;
	skos:definition	"Individuals who have written a computer program using a specialised programming language. " ;
	skos:note	"Break in series because before 2015 the activity could have been carried out ever, but since 2015 it refers to the last 12 months ." ;
	skos:topConceptOf	ns1:indicator .
ns7:i_csk_ge_me	rdf:type	skos:Concept ,
		ns10:Indicator ;
	skos:prefLabel	"Individuals with medium or high computer skills (3 or more of 6 computer activities)" ;
	dct:source	ns35:estat_isoc_sk_cskl_i ;
	skos:notation	"i_csk_ge_me" ;
	skos:altLabel	"Individuals with medium or high computer skills" ;
	ns11:membership	ns18:i_csk_ge_me ;
	skos:definition	"The indicator counts individuals having ever carried out at least 3 of the following 6 activities: coping or moving a file or folder, using copy and paste tools, using basic arithmetic formula in a spreadsheet, compressing (or zipping) files, connecting and installing new devices, writing a computer program using a specialised programming language. Only those having ever used a computer were proposed the question." ;
	skos:topConceptOf	ns1:indicator .
ns7:i_cweb	rdf:type	skos:Concept ,
		ns10:Indicator ;
	skos:prefLabel	"Individuals who have created a Web page" ;
	dct:source	ns35:estat_isoc_sk_iskl_i ;
	skos:notation	"i_cweb" ;
	skos:altLabel	"Have created a Web page" ;
	ns11:membership	ns18:i_cweb ;
	skos:definition	"The activity could have been carried out ever. Only those having ever used the internet were proposed the question." ;
	skos:topConceptOf	ns1:indicator .
ns7:i_dsk_bab	rdf:type	skos:Concept ,
		ns10:Indicator ;
	skos:prefLabel	"Individuals with at least basic digital skills" ;
	dct:source	ns35:estat_isoc_sk_dskl_i ;
	skos:notation	"i_dsk_bab" ;
	skos:altLabel	"Individuals with at least basic digital skills" ;
	ns11:membership	ns25:i_dsk_bab ;
	skos:definition	"Persons that have been using internet during last 3 months are attributed a score on four digital competence domains: information, communication, content-creation and problem-solving, depending the activities they have been able to do. The scores in each domain are basic, above basic and below basic. Individuals not using internet are classified without digital skills. To be classified \"basic or above basic\" on the overall indicator an individual has to have basic or above basic skills in all the four Digital Competence domains included in the index: information, communication, content-creation and problem-solving." ;
	skos:note	"Detailed results are available in the Eurostat table <a href=\"http://appsso.eurostat.ec.europa.eu/nui/show.do?dataset=isoc_sk_dskl_i&lang=en\">ISOC_SK_DSKL_I</a>. Consult the <a href=\"https://ec.europa.eu/digital-agenda/en/news/new-comprehensive-digital-skills-indicator\"> methodological note</a> on DG CONNECT newsroom." ;
	skos:topConceptOf	ns1:indicator .
ns7:i_dsk_c_bab	rdf:type	skos:Concept ,
		ns10:Indicator ;
	skos:prefLabel	"Individuals with at least basic digital skills in Communication domain" ;
	dct:source	ns35:estat_isoc_sk_dskl_i ;
	skos:notation	"i_dsk_c_bab" ;
	skos:altLabel	"Communication Domain - At least Basic  Skills" ;
	ns11:membership	ns25:i_dsk_c_bab ;
	skos:definition	"These skills refer to the ability to communicate in digital environments, share resources through online tools, link with others and collaborate through digital tools, interact with and participate in communities and networks, cross-cultural awareness. The indicator is based on four activities internet users have been able to do online during previous 3 months. The scores are basic, above basic and none. Individuals not using internet are classified without digital skills." ;
	skos:note	"Detailed results are available in the Eurostat table <a href=\"http://appsso.eurostat.ec.europa.eu/nui/show.do?dataset=isoc_sk_dskl_i&lang=en\">ISOC_SK_DSKL_I</a>. Consult the <a href=\"https://ec.europa.eu/digital-agenda/en/news/new-comprehensive-digital-skills-indicator\"> methodological note</a> on DG CONNECT newsroom." ;
	skos:topConceptOf	ns1:indicator .
ns7:i_dsk_i_bab	rdf:type	skos:Concept ,
		ns10:Indicator ;
	skos:prefLabel	"Individuals with at least basic digital skills in Information domain" ;
	dct:source	ns35:estat_isoc_sk_dskl_i ;
	skos:notation	"i_dsk_i_bab" ;
	skos:altLabel	"Information Domain - At least Basic  Skills" ;
	ns11:membership	ns25:i_dsk_i_bab ;
	skos:definition	"Information processing skills refers to the ability to identify, locate, retrieve, store, organise and analyse digital information, judging its relevance and purpose. The indicator is based on five activities internet users have been able to do online during previous 3 months. The scores are basic, above basic and none. Individuals not using internet are classified without digital skills." ;
	skos:note	"Detailed results are available in the Eurostat table <a href=\"http://appsso.eurostat.ec.europa.eu/nui/show.do?dataset=isoc_sk_dskl_i&lang=en\">ISOC_SK_DSKL_I</a>. Consult the <a href=\"https://ec.europa.eu/digital-agenda/en/news/new-comprehensive-digital-skills-indicator\"> methodological note</a> on DG CONNECT newsroom." ;
	skos:topConceptOf	ns1:indicator .
ns7:i_dsk_ps_bab	rdf:type	skos:Concept ,
		ns10:Indicator ;
	skos:prefLabel	"Individuals with at least basic digital skills in Problem solving domain" ;
	dct:source	ns35:estat_isoc_sk_dskl_i ;
	skos:notation	"i_dsk_ps_bab" ;
	skos:altLabel	"Problem Solving Domain - At least Basic  Skills" ;
	ns11:membership	ns25:i_dsk_ps_bab ;
	skos:definition	"Problem solving skills refers to the ability to identify digital needs and resources, make informed decisions as to which are the most appropriate digital tools according to the purpose or need, solve conceptual problems through digital means, creatively use technologies, solve technical problems, update one's own and others' competences. The indicator is based on three basic digital problems and familiarity with four online services internet users have been able to do during previous 3 months. The scores are basic, above basic and none. Individuals not using internet are classified without digital skills." ;
	skos:note	"Detailed results are available in the Eurostat table <a href=\"http://appsso.eurostat.ec.europa.eu/nui/show.do?dataset=isoc_sk_dskl_i&lang=en\">ISOC_SK_DSKL_I</a>. Consult the <a href=\"https://ec.europa.eu/digital-agenda/en/news/new-comprehensive-digital-skills-indicator\"> methodological note</a> on DG CONNECT newsroom." ;
	skos:topConceptOf	ns1:indicator .
ns7:i_dsk_s_bab	rdf:type	skos:Concept ,
		ns10:Indicator ;
	skos:prefLabel	"Individuals with at least basic digital skills in Software domain" ;
	dct:source	ns35:estat_isoc_sk_dskl_i ;
	skos:notation	"i_dsk_s_bab" ;
	skos:altLabel	"Software Domain - At least Basic  Skills" ;
	ns11:membership	ns25:i_dsk_s_bab ;
	skos:definition	"Software skills for content manipulation refer to the ability to create and edit new content (from word processing to images and video); integrate and re-elaborate previous knowledge and content; produce creative expressions, media outputs and programming; deal with and apply intellectual property rights and licences. The indicator is based on six activities internet users have been able to do during previous 3 months. The scores are basic, above basic and none. Individuals not using internet are classified without digital skills." ;
	skos:note	"Detailed results are available in the Eurostat table <a href=\"http://appsso.eurostat.ec.europa.eu/nui/show.do?dataset=isoc_sk_dskl_i&lang=en\">ISOC_SK_DSKL_I</a>. Consult the <a href=\"https://ec.europa.eu/digital-agenda/en/news/new-comprehensive-digital-skills-indicator\"> methodological note</a> on DG CONNECT newsroom." ;
	skos:topConceptOf	ns1:indicator .
ns7:i_ia12ave	rdf:type	skos:Concept ,
		ns10:Indicator ;
	skos:prefLabel	"Diversification index for the activities realised online by internet users" ;
	dct:source	ns35:estat_isoc_bde15cua ;
	skos:notation	"i_ia12ave" ;
	skos:altLabel	"Diversification index for internet usage" ;
	ns11:membership	ns28:i_ia12ave ;
	skos:definition	"The diversification index is based on counting how many activities, out of a list of 12, have been realised at least once in the previous months. It is computed at individual level for those individuals having used internet in the last 3 months." ;
	skos:note	"The 12 activities included in the index are: sending/receiving e-mails, information about goods and services, reading online newspapers/news, information on travel/accommodation services, posting messages to social media, interaction with public authorities, internet banking, telephoning or video calls, selling goods or services, purchases of content (films,music,software,etc), purchase of goods, purchase of services." ;
	skos:topConceptOf	ns1:indicator .
ns7:i_iday	rdf:type	skos:Concept ,
		ns10:Indicator ;
	skos:prefLabel	"Individuals who are frequent internet users (every day or almost every day)" ;
	dct:source	ns35:estat_isoc_bde15cua ;
	skos:notation	"i_iday" ;
	skos:altLabel	"Frequent internet users" ;
	ns11:membership	ns28:i_iday ;
	skos:definition	"Individuals using the internet every day or almost every day, in the last 3 months." ;
	skos:topConceptOf	ns1:indicator .
ns7:i_igov12rt	rdf:type	skos:Concept ,
		ns10:Indicator ;
	skos:prefLabel	"Individuals submitting completed forms to public authorities, over the internet, last 12 months" ;
	dct:source	ns35:estat_isoc_r_gov_i ;
	skos:notation	"i_igov12rt" ;
	skos:altLabel	"Citizens submitting filled forms to eGov services, last 12 months" ;
	ns11:membership	ns21:i_igov12rt ;
	skos:topConceptOf	ns1:indicator .
ns7:i_igovrt	rdf:type	skos:Concept ,
		ns10:Indicator ;
	skos:prefLabel	"sending filled forms to public authorities, over the internet, last 3 months" ;
	dct:source	ns35:estat_isoc_ci_ac_i ;
	skos:notation	"i_igovrt" ;
	skos:altLabel	"Sending filled forms to eGov services, last 3 months" ;
	ns11:membership	ns18:i_igovrt ;
	skos:note	"Indicator collected until 2010." ;
	skos:topConceptOf	ns1:indicator .
ns7:i_ihif	rdf:type	ns10:Indicator ,
		skos:Concept ;
	skos:prefLabel	"seeking online information about health" ;
	dct:source	ns35:estat_isoc_bde15cua ;
	skos:notation	"i_ihif" ;
	skos:altLabel	"Seeking health information" ;
	ns11:membership	ns22:i_ihif ;
	skos:definition	"Individuals using internet in the last 3 months, seeking information about health: injury, disease, nutrition, improving health, etc." ;
	skos:topConceptOf	ns1:indicator .
ns7:i_ilt12	rdf:type	ns10:Indicator ,
		skos:Concept ;
	skos:prefLabel	"Individuals who have used internet in the last 12 months" ;
	dct:source	ns35:estat_isoc_ci_ifp_iu ;
	skos:notation	"i_ilt12" ;
	skos:altLabel	"Internet used in the last 12 months" ;
	ns11:membership	ns28:i_ilt12 ;
	skos:topConceptOf	ns1:indicator .
ns7:i_isk_ge_me	rdf:type	ns10:Indicator ,
		skos:Concept ;
	skos:prefLabel	"Individuals with medium or high internet skills (3 or more of 6 internet activities)" ;
	dct:source	ns35:estat_isoc_sk_iskl_i ;
	skos:notation	"i_isk_ge_me" ;
	skos:altLabel	"Individuals with medium or high internet skills" ;
	ns11:membership	ns18:i_isk_ge_me ;
	skos:definition	"The indicator counts individuals having ever carried out at least 3 of the following 6 activities: using a search engine to find information, sending e-mails with attached files, posting messages to chatrooms, newsgroups or an online discussion forum, using the internet to make telephone calls, using peer-to-peer file sharing for exchanging movies or music, creating a webpage. Only those having ever used the internet were proposed the question." ;
	skos:topConceptOf	ns1:indicator .
ns7:i_iu3	rdf:type	ns10:Indicator ,
		skos:Concept ;
	skos:prefLabel	"Individuals who have used internet in the last 3 months" ;
	dct:source	ns35:estat_isoc_ci_ifp_iu ;
	skos:notation	"i_iu3" ;
	skos:altLabel	"Internet used in the last 3 months" ;
	ns11:membership	ns28:i_iu3 ;
	skos:topConceptOf	ns1:indicator .
ns7:i_iu3g	rdf:type	ns10:Indicator ,
		skos:Concept ;
	skos:prefLabel	"Individuals accessing the Internet through a mobile phone via UMTS (3G)" ;
	dct:source	ns35:estat_isoc_ci_im_i ;
	skos:notation	"i_iu3g" ;
	skos:altLabel	"Use of mobile phones to access the Internet" ;
	ns11:membership	ns29:i_iu3g ;
	skos:definition	"Individuals using a mobile phone or smart phone to access the internet, in the last 3 months. Since 2011 the question specify \"away from home or work\". Until 2012  the question was limited to \"via UMTS, HSDPA (3G or 3G+) connections\"." ;
	skos:note	"Break in series in 2011 and 2012 as the structure of the question has changed. Reconstructed time series using Eurostat variables: i_iu3g, i_iu3G1, i_iuhd_mph, i_iump_mph" ;
	skos:topConceptOf	ns1:indicator .
ns7:i_iubk	rdf:type	ns10:Indicator ,
		skos:Concept ;
	skos:prefLabel	"using online banking" ;
	dct:source	ns35:estat_isoc_ci_ac_i ;
	skos:notation	"i_iubk" ;
	skos:altLabel	"Online banking" ;
	ns11:membership	ns27:i_iubk ;
	skos:definition	"Individuals have used Internet, in the last 3 months, for Internet banking" ;
	skos:topConceptOf	ns1:indicator .
ns7:i_iueduif	rdf:type	ns10:Indicator ,
		skos:Concept ;
	skos:prefLabel	"looking online for information about education, training or course offers" ;
	dct:source	ns35:estat_isoc_ci_ac_i ;
	skos:notation	"i_iueduif" ;
	skos:altLabel	"Information about education & training" ;
	ns11:membership	ns27:i_iueduif ;
	skos:definition	"Individuals have used Internet, in the last 3 months, for looking for information about education, training or course offers" ;
	skos:topConceptOf	ns1:indicator .
ns7:i_iugm	rdf:type	ns10:Indicator ,
		skos:Concept ;
	skos:prefLabel	"playing or downloading games, images, films or music" ;
	dct:source	ns35:estat_isoc_bde15cua ;
	skos:notation	"i_iugm" ;
	skos:altLabel	"Games, images, films or music" ;
	ns11:membership	ns9:i_iugm ;
	skos:definition	"Individuals have used Internet, in the last 3 months, for playing or downloading games, images films or music" ;
	skos:note	"Biennial indicator not collected in 2011" ;
	skos:topConceptOf	ns1:indicator .
ns7:i_iugov	rdf:type	ns10:Indicator ,
		skos:Concept ;
	skos:prefLabel	"interacting online with public authorities, last 3 months" ;
	dct:source	ns35:estat_isoc_ci_ac_i ;
	skos:notation	"i_iugov" ;
	skos:altLabel	"Use of eGovernment services, last 3 months" ;
	ns11:membership	ns18:i_iugov ;
	skos:definition	"Individuals have used Internet, in the last 3 months, for interaction with public authorities. It includes obtaining information from public authorities web sites, downloading official forms and sending filled in forms." ;
	skos:topConceptOf	ns1:indicator .
ns7:i_iugov12	rdf:type	ns10:Indicator ,
		skos:Concept ;
	skos:prefLabel	"Individuals interacting online with public authorities, last 12 months" ;
	dct:source	ns35:estat_isoc_r_gov_i ;
	skos:notation	"i_iugov12" ;
	skos:altLabel	"Citizens' use of eGovernment services, last 12 months" ;
	ns11:membership	ns21:i_iugov12 ;
	skos:definition	"Individuals have used Internet, in the last 12 months, for interaction with public authorities. It includes obtaining information from public authorities web sites, OR downloading official forms OR sending filled in forms." ;
	skos:topConceptOf	ns1:indicator .
ns7:i_iuif	rdf:type	ns10:Indicator ,
		skos:Concept ;
	skos:prefLabel	"looking for information about goods and services online" ;
	dct:source	ns35:estat_isoc_ci_ac_i ;
	skos:notation	"i_iuif" ;
	skos:altLabel	"Information about goods and services" ;
	ns11:membership	ns27:i_iuif ;
	skos:definition	"Individuals have used Internet, in the last 3 months, for finding information about goods and services" ;
	skos:topConceptOf	ns1:indicator .
ns7:i_iujob	rdf:type	ns10:Indicator ,
		skos:Concept ;
	skos:prefLabel	"looking online for a job or sending a job application" ;
	dct:source	ns35:estat_isoc_bde15cua ;
	skos:notation	"i_iujob" ;
	skos:altLabel	"Looking for a job, sending a job application" ;
	ns11:membership	ns27:i_iujob ;
	skos:definition	"Individuals have used Internet, in the last 3 months, for looking for a job or sending a job application" ;
	skos:topConceptOf	ns1:indicator .
ns7:i_iumapp	rdf:type	ns10:Indicator ,
		skos:Concept ;
	skos:prefLabel	"making an appointment with a practitioner via a website" ;
	dct:source	ns35:estat_isoc_bde15cua ;
	skos:notation	"i_iumapp" ;
	skos:altLabel	"Appointment with a practitioner via a website" ;
	ns11:membership	ns22:i_iumapp ;
	skos:definition	"Individuals have used Internet, in the last 3 months, for making an appointment with a practitioner via a website (e.g. of a hospital or a health care centre)" ;
	skos:note	"Biennial indicator" ;
	skos:topConceptOf	ns1:indicator .
ns7:i_iumc	rdf:type	ns10:Indicator ,
		skos:Concept ;
	skos:prefLabel	"Individuals using a laptop/tablet to access the internet, away from home or work " ;
	dct:source	ns35:estat_isoc_ci_im_i ;
	skos:notation	"i_iumc" ;
	skos:altLabel	"Nomadic use of laptop/tablet to access the Internet" ;
	ns11:membership	ns28:i_iumc ;
	skos:definition	"Individuals using a portable computer (laptop) to access the internet away from home or work via any wireless connection (WiFi or cellular networks), in the last 3 months. Since 2012 the question explicitly mention also tablet computer (with touch screen)." ;
	skos:note	"Break in series in 2011 and 2012 as the structure of the question has changed. Reconstructed time series using Eurostat varibales: i_iuport, i_iuport1, i_iumc" ;
	skos:topConceptOf	ns1:indicator .
ns7:i_iunw	rdf:type	ns10:Indicator ,
		skos:Concept ;
	skos:prefLabel	"reading / downloading online newspapers / news magazines" ;
	dct:source	ns35:estat_isoc_bde15cua ;
	skos:notation	"i_iunw" ;
	skos:altLabel	"Reading online newspapers/magazines" ;
	ns11:membership	ns9:i_iunw ;
	skos:definition	"Individuals have used Internet, in the last 3 months, for reading / downloading online newspapers / news magazines" ;
	skos:topConceptOf	ns1:indicator .
ns7:i_iuolc	rdf:type	ns10:Indicator ,
		skos:Concept ;
	skos:prefLabel	"doing an online course (in any subject)" ;
	dct:source	ns35:estat_isoc_bde15cua ;
	skos:notation	"i_iuolc" ;
	skos:altLabel	"Doing an online course" ;
	ns11:membership	ns27:i_iuolc ;
	skos:definition	"Individuals have used Internet, in the last 3 months, for doing an online course (of any subject)" ;
	skos:topConceptOf	ns1:indicator .
ns7:i_iuph1	rdf:type	skos:Concept ,
		ns10:Indicator ;
	skos:prefLabel	"telephoning or video calls (via webcam) over the internet" ;
	dct:source	ns35:estat_isoc_bde15cua ;
	skos:notation	"i_iuph1" ;
	skos:altLabel	"Telephoning or video calls" ;
	ns11:membership	ns27:i_iuph1 ;
	skos:note	"Biennial indicator. Break in time series between 2007 and 2008 because of new wording. Reconstructed time series using Eurostat varibales: i_iuph and i_iuph1." ;
	skos:topConceptOf	ns1:indicator .
ns7:i_iuse	rdf:type	skos:Concept ,
		ns10:Indicator ;
	skos:prefLabel	"Individuals who are regular internet users (at least once a week)" ;
	dct:source	ns35:estat_isoc_ci_ifp_fu ;
	skos:notation	"i_iuse" ;
	skos:altLabel	"Regular internet users" ;
	ns11:membership	ns28:i_iuse ;
	skos:definition	"Individuals using the internet at least once a week in the last 3 months." ;
	skos:topConceptOf	ns1:indicator .
ns7:i_iusell	rdf:type	skos:Concept ,
		ns10:Indicator ;
	skos:prefLabel	"Individuals selling goods or services online (e.g. via auctions)" ;
	dct:source	ns35:estat_isoc_r_iuse_i ;
	skos:notation	"i_iusell" ;
	skos:altLabel	"Selling online (e.g. via auctions)" ;
	ns11:membership	ns20:i_iusell ;
	skos:definition	"Individuals have used Internet, in the last 3 months, for selling goods and services (e.g. via auctions)" ;
	skos:topConceptOf	ns1:indicator .
ns7:i_iusnet	rdf:type	skos:Concept ,
		ns10:Indicator ;
	skos:prefLabel	"participating in social networks, over the internet, last 3 months" ;
	dct:source	ns35:estat_isoc_bde15cua ;
	skos:notation	"i_iusnet" ;
	skos:altLabel	"Participating in social networks" ;
	ns11:membership	ns27:i_iusnet ;
	skos:definition	"Individuals have used Internet, in the last 3 months, for participating in social networks (creating user profile, posting messages or other contributions to facebook, twitter, etc.)" ;
	skos:topConceptOf	ns1:indicator .
ns7:i_iuupl	rdf:type	skos:Concept ,
		ns10:Indicator ;
	skos:prefLabel	"uploading self-created content to be shared" ;
	dct:source	ns35:estat_isoc_bde15cua ;
	skos:notation	"i_iuupl" ;
	skos:altLabel	"Uploading self-created content" ;
	ns11:membership	ns27:i_iuupl ;
	skos:definition	"Individuals have used Internet, in the last 3 months, for uploading self-created content (text, images, photos, videos, music, etc.)" ;
	skos:note	"Biennial indicator not collected in 2011." ;
	skos:topConceptOf	ns1:indicator .
ns7:i_iuvod	rdf:type	skos:Concept ,
		ns10:Indicator ;
	skos:prefLabel	"Individuals watching video on demand from commercial services" ;
	dct:source	ns35:estat_isoc_ci_ac_i ;
	skos:notation	"i_iuvod" ;
	skos:altLabel	"Individuals watching video on demand from commercial services" ;
	ns11:membership	ns9:i_iuvod ;
	skos:definition	"Individuals watching video on demand from commercial services" ;
	skos:topConceptOf	ns1:indicator .
ns7:i_iuvote	rdf:type	skos:Concept ,
		ns10:Indicator ;
	skos:prefLabel	"taking part in on-line consultations or voting to define civic or political issues" ;
	dct:source	ns35:estat_isoc_bde15cua ;
	skos:notation	"i_iuvote" ;
	skos:altLabel	"Taking part in on-line consultations or voting" ;
	ns11:membership	ns27:i_iuvote ;
	skos:definition	"Individuals have used Internet, in the last 3 months, for taking part in on-line consultations or voting to define civic or political issues (e.g. urban planning, signing a petition)" ;
	skos:note	"Biennial indicator not collected in 2012." ;
	skos:topConceptOf	ns1:indicator .
ns7:i_iux	rdf:type	skos:Concept ,
		ns10:Indicator ;
	skos:prefLabel	"Individuals who have never used the internet" ;
	dct:source	ns35:estat_isoc_ci_ifp_iu ;
	skos:notation	"i_iux" ;
	skos:altLabel	"Individuals who have never used the internet" ;
	ns11:membership	ns28:i_iux ;
	skos:topConceptOf	ns1:indicator .
ns7:i_piacadv	rdf:type	skos:Concept ,
		ns10:Indicator ;
	skos:prefLabel	"Individuals not allowing use of personal information for advertising" ;
	dct:source	ns35:estat_isoc_cisci_prv ;
	skos:notation	"i_piacadv" ;
	skos:altLabel	"Individuals not allowing use of personal information for advertising" ;
	ns11:membership	ns32:i_piacadv ;
	skos:definition	"Individuals not allowing use of personal information for advertising" ;
	skos:topConceptOf	ns1:indicator .
ns7:i_sbgood	rdf:type	skos:Concept ,
		ns10:Indicator ;
	skos:prefLabel	"Security concerns kept individual from ordering or buying online" ;
	dct:source	ns35:estat_isoc_cisci_ax ;
	skos:notation	"i_sbgood" ;
	skos:altLabel	"Security concerns kept individual from buying online" ;
	ns11:membership	ns32:i_sbgood ;
	skos:definition	"Security concerns kept individual from ordering or buying goods or services for private use" ;
	skos:topConceptOf	ns1:indicator .
ns7:i_secfl	rdf:type	skos:Concept ,
		ns10:Indicator ;
	skos:prefLabel	"Individuals experienced financial loss" ;
	dct:source	ns35:estat_isoc_cisci_pb ;
	skos:notation	"i_secfl" ;
	skos:altLabel	"Individuals experienced financial loss" ;
	ns11:membership	ns32:i_secfl ;
	skos:definition	"Individuals experienced financial loss due to fraudulent payment (credit or debit) card use OR as a result of receiving fraudulent messages ('phishing') or getting redirected to fake websites asking for personal information ('pharming')." ;
	skos:topConceptOf	ns1:indicator .
ns7:i_secpif1	rdf:type	skos:Concept ,
		ns10:Indicator ;
	skos:prefLabel	"Individuals experienced abuse of personal information and/or other privacy violations" ;
	dct:source	ns35:estat_isoc_cisci_pb ;
	skos:notation	"i_secpif1" ;
	skos:altLabel	"Individuals experienced abuse of personal information/privacy violations " ;
	ns11:membership	ns32:i_secpif1 ;
	skos:definition	"Individuals experienced abuse of personal information sent on the Internet and/or other privacy violations (e.g. abuse of pictures, videos, personal data uploaded on community websites)" ;
	skos:topConceptOf	ns1:indicator .
ns7:i_secvir1	rdf:type	skos:Concept ,
		ns10:Indicator ;
	skos:prefLabel	"Individuals caught a virus or other computer infection resulting in loss of information or time" ;
	dct:source	ns35:estat_isoc_cisci_pb ;
	skos:notation	"i_secvir1" ;
	skos:altLabel	"Individuals caught a virus/computer infection" ;
	ns11:membership	ns32:i_secvir1 ;
	skos:definition	"Individuals caught a virus or other computer infection (e.g. worm or Trojan horse) resulting in loss of information or time" ;
	skos:topConceptOf	ns1:indicator .
ns7:i_skedu	rdf:type	skos:Concept ,
		ns10:Indicator ;
	skos:prefLabel	"Individuals who have obtained ICT skills through formal educational institutions" ;
	dct:source	ns35:estat_isoc_sk_how_i ;
	skos:notation	"i_skedu" ;
	skos:altLabel	"ICT skills obtained through formal educational institutions" ;
	ns11:membership	ns26:i_skedu ;
	skos:definition	"Individuals who have obtained ICT skills through formal educational institutions (school, college, university, etc.)" ;
	skos:topConceptOf	ns1:indicator .
ns7:ict_commit_in_trp	rdf:type	skos:Concept ,
		ns10:Indicator ;
	skos:prefLabel	"EU R&I committed funding for ICT" ;
	dct:source	ns35:abac ;
	skos:notation	"ict_commit_in_trp" ;
	skos:altLabel	"EU R&I committed funding for ICT" ;
	ns11:membership	ns30:ict_commit_in_trp ;
	skos:definition	"Credit commitments for ICT Research and Innovation, during the reference year." ;
	skos:topConceptOf	ns1:indicator .
ns7:ict_exp	rdf:type	skos:Concept ,
		ns10:Indicator ;
	skos:prefLabel	"Export of ICT goods and services" ;
	dct:source	ns35:estat-trade ;
	skos:notation	"ict_exp" ;
	skos:altLabel	"Export of ICT goods and services" ;
	ns11:membership	ns24:ict_exp ;
	skos:definition	"ICT goods include: Computers and peripheral equipment, Communication equipment, Consumer electronic equipment, Electronic components and Miscellaneous. ICT services include: Communications services, Computer and information services. The value of exports cover both intra- and extra- EU.\n\n" ;
	skos:note	"The HS classifications used over time (HS1997, HS2002, HS2007) are bridged using the method described in the OECD document DSTI/ICCP/IIS(2010)5." ;
	skos:topConceptOf	ns1:indicator .
ns7:ict_hgc	rdf:type	ns10:Indicator ,
		skos:Concept ;
	skos:prefLabel	"High Growth Companies in the ICT sector" ;
	dct:source	ns35:euripidis-estat ;
	skos:notation	"ict_hgc" ;
	skos:altLabel	"High Growth ICT Companies" ;
	ns11:membership	ns24:ict_hgc ;
	skos:definition	"High growth companies are companies, with more than 10 employees during the reference year, that grows in employent on average by 10% or more over the last 3 year" ;
	skos:topConceptOf	ns1:indicator .
ns7:ict_imp	rdf:type	ns10:Indicator ,
		skos:Concept ;
	skos:prefLabel	"Import of ICT goods and services" ;
	dct:source	ns35:estat-trade ;
	skos:notation	"ict_imp" ;
	skos:altLabel	"Import of ICT goods and services" ;
	ns11:membership	ns24:ict_imp ;
	skos:definition	"ICT goods include: Computers and peripheral equipment, Communication equipment, Consumer electronic equipment, Electronic components and Miscellaneous. ICT services include: Communications services, Computer and information services. The value of import cover both intra- and extra- EU.\n\n" ;
	skos:note	"The HS classifications used over time (HS1997, HS2002, HS2007) are bridged using the method described in the OECD document DSTI/ICCP/IIS(2010)5." ;
	skos:topConceptOf	ns1:indicator .
ns7:ict_spec3_broad	rdf:type	ns10:Indicator ,
		skos:Concept ;
	skos:prefLabel	"Persons Employed with ICT Specialist Skills (broad measure)" ;
	dct:source	ns35:estat_isoc_sks_itspt ;
	skos:notation	"ict_spec3_broad" ;
	skos:altLabel	"Persons Employed with ICT Specialist Skills (broad measure)" ;
	ns11:membership	ns26:ict_spec3_broad ;
	skos:definition	"The definition of the ICT Specialists' occupations is based on the new ISCO-08 classification. It includes ICT service managers (code 133), ICT professionals (25), ICT technicians (35) and some other groups, from electronic and telecomunnications engineers (215*) up to ICT installers and servicers (7422). Where 4-digit data was not available, the share of computing graduates in the corresponding 3-digit data was estimated. See <a href=\"http://ec.europa.eu/eurostat/cache/metadata/en/isoc_sks_esms.htm\">metadata fiche</a> for a complete explanation of the methodology  (Eurostat table isoc_sks_itspt)" ;
	skos:note	"The definition of the ICT Specialists' occupations before 2010 is based on ISCO-88. It includes codes 213, 312, 313, 1236, 2144, 2359, 3114, 7242, 7243. Due to change of the classification and the related definition, the data on ICT Specialists for 2011 and later are not fully comparable with previous years." ;
	skos:topConceptOf	ns1:indicator .
ns7:ict_specialists	rdf:type	ns10:Indicator ,
		skos:Concept ;
	skos:prefLabel	"Persons Employed with ICT Specialist Skills" ;
	dct:source	ns35:cnect-estat ;
	skos:notation	"ict_specialists" ;
	skos:altLabel	"Persons Employed with ICT Specialist Skills" ;
	ns11:membership	ns18:ict_specialists ;
	skos:definition	" The definition of the ICT Specialists' occupations is based on the new ISCO-08 classification. It includes ICT service managers (code 133), ICT professionals (25), ICT technicians (35) and ICT installers and servicers (7422). " ;
	skos:note	"New ISCO-08 classification of occupations is used from 2011 reference period, replacing the former ISCO-88. Due to change of the classification and the related definition, the data on ICT Specialists for 2011 and later are not fully comparable with previous years. " ;
	skos:topConceptOf	ns1:indicator .
ns7:labour_prod_ict	rdf:type	ns10:Indicator ,
		skos:Concept ;
	skos:prefLabel	"Labour productivity of the ICT sector (per person)" ;
	dct:source	ns35:jrc_ict_randd ;
	skos:notation	"labour_prod_ict" ;
	skos:altLabel	"Labour productivity of the ICT sector (per person)" ;
	ns11:membership	ns24:labour_prod_ict ;
	skos:definition	"Is defined as value added per unit of labour input (persons employed)." ;
	skos:topConceptOf	ns1:indicator .
ns7:mbb_3gcov	rdf:type	ns10:Indicator ,
		skos:Concept ;
	skos:prefLabel	"3G coverage (2005-2010)" ;
	dct:source	ns35:idate ;
	skos:notation	"mbb_3gcov" ;
	skos:altLabel	"3G coverage (2005-2010)" ;
	ns11:membership	ns18:mbb_3gcov ;
	skos:definition	"Coverage is a supply indicator defined as the percentage of population living in areas covered by 3G - third generation mobile networks." ;
	skos:note	"Indicator collected until 2010. Then replaced with a more specific one on advanced 3G mobile broadband (HSPA)." ;
	skos:topConceptOf	ns1:indicator .
ns7:mbb_hspacov	rdf:type	ns10:Indicator ,
		skos:Concept ;
	skos:prefLabel	"Advanced 3G mobile broadband (HSPA) coverage (as a % of households)" ;
	dct:source	ns35:point_topic ;
	skos:notation	"mbb_hspacov" ;
	skos:altLabel	"Advanced 3G mobile broadband coverage" ;
	ns11:membership	ns29:mbb_hspacov ;
	skos:definition	"Coverage is a supply indicator defined as the percentage of Households living in areas covered by advanced third generation mobile broadband (HSPA protocol)" ;
	skos:topConceptOf	ns1:indicator .
ns7:mbb_ltecov	rdf:type	ns10:Indicator ,
		skos:Concept ;
	skos:prefLabel	"4G mobile broadband (LTE) coverage (as a % of households)" ;
	dct:source	ns35:bc2020 ;
	skos:notation	"mbb_ltecov" ;
	skos:altLabel	"4G mobile broadband coverage" ;
	ns11:membership	ns29:mbb_ltecov ;
	skos:definition	"Coverage is a supply indicator defined as the percentage of Households living in areas covered by advanced fourth generation mobile broadband (LTE protocol)" ;
	skos:topConceptOf	ns1:indicator .
ns7:mbb_penet	rdf:type	ns10:Indicator ,
		skos:Concept ;
	skos:prefLabel	"Take-up of mobile broadband (subscriptions/100 people)" ;
	dct:source	ns35:cocom ;
	skos:notation	"mbb_penet" ;
	skos:altLabel	"Mobile broadband take-up  (penetration rate)" ;
	ns11:membership	ns29:mbb_penet ;
	skos:definition	"Mobile Broadband penetration is defined as the number of active mobile broadband SIM cards per 100 people. " ;
	skos:topConceptOf	ns1:indicator .
ns7:mbb_rhspacov	rdf:type	ns10:Indicator ,
		skos:Concept ;
	skos:prefLabel	"Rural advanced 3G mobile broadband (HSPA) coverage (as a % of households)" ;
	dct:source	ns35:point_topic ;
	skos:notation	"mbb_rhspacov" ;
	skos:altLabel	"Rural Advanced 3G mobile broadband coverage" ;
	ns11:membership	ns29:mbb_rhspacov ;
	skos:definition	"Coverage is a supply indicator defined as the percentage of Households living in areas covered by advanced third generation mobile broadband (HSPA protocol). Rural areas are defined as those with less than 100 people per km2." ;
	skos:topConceptOf	ns1:indicator .
ns7:mbb_rltecov	rdf:type	ns10:Indicator ,
		skos:Concept ;
	skos:prefLabel	"Rural 4G mobile broadband (LTE) coverage (as a % of households)" ;
	dct:source	ns35:bc2020 ;
	skos:notation	"mbb_rltecov" ;
	skos:altLabel	"Rural 4G mobile broadband coverage" ;
	ns11:membership	ns29:mbb_rltecov ;
	skos:definition	"Coverage is a supply indicator defined as the percentage of Households living in areas covered by advanced fourth generation mobile broadband (LTE protocol). Rural areas are defined as those with less than 100 people per km2." ;
	skos:topConceptOf	ns1:indicator .
ns7:mob_arpm	rdf:type	ns10:Indicator ,
		skos:Concept ;
	skos:prefLabel	"Average Revenue per Minute in Retail Mobile Voice Communications " ;
	dct:source	ns35:cocom ;
	skos:notation	"mob_arpm" ;
	skos:altLabel	"Average Revenue per Minute in Retail Mobile Voice Communications " ;
	ns11:membership	ns18:mob_arpm ;
	skos:definition	"Total voice related retail revenues divided by total voice minutes" ;
	skos:topConceptOf	ns1:indicator .
ns7:mob_arpu	rdf:type	ns10:Indicator ,
		skos:Concept ;
	skos:prefLabel	"Average Revenue per User (ARPU) in the Retail Mobile Market" ;
	dct:source	ns35:cocom ;
	skos:notation	"mob_arpu" ;
	skos:altLabel	"Average Revenue per User (ARPU) in the Retail Mobile Market" ;
	ns11:membership	ns29:mob_arpu ;
	skos:definition	"Total retail mobile revenues divided by number of active SIM cards" ;
	skos:topConceptOf	ns1:indicator .
ns7:mob_ms	rdf:type	ns10:Indicator ,
		skos:Concept ;
	skos:prefLabel	"Market share of leading operator (in % of active SIM cards)" ;
	dct:source	ns35:cocom ;
	skos:notation	"mob_ms" ;
	skos:altLabel	"Market share of mobile leading operator" ;
	ns11:membership	ns29:mob_ms ;
	skos:definition	"Market share of the market leader based on the number of active SIM cards" ;
	skos:topConceptOf	ns1:indicator .
ns7:mob_mtr	rdf:type	ns10:Indicator ,
		skos:Concept ;
	skos:prefLabel	"Mobile voice termination rate" ;
	dct:source	ns35:cocom ;
	skos:notation	"mob_mtr" ;
	skos:altLabel	"Mobile voice termination rate" ;
	ns11:membership	ns29:mob_mtr ;
	skos:definition	"Wholesale call termination charges in mobile voice tecephony" ;
	skos:topConceptOf	ns1:indicator .
ns7:mob_penet	rdf:type	ns10:Indicator ,
		skos:Concept ;
	skos:prefLabel	"Take-up of mobile  - active SIM cards for voice or data" ;
	dct:source	ns35:cocom ;
	skos:notation	"mob_penet" ;
	skos:altLabel	"Mobile take-up (voice or data)" ;
	ns11:membership	ns29:mob_penet ;
	skos:definition	"Number of active SIM cards divided by population. It includes both voice and data services, installed in telephones, modem, usb keys or other devices." ;
	skos:topConceptOf	ns1:indicator .
ns7:mob_roam	rdf:type	skos:Concept ,
		ns10:Indicator ;
	skos:prefLabel	"Mobile roaming price per minute" ;
	dct:source	ns35:berec_roam ;
	skos:notation	"mob_roam" ;
	skos:altLabel	"Mobile roaming price per minute" ;
	ns11:membership	ns29:mob_roam ;
	skos:definition	"Average retail price per minute (in \u20AC-cents) on Eurotariff for intra-EEA roaming voice calls made" ;
	skos:topConceptOf	ns1:indicator .
ns7:mob_subs	rdf:type	skos:Concept ,
		ns10:Indicator ;
	skos:prefLabel	"Total number of subscriptions (SIM cards)" ;
	dct:source	ns35:cocom ;
	skos:notation	"mob_subs" ;
	skos:altLabel	"Number of mobile subscriptions" ;
	ns11:membership	ns29:mob_subs ;
	skos:definition	"Mobile subscriptions are defined as the number of active SIM cards. It includes both voice and data services, installed in telephones, modem, usb keys or other devices." ;
	skos:topConceptOf	ns1:indicator .
ns7:p_empmd	rdf:type	skos:Concept ,
		ns10:Indicator ;
	skos:prefLabel	"Persons employed which were provided a portable device by their employer (business sector)" ;
	dct:source	ns35:estat_isoc_ci_eu_en2 ;
	skos:notation	"p_empmd" ;
	skos:altLabel	"Persons employed provided with a portable device by their enterprise" ;
	ns11:membership	ns19:p_empmd ;
	skos:definition	"The devices (portable computers, tablets, smartphones, PDA phones, etc.) should be provided for business use and the enterprises pay for all or at least up to a limit the subscription and the use costs. Are included only the enterprises with 10 or more persons employed, from all manufacturing and service sectors, excluding the financial sector." ;
	skos:note	"The 2011 question was limited to portable devices using at least 3G technology to connect to the internet." ;
	skos:topConceptOf	ns1:indicator .
ns7:p_iuse	rdf:type	skos:Concept ,
		ns10:Indicator ;
	skos:prefLabel	"Persons employed using computers with access to the Web at work (business sector)" ;
	dct:source	ns35:estat_isoc_bde15b_p ;
	skos:notation	"p_iuse" ;
	skos:altLabel	"Persons employed using computers at work" ;
	ns11:membership	ns26:p_iuse ;
	skos:definition	"The computers (desktop, laptop, smartphones, etc.) should have access to the World Wide Web and be used at least once a week. Are included only the enterprises with 10 or more persons employed, from all manufacturing and service sectors, excluding the financial sector." ;
	skos:note	"Only the business sector is included in the scope: NACEv2 sectors from C10 to N82 (withouk financial services K) + S951." ;
	skos:topConceptOf	ns1:indicator .
ns7:pay_on_time_projects	rdf:type	skos:Concept ,
		ns10:Indicator ;
	skos:prefLabel	"Projects paid on time" ;
	dct:source	ns35:abac ;
	skos:notation	"pay_on_time_projects" ;
	skos:altLabel	"Projects paid on time" ;
	ns11:membership	ns30:pay_on_time_projects ;
	skos:definition	"Number of research projects paid on time (30-90 days depending on the transaction)" ;
	skos:topConceptOf	ns1:indicator .
ns7:pop	rdf:type	skos:Concept ,
		ns10:Indicator ;
	skos:prefLabel	"Number of individuals aged 16-74" ;
	dct:source	ns35:estat-hh ;
	skos:notation	"pop" ;
	skos:altLabel	"Number of individuals aged 16-74" ;
	ns11:membership	ns13:pop ;
	skos:definition	"Estimation of the number of individuals aged 16-74, for the purpose of the survey on ICT usage by individuals and households." ;
	skos:topConceptOf	ns1:indicator .
ns7:population	rdf:type	skos:Concept ,
		ns10:Indicator ;
	skos:prefLabel	"Total population" ;
	dct:source	ns35:eurostat_pop ;
	skos:notation	"population" ;
	skos:altLabel	"Total population" ;
	ns11:membership	ns13:population ;
	skos:definition	"Total population estimate 1st of January of the same year (Eurostat table demo_pjan)" ;
	skos:topConceptOf	ns1:indicator .
ns7:price_internet_fixed_tel	rdf:type	skos:Concept ,
		ns10:Indicator ;
	skos:prefLabel	"Monthly price of  Fixed Broadband Internet Access offers including Fixed Telephony" ;
	dct:source	ns35:biac ;
	skos:notation	"price_internet_fixed_tel" ;
	skos:altLabel	"Monthly price of  Internet + Fixed Telephony" ;
	ns11:membership	ns14:price_internet_fixed_tel ;
	skos:definition	"Monthly price of Fixed Broadband Internet Access offers including Fixed Telephony, including value added tax, excluding the aditional cost of telephony or cable line (if any). The minimum and median prices refer to the group of similar subscriptions offered by internet service providers. Offers are not weigthed with market shares, so the offers' median price cannot be interpreted as the median price paid by consumers." ;
	skos:note	"If no data is present for a country, it is because no corresponding offers have been found on the national market." ;
	skos:topConceptOf	ns1:indicator .
ns7:price_internet_fixed_tel_tv	rdf:type	skos:Concept ,
		ns10:Indicator ;
	skos:prefLabel	"Monthly price of Internet Acccess + Fixed Telephony + TV bundles" ;
	dct:source	ns35:biac ;
	skos:notation	"price_internet_fixed_tel_tv" ;
	skos:altLabel	"Monthly price of Internet + Fixed Telephony + TV" ;
	ns11:membership	ns14:price_internet_fixed_tel_tv ;
	skos:definition	"Monthly price of Fixed Broadband Internet Access offers including Fixed Telephony and TV (analogue or digital television service), including value added tax, excluding the aditional cost of telephony or cable line (if any). The minimum and median prices refer to the group of similar subscriptions offered by internet service providers. Offers are not weigthed with market shares, so the offers' median price cannot be interpreted as the median price paid by consumers." ;
	skos:note	"If no data is present for a country, it is because no corresponding offers have been found on the national market." ;
	skos:topConceptOf	ns1:indicator .
ns7:price_internet_only	rdf:type	skos:Concept ,
		ns10:Indicator ;
	skos:prefLabel	"Monthly price of standalone internet access" ;
	dct:source	ns35:biac ;
	skos:notation	"price_internet_only" ;
	skos:altLabel	"Monthly price of Internet Access only" ;
	ns11:membership	ns14:price_internet_only ;
	skos:definition	"Monthly price of standalone Fixed Broadband Internet Access offers, including value added tax, excluding the additional cost of telephony or cable line (if any). The minimum and median prices refer to the group of similar subscriptions offered by internet service providers. Offers are not weigthed with market shares, so the offers' median price cannot be interpreted as the median price paid by consumers." ;
	skos:note	"If no data is present for a country, it is because no corresponding offers have been found on the national market." ;
	skos:topConceptOf	ns1:indicator .
ns7:spectrum_wbb	rdf:type	skos:Concept ,
		ns10:Indicator ;
	skos:prefLabel	"Spectrum assigned for wireless broadband in EU harmonised bands" ;
	dct:source	ns35:eco_report_03_efis_comm ;
	skos:notation	"spectrum_wbb" ;
	skos:altLabel	"Assigned spectrum WBB (EU harmonised bands)" ;
	ns11:membership	ns29:spectrum_wbb ;
	skos:definition	"Amount of spectrum assigned by Member States for wireless mobile broadband comunications (WBB) within the ranges harmonised by the European Union. Charts allow to compare with the total value of EU HARMONISED bands and with a simple EU AVERAGE of countries assignements. The policy target is to harmonise and assign 1200 MHz to WBB." ;
	skos:topConceptOf	ns1:indicator .
ns7:st_grad	rdf:type	skos:Concept ,
		ns10:Indicator ;
	skos:prefLabel	"Science and technology graduates" ;
	dct:source	ns35:estat_tps00188 ;
	skos:notation	"st_grad" ;
	skos:altLabel	"Science and technology graduates" ;
	ns11:membership	ns25:st_grad ;
	skos:definition	"Tertiary graduates in science and technology per 1 000 inhabitants aged 20-29 years includes new tertiary graduates in a calendar year from both public and private institutions completing graduate and post graduate studies compared to an age group that corresponds to the typical graduation age in most countries." ;
	skos:topConceptOf	ns1:indicator .
ns7:tel_ftr	rdf:type	skos:Concept ,
		ns10:Indicator ;
	skos:prefLabel	"Fixed voice termination rate" ;
	dct:source	ns35:cocom ;
	skos:notation	"tel_ftr" ;
	skos:altLabel	"Fixed voice termination rate" ;
	ns11:membership	ns33:tel_ftr ;
	skos:definition	"Wholesale call termination charges of the incumbent operator in fixed voice tecephony for local calls" ;
	skos:topConceptOf	ns1:indicator .
ns7:tel_inv	rdf:type	skos:Concept ,
		ns10:Indicator ;
	skos:prefLabel	"Total investment in networks by the electronic communications sector" ;
	dct:source	ns35:cocom ;
	skos:notation	"tel_inv" ;
	skos:altLabel	"Total investment in networks by the electronic communications sector" ;
	ns11:membership	ns33:tel_inv ;
	skos:definition	"Total investment includes both tangible and intangible investment in telecommunication networks (without license fees) by all telecom operators" ;
	skos:topConceptOf	ns1:indicator .
ns7:tel_llu	rdf:type	skos:Concept ,
		ns10:Indicator ;
	skos:prefLabel	"Local Loop Unbundling: total monthly charge" ;
	dct:source	ns35:cocom ;
	skos:notation	"tel_llu" ;
	skos:altLabel	"Local Loop Unbundling: total monthly charge" ;
	ns11:membership	ns33:tel_llu ;
	skos:definition	"The monthly total wholesale cost for Local Loop Unbundling charged by incumbent operators, Calculated as the sum of the monthly charge and 1/36  of the conncetion fee " ;
	skos:topConceptOf	ns1:indicator .
ns7:tel_rev	rdf:type	skos:Concept ,
		ns10:Indicator ;
	skos:prefLabel	"Total revenues of the electronic communications sector" ;
	dct:source	ns35:cocom ;
	skos:notation	"tel_rev" ;
	skos:altLabel	"Total revenues of the electronic communications sector" ;
	ns11:membership	ns33:tel_rev ;
	skos:definition	"Total includes wholesale and retail revenues from electronic communications perceived in the reference year by all telecom operators (VAT excluded)" ;
	skos:topConceptOf	ns1:indicator .
ns7:transparent_egov	rdf:type	ns10:Indicator ,
		skos:Concept ;
	skos:prefLabel	"Transparency Score of eGovernment Services" ;
	dct:source	ns35:egov_bench12 ;
	skos:notation	"transparent_egov" ;
	skos:altLabel	"Transparency Score" ;
	ns11:membership	ns18:transparent_egov ;
	skos:definition	"The Transparency score indicates to what extent eGovernment services are transparent. It assesses three aspects of transparency: to what extent public authorities are transparent regarding their own responsibilities and performance, to what extent they are transparent regarding the process of service delivery, and to what extent they are transparent regarding the personal data involved in service delivery." ;
	skos:topConceptOf	ns1:indicator .
ns7:ttg_in_scope	rdf:type	ns10:Indicator ,
		skos:Concept ;
	skos:prefLabel	"Grants signed within scope" ;
	dct:source	ns35:corda ;
	skos:notation	"ttg_in_scope" ;
	skos:altLabel	"Grants signed within scope" ;
	ns11:membership	ns30:ttg_in_scope ;
	skos:definition	"The Time to Grant (TTG) is defined as the time lapsed from a call's closing date (deadline for submission of proposals) to that of a grant signature by the European Commission. In the case of two-stage calls for proposals, it is the second stage call deadline that is used in the calculation of the Time to Grant. Time to grant is expressed in calendar days. For H2020, signature within scope reflects the grants signed in less than 245 days." ;
	skos:topConceptOf	ns1:indicator .
ns7:user_centric_egov	rdf:type	ns10:Indicator ,
		skos:Concept ;
	skos:prefLabel	"User Centricity Score of eGovernment services" ;
	dct:source	ns35:egov_bench12 ;
	skos:notation	"user_centric_egov" ;
	skos:altLabel	"User Centricity Score" ;
	ns11:membership	ns18:user_centric_egov ;
	skos:definition	"The User centricity score indicates to what extent (information about) a service is provided online and how usable it is (e.g., if support, help and feedback functionality exist online), as well as quality assessments by researchers on the service's ease and speed of use." ;
	skos:topConceptOf	ns1:indicator .
ns7:val_add_ict	rdf:type	ns10:Indicator ,
		skos:Concept ;
	skos:prefLabel	"Value added of the ICT sector" ;
	dct:source	ns35:jrc_ict_randd ;
	skos:notation	"val_add_ict" ;
	skos:altLabel	"Value added of the ICT sector" ;
	ns11:membership	ns24:val_add_ict ;
	skos:definition	"Value added. In the System of National Accounts it is defined as the value of output less the value of intermediate consumption; it is a measure of the contribution to GDP made by an individual producer, industry or sector." ;
	skos:topConceptOf	ns1:indicator .
ns7:vod	rdf:type	ns10:Indicator ,
		skos:Concept ;
	skos:prefLabel	"Households subscribed to Video on Demand" ;
	dct:source	ns35:ihs_tech ;
	skos:notation	"vod" ;
	skos:altLabel	"Households subscribed to Video on Demand" ;
	ns11:membership	ns9:vod ;
	skos:definition	"Percentage of households subscribing to any form of Video on Demand; EU average calculated as the average of the 26 MS (for which data is available) weighted by the number of households in each of them in 2013" ;
	skos:topConceptOf	ns1:indicator .
ns7:wid_ius	rdf:type	ns10:Indicator ,
		skos:Concept ;
	skos:prefLabel	"2 Internet user skills" ;
	dct:source	ns35: ;
	skos:notation	"wid_ius" ;
	skos:altLabel	"2 Internet user skills" ;
	ns11:membership	ns34:wid_ius ;
	skos:definition	"WID Internet user skills dimension calculated as the weighted average of the three indicators: 2.1 At least basic digital skills  (33.3%), 2.2 Above basic digital skills (33.3%), 2.3 Software skills (33.3%)." ;
	skos:topConceptOf	ns1:indicator .
ns7:wid_ius_abs	rdf:type	ns10:Indicator ,
		skos:Concept ;
	skos:prefLabel	"2.2 Above basic digital skills" ;
	dct:source	ns35: ;
	skos:notation	"wid_ius_abs" ;
	skos:altLabel	"2.2 Above basic digital skills" ;
	ns11:membership	ns34:wid_ius_abs ;
	skos:definition	"People with above basic digital skills in each of the following four dimensions: information, communication, problem solving, software for content creation. " ;
	skos:topConceptOf	ns1:indicator .
ns7:wid_ius_bs	rdf:type	ns10:Indicator ,
		skos:Concept ;
	skos:prefLabel	"2.1 At least basic digital skills" ;
	dct:source	ns35: ;
	skos:notation	"wid_ius_bs" ;
	skos:altLabel	"2.1 At least basic digital skills" ;
	ns11:membership	ns34:wid_ius_bs ;
	skos:definition	"People with  at least basic digital skills in each of the following four dimensions: information, communication, problem solving, software for content creation. People possessing, at a minimum, the skills required to perform activities such as using e-mail, editing tools, installing new devices, etc. Further details on calculation methodology here: https://ec.europa.eu/digital-single-market/en/news/new-comprehensive-digital-skills-indicator" ;
	skos:topConceptOf	ns1:indicator .
ns7:wid_ius_ss	rdf:type	ns10:Indicator ,
		skos:Concept ;
	skos:prefLabel	"2.3 Software skills" ;
	dct:source	ns35: ;
	skos:notation	"wid_ius_ss" ;
	skos:altLabel	"2.3 At least basic software skills" ;
	ns11:membership	ns34:wid_ius_ss ;
	skos:definition	"People who, in addition to having used basic software features such as word processing, used advanced spreadsheet functions, created a presentation or document integrating text, pictures and tables or charts, or wrote code in a programming language. " ;
	skos:topConceptOf	ns1:indicator .
ns7:wid_score	rdf:type	ns10:Indicator ,
		skos:Concept ;
	skos:prefLabel	"Women in Digital (WID) score" ;
	dct:source	ns35: ;
	skos:notation	"wid_score" ;
	skos:altLabel	"Women in Digital (WID) score" ;
	ns11:membership	ns34:wid_score ;
	skos:definition	"Women in digital score calculated as the weighted average of the three sub-dimensions: 1 Use of internet  (33.3%), 2 Internet users skills (33.3%), 3 Specialist skills and employment (33.3%).\n\n" ;
	skos:topConceptOf	ns1:indicator .
ns7:wid_sse	rdf:type	ns10:Indicator ,
		skos:Concept ;
	skos:prefLabel	"3 Specialist skills and employment" ;
	dct:source	ns35: ;
	skos:notation	"wid_sse" ;
	skos:altLabel	"3 Specialist skills and employment" ;
	ns11:membership	ns34:wid_sse ;
	skos:definition	"WID Use of Internet Dimension calculated as the weighted average of the three indicators: \n3.1 STEM graduates (33.3%), 3.2 ICT specialists (33.3%), 3.3 Gender pay gap  (33.3%)." ;
	skos:topConceptOf	ns1:indicator .
ns7:wid_sse_gpg	rdf:type	ns10:Indicator ,
		skos:Concept ;
	skos:prefLabel	"3.3 Gender pay gap" ;
	dct:source	ns35: ;
	skos:notation	"wid_sse_gpg" ;
	skos:altLabel	"3.3 Unadjusted gender pay gap" ;
	ns11:membership	ns34:wid_sse_gpg ;
	skos:definition	"Gender pay gap in unadjusted form, measured as the difference between average gross hourly earnings of male paid employees and  female paid employees as a percentage of average gross hourly earnings of male paid employees. The indicator has been defined as unadjusted, because it gives an overall picture of gender inequalities in terms of pay and measures a concept which is broader than the concept of equal pay for equal work. All employees working in firms with ten or more employees, without restrictions for age and hours worked, are included." ;
	skos:topConceptOf	ns1:indicator .
ns7:wid_sse_icts	rdf:type	ns10:Indicator ,
		skos:Concept ;
	skos:prefLabel	"3.2 ICT specialists" ;
	dct:source	ns35: ;
	skos:notation	"wid_sse_icts" ;
	skos:altLabel	"3.2 ICT specialists" ;
	ns11:membership	ns34:wid_sse_icts ;
	skos:definition	"Employed ICT specialists. Broad definition based on the ISCO-08 classification and including jobs like ICT service managers, ICT professionals, ICT technicians, ICT installers and servicers." ;
	skos:topConceptOf	ns1:indicator .
ns7:wid_sse_stem	rdf:type	ns10:Indicator ,
		skos:Concept ;
	skos:prefLabel	"3.1 STEM graduates" ;
	dct:source	ns35: ;
	skos:notation	"wid_sse_stem" ;
	skos:altLabel	"3.1 STEM graduates" ;
	ns11:membership	ns34:wid_sse_stem ;
	skos:definition	"People with a degree in a science, technology, maths or engineering-related subject" ;
	skos:topConceptOf	ns1:indicator .
ns7:wid_ui	rdf:type	ns10:Indicator ,
		skos:Concept ;
	skos:prefLabel	"1 Use of internet" ;
	dct:source	ns35: ;
	skos:notation	"wid_ui" ;
	skos:altLabel	"1 Use of internet" ;
	ns11:membership	ns34:wid_ui ;
	skos:definition	"WID Use of internet dimension calculated as the weighted average of the six indicators: \r\n1.1 Regular internet use (16.67%), 1.2 People who never used the internet (16.67%), 1.3 Online banking (16.67%), 1.4 Doing an online course (16.67%), 1.5 Online consultations or voting (16.67%), 1.6 eGovernment users (16.67%)." ;
	skos:topConceptOf	ns1:indicator .
ns7:wid_ui_egov	rdf:type	ns10:Indicator ,
		skos:Concept ;
	skos:prefLabel	"1.6 eGovernment users " ;
	dct:source	ns35: ;
	skos:notation	"wid_ui_egov" ;
	skos:altLabel	"1.6 eGovernment users " ;
	ns11:membership	ns34:wid_ui_egov ;
	skos:definition	"People who sent filled forms to public authorities, over the internet, previous 12 months " ;
	skos:topConceptOf	ns1:indicator .
ns7:wid_ui_ib	rdf:type	skos:Concept ,
		ns10:Indicator ;
	skos:prefLabel	"1.3 Online banking" ;
	dct:source	ns35: ;
	skos:notation	"wid_ui_ib" ;
	skos:altLabel	"1.3 Online banking" ;
	ns11:membership	ns34:wid_ui_ib ;
	skos:definition	"People who used the Internet to use online banking " ;
	skos:topConceptOf	ns1:indicator .
ns7:wid_ui_iu	rdf:type	skos:Concept ,
		ns10:Indicator ;
	skos:prefLabel	"1.1 Regular internet use" ;
	dct:source	ns35: ;
	skos:notation	"wid_ui_iu" ;
	skos:altLabel	"1.1 Regular internet use" ;
	ns11:membership	ns34:wid_ui_iu ;
	skos:definition	"People who used the Internet at least once a week" ;
	skos:topConceptOf	ns1:indicator .
ns7:wid_ui_nui	rdf:type	skos:Concept ,
		ns10:Indicator ;
	skos:prefLabel	"1.2 People who never used the internet" ;
	dct:source	ns35: ;
	skos:notation	"wid_ui_nui" ;
	skos:altLabel	"1.2 People who never used the internet" ;
	ns11:membership	ns34:wid_ui_nui ;
	skos:definition	"People who never used the Internet" ;
	skos:topConceptOf	ns1:indicator .
ns7:wid_ui_oc	rdf:type	skos:Concept ,
		ns10:Indicator ;
	skos:prefLabel	"1.4 Doing an online course" ;
	dct:source	ns35: ;
	skos:notation	"wid_ui_oc" ;
	skos:altLabel	"1.4 Doing an online course" ;
	ns11:membership	ns34:wid_ui_oc ;
	skos:definition	"People who used the Internet for doing an online course (on any subject)" ;
	skos:topConceptOf	ns1:indicator .
ns7:wid_ui_part	rdf:type	skos:Concept ,
		ns10:Indicator ;
	skos:prefLabel	"1.5 Online consultations or voting" ;
	dct:source	ns35: ;
	skos:notation	"wid_ui_part" ;
	skos:altLabel	"1.5 Online consultations or voting" ;
	ns11:membership	ns34:wid_ui_part ;
	skos:definition	"People who took part in on-line consultations or voting to define civic or political issues (e.g. urban planning, signing a petition)" ;
	skos:topConceptOf	ns1:indicator .
ns34:old_wid_ui_ps	rdf:type	ns10:IndicatorToGroupMembership ;
	rdfs:label	"wid" ;
	ns11:member-of	ns12:wid ;
	ns11:order	"6" .
ns7:old_wid_ui_ps	rdf:type	ns10:Indicator ,
		skos:Concept ;
	skos:prefLabel	"1.4 Using professional social networks" ;
	dct:source	ns35: ;
	skos:notation	"old_wid_ui_ps" ;
	skos:altLabel	"1.4 Using professional social networks" ;
	ns11:membership	ns34:old_wid_ui_ps ;
	skos:definition	"People who used Internet for participating in social or professional networks" ;
	skos:topConceptOf	ns1:indicator .
ns7:e_gov_4b_bm_us	rdf:type	ns10:Indicator ,
		skos:Concept ;
	skos:prefLabel	"4b Business Mobility - Usability" ;
	dct:source	ns35:egov_bench12_17 ;
	skos:notation	"e_gov_4b_bm_us" ;
	skos:altLabel	"4c Business Mobility - Usability" ;
	ns11:membership	ns21:e_gov_4b_bm_us ;
	skos:definition	"Online support and help features on services aimed at foreign businesses." ;
	skos:topConceptOf	ns1:indicator .
ns15:bb_rvhcncov	rdf:type	ns10:IndicatorToGroupMembership ;
	rdfs:label	"broadband" ;
	ns11:member-of	ns12:broadband ;
	ns11:order	"2" .
ns15:bb_vhcncov	rdf:type	ns10:IndicatorToGroupMembership ;
	rdfs:label	"broadband" ;
	ns11:member-of	ns12:broadband ;
	ns11:order	"1" .
ns21:e_gov_1_uc	rdf:type	ns10:IndicatorToGroupMembership ;
	rdfs:label	"egovernment" ;
	ns11:member-of	ns12:egovernment ;
	ns11:order	"1111" .
ns21:e_gov_1a_uc_oa	rdf:type	ns10:IndicatorToGroupMembership ;
	rdfs:label	"egovernment" ;
	ns11:member-of	ns12:egovernment ;
	ns11:order	"11111" .
ns21:e_gov_1b_uc_mf	rdf:type	ns10:IndicatorToGroupMembership ;
	rdfs:label	"egovernment" ;
	ns11:member-of	ns12:egovernment ;
	ns11:order	"11112" .
ns21:e_gov_1c_uc_us	rdf:type	ns10:IndicatorToGroupMembership ;
	rdfs:label	"egovernment" ;
	ns11:member-of	ns12:egovernment ;
	ns11:order	"11113" .
ns21:e_gov_2_tr	rdf:type	ns10:IndicatorToGroupMembership ;
	rdfs:label	"egovernment" ;
	ns11:member-of	ns12:egovernment ;
	ns11:order	"1112" .
ns21:e_gov_2a_tr_sd	rdf:type	ns10:IndicatorToGroupMembership ;
	rdfs:label	"egovernment" ;
	ns11:member-of	ns12:egovernment ;
	ns11:order	"11121" .
ns21:e_gov_2c_tr_pd	rdf:type	ns10:IndicatorToGroupMembership ;
	rdfs:label	"egovernment" ;
	ns11:member-of	ns12:egovernment ;
	ns11:order	"11122" .
ns21:e_gov_2c_tr_sd	rdf:type	ns10:IndicatorToGroupMembership ;
	rdfs:label	"egovernment" ;
	ns11:member-of	ns12:egovernment ;
	ns11:order	"11123" .
ns21:e_gov_2x_tr_po	rdf:type	ns10:IndicatorToGroupMembership ;
	rdfs:label	"egovernment" ;
	ns11:member-of	ns12:egovernment ;
	ns11:order	"11124" .
ns21:e_gov_3_ke	rdf:type	ns10:IndicatorToGroupMembership ;
	rdfs:label	"egovernment" ;
	ns11:member-of	ns12:egovernment ;
	ns11:order	"1113" .
ns21:e_gov_3a_ke_eid	rdf:type	ns10:IndicatorToGroupMembership ;
	rdfs:label	"egovernment" ;
	ns11:member-of	ns12:egovernment ;
	ns11:order	"11131" .
ns21:e_gov_3b_ke_edoc	rdf:type	ns10:IndicatorToGroupMembership ;
	rdfs:label	"egovernment" ;
	ns11:member-of	ns12:egovernment ;
	ns11:order	"11132" .
ns21:e_gov_3c_ke_as	rdf:type	ns10:IndicatorToGroupMembership ;
	rdfs:label	"egovernment" ;
	ns11:member-of	ns12:egovernment ;
	ns11:order	"11133" .
ns21:e_gov_3d_ke_dp	rdf:type	ns10:IndicatorToGroupMembership ;
	rdfs:label	"egovernment" ;
	ns11:member-of	ns12:egovernment ;
	ns11:order	"11134" .
ns21:e_gov_4_cb	rdf:type	ns10:IndicatorToGroupMembership ;
	rdfs:label	"egovernment" ;
	ns11:member-of	ns12:egovernment ;
	ns11:order	"1114" .
ns21:e_gov_4a_cb_oa	rdf:type	ns10:IndicatorToGroupMembership ;
	rdfs:label	"egovernment" ;
	ns11:member-of	ns12:egovernment ;
	ns11:order	"11141" .
ns21:e_gov_4b_cb_us	rdf:type	ns10:IndicatorToGroupMembership ;
	rdfs:label	"egovernment" ;
	ns11:member-of	ns12:egovernment ;
	ns11:order	"11142" .
ns21:e_gov_4c_cb_eid	rdf:type	ns10:IndicatorToGroupMembership ;
	rdfs:label	"egovernment" ;
	ns11:member-of	ns12:egovernment ;
	ns11:order	"11143" .
ns21:e_gov_4d_cb_edoc	rdf:type	ns10:IndicatorToGroupMembership ;
	rdfs:label	"egovernment" ;
	ns11:member-of	ns12:egovernment ;
	ns11:order	"11144" .
ns21:e_gov_dpsc	rdf:type	ns10:IndicatorToGroupMembership ;
	rdfs:label	"egovernment" ;
	ns11:member-of	ns12:egovernment ;
	ns11:order	"3" .
ns21:e_gov_od	rdf:type	ns10:IndicatorToGroupMembership ;
	rdfs:label	"egovernment" ;
	ns11:member-of	ns12:egovernment ;
	ns11:order	"5" .
<http://semantic.digital-agenda-data.eu/codelist/indicator-group/mobile/5g_read>	rdf:type	ns10:IndicatorToGroupMembership ;
	rdfs:label	"mobile" ;
	ns11:member-of	ns12:mobile ;
	ns11:order	"3" .
ns29:mbb_5gcov	rdf:type	ns10:IndicatorToGroupMembership ;
	rdfs:label	"mobile" ;
	ns11:member-of	ns12:mobile ;
	ns11:order	"1" .
ns29:mbb_r5gcov	rdf:type	ns10:IndicatorToGroupMembership ;
	rdfs:label	"mobile" ;
	ns11:member-of	ns12:mobile ;
	ns11:order	"2" .
<http://semantic.digital-agenda-data.eu/codelist/indicator/5g_read>	rdf:type	ns10:Indicator ,
		skos:Concept ;
	skos:prefLabel	"5G readiness" ;
	dct:source	ns35:cocom_new ;
	skos:notation	"5g_read" ;
	skos:altLabel	"5G readiness" ;
	ns11:membership	<http://semantic.digital-agenda-data.eu/codelist/indicator-group/mobile/5g_read> ;
	skos:definition	"The amount of spectrum assigned and ready for 5G use within the so-called 5G pioneer bands. These bands are 700 MHz (703-733 MHz and 758-788 MHz), 3.6 GHz (3400-3800 MHz) and 26 GHz (1000 MHz within 24250-27500 MHz). All three spectrum bands have an equal weight." ;
	skos:topConceptOf	ns1:indicator .
ns7:bb_rvhcncov	rdf:type	ns10:Indicator ,
		skos:Concept ;
	skos:prefLabel	"Rural Fixed Very High Capacity Network (VHCN) coverage" ;
	dct:source	ns35:bc2020 ;
	skos:notation	"bb_rvhcncov" ;
	skos:altLabel	"Rural Fixed Very High Capacity Network (VHCN) coverage" ;
	ns11:membership	ns15:bb_rvhcncov ;
	skos:definition	"Percentage of households covered by any fixed VHCN. The technologies considered are FTTH and FTTB for 2015-2018 and FTTH, FTTB and Cable Docsis 3.1 for 2019 onwards." ;
	skos:topConceptOf	ns1:indicator .
ns7:bb_vhcncov	rdf:type	ns10:Indicator ,
		skos:Concept ;
	skos:prefLabel	"Fixed Very High Capacity Network (VHCN) coverage" ;
	dct:source	ns35:bc2020 ;
	skos:notation	"bb_vhcncov" ;
	skos:altLabel	"Fixed Very High Capacity Network (VHCN) coverage" ;
	ns11:membership	ns15:bb_vhcncov ;
	skos:definition	"Percentage of households covered by any fixed VHCN. The technologies considered are FTTH and FTTB for 2015-2018 and FTTH, FTTB and Cable Docsis 3.1 for 2019 onwards.\nRural areas are defined as those with less than 100 people per km2." ;
	skos:topConceptOf	ns1:indicator .
ns7:e_gov_1_uc	rdf:type	ns10:Indicator ,
		skos:Concept ;
	skos:prefLabel	"1 User centricity" ;
	dct:source	ns35:egov_bench ;
	skos:notation	"e_gov_1_uc" ;
	skos:altLabel	"1 User centricity" ;
	ns11:membership	ns21:e_gov_1_uc ;
	skos:definition	"The extent to which information and services are available online, supported online and compatible with mobile devices.D362" ;
	skos:topConceptOf	ns1:indicator .
ns7:e_gov_1a_uc_oa	rdf:type	ns10:Indicator ,
		skos:Concept ;
	skos:prefLabel	"1.1 User centricity - Online availability" ;
	dct:source	ns35:egov_bench ;
	skos:notation	"e_gov_1a_uc_oa" ;
	skos:altLabel	"1.1 User centricity - Online availability" ;
	ns11:membership	ns21:e_gov_1a_uc_oa ;
	skos:definition	"The extent to which informational and transactional services and information concerning these services is provided online, and can be reached via a portal website." ;
	skos:topConceptOf	ns1:indicator .
ns7:e_gov_1b_uc_mf	rdf:type	ns10:Indicator ,
		skos:Concept ;
	skos:prefLabel	"1.2 User centricity - Mobile friendliness" ;
	dct:source	ns35:egov_bench ;
	skos:notation	"e_gov_1b_uc_mf" ;
	skos:altLabel	"1.2 User centricity - Mobile friendliness" ;
	ns11:membership	ns21:e_gov_1b_uc_mf ;
	skos:definition	"The extent to which services are provided through a mobile-friendly interface, an interface that is responsive to the mobile device." ;
	skos:topConceptOf	ns1:indicator .
ns7:e_gov_1c_uc_us	rdf:type	ns10:Indicator ,
		skos:Concept ;
	skos:prefLabel	"1.3 User centricity - User support" ;
	dct:source	ns35:egov_bench ;
	skos:notation	"e_gov_1c_uc_us" ;
	skos:altLabel	"1.3 User centricity - User support" ;
	ns11:membership	ns21:e_gov_1c_uc_us ;
	skos:definition	"The extent to which online support, help features, and feedback mechanisms are available." ;
	skos:topConceptOf	ns1:indicator .
ns7:e_gov_2_tr	rdf:type	ns10:Indicator ,
		skos:Concept ;
	skos:prefLabel	"2 Transparency" ;
	dct:source	ns35:egov_bench ;
	skos:notation	"e_gov_2_tr" ;
	skos:altLabel	"2 Transparency" ;
	ns11:membership	ns21:e_gov_2_tr ;
	skos:definition	"The extent to which service processes are transparent, services are designed with user involvement and users can manage their personal data." ;
	skos:topConceptOf	ns1:indicator .
ns7:e_gov_2a_tr_sd	rdf:type	ns10:Indicator ,
		skos:Concept ;
	skos:prefLabel	"2.1 Transparency - Transparency of service delivery" ;
	dct:source	ns35:egov_bench ;
	skos:notation	"e_gov_2a_tr_sd" ;
	skos:altLabel	"2.1 Transparency - Transparency of service delivery" ;
	ns11:membership	ns21:e_gov_2a_tr_sd ;
	skos:definition	"The extent to which the service process and expectations are clarified." ;
	skos:topConceptOf	ns1:indicator .
ns7:e_gov_2c_tr_pd	rdf:type	ns10:Indicator ,
		skos:Concept ;
	skos:prefLabel	"2.2 Transparency - Transparency of personal data" ;
	dct:source	ns35:egov_bench ;
	skos:notation	"e_gov_2c_tr_pd" ;
	skos:altLabel	"2.2 Transparency - Transparency of personal data" ;
	ns11:membership	ns21:e_gov_2c_tr_pd ;
	skos:definition	"The extent to which user can manage their personal data held by government organisations." ;
	skos:topConceptOf	ns1:indicator .
ns7:e_gov_2c_tr_sd	rdf:type	ns10:Indicator ,
		skos:Concept ;
	skos:prefLabel	"2.3 Transparency - Transparency of service design" ;
	dct:source	ns35:egov_bench ;
	skos:notation	"e_gov_2c_tr_sd" ;
	skos:altLabel	"2.3 Transparency - Transparency of service design" ;
	ns11:membership	ns21:e_gov_2c_tr_sd ;
	skos:definition	"The extent to which user are informed on and involved in policy and service design processes." ;
	skos:topConceptOf	ns1:indicator .
ns7:e_gov_2x_tr_po	rdf:type	ns10:Indicator ,
		skos:Concept ;
	skos:prefLabel	"2.X Transparency - Transparency of public organisations (old indicator)" ;
	dct:source	ns35:egov_bench ;
	skos:notation	"e_gov_2x_tr_po" ;
	skos:altLabel	"2.X Transparency - Transparency of public organisations (old indicator)" ;
	ns11:membership	ns21:e_gov_2x_tr_po ;
	skos:definition	"The extent to which public administrations publish information about their organisations (e.g. finance, organisational structure and responsibilities), and about their activities (e.g. the decision-making processes and regulations). " ;
	skos:note	"This indicator has been discontinued starting from 2020" ;
	skos:topConceptOf	ns1:indicator .
ns7:e_gov_3_ke	rdf:type	skos:Concept ,
		ns10:Indicator ;
	skos:prefLabel	"3 Key Enablers" ;
	dct:source	ns35:egov_bench ;
	skos:notation	"e_gov_3_ke" ;
	skos:altLabel	"3 Key Enablers" ;
	ns11:membership	ns21:e_gov_3_ke ;
	skos:definition	"The extent to which main IT enablers (eIDs, eDocuments, Authentic sources, Digital post and security) are available during services processes, which can be used to assess the presence of the technical pre-conditions of the efficient and effective use of online services." ;
	skos:topConceptOf	ns1:indicator .
ns7:e_gov_3a_ke_eid	rdf:type	skos:Concept ,
		ns10:Indicator ;
	skos:prefLabel	"3.1 Key enablers - eID" ;
	dct:source	ns35:egov_bench ;
	skos:notation	"e_gov_3a_ke_eid" ;
	skos:altLabel	"3.1 Key enablers - eID" ;
	ns11:membership	ns21:e_gov_3a_ke_eid ;
	skos:definition	"The extent to which electronic Identification (eID), any means accepted by eGovernment services (e.g. smartcards, username and password) for online identification, can be used during service processes." ;
	skos:topConceptOf	ns1:indicator .
ns7:e_gov_3b_ke_edoc	rdf:type	skos:Concept ,
		ns10:Indicator ;
	skos:prefLabel	"3.2 Key enabler - eDocuments" ;
	dct:source	ns35:egov_bench ;
	skos:notation	"e_gov_3b_ke_edoc" ;
	skos:altLabel	"3.2 Key enabler - eDocuments" ;
	ns11:membership	ns21:e_gov_3b_ke_edoc ;
	skos:definition	"The extent to which electronic documents (eDocuments), any document in digital form that the user needs to submit/upload in order to complete an eGovernment service, or that the user obtains as a proof or a result of the service (e.g. certificate, diploma, proof of registration) can be used during service processes. " ;
	skos:topConceptOf	ns1:indicator .
ns7:e_gov_3c_ke_as	rdf:type	skos:Concept ,
		ns10:Indicator ;
	skos:prefLabel	"3.3 Key enabler - Authentic sources" ;
	dct:source	ns35:egov_bench ;
	skos:notation	"e_gov_3c_ke_as" ;
	skos:altLabel	"3.3 Key enabler - Authentic sources" ;
	ns11:membership	ns21:e_gov_3c_ke_as ;
	skos:definition	"The extent to which Authentic Sources, base registries used by governments to automatically validate or fetch data relating to citizens or businesses, can be used during the service process." ;
	skos:topConceptOf	ns1:indicator .
ns7:e_gov_3d_ke_dp	rdf:type	skos:Concept ,
		ns10:Indicator ;
	skos:prefLabel	"3.4 Key enabler - Digital Post" ;
	dct:source	ns35:egov_bench ;
	skos:notation	"e_gov_3d_ke_dp" ;
	skos:altLabel	"3.4 Key enabler - Digital Post" ;
	ns11:membership	ns21:e_gov_3d_ke_dp ;
	skos:definition	"The extent to which public authorities allow citizens to receive communications digitally only and opt-out for paper mailings. Digital Post refers to the possibility that governments communicate electronically-only with citizens or entrepreneurs through e.g. personal mailboxes or other digital postal solutions." ;
	skos:topConceptOf	ns1:indicator .
ns7:e_gov_4_cb	rdf:type	skos:Concept ,
		ns10:Indicator ;
	skos:prefLabel	"4 Cross-border services" ;
	dct:source	ns35:egov_bench ;
	skos:notation	"e_gov_4_cb" ;
	skos:altLabel	"4 Cross-border services" ;
	ns11:membership	ns21:e_gov_4_cb ;
	skos:definition	"The extent to which information and services are available online, usable, and integrated with eIDs and eDocuments for users from other European countries." ;
	skos:topConceptOf	ns1:indicator .
ns7:e_gov_4a_cb_oa	rdf:type	skos:Concept ,
		ns10:Indicator ;
	skos:prefLabel	"4.1 Cross-border services - Cross-border online availability" ;
	dct:source	ns35:egov_bench ;
	skos:notation	"e_gov_4a_cb_oa" ;
	skos:altLabel	"4.1 Cross-border services - Cross-border online availability" ;
	ns11:membership	ns21:e_gov_4a_cb_oa ;
	skos:definition	"The extent to which informational and transactional services and information concerning these services is provided online for users from other European countries." ;
	skos:topConceptOf	ns1:indicator .
ns7:e_gov_4b_cb_us	rdf:type	skos:Concept ,
		ns10:Indicator ;
	skos:prefLabel	"4.2 Cross-border services - Cross-border user support" ;
	dct:source	ns35:egov_bench ;
	skos:notation	"e_gov_4b_cb_us" ;
	skos:altLabel	"4.2 Cross-border services - Cross-border user support" ;
	ns11:membership	ns21:e_gov_4b_cb_us ;
	skos:definition	"The extent to which online support, help features, and feedback mechanisms are available for users from other European countries." ;
	skos:topConceptOf	ns1:indicator .
ns7:e_gov_4c_cb_eid	rdf:type	skos:Concept ,
		ns10:Indicator ;
	skos:prefLabel	"4.3 Cross-border services - Cross-border eID" ;
	dct:source	ns35:egov_bench ;
	skos:notation	"e_gov_4c_cb_eid" ;
	skos:altLabel	"4.3 Cross-border services - Cross-border eID" ;
	ns11:membership	ns21:e_gov_4c_cb_eid ;
	skos:definition	"The extent to which electronic Identification (eID) can be used during service processes by users from other European countries, a government-issued document for online identification, and authentication." ;
	skos:topConceptOf	ns1:indicator .
ns7:e_gov_4d_cb_edoc	rdf:type	skos:Concept ,
		ns10:Indicator ;
	skos:prefLabel	"4.4 Cross-border services - Cross-border eDocuments" ;
	dct:source	ns35:egov_bench ;
	skos:notation	"e_gov_4d_cb_edoc" ;
	skos:altLabel	"4.4 Cross-border services - Cross-border eDocuments" ;
	ns11:membership	ns21:e_gov_4d_cb_edoc ;
	skos:definition	"The extent to which electronic documents (eDocuments) can be used during service processes by users from other European countries, documents that have been authenticated by its issuer using any means recognised under applicable national law, specifically through the use of electronic signatures, e.g. not a regular PDF or Word file." ;
	skos:topConceptOf	ns1:indicator .
ns7:mbb_5gcov	rdf:type	skos:Concept ,
		ns10:Indicator ;
	skos:prefLabel	"5G mobile broadband coverage (as a % of households)" ;
	dct:source	ns35:bc2020 ;
	skos:notation	"mbb_5gcov" ;
	skos:altLabel	"5G mobile broadband coverage" ;
	ns11:membership	ns29:mbb_5gcov ;
	skos:definition	"Coverage is a supply indicator defined as the percentage of Households living in areas covered by fifth generation mobile broadband. " ;
	skos:topConceptOf	ns1:indicator .
ns7:mbb_r5gcov	rdf:type	skos:Concept ,
		ns10:Indicator ;
	skos:prefLabel	"Rural 5G mobile broadband coverage (as a % of households)" ;
	dct:source	ns35:bc2020 ;
	skos:notation	"mbb_r5gcov" ;
	skos:altLabel	"Rural 5G mobile broadband coverage" ;
	ns11:membership	ns29:mbb_r5gcov ;
	skos:definition	"Coverage is a supply indicator defined as the percentage of Households living in areas covered by fifth generation mobile broadband. \nRural areas are defined as those with less than 100 people per km2." ;
	skos:topConceptOf	ns1:indicator .
ns7:desi_4g	rdf:type	ns10:Indicator ,
		skos:Concept ;
	skos:prefLabel	"4G coverage" ;
	dct:source	ns35:desi_4g ;
	skos:notation	"desi_4g" ;
	skos:altLabel	"4G coverage" .
@prefix ns36:	<http://semantic.digital-agenda-data.eu/codelist/indicator-group/desi_ind/> .
ns7:desi_4g	ns11:membership	ns36:desi_4g ;
	skos:definition	"Percentage of populated areas with coverage by 4G" ;
	skos:topConceptOf	ns1:indicator .
ns7:desi_5g	rdf:type	ns10:Indicator ,
		skos:Concept ;
	skos:prefLabel	"5G readiness" ;
	dct:source	ns35:desi_5g ;
	skos:notation	"desi_5g" ;
	skos:altLabel	"5G readiness" ;
	ns11:membership	ns36:desi_5g ;
	skos:definition	"The amount of spectrum assigned and ready for 5G use by the end of 2020 within the so-called 5G pioneer bands. These bands are 700 MHz (703-733 MHz and 758-788 MHz), 3.6 GHz (3400-3800 MHz) and 26 GHz (1000 MHz within 24250-27500 MHz). All three spectrum bands have an equal weight" ;
	skos:topConceptOf	ns1:indicator .
ns7:desi_5gc	rdf:type	ns10:Indicator ,
		skos:Concept ;
	skos:prefLabel	"5G coverage" ;
	dct:source	ns35:desi_5gc ;
	skos:notation	"desi_5gc" ;
	skos:altLabel	"5G coverage" ;
	ns11:membership	ns36:desi_5gc ;
	skos:definition	"Percentage of populated areas with coverage by 5G" ;
	skos:topConceptOf	ns1:indicator .
ns7:desi_bbpi	rdf:type	ns10:Indicator ,
		skos:Concept ;
	skos:prefLabel	"Broadband price index" ;
	dct:source	ns35:desi_bbpi ;
	skos:notation	"desi_bbpi" ;
	skos:altLabel	"Broadband price index" ;
	ns11:membership	ns36:desi_bbpi ;
	skos:definition	"The broadband price index measures the prices of representative baskets of fixed, mobile and converged broadband offers" ;
	skos:topConceptOf	ns1:indicator .
ns7:desi_c_bbpi	rdf:type	ns10:Indicator ,
		skos:Concept ;
	skos:prefLabel	"Broadband price index" ;
	dct:source	ns35: ;
	skos:notation	"desi_c_bbpi" ;
	skos:altLabel	"Broadband price index" .
@prefix ns37:	<http://semantic.digital-agenda-data.eu/codelist/indicator-group/desi_subdim/> .
ns7:desi_c_bbpi	ns11:membership	ns37:desi_c_bbpi ;
	skos:topConceptOf	ns1:indicator .
ns7:desi_c_fbbc	rdf:type	ns10:Indicator ,
		skos:Concept ;
	skos:prefLabel	"Fixed broadband coverage" ;
	dct:source	ns35: ;
	skos:notation	"desi_c_fbbc" ;
	skos:altLabel	"Fixed broadband coverage" ;
	ns11:membership	ns37:desi_c_fbbc ;
	skos:topConceptOf	ns1:indicator .
ns7:desi_c_fbbtc	rdf:type	ns10:Indicator ,
		skos:Concept ;
	skos:prefLabel	"Fixed broadband take-up" ;
	dct:source	ns35: ;
	skos:notation	"desi_c_fbbtc" ;
	skos:altLabel	"Fixed broadband take-up" ;
	ns11:membership	ns37:desi_c_fbbtc ;
	skos:topConceptOf	ns1:indicator .
ns7:desi_c_mbb	rdf:type	ns10:Indicator ,
		skos:Concept ;
	skos:prefLabel	"Mobile broadband" ;
	dct:source	ns35: ;
	skos:notation	"desi_c_mbb" ;
	skos:altLabel	"Mobile broadband" ;
	ns11:membership	ns37:desi_c_mbb ;
	skos:topConceptOf	ns1:indicator .
ns7:desi_conn	rdf:type	ns10:Indicator ,
		skos:Concept ;
	skos:prefLabel	"Connectivity" ;
	dct:source	ns35: ;
	skos:notation	"desi_conn" ;
	skos:altLabel	"Connectivity" .
@prefix ns38:	<http://semantic.digital-agenda-data.eu/codelist/indicator-group/desi_dim/> .
ns7:desi_conn	ns11:membership	ns38:desi_conn ;
	skos:topConceptOf	ns1:indicator .
ns7:desi_dps	rdf:type	ns10:Indicator ,
		skos:Concept ;
	skos:prefLabel	"Digital Public Services" ;
	dct:source	ns35: ;
	skos:notation	"desi_dps" ;
	skos:altLabel	"Digital Public Services" ;
	ns11:membership	ns38:desi_dps ;
	skos:topConceptOf	ns1:indicator .
ns7:desi_dps_egov	rdf:type	ns10:Indicator ,
		skos:Concept ;
	skos:prefLabel	"e-Government" ;
	dct:source	ns35: ;
	skos:notation	"desi_dps_egov" ;
	skos:altLabel	"e-Government" ;
	ns11:membership	ns37:desi_dps_egov ;
	skos:topConceptOf	ns1:indicator .
ns7:desi_dps_egovuser	rdf:type	ns10:Indicator ,
		skos:Concept ;
	skos:prefLabel	"e-Government Users" ;
	dct:source	ns35:desi_dps_egovuser ;
	skos:notation	"desi_dps_egovuser" ;
	skos:altLabel	"e-Government Users" ;
	ns11:membership	ns36:desi_dps_egovuser ;
	skos:definition	"Individuals who used the Internet, in the last 12 months, for interaction with public authorities" ;
	skos:topConceptOf	ns1:indicator .
ns7:desi_dps_opendata	rdf:type	ns10:Indicator ,
		skos:Concept ;
	skos:prefLabel	"Open Data" ;
	dct:source	ns35:desi_dps_opendata ;
	skos:notation	"desi_dps_opendata" ;
	skos:altLabel	"Open Data" ;
	ns11:membership	ns36:desi_dps_opendata ;
	skos:definition	"This composite indicator measures to what extent countries have an open data policy in place (including the transposition of the revised PSI Directive), the estimated political, social and economic impact of open data and the characteristics (functionalities, data availability and usage) of the national data portal." ;
	skos:topConceptOf	ns1:indicator .
ns7:desi_dps_psbiz	rdf:type	ns10:Indicator ,
		skos:Concept ;
	skos:prefLabel	"Digital public services for businesses" ;
	dct:source	ns35:desi_dps_psbiz ;
	skos:notation	"desi_dps_psbiz" ;
	skos:altLabel	"Digital public services for businesses" ;
	ns11:membership	ns36:desi_dps_psbiz ;
	skos:definition	"The indicator broadly reflects the share of public services needed for starting a business and conducting regular business operations that are available online for domestic as well as foreign users. Services provided through a portal receive a higher score, services which provide only information (but have to be completed offline) receive a more limited score." ;
	skos:topConceptOf	ns1:indicator .
ns7:desi_fbbc	rdf:type	ns10:Indicator ,
		skos:Concept ;
	skos:prefLabel	"Fast BB (NGA) coverage" ;
	dct:source	ns35:desi_fbbc ;
	skos:notation	"desi_fbbc" ;
	skos:altLabel	"Fast broadband (NGA) coverage" ;
	ns11:membership	ns36:desi_fbbc ;
	skos:definition	"Percentage of households covered by fixed broadband of at least 30 Mbps download. The technologies considered are FTTH, FTTB, Cable Docsis 3.0 and VDS" ;
	skos:topConceptOf	ns1:indicator .
ns7:desi_fbbtc	rdf:type	skos:Concept ,
		ns10:Indicator ;
	skos:prefLabel	"Overall fixed BB take-up" ;
	dct:source	ns35:desi_fbbtc ;
	skos:notation	"desi_fbbtc" ;
	skos:altLabel	"Overall fixed broadband take-up" ;
	ns11:membership	ns36:desi_fbbtc ;
	skos:definition	"Percentage of households subscribing to fixed broadband" ;
	skos:topConceptOf	ns1:indicator .
ns7:desi_gbpstc	rdf:type	skos:Concept ,
		ns10:Indicator ;
	skos:prefLabel	"At least 1 Gbps take-up" ;
	dct:source	ns35:desi_gbpstc ;
	skos:notation	"desi_gbpstc" ;
	skos:altLabel	"At least 1 Gbps take-up" ;
	ns11:membership	ns36:desi_gbpstc ;
	skos:definition	"Percentage of households subscribing to fixed broadband of at least 1 Gbps, calculated as overall fixed broadband take-up " ;
	skos:topConceptOf	ns1:indicator .
ns7:desi_hc	rdf:type	skos:Concept ,
		ns10:Indicator ;
	skos:prefLabel	"Human Capital" ;
	dct:source	ns35: ;
	skos:notation	"desi_hc" ;
	skos:altLabel	"Human Capital" ;
	ns11:membership	ns38:desi_hc ;
	skos:topConceptOf	ns1:indicator .
ns7:desi_hc_abds	rdf:type	skos:Concept ,
		ns10:Indicator ;
	skos:prefLabel	"Above basic digital skills" ;
	dct:source	ns35:desi_hc_abds ;
	skos:notation	"desi_hc_abds" ;
	skos:altLabel	"Above basic digital skills" ;
	ns11:membership	ns36:desi_hc_abds ;
	skos:definition	"Individuals with \u2018above basic\u2019 digital skills in each of the following four dimensions: information, communication, problem solving and software for content creation (as measured by the number of activities carried out during the previous 3 months). " ;
	skos:topConceptOf	ns1:indicator .
ns7:desi_hc_abss	rdf:type	skos:Concept ,
		ns10:Indicator ;
	skos:prefLabel	"At least basic software skills" ;
	dct:source	ns35:desi_hc_abss ;
	skos:notation	"desi_hc_abss" ;
	skos:altLabel	"At least basic software skills" ;
	ns11:membership	ns36:desi_hc_abss ;
	skos:definition	"Individuals who, in addition to having used basic software features such as word processing, have used advanced spreadsheet functions, created a presentation or document integrating text, pictures and tables or charts, or written code in a programming language. " ;
	skos:topConceptOf	ns1:indicator .
ns7:desi_hc_asd	rdf:type	skos:Concept ,
		ns10:Indicator ;
	skos:prefLabel	"Advanced Skills and Development" ;
	dct:source	ns35: ;
	skos:notation	"desi_hc_asd" ;
	skos:altLabel	"Advanced Skills and Development" ;
	ns11:membership	ns37:desi_hc_asd ;
	skos:topConceptOf	ns1:indicator .
ns7:desi_hc_bds	rdf:type	skos:Concept ,
		ns10:Indicator ;
	skos:prefLabel	"At least Basic Digital Skills" ;
	dct:source	ns35:desi_hc_bds ;
	skos:notation	"desi_hc_bds" ;
	skos:altLabel	"At least Basic Digital Skills" ;
	ns11:membership	ns36:desi_hc_bds ;
	skos:definition	"Individuals with \u2018basic\u2019 or \u2018above basic\u2019 digital skills in each of the following four dimensions: information, communication, problem solving and software for content creation (as measured by the number of activities carried out during the previous 3 months). " ;
	skos:topConceptOf	ns1:indicator .
ns7:desi_hc_bsu	rdf:type	skos:Concept ,
		ns10:Indicator ;
	skos:prefLabel	"Internet User Skills" ;
	dct:source	ns35: ;
	skos:notation	"desi_hc_bsu" ;
	skos:altLabel	"Internet User Skills" ;
	ns11:membership	ns37:desi_hc_bsu ;
	skos:topConceptOf	ns1:indicator .
ns7:desi_hc_entict	rdf:type	skos:Concept ,
		ns10:Indicator ;
	skos:prefLabel	"Enterprises providing ICT training " ;
	dct:source	ns35:desi_hc_entict ;
	skos:notation	"desi_hc_entict" ;
	skos:altLabel	"Enterprises providing ICT training " ;
	ns11:membership	ns36:desi_hc_entict ;
	skos:definition	"Enterprises who provided training in ICT to their personnel" ;
	skos:topConceptOf	ns1:indicator .
ns7:desi_hc_fictspec	rdf:type	skos:Concept ,
		ns10:Indicator ;
	skos:prefLabel	"Female ICT specialists" ;
	dct:source	ns35:desi_hc_fictspec ;
	skos:notation	"desi_hc_fictspec" ;
	skos:altLabel	"Female ICT specialists" ;
	ns11:membership	ns36:desi_hc_fictspec ;
	skos:definition	"Employed female ICT specialists. Broad definition based on the ISCO-08 classification and including jobs like ICT service managers, ICT professionals, ICT technicians, ICT installers and servicers." ;
	skos:topConceptOf	ns1:indicator .
ns7:desi_hc_ictg	rdf:type	skos:Concept ,
		ns10:Indicator ;
	skos:prefLabel	"ICT graduates" ;
	dct:source	ns35:desi_hc_ictg ;
	skos:notation	"desi_hc_ictg" ;
	skos:altLabel	"ICT graduates" ;
	ns11:membership	ns36:desi_hc_ictg ;
	skos:definition	"Individuals with a degree in ICT" ;
	skos:topConceptOf	ns1:indicator .
ns7:desi_hc_ictspec	rdf:type	skos:Concept ,
		ns10:Indicator ;
	skos:prefLabel	"ICT Specialists" ;
	dct:source	ns35:desi_hc_ictspec ;
	skos:notation	"desi_hc_ictspec" ;
	skos:altLabel	"ICT Specialists" ;
	ns11:membership	ns36:desi_hc_ictspec ;
	skos:definition	"Employed ICT specialists. Broad definition based on the ISCO-08 classification and including jobs like ICT service managers, ICT professionals, ICT technicians, ICT installers and servicers." ;
	skos:topConceptOf	ns1:indicator .
ns7:desi_idt	rdf:type	skos:Concept ,
		ns10:Indicator ;
	skos:prefLabel	"Integration of Digital Technology" ;
	dct:source	ns35: ;
	skos:notation	"desi_idt" ;
	skos:altLabel	"Integration of Digital Technology" ;
	ns11:membership	ns38:desi_idt ;
	skos:topConceptOf	ns1:indicator .
ns7:desi_idt_ai	rdf:type	skos:Concept ,
		ns10:Indicator ;
	skos:prefLabel	"Artificial intelligence" ;
	dct:source	ns35:desi_idt_ai ;
	skos:notation	"desi_idt_ai" ;
	skos:altLabel	"AI" ;
	ns11:membership	ns36:desi_idt_ai ;
	skos:definition	"Enterprises using at least 2 AI technologies" ;
	skos:topConceptOf	ns1:indicator .
ns7:desi_idt_bigdat	rdf:type	skos:Concept ,
		ns10:Indicator ;
	skos:prefLabel	"Big data" ;
	dct:source	ns35:desi_idt_bigdat ;
	skos:notation	"desi_idt_bigdat" ;
	skos:altLabel	"Big data" ;
	ns11:membership	ns36:desi_idt_bigdat ;
	skos:definition	"Enterprises analysing big data from any data source" ;
	skos:topConceptOf	ns1:indicator .
ns7:desi_idt_cloud	rdf:type	skos:Concept ,
		ns10:Indicator ;
	skos:prefLabel	"Cloud" ;
	dct:source	ns35:desi_idt_cloud ;
	skos:notation	"desi_idt_cloud" ;
	skos:altLabel	"Cloud" ;
	ns11:membership	ns36:desi_idt_cloud ;
	skos:definition	"Enterprises purchasing at least one of the following cloud computing services: hosting of the enterprise's database, accounting software applications, CRM software, computing power" ;
	skos:topConceptOf	ns1:indicator .
ns7:desi_idt_di	rdf:type	ns10:Indicator ,
		skos:Concept ;
	skos:prefLabel	"Digital intensity" ;
	dct:source	ns35: ;
	skos:notation	"desi_idt_di" ;
	skos:altLabel	"Digital intensity" ;
	ns11:membership	ns37:desi_idt_di ;
	skos:topConceptOf	ns1:indicator .
ns7:desi_idt_dtb	rdf:type	ns10:Indicator ,
		skos:Concept ;
	skos:prefLabel	"Digital technologies for businesses" ;
	dct:source	ns35: ;
	skos:notation	"desi_idt_dtb" ;
	skos:altLabel	"Digital technologies for businesses" ;
	ns11:membership	ns37:desi_idt_dtb ;
	skos:topConceptOf	ns1:indicator .
ns7:desi_idt_ecomm	rdf:type	ns10:Indicator ,
		skos:Concept ;
	skos:prefLabel	"e-Commerce" ;
	dct:source	ns35: ;
	skos:notation	"desi_idt_ecomm" ;
	skos:altLabel	"e-Commerce" ;
	ns11:membership	ns37:desi_idt_ecomm ;
	skos:topConceptOf	ns1:indicator .
ns7:desi_idt_ecomturn	rdf:type	ns10:Indicator ,
		skos:Concept ;
	skos:prefLabel	"e-Commerce turnover" ;
	dct:source	ns35:desi_idt_ecomturn ;
	skos:notation	"desi_idt_ecomturn" ;
	skos:altLabel	"e-Commerce turnover" ;
	ns11:membership	ns36:desi_idt_ecomturn ;
	skos:definition	"SMEs total turnover from e-commerce" ;
	skos:topConceptOf	ns1:indicator .
ns7:desi_idt_einv	rdf:type	ns10:Indicator ,
		skos:Concept ;
	skos:prefLabel	"e-Invoices" ;
	dct:source	ns35:desi_idt_einv ;
	skos:notation	"desi_idt_einv" ;
	skos:altLabel	"e-Invoices" ;
	ns11:membership	ns36:desi_idt_einv ;
	skos:definition	"Enterprises sending e-invoices, suitable for automated processing" ;
	skos:topConceptOf	ns1:indicator .
ns7:desi_idt_eis	rdf:type	ns10:Indicator ,
		skos:Concept ;
	skos:prefLabel	"Electronic Information Sharing" ;
	dct:source	ns35:desi_idt_eis ;
	skos:notation	"desi_idt_eis" ;
	skos:altLabel	"Electronic Information Sharing" ;
	ns11:membership	ns36:desi_idt_eis ;
	skos:definition	"Enterprises who have in use an ERP (enterprise resource planning) software package to share information between different functional areas (e.g. accounting, planning, production, marketing)" ;
	skos:topConceptOf	ns1:indicator .
ns7:desi_idt_ictsust	rdf:type	ns10:Indicator ,
		skos:Concept ;
	skos:prefLabel	"ICT for environmental sustainability" ;
	dct:source	ns35:desi_idt_ictsust ;
	skos:notation	"desi_idt_ictsust" ;
	skos:altLabel	"ICT for environmental sustainability" ;
	ns11:membership	ns36:desi_idt_ictsust ;
	skos:definition	"The indicator measures the level of support that adopted ICT technologies offered to enterprises to engage in more environmentally-friendly actions. The level of intensity is measured based on the number of environmental actions (maximum 10) reported by enterprises to have been facilitated by the use of ICT. The following categorisation was achieved: low intensity (0 to 4 actions), medium intensity (5 to 7 actions) and high intensity (8 to 10 actions)." ;
	skos:topConceptOf	ns1:indicator .
ns7:desi_idt_sellcb	rdf:type	ns10:Indicator ,
		skos:Concept ;
	skos:prefLabel	"Selling online cross-border" ;
	dct:source	ns35:desi_idt_sellcb ;
	skos:notation	"desi_idt_sellcb" ;
	skos:altLabel	"Selling online cross-border" ;
	ns11:membership	ns36:desi_idt_sellcb ;
	skos:definition	"SMEs that carried out electronic sales to other EU countries" ;
	skos:topConceptOf	ns1:indicator .
ns7:desi_idt_smeso	rdf:type	ns10:Indicator ,
		skos:Concept ;
	skos:prefLabel	"SMEs selling online" ;
	dct:source	ns35:desi_idt_smeso ;
	skos:notation	"desi_idt_smeso" ;
	skos:altLabel	"SMEs selling online" ;
	ns11:membership	ns36:desi_idt_smeso ;
	skos:definition	"SMEs selling online (at least 1% of turnover)" ;
	skos:topConceptOf	ns1:indicator .
ns7:desi_idt_socmed	rdf:type	ns10:Indicator ,
		skos:Concept ;
	skos:prefLabel	"Social media" ;
	dct:source	ns35:desi_idt_socmed ;
	skos:notation	"desi_idt_socmed" ;
	skos:altLabel	"Social media" ;
	ns11:membership	ns36:desi_idt_socmed ;
	skos:definition	"Enterprises using two or more of the following social media: social networks, enterprise's blog or microblog, multimedia content sharing websites, wiki-based knowledge sharing tools. Using social media means that the enterprise has a user profile, an account or a user license depending on the requirements and the type of the social media. " ;
	skos:topConceptOf	ns1:indicator .
ns7:desi_mbbtu	rdf:type	ns10:Indicator ,
		skos:Concept ;
	skos:prefLabel	"Mobile BB take-up" ;
	dct:source	ns35:desi_mbbtu ;
	skos:notation	"desi_mbbtu" ;
	skos:altLabel	"Mobile broadband take-up" ;
	ns11:membership	ns36:desi_mbbtu ;
	skos:definition	"Number of mobile data subscriptions per 100 people" ;
	skos:topConceptOf	ns1:indicator .
ns7:desi_total	rdf:type	ns10:Indicator ,
		skos:Concept ;
	skos:prefLabel	"Digital Economy and Society Index" ;
	dct:source	ns35: ;
	skos:notation	"desi_total" ;
	skos:altLabel	"DESI Total " .
@prefix ns39:	<http://semantic.digital-agenda-data.eu/codelist/indicator-group/desi_total/> .
ns7:desi_total	ns11:membership	ns39:desi_total ;
	skos:definition	"DESI overall index score per country" ;
	skos:topConceptOf	ns1:indicator .
ns7:desi_ufbbtu	rdf:type	ns10:Indicator ,
		skos:Concept ;
	skos:prefLabel	"At least 100 Mbps fixed BB take-up" ;
	dct:source	ns35:desi_ufbbtu ;
	skos:notation	"desi_ufbbtu" ;
	skos:altLabel	"At least 100 Mbps fixed broadband take-up" ;
	ns11:membership	ns36:desi_ufbbtu ;
	skos:definition	"Percentage of households subscribing to fixed broadband of at least 100 Mbps, calculated as overall fixed broadband take-up" ;
	skos:topConceptOf	ns1:indicator .
ns7:desi_vhcnc	rdf:type	ns10:Indicator ,
		skos:Concept ;
	skos:prefLabel	"Fixed Very High Capacity Network (VHCN) coverage" ;
	dct:source	ns35:desi_vhcnc ;
	skos:notation	"desi_vhcnc" ;
	skos:altLabel	"Fixed Very High Capacity Network (VHCN) coverage" ;
	ns11:membership	ns36:desi_vhcnc ;
	skos:definition	"Percentage of households covered by any fixed VHCN. The technologies considered are FTTH and FTTB for 2015-2018 and FTTH, FTTB and Cable Docsis 3.1 for 201" ;
	skos:topConceptOf	ns1:indicator .
ns7:desi_dps_prefform	rdf:type	ns10:Indicator ,
		skos:Concept ;
	skos:prefLabel	"Pre-filled Forms" ;
	dct:source	ns35:desi_dps_prefform ;
	skos:notation	"desi_dps_prefform" ;
	skos:altLabel	"Pre-filled Forms" ;
	ns11:membership	ns36:desi_dps_prefform ;
	skos:definition	"Amount of data that is pre-filled in public services' online forms" ;
	skos:topConceptOf	ns1:indicator .
ns7:desi_dps_pscit	rdf:type	ns10:Indicator ,
		skos:Concept ;
	skos:prefLabel	"Digital public services for citizens" ;
	dct:source	ns35:desi_dps_pscit ;
	skos:notation	"desi_dps_pscit" ;
	skos:altLabel	"Digital public services for citizens" ;
	ns11:membership	ns36:desi_dps_pscit ;
	skos:definition	"The share of administrative steps that can be done online for major life events (birth of a child, new residence, etc.) for citizens" ;
	skos:topConceptOf	ns1:indicator .
ns7:desi_idt_smedi	rdf:type	ns10:Indicator ,
		skos:Concept ;
	skos:prefLabel	"SMEs with at least a basic level of digital intensity" ;
	dct:source	ns35:desi_idt_smedi ;
	skos:notation	"desi_idt_smedi" ;
	skos:altLabel	"SMEs with at least a basic level of digital intensity" ;
	ns11:membership	ns36:desi_idt_smedi ;
	skos:definition	"The digital intensity score is based on counting how many out of 12 selected technologies are used by enterprises. A basic level requires usage of at least 4 technologies. " ;
	skos:topConceptOf	ns1:indicator .
ns7:e_gov_dpsc	rdf:type	skos:Concept ,
		ns10:Indicator ;
	skos:prefLabel	"Digital Public Services for Citizens" ;
	dct:source	ns35:e_gov_bench ;
	skos:notation	"e_gov_dpsc" ;
	skos:altLabel	"Digital Public Services for Citizens" ;
	ns11:membership	ns21:e_gov_dpsc ;
	skos:definition	"The extent to which a service or information concerning service for citizens is provided online, and via a portal. Services that are offered fully, partially or not at all online. " ;
	skos:note	"It is calculated as the average of the national and cross-border online availability for basic and extended services within the citizen-related Life Events from the last two\nyears (Family, Career, Studying, Moving, Owning and driving a car and Starting a small claims procedure)." ;
	skos:topConceptOf	ns1:indicator .
ns7:e_gov_od	rdf:type	skos:Concept ,
		ns10:Indicator ;
	skos:prefLabel	"Open Data" ;
	dct:source	ns35:european_data_portal ;
	skos:notation	"e_gov_od" ;
	skos:altLabel	"Open Data" ;
	ns11:membership	ns21:e_gov_od ;
	skos:definition	"A series of indicators have been selected to measure Open Data maturity across Europe. These indicators cover the level of development of national policies promoting Open Data, an assessment of the features made available on national data portals as well as the expected impact and quality of Open Data." ;
	skos:note	"This composite indicator comprises 4 dimensions:\ni)Open Data Policy that focuses on the presence of specific  olicies and strategies to foster open data at national level; \nii) Open Data Impact that looks at the activities performed to monitor and measure open re-use and the impact derived by such re-use; \niii) Open Data Portal that focuses on advanced portal  unctions that enable both versed and less versed users to access open data via the national portal and features that enhance the interaction between publishers and re-users (via forum and discussion boards); and \niv) Open Data Quality that focuses on the measures  dopted by portal managers to ensure the systematic harvesting of metadata from sources across the country, as well as the  urrency of the available metadata and where possible the actual data, the monitoring of the compliance with the DCAT-AP metadata standard as well as the quality of  eployment of the published data.\nBreak in series in 2020 due to methodological changes.\nThe data was recalculated to include EU27 Average.\nFor more information please consult: https://www.europeandataportal.eu/en/impact-studies/open-data-maturity" ;
	skos:topConceptOf	ns1:indicator .
ns7:i_dsk_x	rdf:type	skos:Concept ,
		ns10:Indicator ;
	skos:prefLabel	"Individuals with no digital skills" ;
	dct:source	ns35:estat_isoc_sk_dskl_i ;
	skos:notation	"i_dsk_x" ;
	skos:altLabel	"Individuals with \"no skills\"" ;
	ns11:membership	ns25:i_dsk_x ;
	skos:definition	"Persons that have been using internet during last 3 months are attributed a score on four digital competence domains: information, communication, content-creation and problem-solving, depending the activities they have been able to do. The scores in each domain are basic, above basic and below basic. Individuals not using internet are classified without digital skills. To be classified \"basic or above basic\" on the overall indicator an individual has to have basic or above basic skills in all the four Digital Competence domains included in the index: information, communication, content-creation and problem-solving." ;
	skos:note	"Detailed results are available in the Eurostat table <a href=\"http://appsso.eurostat.ec.europa.eu/nui/show.do?dataset=isoc_sk_dskl_i&lang=en\">ISOC_SK_DSKL_I</a>. Consult the <a href=\"https://ec.europa.eu/digital-agenda/en/news/new-comprehensive-digital-skills-indicator\"> methodological note</a> on DG CONNECT newsroom." ;
	skos:topConceptOf	ns1:indicator .
ns7:i_dsk_c_x	rdf:type	ns10:Indicator ,
		skos:Concept ;
	skos:prefLabel	"Individuals with no digital skills in Communication domain" ;
	dct:source	ns35:estat_isoc_sk_dskl_i ;
	skos:notation	"i_dsk_c_x" ;
	skos:altLabel	"Communication Domain - No Skills" ;
	ns11:membership	ns25:i_dsk_c_x ;
	skos:definition	"These skills refer to the ability to communicate in digital environments, share resources through online tools, link with others and collaborate through digital tools, interact with and participate in communities and networks, cross-cultural awareness. The indicator is based on four activities internet users have been able to do online during previous 3 months. The scores are basic, above basic and none. Individuals not using internet are classified without digital skills." ;
	skos:note	"Detailed results are available in the Eurostat table <a href=\"http://appsso.eurostat.ec.europa.eu/nui/show.do?dataset=isoc_sk_dskl_i&lang=en\">ISOC_SK_DSKL_I</a>. Consult the <a href=\"https://ec.europa.eu/digital-agenda/en/news/new-comprehensive-digital-skills-indicator\"> methodological note</a> on DG CONNECT newsroom." ;
	skos:topConceptOf	ns1:indicator .
ns7:i_dsk_l	rdf:type	skos:Concept ,
		ns10:Indicator ;
	skos:prefLabel	"Individuals with low level of digital skills (missing some type of basic skills)" ;
	dct:source	ns35:estat_isoc_sk_dskl_i ;
	skos:notation	"i_dsk_l" ;
	skos:altLabel	"Individuals with \"low\" level of skills " ;
	ns11:membership	ns25:i_dsk_l ;
	skos:definition	"Persons that have been using internet during last 3 months are attributed a score on four digital competence domains: information, communication, content-creation and problem-solving, depending the activities they have been able to do. The scores in each domain are basic, above basic and below basic. Individuals not using internet are classified without digital skills. To be classified \"basic or above basic\" on the overall indicator an individual has to have basic or above basic skills in all the four Digital Competence domains included in the index: information, communication, content-creation and problem-solving." ;
	skos:note	"Detailed results are available in the Eurostat table <a href=\"http://appsso.eurostat.ec.europa.eu/nui/show.do?dataset=isoc_sk_dskl_i&lang=en\">ISOC_SK_DSKL_I</a>. Consult the <a href=\"https://ec.europa.eu/digital-agenda/en/news/new-comprehensive-digital-skills-indicator\"> methodological note</a> on DG CONNECT newsroom." ;
	skos:topConceptOf	ns1:indicator .
ns7:i_dsk_s_ab	rdf:type	ns10:Indicator ,
		skos:Concept ;
	skos:prefLabel	"Individuals with above basic level of digital skills in Software domain" ;
	dct:source	ns35:estat_isoc_sk_dskl_i ;
	skos:notation	"i_dsk_s_ab" ;
	skos:altLabel	"Software Domain - Above Basic Skills" ;
	ns11:membership	ns25:i_dsk_s_ab ;
	skos:definition	"Software skills for content manipulation refer to the ability to create and edit new content (from word processing to images and video); integrate and re-elaborate previous knowledge and content; produce creative expressions, media outputs and programming; deal with and apply intellectual property rights and licences. The indicator is based on six activities internet users have been able to do during previous 3 months. The scores are basic, above basic and none. Individuals not using internet are classified without digital skills." ;
	skos:note	"Detailed results are available in the Eurostat table <a href=\"http://appsso.eurostat.ec.europa.eu/nui/show.do?dataset=isoc_sk_dskl_i&lang=en\">ISOC_SK_DSKL_I</a>. Consult the <a href=\"https://ec.europa.eu/digital-agenda/en/news/new-comprehensive-digital-skills-indicator\"> methodological note</a> on DG CONNECT newsroom." ;
	skos:topConceptOf	ns1:indicator .
ns7:i_dsk_ps_ab	rdf:type	ns10:Indicator ,
		skos:Concept ;
	skos:prefLabel	"Individuals with above basic level of digital skills in Problem solving domain" ;
	dct:source	ns35:estat_isoc_sk_dskl_i ;
	skos:notation	"i_dsk_ps_ab" ;
	skos:altLabel	"Problem Solving Domain - Above Basic Skills" ;
	ns11:membership	ns25:i_dsk_ps_ab ;
	skos:definition	"Problem solving skills refers to the ability to identify digital needs and resources, make informed decisions as to which are the most appropriate digital tools according to the purpose or need, solve conceptual problems through digital means, creatively use technologies, solve technical problems, update one's own and others' competences. The indicator is based on three basic digital problems and familiarity with four online services internet users have been able to do during previous 3 months. The scores are basic, above basic and none. Individuals not using internet are classified without digital skills." ;
	skos:note	"Detailed results are available in the Eurostat table <a href=\"http://appsso.eurostat.ec.europa.eu/nui/show.do?dataset=isoc_sk_dskl_i&lang=en\">ISOC_SK_DSKL_I</a>. Consult the <a href=\"https://ec.europa.eu/digital-agenda/en/news/new-comprehensive-digital-skills-indicator\"> methodological note</a> on DG CONNECT newsroom." ;
	skos:topConceptOf	ns1:indicator .
ns7:i_dsk_ab	rdf:type	skos:Concept ,
		ns10:Indicator ;
	skos:prefLabel	"Individuals with above basic level of digital skills" ;
	dct:source	ns35:estat_isoc_sk_dskl_i ;
	skos:notation	"i_dsk_ab" ;
	skos:altLabel	"Individuals with above basic level of skills" ;
	ns11:membership	ns25:i_dsk_ab ;
	skos:definition	"Persons that have been using internet during last 3 months are attributed a score on four digital competence domains: information, communication, content-creation and problem-solving, depending the activities they have been able to do. The scores in each domain are basic, above basic and below basic. Individuals not using internet are classified without digital skills. To be classified \"basic or above basic\" on the overall indicator an individual has to have basic or above basic skills in all the four Digital Competence domains included in the index: information, communication, content-creation and problem-solving." ;
	skos:note	"Detailed results are available in the Eurostat table <a href=\"http://appsso.eurostat.ec.europa.eu/nui/show.do?dataset=isoc_sk_dskl_i&lang=en\">ISOC_SK_DSKL_I</a>. Consult the <a href=\"https://ec.europa.eu/digital-agenda/en/news/new-comprehensive-digital-skills-indicator\"> methodological note</a> on DG CONNECT newsroom." ;
	skos:topConceptOf	ns1:indicator .
ns7:i_dsk_i_x	rdf:type	skos:Concept ,
		ns10:Indicator ;
	skos:prefLabel	"Individuals with no digital skills in Information domain" ;
	dct:source	ns35:estat_isoc_sk_dskl_i ;
	skos:notation	"i_dsk_i_x" ;
	skos:altLabel	"Information Domain - No Skills" ;
	ns11:membership	ns25:i_dsk_i_x ;
	skos:definition	"Information processing skills refers to the ability to identify, locate, retrieve, store, organise and analyse digital information, judging its relevance and purpose. The indicator is based on five activities internet users have been able to do online during previous 3 months. The scores are basic, above basic and none. Individuals not using internet are classified without digital skills." ;
	skos:note	"Detailed results are available in the Eurostat table <a href=\"http://appsso.eurostat.ec.europa.eu/nui/show.do?dataset=isoc_sk_dskl_i&lang=en\">ISOC_SK_DSKL_I</a>. Consult the <a href=\"https://ec.europa.eu/digital-agenda/en/news/new-comprehensive-digital-skills-indicator\"> methodological note</a> on DG CONNECT newsroom." ;
	skos:topConceptOf	ns1:indicator .
ns7:i_dsk_ps_x	rdf:type	skos:Concept ,
		ns10:Indicator ;
	skos:prefLabel	"Individuals with no digital skills in Problem solving domain" ;
	dct:source	ns35:estat_isoc_sk_dskl_i ;
	skos:notation	"i_dsk_ps_x" ;
	skos:altLabel	"Problem Solving Domain - No Skills" ;
	ns11:membership	ns25:i_dsk_ps_x ;
	skos:definition	"Problem solving skills refers to the ability to identify digital needs and resources, make informed decisions as to which are the most appropriate digital tools according to the purpose or need, solve conceptual problems through digital means, creatively use technologies, solve technical problems, update one's own and others' competences. The indicator is based on three basic digital problems and familiarity with four online services internet users have been able to do during previous 3 months. The scores are basic, above basic and none. Individuals not using internet are classified without digital skills." ;
	skos:note	"Detailed results are available in the Eurostat table <a href=\"http://appsso.eurostat.ec.europa.eu/nui/show.do?dataset=isoc_sk_dskl_i&lang=en\">ISOC_SK_DSKL_I</a>. Consult the <a href=\"https://ec.europa.eu/digital-agenda/en/news/new-comprehensive-digital-skills-indicator\"> methodological note</a> on DG CONNECT newsroom." ;
	skos:topConceptOf	ns1:indicator .
ns7:i_dsk_i_ab	rdf:type	ns10:Indicator ,
		skos:Concept ;
	skos:prefLabel	"Individuals with above basic level of digital skills in Information domain" ;
	dct:source	ns35:estat_isoc_sk_dskl_i ;
	skos:notation	"i_dsk_i_ab" ;
	skos:altLabel	"Information Domain - Above Basic Skills" ;
	ns11:membership	ns25:i_dsk_i_ab ;
	skos:definition	"Information processing skills refers to the ability to identify, locate, retrieve, store, organise and analyse digital information, judging its relevance and purpose. The indicator is based on five activities internet users have been able to do online during previous 3 months. The scores are basic, above basic and none. Individuals not using internet are classified without digital skills." ;
	skos:note	"Detailed results are available in the Eurostat table <a href=\"http://appsso.eurostat.ec.europa.eu/nui/show.do?dataset=isoc_sk_dskl_i&lang=en\">ISOC_SK_DSKL_I</a>. Consult the <a href=\"https://ec.europa.eu/digital-agenda/en/news/new-comprehensive-digital-skills-indicator\"> methodological note</a> on DG CONNECT newsroom." ;
	skos:topConceptOf	ns1:indicator .
ns25:i_dsk_ab	rdf:type	ns10:IndicatorToGroupMembership ;
	rdfs:label	"ict-skills" ;
	ns11:member-of	ns12:ict-skills ;
	ns11:order	"12" .
ns25:i_dsk_c_ab	rdf:type	ns10:IndicatorToGroupMembership ;
	rdfs:label	"ict-skills" ;
	ns11:member-of	ns12:ict-skills ;
	ns11:order	"21" .
ns25:i_dsk_c_x	rdf:type	ns10:IndicatorToGroupMembership ;
	rdfs:label	"ict-skills" ;
	ns11:member-of	ns12:ict-skills ;
	ns11:order	"23" .
ns25:i_dsk_i_ab	rdf:type	ns10:IndicatorToGroupMembership ;
	rdfs:label	"ict-skills" ;
	ns11:member-of	ns12:ict-skills ;
	ns11:order	"17" .
ns25:i_dsk_i_x	rdf:type	ns10:IndicatorToGroupMembership ;
	rdfs:label	"ict-skills" ;
	ns11:member-of	ns12:ict-skills ;
	ns11:order	"19" .
ns25:i_dsk_l	rdf:type	ns10:IndicatorToGroupMembership ;
	rdfs:label	"ict-skills" ;
	ns11:member-of	ns12:ict-skills ;
	ns11:order	"14" .
ns25:i_dsk_ps_ab	rdf:type	ns10:IndicatorToGroupMembership ;
	rdfs:label	"ict-skills" ;
	ns11:member-of	ns12:ict-skills ;
	ns11:order	"25" .
ns25:i_dsk_ps_x	rdf:type	ns10:IndicatorToGroupMembership ;
	rdfs:label	"ict-skills" ;
	ns11:member-of	ns12:ict-skills ;
	ns11:order	"27" .
ns25:i_dsk_s_ab	rdf:type	ns10:IndicatorToGroupMembership ;
	rdfs:label	"ict-skills" ;
	ns11:member-of	ns12:ict-skills ;
	ns11:order	"30" .
ns25:i_dsk_s_x	rdf:type	ns10:IndicatorToGroupMembership ;
	rdfs:label	"ict-skills" ;
	ns11:member-of	ns12:ict-skills ;
	ns11:order	"32" .
ns25:i_dsk_x	rdf:type	ns10:IndicatorToGroupMembership ;
	rdfs:label	"ict-skills" ;
	ns11:member-of	ns12:ict-skills ;
	ns11:order	"15" .
ns25:old_digskillindex	rdf:type	ns10:IndicatorToGroupMembership ;
	rdfs:label	"ict-skills" ;
	ns11:member-of	ns12:ict-skills ;
	ns11:order	"93" .
ns25:old_digskillindex_basicandabove	rdf:type	ns10:IndicatorToGroupMembership ;
	rdfs:label	"ict-skills" ;
	ns11:member-of	ns12:ict-skills ;
	ns11:order	"92" .
ns25:old_i_dsk_b	rdf:type	ns10:IndicatorToGroupMembership ;
	rdfs:label	"ict-skills" ;
	ns11:member-of	ns12:ict-skills ;
	ns11:order	"11" .
ns25:old_i_dsk_c_b	rdf:type	ns10:IndicatorToGroupMembership ;
	rdfs:label	"ict-skills" ;
	ns11:member-of	ns12:ict-skills ;
	ns11:order	"20" .
ns25:old_i_dsk_i_b	rdf:type	ns10:IndicatorToGroupMembership ;
	rdfs:label	"ict-skills" ;
	ns11:member-of	ns12:ict-skills ;
	ns11:order	"16" .
ns25:old_i_dsk_ps_b	rdf:type	ns10:IndicatorToGroupMembership ;
	rdfs:label	"ict-skills" ;
	ns11:member-of	ns12:ict-skills ;
	ns11:order	"24" .
ns25:old_i_dsk_s_b	rdf:type	ns10:IndicatorToGroupMembership ;
	rdfs:label	"ict-skills" ;
	ns11:member-of	ns12:ict-skills ;
	ns11:order	"28" .
ns26:i_cisk_sfjobx	rdf:type	ns10:IndicatorToGroupMembership ;
	rdfs:label	"ict-specialist" ;
	ns11:member-of	ns12:ict-specialist ;
	ns11:order	"6" .
ns26:i_cprg	rdf:type	ns10:IndicatorToGroupMembership ;
	rdfs:label	"ict-specialist" ;
	ns11:member-of	ns12:ict-specialist ;
	ns11:order	"9" .
ns26:i_skedu	rdf:type	ns10:IndicatorToGroupMembership ;
	rdfs:label	"ict-specialist" ;
	ns11:member-of	ns12:ict-specialist ;
	ns11:order	"7" .
ns26:p_iuse	rdf:type	ns10:IndicatorToGroupMembership ;
	rdfs:label	"ict-specialist" ;
	ns11:member-of	ns12:ict-specialist ;
	ns11:order	"8" .
ns7:old_digskillindex	rdf:type	skos:Concept ,
		ns10:Indicator ;
	skos:prefLabel	"Digital skills indicator (internet users) - pilot 2012/2014" ;
	dct:source	ns35:estat_isoc_sk_dskl_i ;
	skos:notation	"old_digskillindex" ;
	skos:altLabel	"Digital skills indicator (internet users) - pilot 2012/2014" ;
	ns11:membership	ns25:old_digskillindex ;
	skos:definition	"Persons that have been using internet during last 3 months are attributed a score on four digital competence domains: information, communication, content-creation and problem-solving, depending the activities they have been able to do. The scores are basic, above basic and below basic. Individuals not using internet are classified without digital skills. The four digital competence domains are aggregated in four logical groups." ;
	skos:note	"This indicator has been piloted on the 2012 and 2014 micro-data from the Eurostat community survey on ICT usage by Households/Individuals using some proxy variables. It is not fully comparable with the regular implementation starting with the 2015 survey." ;
	skos:topConceptOf	ns1:indicator .
ns7:old_digskillindex_basicandabove	rdf:type	skos:Concept ,
		ns10:Indicator ;
	skos:prefLabel	"Individuals with basic or above basic digital skills - pilot 2012/2014" ;
	dct:source	ns35:estat_isoc_sk_dskl_i ;
	skos:notation	"old_digskillindex_basicandabove" ;
	skos:altLabel	"Individuals with basic or above basic digital skills - pilot 2012/2014" ;
	ns11:membership	ns25:old_digskillindex_basicandabove ;
	skos:definition	"Persons that have been using internet during last 3 months are attributed a score on four digital competence domains: information, communication, content-creation and problem-solving, depending the activities they have been able to do. The scores in each domain are basic, above basic and below basic. Individuals not using internet are classified without digital skills. To be classified \"basic or above basic\" on the overall indicator an individual has to have basic or above basic skills in all the four Digital Competence domains included in the index: information, communication, content-creation and problem-solving." ;
	skos:note	"This indicator has been piloted on the 2012 and 2014 micro-data from the Eurostat community survey on ICT usage by Households/Individuals using some proxy variables. It is not fully comparable with the regular implementation starting with the 2015 survey." ;
	skos:topConceptOf	ns1:indicator .
ns7:old_i_dsk_b	rdf:type	skos:Concept ,
		ns10:Indicator ;
	skos:prefLabel	"Individuals with a basic level of digital skills" ;
	dct:source	ns35:estat_isoc_sk_dskl_i ;
	skos:notation	"old_i_dsk_b" ;
	skos:altLabel	"Individuals with a basic level of skills" ;
	ns11:membership	ns25:old_i_dsk_b ;
	skos:definition	"Persons that have been using internet during last 3 months are attributed a score on four digital competence domains: information, communication, content-creation and problem-solving, depending the activities they have been able to do. The scores in each domain are basic, above basic and below basic. Individuals not using internet are classified without digital skills. To be classified \"basic or above basic\" on the overall indicator an individual has to have basic or above basic skills in all the four Digital Competence domains included in the index: information, communication, content-creation and problem-solving." ;
	skos:note	"Detailed results are available in the Eurostat table <a href=\"http://appsso.eurostat.ec.europa.eu/nui/show.do?dataset=isoc_sk_dskl_i&lang=en\">ISOC_SK_DSKL_I</a>. Consult the <a href=\"https://ec.europa.eu/digital-agenda/en/news/new-comprehensive-digital-skills-indicator\"> methodological note</a> on DG CONNECT newsroom." ;
	skos:topConceptOf	ns1:indicator .
ns7:old_i_dsk_c_b	rdf:type	skos:Concept ,
		ns10:Indicator ;
	skos:prefLabel	"Individuals with a basic level of digital skills in Communication domain" ;
	dct:source	ns35:estat_isoc_sk_dskl_i ;
	skos:notation	"old_i_dsk_c_b" ;
	skos:altLabel	"Communication Domain - Basic Skills" ;
	ns11:membership	ns25:old_i_dsk_c_b ;
	skos:definition	"These skills refer to the ability to communicate in digital environments, share resources through online tools, link with others and collaborate through digital tools, interact with and participate in communities and networks, cross-cultural awareness. The indicator is based on four activities internet users have been able to do online during previous 3 months. The scores are basic, above basic and none. Individuals not using internet are classified without digital skills." ;
	skos:note	"Detailed results are available in the Eurostat table <a href=\"http://appsso.eurostat.ec.europa.eu/nui/show.do?dataset=isoc_sk_dskl_i&lang=en\">ISOC_SK_DSKL_I</a>. Consult the <a href=\"https://ec.europa.eu/digital-agenda/en/news/new-comprehensive-digital-skills-indicator\"> methodological note</a> on DG CONNECT newsroom." ;
	skos:topConceptOf	ns1:indicator .
ns7:old_i_dsk_i_b	rdf:type	ns10:Indicator ,
		skos:Concept ;
	skos:prefLabel	"Individuals with a basic level of digital skills in Information domain" ;
	dct:source	ns35:estat_isoc_sk_dskl_i ;
	skos:notation	"old_i_dsk_i_b" ;
	skos:altLabel	"Information Domain - Basic Skills" ;
	ns11:membership	ns25:old_i_dsk_i_b ;
	skos:definition	"Information processing skills refers to the ability to identify, locate, retrieve, store, organise and analyse digital information, judging its relevance and purpose. The indicator is based on five activities internet users have been able to do online during previous 3 months. The scores are basic, above basic and none. Individuals not using internet are classified without digital skills." ;
	skos:note	"Detailed results are available in the Eurostat table <a href=\"http://appsso.eurostat.ec.europa.eu/nui/show.do?dataset=isoc_sk_dskl_i&lang=en\">ISOC_SK_DSKL_I</a>. Consult the <a href=\"https://ec.europa.eu/digital-agenda/en/news/new-comprehensive-digital-skills-indicator\"> methodological note</a> on DG CONNECT newsroom." ;
	skos:topConceptOf	ns1:indicator .
ns7:old_i_dsk_ps_b	rdf:type	ns10:Indicator ,
		skos:Concept ;
	skos:prefLabel	"Individuals with a basic level of digital skills in Problem solving domain" ;
	dct:source	ns35:estat_isoc_sk_dskl_i ;
	skos:notation	"old_i_dsk_ps_b" ;
	skos:altLabel	"Problem Solving Domain - Basic Skills" ;
	ns11:membership	ns25:old_i_dsk_ps_b ;
	skos:definition	"Problem solving skills refers to the ability to identify digital needs and resources, make informed decisions as to which are the most appropriate digital tools according to the purpose or need, solve conceptual problems through digital means, creatively use technologies, solve technical problems, update one's own and others' competences. The indicator is based on three basic digital problems and familiarity with four online services internet users have been able to do during previous 3 months. The scores are basic, above basic and none. Individuals not using internet are classified without digital skills." ;
	skos:note	"Detailed results are available in the Eurostat table <a href=\"http://appsso.eurostat.ec.europa.eu/nui/show.do?dataset=isoc_sk_dskl_i&lang=en\">ISOC_SK_DSKL_I</a>. Consult the <a href=\"https://ec.europa.eu/digital-agenda/en/news/new-comprehensive-digital-skills-indicator\"> methodological note</a> on DG CONNECT newsroom." ;
	skos:topConceptOf	ns1:indicator .
ns7:old_i_dsk_s_b	rdf:type	ns10:Indicator ,
		skos:Concept ;
	skos:prefLabel	"Individuals with a basic level of digital skills in Software domain" ;
	dct:source	ns35:estat_isoc_sk_dskl_i ;
	skos:notation	"old_i_dsk_s_b" ;
	skos:altLabel	"Software Domain - Basic Skills" ;
	ns11:membership	ns25:old_i_dsk_s_b ;
	skos:definition	"Software skills for content manipulation refer to the ability to create and edit new content (from word processing to images and video); integrate and re-elaborate previous knowledge and content; produce creative expressions, media outputs and programming; deal with and apply intellectual property rights and licences. The indicator is based on six activities internet users have been able to do during previous 3 months. The scores are basic, above basic and none. Individuals not using internet are classified without digital skills." ;
	skos:note	"Detailed results are available in the Eurostat table <a href=\"http://appsso.eurostat.ec.europa.eu/nui/show.do?dataset=isoc_sk_dskl_i&lang=en\">ISOC_SK_DSKL_I</a>. Consult the <a href=\"https://ec.europa.eu/digital-agenda/en/news/new-comprehensive-digital-skills-indicator\"> methodological note</a> on DG CONNECT newsroom." ;
	skos:topConceptOf	ns1:indicator .
ns15:h_fbbfix	rdf:type	ns10:IndicatorToGroupMembership ;
	rdfs:label	"broadband" ;
	ns11:member-of	ns12:broadband ;
	ns11:order	"11" .
ns15:h_ubbfix	rdf:type	ns10:IndicatorToGroupMembership ;
	rdfs:label	"broadband" ;
	ns11:member-of	ns12:broadband ;
	ns11:order	"12" .
ns7:h_fbbfix	rdf:type	ns10:Indicator ,
		skos:Concept ;
	skos:prefLabel	"Households with fast fixed broadband connection" ;
	dct:source	ns35:estathh_cocom ;
	skos:notation	"h_fbbfix" ;
	skos:altLabel	"Households with fast fixed broadband connection" ;
	ns11:membership	ns15:h_fbbfix ;
	skos:definition	"Households with fast fixed broadband connection" ;
	skos:topConceptOf	ns1:indicator .
ns7:h_ubbfix	rdf:type	ns10:Indicator ,
		skos:Concept ;
	skos:prefLabel	"Households with ultrafast fixed broadband connection" ;
	dct:source	ns35:estathh_cocom ;
	skos:notation	"h_ubbfix" ;
	skos:altLabel	"Households with ultrafast fixed broadband connection" ;
	ns11:membership	ns15:h_ubbfix ;
	skos:definition	"Households with ultrafast fixed broadband connection" ;
	skos:topConceptOf	ns1:indicator .
ns21:e_gov_ebus	rdf:type	ns10:IndicatorToGroupMembership ;
	rdfs:label	"egovernment" ;
	ns11:member-of	ns12:egovernment ;
	ns11:order	"4" .
ns7:e_gov_ebus	rdf:type	ns10:Indicator ,
		skos:Concept ;
	skos:prefLabel	"Digital Public Services for Businesses" ;
	dct:source	ns35:egov_bench ;
	skos:notation	"e_gov_ebus" ;
	skos:altLabel	"Digital Public Services for Businesses" ;
	ns11:membership	ns21:e_gov_ebus ;
	skos:definition	"The extent to which a service or information concerning service for businesses is provided online and via a portal. Services that are offered fully, partially or not at all online. " ;
	skos:note	"It is calculated as the average of the national and cross-border online availability for basic and extended services within the business-related Life Events from the last two\nyears (Business Start-up and Regular Business\nOperations). Until 2019 (included), the indicator was measuring Basic services for National and Cross-Border. Meaning that as of 2020, the extended services were also added.\nThe data was recalculated to include EU27 Average. " ;
	skos:topConceptOf	ns1:indicator .
ns7:i_dsk_s_x	rdf:type	ns10:Indicator ,
		skos:Concept ;
	skos:prefLabel	"Individuals with no digital skills in Software domain" ;
	dct:source	ns35:estat_isoc_sk_dskl_i ;
	skos:notation	"i_dsk_s_x" ;
	skos:altLabel	"Software Domain - No Skills" ;
	ns11:membership	ns25:i_dsk_s_x ;
	skos:definition	"Software skills for content manipulation refer to the ability to create and edit new content (from word processing to images and video); integrate and re-elaborate previous knowledge and content; produce creative expressions, media outputs and programming; deal with and apply intellectual property rights and licences. The indicator is based on six activities internet users have been able to do during previous 3 months. The scores are basic, above basic and none. Individuals not using internet are classified without digital skills." ;
	skos:note	"Detailed results are available in the Eurostat table <a href=\"http://appsso.eurostat.ec.europa.eu/nui/show.do?dataset=isoc_sk_dskl_i&lang=en\">ISOC_SK_DSKL_I</a>. Consult the <a href=\"https://ec.europa.eu/digital-agenda/en/news/new-comprehensive-digital-skills-indicator\"> methodological note</a> on DG CONNECT newsroom." ;
	skos:topConceptOf	ns1:indicator .
ns7:i_dsk_c_ab	rdf:type	ns10:Indicator ,
		skos:Concept ;
	skos:prefLabel	"Individuals with above basic level of digital skills in Communication domain" ;
	dct:source	ns35:estat_isoc_sk_dskl_i ;
	skos:notation	"i_dsk_c_ab" ;
	skos:altLabel	"Communication Domain - Above Basic Skills" ;
	ns11:membership	ns25:i_dsk_c_ab ;
	skos:definition	"These skills refer to the ability to communicate in digital environments, share resources through online tools, link with others and collaborate through digital tools, interact with and participate in communities and networks, cross-cultural awareness. The indicator is based on four activities internet users have been able to do online during previous 3 months. The scores are basic, above basic and none. Individuals not using internet are classified without digital skills." ;
	skos:note	"Detailed results are available in the Eurostat table <a href=\"http://appsso.eurostat.ec.europa.eu/nui/show.do?dataset=isoc_sk_dskl_i&lang=en\">ISOC_SK_DSKL_I</a>. Consult the <a href=\"https://ec.europa.eu/digital-agenda/en/news/new-comprehensive-digital-skills-indicator\"> methodological note</a> on DG CONNECT newsroom." ;
	skos:topConceptOf	ns1:indicator .
ns38:desi_conn	rdf:type	ns10:IndicatorToGroupMembership ;
	rdfs:label	"desi_dim" ;
	ns11:member-of	ns12:desi_dim ;
	ns11:order	"2" .
ns38:desi_dps	rdf:type	ns10:IndicatorToGroupMembership ;
	rdfs:label	"desi_dim" ;
	ns11:member-of	ns12:desi_dim ;
	ns11:order	"4" .
ns38:desi_hc	rdf:type	ns10:IndicatorToGroupMembership ;
	rdfs:label	"desi_dim" ;
	ns11:member-of	ns12:desi_dim ;
	ns11:order	"1" .
ns38:desi_idt	rdf:type	ns10:IndicatorToGroupMembership ;
	rdfs:label	"desi_dim" ;
	ns11:member-of	ns12:desi_dim ;
	ns11:order	"3" .
ns36:desi_4g	rdf:type	ns10:IndicatorToGroupMembership ;
	rdfs:label	"desi_ind" ;
	ns11:member-of	ns12:desi_ind ;
	ns11:order	"231" .
ns36:desi_5g	rdf:type	ns10:IndicatorToGroupMembership ;
	rdfs:label	"desi_ind" ;
	ns11:member-of	ns12:desi_ind ;
	ns11:order	"232" .
ns36:desi_5gc	rdf:type	ns10:IndicatorToGroupMembership ;
	rdfs:label	"desi_ind" ;
	ns11:member-of	ns12:desi_ind ;
	ns11:order	"233" .
ns36:desi_bbpi	rdf:type	ns10:IndicatorToGroupMembership ;
	rdfs:label	"desi_ind" ;
	ns11:member-of	ns12:desi_ind ;
	ns11:order	"241" .
ns36:desi_dps_egovuser	rdf:type	ns10:IndicatorToGroupMembership ;
	rdfs:label	"desi_ind" ;
	ns11:member-of	ns12:desi_ind ;
	ns11:order	"411" .
ns36:desi_dps_opendata	rdf:type	ns10:IndicatorToGroupMembership ;
	rdfs:label	"desi_ind" ;
	ns11:member-of	ns12:desi_ind ;
	ns11:order	"415" .
ns36:desi_dps_prefform	rdf:type	ns10:IndicatorToGroupMembership ;
	rdfs:label	"desi_ind" ;
	ns11:member-of	ns12:desi_ind ;
	ns11:order	"412" .
ns36:desi_dps_psbiz	rdf:type	ns10:IndicatorToGroupMembership ;
	rdfs:label	"desi_ind" ;
	ns11:member-of	ns12:desi_ind ;
	ns11:order	"414" .
ns36:desi_dps_pscit	rdf:type	ns10:IndicatorToGroupMembership ;
	rdfs:label	"desi_ind" ;
	ns11:member-of	ns12:desi_ind ;
	ns11:order	"413" .
ns36:desi_fbbc	rdf:type	ns10:IndicatorToGroupMembership ;
	rdfs:label	"desi_ind" ;
	ns11:member-of	ns12:desi_ind ;
	ns11:order	"221" .
ns36:desi_fbbtc	rdf:type	ns10:IndicatorToGroupMembership ;
	rdfs:label	"desi_ind" ;
	ns11:member-of	ns12:desi_ind ;
	ns11:order	"211" .
ns36:desi_gbpstc	rdf:type	ns10:IndicatorToGroupMembership ;
	rdfs:label	"desi_ind" ;
	ns11:member-of	ns12:desi_ind ;
	ns11:order	"213" .
ns36:desi_hc_abds	rdf:type	ns10:IndicatorToGroupMembership ;
	rdfs:label	"desi_ind" ;
	ns11:member-of	ns12:desi_ind ;
	ns11:order	"112" .
ns36:desi_hc_abss	rdf:type	ns10:IndicatorToGroupMembership ;
	rdfs:label	"desi_ind" ;
	ns11:member-of	ns12:desi_ind ;
	ns11:order	"113" .
ns36:desi_hc_bds	rdf:type	ns10:IndicatorToGroupMembership ;
	rdfs:label	"desi_ind" ;
	ns11:member-of	ns12:desi_ind ;
	ns11:order	"111" .
ns36:desi_hc_entict	rdf:type	ns10:IndicatorToGroupMembership ;
	rdfs:label	"desi_ind" ;
	ns11:member-of	ns12:desi_ind ;
	ns11:order	"123" .
ns36:desi_hc_fictspec	rdf:type	ns10:IndicatorToGroupMembership ;
	rdfs:label	"desi_ind" ;
	ns11:member-of	ns12:desi_ind ;
	ns11:order	"122" .
ns36:desi_hc_ictg	rdf:type	ns10:IndicatorToGroupMembership ;
	rdfs:label	"desi_ind" ;
	ns11:member-of	ns12:desi_ind ;
	ns11:order	"124" .
ns36:desi_hc_ictspec	rdf:type	ns10:IndicatorToGroupMembership ;
	rdfs:label	"desi_ind" ;
	ns11:member-of	ns12:desi_ind ;
	ns11:order	"121" .
ns36:desi_idt_ai	rdf:type	ns10:IndicatorToGroupMembership ;
	rdfs:label	"desi_ind" ;
	ns11:member-of	ns12:desi_ind ;
	ns11:order	"325" .
ns36:desi_idt_bigdat	rdf:type	ns10:IndicatorToGroupMembership ;
	rdfs:label	"desi_ind" ;
	ns11:member-of	ns12:desi_ind ;
	ns11:order	"323" .
ns36:desi_idt_cloud	rdf:type	ns10:IndicatorToGroupMembership ;
	rdfs:label	"desi_ind" ;
	ns11:member-of	ns12:desi_ind ;
	ns11:order	"324" .
ns36:desi_idt_ecomturn	rdf:type	ns10:IndicatorToGroupMembership ;
	rdfs:label	"desi_ind" ;
	ns11:member-of	ns12:desi_ind ;
	ns11:order	"332" .
ns36:desi_idt_einv	rdf:type	ns10:IndicatorToGroupMembership ;
	rdfs:label	"desi_ind" ;
	ns11:member-of	ns12:desi_ind ;
	ns11:order	"327" .
ns36:desi_idt_eis	rdf:type	ns10:IndicatorToGroupMembership ;
	rdfs:label	"desi_ind" ;
	ns11:member-of	ns12:desi_ind ;
	ns11:order	"321" .
ns36:desi_idt_ictsust	rdf:type	ns10:IndicatorToGroupMembership ;
	rdfs:label	"desi_ind" ;
	ns11:member-of	ns12:desi_ind ;
	ns11:order	"326" .
ns36:desi_idt_sellcb	rdf:type	ns10:IndicatorToGroupMembership ;
	rdfs:label	"desi_ind" ;
	ns11:member-of	ns12:desi_ind ;
	ns11:order	"333" .
ns36:desi_idt_smedi	rdf:type	ns10:IndicatorToGroupMembership ;
	rdfs:label	"desi_ind" ;
	ns11:member-of	ns12:desi_ind ;
	ns11:order	"311" .
ns36:desi_idt_smeso	rdf:type	ns10:IndicatorToGroupMembership ;
	rdfs:label	"desi_ind" ;
	ns11:member-of	ns12:desi_ind ;
	ns11:order	"331" .
ns36:desi_idt_socmed	rdf:type	ns10:IndicatorToGroupMembership ;
	rdfs:label	"desi_ind" ;
	ns11:member-of	ns12:desi_ind ;
	ns11:order	"322" .
ns36:desi_mbbtu	rdf:type	ns10:IndicatorToGroupMembership ;
	rdfs:label	"desi_ind" ;
	ns11:member-of	ns12:desi_ind ;
	ns11:order	"234" .
ns36:desi_ufbbtu	rdf:type	ns10:IndicatorToGroupMembership ;
	rdfs:label	"desi_ind" ;
	ns11:member-of	ns12:desi_ind ;
	ns11:order	"212" .
ns36:desi_vhcnc	rdf:type	ns10:IndicatorToGroupMembership ;
	rdfs:label	"desi_ind" ;
	ns11:member-of	ns12:desi_ind ;
	ns11:order	"222" .
ns37:desi_c_bbpi	rdf:type	ns10:IndicatorToGroupMembership ;
	rdfs:label	"desi_subdim" ;
	ns11:member-of	ns12:desi_subdim ;
	ns11:order	"24" .
ns37:desi_c_fbbc	rdf:type	ns10:IndicatorToGroupMembership ;
	rdfs:label	"desi_subdim" ;
	ns11:member-of	ns12:desi_subdim ;
	ns11:order	"22" .
ns37:desi_c_fbbtc	rdf:type	ns10:IndicatorToGroupMembership ;
	rdfs:label	"desi_subdim" ;
	ns11:member-of	ns12:desi_subdim ;
	ns11:order	"21" .
ns37:desi_c_mbb	rdf:type	ns10:IndicatorToGroupMembership ;
	rdfs:label	"desi_subdim" ;
	ns11:member-of	ns12:desi_subdim ;
	ns11:order	"23" .
ns37:desi_dps_egov	rdf:type	ns10:IndicatorToGroupMembership ;
	rdfs:label	"desi_subdim" ;
	ns11:member-of	ns12:desi_subdim ;
	ns11:order	"41" .
ns37:desi_hc_asd	rdf:type	ns10:IndicatorToGroupMembership ;
	rdfs:label	"desi_subdim" ;
	ns11:member-of	ns12:desi_subdim ;
	ns11:order	"12" .
ns37:desi_hc_bsu	rdf:type	ns10:IndicatorToGroupMembership ;
	rdfs:label	"desi_subdim" ;
	ns11:member-of	ns12:desi_subdim ;
	ns11:order	"11" .
ns37:desi_idt_di	rdf:type	ns10:IndicatorToGroupMembership ;
	rdfs:label	"desi_subdim" ;
	ns11:member-of	ns12:desi_subdim ;
	ns11:order	"31" .
ns37:desi_idt_dtb	rdf:type	ns10:IndicatorToGroupMembership ;
	rdfs:label	"desi_subdim" ;
	ns11:member-of	ns12:desi_subdim ;
	ns11:order	"32" .
ns37:desi_idt_ecomm	rdf:type	ns10:IndicatorToGroupMembership ;
	rdfs:label	"desi_subdim" ;
	ns11:member-of	ns12:desi_subdim ;
	ns11:order	"33" .
ns39:desi_total	rdf:type	ns10:IndicatorToGroupMembership ;
	rdfs:label	"desi_total" ;
	ns11:member-of	ns12:desi_total ;
	ns11:order	"1" .