@prefix rdf:	<http://www.w3.org/1999/02/22-rdf-syntax-ns#> .
@prefix ns1:	<http://semantic.digital-agenda-data.eu/codelist/source/> .
@prefix ns2:	<http://semantic.digital-agenda-data.eu/def/class/> .
@prefix skos:	<http://www.w3.org/2004/02/skos/core#> .
@prefix foaf:	<http://xmlns.com/foaf/0.1/> .
@prefix ns5:	<https://ec.europa.eu/eurostat/web/products-datasets/-/> .
@prefix ns6:	<http://semantic.digital-agenda-data.eu/codelist/> .
@prefix xsd:	<http://www.w3.org/2001/XMLSchema#> .
@prefix dct:	<http://purl.org/dc/terms/> .
@prefix rdfs:	<http://www.w3.org/2000/01/rdf-schema#> .
@prefix ns10:	<http://semantic.digital-agenda-data.eu/def/> .
@prefix ns11:	<https://ec.europa.eu/digital-agenda/en/news/> .
@prefix ns12:	<http://ec.europa.eu/information_society/eeurope/i2010/benchmarking/index_en.htm#> .
@prefix ns13:	<http://ec.europa.eu/digital-agenda/> .
@prefix ns14:	<http://www.cept.org/eco/deliverables/> .
@prefix ns15:	<https://ec.europa.eu/digital-single-market/en/news/> .
@prefix ns16:	<http://www.obs.coe.int/eservices/> .
@prefix ns17:	<http://www.epsiplatform.eu/content/> .
@prefix ns18:	<http://ec.europa.eu/eurostat/web/digital-economy-and-society/data/> .
@prefix ns19:	<http://ec.europa.eu/eurostat/web/lfs/data/> .
@prefix ns20:	<http://ec.europa.eu/eurostat/web/international-trade/data/> .
@prefix ns21:	<http://ec.europa.eu/eurostat/web/products-datasets/-/> .
@prefix ns22:	<http://ec.europa.eu/eurostat/web/science-technology-innovation/data/> .
@prefix ns23:	<http://ec.europa.eu/eurostat/web/national-accounts/data/> .
@prefix ns24:	<http://ec.europa.eu/eurostat/web/population-demography-migration-projections/population-data/> .
@prefix ns25:	<http://ec.europa.eu/digital-agenda/en/news/> .
@prefix ns26:	<http://epp.eurostat.ec.europa.eu/portal/page/portal/employment_unemployment_lfs/methodology/> .
@prefix ns27:	<http://ec.europa.eu/digital-agenda/en/digital-agenda-you/> .
@prefix ns28:	<https://ec.europa.eu/digital-single-market/en/> .
@prefix ns29:	<https://www.europeandataportal.eu/en/impact-studies/> .

ns1:estat_educ_uoe_grad03
	rdf:type	ns2:Source , skos:Concept ;
	skos:prefLabel	"Eurostat, Table educ_uoe_grad03: Distribution of graduates at education level and programme orientation by sex and field of education" ;
	foaf:page	ns5:educ_uoe_grad03 ;
	skos:notation	"estat_educ_uoe_grad03" ;
	skos:definition	"Eurostat (table educ_uoe_grad03, using selection ISCED11=ED5-8) and and ISCEDF_13 [F06] Information and Communication Technologies" ;
	skos:topConceptOf	ns6:source .
ns6:source
	rdf:type	skos:ConceptScheme ;
	dct:modified	"2022-04-06T17:18:05"^^xsd:dateTime ;
	rdfs:isDefinedBy	<http://digital-agenda-data.eu/> ;
	skos:prefLabel	"Sources used by Digital Agenda Scoreboard indicators" ;
	skos:notation	"CL_SOURCE" ;
	skos:hasTopConcept	ns1:estat_educ_uoe_grad03 , ns1:abac , ns1:bench_gp , ns1:berec_roam , ns1:biac , ns1:capgemini , ns1:cnect-estat , ns1:cocom , ns1:corda , ns1:eco_report_03_efis_comm , ns1:egov_bench12 , ns1:egov_bench12_17 , ns1:einfraegi , ns1:einfrageant , ns1:einfraprace , ns1:eoa_smart12-26 , ns1:eoa_yearbook2014 , ns1:epsi , ns1:epsiplatform , ns1:estat-ent , ns1:estat-hh , ns1:estat-lfs , ns1:estat-lfs-sks , ns1:estat-trade , ns1:estat_gba_nabsfin07 , ns1:estat_isoc_bde15b_e , ns1:estat_isoc_bde15b_h , ns1:estat_isoc_bde15b_p , ns1:estat_isoc_bde15cbc , ns1:estat_isoc_bde15cua , ns1:estat_isoc_bde15dec , ns1:estat_isoc_bde15dip , ns1:estat_isoc_bde15disc , ns1:estat_isoc_bde15dth , ns1:estat_isoc_bde15ee , ns1:estat_isoc_ci_ac_i , ns1:estat_isoc_ci_eu_en2 , ns1:estat_isoc_ci_eu_i , ns1:estat_isoc_ci_ifp_fu , ns1:estat_isoc_ci_ifp_iu , ns1:estat_isoc_ci_im_i , ns1:estat_isoc_cicce_use , ns1:estat_isoc_cisci_ax , ns1:estat_isoc_cisci_pb , ns1:estat_isoc_cisci_prv , ns1:estat_isoc_cismt , ns1:estat_isoc_ec_eseln2 , ns1:estat_isoc_ec_ibuy , ns1:estat_isoc_ec_iprb , ns1:estat_isoc_pibi_ictbn2 , ns1:estat_isoc_r_gov_i , ns1:estat_isoc_r_iuse_i , ns1:estat_isoc_sk_cskl_i , ns1:estat_isoc_sk_dskl_i , ns1:estat_isoc_sk_how_i , ns1:estat_isoc_sk_iskl_i , ns1:estat_isoc_ske_ittn2 , ns1:estat_isoc_sks_itspt , ns1:estat_lfst_hhnhwhtc , ns1:estat_nama_gdp_c , ns1:estat_randd , ns1:estat_tps00188 , ns1:eun12 , ns1:euripidis-estat , ns1:eurostat_ed , ns1:eurostat_nat_acc , ns1:eurostat_pop , ns1:idate , ns1:ihs_tech , ns1:ipv6obs , ns1:jrc-ictspec3 , ns1:jrc_ict_randd , ns1:mis , ns1:nif_database , ns1:point_topic , ns1:samknows , ns1:smart11_39 , ns1:cocom_new , ns1:european_data_portal , ns1:estat_isoc_eb_ai , ns1:estat_isoc_sk_dskl_i21 , ns1:bc2020 , ns1:estat_isoc_e_dii , ns1:estat_isoc_eb_bd , ns1:estathh_cocom , ns1:e_gov_bench , ns1:desi_4g , ns1:desi_5g , ns1:desi_5gc , ns1:desi_bbpi , ns1:desi_dps_egovuser , ns1:desi_dps_opendata , ns1:desi_dps_prefform , ns1:desi_dps_psbiz , ns1:desi_dps_pscit , ns1:desi_fbbc , ns1:desi_fbbtc , ns1:desi_gbpstc , ns1:desi_hc_abds , ns1:desi_hc_abss , ns1:desi_hc_bds , ns1:desi_hc_entict , ns1:desi_hc_fictspec , ns1:desi_hc_ictg , ns1:desi_hc_ictspec , ns1:desi_idt_ai , ns1:desi_idt_bigdat , ns1:desi_idt_cloud , ns1:desi_idt_ecomturn , ns1:desi_idt_einv , ns1:desi_idt_eis , ns1:desi_idt_ictsust , ns1:desi_idt_sellcb , ns1:desi_idt_smedi , ns1:desi_idt_smeso , ns1:desi_idt_socmed , ns1:desi_mbbtu , ns1:desi_ufbbtu , ns1:desi_vhcnc ;
	skos:inScheme	ns10:scheme .
ns1:abac
	rdf:type	ns2:Source , skos:Concept ;
	skos:prefLabel	"ABAC" ;
	foaf:page	<http://europa.eu/rapid/press-release_MEMO-05-94_en.htm?locale=en> ;
	skos:notation	"abac" ;
	skos:definition	"ABAC is a transversal, transactional information system allowing for the execution and monitoring of all budgetary and accounting operations by the Commission, an Agency or Institution." ;
	skos:topConceptOf	ns6:source .
ns1:bench_gp
	rdf:type	ns2:Source , skos:Concept ;
	skos:prefLabel	"Benchmarking deployment of eHealth among General Practitioners" ;
	foaf:page	ns11:benchmarking-deployment-ehealth-among-general-practitioners-2013-smart-20110033 ;
	skos:notation	"bench_gp" ;
	skos:definition	"Studies committed by DG Connect to monitor the adoption of eHealth technologies by General Practitioners: 2007, 2013" ;
	skos:topConceptOf	ns6:source .
ns1:berec_roam
	rdf:type	ns2:Source , skos:Concept ;
	skos:prefLabel	"International Roaming BEREC Benchmark Data Report" ;
	foaf:page	<http://berec.europa.eu/eng/document_register/subject_matter/berec/reports/1159-international-roaming-berec-benchmark-data-report-january-2012-8211-june-2012> ;
	skos:notation	"berec_roam" ;
	skos:definition	"International Roaming Benchmark Data Report by BEREC - The Body of European Regulators for Electronic Communications" ;
	skos:note	"Document date: 28.01.2013 (Document number: BoR (13) 05)." ;
	skos:topConceptOf	ns6:source .
ns1:biac
	rdf:type	ns2:Source , skos:Concept ;
	skos:prefLabel	"Broadband Internet Access Cost (BIAC) annual studies" ;
	foaf:page	ns11:study-retail-broadband-access-prices-2013-smart-20100038 ;
	skos:notation	"biac" ;
	skos:definition	"Broadband Internet Access Cost (BIAC), annual studies for the EC realised by Van Dijk, covering EU 28 Member States as well as Canada, Iceland, Japan, South Korea, Liechtenstein, FYROM, Norway, State of California, State of Colorado, State of New York, Switzerland and Turkey." ;
	skos:note	"update until feb 2012 data collection" ;
	skos:topConceptOf	ns6:source .
ns1:capgemini
	rdf:type	ns2:Source , skos:Concept ;
	skos:prefLabel	"eGovernment Benchmarking Reports 2001-2010" ;
	foaf:page	ns12:e-Government_Benchmarking_Reports ;
	skos:notation	"capgemini" ;
	skos:definition	"eGovernment Benchmarking Report, Study for the EC realised by Capgemini (2001-2010 data)" ;
	skos:note	"Extraction 20 May 2011" ;
	skos:topConceptOf	ns6:source .
ns1:cnect-estat
	rdf:type	ns2:Source , skos:Concept ;
	skos:prefLabel	"Pilot of new Digital Skills Indicators" ;
	foaf:page	<http://ec.europa.eu/information_society/newsroom/cf/dae/document.cfm?action=display&doc_id=5406> ;
	skos:notation	"cnect-estat" ;
	skos:definition	"Pilot work carried out by DG CONNECT/F4 in relation to action 62 of the Digital Agenda to propose \"EU-wide indicators of digital competence\". These indicators have been piloted on the 2012 microdata from the Eurostat community survey on ICT usage by Households/Individuals. It is proposed for regular implementation starting with the 2015 survey." ;
	skos:topConceptOf	ns6:source .
ns1:cocom
	rdf:type	ns2:Source , skos:Concept ;
	skos:prefLabel	"Communications Committee survey" ;
	foaf:page	ns13:about-fast-and-ultra-fast-internet-access ;
	skos:notation	"cocom" ;
	skos:definition	"Electronic communications market indicators collected by Commission services, through National Regulatory Authorities, for the Communications Committee (COCOM) - January and July reports." ;
	skos:note	"extraction 22 May 2013" ;
	skos:topConceptOf	ns6:source .
ns1:corda
	rdf:type	ns2:Source , skos:Concept ;
	skos:prefLabel	"CORDA " ;
	foaf:page	<http://webcorda.rtd.cec.eu.int/index.cfm?page=index> ;
	skos:notation	"corda" ;
	skos:definition	"Common Research Data Warehouse" ;
	skos:topConceptOf	ns6:source .
ns1:eco_report_03_efis_comm
	rdf:type	ns2:Source , skos:Concept ;
	skos:prefLabel	"ECO Report 03" ;
	foaf:page	ns14:eco-reports ;
	skos:notation	"eco_report_03_efis_comm" ;
	skos:definition	"ECO Report 03, based on EFIS database, completed with direct communications between EU and Member States" ;
	skos:topConceptOf	ns6:source .
ns1:egov_bench12
	rdf:type	ns2:Source , skos:Concept ;
	skos:prefLabel	"eGovernment Benchmarking reports 2012-2014" ;
	foaf:page	<https://ec.europa.eu/digital-agenda/news-redirect/16475> ;
	skos:notation	"egov_bench12" ;
	skos:definition	"eGovernment Benchmarking Report, Studies for the EC peformed by Capgemini (2012-2014)" ;
	skos:topConceptOf	ns6:source .
ns1:egov_bench12_17
	rdf:type	ns2:Source , skos:Concept ;
	skos:prefLabel	"eGovernment Benchmarking Report, Studies for the EC performed by Capgemini (2012-2017)\u00A0" ;
	foaf:page	ns15:new-study-egovernment-services-europe-improving-cross-border-availability-services ;
	skos:notation	"egov_bench12_17" ;
	skos:definition	"eGovernment Benchmarking Report, Studies for the EC performed by Capgemini (2012-2017)\u00A0" ;
	skos:topConceptOf	ns6:source .
ns1:einfraegi
	rdf:type	ns2:Source , skos:Concept ;
	skos:prefLabel	"e-infrastructure project EGI" ;
	foaf:page	<http://www.egi.eu> ;
	skos:notation	"einfraegi" ;
	skos:definition	"e-infrastructure project EGI" ;
	skos:topConceptOf	ns6:source .
ns1:einfrageant
	rdf:type	ns2:Source , skos:Concept ;
	skos:prefLabel	"e-infrastructure project G\u00E9ant" ;
	foaf:page	<http://www.geant.net> ;
	skos:notation	"einfrageant" ;
	skos:definition	"e-infrastructure project G\u00E9ant" ;
	skos:topConceptOf	ns6:source .
ns1:einfraprace
	rdf:type	ns2:Source , skos:Concept ;
	skos:prefLabel	"e-infrastructure project PRACE" ;
	foaf:page	<http://www.prace-ri.eu> ;
	skos:notation	"einfraprace" ;
	skos:definition	"e-infrastructure project PRACE" ;
	skos:topConceptOf	ns6:source .
ns1:eoa_smart12-26
	rdf:type	ns2:Source , skos:Concept ;
	skos:prefLabel	"European Audiovisual Observatory - study \"On demand audiovisual markets in the EU\"" ;
	foaf:page	ns11:demand-audiovisual-markets-european-union-smart-20120028 ;
	skos:notation	"eoa_smart12-26" ;
	skos:definition	"European Audiovisual Observatory - study \"On demand audiovisual markets in the EU\", of April 2014 (smart 2012-0026)" ;
	skos:note	"page 20 table 4" ;
	skos:topConceptOf	ns6:source .
ns1:eoa_yearbook2014
	rdf:type	ns2:Source , skos:Concept ;
	skos:prefLabel	"European Audiovisual Observatory Yearbook 2014" ;
	foaf:page	ns16:premiumservice ;
	skos:notation	"eoa_yearbook2014" ;
	skos:definition	"European Audiovisual Observatory Yearbook 2014" ;
	skos:topConceptOf	ns6:source .
ns1:epsi
	rdf:type	ns2:Source , skos:Concept ;
	skos:prefLabel	"The PSI Scoreboard" ;
	foaf:page	ns17:european-psi-scoreboard ;
	skos:notation	"epsi" ;
	skos:definition	"The PSI Scoreboard is a \u2018crowdsourced\u2019 tool to measure the status of Open Data and PSI re-use throughout the EU." ;
	skos:topConceptOf	ns6:source .
ns1:epsiplatform
	rdf:type	ns2:Source , skos:Concept ;
	skos:prefLabel	"The PSI Scoreboard" ;
	foaf:page	ns17:european-psi-scoreboard ;
	skos:notation	"epsiplatform" ;
	skos:definition	"The PSI Scoreboard is a \u2018crowdsourced\u2019 tool to measure the status of Open Data and PSI re-use throughout the EU. It does NOT monitor government policies, but aims to assess the overall PSI re-use situation, which includes the open data community's activities." ;
	skos:topConceptOf	ns6:source .
ns1:estat-ent
	rdf:type	ns2:Source , skos:Concept ;
	skos:prefLabel	"Eurostat - European Union survey on ICT usage and eCommerce in Enterprises" ;
	foaf:page	ns18:comprehensive-database ;
	skos:notation	"estat-ent" ;
	skos:definition	"Eurostat - Community survey on ICT usage and eCommerce in Enterprises <a href=\"http://ec.europa.eu/eurostat/web/digital-economy-and-society/data/comprehensive-database\">More information</a>." ;
	skos:note	"Extraction from ENT2 comprehensive database (NACE Rev 2 in ACCESS 133 MB) version 16 Apr 2013, and from ENT (NACE Rev 1.1 in ACCESS 104 MB) version 12 Dec 2011." ;
	skos:topConceptOf	ns6:source .
ns1:estat-hh
	rdf:type	ns2:Source , skos:Concept ;
	skos:prefLabel	"Eurostat - European Union survey on ICT usage in Households and by Individuals" ;
	foaf:page	ns18:comprehensive-database ;
	skos:notation	"estat-hh" ;
	skos:definition	"Eurostat - Community survey on ICT usage in Households and by Individuals <a href=\"http://ec.europa.eu/eurostat/web/digital-economy-and-society/data/comprehensive-database\">More information</a>." ;
	skos:note	"Extraction from HH/Indiv comprehensive database (ACCESS) version\u00A029 April 2013" ;
	skos:topConceptOf	ns6:source .
ns1:estat-lfs
	rdf:type	ns2:Source , skos:Concept ;
	skos:prefLabel	"Eurostat - Labour Force Survey" ;
	foaf:page	ns19:database ;
	skos:notation	"estat-lfs" ;
	skos:definition	"Eurostat - Labour Force Survey" ;
	skos:note	"Extraction May 2013, ESTAT-G6" ;
	skos:topConceptOf	ns6:source .
ns1:estat-lfs-sks
	rdf:type	ns2:Source , skos:Concept ;
	skos:prefLabel	"Eurostat - ICT specialist statistics (derived from Labour Force Survey)" ;
	foaf:page	<http://ec.europa.eu/eurostat/cache/metadata/en/isoc_skslf_esms.htm> ;
	skos:notation	"estat-lfs-sks" ;
	skos:definition	"Eurostat - ICT specialist statistics (derived from Labour Force Survey)" ;
	skos:topConceptOf	ns6:source .
ns1:estat-trade
	rdf:type	ns2:Source , skos:Concept ;
	skos:prefLabel	"Eurostat - Trade statistics" ;
	foaf:page	ns20:database ;
	skos:notation	"estat-trade" ;
	skos:definition	"Eurostat - Trade statistics" ;
	skos:note	"Extraction May 2013, ESTAT-G6" ;
	skos:topConceptOf	ns6:source .
ns1:estat_gba_nabsfin07
	rdf:type	ns2:Source , skos:Concept ;
	skos:prefLabel	"Eurostat, Table gba_nabsfin07: Total GBAORD by NABS 2007 socio-economic objectives" ;
	foaf:page	ns21:gba_nabsfin07 ;
	skos:notation	"estat_gba_nabsfin07" ;
	skos:definition	"Eurostat, Table gba_nabsfin07: Total GBAORD by NABS 2007 socio-economic objectives" ;
	skos:note	"Double check? Predict?" ;
	skos:topConceptOf	ns6:source .
ns1:estat_isoc_bde15b_e
	rdf:type	ns2:Source , skos:Concept ;
	skos:prefLabel	"Eurostat, Table isoc_bde15b_e: Broadband and connectivity - enterprises" ;
	foaf:page	ns21:isoc_bde15b_e ;
	skos:notation	"estat_isoc_bde15b_e" ;
	skos:definition	"Eurostat, Table isoc_bde15b_e: Broadband and connectivity - enterprises" ;
	skos:topConceptOf	ns6:source .
ns1:estat_isoc_bde15b_h
	rdf:type	ns2:Source , skos:Concept ;
	skos:prefLabel	"Eurostat, Table isoc_bde15b_h: Broadband and connectivity - households" ;
	foaf:page	ns21:isoc_bde15b_h ;
	skos:notation	"estat_isoc_bde15b_h" ;
	skos:definition	"Eurostat, Table isoc_bde15b_h: Broadband and connectivity - households" ;
	skos:topConceptOf	ns6:source .
ns1:estat_isoc_bde15b_p
	rdf:type	ns2:Source , skos:Concept ;
	skos:prefLabel	"Eurostat, Table isoc_bde15b_p: Broadband and connectivity - persons employed" ;
	foaf:page	ns21:isoc_bde15b_p ;
	skos:notation	"estat_isoc_bde15b_p" ;
	skos:definition	"Eurostat, Table isoc_bde15b_p: Broadband and connectivity - persons employed" ;
	skos:topConceptOf	ns6:source .
ns1:estat_isoc_bde15cbc
	rdf:type	ns2:Source , skos:Concept ;
	skos:prefLabel	"Eurostat, Table isoc_bde15cbc: E-banking and e-commerce" ;
	foaf:page	ns21:isoc_bde15cbc ;
	skos:notation	"estat_isoc_bde15cbc" ;
	skos:definition	"Eurostat, Table isoc_bde15cbc: E-banking and e-commerce" ;
	skos:topConceptOf	ns6:source .
ns1:estat_isoc_bde15cua
	rdf:type	ns2:Source , skos:Concept ;
	skos:prefLabel	"Eurostat, Table isoc_bde15cua: Internet use and activities" ;
	foaf:page	ns21:isoc_bde15cua ;
	skos:notation	"estat_isoc_bde15cua" ;
	skos:definition	"Eurostat, Table isoc_bde15cua: Internet use and activities" ;
	skos:topConceptOf	ns6:source .
ns1:estat_isoc_bde15dec
	rdf:type	ns2:Source , skos:Concept ;
	skos:prefLabel	"Eurostat, Table estat_isoc_bde15dec: E-commerce, customer relation management (CRM) and secure transactions" ;
	foaf:page	ns21:isoc_bde15dec ;
	skos:notation	"estat_isoc_bde15dec" ;
	skos:definition	"Eurostat, Table estat_isoc_bde15dec: E-commerce, customer relation management (CRM) and secure transactions" ;
	skos:topConceptOf	ns6:source .
ns1:estat_isoc_bde15dip
	rdf:type	ns2:Source , skos:Concept ;
	skos:prefLabel	"Eurostat, Table isoc_bde15dip: Integration of internal processes" ;
	foaf:page	ns21:isoc_bde15dip ;
	skos:notation	"estat_isoc_bde15dip" ;
	skos:definition	"Eurostat, Table isoc_bde15dip: Integration of internal processes" ;
	skos:topConceptOf	ns6:source .
ns1:estat_isoc_bde15disc
	rdf:type	ns2:Source , skos:Concept ;
	skos:prefLabel	"Eurostat, Table isoc_bde15disc: Integration with customers/suppliers and SCM" ;
	foaf:page	ns21:isoc_bde15disc ;
	skos:notation	"estat_isoc_bde15disc" ;
	skos:definition	"Eurostat, Table isoc_bde15disc: Integration with customers/suppliers and SCM" ;
	skos:topConceptOf	ns6:source .
ns1:estat_isoc_bde15dth
	rdf:type	ns2:Source , skos:Concept ;
	skos:prefLabel	"Eurostat, Table isoc_bde15dth: Key technologies for the internet of things" ;
	foaf:page	ns21:isoc_bde15dth ;
	skos:notation	"estat_isoc_bde15dth" ;
	skos:definition	"Eurostat, Table isoc_bde15dth: Key technologies for the internet of things" ;
	skos:topConceptOf	ns6:source .
ns1:estat_isoc_bde15ee
	rdf:type	ns2:Source , skos:Concept ;
	skos:prefLabel	"Eurostat, Table isoc_bde15ee: Enterprises using the internet for interacting with public authorities" ;
	foaf:page	ns21:isoc_bde15ee ;
	skos:notation	"estat_isoc_bde15ee" ;
	skos:definition	"Eurostat, Table isoc_bde15ee: Enterprises using the internet for interacting with public authorities" ;
	skos:topConceptOf	ns6:source .
ns1:estat_isoc_ci_ac_i
	rdf:type	ns2:Source , skos:Concept ;
	skos:prefLabel	"Eurostat, Table isoc_ci_ac_i: Individuals - internet activities" , "Eurostat, Table isoc_ci_ac_i: Internet activities - individuals" ;
	foaf:page	ns21:isoc_ci_ac_i ;
	skos:notation	"estat_isoc_ci_ac_i" ;
	skos:definition	"Eurostat, Table isoc_pibi_ioa: Individuals doing specific online activities in the previous 3 months" , "Eurostat - Community survey on ICT usage in Households and by Individuals, Table: Internet activities - individuals" ;
	skos:topConceptOf	ns6:source .
ns1:estat_isoc_ci_eu_en2
	rdf:type	ns2:Source , skos:Concept ;
	skos:prefLabel	"Eurostat, Table isoc_ci_eu_en2: Computers and the internet: enterprises - summary of EU aggregates (NACE Rev. 2 activity) " , "Eurostat, Table isoc_ci_eu_en2: Computers and the internet: enterprises - summary of EU aggregates (NACE Rev. 2 activity)" ;
	foaf:page	ns21:isoc_ci_eu_en2 ;
	skos:notation	"estat_isoc_ci_eu_en2" ;
	skos:definition	"Eurostat, Table isoc_ci_eu_en2: Computers and the internet: enterprises - summary of EU aggregates (NACE Rev. 2 activity) " , "Eurostat, Table isoc_ci_eu_en2: Computers and the internet: enterprises - summary of EU aggregates (NACE Rev. 2 activity)" ;
	skos:topConceptOf	ns6:source .
ns1:estat_isoc_ci_eu_i
	rdf:type	ns2:Source , skos:Concept ;
	skos:prefLabel	"Eurostat, Table isoc_ci_eu_i: Computers and the internet: individuals - summary of EU aggregates" ;
	foaf:page	ns21:isoc_ci_eu_i ;
	skos:notation	"estat_isoc_ci_eu_i" ;
	skos:definition	"Eurostat, Table isoc_ci_eu_i: Computers and the internet: individuals - summary of EU aggregates" ;
	skos:topConceptOf	ns6:source .
ns1:estat_isoc_ci_ifp_fu
	rdf:type	ns2:Source , skos:Concept ;
	skos:prefLabel	"Eurostat, Table isoc_ci_ifp_fu: Frequency of internet use  - individuals" ;
	foaf:page	ns21:isoc_ci_ifp_fu ;
	skos:notation	"estat_isoc_ci_ifp_fu" ;
	skos:definition	"Eurostat, Table isoc_ci_ifp_fu: Frequency of internet use  - individuals" ;
	skos:topConceptOf	ns6:source .
ns1:estat_isoc_ci_ifp_iu
	rdf:type	ns2:Source , skos:Concept ;
	skos:prefLabel	"Eurostat, Table isoc_ci_ifp_iu: Internet use  - individuals" ;
	foaf:page	ns21:isoc_ci_ifp_iu ;
	skos:notation	"estat_isoc_ci_ifp_iu" ;
	skos:definition	"Eurostat, Table isoc_ci_ifp_iu: Internet use  - individuals" ;
	skos:topConceptOf	ns6:source .
ns1:estat_isoc_ci_im_i
	rdf:type	ns2:Source , skos:Concept ;
	skos:prefLabel	"Eurostat, Table isoc_ci_im_i: Mobile internet access  - individuals" ;
	foaf:page	ns21:isoc_ci_im_i ;
	skos:notation	"estat_isoc_ci_im_i" ;
	skos:definition	"Eurostat, Table isoc_ci_im_i: Mobile internet access  - individuals" ;
	skos:topConceptOf	ns6:source .
ns1:estat_isoc_cicce_use
	rdf:type	ns2:Source , skos:Concept ;
	skos:prefLabel	"Eurostat, Table isoc_cicce_use: Cloud computing services" ;
	foaf:page	ns21:isoc_cicce_use ;
	skos:notation	"estat_isoc_cicce_use" ;
	skos:definition	"Eurostat, Table isoc_cicce_use: Cloud computing services" ;
	skos:topConceptOf	ns6:source .
ns1:estat_isoc_cisci_ax
	rdf:type	ns2:Source , skos:Concept ;
	skos:prefLabel	"Eurostat, Table isoc_cisci_ax: Activities via internet not done because of security concerns" ;
	foaf:page	ns21:isoc_cisci_ax ;
	skos:notation	"estat_isoc_cisci_ax" ;
	skos:definition	"Eurostat, Table isoc_cisci_ax: Activities via internet not done because of security concerns" ;
	skos:topConceptOf	ns6:source .
ns1:estat_isoc_cisci_pb
	rdf:type	ns2:Source , skos:Concept ;
	skos:prefLabel	"Eurostat, Table isoc_cisci_pb: Security related problems experienced through using the internet for private purposes" ;
	foaf:page	ns21:isoc_cisci_pb ;
	skos:notation	"estat_isoc_cisci_pb" ;
	skos:definition	"Eurostat, Table isoc_cisci_pb: Security related problems experienced through using the internet for private purposes" ;
	skos:topConceptOf	ns6:source .
ns1:estat_isoc_cisci_prv
	rdf:type	ns2:Source , skos:Concept ;
	skos:prefLabel	"Eurostat, Table isoc_cisci_prv: Privacy and protection of personal information" ;
	foaf:page	ns21:isoc_cisci_prv ;
	skos:notation	"estat_isoc_cisci_prv" ;
	skos:definition	"Eurostat, Table isoc_cisci_prv: Privacy and protection of personal information" ;
	skos:topConceptOf	ns6:source .
ns1:estat_isoc_cismt
	rdf:type	ns2:Source , skos:Concept ;
	skos:prefLabel	"Eurostat, Table isoc_cismt: Social media use by type" ;
	foaf:page	ns21:isoc_cismt ;
	skos:notation	"estat_isoc_cismt" ;
	skos:definition	"Eurostat, Table isoc_cismt: Social media use by type" ;
	skos:topConceptOf	ns6:source .
ns1:estat_isoc_ec_eseln2
	rdf:type	ns2:Source , skos:Concept ;
	skos:prefLabel	"Eurostat, Table isoc_ec_eseln2: Enterprises selling via internet and/or networks other than internet (NACE Rev. 2 activity)" ;
	foaf:page	ns21:isoc_ec_eseln2 ;
	skos:notation	"estat_isoc_ec_eseln2" ;
	skos:definition	"Eurostat, Table isoc_ec_eseln2: Enterprises selling via internet and/or networks other than internet (NACE Rev. 2 activity)" ;
	skos:topConceptOf	ns6:source .
ns1:estat_isoc_ec_ibuy
	rdf:type	ns2:Source , skos:Concept ;
	skos:prefLabel	"Eurostat, Table isoc_ec_ibuy: Internet purchases by individuals" ;
	foaf:page	ns21:isoc_ec_ibuy ;
	skos:notation	"estat_isoc_ec_ibuy" ;
	skos:definition	"Eurostat, Table isoc_ec_ibuy: Internet purchases by individuals" ;
	skos:topConceptOf	ns6:source .
ns1:estat_isoc_ec_iprb
	rdf:type	ns2:Source , skos:Concept ;
	skos:prefLabel	"eurostat table isoc_ec_iprb " ;
	foaf:page	<http://appsso.eurostat.ec.europa.eu/nui/show.do?dataset=isoc_ec_iprb&lang=en> ;
	skos:notation	"estat_isoc_ec_iprb" ;
	skos:definition	"eurostat table isoc_ec_iprb Problems encountered by individuals when buying/ordering over the internet " ;
	skos:topConceptOf	ns6:source .
ns1:estat_isoc_pibi_ictbn2
	rdf:type	ns2:Source , skos:Concept ;
	skos:prefLabel	"Eurostat, Table isoc_pibi_ictbn2: Adoption of ICT by businesses (NACE Rev. 2 activity)" ;
	foaf:page	ns21:isoc_pibi_ictbn2 ;
	skos:notation	"estat_isoc_pibi_ictbn2" ;
	skos:definition	"Eurostat, Table isoc_pibi_ictbn2: Adoption of ICT by businesses (NACE Rev. 2 activity)" ;
	skos:topConceptOf	ns6:source .
ns1:estat_isoc_r_gov_i
	rdf:type	ns2:Source , skos:Concept ;
	skos:prefLabel	"Eurostat, Table isoc_r_gov_i: Individuals who used the internet for interaction with public authorities" ;
	foaf:page	ns21:isoc_r_gov_i ;
	skos:notation	"estat_isoc_r_gov_i" ;
	skos:definition	"Eurostat, Table isoc_r_gov_i: Individuals who used the internet for interaction with public authorities" ;
	skos:topConceptOf	ns6:source .
ns1:estat_isoc_r_iuse_i
	rdf:type	ns2:Source , skos:Concept ;
	skos:prefLabel	"Eurostat, Table isoc_r_iuse_i: Individuals who used the internet, frequency of use and activities" ;
	foaf:page	ns21:isoc_r_iuse_i ;
	skos:notation	"estat_isoc_r_iuse_i" ;
	skos:definition	"Eurostat, Table isoc_r_iuse_i: Individuals who used the internet, frequency of use and activities" ;
	skos:topConceptOf	ns6:source .
ns1:estat_isoc_sk_cskl_i
	rdf:type	ns2:Source , skos:Concept ;
	skos:prefLabel	"Eurostat, Table isoc_sk_cskl_i: Individuals' level of computer skills" ;
	foaf:page	ns21:isoc_sk_cskl_i ;
	skos:notation	"estat_isoc_sk_cskl_i" ;
	skos:definition	"Eurostat, Table isoc_sk_cskl_i: Individuals' level of computer skills" ;
	skos:topConceptOf	ns6:source .
ns1:estat_isoc_sk_dskl_i
	rdf:type	ns2:Source , skos:Concept ;
	skos:prefLabel	"Eurostat, Table isoc_sk_dskl_i: Individuals' level of digital skills" ;
	foaf:page	ns21:isoc_sk_dskl_i ;
	skos:notation	"estat_isoc_sk_dskl_i" ;
	skos:definition	"Eurostat, Table isoc_sk_dskl_i: Individuals' level of digital skills" ;
	skos:topConceptOf	ns6:source .
ns1:estat_isoc_sk_how_i
	rdf:type	ns2:Source , skos:Concept ;
	skos:prefLabel	"Eurostat, Table isoc_sk_how_i: Way of obtaining e-skills" ;
	foaf:page	ns21:isoc_sk_how_i ;
	skos:notation	"estat_isoc_sk_how_i" ;
	skos:definition	"Eurostat, Table isoc_sk_how_i: Way of obtaining e-skills" ;
	skos:topConceptOf	ns6:source .
ns1:estat_isoc_sk_iskl_i
	rdf:type	ns2:Source , skos:Concept ;
	skos:prefLabel	"Eurostat, Table isoc_sk_iskl_i:  Individuals' level of internet skills" ;
	foaf:page	ns21:isoc_sk_iskl_i ;
	skos:notation	"estat_isoc_sk_iskl_i" ;
	skos:definition	"Eurostat, Table isoc_sk_iskl_i:  Individuals' level of internet skills" ;
	skos:topConceptOf	ns6:source .
ns1:estat_isoc_ske_ittn2
	rdf:type	ns2:Source , skos:Concept ;
	skos:prefLabel	"Eurostat, Table isoc_ske_ittn2 : Enterprises that provided training to develop/upgrade ICT skills of their personnel (NACE Rev. 2 activity)" ;
	foaf:page	ns21:isoc_ske_ittn2 ;
	skos:notation	"estat_isoc_ske_ittn2" ;
	skos:definition	"Eurostat, Table isoc_ske_ittn2 : Enterprises that provided training to develop/upgrade ICT skills of their personnel (NACE Rev. 2 activity)" ;
	skos:topConceptOf	ns6:source .
ns1:estat_isoc_sks_itspt
	rdf:type	ns2:Source , skos:Concept ;
	skos:prefLabel	"Eurostat, Table isoc_sks_itspt: ICT specialists - total" ;
	foaf:page	ns21:isoc_sks_itspt ;
	skos:notation	"estat_isoc_sks_itspt" ;
	skos:definition	"Eurostat, Table isoc_sks_itspt: ICT specialists - total" ;
	skos:topConceptOf	ns6:source .
ns1:estat_lfst_hhnhwhtc
	rdf:type	ns2:Source , skos:Concept ;
	skos:prefLabel	"Eurostat, Table eurostat_lfst_hhnhwhtc: Number of private households by household composition, number of children and working status within households (1 000)" ;
	foaf:page	ns21:lfst_hhnhwhtc ;
	skos:notation	"estat_lfst_hhnhwhtc" ;
	skos:definition	"Eurostat, Table eurostat_lfst_hhnhwhtc: Number of private households by household composition, number of children and working status within households (1 000)" ;
	skos:topConceptOf	ns6:source .
ns1:estat_nama_gdp_c
	rdf:type	ns2:Source , skos:Concept ;
	skos:prefLabel	"Eurostat, Table estat_nama_gdp_c: GDP and main components - Current prices" ;
	foaf:page	ns21:nama_gdp_c ;
	skos:notation	"estat_nama_gdp_c" ;
	skos:definition	"Eurostat, Table estat_nama_gdp_c: GDP and main components - Current prices" ;
	skos:topConceptOf	ns6:source .
ns1:estat_randd
	rdf:type	ns2:Source , skos:Concept ;
	skos:prefLabel	"Eurostat\u2019s statistics on R&D expenditure" ;
	foaf:page	ns22:database ;
	skos:notation	"estat_randd" ;
	skos:definition	"Eurostat\u2019s statistics on R&D expenditure are compiled using guidelines laid out in the Frascati manual (http://www.oecd.org/document/6/0,3343,en_2649_34451_33828550_1_1_1_1,00.html)" ;
	skos:topConceptOf	ns6:source .
ns1:estat_tps00188
	rdf:type	ns2:Source , skos:Concept ;
	skos:prefLabel	"Eurostat, Table estat_tps00188: Science and technology graduates by sex" ;
	foaf:page	ns21:educ_uoe_grad04 ;
	skos:notation	"estat_tps00188" ;
	skos:definition	"Eurostat, Table estat_tps00188: Science and technology graduates by sex" ;
	skos:topConceptOf	ns6:source .
ns1:eun12
	rdf:type	ns2:Source , skos:Concept ;
	skos:prefLabel	"ESSIE Survey about ICT in Education - SMART 2010/0039" ;
	foaf:page	ns21:educ_uoe_grad02 ;
	skos:notation	"eun12" ;
	skos:definition	"The ESSIE Survey about ICT in Education - SMART 2010/0039 - is based on over 190,000 filled questionnaires from students, teachers and head teachers in 27 countries, collected during school-year 2011-12  (mainly between September and December 2011), with the purpose of benchmarking access, use and attitudes to IC Technologies in Europe's schools (Primary; Lower secondary; Upper secondary, both general and vocational)." ;
	skos:note	"Data for 2006 comes from a previous study for the EC by Empirica, only partially comparable." ;
	skos:topConceptOf	ns6:source .
ns1:euripidis-estat
	rdf:type	ns2:Source , skos:Concept ;
	skos:prefLabel	"JRC-IPTS Euripidis project based on Eurostat Business demography data" ;
	foaf:page	ns21:educ_uoe_grad03 ;
	skos:notation	"euripidis-estat" ;
	skos:definition	"Garry Gabison, (forthcoming) \u201CBirth, Survival, Growth, and Death of ICT Companies. How are ICT companies faring in the European Union: a Macroeconomic Analysis.\u201D JRC Scientific and Policy Reports. Seville: JRC-IPTS.  " ;
	skos:topConceptOf	ns6:source .
ns1:eurostat_ed
	rdf:type	ns2:Source , skos:Concept ;
	skos:prefLabel	"Eurostat education statistics (table educ_uoe_grad04 and tps00188) " ;
	foaf:page	ns21:educ_uoe_grad04 ;
	skos:notation	"eurostat_ed" ;
	skos:definition	"Eurostat education statistics (table educ_uoe_grad04 and tps00188) " ;
	skos:topConceptOf	ns6:source .
ns1:eurostat_nat_acc
	rdf:type	ns2:Source , skos:Concept ;
	skos:prefLabel	"Eurostat national accounts" ;
	foaf:page	ns23:database ;
	skos:notation	"eurostat_nat_acc" ;
	skos:definition	"Eurostat national accounts" ;
	skos:note	"extracted 21 may 2014" ;
	skos:topConceptOf	ns6:source .
ns1:eurostat_pop
	rdf:type	ns2:Source , skos:Concept ;
	skos:prefLabel	"Eurostat population statistics" ;
	foaf:page	ns24:database ;
	skos:notation	"eurostat_pop" ;
	skos:definition	"Eurostat population statistics" ;
	skos:note	"extracted 21 may 2013" ;
	skos:topConceptOf	ns6:source .
ns1:idate
	rdf:type	ns2:Source , skos:Concept ;
	skos:prefLabel	"IDATE - Broadband coverage studies (2005-2010)" ;
	foaf:page	ns25:broadband-coverage-eu-272-phase-iii-smart-20100037 ;
	skos:notation	"idate" ;
	skos:definition	"Broadband Coverage in Europe, Studies for the EC realised by IDATE (2005-2010 data), SMART 2010/037" ;
	skos:note	"extraction 4 May 2011" ;
	skos:topConceptOf	ns6:source .
ns1:ihs_tech
	rdf:type	ns2:Source , skos:Concept ;
	skos:prefLabel	"IHS TV Media Intelligence" ;
	foaf:page	<https://technology.ihs.com/account/login?returnUrl=> ;
	skos:notation	"ihs_tech" ;
	skos:definition	"IHS TV Media Intelligence" ;
	skos:topConceptOf	ns6:source .
ns1:ipv6obs
	rdf:type	ns2:Source , skos:Concept ;
	skos:prefLabel	"EC - IPv6 Observatory" ;
	foaf:page	<http://www.ipv6observatory.eu/the-study/> ;
	skos:notation	"ipv6obs" ;
	skos:definition	"IPv6 Observatory, Study for the EC realized by inno" ;
	skos:note	"extraction published 3 June 2012" ;
	skos:topConceptOf	ns6:source .
ns1:jrc-ictspec3
	rdf:type	ns2:Source , skos:Concept ;
	skos:prefLabel	"JRC report on ICT employment 2000-2012" ;
	foaf:page	ns26:definitions ;
	skos:notation	"jrc-ictspec3" ;
	skos:definition	"JRC (IPTS) \"The evolution of EU ICT employment 2000-2012\" Technical report (forthcoming) based on Eurostat - Labour Force Survey" ;
	skos:note	"(forthcoming)" ;
	skos:topConceptOf	ns6:source .
ns1:jrc_ict_randd
	rdf:type	ns2:Source , skos:Concept ;
	skos:prefLabel	"JRC-IPTS Reports on Public ICT R&D Expenditures" ;
	foaf:page	<http://is.jrc.ec.europa.eu/pages/ISG/PREDICT.html> ;
	skos:notation	"jrc_ict_randd" ;
	skos:definition	"JRC-IPTS Reports estimating Public ICT R&D Expenditures in the EU (PREDICT2 project)" ;
	skos:note	"2013 report" ;
	skos:topConceptOf	ns6:source .
ns1:mis
	rdf:type	ns2:Source , skos:Concept ;
	skos:prefLabel	"EC - FP7 ICT research projects" ;
	foaf:page	ns11:ict-research-projects-under-eus-seventh-framework-programme-fp7 ;
	skos:notation	"mis" ;
	skos:definition	"EC database of ICT research projects under the EU's Seventh Framework Programme (FP7) - Cooperation and Capacities (e-infrastructures) programs. Projects under the CIP ICT PSP are not included. More information on the Programmes at http://cordis.europa.eu/fp7/ict/home_en.html" ;
	skos:note	"Extraction January 2013" ;
	skos:topConceptOf	ns6:source .
ns1:nif_database
	rdf:type	ns2:Source , skos:Concept ;
	skos:prefLabel	"NIF_database" ;
	skos:notation	"nif_database" ;
	skos:definition	"NIF_database" ;
	skos:topConceptOf	ns6:source .
ns1:point_topic
	rdf:type	ns2:Source , skos:Concept ;
	skos:prefLabel	"Point Topic Study on broadband coverage" ;
	foaf:page	ns13:about-fast-and-ultra-fast-internet-access ;
	skos:notation	"point_topic" ;
	skos:definition	"Broadband coverage in Europe, studies for the EC by Point Topic (2011-2012 figures, SMART 2011/0027 and 2012/0035) and IHS and Valdani, Vicari & Associati (2013 figures, SMART 2013/0054)" ;
	skos:topConceptOf	ns6:source .
ns1:samknows
	rdf:type	ns2:Source , skos:Concept ;
	skos:prefLabel	"Study on \"Quality of Broadband Services in the EU\u201D SMART 2010/0036" ;
	foaf:page	ns25:quality-broadband-services-eu-samknows-study-internet-speeds ;
	skos:notation	"samknows" ;
	skos:definition	"Study on \"Quality of Broadband Services in the EU\u201D (SMART 2010/0036). For the purposes of this study 9,104 households across the European Union were given a specially configured hardware device (SamKnows Whitebox), which runs a series of purpose-built tests to measure every aspect of Internet performance. The sample is designed to represent tha main fixed broadband services, used by consumers and available all around the country." ;
	skos:note	"April 2013 Report" ;
	skos:topConceptOf	ns6:source .
ns1:smart11_39
	rdf:type	ns2:Source , skos:Concept ;
	skos:prefLabel	"Analysis of publications and patents of ICT research in FP7" ;
	foaf:page	ns27:our-studies-and-open-datasets ;
	skos:notation	"smart11_39" ;
	skos:definition	"Analysis conducted by DG CONNECT Unit F4, based on results of the study SMART 2011/0039 which main results are published in: Jacob, J., Sanditov, B., Smirnov, E., Wintjes, R., Surpatean, A., Notten, A., & Sasso, S. (Forthcoming). Analysis of publications and patents of ICT research in FP7. Brussels, European Commission. " ;
	skos:topConceptOf	ns6:source .
ns1:cocom_new
	rdf:type	ns2:Source , skos:Concept ;
	skos:prefLabel	"Communications Committee survey" ;
	foaf:page	ns28:broadband-connectivity ;
	skos:notation	"cocom_new" ;
	skos:definition	"European Commission services, through the Communications Committee (COCOM)" ;
	skos:topConceptOf	ns6:source .
ns1:european_data_portal
	rdf:type	ns2:Source , skos:Concept ;
	skos:prefLabel	"European Data Portal" ;
	foaf:page	ns29:open-data-maturity ;
	skos:notation	"european_data_portal" ;
	skos:definition	"European Data Portal" ;
	skos:topConceptOf	ns6:source .
ns1:estat_isoc_eb_ai
	rdf:type	ns2:Source , skos:Concept ;
	skos:prefLabel	"Eurostat, Table isoc_eb_ai: Artificial intelligence" ;
	foaf:page	ns5:isoc_eb_ai ;
	skos:notation	"estat_isoc_eb_ai" ;
	skos:definition	"Eurostat, Table isoc_eb_ai: Artificial intelligence" ;
	skos:topConceptOf	ns6:source .
ns1:estat_isoc_sk_dskl_i21
	rdf:type	ns2:Source , skos:Concept ;
	skos:prefLabel	"Eurostat, Table isoc_sk_dskl_i21: Individuals' level of digital skills" ;
	foaf:page	ns5:isoc_sk_dskl_i21 ;
	skos:notation	"estat_isoc_sk_dskl_i21" ;
	skos:definition	"Eurostat, Table isoc_sk_dskl_i21: Individuals' level of digital skills (from 2021 onwards)" ;
	skos:topConceptOf	ns6:source .
ns1:bc2020
	rdf:type	ns2:Source , skos:Concept ;
	skos:prefLabel	"Broadband coverage in Europe studies" ;
	foaf:page	ns28:broadband-connectivity ;
	skos:notation	"bc2020" ;
	skos:definition	"IHS Markit, Omdia, Point Topic and VVA, Broadband coverage in Europe studies" ;
	skos:topConceptOf	ns6:source .
ns1:estat_isoc_e_dii
	rdf:type	ns2:Source , skos:Concept ;
	skos:prefLabel	"Eurostat, Table isoc_e_dii: Digital Intensity" ;
	foaf:page	ns5:isoc_e_dii ;
	skos:notation	"estat_isoc_e_dii" ;
	skos:definition	"Eurostat, Table isoc_e_dii: Digital Intensity" ;
	skos:topConceptOf	ns6:source .
ns1:estat_isoc_eb_bd
	rdf:type	ns2:Source , skos:Concept ;
	skos:prefLabel	"Eurostat, Table isoc_eb_bd: Big data analysis" ;
	foaf:page	ns5:isoc_eb_bd ;
	skos:notation	"estat_isoc_eb_bd" ;
	skos:definition	"Eurostat, Table isoc_eb_bd: Big data analysis" ;
	skos:topConceptOf	ns6:source .
ns1:estathh_cocom
	rdf:type	ns2:Source , skos:Concept ;
	skos:prefLabel	"European Commission based on Eurostat - ICT Household survey and Communications Committee survey" ;
	skos:notation	"estathh_cocom" ;
	skos:definition	"European Commission based on Eurostat - Community survey on ICT usage in Households and by Individuals, and Electronic communications market indicators collected by Commission services, through National Regulatory Authorities, for the Communications Committee (COCOM) - January and July reports." ;
	skos:topConceptOf	ns6:source .
ns1:e_gov_bench
	rdf:type	ns2:Source , skos:Concept ;
	skos:prefLabel	"eGovernment Benchmarking Report" ;
	foaf:page	ns15:egovernment-benchmark-2018-digital-efforts-european-countries-are-visibly-paying ;
	skos:notation	"e_gov_bench" ;
	skos:definition	"eGovernment Benchmarking Report" ;
	skos:topConceptOf	ns6:source .
ns1:desi_4g
	rdf:type	ns2:Source , skos:Concept ;
	skos:prefLabel	"Broadband coverage in Europe studies for the European Commission by IHS Markit, Omdia and Point Topic" ;
	skos:notation	"desi_4g" ;
	skos:definition	"Broadband coverage in Europe studies for the European Commission by IHS Markit, Omdia and Point Topic" ;
	skos:topConceptOf	ns6:source .
ns1:desi_5g
	rdf:type	ns2:Source , skos:Concept ;
	skos:prefLabel	"European Commission services, through the Communications Committee (COCOM)" ;
	skos:notation	"desi_5g" ;
	skos:definition	"European Commission services, through the Communications Committee (COCOM)" ;
	skos:topConceptOf	ns6:source .
ns1:desi_5gc
	rdf:type	ns2:Source , skos:Concept ;
	skos:prefLabel	"Broadband coverage in Europe studies for the European Commission by IHS Markit, Omdia and Point Topic" ;
	skos:notation	"desi_5gc" ;
	skos:definition	"Broadband coverage in Europe studies for the European Commission by IHS Markit, Omdia and Point Topic" ;
	skos:topConceptOf	ns6:source .
ns1:desi_bbpi
	rdf:type	ns2:Source , skos:Concept ;
	skos:prefLabel	"Broadband retail prices study, annual studies for the European Commission realised by Empirica" ;
	skos:notation	"desi_bbpi" ;
	skos:definition	"Broadband retail prices study, annual studies for the European Commission realised by Empirica" ;
	skos:topConceptOf	ns6:source .
ns1:desi_dps_egovuser
	rdf:type	ns2:Source , skos:Concept ;
	skos:prefLabel	"Eurostat - European Union survey on ICT usage in Households and by Individuals (I_IUGOV12)" ;
	skos:notation	"desi_dps_egovuser" ;
	skos:definition	"Eurostat - European Union survey on ICT usage in Households and by Individuals (I_IUGOV12)" ;
	skos:topConceptOf	ns6:source .
ns1:desi_dps_opendata
	rdf:type	ns2:Source , skos:Concept ;
	skos:prefLabel	"European Data Portal" ;
	skos:notation	"desi_dps_opendata" ;
	skos:definition	"European Data Portal" ;
	skos:topConceptOf	ns6:source .
ns1:desi_dps_prefform
	rdf:type	ns2:Source , skos:Concept ;
	skos:prefLabel	"eGovernment Benchmark" ;
	skos:notation	"desi_dps_prefform" ;
	skos:definition	"eGovernment Benchmark" ;
	skos:topConceptOf	ns6:source .
ns1:desi_dps_psbiz
	rdf:type	ns2:Source , skos:Concept ;
	skos:prefLabel	"eGovernment Benchmark" ;
	skos:notation	"desi_dps_psbiz" ;
	skos:definition	"eGovernment Benchmark" ;
	skos:topConceptOf	ns6:source .
ns1:desi_dps_pscit
	rdf:type	ns2:Source , skos:Concept ;
	skos:prefLabel	"eGovernment Benchmark" ;
	skos:notation	"desi_dps_pscit" ;
	skos:definition	"eGovernment Benchmark" ;
	skos:topConceptOf	ns6:source .
ns1:desi_fbbc
	rdf:type	ns2:Source , skos:Concept ;
	skos:prefLabel	"Broadband coverage in Europe studies for the European Commission by IHS Markit, Omdia and Point Topic" ;
	skos:notation	"desi_fbbc" ;
	skos:definition	"Broadband coverage in Europe studies for the European Commission by IHS Markit, Omdia and Point Topic" ;
	skos:topConceptOf	ns6:source .
ns1:desi_fbbtc
	rdf:type	ns2:Source , skos:Concept ;
	skos:prefLabel	"Eurostat - European Union survey on ICT usage in Households and by Individuals [H_BBFIX]" ;
	skos:notation	"desi_fbbtc" ;
	skos:definition	"Eurostat - European Union survey on ICT usage in Households and by Individuals [H_BBFIX]" ;
	skos:topConceptOf	ns6:source .
ns1:desi_gbpstc
	rdf:type	ns2:Source , skos:Concept ;
	skos:prefLabel	"European  Commission, through the Communications Committee (COCOM) and Eurostat - European Union survey on ICT usage in Households and by Individuals" ;
	skos:notation	"desi_gbpstc" ;
	skos:definition	"European  Commission, through the Communications Committee (COCOM) and Eurostat - European Union survey on ICT usage in Households and by Individuals" ;
	skos:topConceptOf	ns6:source .
ns1:desi_hc_abds
	rdf:type	ns2:Source , skos:Concept ;
	skos:prefLabel	"Eurostat - European Union survey on ICT usage in Households and by Individuals" ;
	skos:notation	"desi_hc_abds" ;
	skos:definition	"Eurostat - European Union survey on ICT usage in Households and by Individuals" ;
	skos:topConceptOf	ns6:source .
ns1:desi_hc_abss
	rdf:type	ns2:Source , skos:Concept ;
	skos:prefLabel	"Eurostat - European Union survey on ICT usage in Households and by Individuals" ;
	skos:notation	"desi_hc_abss" ;
	skos:definition	"Eurostat - European Union survey on ICT usage in Households and by Individuals" ;
	skos:topConceptOf	ns6:source .
ns1:desi_hc_bds
	rdf:type	ns2:Source , skos:Concept ;
	skos:prefLabel	"Eurostat - European Union survey on ICT usage in Households and by Individuals" ;
	skos:notation	"desi_hc_bds" ;
	skos:definition	"Eurostat - European Union survey on ICT usage in Households and by Individuals" ;
	skos:topConceptOf	ns6:source .
ns1:desi_hc_entict
	rdf:type	ns2:Source , skos:Concept ;
	skos:prefLabel	"Eurostat - European Union survey on ICT usage and eCommerce in Enterprises (E_ITT2)" ;
	skos:notation	"desi_hc_entict" ;
	skos:definition	"Eurostat - European Union survey on ICT usage and eCommerce in Enterprises (E_ITT2)" ;
	skos:topConceptOf	ns6:source .
ns1:desi_hc_fictspec
	rdf:type	ns2:Source , skos:Concept ;
	skos:prefLabel	"Eurostat - Labour force survey (isoc_sks_itsps)" ;
	skos:notation	"desi_hc_fictspec" ;
	skos:definition	"Eurostat - Labour force survey (isoc_sks_itsps)" ;
	skos:topConceptOf	ns6:source .
ns1:desi_hc_ictg
	rdf:type	ns2:Source , skos:Concept ;
	skos:prefLabel	"Eurostat (table educ_uoe_grad03, using selection ISCED11=ED5-8) and and ISCEDF_13 [F06] Information and Communication Technologies " ;
	skos:notation	"desi_hc_ictg" ;
	skos:definition	"Eurostat (table educ_uoe_grad03, using selection ISCED11=ED5-8) and and ISCEDF_13 [F06] Information and Communication Technologies " ;
	skos:topConceptOf	ns6:source .
ns1:desi_hc_ictspec
	rdf:type	ns2:Source , skos:Concept ;
	skos:prefLabel	"Eurostat - Labour force survey (isoc_sks_itspt)" ;
	skos:notation	"desi_hc_ictspec" ;
	skos:definition	"Eurostat - Labour force survey (isoc_sks_itspt)" ;
	skos:topConceptOf	ns6:source .
ns1:desi_idt_ai
	rdf:type	ns2:Source , skos:Concept ;
	skos:prefLabel	"European enterprise survey on the use of technologies based on artificial intelligence by Ipsos and iCite" ;
	skos:notation	"desi_idt_ai" ;
	skos:definition	"European enterprise survey on the use of technologies based on artificial intelligence by Ipsos and iCite" ;
	skos:topConceptOf	ns6:source .
ns1:desi_idt_bigdat
	rdf:type	ns2:Source , skos:Concept ;
	skos:prefLabel	"Eurostat - European Union survey on ICT usage and eCommerce in Enterprises (E_BDA)" ;
	skos:notation	"desi_idt_bigdat" ;
	skos:definition	"Eurostat - European Union survey on ICT usage and eCommerce in Enterprises (E_BDA)" ;
	skos:topConceptOf	ns6:source .
ns1:desi_idt_cloud
	rdf:type	ns2:Source , skos:Concept ;
	skos:prefLabel	"Eurostat - European Union survey on ICT usage and eCommerce in Enterprises (E_CC_GE_ME)" ;
	skos:notation	"desi_idt_cloud" ;
	skos:definition	"Eurostat - European Union survey on ICT usage and eCommerce in Enterprises (E_CC_GE_ME)" ;
	skos:topConceptOf	ns6:source .
ns1:desi_idt_ecomturn
	rdf:type	ns2:Source , skos:Concept ;
	skos:prefLabel	"Eurostat - European Union survey on ICT usage and eCommerce in Enterprises (E_ETURN)" ;
	skos:notation	"desi_idt_ecomturn" ;
	skos:definition	"Eurostat - European Union survey on ICT usage and eCommerce in Enterprises (E_ETURN)" ;
	skos:topConceptOf	ns6:source .
ns1:desi_idt_einv
	rdf:type	ns2:Source , skos:Concept ;
	skos:prefLabel	"Eurostat - European Union survey on ICT usage and eCommerce in Enterprises (E_INV4S_AP)" ;
	skos:notation	"desi_idt_einv" ;
	skos:definition	"Eurostat - European Union survey on ICT usage and eCommerce in Enterprises (E_INV4S_AP)" ;
	skos:topConceptOf	ns6:source .
ns1:desi_idt_eis
	rdf:type	ns2:Source , skos:Concept ;
	skos:prefLabel	"Eurostat - European Union survey on ICT usage and eCommerce in Enterprises (E_ERP1)" ;
	skos:notation	"desi_idt_eis" ;
	skos:definition	"Eurostat - European Union survey on ICT usage and eCommerce in Enterprises (E_ERP1)" ;
	skos:topConceptOf	ns6:source .
ns1:desi_idt_ictsust
	rdf:type	ns2:Source , skos:Concept ;
	skos:prefLabel	"Survey of businesses on the use of digital technologies by Ipsos and iCite" ;
	skos:notation	"desi_idt_ictsust" ;
	skos:definition	"Survey of businesses on the use of digital technologies by Ipsos and iCite" ;
	skos:topConceptOf	ns6:source .
ns1:desi_idt_sellcb
	rdf:type	ns2:Source , skos:Concept ;
	skos:prefLabel	"Eurostat - European Union survey on ICT usage and eCommerce in Enterprises (E_AESEU)" ;
	skos:notation	"desi_idt_sellcb" ;
	skos:definition	"Eurostat - European Union survey on ICT usage and eCommerce in Enterprises (E_AESEU)" ;
	skos:topConceptOf	ns6:source .
ns1:desi_idt_smedi
	rdf:type	ns2:Source , skos:Concept ;
	skos:prefLabel	"Eurostat - European Union survey on ICT usage and eCommerce in Enterprises" ;
	skos:notation	"desi_idt_smedi" ;
	skos:definition	"Eurostat - European Union survey on ICT usage and eCommerce in Enterprises" ;
	skos:topConceptOf	ns6:source .
ns1:desi_idt_smeso
	rdf:type	ns2:Source , skos:Concept ;
	skos:prefLabel	"Eurostat - European Union survey on ICT usage and eCommerce in Enterprises (E_ESELL)" ;
	skos:notation	"desi_idt_smeso" ;
	skos:definition	"Eurostat - European Union survey on ICT usage and eCommerce in Enterprises (E_ESELL)" ;
	skos:topConceptOf	ns6:source .
ns1:desi_idt_socmed
	rdf:type	ns2:Source , skos:Concept ;
	skos:prefLabel	"Eurostat - European Union survey on ICT usage and eCommerce in Enterprises (E_SM1_GE2)" ;
	skos:notation	"desi_idt_socmed" ;
	skos:definition	"Eurostat - European Union survey on ICT usage and eCommerce in Enterprises (E_SM1_GE2)" ;
	skos:topConceptOf	ns6:source .
ns1:desi_mbbtu
	rdf:type	ns2:Source , skos:Concept ;
	skos:prefLabel	"Eurostat - European Union survey on ICT usage in Households and by Individuals [I_IUMP]" ;
	skos:notation	"desi_mbbtu" ;
	skos:definition	"Eurostat - European Union survey on ICT usage in Households and by Individuals [I_IUMP]" ;
	skos:topConceptOf	ns6:source .
ns1:desi_ufbbtu
	rdf:type	ns2:Source , skos:Concept ;
	skos:prefLabel	"European  Commission, through the Communications Committee (COCOM) and Eurostat - European Union survey on ICT usage in Households and by Individuals" ;
	skos:notation	"desi_ufbbtu" ;
	skos:definition	"European  Commission, through the Communications Committee (COCOM) and Eurostat - European Union survey on ICT usage in Households and by Individuals" ;
	skos:topConceptOf	ns6:source .
ns1:desi_vhcnc
	rdf:type	ns2:Source , skos:Concept ;
	skos:prefLabel	"Broadband coverage in Europe studies for the European Commission by IHS Markit, Omdia and Point Topic" ;
	skos:notation	"desi_vhcnc" ;
	skos:definition	"Broadband coverage in Europe studies for the European Commission by IHS Markit, Omdia and Point Topic" ;
	skos:topConceptOf	ns6:source .
