@prefix rdf:	<http://www.w3.org/1999/02/22-rdf-syntax-ns#> .
@prefix ns1:	<http://semantic.digital-agenda-data.eu/codelist/> .
@prefix skos:	<http://www.w3.org/2004/02/skos/core#> .
ns1:breakdown	rdf:type	skos:ConceptScheme .
@prefix ns3:	<http://purl.org/linked-data/sdmx#> .
ns1:breakdown	rdf:type	ns3:CodeList .
@prefix xsd:	<http://www.w3.org/2001/XMLSchema#> .
@prefix dct:	<http://purl.org/dc/terms/> .
ns1:breakdown	dct:modified	"2018-12-07T18:30:29+02:00"^^xsd:dateTime .
@prefix rdfs:	<http://www.w3.org/2000/01/rdf-schema#> .
ns1:breakdown	rdfs:isDefinedBy	<http://digital-agenda-data.eu/> ;
	skos:notation	"CL_BREAKDOWN" .
@prefix ns7:	<http://semantic.digital-agenda-data.eu/codelist/breakdown/> .
ns1:breakdown	skos:hasTopConcept	ns7:e_gov_events_4 ,
		ns7:e_gov_events_5 ,
		ns7:e_gov_events_2 ,
		ns7:e_gov_events_3 ,
		ns7:e_gov_events_8 ,
		ns7:egov_life_events ,
		ns7:e_gov_events_6 ,
		ns7:e_gov_events_7 ,
		ns7:e_gov_5b_ke_edoc ,
		ns7:e_gov_5c_ke_as ,
		ns7:e_gov_4f_bm_su ,
		ns7:e_gov_5a_ke_eid ,
		ns7:e_gov_5f_ke_sso ,
		ns7:e_gov_events_1 ,
		ns7:e_gov_5d_ke_dp ,
		ns7:e_gov_5e_ke_esafe ,
		ns7:e_gov_3f_cm_su ,
		ns7:e_gov_4a_bm_oa ,
		ns7:e_gov_3d_cm_edoccb ,
		ns7:e_gov_3e_cm_eu ,
		ns7:e_gov_4d_bm_edoccb ,
		ns7:e_gov_4e_bm_eu ,
		ns7:e_gov_4b_bm_us ,
		ns7:e_gov_4c_bm_eidcb ,
		ns7:e_gov_2a_tg_sd ,
		ns7:e_gov_2b_tg_po ,
		ns7:e_gov_1d_ucg_eu ,
		ns7:e_gov_1e_ucg_su ,
		ns7:e_gov_3b_cm_us ,
		ns7:e_gov_3c_cm_eidcb ,
		ns7:e_gov_2c_tg_pd ,
		ns7:e_gov_3a_cm_oa ,
		ns7:e_gov_1b_ucg_us ,
		ns7:e_gov_1c_ucg_mf ,
		ns7:e_gov_1a_ucg_oa ,
		ns7:egov_le_bus ,
		ns7:desi_5a_egov ,
		ns7:desi_5b1_mdataexch ,
		ns7:desi_5a3_osercomp ,
		ns7:desi_5a4_opendata ,
		ns7:desi_total ,
		ns7:ds_a_basic ,
		ns7:desi_5b2_epresc ,
		ns7:desi_5b_ehealth ,
		ns7:desi_4b2_ecomturn ,
		ns7:desi_4b3_sellcb ,
		ns7:desi_4a_bd ,
		ns7:desi_4b1_smeso ,
		ns7:desi_5a1_egovu ,
		ns7:desi_5a2_prefform ,
		ns7:desi_4b_ecomm ,
		ns7:desi_5_dps ,
		ns7:desi_4_idt ,
		ns7:desi_4a1_eis ,
		ns7:desi_3c2_shop ,
		ns7:desi_3c_trans ,
		ns7:desi_4a4_einv ,
		ns7:desi_4a5_cloud ,
		ns7:desi_4a2_rfid ,
		ns7:desi_4a3_socmed ,
		ns7:desi_3a4_iptv ,
		ns7:desi_3a_cont ,
		ns7:desi_3a2_mvg ,
		ns7:desi_3a3_vod ,
		ns7:desi_3b_comm ,
		ns7:desi_3c1_bank ,
		ns7:desi_3b1_vidcall ,
		ns7:desi_3b2_socnet ,
		ns7:epsiscore_practice ,
		ns7:epsiscore_pricing ,
		ns7:epsiscore_implem ,
		ns7:epsiscore_localpsi ,
		ns7:f_y16_74 ,
		ns7:fttx ,
		ns7:epsiscore_total ,
		ns7:f ,
		ns7:ent_m_xfin ,
		ns7:ent_s_xfin ,
		ns7:ent_all_xfin ,
		ns7:ent_l_xfin ,
		ns7:epsiscore_exarrange ,
		ns7:epsiscore_formats ,
		ns7:ent_sm_xfin ,
		ns7:epsiscore_events ,
		ns7:e_di_lo ,
		ns7:e_di_vhi ,
		ns7:e_cc_me ,
		ns7:e_di_hi ,
		ns7:einfra ,
		ns7:empl_une ,
		ns7:e_di_vlo ,
		ns7:ec_all ,
		ns7:ds_no ,
		ns7:dsk_ab ,
		ns7:ds_b_basic ,
		ns7:ds_basic ,
		ns7:e_cc_hi ,
		ns7:e_cc_lo ,
		ns7:dsk_b ,
		ns7:dsk_x ,
		ns7:cc_eu_for ,
		ns7:cc_ext_eu ,
		ns7:cb_ext_eu ,
		ns7:cb_nat ,
		ns7:cnect_all ,
		<http://semantic.digital-agenda-data.eu/codelist/breakdown/cnect_b+> ,
		ns7:cc_nat ,
		ns7:cnect_a ,
		ns7:all_dch ,
		ns7:all_egov_le ,
		<http://semantic.digital-agenda-data.eu/codelist/breakdown/800_mhz> ,
		<http://semantic.digital-agenda-data.eu/codelist/breakdown/900_mhz> ,
		ns7:cable ,
		ns7:cb_eu_for ,
		ns7:all_ndch ,
		ns7:bus_startup ,
		<http://semantic.digital-agenda-data.eu/codelist/breakdown/3_4_ghz> ,
		<http://semantic.digital-agenda-data.eu/codelist/breakdown/3_6_ghz> ,
		<http://semantic.digital-agenda-data.eu/codelist/breakdown/2_6_ghz> ,
		<http://semantic.digital-agenda-data.eu/codelist/breakdown/2_ghz_paired> ,
		<http://semantic.digital-agenda-data.eu/codelist/breakdown/61_582_62_631_951> ,
		<http://semantic.digital-agenda-data.eu/codelist/breakdown/700_mhz> ,
		<http://semantic.digital-agenda-data.eu/codelist/breakdown/582_62_631_951> ,
		<http://semantic.digital-agenda-data.eu/codelist/breakdown/61> ,
		<http://semantic.digital-agenda-data.eu/codelist/breakdown/261> ,
		<http://semantic.digital-agenda-data.eu/codelist/breakdown/261to264> ,
		<http://semantic.digital-agenda-data.eu/codelist/breakdown/1800_mhz> ,
		<http://semantic.digital-agenda-data.eu/codelist/breakdown/1m_websites> ,
		<http://semantic.digital-agenda-data.eu/codelist/breakdown/263> ,
		<http://semantic.digital-agenda-data.eu/codelist/breakdown/264> ,
		<http://semantic.digital-agenda-data.eu/codelist/breakdown/261to264_582_61_62_631_951> ,
		<http://semantic.digital-agenda-data.eu/codelist/breakdown/262> ,
		ns7:desi_2a_bsu ,
		ns7:desi_2b1_ictspec ,
		ns7:desi_2a1_iu ,
		ns7:desi_2a2_bds ,
		ns7:desi_3_ui ,
		ns7:desi_3a1_news ,
		ns7:desi_2b2_stemg ,
		ns7:desi_2b_asd ,
		ns7:desi_1c1_ngac ,
		ns7:desi_1c2_sfbb ,
		ns7:desi_1b3_spec ,
		ns7:desi_1b_mbb ,
		ns7:desi_1d_aff ,
		ns7:desi_2_hc ,
		ns7:desi_1c_speed ,
		ns7:desi_1d1_fbbp ,
		ns7:desi_1_conn ,
		ns7:desi_1a1_fbbc ,
		ns7:csk_lo ,
		ns7:cskx ,
		ns7:desi_1b1_mbbtu ,
		ns7:desi_1b2_4g ,
		ns7:desi_1a2_fbbtu ,
		ns7:desi_1a_fbb ,
		ns7:cnect_e ,
		ns7:cnect_f ,
		ns7:cnect_c ,
		ns7:cnect_d ,
		ns7:cnect_r ,
		ns7:csk_hi ,
		ns7:cnect_g ,
		ns7:cnect_h ,
		ns7:so_18 ,
		ns7:so_19 ,
		ns7:so_16 ,
		ns7:so_17 ,
		ns7:so_22_1 ,
		ns7:so_22_2 ,
		ns7:so_20 ,
		ns7:so_21 ,
		ns7:so_10 ,
		ns7:so_11 ,
		ns7:so_08 ,
		ns7:so_09 ,
		ns7:so_14 ,
		ns7:so_15 ,
		ns7:so_12 ,
		ns7:so_13 ,
		ns7:so_02 ,
		ns7:so_03 ,
		ns7:small_claims ,
		ns7:so_01 ,
		ns7:so_06 ,
		ns7:so_07 ,
		ns7:so_04 ,
		ns7:so_05 ,
		ns7:s_c10_f43 ,
		ns7:s_c10_s951_xk ,
		ns7:rf_ge2 ,
		ns7:rural_pop ,
		ns7:services ,
		ns7:sm_c10_s951_xk ,
		ns7:s_g45_s951_xk ,
		ns7:sal_self_fam ,
		ns7:y25_64 ,
		ns7:y35_44 ,
		ns7:y16_24 ,
		ns7:y25_34 ,
		ns7:y55_74 ,
		ns7:y65_74 ,
		ns7:y45_54 ,
		ns7:y55_64 ,
		ns7:total_pop ,
		ns7:total_pophh ,
		ns7:total_mob ,
		ns7:total_offers8plus ,
		ns7:une ,
		ns7:xdsl ,
		ns7:total_sos ,
		ns7:total_tel ,
		ns7:stud ,
		ns7:study ,
		ns7:speed_ge100 ,
		ns7:speed_l2 ,
		ns7:total_fbb ,
		ns7:total_mbb ,
		ns7:tot_ict_products ,
		ns7:total ,
		ns7:so_24 ,
		ns7:so_25 ,
		ns7:so_22_3 ,
		ns7:so_23 ,
		ns7:speed_2l10 ,
		ns7:speed_30l100 ,
		ns7:so_26 ,
		ns7:speed_10l30 ,
		ns7:infso_a ,
		ns7:infso_all ,
		ns7:ind_o1 ,
		ns7:ind_total ,
		ns7:infso_d ,
		ns7:infso_e ,
		ns7:infso_b ,
		ns7:infso_c ,
		ns7:i3_4 ,
		ns7:i5_8 ,
		ns7:i0_2 ,
		ns7:i0_4 ,
		ns7:ind_deg3 ,
		ns7:ind_no1 ,
		ns7:ind_deg1 ,
		ns7:ind_deg2 ,
		ns7:hh_o1 ,
		ns7:hh_total ,
		ns7:hh_deg3 ,
		ns7:hh_no1 ,
		ns7:hhi_q3 ,
		ns7:hhi_q4 ,
		ns7:hhi_q1 ,
		ns7:hhi_q2 ,
		ns7:grade11gen ,
		ns7:grade11voc ,
		ns7:gen_admin_move ,
		ns7:goods ,
		ns7:hh_deg1 ,
		ns7:hh_deg2 ,
		ns7:grade4 ,
		ns7:grade8 ,
		ns7:own_drive_car ,
		ns7:reg_bus_op ,
		ns7:other_eu_countries ,
		ns7:own_country ,
		ns7:rf_0 ,
		ns7:rf_ge1 ,
		ns7:rest_world ,
		ns7:retir_other ,
		ns7:offer_8_12_mbps ,
		ns7:orgclass_hesrec ,
		ns7:offer_30_100_mbps ,
		ns7:offer_30_mbps ,
		ns7:orgclass_sme ,
		ns7:orgclass_total ,
		ns7:orgclass_le ,
		ns7:orgclass_nil ,
		ns7:m_c10_s951_xk ,
		ns7:m_g45_s951_xk ,
		ns7:m ,
		ns7:m_c10_f43 ,
		ns7:offer_100_mbps ,
		ns7:offer_12_30_mbps ,
		ns7:m_y16_74 ,
		ns7:not_assigned ,
		ns7:infso_h ,
		ns7:infso_r ,
		ns7:infso_f ,
		ns7:infso_g ,
		ns7:l_g45_s951_xk ,
		ns7:lose_find_job ,
		ns7:l_c10_f43 ,
		ns7:l_c10_s951_xk ,
		<http://semantic.digital-agenda-data.eu/codelist/breakdown/10_j62_63> ,
		<http://semantic.digital-agenda-data.eu/codelist/breakdown/10_l68> ,
		<http://semantic.digital-agenda-data.eu/codelist/breakdown/10_j58_60> ,
		<http://semantic.digital-agenda-data.eu/codelist/breakdown/10_j61> ,
		<http://semantic.digital-agenda-data.eu/codelist/breakdown/10_s951> ,
		<http://semantic.digital-agenda-data.eu/codelist/breakdown/1500_mhz> ,
		<http://semantic.digital-agenda-data.eu/codelist/breakdown/10_m69_74> ,
		<http://semantic.digital-agenda-data.eu/codelist/breakdown/10_n77_82> ,
		<http://semantic.digital-agenda-data.eu/codelist/breakdown/10_c31_33> ,
		<http://semantic.digital-agenda-data.eu/codelist/breakdown/10_f41_43> ,
		<http://semantic.digital-agenda-data.eu/codelist/breakdown/10_c27_28> ,
		<http://semantic.digital-agenda-data.eu/codelist/breakdown/10_c29_30> ,
		<http://semantic.digital-agenda-data.eu/codelist/breakdown/10_h49_53> ,
		<http://semantic.digital-agenda-data.eu/codelist/breakdown/10_i55_56> ,
		<http://semantic.digital-agenda-data.eu/codelist/breakdown/10_g46> ,
		<http://semantic.digital-agenda-data.eu/codelist/breakdown/10_g47> ,
		<http://semantic.digital-agenda-data.eu/codelist/breakdown/10_c13_15> ,
		<http://semantic.digital-agenda-data.eu/codelist/breakdown/10_c16_18> ,
		<http://semantic.digital-agenda-data.eu/codelist/breakdown/10_c10_33> ,
		<http://semantic.digital-agenda-data.eu/codelist/breakdown/10_c10_s951_xk> ,
		<http://semantic.digital-agenda-data.eu/codelist/breakdown/10_c26> ,
		<http://semantic.digital-agenda-data.eu/codelist/breakdown/10_c26_33> ,
		<http://semantic.digital-agenda-data.eu/codelist/breakdown/10_c19_23> ,
		<http://semantic.digital-agenda-data.eu/codelist/breakdown/10_c24_25> ,
		<http://semantic.digital-agenda-data.eu/codelist/breakdown/10_c10_12> ,
		<http://semantic.digital-agenda-data.eu/codelist/breakdown/10_c10_18> ,
		ns7:wid_score ,
		ns7:info_online_portal ,
		ns7:offline ,
		ns7:family ,
		ns7:info_online_no_portal ,
		ns7:serv_online_no_portal ,
		ns7:serv_online_portal ,
		ns7:desi_5a5_opendata ,
		ns7:desi_5b1_ehs ,
		ns7:desi_1e_bbpi ,
		ns7:desi_5a4_psb ,
		ns7:edocuments ,
		ns7:eid ,
		ns7:desi_5b_ehs ,
		ns7:digital_post ,
		ns7:desi_1b1_4g ,
		ns7:desi_1b2_mbbtu ,
		ns7:authentic_sources ,
		ns7:auto_service ,
		ns7:desi_1d_ultra ,
		ns7:desi_1e1_bbpi ,
		ns7:desi_1d1_ubbc ,
		ns7:desi_1d2_ubbta ,
		<http://semantic.digital-agenda-data.eu/codelist/breakdown/10_d35_e39> ,
		ns7:csk_me ,
		<http://semantic.digital-agenda-data.eu/codelist/breakdown/10_g45> ,
		ns7:y25_54 .
@prefix ns8:	<http://semantic.digital-agenda-data.eu/def/> .
ns1:breakdown	skos:inScheme	ns8:scheme ;
	skos:prefLabel	"Code list for breakdowns used by Digital Agenda Scoreboard" .
@prefix ns9:	<http://semantic.digital-agenda-data.eu/codelist/breakdown-group/by_location/> .
@prefix ns10:	<http://semantic.digital-agenda-data.eu/def/class/> .
ns9:other_eu_countries	rdf:type	ns10:BreakdownToGroupMembership ;
	rdfs:label	"by_location" .
@prefix ns11:	<http://semantic.digital-agenda-data.eu/def/property/> .
@prefix ns12:	<http://semantic.digital-agenda-data.eu/codelist/breakdown-group/> .
ns9:other_eu_countries	ns11:member-of	ns12:by_location ;
	ns11:order	"2" .
ns9:own_country	rdf:type	ns10:BreakdownToGroupMembership ;
	rdfs:label	"by_location" ;
	ns11:member-of	ns12:by_location ;
	ns11:order	"1" .
ns9:rest_world	rdf:type	ns10:BreakdownToGroupMembership ;
	rdfs:label	"by_location" ;
	ns11:member-of	ns12:by_location ;
	ns11:order	"3" .
@prefix ns13:	<http://semantic.digital-agenda-data.eu/codelist/breakdown-group/byage3classes/> .
ns13:y16_24	rdf:type	ns10:BreakdownToGroupMembership ;
	rdfs:label	"byage3classes" ;
	ns11:member-of	ns12:byage3classes ;
	ns11:order	"3" .
ns13:y25_54	rdf:type	ns10:BreakdownToGroupMembership ;
	rdfs:label	"byage3classes" ;
	ns11:member-of	ns12:byage3classes ;
	ns11:order	"4" .
ns13:y55_74	rdf:type	ns10:BreakdownToGroupMembership ;
	rdfs:label	"byage3classes" ;
	ns11:member-of	ns12:byage3classes ;
	ns11:order	"5" .
@prefix ns14:	<http://semantic.digital-agenda-data.eu/codelist/breakdown-group/byage6classes/> .
ns14:y16_24	rdf:type	ns10:BreakdownToGroupMembership ;
	rdfs:label	"byage6classes" ;
	ns11:member-of	ns12:byage6classes ;
	ns11:order	"3" .
ns14:y25_34	rdf:type	ns10:BreakdownToGroupMembership ;
	rdfs:label	"byage6classes" ;
	ns11:member-of	ns12:byage6classes ;
	ns11:order	"16" .
ns14:y35_44	rdf:type	ns10:BreakdownToGroupMembership ;
	rdfs:label	"byage6classes" ;
	ns11:member-of	ns12:byage6classes ;
	ns11:order	"17" .
ns14:y45_54	rdf:type	ns10:BreakdownToGroupMembership ;
	rdfs:label	"byage6classes" ;
	ns11:member-of	ns12:byage6classes ;
	ns11:order	"18" .
ns14:y55_64	rdf:type	ns10:BreakdownToGroupMembership ;
	rdfs:label	"byage6classes" ;
	ns11:member-of	ns12:byage6classes ;
	ns11:order	"19" .
ns14:y65_74	rdf:type	ns10:BreakdownToGroupMembership ;
	rdfs:label	"byage6classes" ;
	ns11:member-of	ns12:byage6classes ;
	ns11:order	"20" .
@prefix ns15:	<http://semantic.digital-agenda-data.eu/codelist/breakdown-group/bycbirth/> .
ns15:cb_eu_for	rdf:type	ns10:BreakdownToGroupMembership ;
	rdfs:label	"bycbirth" ;
	ns11:member-of	ns12:bycbirth ;
	ns11:order	"27" .
ns15:cb_ext_eu	rdf:type	ns10:BreakdownToGroupMembership ;
	rdfs:label	"bycbirth" ;
	ns11:member-of	ns12:bycbirth ;
	ns11:order	"28" .
ns15:cb_nat	rdf:type	ns10:BreakdownToGroupMembership ;
	rdfs:label	"bycbirth" ;
	ns11:member-of	ns12:bycbirth ;
	ns11:order	"26" .
@prefix ns16:	<http://semantic.digital-agenda-data.eu/codelist/breakdown-group/byccitizen/> .
ns16:cc_eu_for	rdf:type	ns10:BreakdownToGroupMembership ;
	rdfs:label	"byccitizen" ;
	ns11:member-of	ns12:byccitizen ;
	ns11:order	"30" .
ns16:cc_ext_eu	rdf:type	ns10:BreakdownToGroupMembership ;
	rdfs:label	"byccitizen" ;
	ns11:member-of	ns12:byccitizen ;
	ns11:order	"31" .
ns16:cc_nat	rdf:type	ns10:BreakdownToGroupMembership ;
	rdfs:label	"byccitizen" ;
	ns11:member-of	ns12:byccitizen ;
	ns11:order	"29" .
@prefix ns17:	<http://semantic.digital-agenda-data.eu/codelist/breakdown-group/byccsophistication/> .
ns17:e_cc_hi	rdf:type	ns10:BreakdownToGroupMembership ;
	rdfs:label	"byccsophistication" ;
	ns11:member-of	ns12:byccsophistication ;
	ns11:order	"1" .
ns17:e_cc_lo	rdf:type	ns10:BreakdownToGroupMembership ;
	rdfs:label	"byccsophistication" ;
	ns11:member-of	ns12:byccsophistication ;
	ns11:order	"3" .
ns17:e_cc_me	rdf:type	ns10:BreakdownToGroupMembership ;
	rdfs:label	"byccsophistication" ;
	ns11:member-of	ns12:byccsophistication ;
	ns11:order	"2" .
@prefix ns18:	<http://semantic.digital-agenda-data.eu/codelist/breakdown-group/bydensity/> .
ns18:hh_deg1	rdf:type	ns10:BreakdownToGroupMembership ;
	rdfs:label	"bydensity" ;
	ns11:member-of	ns12:bydensity ;
	ns11:order	"48" .
ns18:hh_deg2	rdf:type	ns10:BreakdownToGroupMembership ;
	rdfs:label	"bydensity" ;
	ns11:member-of	ns12:bydensity ;
	ns11:order	"49" .
ns18:hh_deg3	rdf:type	ns10:BreakdownToGroupMembership ;
	rdfs:label	"bydensity" ;
	ns11:member-of	ns12:bydensity ;
	ns11:order	"50" .
ns18:ind_deg1	rdf:type	ns10:BreakdownToGroupMembership ;
	rdfs:label	"bydensity" ;
	ns11:member-of	ns12:bydensity ;
	ns11:order	"21" .
ns18:ind_deg2	rdf:type	ns10:BreakdownToGroupMembership ;
	rdfs:label	"bydensity" ;
	ns11:member-of	ns12:bydensity ;
	ns11:order	"22" .
ns18:ind_deg3	rdf:type	ns10:BreakdownToGroupMembership ;
	rdfs:label	"bydensity" ;
	ns11:member-of	ns12:bydensity ;
	ns11:order	"23" .
@prefix ns19:	<http://semantic.digital-agenda-data.eu/codelist/breakdown-group/bydigint2015/> .
ns19:e_di_hi	rdf:type	ns10:BreakdownToGroupMembership ;
	rdfs:label	"bydigint2015" ;
	ns11:member-of	ns12:bydigint2015 ;
	ns11:order	"3" .
ns19:e_di_lo	rdf:type	ns10:BreakdownToGroupMembership ;
	rdfs:label	"bydigint2015" ;
	ns11:member-of	ns12:bydigint2015 ;
	ns11:order	"2" .
ns19:e_di_vhi	rdf:type	ns10:BreakdownToGroupMembership ;
	rdfs:label	"bydigint2015" ;
	ns11:member-of	ns12:bydigint2015 ;
	ns11:order	"4" .
ns19:e_di_vlo	rdf:type	ns10:BreakdownToGroupMembership ;
	rdfs:label	"bydigint2015" ;
	ns11:member-of	ns12:bydigint2015 ;
	ns11:order	"1" .
@prefix ns20:	<http://semantic.digital-agenda-data.eu/codelist/breakdown-group/bydownloadspeed/> .
ns20:offer_30_mbps	rdf:type	ns10:BreakdownToGroupMembership ;
	rdfs:label	"bydownloadspeed" ;
	ns11:member-of	ns12:bydownloadspeed ;
	ns11:order	"56" .
ns20:speed_10l30	rdf:type	ns10:BreakdownToGroupMembership ;
	rdfs:label	"bydownloadspeed" ;
	ns11:member-of	ns12:bydownloadspeed ;
	ns11:order	"3" .
ns20:speed_2l10	rdf:type	ns10:BreakdownToGroupMembership ;
	rdfs:label	"bydownloadspeed" ;
	ns11:member-of	ns12:bydownloadspeed ;
	ns11:order	"2" .
ns20:speed_30l100	rdf:type	ns10:BreakdownToGroupMembership ;
	rdfs:label	"bydownloadspeed" ;
	ns11:member-of	ns12:bydownloadspeed ;
	ns11:order	"4" .
ns20:speed_ge100	rdf:type	ns10:BreakdownToGroupMembership ;
	rdfs:label	"bydownloadspeed" ;
	ns11:member-of	ns12:bydownloadspeed ;
	ns11:order	"5" .
ns20:speed_l2	rdf:type	ns10:BreakdownToGroupMembership ;
	rdfs:label	"bydownloadspeed" ;
	ns11:member-of	ns12:bydownloadspeed ;
	ns11:order	"1" .
@prefix ns21:	<http://semantic.digital-agenda-data.eu/codelist/breakdown-group/bydownloadspeed4/> .
ns21:offer_100_mbps	rdf:type	ns10:BreakdownToGroupMembership ;
	rdfs:label	"bydownloadspeed4" ;
	ns11:member-of	ns12:bydownloadspeed4 ;
	ns11:order	"4" .
ns21:offer_12_30_mbps	rdf:type	ns10:BreakdownToGroupMembership ;
	rdfs:label	"bydownloadspeed4" ;
	ns11:member-of	ns12:bydownloadspeed4 ;
	ns11:order	"2" .
ns21:offer_30_100_mbps	rdf:type	ns10:BreakdownToGroupMembership ;
	rdfs:label	"bydownloadspeed4" ;
	ns11:member-of	ns12:bydownloadspeed4 ;
	ns11:order	"3" .
ns21:offer_8_12_mbps	rdf:type	ns10:BreakdownToGroupMembership ;
	rdfs:label	"bydownloadspeed4" ;
	ns11:member-of	ns12:bydownloadspeed4 ;
	ns11:order	"1" .
@prefix ns22:	<http://semantic.digital-agenda-data.eu/codelist/breakdown-group/byedu/> .
ns22:i0_2	rdf:type	ns10:BreakdownToGroupMembership ;
	rdfs:label	"byedu" ;
	ns11:member-of	ns12:byedu ;
	ns11:order	"8" .
ns22:i0_4	rdf:type	ns10:BreakdownToGroupMembership ;
	rdfs:label	"byedu" ;
	ns11:member-of	ns12:byedu ;
	ns11:order	"9" .
ns22:i3_4	rdf:type	ns10:BreakdownToGroupMembership ;
	rdfs:label	"byedu" ;
	ns11:member-of	ns12:byedu ;
	ns11:order	"10" .
ns22:i5_8	rdf:type	ns10:BreakdownToGroupMembership ;
	rdfs:label	"byedu" ;
	ns11:member-of	ns12:byedu ;
	ns11:order	"11" .
@prefix ns23:	<http://semantic.digital-agenda-data.eu/codelist/breakdown-group/byedugrade/> .
ns23:grade11gen	rdf:type	ns10:BreakdownToGroupMembership ;
	rdfs:label	"byedugrade" ;
	ns11:member-of	ns12:byedugrade ;
	ns11:order	"3" .
ns23:grade11voc	rdf:type	ns10:BreakdownToGroupMembership ;
	rdfs:label	"byedugrade" ;
	ns11:member-of	ns12:byedugrade ;
	ns11:order	"4" .
ns23:grade4	rdf:type	ns10:BreakdownToGroupMembership ;
	rdfs:label	"byedugrade" ;
	ns11:member-of	ns12:byedugrade ;
	ns11:order	"1" .
ns23:grade8	rdf:type	ns10:BreakdownToGroupMembership ;
	rdfs:label	"byedugrade" ;
	ns11:member-of	ns12:byedugrade ;
	ns11:order	"2" .
@prefix ns24:	<http://semantic.digital-agenda-data.eu/codelist/breakdown-group/byemp/> .
ns24:retir_other	rdf:type	ns10:BreakdownToGroupMembership ;
	rdfs:label	"byemp" ;
	ns11:member-of	ns12:byemp ;
	ns11:order	"14" .
ns24:sal_self_fam	rdf:type	ns10:BreakdownToGroupMembership ;
	rdfs:label	"byemp" ;
	ns11:member-of	ns12:byemp ;
	ns11:order	"11" .
ns24:stud	rdf:type	ns10:BreakdownToGroupMembership ;
	rdfs:label	"byemp" ;
	ns11:member-of	ns12:byemp ;
	ns11:order	"13" .
ns24:une	rdf:type	ns10:BreakdownToGroupMembership ;
	rdfs:label	"byemp" ;
	ns11:member-of	ns12:byemp ;
	ns11:order	"12" .
@prefix ns25:	<http://semantic.digital-agenda-data.eu/codelist/breakdown-group/byentsize/> .
ns25:ent_l_xfin	rdf:type	ns10:BreakdownToGroupMembership ;
	rdfs:label	"byentsize" ;
	ns11:member-of	ns12:byentsize ;
	ns11:order	"59" .
ns25:ent_sm_xfin	rdf:type	ns10:BreakdownToGroupMembership ;
	rdfs:label	"byentsize" ;
	ns11:member-of	ns12:byentsize ;
	ns11:order	"58" .
ns25:l_c10_s951_xk	rdf:type	ns10:BreakdownToGroupMembership ;
	rdfs:label	"byentsize" ;
	ns11:member-of	ns12:byentsize ;
	ns11:order	"2" .
ns25:sm_c10_s951_xk	rdf:type	ns10:BreakdownToGroupMembership ;
	rdfs:label	"byentsize" ;
	ns11:member-of	ns12:byentsize ;
	ns11:order	"1" .
@prefix ns26:	<http://semantic.digital-agenda-data.eu/codelist/breakdown-group/byentsize_s_m_l/> .
ns26:ent_l_xfin	rdf:type	ns10:BreakdownToGroupMembership ;
	rdfs:label	"byentsize_s_m_l" ;
	ns11:member-of	ns12:byentsize_s_m_l ;
	ns11:order	"62" .
ns26:ent_m_xfin	rdf:type	ns10:BreakdownToGroupMembership ;
	rdfs:label	"byentsize_s_m_l" ;
	ns11:member-of	ns12:byentsize_s_m_l ;
	ns11:order	"61" .
ns26:ent_s_xfin	rdf:type	ns10:BreakdownToGroupMembership ;
	rdfs:label	"byentsize_s_m_l" ;
	ns11:member-of	ns12:byentsize_s_m_l ;
	ns11:order	"60" .
ns26:l_c10_s951_xk	rdf:type	ns10:BreakdownToGroupMembership ;
	rdfs:label	"byentsize_s_m_l" ;
	ns11:member-of	ns12:byentsize_s_m_l ;
	ns11:order	"3" .
ns26:m_c10_s951_xk	rdf:type	ns10:BreakdownToGroupMembership ;
	rdfs:label	"byentsize_s_m_l" ;
	ns11:member-of	ns12:byentsize_s_m_l ;
	ns11:order	"2" .
ns26:s_c10_s951_xk	rdf:type	ns10:BreakdownToGroupMembership ;
	rdfs:label	"byentsize_s_m_l" ;
	ns11:member-of	ns12:byentsize_s_m_l ;
	ns11:order	"1" .
@prefix ns27:	<http://semantic.digital-agenda-data.eu/codelist/breakdown-group/byfbbtech/> .
ns27:cable	rdf:type	ns10:BreakdownToGroupMembership ;
	rdfs:label	"byfbbtech" ;
	ns11:member-of	ns12:byfbbtech ;
	ns11:order	"61" .
ns27:fttx	rdf:type	ns10:BreakdownToGroupMembership ;
	rdfs:label	"byfbbtech" ;
	ns11:member-of	ns12:byfbbtech ;
	ns11:order	"62" .
ns27:xdsl	rdf:type	ns10:BreakdownToGroupMembership ;
	rdfs:label	"byfbbtech" ;
	ns11:member-of	ns12:byfbbtech ;
	ns11:order	"60" .
@prefix ns28:	<http://semantic.digital-agenda-data.eu/codelist/breakdown-group/bygender/> .
ns28:f	rdf:type	ns10:BreakdownToGroupMembership ;
	rdfs:label	"bygender" ;
	ns11:member-of	ns12:bygender ;
	ns11:order	"8" .
ns28:f_y16_74	rdf:type	ns10:BreakdownToGroupMembership ;
	rdfs:label	"bygender" ;
	ns11:member-of	ns12:bygender ;
	ns11:order	"6" .
ns28:m	rdf:type	ns10:BreakdownToGroupMembership ;
	rdfs:label	"bygender" ;
	ns11:member-of	ns12:bygender ;
	ns11:order	"9" .
ns28:m_y16_74	rdf:type	ns10:BreakdownToGroupMembership ;
	rdfs:label	"bygender" ;
	ns11:member-of	ns12:bygender ;
	ns11:order	"7" .
<http://semantic.digital-agenda-data.eu/codelist/breakdown-group/byictsector2subsec/261to264>	rdf:type	ns10:BreakdownToGroupMembership ;
	rdfs:label	"byictsector2subsec" ;
	ns11:member-of	ns12:byictsector2subsec ;
	ns11:order	"1" .
<http://semantic.digital-agenda-data.eu/codelist/breakdown-group/byictsector2subsec/61_582_62_631_951>	rdf:type	ns10:BreakdownToGroupMembership ;
	rdfs:label	"byictsector2subsec" ;
	ns11:member-of	ns12:byictsector2subsec ;
	ns11:order	"2" .
<http://semantic.digital-agenda-data.eu/codelist/breakdown-group/byictsector6subsec/261>	rdf:type	ns10:BreakdownToGroupMembership ;
	rdfs:label	"byictsector6subsec" ;
	ns11:member-of	ns12:byictsector6subsec ;
	ns11:order	"1" .
<http://semantic.digital-agenda-data.eu/codelist/breakdown-group/byictsector6subsec/262>	rdf:type	ns10:BreakdownToGroupMembership ;
	rdfs:label	"byictsector6subsec" ;
	ns11:member-of	ns12:byictsector6subsec ;
	ns11:order	"2" .
<http://semantic.digital-agenda-data.eu/codelist/breakdown-group/byictsector6subsec/263>	rdf:type	ns10:BreakdownToGroupMembership ;
	rdfs:label	"byictsector6subsec" ;
	ns11:member-of	ns12:byictsector6subsec ;
	ns11:order	"3" .
<http://semantic.digital-agenda-data.eu/codelist/breakdown-group/byictsector6subsec/264>	rdf:type	ns10:BreakdownToGroupMembership ;
	rdfs:label	"byictsector6subsec" ;
	ns11:member-of	ns12:byictsector6subsec ;
	ns11:order	"4" .
<http://semantic.digital-agenda-data.eu/codelist/breakdown-group/byictsector6subsec/582_62_631_951>	rdf:type	ns10:BreakdownToGroupMembership ;
	rdfs:label	"byictsector6subsec" ;
	ns11:member-of	ns12:byictsector6subsec ;
	ns11:order	"5" .
<http://semantic.digital-agenda-data.eu/codelist/breakdown-group/byictsector6subsec/61>	rdf:type	ns10:BreakdownToGroupMembership ;
	rdfs:label	"byictsector6subsec" ;
	ns11:member-of	ns12:byictsector6subsec ;
	ns11:order	"6" .
@prefix ns29:	<http://semantic.digital-agenda-data.eu/codelist/breakdown-group/byorganizationclass/> .
ns29:orgclass_hesrec	rdf:type	ns10:BreakdownToGroupMembership ;
	rdfs:label	"byorganizationclass" ;
	ns11:member-of	ns12:byorganizationclass ;
	ns11:order	"66" .
ns29:orgclass_le	rdf:type	ns10:BreakdownToGroupMembership ;
	rdfs:label	"byorganizationclass" ;
	ns11:member-of	ns12:byorganizationclass ;
	ns11:order	"65" .
ns29:orgclass_nil	rdf:type	ns10:BreakdownToGroupMembership ;
	rdfs:label	"byorganizationclass" ;
	ns11:member-of	ns12:byorganizationclass ;
	ns11:order	"67" .
ns29:orgclass_sme	rdf:type	ns10:BreakdownToGroupMembership ;
	rdfs:label	"byorganizationclass" ;
	ns11:member-of	ns12:byorganizationclass ;
	ns11:order	"64" .
@prefix ns30:	<http://semantic.digital-agenda-data.eu/codelist/breakdown-group/byregion/> .
ns30:hh_no1	rdf:type	ns10:BreakdownToGroupMembership ;
	rdfs:label	"byregion" ;
	ns11:member-of	ns12:byregion ;
	ns11:order	"52" .
ns30:hh_o1	rdf:type	ns10:BreakdownToGroupMembership ;
	rdfs:label	"byregion" ;
	ns11:member-of	ns12:byregion ;
	ns11:order	"51" .
ns30:ind_no1	rdf:type	ns10:BreakdownToGroupMembership ;
	rdfs:label	"byregion" ;
	ns11:member-of	ns12:byregion ;
	ns11:order	"25" .
ns30:ind_o1	rdf:type	ns10:BreakdownToGroupMembership ;
	rdfs:label	"byregion" ;
	ns11:member-of	ns12:byregion ;
	ns11:order	"24" .
@prefix ns31:	<http://semantic.digital-agenda-data.eu/codelist/breakdown-group/byrisk/> .
ns31:rf_0	rdf:type	ns10:BreakdownToGroupMembership ;
	rdfs:label	"byrisk" ;
	ns11:member-of	ns12:byrisk ;
	ns11:order	"32" .
ns31:rf_ge1	rdf:type	ns10:BreakdownToGroupMembership ;
	rdfs:label	"byrisk" ;
	ns11:member-of	ns12:byrisk ;
	ns11:order	"33" .
ns31:rf_ge2	rdf:type	ns10:BreakdownToGroupMembership ;
	rdfs:label	"byrisk" ;
	ns11:member-of	ns12:byrisk ;
	ns11:order	"34" .
@prefix ns32:	<http://semantic.digital-agenda-data.eu/codelist/breakdown-group/byskills/> .
ns32:csk_hi	rdf:type	ns10:BreakdownToGroupMembership ;
	rdfs:label	"byskills" ;
	ns11:member-of	ns12:byskills ;
	ns11:order	"35" .
ns32:csk_lo	rdf:type	ns10:BreakdownToGroupMembership ;
	rdfs:label	"byskills" ;
	ns11:member-of	ns12:byskills ;
	ns11:order	"37" .
ns32:csk_me	rdf:type	ns10:BreakdownToGroupMembership ;
	rdfs:label	"byskills" ;
	ns11:member-of	ns12:byskills ;
	ns11:order	"36" .
ns32:cskx	rdf:type	ns10:BreakdownToGroupMembership ;
	rdfs:label	"byskills" ;
	ns11:member-of	ns12:byskills ;
	ns11:order	"38" .
@prefix ns33:	<http://semantic.digital-agenda-data.eu/codelist/breakdown-group/bytypeproduct/> .
ns33:goods	rdf:type	ns10:BreakdownToGroupMembership ;
	rdfs:label	"bytypeproduct" ;
	ns11:member-of	ns12:bytypeproduct ;
	ns11:order	"1" .
ns33:services	rdf:type	ns10:BreakdownToGroupMembership ;
	rdfs:label	"bytypeproduct" ;
	ns11:member-of	ns12:bytypeproduct ;
	ns11:order	"2" .
@prefix ns34:	<http://semantic.digital-agenda-data.eu/codelist/breakdown-group/cnect_directorates/> .
ns34:cnect_a	rdf:type	ns10:BreakdownToGroupMembership ;
	rdfs:label	"cnect_directorates" ;
	ns11:member-of	ns12:cnect_directorates ;
	ns11:order	"12" .
ns34:cnect_all	rdf:type	ns10:BreakdownToGroupMembership ;
	rdfs:label	"cnect_directorates" ;
	ns11:member-of	ns12:cnect_directorates ;
	ns11:order	"11" .
<http://semantic.digital-agenda-data.eu/codelist/breakdown-group/cnect_directorates/cnect_b+>	rdf:type	ns10:BreakdownToGroupMembership ;
	rdfs:label	"cnect_directorates" ;
	ns11:member-of	ns12:cnect_directorates ;
	ns11:order	"13" .
ns34:cnect_c	rdf:type	ns10:BreakdownToGroupMembership ;
	rdfs:label	"cnect_directorates" ;
	ns11:member-of	ns12:cnect_directorates ;
	ns11:order	"14" .
ns34:cnect_d	rdf:type	ns10:BreakdownToGroupMembership ;
	rdfs:label	"cnect_directorates" ;
	ns11:member-of	ns12:cnect_directorates ;
	ns11:order	"15" .
ns34:cnect_e	rdf:type	ns10:BreakdownToGroupMembership ;
	rdfs:label	"cnect_directorates" ;
	ns11:member-of	ns12:cnect_directorates ;
	ns11:order	"16" .
ns34:cnect_f	rdf:type	ns10:BreakdownToGroupMembership ;
	rdfs:label	"cnect_directorates" ;
	ns11:member-of	ns12:cnect_directorates ;
	ns11:order	"17" .
ns34:cnect_g	rdf:type	ns10:BreakdownToGroupMembership ;
	rdfs:label	"cnect_directorates" ;
	ns11:member-of	ns12:cnect_directorates ;
	ns11:order	"18" .
ns34:cnect_h	rdf:type	ns10:BreakdownToGroupMembership ;
	rdfs:label	"cnect_directorates" ;
	ns11:member-of	ns12:cnect_directorates ;
	ns11:order	"19" .
ns34:cnect_r	rdf:type	ns10:BreakdownToGroupMembership ;
	rdfs:label	"cnect_directorates" ;
	ns11:member-of	ns12:cnect_directorates ;
	ns11:order	"20" .
ns34:ec_all	rdf:type	ns10:BreakdownToGroupMembership ;
	rdfs:label	"cnect_directorates" ;
	ns11:member-of	ns12:cnect_directorates ;
	ns11:order	"22" .
@prefix ns35:	<http://semantic.digital-agenda-data.eu/codelist/breakdown-group/desi/> .
ns35:desi_1_conn	rdf:type	ns10:BreakdownToGroupMembership ;
	rdfs:label	"desi" ;
	ns11:member-of	ns12:desi ;
	ns11:order	"1" .
ns35:desi_2_hc	rdf:type	ns10:BreakdownToGroupMembership ;
	rdfs:label	"desi" ;
	ns11:member-of	ns12:desi ;
	ns11:order	"2" .
ns35:desi_3_ui	rdf:type	ns10:BreakdownToGroupMembership ;
	rdfs:label	"desi" ;
	ns11:member-of	ns12:desi ;
	ns11:order	"3" .
ns35:desi_4_idt	rdf:type	ns10:BreakdownToGroupMembership ;
	rdfs:label	"desi" ;
	ns11:member-of	ns12:desi ;
	ns11:order	"4" .
ns35:desi_5_dps	rdf:type	ns10:BreakdownToGroupMembership ;
	rdfs:label	"desi" ;
	ns11:member-of	ns12:desi ;
	ns11:order	"5" .
@prefix ns36:	<http://semantic.digital-agenda-data.eu/codelist/breakdown-group/desi_1_conn/> .
ns36:desi_1a_fbb	rdf:type	ns10:BreakdownToGroupMembership ;
	rdfs:label	"desi_1_conn" ;
	ns11:member-of	ns12:desi_1_conn ;
	ns11:order	"2" .
ns36:desi_1b_mbb	rdf:type	ns10:BreakdownToGroupMembership ;
	rdfs:label	"desi_1_conn" ;
	ns11:member-of	ns12:desi_1_conn ;
	ns11:order	"3" .
ns36:desi_1c_speed	rdf:type	ns10:BreakdownToGroupMembership ;
	rdfs:label	"desi_1_conn" ;
	ns11:member-of	ns12:desi_1_conn ;
	ns11:order	"4" .
ns36:desi_1d_aff	rdf:type	ns10:BreakdownToGroupMembership ;
	rdfs:label	"desi_1_conn" ;
	ns11:member-of	ns12:desi_1_conn ;
	ns11:order	"5" .
@prefix ns37:	<http://semantic.digital-agenda-data.eu/codelist/breakdown-group/desi_1a_fbb/> .
ns37:desi_1a1_fbbc	rdf:type	ns10:BreakdownToGroupMembership ;
	rdfs:label	"desi_1a_fbb" ;
	ns11:member-of	ns12:desi_1a_fbb ;
	ns11:order	"1" .
ns37:desi_1a2_fbbtu	rdf:type	ns10:BreakdownToGroupMembership ;
	rdfs:label	"desi_1a_fbb" ;
	ns11:member-of	ns12:desi_1a_fbb ;
	ns11:order	"2" .
@prefix ns38:	<http://semantic.digital-agenda-data.eu/codelist/breakdown-group/desi_1b_mbb/> .
ns38:desi_1b1_mbbtu	rdf:type	ns10:BreakdownToGroupMembership ;
	rdfs:label	"desi_1b_mbb" ;
	ns11:member-of	ns12:desi_1b_mbb ;
	ns11:order	"1" .
ns38:desi_1b2_4g	rdf:type	ns10:BreakdownToGroupMembership ;
	rdfs:label	"desi_1b_mbb" ;
	ns11:member-of	ns12:desi_1b_mbb ;
	ns11:order	"2" .
ns38:desi_1b3_spec	rdf:type	ns10:BreakdownToGroupMembership ;
	rdfs:label	"desi_1b_mbb" ;
	ns11:member-of	ns12:desi_1b_mbb ;
	ns11:order	"3" .
@prefix ns39:	<http://semantic.digital-agenda-data.eu/codelist/breakdown-group/desi_1c_speed/> .
ns39:desi_1c1_ngac	rdf:type	ns10:BreakdownToGroupMembership ;
	rdfs:label	"desi_1c_speed" ;
	ns11:member-of	ns12:desi_1c_speed ;
	ns11:order	"1" .
ns39:desi_1c2_sfbb	rdf:type	ns10:BreakdownToGroupMembership ;
	rdfs:label	"desi_1c_speed" ;
	ns11:member-of	ns12:desi_1c_speed ;
	ns11:order	"2" .
@prefix ns40:	<http://semantic.digital-agenda-data.eu/codelist/breakdown-group/desi_1d_aff/> .
ns40:desi_1d1_fbbp	rdf:type	ns10:BreakdownToGroupMembership ;
	rdfs:label	"desi_1d_aff" ;
	ns11:member-of	ns12:desi_1d_aff ;
	ns11:order	"1" .
@prefix ns41:	<http://semantic.digital-agenda-data.eu/codelist/breakdown-group/desi_2_hc/> .
ns41:desi_2a_bsu	rdf:type	ns10:BreakdownToGroupMembership ;
	rdfs:label	"desi_2_hc" ;
	ns11:member-of	ns12:desi_2_hc ;
	ns11:order	"1" .
ns41:desi_2b_asd	rdf:type	ns10:BreakdownToGroupMembership ;
	rdfs:label	"desi_2_hc" ;
	ns11:member-of	ns12:desi_2_hc ;
	ns11:order	"2" .
@prefix ns42:	<http://semantic.digital-agenda-data.eu/codelist/breakdown-group/desi_2a_bsu/> .
ns42:desi_2a1_iu	rdf:type	ns10:BreakdownToGroupMembership ;
	rdfs:label	"desi_2a_bsu" ;
	ns11:member-of	ns12:desi_2a_bsu ;
	ns11:order	"1" .
ns42:desi_2a2_bds	rdf:type	ns10:BreakdownToGroupMembership ;
	rdfs:label	"desi_2a_bsu" ;
	ns11:member-of	ns12:desi_2a_bsu ;
	ns11:order	"2" .
@prefix ns43:	<http://semantic.digital-agenda-data.eu/codelist/breakdown-group/desi_2b_asd/> .
ns43:desi_2b1_ictspec	rdf:type	ns10:BreakdownToGroupMembership ;
	rdfs:label	"desi_2b_asd" ;
	ns11:member-of	ns12:desi_2b_asd ;
	ns11:order	"1" .
ns43:desi_2b2_stemg	rdf:type	ns10:BreakdownToGroupMembership ;
	rdfs:label	"desi_2b_asd" ;
	ns11:member-of	ns12:desi_2b_asd ;
	ns11:order	"2" .
@prefix ns44:	<http://semantic.digital-agenda-data.eu/codelist/breakdown-group/desi_3_ui/> .
ns44:desi_3a_cont	rdf:type	ns10:BreakdownToGroupMembership ;
	rdfs:label	"desi_3_ui" ;
	ns11:member-of	ns12:desi_3_ui ;
	ns11:order	"1" .
ns44:desi_3b_comm	rdf:type	ns10:BreakdownToGroupMembership ;
	rdfs:label	"desi_3_ui" ;
	ns11:member-of	ns12:desi_3_ui ;
	ns11:order	"2" .
ns44:desi_3c_trans	rdf:type	ns10:BreakdownToGroupMembership ;
	rdfs:label	"desi_3_ui" ;
	ns11:member-of	ns12:desi_3_ui ;
	ns11:order	"3" .
@prefix ns45:	<http://semantic.digital-agenda-data.eu/codelist/breakdown-group/desi_3a_cont/> .
ns45:desi_3a1_news	rdf:type	ns10:BreakdownToGroupMembership ;
	rdfs:label	"desi_3a_cont" ;
	ns11:member-of	ns12:desi_3a_cont ;
	ns11:order	"1" .
ns45:desi_3a2_mvg	rdf:type	ns10:BreakdownToGroupMembership ;
	rdfs:label	"desi_3a_cont" ;
	ns11:member-of	ns12:desi_3a_cont ;
	ns11:order	"2" .
ns45:desi_3a3_vod	rdf:type	ns10:BreakdownToGroupMembership ;
	rdfs:label	"desi_3a_cont" ;
	ns11:member-of	ns12:desi_3a_cont ;
	ns11:order	"3" .
ns45:desi_3a4_iptv	rdf:type	ns10:BreakdownToGroupMembership ;
	rdfs:label	"desi_3a_cont" ;
	ns11:member-of	ns12:desi_3a_cont ;
	ns11:order	"4" .
@prefix ns46:	<http://semantic.digital-agenda-data.eu/codelist/breakdown-group/desi_3b_comm/> .
ns46:desi_3b1_vidcall	rdf:type	ns10:BreakdownToGroupMembership ;
	rdfs:label	"desi_3b_comm" ;
	ns11:member-of	ns12:desi_3b_comm ;
	ns11:order	"1" .
ns46:desi_3b2_socnet	rdf:type	ns10:BreakdownToGroupMembership ;
	rdfs:label	"desi_3b_comm" ;
	ns11:member-of	ns12:desi_3b_comm ;
	ns11:order	"2" .
@prefix ns47:	<http://semantic.digital-agenda-data.eu/codelist/breakdown-group/desi_3c_trans/> .
ns47:desi_3c1_bank	rdf:type	ns10:BreakdownToGroupMembership ;
	rdfs:label	"desi_3c_trans" ;
	ns11:member-of	ns12:desi_3c_trans ;
	ns11:order	"1" .
ns47:desi_3c2_shop	rdf:type	ns10:BreakdownToGroupMembership ;
	rdfs:label	"desi_3c_trans" ;
	ns11:member-of	ns12:desi_3c_trans ;
	ns11:order	"2" .
@prefix ns48:	<http://semantic.digital-agenda-data.eu/codelist/breakdown-group/desi_4_idt/> .
ns48:desi_4a_bd	rdf:type	ns10:BreakdownToGroupMembership ;
	rdfs:label	"desi_4_idt" ;
	ns11:member-of	ns12:desi_4_idt ;
	ns11:order	"1" .
ns48:desi_4b_ecomm	rdf:type	ns10:BreakdownToGroupMembership ;
	rdfs:label	"desi_4_idt" ;
	ns11:member-of	ns12:desi_4_idt ;
	ns11:order	"2" .
@prefix ns49:	<http://semantic.digital-agenda-data.eu/codelist/breakdown-group/desi_4a_bd/> .
ns49:desi_4a1_eis	rdf:type	ns10:BreakdownToGroupMembership ;
	rdfs:label	"desi_4a_bd" ;
	ns11:member-of	ns12:desi_4a_bd ;
	ns11:order	"1" .
ns49:desi_4a2_rfid	rdf:type	ns10:BreakdownToGroupMembership ;
	rdfs:label	"desi_4a_bd" ;
	ns11:member-of	ns12:desi_4a_bd ;
	ns11:order	"2" .
ns49:desi_4a3_socmed	rdf:type	ns10:BreakdownToGroupMembership ;
	rdfs:label	"desi_4a_bd" ;
	ns11:member-of	ns12:desi_4a_bd ;
	ns11:order	"3" .
ns49:desi_4a4_einv	rdf:type	ns10:BreakdownToGroupMembership ;
	rdfs:label	"desi_4a_bd" ;
	ns11:member-of	ns12:desi_4a_bd ;
	ns11:order	"4" .
ns49:desi_4a5_cloud	rdf:type	ns10:BreakdownToGroupMembership ;
	rdfs:label	"desi_4a_bd" ;
	ns11:member-of	ns12:desi_4a_bd ;
	ns11:order	"5" .
@prefix ns50:	<http://semantic.digital-agenda-data.eu/codelist/breakdown-group/desi_4b_ecomm/> .
ns50:desi_4b1_smeso	rdf:type	ns10:BreakdownToGroupMembership ;
	rdfs:label	"desi_4b_ecomm" ;
	ns11:member-of	ns12:desi_4b_ecomm ;
	ns11:order	"1" .
ns50:desi_4b2_ecomturn	rdf:type	ns10:BreakdownToGroupMembership ;
	rdfs:label	"desi_4b_ecomm" ;
	ns11:member-of	ns12:desi_4b_ecomm ;
	ns11:order	"2" .
ns50:desi_4b3_sellcb	rdf:type	ns10:BreakdownToGroupMembership ;
	rdfs:label	"desi_4b_ecomm" ;
	ns11:member-of	ns12:desi_4b_ecomm ;
	ns11:order	"3" .
@prefix ns51:	<http://semantic.digital-agenda-data.eu/codelist/breakdown-group/desi_5_dps/> .
ns51:desi_5a_egov	rdf:type	ns10:BreakdownToGroupMembership ;
	rdfs:label	"desi_5_dps" ;
	ns11:member-of	ns12:desi_5_dps ;
	ns11:order	"1" .
ns51:desi_5b_ehealth	rdf:type	ns10:BreakdownToGroupMembership ;
	rdfs:label	"desi_5_dps" ;
	ns11:member-of	ns12:desi_5_dps ;
	ns11:order	"2" .
@prefix ns52:	<http://semantic.digital-agenda-data.eu/codelist/breakdown-group/desi_5a_egov/> .
ns52:desi_5a1_egovu	rdf:type	ns10:BreakdownToGroupMembership ;
	rdfs:label	"desi_5a_egov" ;
	ns11:member-of	ns12:desi_5a_egov ;
	ns11:order	"1" .
ns52:desi_5a2_prefform	rdf:type	ns10:BreakdownToGroupMembership ;
	rdfs:label	"desi_5a_egov" ;
	ns11:member-of	ns12:desi_5a_egov ;
	ns11:order	"2" .
ns52:desi_5a3_osercomp	rdf:type	ns10:BreakdownToGroupMembership ;
	rdfs:label	"desi_5a_egov" ;
	ns11:member-of	ns12:desi_5a_egov ;
	ns11:order	"3" .
ns52:desi_5a4_opendata	rdf:type	ns10:BreakdownToGroupMembership ;
	rdfs:label	"desi_5a_egov" ;
	ns11:member-of	ns12:desi_5a_egov ;
	ns11:order	"4" .
@prefix ns53:	<http://semantic.digital-agenda-data.eu/codelist/breakdown-group/desi_5b_ehealth/> .
ns53:desi_5b1_mdataexch	rdf:type	ns10:BreakdownToGroupMembership ;
	rdfs:label	"desi_5b_ehealth" ;
	ns11:member-of	ns12:desi_5b_ehealth ;
	ns11:order	"1" .
ns53:desi_5b2_epresc	rdf:type	ns10:BreakdownToGroupMembership ;
	rdfs:label	"desi_5b_ehealth" ;
	ns11:member-of	ns12:desi_5b_ehealth ;
	ns11:order	"2" .
@prefix ns54:	<http://semantic.digital-agenda-data.eu/codelist/breakdown-group/desi_totals/> .
ns54:desi_total	rdf:type	ns10:BreakdownToGroupMembership ;
	rdfs:label	"desi_totals" ;
	ns11:member-of	ns12:desi_totals ;
	ns11:order	"1" .
@prefix ns55:	<http://semantic.digital-agenda-data.eu/codelist/breakdown-group/digskill_level/> .
ns55:ds_a_basic	rdf:type	ns10:BreakdownToGroupMembership ;
	rdfs:label	"digskill_level" ;
	ns11:member-of	ns12:digskill_level ;
	ns11:order	"1" .
ns55:ds_b_basic	rdf:type	ns10:BreakdownToGroupMembership ;
	rdfs:label	"digskill_level" ;
	ns11:member-of	ns12:digskill_level ;
	ns11:order	"3" .
ns55:ds_basic	rdf:type	ns10:BreakdownToGroupMembership ;
	rdfs:label	"digskill_level" ;
	ns11:member-of	ns12:digskill_level ;
	ns11:order	"2" .
ns55:ds_no	rdf:type	ns10:BreakdownToGroupMembership ;
	rdfs:label	"digskill_level" ;
	ns11:member-of	ns12:digskill_level ;
	ns11:order	"4" .
ns55:dsk_ab	rdf:type	ns10:BreakdownToGroupMembership ;
	rdfs:label	"digskill_level" ;
	ns11:member-of	ns12:digskill_level ;
	ns11:order	"5" .
ns55:dsk_b	rdf:type	ns10:BreakdownToGroupMembership ;
	rdfs:label	"digskill_level" ;
	ns11:member-of	ns12:digskill_level ;
	ns11:order	"6" .
ns55:dsk_x	rdf:type	ns10:BreakdownToGroupMembership ;
	rdfs:label	"digskill_level" ;
	ns11:member-of	ns12:digskill_level ;
	ns11:order	"7" .
<http://semantic.digital-agenda-data.eu/codelist/breakdown-group/econsector/10_c10_18>	rdf:type	ns10:BreakdownToGroupMembership ;
	rdfs:label	"econsector" ;
	ns11:member-of	ns12:econsector ;
	ns11:order	"1" .
<http://semantic.digital-agenda-data.eu/codelist/breakdown-group/econsector/10_c19_23>	rdf:type	ns10:BreakdownToGroupMembership ;
	rdfs:label	"econsector" ;
	ns11:member-of	ns12:econsector ;
	ns11:order	"2" .
<http://semantic.digital-agenda-data.eu/codelist/breakdown-group/econsector/10_c24_25>	rdf:type	ns10:BreakdownToGroupMembership ;
	rdfs:label	"econsector" ;
	ns11:member-of	ns12:econsector ;
	ns11:order	"3" .
<http://semantic.digital-agenda-data.eu/codelist/breakdown-group/econsector/10_c26_33>	rdf:type	ns10:BreakdownToGroupMembership ;
	rdfs:label	"econsector" ;
	ns11:member-of	ns12:econsector ;
	ns11:order	"4" .
<http://semantic.digital-agenda-data.eu/codelist/breakdown-group/econsector/10_d35_e39>	rdf:type	ns10:BreakdownToGroupMembership ;
	rdfs:label	"econsector" ;
	ns11:member-of	ns12:econsector ;
	ns11:order	"5" .
<http://semantic.digital-agenda-data.eu/codelist/breakdown-group/econsector/10_f41_43>	rdf:type	ns10:BreakdownToGroupMembership ;
	rdfs:label	"econsector" ;
	ns11:member-of	ns12:econsector ;
	ns11:order	"6" .
<http://semantic.digital-agenda-data.eu/codelist/breakdown-group/econsector/10_g45>	rdf:type	ns10:BreakdownToGroupMembership ;
	rdfs:label	"econsector" ;
	ns11:member-of	ns12:econsector ;
	ns11:order	"7" .
<http://semantic.digital-agenda-data.eu/codelist/breakdown-group/econsector/10_g46>	rdf:type	ns10:BreakdownToGroupMembership ;
	rdfs:label	"econsector" ;
	ns11:member-of	ns12:econsector ;
	ns11:order	"8" .
<http://semantic.digital-agenda-data.eu/codelist/breakdown-group/econsector/10_g47>	rdf:type	ns10:BreakdownToGroupMembership ;
	rdfs:label	"econsector" ;
	ns11:member-of	ns12:econsector ;
	ns11:order	"9" .
<http://semantic.digital-agenda-data.eu/codelist/breakdown-group/econsector/10_h49_53>	rdf:type	ns10:BreakdownToGroupMembership ;
	rdfs:label	"econsector" ;
	ns11:member-of	ns12:econsector ;
	ns11:order	"10" .
<http://semantic.digital-agenda-data.eu/codelist/breakdown-group/econsector/10_i55_56>	rdf:type	ns10:BreakdownToGroupMembership ;
	rdfs:label	"econsector" ;
	ns11:member-of	ns12:econsector ;
	ns11:order	"11" .
<http://semantic.digital-agenda-data.eu/codelist/breakdown-group/econsector/10_j58_60>	rdf:type	ns10:BreakdownToGroupMembership ;
	rdfs:label	"econsector" ;
	ns11:member-of	ns12:econsector ;
	ns11:order	"12" .
<http://semantic.digital-agenda-data.eu/codelist/breakdown-group/econsector/10_j61>	rdf:type	ns10:BreakdownToGroupMembership ;
	rdfs:label	"econsector" ;
	ns11:member-of	ns12:econsector ;
	ns11:order	"13" .
<http://semantic.digital-agenda-data.eu/codelist/breakdown-group/econsector/10_j62_63>	rdf:type	ns10:BreakdownToGroupMembership ;
	rdfs:label	"econsector" ;
	ns11:member-of	ns12:econsector ;
	ns11:order	"14" .
<http://semantic.digital-agenda-data.eu/codelist/breakdown-group/econsector/10_l68>	rdf:type	ns10:BreakdownToGroupMembership ;
	rdfs:label	"econsector" ;
	ns11:member-of	ns12:econsector ;
	ns11:order	"15" .
<http://semantic.digital-agenda-data.eu/codelist/breakdown-group/econsector/10_m69_74>	rdf:type	ns10:BreakdownToGroupMembership ;
	rdfs:label	"econsector" ;
	ns11:member-of	ns12:econsector ;
	ns11:order	"16" .
<http://semantic.digital-agenda-data.eu/codelist/breakdown-group/econsector/10_n77_82>	rdf:type	ns10:BreakdownToGroupMembership ;
	rdfs:label	"econsector" ;
	ns11:member-of	ns12:econsector ;
	ns11:order	"17" .
<http://semantic.digital-agenda-data.eu/codelist/breakdown-group/econsector/10_s951>	rdf:type	ns10:BreakdownToGroupMembership ;
	rdfs:label	"econsector" ;
	ns11:member-of	ns12:econsector ;
	ns11:order	"18" .
@prefix ns56:	<http://semantic.digital-agenda-data.eu/codelist/breakdown-group/econsector_size/> .
ns56:l_c10_f43	rdf:type	ns10:BreakdownToGroupMembership ;
	rdfs:label	"econsector_size" ;
	ns11:member-of	ns12:econsector_size ;
	ns11:order	"1" .
ns56:l_g45_s951_xk	rdf:type	ns10:BreakdownToGroupMembership ;
	rdfs:label	"econsector_size" ;
	ns11:member-of	ns12:econsector_size ;
	ns11:order	"2" .
ns56:m_c10_f43	rdf:type	ns10:BreakdownToGroupMembership ;
	rdfs:label	"econsector_size" ;
	ns11:member-of	ns12:econsector_size ;
	ns11:order	"3" .
ns56:m_g45_s951_xk	rdf:type	ns10:BreakdownToGroupMembership ;
	rdfs:label	"econsector_size" ;
	ns11:member-of	ns12:econsector_size ;
	ns11:order	"4" .
ns56:s_c10_f43	rdf:type	ns10:BreakdownToGroupMembership ;
	rdfs:label	"econsector_size" ;
	ns11:member-of	ns12:econsector_size ;
	ns11:order	"5" .
ns56:s_g45_s951_xk	rdf:type	ns10:BreakdownToGroupMembership ;
	rdfs:label	"econsector_size" ;
	ns11:member-of	ns12:econsector_size ;
	ns11:order	"6" .
@prefix ns57:	<http://semantic.digital-agenda-data.eu/codelist/breakdown-group/egov_le/> .
ns57:bus_startup	rdf:type	ns10:BreakdownToGroupMembership ;
	rdfs:label	"egov_le" ;
	ns11:member-of	ns12:egov_le ;
	ns11:order	"2" .
ns57:gen_admin_move	rdf:type	ns10:BreakdownToGroupMembership ;
	rdfs:label	"egov_le" ;
	ns11:member-of	ns12:egov_le ;
	ns11:order	"6" .
ns57:lose_find_job	rdf:type	ns10:BreakdownToGroupMembership ;
	rdfs:label	"egov_le" ;
	ns11:member-of	ns12:egov_le ;
	ns11:order	"3" .
ns57:own_drive_car	rdf:type	ns10:BreakdownToGroupMembership ;
	rdfs:label	"egov_le" ;
	ns11:member-of	ns12:egov_le ;
	ns11:order	"7" .
ns57:reg_bus_op	rdf:type	ns10:BreakdownToGroupMembership ;
	rdfs:label	"egov_le" ;
	ns11:member-of	ns12:egov_le ;
	ns11:order	"5" .
ns57:small_claims	rdf:type	ns10:BreakdownToGroupMembership ;
	rdfs:label	"egov_le" ;
	ns11:member-of	ns12:egov_le ;
	ns11:order	"8" .
ns57:study	rdf:type	ns10:BreakdownToGroupMembership ;
	rdfs:label	"egov_le" ;
	ns11:member-of	ns12:egov_le ;
	ns11:order	"4" .
@prefix ns58:	<http://semantic.digital-agenda-data.eu/codelist/breakdown-group/epsi_dimensions/> .
ns58:epsiscore_events	rdf:type	ns10:BreakdownToGroupMembership ;
	rdfs:label	"epsi_dimensions" ;
	ns11:member-of	ns12:epsi_dimensions ;
	ns11:order	"7" .
ns58:epsiscore_exarrange	rdf:type	ns10:BreakdownToGroupMembership ;
	rdfs:label	"epsi_dimensions" ;
	ns11:member-of	ns12:epsi_dimensions ;
	ns11:order	"5" .
ns58:epsiscore_formats	rdf:type	ns10:BreakdownToGroupMembership ;
	rdfs:label	"epsi_dimensions" ;
	ns11:member-of	ns12:epsi_dimensions ;
	ns11:order	"3" .
ns58:epsiscore_implem	rdf:type	ns10:BreakdownToGroupMembership ;
	rdfs:label	"epsi_dimensions" ;
	ns11:member-of	ns12:epsi_dimensions ;
	ns11:order	"1" .
ns58:epsiscore_localpsi	rdf:type	ns10:BreakdownToGroupMembership ;
	rdfs:label	"epsi_dimensions" ;
	ns11:member-of	ns12:epsi_dimensions ;
	ns11:order	"6" .
ns58:epsiscore_practice	rdf:type	ns10:BreakdownToGroupMembership ;
	rdfs:label	"epsi_dimensions" ;
	ns11:member-of	ns12:epsi_dimensions ;
	ns11:order	"2" .
ns58:epsiscore_pricing	rdf:type	ns10:BreakdownToGroupMembership ;
	rdfs:label	"epsi_dimensions" ;
	ns11:member-of	ns12:epsi_dimensions ;
	ns11:order	"4" .
@prefix ns59:	<http://semantic.digital-agenda-data.eu/codelist/breakdown-group/hhbyiq/> .
ns59:hhi_q1	rdf:type	ns10:BreakdownToGroupMembership ;
	rdfs:label	"hhbyiq" ;
	ns11:member-of	ns12:hhbyiq ;
	ns11:order	"42" .
ns59:hhi_q2	rdf:type	ns10:BreakdownToGroupMembership ;
	rdfs:label	"hhbyiq" ;
	ns11:member-of	ns12:hhbyiq ;
	ns11:order	"43" .
ns59:hhi_q3	rdf:type	ns10:BreakdownToGroupMembership ;
	rdfs:label	"hhbyiq" ;
	ns11:member-of	ns12:hhbyiq ;
	ns11:order	"44" .
ns59:hhi_q4	rdf:type	ns10:BreakdownToGroupMembership ;
	rdfs:label	"hhbyiq" ;
	ns11:member-of	ns12:hhbyiq ;
	ns11:order	"45" .
@prefix ns60:	<http://semantic.digital-agenda-data.eu/codelist/breakdown-group/hhbytype/> .
ns60:all_dch	rdf:type	ns10:BreakdownToGroupMembership ;
	rdfs:label	"hhbytype" ;
	ns11:member-of	ns12:hhbytype ;
	ns11:order	"46" .
ns60:all_ndch	rdf:type	ns10:BreakdownToGroupMembership ;
	rdfs:label	"hhbytype" ;
	ns11:member-of	ns12:hhbytype ;
	ns11:order	"47" .
@prefix ns61:	<http://semantic.digital-agenda-data.eu/codelist/breakdown-group/infso_directorates/> .
ns61:ec_all	rdf:type	ns10:BreakdownToGroupMembership ;
	rdfs:label	"infso_directorates" ;
	ns11:member-of	ns12:infso_directorates ;
	ns11:order	"21" .
ns61:infso_a	rdf:type	ns10:BreakdownToGroupMembership ;
	rdfs:label	"infso_directorates" ;
	ns11:member-of	ns12:infso_directorates ;
	ns11:order	"2" .
ns61:infso_all	rdf:type	ns10:BreakdownToGroupMembership ;
	rdfs:label	"infso_directorates" ;
	ns11:member-of	ns12:infso_directorates ;
	ns11:order	"1" .
ns61:infso_b	rdf:type	ns10:BreakdownToGroupMembership ;
	rdfs:label	"infso_directorates" ;
	ns11:member-of	ns12:infso_directorates ;
	ns11:order	"3" .
ns61:infso_c	rdf:type	ns10:BreakdownToGroupMembership ;
	rdfs:label	"infso_directorates" ;
	ns11:member-of	ns12:infso_directorates ;
	ns11:order	"4" .
ns61:infso_d	rdf:type	ns10:BreakdownToGroupMembership ;
	rdfs:label	"infso_directorates" ;
	ns11:member-of	ns12:infso_directorates ;
	ns11:order	"5" .
ns61:infso_e	rdf:type	ns10:BreakdownToGroupMembership ;
	rdfs:label	"infso_directorates" ;
	ns11:member-of	ns12:infso_directorates ;
	ns11:order	"6" .
ns61:infso_f	rdf:type	ns10:BreakdownToGroupMembership ;
	rdfs:label	"infso_directorates" ;
	ns11:member-of	ns12:infso_directorates ;
	ns11:order	"7" .
ns61:infso_g	rdf:type	ns10:BreakdownToGroupMembership ;
	rdfs:label	"infso_directorates" ;
	ns11:member-of	ns12:infso_directorates ;
	ns11:order	"8" .
ns61:infso_h	rdf:type	ns10:BreakdownToGroupMembership ;
	rdfs:label	"infso_directorates" ;
	ns11:member-of	ns12:infso_directorates ;
	ns11:order	"9" .
ns61:infso_r	rdf:type	ns10:BreakdownToGroupMembership ;
	rdfs:label	"infso_directorates" ;
	ns11:member-of	ns12:infso_directorates ;
	ns11:order	"10" .
@prefix ns62:	<http://semantic.digital-agenda-data.eu/codelist/breakdown-group/labour_force/> .
ns62:empl_une	rdf:type	ns10:BreakdownToGroupMembership ;
	rdfs:label	"labour_force" ;
	ns11:member-of	ns12:labour_force ;
	ns11:order	"1" .
<http://semantic.digital-agenda-data.eu/codelist/breakdown-group/manuf/10_c10_12>	rdf:type	ns10:BreakdownToGroupMembership ;
	rdfs:label	"manuf" ;
	ns11:member-of	ns12:manuf ;
	ns11:order	"1" .
<http://semantic.digital-agenda-data.eu/codelist/breakdown-group/manuf/10_c13_15>	rdf:type	ns10:BreakdownToGroupMembership ;
	rdfs:label	"manuf" ;
	ns11:member-of	ns12:manuf ;
	ns11:order	"2" .
<http://semantic.digital-agenda-data.eu/codelist/breakdown-group/manuf/10_c16_18>	rdf:type	ns10:BreakdownToGroupMembership ;
	rdfs:label	"manuf" ;
	ns11:member-of	ns12:manuf ;
	ns11:order	"3" .
<http://semantic.digital-agenda-data.eu/codelist/breakdown-group/manuf/10_c19_23>	rdf:type	ns10:BreakdownToGroupMembership ;
	rdfs:label	"manuf" ;
	ns11:member-of	ns12:manuf ;
	ns11:order	"4" .
<http://semantic.digital-agenda-data.eu/codelist/breakdown-group/manuf/10_c24_25>	rdf:type	ns10:BreakdownToGroupMembership ;
	rdfs:label	"manuf" ;
	ns11:member-of	ns12:manuf ;
	ns11:order	"5" .
<http://semantic.digital-agenda-data.eu/codelist/breakdown-group/manuf/10_c26>	rdf:type	ns10:BreakdownToGroupMembership ;
	rdfs:label	"manuf" ;
	ns11:member-of	ns12:manuf ;
	ns11:order	"6" .
<http://semantic.digital-agenda-data.eu/codelist/breakdown-group/manuf/10_c27_28>	rdf:type	ns10:BreakdownToGroupMembership ;
	rdfs:label	"manuf" ;
	ns11:member-of	ns12:manuf ;
	ns11:order	"7" .
<http://semantic.digital-agenda-data.eu/codelist/breakdown-group/manuf/10_c29_30>	rdf:type	ns10:BreakdownToGroupMembership ;
	rdfs:label	"manuf" ;
	ns11:member-of	ns12:manuf ;
	ns11:order	"8" .
<http://semantic.digital-agenda-data.eu/codelist/breakdown-group/manuf/10_c31_33>	rdf:type	ns10:BreakdownToGroupMembership ;
	rdfs:label	"manuf" ;
	ns11:member-of	ns12:manuf ;
	ns11:order	"9" .
<http://semantic.digital-agenda-data.eu/codelist/breakdown-group/mhz_bands/1500_mhz>	rdf:type	ns10:BreakdownToGroupMembership ;
	rdfs:label	"mhz_bands" ;
	ns11:member-of	ns12:mhz_bands ;
	ns11:order	"7" .
<http://semantic.digital-agenda-data.eu/codelist/breakdown-group/mhz_bands/1800_mhz>	rdf:type	ns10:BreakdownToGroupMembership ;
	rdfs:label	"mhz_bands" ;
	ns11:member-of	ns12:mhz_bands ;
	ns11:order	"6" .
<http://semantic.digital-agenda-data.eu/codelist/breakdown-group/mhz_bands/2_6_ghz>	rdf:type	ns10:BreakdownToGroupMembership ;
	rdfs:label	"mhz_bands" ;
	ns11:member-of	ns12:mhz_bands ;
	ns11:order	"4" .
<http://semantic.digital-agenda-data.eu/codelist/breakdown-group/mhz_bands/2_ghz_paired>	rdf:type	ns10:BreakdownToGroupMembership ;
	rdfs:label	"mhz_bands" ;
	ns11:member-of	ns12:mhz_bands ;
	ns11:order	"5" .
<http://semantic.digital-agenda-data.eu/codelist/breakdown-group/mhz_bands/3_4_ghz>	rdf:type	ns10:BreakdownToGroupMembership ;
	rdfs:label	"mhz_bands" ;
	ns11:member-of	ns12:mhz_bands ;
	ns11:order	"3" .
<http://semantic.digital-agenda-data.eu/codelist/breakdown-group/mhz_bands/3_6_ghz>	rdf:type	ns10:BreakdownToGroupMembership ;
	rdfs:label	"mhz_bands" ;
	ns11:member-of	ns12:mhz_bands ;
	ns11:order	"2" .
<http://semantic.digital-agenda-data.eu/codelist/breakdown-group/mhz_bands/700_mhz>	rdf:type	ns10:BreakdownToGroupMembership ;
	rdfs:label	"mhz_bands" ;
	ns11:member-of	ns12:mhz_bands ;
	ns11:order	"10" .
<http://semantic.digital-agenda-data.eu/codelist/breakdown-group/mhz_bands/800_mhz>	rdf:type	ns10:BreakdownToGroupMembership ;
	rdfs:label	"mhz_bands" ;
	ns11:member-of	ns12:mhz_bands ;
	ns11:order	"9" .
<http://semantic.digital-agenda-data.eu/codelist/breakdown-group/mhz_bands/900_mhz>	rdf:type	ns10:BreakdownToGroupMembership ;
	rdfs:label	"mhz_bands" ;
	ns11:member-of	ns12:mhz_bands ;
	ns11:order	"8" .
@prefix ns63:	<http://semantic.digital-agenda-data.eu/codelist/breakdown-group/mhz_bands/> .
ns63:not_assigned	rdf:type	ns10:BreakdownToGroupMembership ;
	rdfs:label	"mhz_bands" ;
	ns11:member-of	ns12:mhz_bands ;
	ns11:order	"1" .
@prefix ns64:	<http://semantic.digital-agenda-data.eu/codelist/breakdown-group/others/> .
ns64:y25_64	rdf:type	ns10:BreakdownToGroupMembership ;
	rdfs:label	"others" ;
	ns11:member-of	ns12:others ;
	ns11:order	"91" .
@prefix ns65:	<http://semantic.digital-agenda-data.eu/codelist/breakdown-group/rural_pop/> .
ns65:rural_pop	rdf:type	ns10:BreakdownToGroupMembership ;
	rdfs:label	"rural_pop" ;
	ns11:member-of	ns12:rural_pop ;
	ns11:order	"1" .
@prefix ns66:	<http://semantic.digital-agenda-data.eu/codelist/breakdown-group/sos_agg/> .
ns66:einfra	rdf:type	ns10:BreakdownToGroupMembership ;
	rdfs:label	"sos_agg" ;
	ns11:member-of	ns12:sos_agg ;
	ns11:order	"29" .
ns66:so_01	rdf:type	ns10:BreakdownToGroupMembership ;
	rdfs:label	"sos_agg" ;
	ns11:member-of	ns12:sos_agg ;
	ns11:order	"1" .
ns66:so_02	rdf:type	ns10:BreakdownToGroupMembership ;
	rdfs:label	"sos_agg" ;
	ns11:member-of	ns12:sos_agg ;
	ns11:order	"2" .
ns66:so_03	rdf:type	ns10:BreakdownToGroupMembership ;
	rdfs:label	"sos_agg" ;
	ns11:member-of	ns12:sos_agg ;
	ns11:order	"3" .
ns66:so_04	rdf:type	ns10:BreakdownToGroupMembership ;
	rdfs:label	"sos_agg" ;
	ns11:member-of	ns12:sos_agg ;
	ns11:order	"4" .
ns66:so_05	rdf:type	ns10:BreakdownToGroupMembership ;
	rdfs:label	"sos_agg" ;
	ns11:member-of	ns12:sos_agg ;
	ns11:order	"5" .
ns66:so_06	rdf:type	ns10:BreakdownToGroupMembership ;
	rdfs:label	"sos_agg" ;
	ns11:member-of	ns12:sos_agg ;
	ns11:order	"6" .
ns66:so_07	rdf:type	ns10:BreakdownToGroupMembership ;
	rdfs:label	"sos_agg" ;
	ns11:member-of	ns12:sos_agg ;
	ns11:order	"7" .
ns66:so_08	rdf:type	ns10:BreakdownToGroupMembership ;
	rdfs:label	"sos_agg" ;
	ns11:member-of	ns12:sos_agg ;
	ns11:order	"8" .
ns66:so_09	rdf:type	ns10:BreakdownToGroupMembership ;
	rdfs:label	"sos_agg" ;
	ns11:member-of	ns12:sos_agg ;
	ns11:order	"9" .
ns66:so_10	rdf:type	ns10:BreakdownToGroupMembership ;
	rdfs:label	"sos_agg" ;
	ns11:member-of	ns12:sos_agg ;
	ns11:order	"10" .
ns66:so_11	rdf:type	ns10:BreakdownToGroupMembership ;
	rdfs:label	"sos_agg" ;
	ns11:member-of	ns12:sos_agg ;
	ns11:order	"11" .
ns66:so_12	rdf:type	ns10:BreakdownToGroupMembership ;
	rdfs:label	"sos_agg" ;
	ns11:member-of	ns12:sos_agg ;
	ns11:order	"12" .
ns66:so_13	rdf:type	ns10:BreakdownToGroupMembership ;
	rdfs:label	"sos_agg" ;
	ns11:member-of	ns12:sos_agg ;
	ns11:order	"13" .
ns66:so_14	rdf:type	ns10:BreakdownToGroupMembership ;
	rdfs:label	"sos_agg" ;
	ns11:member-of	ns12:sos_agg ;
	ns11:order	"14" .
ns66:so_15	rdf:type	ns10:BreakdownToGroupMembership ;
	rdfs:label	"sos_agg" ;
	ns11:member-of	ns12:sos_agg ;
	ns11:order	"15" .
ns66:so_16	rdf:type	ns10:BreakdownToGroupMembership ;
	rdfs:label	"sos_agg" ;
	ns11:member-of	ns12:sos_agg ;
	ns11:order	"16" .
ns66:so_17	rdf:type	ns10:BreakdownToGroupMembership ;
	rdfs:label	"sos_agg" ;
	ns11:member-of	ns12:sos_agg ;
	ns11:order	"17" .
ns66:so_18	rdf:type	ns10:BreakdownToGroupMembership ;
	rdfs:label	"sos_agg" ;
	ns11:member-of	ns12:sos_agg ;
	ns11:order	"18" .
ns66:so_19	rdf:type	ns10:BreakdownToGroupMembership ;
	rdfs:label	"sos_agg" ;
	ns11:member-of	ns12:sos_agg ;
	ns11:order	"19" .
ns66:so_20	rdf:type	ns10:BreakdownToGroupMembership ;
	rdfs:label	"sos_agg" ;
	ns11:member-of	ns12:sos_agg ;
	ns11:order	"20" .
ns66:so_21	rdf:type	ns10:BreakdownToGroupMembership ;
	rdfs:label	"sos_agg" ;
	ns11:member-of	ns12:sos_agg ;
	ns11:order	"21" .
ns66:so_22_1	rdf:type	ns10:BreakdownToGroupMembership ;
	rdfs:label	"sos_agg" ;
	ns11:member-of	ns12:sos_agg ;
	ns11:order	"22" .
ns66:so_22_2	rdf:type	ns10:BreakdownToGroupMembership ;
	rdfs:label	"sos_agg" ;
	ns11:member-of	ns12:sos_agg ;
	ns11:order	"23" .
ns66:so_22_3	rdf:type	ns10:BreakdownToGroupMembership ;
	rdfs:label	"sos_agg" ;
	ns11:member-of	ns12:sos_agg ;
	ns11:order	"24" .
ns66:so_23	rdf:type	ns10:BreakdownToGroupMembership ;
	rdfs:label	"sos_agg" ;
	ns11:member-of	ns12:sos_agg ;
	ns11:order	"25" .
ns66:so_24	rdf:type	ns10:BreakdownToGroupMembership ;
	rdfs:label	"sos_agg" ;
	ns11:member-of	ns12:sos_agg ;
	ns11:order	"26" .
ns66:so_25	rdf:type	ns10:BreakdownToGroupMembership ;
	rdfs:label	"sos_agg" ;
	ns11:member-of	ns12:sos_agg ;
	ns11:order	"27" .
ns66:so_26	rdf:type	ns10:BreakdownToGroupMembership ;
	rdfs:label	"sos_agg" ;
	ns11:member-of	ns12:sos_agg ;
	ns11:order	"28" .
ns66:total_sos	rdf:type	ns10:BreakdownToGroupMembership ;
	rdfs:label	"sos_agg" ;
	ns11:member-of	ns12:sos_agg ;
	ns11:order	"30" .
<http://semantic.digital-agenda-data.eu/codelist/breakdown-group/total/1m_websites>	rdf:type	ns10:BreakdownToGroupMembership ;
	rdfs:label	"total" ;
	ns11:member-of	ns12:total ;
	ns11:order	"1" .
<http://semantic.digital-agenda-data.eu/codelist/breakdown-group/total/261to264_582_61_62_631_951>	rdf:type	ns10:BreakdownToGroupMembership ;
	rdfs:label	"total" ;
	ns11:member-of	ns12:total ;
	ns11:order	"1" .
@prefix ns67:	<http://semantic.digital-agenda-data.eu/codelist/breakdown-group/total/> .
ns67:all_egov_le	rdf:type	ns10:BreakdownToGroupMembership ;
	rdfs:label	"total" ;
	ns11:member-of	ns12:total ;
	ns11:order	"1" .
ns67:ent_all_xfin	rdf:type	ns10:BreakdownToGroupMembership ;
	rdfs:label	"total" ;
	ns11:member-of	ns12:total ;
	ns11:order	"57" .
ns67:epsiscore_total	rdf:type	ns10:BreakdownToGroupMembership ;
	rdfs:label	"total" ;
	ns11:member-of	ns12:total ;
	ns11:order	"1" .
ns67:hh_total	rdf:type	ns10:BreakdownToGroupMembership ;
	rdfs:label	"total" ;
	ns11:member-of	ns12:total ;
	ns11:order	"41" .
ns67:ind_total	rdf:type	ns10:BreakdownToGroupMembership ;
	rdfs:label	"total" ;
	ns11:member-of	ns12:total ;
	ns11:order	"2" .
ns67:orgclass_total	rdf:type	ns10:BreakdownToGroupMembership ;
	rdfs:label	"total" ;
	ns11:member-of	ns12:total ;
	ns11:order	"63" .
ns67:tot_ict_products	rdf:type	ns10:BreakdownToGroupMembership ;
	rdfs:label	"total" ;
	ns11:member-of	ns12:total ;
	ns11:order	"1" .
ns67:total	rdf:type	ns10:BreakdownToGroupMembership ;
	rdfs:label	"total" ;
	ns11:member-of	ns12:total ;
	ns11:order	"1" .
ns67:total_fbb	rdf:type	ns10:BreakdownToGroupMembership ;
	rdfs:label	"total" ;
	ns11:member-of	ns12:total ;
	ns11:order	"1" .
ns67:total_mbb	rdf:type	ns10:BreakdownToGroupMembership ;
	rdfs:label	"total" ;
	ns11:member-of	ns12:total ;
	ns11:order	"1" .
ns67:total_mob	rdf:type	ns10:BreakdownToGroupMembership ;
	rdfs:label	"total" ;
	ns11:member-of	ns12:total ;
	ns11:order	"1" .
ns67:total_offers8plus	rdf:type	ns10:BreakdownToGroupMembership ;
	rdfs:label	"total" ;
	ns11:member-of	ns12:total ;
	ns11:order	"53" .
ns67:total_pop	rdf:type	ns10:BreakdownToGroupMembership ;
	rdfs:label	"total" ;
	ns11:member-of	ns12:total ;
	ns11:order	"1" .
ns67:total_pophh	rdf:type	ns10:BreakdownToGroupMembership ;
	rdfs:label	"total" ;
	ns11:member-of	ns12:total ;
	ns11:order	"1" .
ns67:total_tel	rdf:type	ns10:BreakdownToGroupMembership ;
	rdfs:label	"total" ;
	ns11:member-of	ns12:total ;
	ns11:order	"1" .
<http://semantic.digital-agenda-data.eu/codelist/breakdown-group/total_manufacturing/10_c10_33>	rdf:type	ns10:BreakdownToGroupMembership ;
	rdfs:label	"total_manufacturing" ;
	ns11:member-of	ns12:total_manufacturing ;
	ns11:order	"1" .
<http://semantic.digital-agenda-data.eu/codelist/breakdown/10_c10_12>	rdf:type	ns10:Breakdown ,
		skos:Concept ;
	skos:notation	"10_c10_12" ;
	skos:definition	"Nace rev.2 sector c10_12 - Manufacture of beverages, food and tobacco products " ;
	skos:topConceptOf	ns1:breakdown ;
	ns11:membership	<http://semantic.digital-agenda-data.eu/codelist/breakdown-group/manuf/10_c10_12> ;
	skos:altLabel	"Beverages, food and tobacco" ;
	skos:prefLabel	"Beverages, food and tobacco products " .
<http://semantic.digital-agenda-data.eu/codelist/breakdown/10_c10_18>	rdf:type	ns10:Breakdown ,
		skos:Concept ;
	skos:notation	"10_C10_18" ;
	skos:topConceptOf	ns1:breakdown ;
	ns11:membership	<http://semantic.digital-agenda-data.eu/codelist/breakdown-group/econsector/10_c10_18> ;
	skos:altLabel	"Manufacture: food, beverages, tobacco, textile, leather, wood, paper; publishing and printing 10+" ;
	skos:prefLabel	"Manufacture: food, beverages, tobacco, textile, leather, wood, paper; publishing and printing 10+" .
<http://semantic.digital-agenda-data.eu/codelist/breakdown/10_c10_33>	rdf:type	ns10:Breakdown ,
		skos:Concept ;
	skos:notation	"10_c10_33" ;
	skos:definition	"Nace rev.2 c10_33 - Manufacturing " ;
	skos:topConceptOf	ns1:breakdown ;
	ns11:membership	<http://semantic.digital-agenda-data.eu/codelist/breakdown-group/total_manufacturing/10_c10_33> ;
	skos:altLabel	"Manufacturing sector" ;
	skos:prefLabel	"Manufacturing sector" .
<http://semantic.digital-agenda-data.eu/codelist/breakdown/10_c10_s951_xk>	rdf:type	ns10:Breakdown ,
		skos:Concept ;
	skos:notation	"10_C10_S951_XK" ;
	skos:definition	"Eurostat definition of Nace2 codes: 10_C10_S951_XK" ;
	skos:topConceptOf	ns1:breakdown ;
	skos:altLabel	"All enterprises" ;
	skos:prefLabel	"All enterprises, without financial sector (10 persons employed or more)" .
<http://semantic.digital-agenda-data.eu/codelist/breakdown/10_c13_15>	rdf:type	ns10:Breakdown ,
		skos:Concept ;
	skos:notation	"10_c13_15" ;
	skos:definition	"Nace rev.2 c13_15 - Manufacture of textiles, wearing apparel, leather and related products " ;
	skos:topConceptOf	ns1:breakdown ;
	ns11:membership	<http://semantic.digital-agenda-data.eu/codelist/breakdown-group/manuf/10_c13_15> ;
	skos:altLabel	"Textiles, leather, etc" ;
	skos:prefLabel	"Textiles, wearing apparel, leather and related products " .
<http://semantic.digital-agenda-data.eu/codelist/breakdown/10_c16_18>	rdf:type	ns10:Breakdown ,
		skos:Concept ;
	skos:notation	"10_c16_18" ;
	skos:definition	"Nace rev.2 c16_18 - Manufacture of wood & products of wood & cork, except furniture; articles of straw & plaiting materials; paper & paper products; printing & reproduction of recorded media " ;
	skos:topConceptOf	ns1:breakdown ;
	ns11:membership	<http://semantic.digital-agenda-data.eu/codelist/breakdown-group/manuf/10_c16_18> ;
	skos:altLabel	"Wood, Paper, etc" ;
	skos:prefLabel	"Wood & cork, Paper, printing & reproduction of recorded media" .
<http://semantic.digital-agenda-data.eu/codelist/breakdown/10_c19_23>	rdf:type	ns10:Breakdown ,
		skos:Concept ;
	skos:notation	"10_c19_23" ;
	skos:topConceptOf	ns1:breakdown ;
	ns11:membership	<http://semantic.digital-agenda-data.eu/codelist/breakdown-group/manuf/10_c19_23> ,
		<http://semantic.digital-agenda-data.eu/codelist/breakdown-group/econsector/10_c19_23> ;
	skos:altLabel	"Manufacture: coke, petroleum, chemical, plastics, other non-metallic mineral products 10+" ;
	skos:prefLabel	"Manufacture: coke, petroleum, chemical, plastics, other non-metallic mineral products 10+" .
<http://semantic.digital-agenda-data.eu/codelist/breakdown/10_c24_25>	rdf:type	ns10:Breakdown ,
		skos:Concept ;
	skos:notation	"10_C24_25" ;
	skos:topConceptOf	ns1:breakdown ;
	ns11:membership	<http://semantic.digital-agenda-data.eu/codelist/breakdown-group/manuf/10_c24_25> ,
		<http://semantic.digital-agenda-data.eu/codelist/breakdown-group/econsector/10_c24_25> ;
	skos:altLabel	"Manufacture: basic metals & fabricated metal products excluding machines & equipments 10+" ;
	skos:prefLabel	"Manufacture: basic metals & fabricated metal products excluding machines & equipments 10+" .
<http://semantic.digital-agenda-data.eu/codelist/breakdown/10_c26>	rdf:type	ns10:Breakdown ,
		skos:Concept ;
	skos:notation	"10_c26" ;
	skos:definition	"Nace rev.2 c26 - Manufacture of computer, electronic and optical products " ;
	skos:topConceptOf	ns1:breakdown ;
	ns11:membership	<http://semantic.digital-agenda-data.eu/codelist/breakdown-group/manuf/10_c26> ;
	skos:altLabel	"Computer, electronic and optical " ;
	skos:prefLabel	"Computer, electronic and optical products " .
<http://semantic.digital-agenda-data.eu/codelist/breakdown/10_c26_33>	rdf:type	ns10:Breakdown ,
		skos:Concept ;
	skos:notation	"10_C26_33" ;
	skos:topConceptOf	ns1:breakdown ;
	ns11:membership	<http://semantic.digital-agenda-data.eu/codelist/breakdown-group/econsector/10_c26_33> ;
	skos:altLabel	"Manufacture: computers, electric & optical, motor vehicles, transport equipment, furniture, repair 10+" ;
	skos:prefLabel	"Manufacture: computers, electric & optical, motor vehicles, transport equipment, furniture, repair 10+" .
<http://semantic.digital-agenda-data.eu/codelist/breakdown/10_c27_28>	rdf:type	ns10:Breakdown ,
		skos:Concept ;
	skos:notation	"10_c27_28" ;
	skos:definition	"Nace rev.2 c27_28 - Manufacture of electrical equipment, machinery and equipment n.e.c. " ;
	skos:topConceptOf	ns1:breakdown ;
	ns11:membership	<http://semantic.digital-agenda-data.eu/codelist/breakdown-group/manuf/10_c27_28> ;
	skos:altLabel	"Electrical equipment & machinery" ;
	skos:prefLabel	"Electrical equipment, machinery and equipment n.e.c. " .
<http://semantic.digital-agenda-data.eu/codelist/breakdown/10_c29_30>	rdf:type	ns10:Breakdown ,
		skos:Concept ;
	skos:notation	"10_c29_30" ;
	skos:definition	"Nace rev.2 c29_30 - Manufacture of motor vehicles, trailers and semi-trailers, other transport equipment " ;
	skos:topConceptOf	ns1:breakdown ;
	ns11:membership	<http://semantic.digital-agenda-data.eu/codelist/breakdown-group/manuf/10_c29_30> ;
	skos:altLabel	"Motor vehicles & transport equipment " ;
	skos:prefLabel	"Motor vehicles, trailers, other transport equipment " .
<http://semantic.digital-agenda-data.eu/codelist/breakdown/10_c31_33>	rdf:type	ns10:Breakdown ,
		skos:Concept ;
	skos:notation	"10_c31_33" ;
	skos:definition	"Nace rev.2 c31_33 - Manufacture of furniture and other manufacturing; repair and installation of machinery and equipment " ;
	skos:topConceptOf	ns1:breakdown ;
	ns11:membership	<http://semantic.digital-agenda-data.eu/codelist/breakdown-group/manuf/10_c31_33> ;
	skos:altLabel	"Furniture; Repair of machinery" ;
	skos:prefLabel	"Furniture; repair and installation of machinery" .
<http://semantic.digital-agenda-data.eu/codelist/breakdown/10_f41_43>	rdf:type	ns10:Breakdown ,
		skos:Concept ;
	skos:notation	"10_F41_43" ;
	skos:topConceptOf	ns1:breakdown ;
	ns11:membership	<http://semantic.digital-agenda-data.eu/codelist/breakdown-group/econsector/10_f41_43> ;
	skos:altLabel	"Construction 10+" ;
	skos:prefLabel	"Construction 10+" .
<http://semantic.digital-agenda-data.eu/codelist/breakdown/10_g46>	rdf:type	ns10:Breakdown ,
		skos:Concept ;
	skos:notation	"10_G46" ;
	skos:topConceptOf	ns1:breakdown ;
	ns11:membership	<http://semantic.digital-agenda-data.eu/codelist/breakdown-group/econsector/10_g46> ;
	skos:altLabel	"Wholesale trade, except of motor vehicles and motorcycles 10+" ;
	skos:prefLabel	"Wholesale trade, except of motor vehicles and motorcycles 10+" .
<http://semantic.digital-agenda-data.eu/codelist/breakdown/10_g47>	rdf:type	ns10:Breakdown ,
		skos:Concept ;
	skos:notation	"10_G47" ;
	skos:topConceptOf	ns1:breakdown ;
	ns11:membership	<http://semantic.digital-agenda-data.eu/codelist/breakdown-group/econsector/10_g47> ;
	skos:altLabel	"Retail trade, except of motor vehicles and motorcycles 10+" ;
	skos:prefLabel	"Retail trade, except of motor vehicles and motorcycles 10+" .
<http://semantic.digital-agenda-data.eu/codelist/breakdown/10_h49_53>	rdf:type	ns10:Breakdown ,
		skos:Concept ;
	skos:notation	"10_H49_53" ;
	skos:topConceptOf	ns1:breakdown ;
	ns11:membership	<http://semantic.digital-agenda-data.eu/codelist/breakdown-group/econsector/10_h49_53> ;
	skos:altLabel	"Transport and storage 10+" ;
	skos:prefLabel	"Transport and storage 10+" .
<http://semantic.digital-agenda-data.eu/codelist/breakdown/10_i55_56>	rdf:type	ns10:Breakdown ,
		skos:Concept ;
	skos:notation	"10_I55_56" ;
	skos:topConceptOf	ns1:breakdown ;
	ns11:membership	<http://semantic.digital-agenda-data.eu/codelist/breakdown-group/econsector/10_i55_56> ;
	skos:altLabel	"Accommodation and food service activities 10+" ;
	skos:prefLabel	"Accommodation and food service activities 10+" .
<http://semantic.digital-agenda-data.eu/codelist/breakdown/10_j58_60>	rdf:type	ns10:Breakdown ,
		skos:Concept ;
	skos:notation	"10_J58_60" ;
	skos:topConceptOf	ns1:breakdown ;
	ns11:membership	<http://semantic.digital-agenda-data.eu/codelist/breakdown-group/econsector/10_j58_60> ;
	skos:altLabel	"Publishing activities; films & television, sound & music publishing; broadcasting 10+" ;
	skos:prefLabel	"Publishing activities; films & television, sound & music publishing; broadcasting 10+" .
<http://semantic.digital-agenda-data.eu/codelist/breakdown/10_j61>	rdf:type	ns10:Breakdown ,
		skos:Concept ;
	skos:notation	"10_J61" ;
	skos:topConceptOf	ns1:breakdown ;
	ns11:membership	<http://semantic.digital-agenda-data.eu/codelist/breakdown-group/econsector/10_j61> ;
	skos:altLabel	"Telecommunications 10+" ;
	skos:prefLabel	"Telecommunications 10+" .
<http://semantic.digital-agenda-data.eu/codelist/breakdown/10_j62_63>	rdf:type	ns10:Breakdown ,
		skos:Concept ;
	skos:notation	"10_J62_63" ;
	skos:topConceptOf	ns1:breakdown ;
	ns11:membership	<http://semantic.digital-agenda-data.eu/codelist/breakdown-group/econsector/10_j62_63> ;
	skos:altLabel	"Computer programming, consultancy and related activities, information services 10+" ;
	skos:prefLabel	"Computer programming, consultancy and related activities, information services 10+" .
<http://semantic.digital-agenda-data.eu/codelist/breakdown/10_l68>	rdf:type	ns10:Breakdown ,
		skos:Concept ;
	skos:notation	"10_L68" ;
	skos:topConceptOf	ns1:breakdown ;
	ns11:membership	<http://semantic.digital-agenda-data.eu/codelist/breakdown-group/econsector/10_l68> ;
	skos:altLabel	"Real estate activities 10+" ;
	skos:prefLabel	"Real estate activities 10+" .
<http://semantic.digital-agenda-data.eu/codelist/breakdown/10_m69_74>	rdf:type	ns10:Breakdown ,
		skos:Concept ;
	skos:notation	"10_M69_74" ;
	skos:topConceptOf	ns1:breakdown ;
	ns11:membership	<http://semantic.digital-agenda-data.eu/codelist/breakdown-group/econsector/10_m69_74> ;
	skos:altLabel	"Professional, scientific and technical activities 10+" ;
	skos:prefLabel	"Professional, scientific and technical activities 10+" .
<http://semantic.digital-agenda-data.eu/codelist/breakdown/10_n77_82>	rdf:type	ns10:Breakdown ,
		skos:Concept ;
	skos:notation	"10_N77_82" ;
	skos:topConceptOf	ns1:breakdown ;
	ns11:membership	<http://semantic.digital-agenda-data.eu/codelist/breakdown-group/econsector/10_n77_82> ;
	skos:altLabel	"Administrative and support service activities 10+" ;
	skos:prefLabel	"Administrative and support service activities 10+" .
<http://semantic.digital-agenda-data.eu/codelist/breakdown/10_s951>	rdf:type	ns10:Breakdown ,
		skos:Concept ;
	skos:notation	"10_S951" ;
	skos:topConceptOf	ns1:breakdown ;
	ns11:membership	<http://semantic.digital-agenda-data.eu/codelist/breakdown-group/econsector/10_s951> ;
	skos:altLabel	"Repair of computers and communication equipment" ;
	skos:prefLabel	"Repair of computers and communication equipment" .
<http://semantic.digital-agenda-data.eu/codelist/breakdown/1500_mhz>	rdf:type	ns10:Breakdown ,
		skos:Concept ;
	skos:notation	"1500_MHz" ;
	skos:topConceptOf	ns1:breakdown ;
	ns11:membership	<http://semantic.digital-agenda-data.eu/codelist/breakdown-group/mhz_bands/1500_mhz> ;
	skos:prefLabel	"1500 MHz" .
<http://semantic.digital-agenda-data.eu/codelist/breakdown/1800_mhz>	rdf:type	ns10:Breakdown ,
		skos:Concept ;
	skos:notation	"1800_MHz" ;
	skos:topConceptOf	ns1:breakdown ;
	ns11:membership	<http://semantic.digital-agenda-data.eu/codelist/breakdown-group/mhz_bands/1800_mhz> ;
	skos:prefLabel	"1800 MHz" .
<http://semantic.digital-agenda-data.eu/codelist/breakdown/1m_websites>	rdf:type	ns10:Breakdown ,
		skos:Concept ;
	skos:notation	"1M_websites" ;
	skos:definition	"From the list of 1 million most visited websites, provided by Alexa" ;
	skos:topConceptOf	ns1:breakdown ;
	ns11:membership	<http://semantic.digital-agenda-data.eu/codelist/breakdown-group/total/1m_websites> ;
	skos:altLabel	"Total" ;
	skos:prefLabel	"Total" .
<http://semantic.digital-agenda-data.eu/codelist/breakdown/261>	rdf:type	ns10:Breakdown ,
		skos:Concept ;
	skos:notation	"261" ;
	skos:definition	"NACE2 261 Manufacture of electronic components and boards" ;
	skos:topConceptOf	ns1:breakdown ;
	ns11:membership	<http://semantic.digital-agenda-data.eu/codelist/breakdown-group/byictsector6subsec/261> ;
	skos:altLabel	"Manufacture of electronic components and boards" ;
	skos:prefLabel	"Manufacture of electronic components and boards" .
<http://semantic.digital-agenda-data.eu/codelist/breakdown/261to264>	rdf:type	ns10:Breakdown ,
		skos:Concept ;
	skos:notation	"261to264" ;
	skos:definition	"NACE2 261 to 264 - 261 Manufacture of electronic components and boards, 262 Manufacture of computers and peripheral equipment,  263 Manufacture of communication equipment, 264 Manufacture of consumer electronics" ;
	skos:topConceptOf	ns1:breakdown ;
	ns11:membership	<http://semantic.digital-agenda-data.eu/codelist/breakdown-group/byictsector2subsec/261to264> ;
	skos:altLabel	"ICT manufacturing industries" ;
	skos:prefLabel	"ICT manufacturing industries" .
<http://semantic.digital-agenda-data.eu/codelist/breakdown/261to264_582_61_62_631_951>	rdf:type	ns10:Breakdown ,
		skos:Concept ;
	skos:notation	"261to264_582_61_62_631_951" ;
	skos:definition	"NACE2 261 to 264, 582,61, 62, 631, 951 ; 261 Manufacture of electronic components and boards, 262 Manufacture of computers and peripheral equipment,  263 Manufacture of communication equipment, 264 Manufacture of consumer electronics; 582 Software publishing; 61 Telecomunications; 62 Computer programing, consultancy and related activities; 631 Data processing, hosting and related activities, web portals; 951 Repair of computers and communication equipment " ;
	skos:topConceptOf	ns1:breakdown ;
	ns11:membership	<http://semantic.digital-agenda-data.eu/codelist/breakdown-group/total/261to264_582_61_62_631_951> ;
	skos:altLabel	"ICT industries total (6 subsectors)" ;
	skos:prefLabel	"ICT industries total (6 subsectors)" .
<http://semantic.digital-agenda-data.eu/codelist/breakdown/262>	rdf:type	ns10:Breakdown ,
		skos:Concept ;
	skos:notation	"262" ;
	skos:definition	"NACE2 262 Manufacture of computers and peripheral equipment" ;
	skos:topConceptOf	ns1:breakdown ;
	ns11:membership	<http://semantic.digital-agenda-data.eu/codelist/breakdown-group/byictsector6subsec/262> ;
	skos:altLabel	"Manufacture of computers and peripheral equipment" ;
	skos:prefLabel	"Manufacture of computers and peripheral equipment" .
<http://semantic.digital-agenda-data.eu/codelist/breakdown/263>	rdf:type	ns10:Breakdown ,
		skos:Concept ;
	skos:notation	"263" ;
	skos:definition	"NACE2 263 Manufacture of communication equipment" ;
	skos:topConceptOf	ns1:breakdown ;
	ns11:membership	<http://semantic.digital-agenda-data.eu/codelist/breakdown-group/byictsector6subsec/263> ;
	skos:altLabel	"Manufacture of communication equipment" ;
	skos:prefLabel	"Manufacture of communication equipment" .
<http://semantic.digital-agenda-data.eu/codelist/breakdown/264>	rdf:type	ns10:Breakdown ,
		skos:Concept ;
	skos:notation	"264" ;
	skos:definition	"NACE2 264 Manufacture of consumer electronics" ;
	skos:topConceptOf	ns1:breakdown ;
	ns11:membership	<http://semantic.digital-agenda-data.eu/codelist/breakdown-group/byictsector6subsec/264> ;
	skos:altLabel	"Manufacture of consumer electronics" ;
	skos:prefLabel	"Manufacture of consumer electronics" .
<http://semantic.digital-agenda-data.eu/codelist/breakdown/2_6_ghz>	rdf:type	ns10:Breakdown ,
		skos:Concept ;
	skos:notation	"2_6_GHz" ;
	skos:topConceptOf	ns1:breakdown ;
	ns11:membership	<http://semantic.digital-agenda-data.eu/codelist/breakdown-group/mhz_bands/2_6_ghz> ;
	skos:prefLabel	"2.6 GHz" .
<http://semantic.digital-agenda-data.eu/codelist/breakdown/2_ghz_paired>	rdf:type	ns10:Breakdown ,
		skos:Concept ;
	skos:notation	"2_GHz_paired" ;
	skos:topConceptOf	ns1:breakdown ;
	ns11:membership	<http://semantic.digital-agenda-data.eu/codelist/breakdown-group/mhz_bands/2_ghz_paired> ;
	skos:prefLabel	"2 GHz paired" .
<http://semantic.digital-agenda-data.eu/codelist/breakdown/3_4_ghz>	rdf:type	ns10:Breakdown ,
		skos:Concept ;
	skos:notation	"3_4_GHz" ;
	skos:topConceptOf	ns1:breakdown ;
	ns11:membership	<http://semantic.digital-agenda-data.eu/codelist/breakdown-group/mhz_bands/3_4_ghz> ;
	skos:prefLabel	"3.4-3.6 GHz" .
<http://semantic.digital-agenda-data.eu/codelist/breakdown/3_6_ghz>	rdf:type	ns10:Breakdown ,
		skos:Concept ;
	skos:notation	"3_6_GHz" ;
	skos:topConceptOf	ns1:breakdown ;
	ns11:membership	<http://semantic.digital-agenda-data.eu/codelist/breakdown-group/mhz_bands/3_6_ghz> ;
	skos:prefLabel	"3.6-3.8 GHz" .
<http://semantic.digital-agenda-data.eu/codelist/breakdown/582_62_631_951>	rdf:type	ns10:Breakdown ,
		skos:Concept ;
	skos:notation	"582_62_631_951" ;
	skos:definition	"NACE2 582, 62, 631, 951\nComputer and related activities inc. Software publishing; Computer programing, consultancy and related activities; Data processing, hosting and related activities, web portals; Repair of computers and communication equipment " ;
	skos:topConceptOf	ns1:breakdown ;
	ns11:membership	<http://semantic.digital-agenda-data.eu/codelist/breakdown-group/byictsector6subsec/582_62_631_951> ;
	skos:altLabel	"Computer and related activities" ;
	skos:prefLabel	"Computer and related activities" .
<http://semantic.digital-agenda-data.eu/codelist/breakdown/61>	rdf:type	ns10:Breakdown ,
		skos:Concept ;
	skos:notation	"61" ;
	skos:definition	"NACE2 61 Telecommunications" ;
	skos:topConceptOf	ns1:breakdown ;
	ns11:membership	<http://semantic.digital-agenda-data.eu/codelist/breakdown-group/byictsector6subsec/61> ;
	skos:altLabel	"Telecommunications" ;
	skos:prefLabel	"Telecommunications" .
<http://semantic.digital-agenda-data.eu/codelist/breakdown/61_582_62_631_951>	rdf:type	ns10:Breakdown ,
		skos:Concept ;
	skos:notation	"61_582_62_631_951" ;
	skos:definition	"NACE2 582,61, 62, 631, 951\n582 Software publishing; 61 Telecomunications; 62 Computer programing, consultancy and related activities; 631 Data processing, hosting and related activities, web portals; 951 Repair of computers and communication equipment " ;
	skos:topConceptOf	ns1:breakdown ;
	ns11:membership	<http://semantic.digital-agenda-data.eu/codelist/breakdown-group/byictsector2subsec/61_582_62_631_951> ;
	skos:altLabel	"ICT services industries" ;
	skos:prefLabel	"ICT services industries" .
<http://semantic.digital-agenda-data.eu/codelist/breakdown/700_mhz>	rdf:type	ns10:Breakdown ,
		skos:Concept ;
	skos:notation	"700_MHz" ;
	skos:topConceptOf	ns1:breakdown ;
	ns11:membership	<http://semantic.digital-agenda-data.eu/codelist/breakdown-group/mhz_bands/700_mhz> ;
	skos:prefLabel	"700 MHz" .
<http://semantic.digital-agenda-data.eu/codelist/breakdown/800_mhz>	rdf:type	ns10:Breakdown ,
		skos:Concept ;
	skos:notation	"800_MHz" ;
	skos:topConceptOf	ns1:breakdown ;
	ns11:membership	<http://semantic.digital-agenda-data.eu/codelist/breakdown-group/mhz_bands/800_mhz> ;
	skos:prefLabel	"800 MHz" .
<http://semantic.digital-agenda-data.eu/codelist/breakdown/900_mhz>	rdf:type	ns10:Breakdown ,
		skos:Concept ;
	skos:notation	"900_MHz" ;
	skos:topConceptOf	ns1:breakdown ;
	ns11:membership	<http://semantic.digital-agenda-data.eu/codelist/breakdown-group/mhz_bands/900_mhz> ;
	skos:prefLabel	"900 MHz" .
ns7:all_dch	rdf:type	ns10:Breakdown ,
		skos:Concept ;
	skos:notation	"ALL_DCH" ;
	skos:definition	"dependent childrens are under 16" ;
	skos:topConceptOf	ns1:breakdown ;
	ns11:membership	ns60:all_dch ;
	skos:altLabel	"with dependent childrens" ;
	skos:prefLabel	"Household with dependent children" .
ns7:all_egov_le	rdf:type	ns10:Breakdown ,
		skos:Concept ;
	skos:notation	"all_eGov_le" ;
	skos:definition	"The following life events are included in the scope: Business Start Up, Losing and Finding a Job, Studying, Regular business operations, moving (General administration), Owning and driving a car, Starting a Small Claims procedure." ;
	skos:topConceptOf	ns1:breakdown ;
	ns11:membership	ns67:all_egov_le ;
	skos:altLabel	"All Life Events" ;
	skos:prefLabel	"All Life Events" .
ns7:all_ndch	rdf:type	ns10:Breakdown ,
		skos:Concept ;
	skos:notation	"ALL_NDCH" ;
	skos:definition	"dependent childrens are under 16" ;
	skos:topConceptOf	ns1:breakdown ;
	ns11:membership	ns60:all_ndch ;
	skos:altLabel	"without dependent childrens" ;
	skos:prefLabel	"Household without dependent children" .
ns7:bus_startup	rdf:type	ns10:Breakdown ,
		skos:Concept ;
	skos:notation	"bus_startup" ;
	skos:definition	"eGovernment services related to the life event: Business Start Up" ;
	skos:topConceptOf	ns1:breakdown ;
	ns11:membership	ns57:bus_startup ;
	skos:altLabel	"Business Start Up" ;
	skos:prefLabel	"Business Start Up Life Event" .
ns7:cable	rdf:type	ns10:Breakdown ,
		skos:Concept ;
	skos:notation	"cable" ;
	skos:topConceptOf	ns1:breakdown ;
	ns11:membership	ns27:cable ;
	skos:altLabel	"Cable modem" ;
	skos:prefLabel	"Cable modem" .
ns7:cb_eu_for	rdf:type	ns10:Breakdown ,
		skos:Concept .
@prefix ns68:	<http://eurostat.linked-statistics.org/dic/ind_type#> .
ns7:cb_eu_for	rdfs:seeAlso	ns68:CB_EU_FOR ;
	skos:notation	"CB_EU_FOR" ;
	skos:topConceptOf	ns1:breakdown ;
	ns11:membership	ns15:cb_eu_for ;
	skos:altLabel	"Another EU state" ;
	skos:prefLabel	"Individuals who are born in another EU Member State" .
ns7:cb_ext_eu	rdf:type	ns10:Breakdown ,
		skos:Concept ;
	rdfs:seeAlso	ns68:CB_EXT_EU ;
	skos:notation	"CB_EXT_EU" ;
	skos:topConceptOf	ns1:breakdown ;
	ns11:membership	ns15:cb_ext_eu ;
	skos:altLabel	"Non-EU country" ;
	skos:prefLabel	"Individuals who are born in non-EU country" .
ns7:cb_nat	rdf:type	ns10:Breakdown ,
		skos:Concept ;
	rdfs:seeAlso	ns68:CB_NAT ;
	skos:notation	"CB_NAT" ;
	skos:topConceptOf	ns1:breakdown ;
	ns11:membership	ns15:cb_nat ;
	skos:altLabel	"Native" ;
	skos:prefLabel	"Individuals who are native-born" .
ns7:cc_eu_for	rdf:type	ns10:Breakdown ,
		skos:Concept ;
	rdfs:seeAlso	ns68:CC_EU_FOR ;
	skos:notation	"CC_EU_FOR" ;
	skos:topConceptOf	ns1:breakdown ;
	ns11:membership	ns16:cc_eu_for ;
	skos:altLabel	"Nationals another EU" ;
	skos:prefLabel	"Nationals of another EU-Member State" .
ns7:cc_ext_eu	rdf:type	ns10:Breakdown ,
		skos:Concept ;
	rdfs:seeAlso	ns68:CC_EXT_EU ;
	skos:notation	"CC_EXT_EU" ;
	skos:topConceptOf	ns1:breakdown ;
	ns11:membership	ns16:cc_ext_eu ;
	skos:altLabel	"Nationals non-EU" ;
	skos:prefLabel	"Nationals of non-EU country" .
ns7:cc_nat	rdf:type	ns10:Breakdown ,
		skos:Concept ;
	rdfs:seeAlso	ns68:CC_NAT ;
	skos:notation	"CC_NAT" ;
	skos:topConceptOf	ns1:breakdown ;
	ns11:membership	ns16:cc_nat ;
	skos:altLabel	"Nationals" ;
	skos:prefLabel	"Nationals" .
ns7:cnect_a	rdf:type	ns10:Breakdown ,
		skos:Concept ;
	skos:notation	"cnect_a" ;
	skos:topConceptOf	ns1:breakdown ;
	ns11:membership	ns34:cnect_a ;
	skos:altLabel	"Directorate A" ;
	skos:prefLabel	"Directorate A, DG CONNECT" .
ns7:cnect_all	rdf:type	ns10:Breakdown ,
		skos:Concept ;
	skos:notation	"cnect_all" ;
	skos:topConceptOf	ns1:breakdown ;
	ns11:membership	ns34:cnect_all ;
	skos:altLabel	"DG CONNECT" ;
	skos:prefLabel	"DG CONNECT" .
<http://semantic.digital-agenda-data.eu/codelist/breakdown/cnect_b+>	rdf:type	ns10:Breakdown ,
		skos:Concept ;
	skos:notation	"cnect_b " ;
	skos:topConceptOf	ns1:breakdown ;
	ns11:membership	<http://semantic.digital-agenda-data.eu/codelist/breakdown-group/cnect_directorates/cnect_b+> ;
	skos:altLabel	"Directorate B" ;
	skos:prefLabel	"Directorate B, DG CONNECT" .
ns7:cnect_c	rdf:type	ns10:Breakdown ,
		skos:Concept ;
	skos:notation	"cnect_c" ;
	skos:topConceptOf	ns1:breakdown ;
	ns11:membership	ns34:cnect_c ;
	skos:altLabel	"Directorate C" ;
	skos:prefLabel	"Directorate C, DG CONNECT" .
ns7:cnect_d	rdf:type	ns10:Breakdown ,
		skos:Concept ;
	skos:notation	"cnect_d" ;
	skos:topConceptOf	ns1:breakdown ;
	ns11:membership	ns34:cnect_d ;
	skos:altLabel	"Directorate D" ;
	skos:prefLabel	"Directorate D, DG CONNECT" .
ns7:cnect_e	rdf:type	ns10:Breakdown ,
		skos:Concept ;
	skos:notation	"cnect_e" ;
	skos:topConceptOf	ns1:breakdown ;
	ns11:membership	ns34:cnect_e ;
	skos:altLabel	"Directorate E" ;
	skos:prefLabel	"Directorate E, DG CONNECT" .
ns7:cnect_f	rdf:type	ns10:Breakdown ,
		skos:Concept ;
	skos:notation	"cnect_f" ;
	skos:topConceptOf	ns1:breakdown ;
	ns11:membership	ns34:cnect_f ;
	skos:altLabel	"Directorate F" ;
	skos:prefLabel	"Directorate F, DG CONNECT" .
ns7:cnect_g	rdf:type	ns10:Breakdown ,
		skos:Concept ;
	skos:notation	"cnect_g" ;
	skos:topConceptOf	ns1:breakdown ;
	ns11:membership	ns34:cnect_g ;
	skos:altLabel	"Directorate G" ;
	skos:prefLabel	"Directorate G, DG CONNECT" .
ns7:cnect_h	rdf:type	ns10:Breakdown ,
		skos:Concept ;
	skos:notation	"cnect_h" ;
	skos:topConceptOf	ns1:breakdown ;
	ns11:membership	ns34:cnect_h ;
	skos:altLabel	"Directorate H" ;
	skos:prefLabel	"Directorate H, DG CONNECT" .
ns7:cnect_r	rdf:type	ns10:Breakdown ,
		skos:Concept ;
	skos:notation	"cnect_r" ;
	skos:topConceptOf	ns1:breakdown ;
	ns11:membership	ns34:cnect_r ;
	skos:altLabel	"Directorate R" ;
	skos:prefLabel	"Directorate R, DG CONNECT" .
ns7:csk_hi	rdf:type	ns10:Breakdown ,
		skos:Concept .
@prefix ns69:	<http://eurostat.linked-statistics.org/dic/indic_is#> .
ns7:csk_hi	rdfs:seeAlso	ns69:I_CSK_HI ;
	skos:notation	"csk_hi" ;
	skos:definition	"Individuals having ever carried out at least 5 of the following 6 activities: coping or moving a file or folder, using copy and paste tools, using basic arithmetic formula in a spreadsheet, compressing (or zipping) files, connecting and installing new devices, writing a computer program using a specialised programming language. Only those having ever used a computer were proposed the question." ;
	skos:topConceptOf	ns1:breakdown ;
	ns11:membership	ns32:csk_hi ;
	skos:altLabel	"high computer skills" ;
	skos:prefLabel	"Individuals with high computer skills" .
ns7:csk_lo	rdf:type	ns10:Breakdown ,
		skos:Concept ;
	rdfs:seeAlso	ns69:I_CSK_LO ;
	skos:notation	"csk_lo" ;
	skos:definition	"Individuals having ever carried out only 1 or 2 of the following 6 activities: coping or moving a file or folder, using copy and paste tools, using basic arithmetic formula in a spreadsheet, compressing (or zipping) files, connecting and installing new devices, writing a computer program using a specialised programming language. Only those having ever used a computer were proposed the question." ;
	skos:topConceptOf	ns1:breakdown ;
	ns11:membership	ns32:csk_lo ;
	skos:altLabel	"low computer skills" ;
	skos:prefLabel	"Individuals with low computer skills" .
ns7:cskx	rdf:type	ns10:Breakdown ,
		skos:Concept ;
	rdfs:seeAlso	ns69:I_I0 ;
	skos:notation	"cskx" ;
	skos:definition	"Individuals having ever used a computer, but having carried out none of the following 6 activities: coping or moving a file or folder, using copy and paste tools, using basic arithmetic formula in a spreadsheet, compressing (or zipping) files, connecting and installing new devices, writing a computer program using a specialised programming language. Only those having ever used a computer were proposed the question." ;
	skos:topConceptOf	ns1:breakdown ;
	ns11:membership	ns32:cskx ;
	skos:altLabel	"no computer skills" ;
	skos:prefLabel	"Individuals with no computer skills" .
ns7:desi_1_conn	rdf:type	ns10:Breakdown ,
		skos:Concept ;
	skos:notation	"DESI_1_CONN" ;
	skos:topConceptOf	ns1:breakdown ;
	ns11:membership	ns35:desi_1_conn ;
	skos:altLabel	"1 Connectivity" ;
	skos:prefLabel	"1 Connectivity" .
ns7:desi_1a1_fbbc	rdf:type	ns10:Breakdown ,
		skos:Concept ;
	skos:notation	"DESI_1A1_FBBC" ;
	skos:topConceptOf	ns1:breakdown ;
	ns11:membership	ns37:desi_1a1_fbbc ;
	skos:altLabel	"1a1 Fixed BB Coverage" ;
	skos:prefLabel	"1a1 Fixed BB Coverage" .
ns7:desi_1a2_fbbtu	rdf:type	ns10:Breakdown ,
		skos:Concept ;
	skos:notation	"DESI_1A2_FBBTU" ;
	skos:topConceptOf	ns1:breakdown ;
	ns11:membership	ns37:desi_1a2_fbbtu ;
	skos:altLabel	"1a2 Fixed BB Take-up" ;
	skos:prefLabel	"1a2 Fixed BB Take-up" .
ns7:desi_1a_fbb	rdf:type	ns10:Breakdown ,
		skos:Concept ;
	skos:notation	"DESI_1A_FBB" ;
	skos:topConceptOf	ns1:breakdown ;
	ns11:membership	ns36:desi_1a_fbb ;
	skos:altLabel	"1a Fixed Broadband" ;
	skos:prefLabel	"1a Fixed Broadband" .
ns7:desi_1b1_mbbtu	rdf:type	ns10:Breakdown ,
		skos:Concept ;
	skos:notation	"DESI_1B1_MBBTU" ;
	skos:topConceptOf	ns1:breakdown ;
	ns11:membership	ns38:desi_1b1_mbbtu ;
	skos:altLabel	"1b1 Mobile BB Take-up" ;
	skos:prefLabel	"1b1 Mobile BB Take-up" .
ns7:desi_1b2_4g	rdf:type	ns10:Breakdown ,
		skos:Concept ;
	skos:notation	"DESI_1B2_4G" ;
	skos:topConceptOf	ns1:breakdown ;
	ns11:membership	ns38:desi_1b2_4g ;
	skos:altLabel	"1b2 4G Coverage" ;
	skos:prefLabel	"1b2 4G Coverage" .
ns7:desi_1b3_spec	rdf:type	ns10:Breakdown ,
		skos:Concept ;
	skos:notation	"DESI_1B3_SPEC" ;
	skos:topConceptOf	ns1:breakdown ;
	ns11:membership	ns38:desi_1b3_spec ;
	skos:altLabel	"1b3 Spectrum" ;
	skos:prefLabel	"1b3 Spectrum" .
ns7:desi_1b_mbb	rdf:type	ns10:Breakdown ,
		skos:Concept ;
	skos:notation	"DESI_1B_MBB" ;
	skos:topConceptOf	ns1:breakdown ;
	ns11:membership	ns36:desi_1b_mbb ;
	skos:altLabel	"1b Mobile Broadband" ;
	skos:prefLabel	"1b Mobile Broadband" .
ns7:desi_1c1_ngac	rdf:type	ns10:Breakdown ,
		skos:Concept ;
	skos:notation	"DESI_1C1_NGAC" ;
	skos:topConceptOf	ns1:breakdown ;
	ns11:membership	ns39:desi_1c1_ngac ;
	skos:altLabel	"1c1 NGA Coverage" ;
	skos:prefLabel	"1c1 NGA Coverage" .
ns7:desi_1c2_sfbb	rdf:type	ns10:Breakdown ,
		skos:Concept ;
	skos:notation	"DESI_1C2_SFBB" ;
	skos:topConceptOf	ns1:breakdown ;
	ns11:membership	ns39:desi_1c2_sfbb ;
	skos:altLabel	"1c2 Subscriptions to Fast BB" ;
	skos:prefLabel	"1c2 Subscriptions to Fast BB" .
ns7:desi_1c_speed	rdf:type	ns10:Breakdown ,
		skos:Concept ;
	skos:notation	"DESI_1C_SPEED" ;
	skos:topConceptOf	ns1:breakdown ;
	ns11:membership	ns36:desi_1c_speed ;
	skos:altLabel	"1c Speed" ,
		"1c Fast Broadband" ;
	skos:prefLabel	"1c Speed" ,
		"1c Fast Broadband" .
ns7:desi_1d1_fbbp	rdf:type	ns10:Breakdown ,
		skos:Concept ;
	skos:notation	"DESI_1D1_FBBP" ;
	skos:topConceptOf	ns1:breakdown ;
	ns11:membership	ns40:desi_1d1_fbbp ;
	skos:altLabel	"1d1 Fixed BB Price" ;
	skos:prefLabel	"1d1 Fixed BB Price" .
ns7:desi_1d_aff	rdf:type	ns10:Breakdown ,
		skos:Concept ;
	skos:notation	"DESI_1D_AFF" ;
	skos:topConceptOf	ns1:breakdown ;
	ns11:membership	ns36:desi_1d_aff ;
	skos:altLabel	"1d Affordability" ;
	skos:prefLabel	"1d Affordability" .
ns7:desi_2_hc	rdf:type	ns10:Breakdown ,
		skos:Concept ;
	skos:notation	"DESI_2_HC" ;
	skos:topConceptOf	ns1:breakdown ;
	ns11:membership	ns35:desi_2_hc ;
	skos:altLabel	"2 Human Capital" ;
	skos:prefLabel	"2 Human Capital" .
ns7:desi_2a1_iu	rdf:type	ns10:Breakdown ,
		skos:Concept ;
	skos:notation	"DESI_2A1_IU" ;
	skos:topConceptOf	ns1:breakdown ;
	ns11:membership	ns42:desi_2a1_iu ;
	skos:altLabel	"2a1 Internet Users" ;
	skos:prefLabel	"2a1 Internet Users" .
ns7:desi_2a2_bds	rdf:type	ns10:Breakdown ,
		skos:Concept ;
	skos:notation	"DESI_2A2_BDS" ;
	skos:topConceptOf	ns1:breakdown ;
	ns11:membership	ns42:desi_2a2_bds ;
	skos:altLabel	"2a2 At least Basic Digital Skills" ,
		"2a2 Basic Digital Skills" ;
	skos:prefLabel	"2a2 At least Basic Digital Skills" ,
		"2a2 Basic Digital Skills" .
ns7:desi_2a_bsu	rdf:type	ns10:Breakdown ,
		skos:Concept ;
	skos:notation	"DESI_2A_BSU" ;
	skos:topConceptOf	ns1:breakdown ;
	ns11:membership	ns41:desi_2a_bsu ;
	skos:altLabel	"2a Basic Skills and Usage" ;
	skos:prefLabel	"2a Basic Skills and Usage" .
ns7:desi_2b1_ictspec	rdf:type	ns10:Breakdown ,
		skos:Concept ;
	skos:notation	"DESI_2B1_ICTSPEC" ;
	skos:topConceptOf	ns1:breakdown ;
	ns11:membership	ns43:desi_2b1_ictspec ;
	skos:altLabel	"2b1 ICT Specialists" ;
	skos:prefLabel	"2b1 ICT Specialists" .
ns7:desi_2b2_stemg	rdf:type	ns10:Breakdown ,
		skos:Concept ;
	skos:notation	"DESI_2B2_STEMG" ;
	skos:topConceptOf	ns1:breakdown ;
	ns11:membership	ns43:desi_2b2_stemg ;
	skos:altLabel	"2b2 STEM Graduates" ;
	skos:prefLabel	"2b2 STEM Graduates" .
ns7:desi_2b_asd	rdf:type	ns10:Breakdown ,
		skos:Concept ;
	skos:notation	"DESI_2B_ASD" ;
	skos:topConceptOf	ns1:breakdown ;
	ns11:membership	ns41:desi_2b_asd ;
	skos:altLabel	"2b Advanced skills and Development" ;
	skos:prefLabel	"2b Advanced skills and Development" .
ns7:desi_3_ui	rdf:type	ns10:Breakdown ,
		skos:Concept ;
	skos:notation	"DESI_3_UI" ;
	skos:topConceptOf	ns1:breakdown ;
	ns11:membership	ns35:desi_3_ui ;
	skos:altLabel	"3 Use of Internet" ;
	skos:prefLabel	"3 Use of Internet" .
ns7:desi_3a1_news	rdf:type	ns10:Breakdown ,
		skos:Concept ;
	skos:notation	"DESI_3A1_NEWS" ;
	skos:topConceptOf	ns1:breakdown ;
	ns11:membership	ns45:desi_3a1_news ;
	skos:altLabel	"3a1 News" ;
	skos:prefLabel	"3a1 News" .
ns7:desi_3a2_mvg	rdf:type	ns10:Breakdown ,
		skos:Concept ;
	skos:notation	"DESI_3A2_MVG" ;
	skos:topConceptOf	ns1:breakdown ;
	ns11:membership	ns45:desi_3a2_mvg ;
	skos:altLabel	"3a2 Music, Videos and Games" ;
	skos:prefLabel	"3a2 Music, Videos and Games" .
ns7:desi_3a3_vod	rdf:type	ns10:Breakdown ,
		skos:Concept ;
	skos:notation	"DESI_3A3_VOD" ;
	skos:topConceptOf	ns1:breakdown ;
	ns11:membership	ns45:desi_3a3_vod ;
	skos:altLabel	"3a3 Video on Demand" ;
	skos:prefLabel	"3a3 Video on Demand" .
ns7:desi_3a4_iptv	rdf:type	ns10:Breakdown ,
		skos:Concept ;
	skos:notation	"DESI_3A4_IPTV" ;
	skos:topConceptOf	ns1:breakdown ;
	ns11:membership	ns45:desi_3a4_iptv ;
	skos:altLabel	"3a4 IPTV" ;
	skos:prefLabel	"3a4 IPTV" .
ns7:desi_3a_cont	rdf:type	ns10:Breakdown ,
		skos:Concept ;
	skos:notation	"DESI_3A_CONT" ;
	skos:topConceptOf	ns1:breakdown ;
	ns11:membership	ns44:desi_3a_cont ;
	skos:altLabel	"3a Content" ;
	skos:prefLabel	"3a Content" .
ns7:desi_3b1_vidcall	rdf:type	ns10:Breakdown ,
		skos:Concept ;
	skos:notation	"DESI_3B1_VIDCALL" ;
	skos:topConceptOf	ns1:breakdown ;
	ns11:membership	ns46:desi_3b1_vidcall ;
	skos:altLabel	"3b1 Video Calls" ;
	skos:prefLabel	"3b1 Video Calls" .
ns7:desi_3b2_socnet	rdf:type	ns10:Breakdown ,
		skos:Concept ;
	skos:notation	"DESI_3B2_SOCNET" ;
	skos:topConceptOf	ns1:breakdown ;
	ns11:membership	ns46:desi_3b2_socnet ;
	skos:altLabel	"3b2 Social Networks" ;
	skos:prefLabel	"3b2 Social Networks" .
ns7:desi_3b_comm	rdf:type	ns10:Breakdown ,
		skos:Concept ;
	skos:notation	"DESI_3B_COMM" ;
	skos:topConceptOf	ns1:breakdown ;
	ns11:membership	ns44:desi_3b_comm ;
	skos:altLabel	"3b Communication" ;
	skos:prefLabel	"3b Communication" .
ns7:desi_3c1_bank	rdf:type	ns10:Breakdown ,
		skos:Concept ;
	skos:notation	"DESI_3C1_BANK" ;
	skos:topConceptOf	ns1:breakdown ;
	ns11:membership	ns47:desi_3c1_bank ;
	skos:altLabel	"3c1 Banking" ;
	skos:prefLabel	"3c1 Banking" .
ns7:desi_3c2_shop	rdf:type	ns10:Breakdown ,
		skos:Concept ;
	skos:notation	"DESI_3C2_SHOP" ;
	skos:topConceptOf	ns1:breakdown ;
	ns11:membership	ns47:desi_3c2_shop ;
	skos:altLabel	"3c2 Shopping" ;
	skos:prefLabel	"3c2 Shopping" .
ns7:desi_3c_trans	rdf:type	ns10:Breakdown ,
		skos:Concept ;
	skos:notation	"DESI_3C_TRANS" ;
	skos:topConceptOf	ns1:breakdown ;
	ns11:membership	ns44:desi_3c_trans ;
	skos:altLabel	"3c Transactions" ;
	skos:prefLabel	"3c Transactions" .
ns7:desi_4_idt	rdf:type	ns10:Breakdown ,
		skos:Concept ;
	skos:notation	"DESI_4_IDT" ;
	skos:topConceptOf	ns1:breakdown ;
	ns11:membership	ns35:desi_4_idt ;
	skos:altLabel	"4 Integration of Digital Technology" ;
	skos:prefLabel	"4 Integration of Digital Technology" .
ns7:desi_4a1_eis	rdf:type	ns10:Breakdown ,
		skos:Concept ;
	skos:notation	"DESI_4A1_EIS" ;
	skos:topConceptOf	ns1:breakdown ;
	ns11:membership	ns49:desi_4a1_eis ;
	skos:altLabel	"4a1 Electronic Information Sharing" ;
	skos:prefLabel	"4a1 Electronic Information Sharing" .
ns7:desi_4a2_rfid	rdf:type	ns10:Breakdown ,
		skos:Concept ;
	skos:notation	"DESI_4A2_RFID" ;
	skos:topConceptOf	ns1:breakdown ;
	ns11:membership	ns49:desi_4a2_rfid ;
	skos:altLabel	"4a2 RFID" ;
	skos:prefLabel	"4a2 RFID" .
ns7:desi_4a3_socmed	rdf:type	ns10:Breakdown ,
		skos:Concept ;
	skos:notation	"DESI_4A3_SOCMED" ;
	skos:topConceptOf	ns1:breakdown ;
	ns11:membership	ns49:desi_4a3_socmed ;
	skos:altLabel	"4a3 Social Media" ;
	skos:prefLabel	"4a3 Social Media" .
ns7:desi_4a4_einv	rdf:type	ns10:Breakdown ,
		skos:Concept ;
	skos:notation	"DESI_4A4_EINV" ;
	skos:topConceptOf	ns1:breakdown ;
	ns11:membership	ns49:desi_4a4_einv ;
	skos:altLabel	"4a4 eInvoices" ;
	skos:prefLabel	"4a4 eInvoices" .
ns7:desi_4a5_cloud	rdf:type	ns10:Breakdown ,
		skos:Concept ;
	skos:notation	"DESI_4A5_CLOUD" ;
	skos:topConceptOf	ns1:breakdown ;
	ns11:membership	ns49:desi_4a5_cloud ;
	skos:altLabel	"4a5 Cloud" ;
	skos:prefLabel	"4a5 Cloud" .
ns7:desi_4a_bd	rdf:type	ns10:Breakdown ,
		skos:Concept ;
	skos:notation	"DESI_4A_BD" ;
	skos:topConceptOf	ns1:breakdown ;
	ns11:membership	ns48:desi_4a_bd ;
	skos:altLabel	"4a Business digitization" ;
	skos:prefLabel	"4a Business digitization" .
ns7:desi_4b1_smeso	rdf:type	ns10:Breakdown ,
		skos:Concept ;
	skos:notation	"DESI_4B1_SMESO" ;
	skos:topConceptOf	ns1:breakdown ;
	ns11:membership	ns50:desi_4b1_smeso ;
	skos:altLabel	"4b1 SMEs Selling Online" ;
	skos:prefLabel	"4b1 SMEs Selling Online" .
ns7:desi_4b2_ecomturn	rdf:type	ns10:Breakdown ,
		skos:Concept ;
	skos:notation	"DESI_4B2_ECOMTURN" ;
	skos:topConceptOf	ns1:breakdown ;
	ns11:membership	ns50:desi_4b2_ecomturn ;
	skos:altLabel	"4b2 eCommerce Turnover" ;
	skos:prefLabel	"4b2 eCommerce Turnover" .
ns7:desi_4b3_sellcb	rdf:type	ns10:Breakdown ,
		skos:Concept ;
	skos:notation	"DESI_4B3_SELLCB" ;
	skos:topConceptOf	ns1:breakdown ;
	ns11:membership	ns50:desi_4b3_sellcb ;
	skos:altLabel	"4b3 Selling Online Cross-border" ;
	skos:prefLabel	"4b3 Selling Online Cross-border" .
ns7:desi_4b_ecomm	rdf:type	ns10:Breakdown ,
		skos:Concept ;
	skos:notation	"DESI_4B_ECOMM" ;
	skos:topConceptOf	ns1:breakdown ;
	ns11:membership	ns48:desi_4b_ecomm ;
	skos:altLabel	"4b eCommerce" ;
	skos:prefLabel	"4b eCommerce" .
ns7:desi_5_dps	rdf:type	ns10:Breakdown ,
		skos:Concept ;
	skos:notation	"DESI_5_DPS" ;
	skos:topConceptOf	ns1:breakdown ;
	ns11:membership	ns35:desi_5_dps ;
	skos:altLabel	"5 Digital Public Services" ;
	skos:prefLabel	"5 Digital Public Services" .
ns7:desi_5a1_egovu	rdf:type	ns10:Breakdown ,
		skos:Concept ;
	skos:notation	"DESI_5A1_EGOVU" ;
	skos:topConceptOf	ns1:breakdown ;
	ns11:membership	ns52:desi_5a1_egovu ;
	skos:altLabel	"5a1 eGovernment Users" ;
	skos:prefLabel	"5a1 eGovernment Users" .
ns7:desi_5a2_prefform	rdf:type	ns10:Breakdown ,
		skos:Concept ;
	skos:notation	"DESI_5A2_PREFFORM" ;
	skos:topConceptOf	ns1:breakdown ;
	ns11:membership	ns52:desi_5a2_prefform ;
	skos:altLabel	"5a2 Pre-filled Forms" ;
	skos:prefLabel	"5a2 Pre-filled Forms" .
ns7:desi_5a3_osercomp	rdf:type	ns10:Breakdown ,
		skos:Concept ;
	skos:notation	"DESI_5A3_OSERCOMP" ;
	skos:topConceptOf	ns1:breakdown ;
	ns11:membership	ns52:desi_5a3_osercomp ;
	skos:altLabel	"5a3 Online Service Completion" ;
	skos:prefLabel	"5a3 Online Service Completion" .
ns7:desi_5a4_opendata	rdf:type	ns10:Breakdown ,
		skos:Concept ;
	skos:notation	"DESI_5A4_OPENDATA" ;
	skos:topConceptOf	ns1:breakdown ;
	ns11:membership	ns52:desi_5a4_opendata ;
	skos:altLabel	"5a4 Open Data" ;
	skos:prefLabel	"5a4 Open Data" .
ns7:desi_5a_egov	rdf:type	ns10:Breakdown ,
		skos:Concept ;
	skos:notation	"DESI_5A_EGOV" ;
	skos:topConceptOf	ns1:breakdown ;
	ns11:membership	ns51:desi_5a_egov ;
	skos:altLabel	"5a eGovernment" ;
	skos:prefLabel	"5a eGovernment" .
ns7:desi_5b1_mdataexch	rdf:type	ns10:Breakdown ,
		skos:Concept ;
	skos:notation	"DESI_5B1_MDATAEXCH" ;
	skos:topConceptOf	ns1:breakdown ;
	ns11:membership	ns53:desi_5b1_mdataexch ;
	skos:altLabel	"5b1 Medical Data Exchange" ;
	skos:prefLabel	"5b1 Medical Data Exchange" .
ns7:desi_5b2_epresc	rdf:type	ns10:Breakdown ,
		skos:Concept ;
	skos:notation	"DESI_5B2_EPRESC" ;
	skos:topConceptOf	ns1:breakdown ;
	ns11:membership	ns53:desi_5b2_epresc ;
	skos:altLabel	"5b2 ePrescription" ;
	skos:prefLabel	"5b2 ePrescription" .
ns7:desi_5b_ehealth	rdf:type	ns10:Breakdown ,
		skos:Concept ;
	skos:notation	"DESI_5B_EHEALTH" ;
	skos:topConceptOf	ns1:breakdown ;
	ns11:membership	ns51:desi_5b_ehealth ;
	skos:altLabel	"5b eHealth" ;
	skos:prefLabel	"5b eHealth" .
ns7:desi_total	rdf:type	ns10:Breakdown ,
		skos:Concept ;
	skos:notation	"DESI_TOTAL" ;
	skos:topConceptOf	ns1:breakdown ;
	ns11:membership	ns54:desi_total ;
	skos:altLabel	"Aggregate score" ;
	skos:prefLabel	"Aggregate score" .
ns7:ds_a_basic	rdf:type	ns10:Breakdown ,
		skos:Concept ;
	skos:notation	"ds_a_basic" ;
	skos:definition	"Individual having \"above basic\" skills in ALL the four Digital Competence domains included in the index: information, communication, content-creation and problem-solving." ;
	skos:topConceptOf	ns1:breakdown ;
	ns11:membership	ns55:ds_a_basic ;
	skos:altLabel	"level: Above Basic" ;
	skos:prefLabel	"level: Above Basic" .
ns7:ds_b_basic	rdf:type	ns10:Breakdown ,
		skos:Concept ;
	skos:notation	"ds_b_basic" ;
	skos:definition	"Individual \"without basic\" skills in AT LEAST ONE of the four Digital Competence domains included in the index: information, communication, content-creation and problem-solving." ;
	skos:topConceptOf	ns1:breakdown ;
	ns11:membership	ns55:ds_b_basic ;
	skos:altLabel	"level: Low" ;
	skos:prefLabel	"level: Low" .
ns7:ds_basic	rdf:type	ns10:Breakdown ,
		skos:Concept ;
	skos:notation	"ds_basic" ;
	skos:definition	"Individual having at least \"basic\" skills in ALL the four Digital Competence domains included in the index: information, communication, content-creation and problem-solving, but no more than three above basic." ;
	skos:topConceptOf	ns1:breakdown ;
	ns11:membership	ns55:ds_basic ;
	skos:altLabel	"level: Basic" ;
	skos:prefLabel	"level: Basic" .
ns7:ds_no	rdf:type	ns10:Breakdown ,
		skos:Concept ;
	skos:notation	"ds_no" ;
	skos:definition	"Individuals that have not used internet during last 3 months." ;
	skos:topConceptOf	ns1:breakdown ;
	ns11:membership	ns55:ds_no ;
	skos:altLabel	"No" ;
	skos:prefLabel	"No digital skills " .
ns7:dsk_ab	rdf:type	ns10:Breakdown ,
		skos:Concept ;
	skos:notation	"DSK_AB" ;
	skos:topConceptOf	ns1:breakdown ;
	ns11:membership	ns55:dsk_ab ;
	skos:altLabel	"level: Above Basic" ;
	skos:prefLabel	"level: Above Basic" .
ns7:dsk_b	rdf:type	ns10:Breakdown ,
		skos:Concept ;
	skos:notation	"DSK_B" ;
	skos:topConceptOf	ns1:breakdown ;
	ns11:membership	ns55:dsk_b ;
	skos:altLabel	"level: Basic" ;
	skos:prefLabel	"level: Basic" .
ns7:dsk_x	rdf:type	ns10:Breakdown ,
		skos:Concept ;
	skos:notation	"dsk_x" ;
	skos:topConceptOf	ns1:breakdown ;
	ns11:membership	ns55:dsk_x ;
	skos:altLabel	"level: none" ;
	skos:prefLabel	"level: none" .
ns7:e_cc_hi	rdf:type	ns10:Breakdown ,
		skos:Concept ;
	skos:notation	"e_cc_hi" ;
	skos:definition	"Usage of any of the following Cloud computing services: accounting software applications, CRM software, computing power." ;
	skos:topConceptOf	ns1:breakdown ;
	ns11:membership	ns17:e_cc_hi ;
	skos:altLabel	"High sophistication" ;
	skos:prefLabel	"High sophistication" .
ns7:e_cc_lo	rdf:type	ns10:Breakdown ,
		skos:Concept ;
	skos:notation	"e_cc_lo" ;
	skos:definition	"Usage of Cloud computing services for e-mail, office software, storage of files, but none of the other medium-high sophistication services proposed in the questionnaire." ;
	skos:topConceptOf	ns1:breakdown ;
	ns11:membership	ns17:e_cc_lo ;
	skos:altLabel	"Low sophistication" ;
	skos:prefLabel	"Low sophistication" .
ns7:e_cc_me	rdf:type	ns10:Breakdown ,
		skos:Concept ;
	skos:notation	"e_cc_me" ;
	skos:definition	"Usage of Cloud computing services for hosting of the enterprise's database, but none of the high sophistication services proposed in the questionnaire: accounting software applications, CRM software, computing power. Include other non specified services." ;
	skos:topConceptOf	ns1:breakdown ;
	ns11:membership	ns17:e_cc_me ;
	skos:altLabel	"Medium sophistication" ;
	skos:prefLabel	"Medium sophistication" .
ns7:e_di_hi	rdf:type	ns10:Breakdown ,
		skos:Concept ;
	skos:notation	"e_di_hi" ;
	skos:topConceptOf	ns1:breakdown ;
	ns11:membership	ns19:e_di_hi ;
	skos:altLabel	"High (7-9)" ;
	skos:prefLabel	"High (7-9)" .
ns7:e_di_lo	rdf:type	ns10:Breakdown ,
		skos:Concept ;
	skos:notation	"e_di_lo" ;
	skos:topConceptOf	ns1:breakdown ;
	ns11:membership	ns19:e_di_lo ;
	skos:altLabel	"Low (4-6)" ;
	skos:prefLabel	"Low (4-6)" .
ns7:e_di_vhi	rdf:type	ns10:Breakdown ,
		skos:Concept ;
	skos:notation	"e_di_vhi" ;
	skos:topConceptOf	ns1:breakdown ;
	ns11:membership	ns19:e_di_vhi ;
	skos:altLabel	"Very High (10-12)" ;
	skos:prefLabel	"Very High (10-12)" .
ns7:e_di_vlo	rdf:type	ns10:Breakdown ,
		skos:Concept ;
	skos:notation	"e_di_vlo" ;
	skos:topConceptOf	ns1:breakdown ;
	ns11:membership	ns19:e_di_vlo ;
	skos:altLabel	"Very Low (0-3)" ;
	skos:prefLabel	"Very Low (0-3)" .
ns7:ec_all	rdf:type	ns10:Breakdown ,
		skos:Concept ;
	skos:notation	"EC_all" ;
	skos:topConceptOf	ns1:breakdown ;
	ns11:membership	ns61:ec_all ,
		ns34:ec_all ;
	skos:altLabel	"EC all reserach DGs" ;
	skos:prefLabel	"All research DGs of the European Commission" .
ns7:einfra	rdf:type	ns10:Breakdown ,
		skos:Concept ;
	skos:notation	"eInfra" ;
	skos:topConceptOf	ns1:breakdown ;
	ns11:membership	ns66:einfra ;
	skos:altLabel	"eInfra" ;
	skos:prefLabel	"eInfrastructures" .
ns7:empl_une	rdf:type	ns10:Breakdown ,
		skos:Concept ;
	rdfs:seeAlso	ns68:EMPL_UNE ;
	skos:notation	"EMPL_UNE" ;
	skos:topConceptOf	ns1:breakdown ;
	ns11:membership	ns62:empl_une ;
	skos:altLabel	"Employed and unemployed" ;
	skos:prefLabel	"Active labour force (employed and unemployed)" .
ns7:ent_all_xfin	rdf:type	ns10:Breakdown ,
		skos:Concept ;
	skos:notation	"ent_all_xfin" ;
	skos:definition	"Since 2010: 10_C10_S951_XK, 2009: 10_C10_N82_XK, until 2008: 10_dfghiko" ;
	skos:topConceptOf	ns1:breakdown ;
	ns11:membership	ns67:ent_all_xfin ;
	skos:altLabel	"All enterprises" ;
	skos:prefLabel	"All enterprises, without financial sector (10 persons employed or more)" .
ns7:ent_l_xfin	rdf:type	ns10:Breakdown ,
		skos:Concept ;
	skos:notation	"ent_l_xfin" ;
	skos:definition	"Since 2010: L_C10_S951_XK, 2009: L_C10_N82_XK, until 2008: l_dfghiko" ;
	skos:topConceptOf	ns1:breakdown ;
	ns11:membership	ns26:ent_l_xfin ,
		ns25:ent_l_xfin ;
	skos:altLabel	"Large enterprises" ;
	skos:prefLabel	"Large enterprises (250 persons employed or more), without financial sector" .
ns7:ent_m_xfin	rdf:type	ns10:Breakdown ,
		skos:Concept ;
	skos:notation	"ent_m_xfin" ;
	skos:definition	"Since 2010: L_C10_S951_XK, 2009: L_C10_N82_XK, until 2008: l_dfghiko" ;
	skos:topConceptOf	ns1:breakdown ;
	ns11:membership	ns26:ent_m_xfin ;
	skos:altLabel	"Medium enterprises" ;
	skos:prefLabel	"Medium enterprises (50-249 persons employed), without financial sector" .
ns7:ent_s_xfin	rdf:type	ns10:Breakdown ,
		skos:Concept ;
	skos:notation	"ent_s_xfin" ;
	skos:definition	"Since 2010: L_C10_S951_XK, 2009: L_C10_N82_XK, until 2008: l_dfghiko" ;
	skos:topConceptOf	ns1:breakdown ;
	ns11:membership	ns26:ent_s_xfin ;
	skos:altLabel	"Small enterprises" ;
	skos:prefLabel	"Small enterprises (10-49 persons employed), without financial sector" .
ns7:ent_sm_xfin	rdf:type	ns10:Breakdown ,
		skos:Concept ;
	skos:notation	"ent_sm_xfin" ;
	skos:definition	"Since 2010: SM_C10_S951_XK, 2009: SM_C10_N82_XK, until 2008: sm_dfghiko" ;
	skos:topConceptOf	ns1:breakdown ;
	ns11:membership	ns25:ent_sm_xfin ;
	skos:altLabel	"SMEs (10-249 persons employed)" ;
	skos:prefLabel	"SMEs (10-249 persons employed), without financial sector" .
ns7:epsiscore_events	rdf:type	ns10:Breakdown ,
		skos:Concept ;
	skos:notation	"epsiscore_events" ;
	skos:definition	"PSI-related vents and activities (3 indicators: some national or inter-regional events; a moderate number of national or inter-regional events; a considerable number of national or inter-regional events)" ;
	skos:topConceptOf	ns1:breakdown ;
	ns11:membership	ns58:epsiscore_events ;
	skos:altLabel	"Events and activities" ;
	skos:prefLabel	"PSI events and activities" .
ns7:epsiscore_exarrange	rdf:type	ns10:Breakdown ,
		skos:Concept ;
	skos:notation	"epsiscore_exarrange" ;
	skos:definition	"PSI exclusive arrangements (3 indicators: prohibition of exclusive arrangements; legal action against exclusive arrangements; ending exclusive arrangements)" ;
	skos:topConceptOf	ns1:breakdown ;
	ns11:membership	ns58:epsiscore_exarrange ;
	skos:altLabel	"Exclusive arrangements" ;
	skos:prefLabel	"PSI use of exclusive arrangements" .
ns7:epsiscore_formats	rdf:type	ns10:Breakdown ,
		skos:Concept ;
	skos:notation	"epsiscore_formats" ;
	skos:definition	"PSI dataset formats (4 indicators: endorsement of \u2018raw\u2019 data and open standards; obligatory \u2018raw\u2019 data and open standards; endorsement of \u2018Linked Open Data\u2019; existence of national or regional data catalogue(s))" ;
	skos:topConceptOf	ns1:breakdown ;
	ns11:membership	ns58:epsiscore_formats ;
	skos:altLabel	"Formats" ;
	skos:prefLabel	"PSI formats" .
ns7:epsiscore_implem	rdf:type	ns10:Breakdown ,
		skos:Concept ;
	skos:notation	"epsiscore_implem" ;
	skos:definition	"Implementation of the PSI Directive (2 indicators: implementation and absence of infringement procedures and exemptions granted)" ;
	skos:topConceptOf	ns1:breakdown ;
	ns11:membership	ns58:epsiscore_implem ;
	skos:altLabel	"PSI mplementation" ;
	skos:prefLabel	"Implementation of the PSI Directive" .
ns7:epsiscore_localpsi	rdf:type	ns10:Breakdown ,
		skos:Concept ;
	skos:notation	"epsiscore_localpsi" ;
	skos:definition	"Local and regional PSI availability and open data communities (3 indicators: some local or regional PSI available and community activity; moderate local or regional PSI available and community activity; considerable local or regional PSI available and community activity)" ;
	skos:topConceptOf	ns1:breakdown ;
	ns11:membership	ns58:epsiscore_localpsi ;
	skos:altLabel	"Local PSI" ;
	skos:prefLabel	"Local and regional PSI availability and open data communities" .
ns7:epsiscore_practice	rdf:type	ns10:Breakdown ,
		skos:Concept ;
	skos:notation	"epsiscore_practice" ;
	skos:definition	"National PSI re-use policy (5 indicators: general right of re-use; distinction between commercial and non-commercial re-use; redress mechanisms; pro-active publishing of PSI for re-use; availability of standard licences)" ;
	skos:topConceptOf	ns1:breakdown ;
	ns11:membership	ns58:epsiscore_practice ;
	skos:altLabel	"The practice of re-use" ;
	skos:prefLabel	"National PSI re-use practice" .
ns7:epsiscore_pricing	rdf:type	ns10:Breakdown ,
		skos:Concept ;
	skos:notation	"epsiscore_pricing" ;
	skos:definition	"PSI pricing (3 indicators: cost-recovery model or marginal costing model; no exceptions to marginal costing model)" ;
	skos:topConceptOf	ns1:breakdown ;
	ns11:membership	ns58:epsiscore_pricing ;
	skos:altLabel	"Pricing" ;
	skos:prefLabel	"PSI pricing" .
ns7:epsiscore_total	rdf:type	ns10:Breakdown ,
		skos:Concept ;
	skos:notation	"epsiscore_total" ;
	skos:topConceptOf	ns1:breakdown ;
	ns11:membership	ns67:epsiscore_total ;
	skos:altLabel	"PSI overall score" ;
	skos:prefLabel	"PSI overall score" .
ns7:f	rdf:type	ns10:Breakdown ,
		skos:Concept ;
	skos:notation	"F" ;
	skos:topConceptOf	ns1:breakdown ;
	ns11:membership	ns28:f ;
	skos:altLabel	"Females" ;
	skos:prefLabel	"Females " .
ns7:f_y16_74	rdf:type	ns10:Breakdown ,
		skos:Concept ;
	rdfs:seeAlso	ns68:F_Y16_74 ;
	skos:notation	"F_Y16_74" ;
	skos:topConceptOf	ns1:breakdown ;
	ns11:membership	ns28:f_y16_74 ;
	skos:altLabel	"Females" ;
	skos:prefLabel	"Females, 16 to 74 years old" .
ns7:fttx	rdf:type	ns10:Breakdown ,
		skos:Concept ;
	skos:notation	"FTTx" ;
	skos:topConceptOf	ns1:breakdown ;
	ns11:membership	ns27:fttx ;
	skos:altLabel	"Fiber to the x" ;
	skos:prefLabel	"Fiber to the x" .
ns7:gen_admin_move	rdf:type	ns10:Breakdown ,
		skos:Concept ;
	skos:notation	"gen_admin_move" ;
	skos:definition	"eGovernment services related to the life event: moving (General administration)" ;
	skos:topConceptOf	ns1:breakdown ;
	ns11:membership	ns57:gen_admin_move ;
	skos:altLabel	"General administration: moving" ;
	skos:prefLabel	"General administration: moving Life Event" .
ns7:goods	rdf:type	ns10:Breakdown ,
		skos:Concept ;
	skos:notation	"goods" ;
	skos:topConceptOf	ns1:breakdown ;
	ns11:membership	ns33:goods ;
	skos:altLabel	"Goods" ;
	skos:prefLabel	"Goods" .
ns7:grade11gen	rdf:type	ns10:Breakdown ,
		skos:Concept ;
	skos:notation	"grade11gen" ;
	skos:definition	"Students enrolled are at the eleventh year of schooling, counting from the first year of Primary - ISCED level 1. Mean age of students in Grade11 is at least 16,5 years." ;
	skos:topConceptOf	ns1:breakdown ;
	ns11:membership	ns23:grade11gen ;
	skos:altLabel	"Grade 11 Vocational" ;
	skos:prefLabel	"Grade 11 (Upper secondary, vocational)" .
ns7:grade11voc	rdf:type	ns10:Breakdown ,
		skos:Concept ;
	skos:notation	"grade11voc" ;
	skos:definition	"Students enrolled are at the eleventh year of schooling, counting from the first year of Primary - ISCED level 1. Mean age of students in Grade11 is at least 16,5 years." ;
	skos:topConceptOf	ns1:breakdown ;
	ns11:membership	ns23:grade11voc ;
	skos:altLabel	"Grade 11 General" ;
	skos:prefLabel	"Grade 11 (Upper secondary, general)" .
ns7:grade4	rdf:type	ns10:Breakdown ,
		skos:Concept ;
	skos:notation	"grade4" ;
	skos:definition	"Students enrolled are at the fourth year of schooling, counting from the first year of Primary - ISCED level 1. Mean age of students in Grade4 is at least 9,5 years." ;
	skos:topConceptOf	ns1:breakdown ;
	ns11:membership	ns23:grade4 ;
	skos:altLabel	"Grade 4" ;
	skos:prefLabel	"Grade 4 (Primary school)" .
ns7:grade8	rdf:type	ns10:Breakdown ,
		skos:Concept ;
	skos:notation	"grade8" ;
	skos:definition	"Students enrolled are at the eighth year of schooling, counting from the first year of Primary - ISCED level 1. Mean age of students in Grade8 is at least 13,5 years." ;
	skos:topConceptOf	ns1:breakdown ;
	ns11:membership	ns23:grade8 ;
	skos:altLabel	"Grade 8" ;
	skos:prefLabel	"Grade 8 (Lower secondary)" .
ns7:hh_deg1	rdf:type	ns10:Breakdown ,
		skos:Concept ;
	skos:notation	"HH_DEG1" ;
	skos:definition	"Densely-populated area with at least 500 inhabitants/Km2." ;
	skos:topConceptOf	ns1:breakdown ;
	ns11:membership	ns18:hh_deg1 ;
	skos:altLabel	"Urban areas" ;
	skos:prefLabel	"Households living in densely-populated area" .
ns7:hh_deg2	rdf:type	ns10:Breakdown ,
		skos:Concept ;
	skos:notation	"HH_DEG2" ;
	skos:definition	"Intermediate urbanized area with between 100 and 499 inhabitants/Km2." ;
	skos:topConceptOf	ns1:breakdown ;
	ns11:membership	ns18:hh_deg2 ;
	skos:altLabel	"Intermediate areas" ;
	skos:prefLabel	"Households living in intermediate urbanized area" .
ns7:hh_deg3	rdf:type	ns10:Breakdown ,
		skos:Concept ;
	skos:notation	"HH_DEG3" ;
	skos:definition	"Sparsely populated area with less than 100 inhabitants/Km2." ;
	skos:topConceptOf	ns1:breakdown ;
	ns11:membership	ns18:hh_deg3 ;
	skos:altLabel	"Rural areas" ;
	skos:prefLabel	"Households living in sparsely populated area" .
ns7:hh_no1	rdf:type	ns10:Breakdown ,
		skos:Concept ;
	skos:notation	"HH_NO1" ;
	skos:definition	"As defined in Structural Funds regulations" ;
	skos:topConceptOf	ns1:breakdown ;
	ns11:membership	ns30:hh_no1 ;
	skos:altLabel	"Other regions" ;
	skos:prefLabel	"Living in Not Objective 1 regions / 'Regional Competitiveness and Employment' Region" .
ns7:hh_o1	rdf:type	ns10:Breakdown ,
		skos:Concept ;
	skos:notation	"HH_O1" ;
	skos:definition	"As defined in Structural Funds regulations" ;
	skos:topConceptOf	ns1:breakdown ;
	ns11:membership	ns30:hh_o1 ;
	skos:altLabel	"Objective1-Convergence regions" ;
	skos:prefLabel	"Living in Objective 1 regions / 'Convergence' regions" .
ns7:hh_total	rdf:type	ns10:Breakdown ,
		skos:Concept ;
	skos:notation	"HH_total" ;
	skos:definition	"All households with at least one individual aged 16-74." ;
	skos:topConceptOf	ns1:breakdown ;
	ns11:membership	ns67:hh_total ;
	skos:altLabel	"All households" ;
	skos:prefLabel	"All households" .
ns7:hhi_q1	rdf:type	ns10:Breakdown ,
		skos:Concept ;
	rdfs:seeAlso	ns68:HHI_Q1 ;
	skos:notation	"HHI_Q1" ;
	skos:definition	"Income in the first quartile means income among the 25% lowest income observed" ;
	skos:topConceptOf	ns1:breakdown ;
	ns11:membership	ns59:hhi_q1 ;
	skos:altLabel	"low income households" ;
	skos:prefLabel	"Individuals living in a household with income in first quartile (lowest)" .
ns7:hhi_q2	rdf:type	ns10:Breakdown ,
		skos:Concept ;
	rdfs:seeAlso	ns68:HHI_Q2 ;
	skos:notation	"HHI_Q2" ;
	skos:definition	"Income in the second quartile means income among the 50% lowest incomes observed, but not among the 25% lowest" ;
	skos:topConceptOf	ns1:breakdown ;
	ns11:membership	ns59:hhi_q2 ;
	skos:altLabel	"medium/low income households" ;
	skos:prefLabel	"Individuals living in a household with income in second quartile" .
ns7:hhi_q3	rdf:type	ns10:Breakdown ,
		skos:Concept ;
	rdfs:seeAlso	ns68:HHI_Q3 ;
	skos:notation	"HHI_Q3" ;
	skos:definition	"Income in the third quartile means income among the 50% highest incomes observed, but not among the 25% highest" ;
	skos:topConceptOf	ns1:breakdown ;
	ns11:membership	ns59:hhi_q3 ;
	skos:altLabel	"medium/high income households" ;
	skos:prefLabel	"Individuals living in a household with income in third quartile" .
ns7:hhi_q4	rdf:type	ns10:Breakdown ,
		skos:Concept ;
	rdfs:seeAlso	ns68:HHI_Q4 ;
	skos:notation	"HHI_Q4" ;
	skos:definition	"Income in the fourth quartile means income among the 25% highest incomes observed" ;
	skos:topConceptOf	ns1:breakdown ;
	ns11:membership	ns59:hhi_q4 ;
	skos:altLabel	"high income households" ;
	skos:prefLabel	"Individuals living in a household with income in fourth quartile (highest)" .
ns7:i0_2	rdf:type	ns10:Breakdown ,
		skos:Concept ;
	rdfs:seeAlso	ns68:I0_2 ;
	skos:notation	"I0_2" ;
	skos:definition	"Having maximum Primary or Lower secondary education (ISCED 0, 1 or 2)" ;
	skos:topConceptOf	ns1:breakdown ;
	ns11:membership	ns22:i0_2 ;
	skos:altLabel	"low education level" ;
	skos:prefLabel	"Individuals with no or low formal education" .
ns7:i0_4	rdf:type	ns10:Breakdown ,
		skos:Concept ;
	skos:notation	"I0_4" ;
	skos:definition	"Having maximum post post secondary education, but not tertiary  (ISCED 1997 0-4 Level 0 \u2013 Pre-primary education Level 1 \u2013 Primary education or first stage of basic education, Level 2 \u2013 Lower secondary or second stage of basic education, Level 3 \u2013 (Upper) secondary education, Level 4 \u2013 Post-secondary non-tertiary education)\n " ;
	skos:topConceptOf	ns1:breakdown ;
	ns11:membership	ns22:i0_4 ;
	skos:altLabel	"no high education" ;
	skos:prefLabel	"Individuals with no high education" .
ns7:i3_4	rdf:type	ns10:Breakdown ,
		skos:Concept ;
	rdfs:seeAlso	ns68:I3_4 ;
	skos:notation	"I3_4" ;
	skos:definition	"Having Upper or post secondary education, but not tertiary (ISCED 3 or 4)" ;
	skos:topConceptOf	ns1:breakdown ;
	ns11:membership	ns22:i3_4 ;
	skos:altLabel	"medium education level" ;
	skos:prefLabel	"Individuals with medium formal education" .
ns7:i5_8	rdf:type	ns10:Breakdown ,
		skos:Concept ;
	rdfs:seeAlso	ns68:I5_8 ;
	skos:notation	"I5_8" ;
	skos:definition	"(ISCED 2011 5-8 Level 5 \u2013 Short-cycle tertiary education, Level 6 \u2013 Bachelor\u2019s or equivalent level, Level 7 \u2013 Master\u2019s or equivalent level, Level 8 \u2013 Doctoral or equivalent level)\n" ;
	skos:topConceptOf	ns1:breakdown ;
	ns11:membership	ns22:i5_8 ;
	skos:altLabel	"high education level" ;
	skos:prefLabel	"Individuals with high formal education" .
ns7:ind_deg1	rdf:type	ns10:Breakdown ,
		skos:Concept ;
	skos:notation	"IND_DEG1" ;
	skos:definition	"Densely-populated area with at least 500 inhabitants/Km2." ;
	skos:topConceptOf	ns1:breakdown ;
	ns11:membership	ns18:ind_deg1 ;
	skos:altLabel	"Urban areas" ;
	skos:prefLabel	"Individuals living in densely-populated area" .
ns7:ind_deg2	rdf:type	ns10:Breakdown ,
		skos:Concept ;
	skos:notation	"IND_DEG2" ;
	skos:definition	"Intermediate urbanized area with between 100 and 499 inhabitants/Km2." ;
	skos:topConceptOf	ns1:breakdown ;
	ns11:membership	ns18:ind_deg2 ;
	skos:altLabel	"Intermediate areas" ;
	skos:prefLabel	"Individuals living in intermediate urbanized area" .
ns7:ind_deg3	rdf:type	ns10:Breakdown ,
		skos:Concept ;
	skos:notation	"IND_DEG3" ;
	skos:definition	"Sparsely populated area with less than 100 inhabitants/Km2." ;
	skos:topConceptOf	ns1:breakdown ;
	ns11:membership	ns18:ind_deg3 ;
	skos:altLabel	"Rural areas" ;
	skos:prefLabel	"Individuals living in sparsely populated area" .
ns7:ind_no1	rdf:type	ns10:Breakdown ,
		skos:Concept ;
	skos:notation	"IND_NO1" ;
	skos:definition	"As defined in Structural Funds regulations" ;
	skos:topConceptOf	ns1:breakdown ;
	ns11:membership	ns30:ind_no1 ;
	skos:altLabel	"Other regions" ;
	skos:prefLabel	"Living in Not Objective 1 regions / 'Regional Competitiveness and Employment' Region" .
ns7:ind_o1	rdf:type	ns10:Breakdown ,
		skos:Concept ;
	skos:notation	"IND_O1" ;
	skos:definition	"As defined in Structural Funds regulations" ;
	skos:topConceptOf	ns1:breakdown ;
	ns11:membership	ns30:ind_o1 ;
	skos:altLabel	"Objective1-Convergence regions" ;
	skos:prefLabel	"Living in Objective 1 regions / 'Convergence' regions" .
ns7:ind_total	rdf:type	ns10:Breakdown ,
		skos:Concept ;
	rdfs:seeAlso	ns68:IND_TOTAL ;
	skos:notation	"IND_TOTAL" ;
	skos:topConceptOf	ns1:breakdown ;
	ns11:membership	ns67:ind_total ;
	skos:altLabel	"All individuals" ;
	skos:prefLabel	"All Individuals (aged 16-74)" .
ns7:infso_a	rdf:type	ns10:Breakdown ,
		skos:Concept ;
	skos:notation	"infso_a" ;
	skos:topConceptOf	ns1:breakdown ;
	ns11:membership	ns61:infso_a ;
	skos:altLabel	"Directorate A" ;
	skos:prefLabel	"Directorate A, DG INFSO" .
ns7:infso_all	rdf:type	ns10:Breakdown ,
		skos:Concept ;
	skos:notation	"infso_all" ;
	skos:topConceptOf	ns1:breakdown ;
	ns11:membership	ns61:infso_all ;
	skos:altLabel	"DG INFSO" ;
	skos:prefLabel	"DG INFSO" .
ns7:infso_b	rdf:type	ns10:Breakdown ,
		skos:Concept ;
	skos:notation	"infso_b" ;
	skos:topConceptOf	ns1:breakdown ;
	ns11:membership	ns61:infso_b ;
	skos:altLabel	"Directorate B" ;
	skos:prefLabel	"Directorate B, DG INFSO" .
ns7:infso_c	rdf:type	ns10:Breakdown ,
		skos:Concept ;
	skos:notation	"infso_c" ;
	skos:topConceptOf	ns1:breakdown ;
	ns11:membership	ns61:infso_c ;
	skos:altLabel	"Directorate C" ;
	skos:prefLabel	"Directorate C, DG INFSO" .
ns7:infso_d	rdf:type	ns10:Breakdown ,
		skos:Concept ;
	skos:notation	"infso_d" ;
	skos:topConceptOf	ns1:breakdown ;
	ns11:membership	ns61:infso_d ;
	skos:altLabel	"Directorate D" ;
	skos:prefLabel	"Directorate D, DG INFSO" .
ns7:infso_e	rdf:type	ns10:Breakdown ,
		skos:Concept ;
	skos:notation	"infso_e" ;
	skos:topConceptOf	ns1:breakdown ;
	ns11:membership	ns61:infso_e ;
	skos:altLabel	"Directorate E" ;
	skos:prefLabel	"Directorate E, DG INFSO" .
ns7:infso_f	rdf:type	ns10:Breakdown ,
		skos:Concept ;
	skos:notation	"infso_f" ;
	skos:topConceptOf	ns1:breakdown ;
	ns11:membership	ns61:infso_f ;
	skos:altLabel	"Directorate F" ;
	skos:prefLabel	"Directorate F, DG INFSO" .
ns7:infso_g	rdf:type	ns10:Breakdown ,
		skos:Concept ;
	skos:notation	"infso_g" ;
	skos:topConceptOf	ns1:breakdown ;
	ns11:membership	ns61:infso_g ;
	skos:altLabel	"Directorate G" ;
	skos:prefLabel	"Directorate G, DG INFSO" .
ns7:infso_h	rdf:type	ns10:Breakdown ,
		skos:Concept ;
	skos:notation	"infso_h" ;
	skos:topConceptOf	ns1:breakdown ;
	ns11:membership	ns61:infso_h ;
	skos:altLabel	"Directorate H" ;
	skos:prefLabel	"Directorate H, DG INFSO" .
ns7:infso_r	rdf:type	ns10:Breakdown ,
		skos:Concept ;
	skos:notation	"infso_r" ;
	skos:topConceptOf	ns1:breakdown ;
	ns11:membership	ns61:infso_r ;
	skos:altLabel	"Directorate R" ;
	skos:prefLabel	"Directorate R, DG INFSO" .
ns7:l_c10_f43	rdf:type	ns10:Breakdown ,
		skos:Concept ;
	skos:notation	"L_C10_F43" ;
	skos:topConceptOf	ns1:breakdown ;
	ns11:membership	ns56:l_c10_f43 ;
	skos:altLabel	"Large enterprises in manufacturing, electricity, gaz; water supply and construction" ;
	skos:prefLabel	"Large enterprises in manufacturing, electricity, gaz; water supply and construction" .
ns7:l_c10_s951_xk	rdf:type	ns10:Breakdown ,
		skos:Concept ;
	skos:notation	"L_C10_S951_XK" ;
	skos:topConceptOf	ns1:breakdown ;
	ns11:membership	ns26:l_c10_s951_xk ,
		ns25:l_c10_s951_xk ;
	skos:altLabel	"Large enterprises" ;
	skos:prefLabel	"Large enterprises (250 persons employed or more), without financial sector" .
ns7:l_g45_s951_xk	rdf:type	ns10:Breakdown ,
		skos:Concept ;
	skos:notation	"L_G45_S951_XK" ;
	skos:topConceptOf	ns1:breakdown ;
	ns11:membership	ns56:l_g45_s951_xk ;
	skos:altLabel	"Large enterprises in services, without financial" ;
	skos:prefLabel	"Large enterprises in services, without financial" .
ns7:lose_find_job	rdf:type	ns10:Breakdown ,
		skos:Concept ;
	skos:notation	"lose_find_job" ;
	skos:definition	"eGovernment services related to the life event: Losing and Finding a Job" ;
	skos:topConceptOf	ns1:breakdown ;
	ns11:membership	ns57:lose_find_job ;
	skos:altLabel	"Losing and Finding a Job" ;
	skos:prefLabel	"Losing and Finding a Job Life Event" .
ns7:m	rdf:type	ns10:Breakdown ,
		skos:Concept ;
	skos:notation	"M" ;
	skos:topConceptOf	ns1:breakdown ;
	ns11:membership	ns28:m ;
	skos:altLabel	"Males" ;
	skos:prefLabel	"Males" .
ns7:m_c10_f43	rdf:type	ns10:Breakdown ,
		skos:Concept ;
	skos:notation	"M_C10_F43" ;
	skos:topConceptOf	ns1:breakdown ;
	ns11:membership	ns56:m_c10_f43 ;
	skos:altLabel	"Medium enterprises in manufacturing, electricity, gaz; water supply and construction" ;
	skos:prefLabel	"Medium enterprises in manufacturing, electricity, gaz; water supply and construction" .
ns7:m_c10_s951_xk	rdf:type	ns10:Breakdown ,
		skos:Concept ;
	skos:notation	"M_C10_S951_XK" ;
	skos:topConceptOf	ns1:breakdown ;
	ns11:membership	ns26:m_c10_s951_xk ;
	skos:altLabel	"Medium enterprises" ;
	skos:prefLabel	"Medium enterprises (50-249 persons employed), without financial sector" .
ns7:m_g45_s951_xk	rdf:type	ns10:Breakdown ,
		skos:Concept ;
	skos:notation	"M_G45_S951_XK" ;
	skos:topConceptOf	ns1:breakdown ;
	ns11:membership	ns56:m_g45_s951_xk ;
	skos:altLabel	"Medium enterprises in services, without financial" ;
	skos:prefLabel	"Medium enterprises in services, without financial" .
ns7:m_y16_74	rdf:type	ns10:Breakdown ,
		skos:Concept ;
	rdfs:seeAlso	ns68:M_Y16_74 ;
	skos:notation	"M_Y16_74" ;
	skos:topConceptOf	ns1:breakdown ;
	ns11:membership	ns28:m_y16_74 ;
	skos:altLabel	"Males" ;
	skos:prefLabel	"Males, 16 to 74 years old" .
ns7:not_assigned	rdf:type	ns10:Breakdown ,
		skos:Concept ;
	skos:notation	"Not_assigned" ;
	skos:topConceptOf	ns1:breakdown ;
	ns11:membership	ns63:not_assigned ;
	skos:prefLabel	"Total not assigned due to lack of demand" .
ns7:offer_100_mbps	rdf:type	ns10:Breakdown ,
		skos:Concept ;
	skos:notation	"offer_100_Mbps" ;
	skos:definition	"Offers with a maximum advertised download speed above 100 Mbps" ;
	skos:topConceptOf	ns1:breakdown ;
	ns11:membership	ns21:offer_100_mbps ;
	skos:altLabel	"Advertised download speed above 100 Mbps" ;
	skos:prefLabel	"Advertised download speed above 100 Mbps" .
ns7:offer_12_30_mbps	rdf:type	ns10:Breakdown ,
		skos:Concept ;
	skos:notation	"offer_12_30_Mbps" ;
	skos:definition	"Offers with a maximum advertised download speed above 12 and up to 30 Mbps (Iincluded)" ;
	skos:topConceptOf	ns1:breakdown ;
	ns11:membership	ns21:offer_12_30_mbps ;
	skos:altLabel	"Advertised download speed above 12 and up to 30 Mbps" ;
	skos:prefLabel	"Advertised download speed above 12 and up to 30 Mbps" .
ns7:offer_30_100_mbps	rdf:type	ns10:Breakdown ,
		skos:Concept ;
	skos:notation	"offer_30_100_Mbps" ;
	skos:definition	"Offers with a maximum advertised download speed above 30 and up to 100 Mbps (included)" ;
	skos:topConceptOf	ns1:breakdown ;
	ns11:membership	ns21:offer_30_100_mbps ;
	skos:altLabel	"Advertised download speed above 30 and up to 100 Mbps" ;
	skos:prefLabel	"Advertised download speed above 30 and up to 100 Mbps" .
ns7:offer_30_mbps	rdf:type	ns10:Breakdown ,
		skos:Concept ;
	skos:notation	"offer_30_Mbps" ;
	skos:definition	"Offers with a maximum advertised download speed of at least 30 Mbps or above." ;
	skos:topConceptOf	ns1:breakdown ;
	ns11:membership	ns20:offer_30_mbps ;
	skos:altLabel	"Advertised download equal or above 30 Mbps" ;
	skos:prefLabel	"Advertised download speed of 30 Mbps or above" .
ns7:offer_8_12_mbps	rdf:type	ns10:Breakdown ,
		skos:Concept ;
	skos:notation	"offer_8_12_Mbps" ;
	skos:definition	"Offers with a maximum advertised download speed above 8 and up to 12 Mbps (included)" ;
	skos:topConceptOf	ns1:breakdown ;
	ns11:membership	ns21:offer_8_12_mbps ;
	skos:altLabel	"Advertised download speed above 8 and up to 12 Mbps" ;
	skos:prefLabel	"Advertised download speed above 8 and up to 12 Mbps" .
ns7:orgclass_hesrec	rdf:type	ns10:Breakdown ,
		skos:Concept ;
	skos:notation	"orgclass_hesrec" ;
	skos:definition	"Public or private higher education institutions and not for profit research organisations (HES/REC)." ;
	skos:topConceptOf	ns1:breakdown ;
	ns11:membership	ns29:orgclass_hesrec ;
	skos:altLabel	"Higher education/research org." ;
	skos:prefLabel	"Higher education and non-profit research organisations" .
ns7:orgclass_le	rdf:type	ns10:Breakdown ,
		skos:Concept ;
	skos:notation	"orgclass_le" ;
	skos:definition	"Large enterprises with more than 250 employed persons or a turnover \u2265 50 millions euro and a balance sheet total \u2265 43 millions euro. " ;
	skos:topConceptOf	ns1:breakdown ;
	ns11:membership	ns29:orgclass_le ;
	skos:altLabel	"Large enterprises" ;
	skos:prefLabel	"Large enterprises" .
ns7:orgclass_nil	rdf:type	ns10:Breakdown ,
		skos:Concept ;
	skos:notation	"orgclass_nil" ;
	skos:definition	"All other types of organisations (i.e. public administrations, NGO, public sector enterprises, etc.) (NIL)." ;
	skos:topConceptOf	ns1:breakdown ;
	ns11:membership	ns29:orgclass_nil ;
	skos:altLabel	"Other organizations" ;
	skos:prefLabel	"Other organizations" .
ns7:orgclass_sme	rdf:type	ns10:Breakdown ,
		skos:Concept ;
	skos:notation	"orgclass_sme" ;
	skos:definition	"Small and medium individual private enterprises (SME) with less than 250 employed persons and a turnover \u2264 50 millions euro or a balance sheet total \u2264 43 millions euro. " ;
	skos:topConceptOf	ns1:breakdown ;
	ns11:membership	ns29:orgclass_sme ;
	skos:altLabel	"SME" ;
	skos:prefLabel	"Small and medium enterprises" .
ns7:orgclass_total	rdf:type	ns10:Breakdown ,
		skos:Concept ;
	skos:notation	"orgclass_total" ;
	skos:topConceptOf	ns1:breakdown ;
	ns11:membership	ns67:orgclass_total ;
	skos:altLabel	"All organizations" ;
	skos:prefLabel	"All organizations" .
ns7:other_eu_countries	rdf:type	ns10:Breakdown ,
		skos:Concept ;
	skos:notation	"Other_EU_countries" ;
	skos:topConceptOf	ns1:breakdown ;
	ns11:membership	ns9:other_eu_countries ;
	skos:altLabel	"Customers, other EU countries" ;
	skos:prefLabel	"Customers, other EU countries" .
ns7:own_country	rdf:type	ns10:Breakdown ,
		skos:Concept ;
	skos:notation	"Own_country" ;
	skos:topConceptOf	ns1:breakdown ;
	ns11:membership	ns9:own_country ;
	skos:altLabel	"Customers, own country" ;
	skos:prefLabel	"Customers, own country" .
ns7:own_drive_car	rdf:type	ns10:Breakdown ,
		skos:Concept ;
	skos:notation	"own_drive_car" ;
	skos:definition	"eGovernment services related to the life event: Owning and driving a car" ;
	skos:topConceptOf	ns1:breakdown ;
	ns11:membership	ns57:own_drive_car ;
	skos:altLabel	"Owning and driving a car" ;
	skos:prefLabel	"Owning and driving a car Life Event" .
ns7:reg_bus_op	rdf:type	ns10:Breakdown ,
		skos:Concept ;
	skos:notation	"reg_bus_op" ;
	skos:definition	"eGovernment services related to the life event: Regular business operations" ;
	skos:topConceptOf	ns1:breakdown ;
	ns11:membership	ns57:reg_bus_op ;
	skos:altLabel	"Regular business operations" ;
	skos:prefLabel	"Regular business operations Life Event" .
ns7:rest_world	rdf:type	ns10:Breakdown ,
		skos:Concept ;
	skos:notation	"Rest_world" ;
	skos:topConceptOf	ns1:breakdown ;
	ns11:membership	ns9:rest_world ;
	skos:altLabel	"Customers, rest of the world" ;
	skos:prefLabel	"Customers, rest of the world" .
ns7:retir_other	rdf:type	ns10:Breakdown ,
		skos:Concept ;
	rdfs:seeAlso	ns68:RETIR_OTHER ;
	skos:notation	"RETIR_OTHER" ;
	skos:topConceptOf	ns1:breakdown ;
	ns11:membership	ns24:retir_other ;
	skos:altLabel	"Retired and inactive" ;
	skos:prefLabel	"Retired and other inactive" .
ns7:rf_0	rdf:type	ns10:Breakdown ,
		skos:Concept ;
	rdfs:seeAlso	<http://epp.eurostat.ec.europa.eu/portal/page/portal/information_society/documents/Tab/Breakdowns%20summary%20HH%202003-2011.pdf> ;
	skos:notation	"rf_0" ;
	skos:definition	"Individuals with none of the 3 following characteristics: 55 to 74 years old; low education; unemployed or inactive or retired" ;
	skos:topConceptOf	ns1:breakdown ;
	ns11:membership	ns31:rf_0 ;
	skos:altLabel	"No disadvantage factor" ;
	skos:prefLabel	"Individuals with no disadvantage factor" .
ns7:rf_ge1	rdf:type	ns10:Breakdown ,
		skos:Concept ;
	rdfs:seeAlso	ns68:RF_GE1 ;
	skos:notation	"rf_ge1" ;
	skos:definition	"Individuals with at least one of the 3 following characteristics: 55 to 74 years old; low education; unemployed or inactive or retired" ;
	skos:topConceptOf	ns1:breakdown ;
	ns11:membership	ns31:rf_ge1 ;
	skos:altLabel	"At least 1 disadvantage factor" ;
	skos:prefLabel	"Individuals with at least 1 disadvantage factor" .
ns7:rf_ge2	rdf:type	ns10:Breakdown ,
		skos:Concept ;
	rdfs:seeAlso	ns68:RF_GE2 ;
	skos:notation	"rf_ge2" ;
	skos:definition	"Individuals with at least two of the 3 following characteristics: 55 to 74 years old; low education; unemployed or inactive or retired" ;
	skos:topConceptOf	ns1:breakdown ;
	ns11:membership	ns31:rf_ge2 ;
	skos:altLabel	"At least 2 disadvantage factors" ;
	skos:prefLabel	"Individuals with at least 2 disadvantage factor" .
ns7:rural_pop	rdf:type	ns10:Breakdown ,
		skos:Concept ;
	skos:notation	"RURAL_POP" ;
	skos:topConceptOf	ns1:breakdown ;
	ns11:membership	ns65:rural_pop ;
	skos:altLabel	"Rural population" ;
	skos:prefLabel	"Rural population" .
ns7:s_c10_f43	rdf:type	ns10:Breakdown ,
		skos:Concept ;
	skos:notation	"S_C10_F43" ;
	skos:topConceptOf	ns1:breakdown ;
	ns11:membership	ns56:s_c10_f43 ;
	skos:altLabel	"Small enterprises in manufacturing, electricity, gaz; water supply and construction" ;
	skos:prefLabel	"Small enterprises in manufacturing, electricity, gaz; water supply and construction" .
ns7:s_c10_s951_xk	rdf:type	ns10:Breakdown ,
		skos:Concept ;
	skos:notation	"S_C10_S951_XK" ;
	skos:topConceptOf	ns1:breakdown ;
	ns11:membership	ns26:s_c10_s951_xk ;
	skos:altLabel	"Small enterprises" ;
	skos:prefLabel	"Small enterprises (10-49 persons employed), without financial sector" .
ns7:s_g45_s951_xk	rdf:type	ns10:Breakdown ,
		skos:Concept ;
	skos:notation	"S_G45_S951_XK" ;
	skos:topConceptOf	ns1:breakdown ;
	ns11:membership	ns56:s_g45_s951_xk ;
	skos:altLabel	"Small enterprises in services, without financial" ;
	skos:prefLabel	"Small enterprises in services, without financial" .
ns7:sal_self_fam	rdf:type	ns10:Breakdown ,
		skos:Concept ;
	rdfs:seeAlso	ns68:SAL_SELF_FAM ;
	skos:notation	"SAL_SELF_FAM" ;
	skos:topConceptOf	ns1:breakdown ;
	ns11:membership	ns24:sal_self_fam ;
	skos:altLabel	"Employees, self-employed, family workers" ;
	skos:prefLabel	"Employees, self-employed, family workers" .
ns7:services	rdf:type	ns10:Breakdown ,
		skos:Concept ;
	skos:notation	"services" ;
	skos:topConceptOf	ns1:breakdown ;
	ns11:membership	ns33:services ;
	skos:altLabel	"Services" ;
	skos:prefLabel	"Services" .
ns7:sm_c10_s951_xk	rdf:type	ns10:Breakdown ,
		skos:Concept ;
	skos:notation	"SM_C10_S951_XK" ;
	skos:topConceptOf	ns1:breakdown ;
	ns11:membership	ns25:sm_c10_s951_xk ;
	skos:altLabel	"SMEs (10-249 persons employed)" ;
	skos:prefLabel	"SMEs (10-249 persons employed), without financial sector" .
ns7:small_claims	rdf:type	ns10:Breakdown ,
		skos:Concept ;
	skos:notation	"small_claims" ;
	skos:definition	"eGovernment services related to the life event: Starting a Small Claims procedure" ;
	skos:topConceptOf	ns1:breakdown ;
	ns11:membership	ns57:small_claims ;
	skos:altLabel	"Starting a Small Claims procedure" ;
	skos:prefLabel	"Starting a Small Claims procedure Life Event" .
ns7:so_01	rdf:type	ns10:Breakdown ,
		skos:Concept ;
	skos:notation	"SO_01" ;
	skos:topConceptOf	ns1:breakdown ;
	ns11:membership	ns66:so_01 ;
	skos:altLabel	"SO 01" ;
	skos:prefLabel	"01 Future Networks and Internet" .
ns7:so_02	rdf:type	ns10:Breakdown ,
		skos:Concept ;
	skos:notation	"SO_02" ;
	skos:topConceptOf	ns1:breakdown ;
	ns11:membership	ns66:so_02 ;
	skos:altLabel	"SO 02" ;
	skos:prefLabel	"02 Software, Services and internet connected objects" .
ns7:so_03	rdf:type	ns10:Breakdown ,
		skos:Concept ;
	skos:notation	"SO_03" ;
	skos:topConceptOf	ns1:breakdown ;
	ns11:membership	ns66:so_03 ;
	skos:altLabel	"SO 03" ;
	skos:prefLabel	"03 Trustworthy ICT" .
ns7:so_04	rdf:type	ns10:Breakdown ,
		skos:Concept ;
	skos:notation	"SO_04" ;
	skos:topConceptOf	ns1:breakdown ;
	ns11:membership	ns66:so_04 ;
	skos:altLabel	"SO 04" ;
	skos:prefLabel	"04 Networked Media" .
ns7:so_05	rdf:type	ns10:Breakdown ,
		skos:Concept ;
	skos:notation	"SO_05" ;
	skos:topConceptOf	ns1:breakdown ;
	ns11:membership	ns66:so_05 ;
	skos:altLabel	"SO 05" ;
	skos:prefLabel	"05 Cognitive Systems and Robotics" .
ns7:so_06	rdf:type	ns10:Breakdown ,
		skos:Concept ;
	skos:notation	"SO_06" ;
	skos:topConceptOf	ns1:breakdown ;
	ns11:membership	ns66:so_06 ;
	skos:altLabel	"SO 06" ;
	skos:prefLabel	"06 Nanoelectronics" .
ns7:so_07	rdf:type	ns10:Breakdown ,
		skos:Concept ;
	skos:notation	"SO_07" ;
	skos:topConceptOf	ns1:breakdown ;
	ns11:membership	ns66:so_07 ;
	skos:altLabel	"SO 07" ;
	skos:prefLabel	"07 Micro/nanosystems" .
ns7:so_08	rdf:type	ns10:Breakdown ,
		skos:Concept ;
	skos:notation	"SO_08" ;
	skos:topConceptOf	ns1:breakdown ;
	ns11:membership	ns66:so_08 ;
	skos:altLabel	"SO 08" ;
	skos:prefLabel	"08 Embedded Systems" .
ns7:so_09	rdf:type	ns10:Breakdown ,
		skos:Concept ;
	skos:notation	"SO_09" ;
	skos:topConceptOf	ns1:breakdown ;
	ns11:membership	ns66:so_09 ;
	skos:altLabel	"SO 09" ;
	skos:prefLabel	"09 Photonics" .
ns7:so_10	rdf:type	ns10:Breakdown ,
		skos:Concept ;
	skos:notation	"SO_10" ;
	skos:topConceptOf	ns1:breakdown ;
	ns11:membership	ns66:so_10 ;
	skos:altLabel	"SO 10" ;
	skos:prefLabel	"10 Organic and large area Electronics" .
ns7:so_11	rdf:type	ns10:Breakdown ,
		skos:Concept ;
	skos:notation	"SO_11" ;
	skos:topConceptOf	ns1:breakdown ;
	ns11:membership	ns66:so_11 ;
	skos:altLabel	"SO 11" ;
	skos:prefLabel	"11 Language Technologies" .
ns7:so_12	rdf:type	ns10:Breakdown ,
		skos:Concept ;
	skos:notation	"SO_12" ;
	skos:topConceptOf	ns1:breakdown ;
	ns11:membership	ns66:so_12 ;
	skos:altLabel	"SO 12" ;
	skos:prefLabel	"12 Intelligent Information Management" .
ns7:so_13	rdf:type	ns10:Breakdown ,
		skos:Concept ;
	skos:notation	"SO_13" ;
	skos:topConceptOf	ns1:breakdown ;
	ns11:membership	ns66:so_13 ;
	skos:altLabel	"SO 13" ;
	skos:prefLabel	"13 ICT for Health" .
ns7:so_14	rdf:type	ns10:Breakdown ,
		skos:Concept ;
	skos:notation	"SO_14" ;
	skos:topConceptOf	ns1:breakdown ;
	ns11:membership	ns66:so_14 ;
	skos:altLabel	"SO 14" ;
	skos:prefLabel	"14 ICT and Ageing" .
ns7:so_15	rdf:type	ns10:Breakdown ,
		skos:Concept ;
	skos:notation	"SO_15" ;
	skos:topConceptOf	ns1:breakdown ;
	ns11:membership	ns66:so_15 ;
	skos:altLabel	"SO 15" ;
	skos:prefLabel	"15 ICT for Inclusion" .
ns7:so_16	rdf:type	ns10:Breakdown ,
		skos:Concept ;
	skos:notation	"SO_16" ;
	skos:topConceptOf	ns1:breakdown ;
	ns11:membership	ns66:so_16 ;
	skos:altLabel	"SO 16" ;
	skos:prefLabel	"16 ICT for Governance and Policy Modelling" .
ns7:so_17	rdf:type	ns10:Breakdown ,
		skos:Concept ;
	skos:notation	"SO_17" ;
	skos:topConceptOf	ns1:breakdown ;
	ns11:membership	ns66:so_17 ;
	skos:altLabel	"SO 17" ;
	skos:prefLabel	"17 ICT for Energy Efficiency" .
ns7:so_18	rdf:type	ns10:Breakdown ,
		skos:Concept ;
	skos:notation	"SO_18" ;
	skos:topConceptOf	ns1:breakdown ;
	ns11:membership	ns66:so_18 ;
	skos:altLabel	"SO 18" ;
	skos:prefLabel	"18 ICT for Transport" .
ns7:so_19	rdf:type	ns10:Breakdown ,
		skos:Concept ;
	skos:notation	"SO_19" ;
	skos:topConceptOf	ns1:breakdown ;
	ns11:membership	ns66:so_19 ;
	skos:altLabel	"SO 19" ;
	skos:prefLabel	"19 ICT for the Enterprise" .
ns7:so_20	rdf:type	ns10:Breakdown ,
		skos:Concept ;
	skos:notation	"SO_20" ;
	skos:topConceptOf	ns1:breakdown ;
	ns11:membership	ns66:so_20 ;
	skos:altLabel	"SO 20" ;
	skos:prefLabel	"20 ICT for Learning" .
ns7:so_21	rdf:type	ns10:Breakdown ,
		skos:Concept ;
	skos:notation	"SO_21" ;
	skos:topConceptOf	ns1:breakdown ;
	ns11:membership	ns66:so_21 ;
	skos:altLabel	"SO 21" ;
	skos:prefLabel	"21 Digital Libraries" .
ns7:so_22_1	rdf:type	ns10:Breakdown ,
		skos:Concept ;
	skos:notation	"SO_22_1" ;
	skos:topConceptOf	ns1:breakdown ;
	ns11:membership	ns66:so_22_1 ;
	skos:altLabel	"SO 22.1" ;
	skos:prefLabel	"22.1 FET Open" .
ns7:so_22_2	rdf:type	ns10:Breakdown ,
		skos:Concept ;
	skos:notation	"SO_22_2" ;
	skos:topConceptOf	ns1:breakdown ;
	ns11:membership	ns66:so_22_2 ;
	skos:altLabel	"SO 22.2" ;
	skos:prefLabel	"22.2 FET Proactive" .
ns7:so_22_3	rdf:type	ns10:Breakdown ,
		skos:Concept ;
	skos:notation	"SO_22_3" ;
	skos:topConceptOf	ns1:breakdown ;
	ns11:membership	ns66:so_22_3 ;
	skos:altLabel	"SO 22.3" ;
	skos:prefLabel	"22.3 FET Flagship" .
ns7:so_23	rdf:type	ns10:Breakdown ,
		skos:Concept ;
	skos:notation	"SO_23" ;
	skos:topConceptOf	ns1:breakdown ;
	ns11:membership	ns66:so_23 ;
	skos:altLabel	"SO 23" ;
	skos:prefLabel	"23 International Cooperation" .
ns7:so_24	rdf:type	ns10:Breakdown ,
		skos:Concept ;
	skos:notation	"SO_24" ;
	skos:topConceptOf	ns1:breakdown ;
	ns11:membership	ns66:so_24 ;
	skos:altLabel	"SO 24" ;
	skos:prefLabel	"24 Accompanying Measures" .
ns7:so_25	rdf:type	ns10:Breakdown ,
		skos:Concept ;
	skos:notation	"SO_25" ;
	skos:topConceptOf	ns1:breakdown ;
	ns11:membership	ns66:so_25 ;
	skos:altLabel	"SO 25" ;
	skos:prefLabel	"25 Big Data" .
ns7:so_26	rdf:type	ns10:Breakdown ,
		skos:Concept ;
	skos:notation	"SO_26" ;
	skos:topConceptOf	ns1:breakdown ;
	ns11:membership	ns66:so_26 ;
	skos:altLabel	"SO 26" ;
	skos:prefLabel	"26 Creativity" .
ns7:speed_10l30	rdf:type	ns10:Breakdown ,
		skos:Concept ;
	skos:notation	"speed_10l30" ;
	skos:definition	"Based on the advertised download speed" ;
	skos:topConceptOf	ns1:breakdown ;
	ns11:membership	ns20:speed_10l30 ;
	skos:altLabel	"at least 10 but below 30 Mbps" ;
	skos:prefLabel	"at least 10 but below 30 Mbps" .
ns7:speed_2l10	rdf:type	ns10:Breakdown ,
		skos:Concept ;
	skos:notation	"speed_2l10" ;
	skos:definition	"Based on the advertised download speed" ;
	skos:topConceptOf	ns1:breakdown ;
	ns11:membership	ns20:speed_2l10 ;
	skos:altLabel	"at least 2 but below 10 Mbps" ;
	skos:prefLabel	"at least 2 but below 10 Mbps" .
ns7:speed_30l100	rdf:type	ns10:Breakdown ,
		skos:Concept ;
	skos:notation	"speed_30l100" ;
	skos:definition	"Based on the advertised download speed" ;
	skos:topConceptOf	ns1:breakdown ;
	ns11:membership	ns20:speed_30l100 ;
	skos:altLabel	"at least 30 but below 100 Mbps" ;
	skos:prefLabel	"at least 30 but below 100 Mbps" .
ns7:speed_ge100	rdf:type	ns10:Breakdown ,
		skos:Concept ;
	skos:notation	"speed_ge100" ;
	skos:definition	"Based on the advertised download speed" ;
	skos:topConceptOf	ns1:breakdown ;
	ns11:membership	ns20:speed_ge100 ;
	skos:altLabel	"above 100 Mbps" ;
	skos:prefLabel	"above 100 Mbps" .
ns7:speed_l2	rdf:type	ns10:Breakdown ,
		skos:Concept ;
	skos:notation	"speed_l2" ;
	skos:definition	"Based on the advertised download speed" ;
	skos:topConceptOf	ns1:breakdown ;
	ns11:membership	ns20:speed_l2 ;
	skos:altLabel	"below 2 Mbps" ;
	skos:prefLabel	"below 2 Mbps" .
ns7:stud	rdf:type	ns10:Breakdown ,
		skos:Concept ;
	rdfs:seeAlso	ns68:STUD ;
	skos:notation	"STUD" ;
	skos:topConceptOf	ns1:breakdown ;
	ns11:membership	ns24:stud ;
	skos:altLabel	"Students" ;
	skos:prefLabel	"Students" .
ns7:study	rdf:type	ns10:Breakdown ,
		skos:Concept ;
	skos:notation	"study" ;
	skos:definition	"eGovernment services related to the life event: Studying" ;
	skos:topConceptOf	ns1:breakdown ;
	ns11:membership	ns57:study ;
	skos:altLabel	"Studying" ;
	skos:prefLabel	"Studying Life Event" .
ns7:tot_ict_products	rdf:type	ns10:Breakdown ,
		skos:Concept ;
	skos:notation	"tot_ict_products" ;
	skos:definition	"Scope: Total of ICT products (goods and services)" ;
	skos:topConceptOf	ns1:breakdown ;
	ns11:membership	ns67:tot_ict_products ;
	skos:altLabel	"Total" ;
	skos:prefLabel	"Total" .
ns7:total	rdf:type	ns10:Breakdown ,
		skos:Concept ;
	skos:notation	"TOTAL" ;
	skos:topConceptOf	ns1:breakdown ;
	ns11:membership	ns67:total ;
	skos:altLabel	"Total" ;
	skos:prefLabel	"Total" .
ns7:total_fbb	rdf:type	ns10:Breakdown ,
		skos:Concept ;
	skos:notation	"TOTAL_FBB" ;
	skos:definition	"Scope: Total number of fixed broadband subscriptions" ;
	skos:topConceptOf	ns1:breakdown ;
	ns11:membership	ns67:total_fbb ;
	skos:altLabel	"Total" ;
	skos:prefLabel	"Total" .
ns7:total_mbb	rdf:type	ns10:Breakdown ,
		skos:Concept ;
	skos:notation	"TOTAL_MBB" ;
	skos:definition	"Scope: Total number of mobile broadband subscriptions" ;
	skos:topConceptOf	ns1:breakdown ;
	ns11:membership	ns67:total_mbb ;
	skos:altLabel	"Total" ;
	skos:prefLabel	"Total" .
ns7:total_mob	rdf:type	ns10:Breakdown ,
		skos:Concept ;
	skos:notation	"TOTAL_MOB" ;
	skos:definition	"Scope: Total number of mobile subscriptions (SIM Cards)" ;
	skos:topConceptOf	ns1:breakdown ;
	ns11:membership	ns67:total_mob ;
	skos:altLabel	"Total" ;
	skos:prefLabel	"Total" .
ns7:total_offers8plus	rdf:type	ns10:Breakdown ,
		skos:Concept ;
	skos:notation	"total_offers8plus" ;
	skos:definition	"Offers with a maximum advertised download speed of at least 8 Mbps or above." ;
	skos:topConceptOf	ns1:breakdown ;
	ns11:membership	ns67:total_offers8plus ;
	skos:altLabel	"Advertised download equal or above 8 Mbps" ;
	skos:prefLabel	"Advertised download speed of 8 Mbps or above" .
ns7:total_pop	rdf:type	ns10:Breakdown ,
		skos:Concept ;
	skos:notation	"TOTAL_POP" ;
	skos:definition	"Scope: Total population" ;
	skos:topConceptOf	ns1:breakdown ;
	ns11:membership	ns67:total_pop ;
	skos:altLabel	"Total" ;
	skos:prefLabel	"Total" .
ns7:total_pophh	rdf:type	ns10:Breakdown ,
		skos:Concept ;
	skos:notation	"TOTAL_POPHH" ;
	skos:definition	"Scope: Total number of households" ;
	skos:topConceptOf	ns1:breakdown ;
	ns11:membership	ns67:total_pophh ;
	skos:altLabel	"Total" ;
	skos:prefLabel	"Total" .
ns7:total_sos	rdf:type	ns10:Breakdown ,
		skos:Concept ;
	skos:notation	"Total_SOs" ;
	skos:topConceptOf	ns1:breakdown ;
	ns11:membership	ns66:total_sos ;
	skos:altLabel	"All SOs" ;
	skos:prefLabel	"All Strategic Objectives and eInfrastructures" .
ns7:total_tel	rdf:type	ns10:Breakdown ,
		skos:Concept ;
	skos:notation	"TOTAL_TEL" ;
	skos:definition	"Scope: Total of the Electronic Communications sector" ;
	skos:topConceptOf	ns1:breakdown ;
	ns11:membership	ns67:total_tel ;
	skos:altLabel	"Total" ;
	skos:prefLabel	"Total" .
ns7:une	rdf:type	ns10:Breakdown ,
		skos:Concept ;
	rdfs:seeAlso	ns68:UNE ;
	skos:notation	"UNE" ;
	skos:topConceptOf	ns1:breakdown ;
	ns11:membership	ns24:une ;
	skos:altLabel	"Unemployed" ;
	skos:prefLabel	"Unemployed" .
ns7:xdsl	rdf:type	ns10:Breakdown ,
		skos:Concept ;
	skos:notation	"xdsl" ;
	skos:topConceptOf	ns1:breakdown ;
	ns11:membership	ns27:xdsl ;
	skos:altLabel	"xDSL technology" ;
	skos:prefLabel	"xDSL technology" .
ns7:y16_24	rdf:type	ns10:Breakdown ,
		skos:Concept ;
	rdfs:seeAlso	ns68:Y16_24 ;
	skos:notation	"Y16_24" ;
	skos:topConceptOf	ns1:breakdown ;
	ns11:membership	ns13:y16_24 ,
		ns14:y16_24 ;
	skos:altLabel	"16-24" ;
	skos:prefLabel	"Individuals, 16 to 24 years old" .
ns7:y25_34	rdf:type	ns10:Breakdown ,
		skos:Concept ;
	rdfs:seeAlso	ns68:Y25_34 ;
	skos:notation	"Y25_34" ;
	skos:topConceptOf	ns1:breakdown ;
	ns11:membership	ns14:y25_34 ;
	skos:altLabel	"25-34" ;
	skos:prefLabel	"Individuals, 25 to 34 years old" .
ns7:y25_64	rdf:type	ns10:Breakdown ,
		skos:Concept ;
	rdfs:seeAlso	ns68:Y25_64 ;
	skos:notation	"Y25_64" ;
	skos:topConceptOf	ns1:breakdown ;
	ns11:membership	ns64:y25_64 ;
	skos:altLabel	"25-64" ;
	skos:prefLabel	"Individuals, 25 to 64 years old" .
ns7:y35_44	rdf:type	ns10:Breakdown ,
		skos:Concept ;
	rdfs:seeAlso	ns68:Y35_44 ;
	skos:notation	"Y35_44" ;
	skos:topConceptOf	ns1:breakdown ;
	ns11:membership	ns14:y35_44 ;
	skos:altLabel	"35-44" ;
	skos:prefLabel	"Individuals, 35 to 44 years old" .
ns7:y45_54	rdf:type	ns10:Breakdown ,
		skos:Concept ;
	rdfs:seeAlso	ns68:Y45_54 ;
	skos:notation	"Y45_54" ;
	skos:topConceptOf	ns1:breakdown ;
	ns11:membership	ns14:y45_54 ;
	skos:altLabel	"45-54" ;
	skos:prefLabel	"Individuals, 45 to 54 years old" .
ns7:y55_64	rdf:type	ns10:Breakdown ,
		skos:Concept ;
	rdfs:seeAlso	ns68:Y55_64 ;
	skos:notation	"Y55_64" ;
	skos:topConceptOf	ns1:breakdown ;
	ns11:membership	ns14:y55_64 ;
	skos:altLabel	"55-64" ;
	skos:prefLabel	"Individuals, 55 to 64 years old" .
ns7:y55_74	rdf:type	ns10:Breakdown ,
		skos:Concept ;
	rdfs:seeAlso	ns68:Y55_74 ;
	skos:notation	"Y55_74" ;
	skos:topConceptOf	ns1:breakdown ;
	ns11:membership	ns13:y55_74 ;
	skos:altLabel	"55-74" ;
	skos:prefLabel	"Individuals, 55 to 74 years old" .
ns7:y65_74	rdf:type	ns10:Breakdown ,
		skos:Concept ;
	rdfs:seeAlso	ns68:Y65_74 ;
	skos:notation	"Y65_74" ;
	skos:topConceptOf	ns1:breakdown ;
	ns11:membership	ns14:y65_74 ;
	skos:altLabel	"65-74" ;
	skos:prefLabel	"Individuals, 65 to 74 years old" .
<http://semantic.digital-agenda-data.eu/codelist/breakdown/10_d35_e39>	rdf:type	ns10:Breakdown ,
		skos:Concept ;
	skos:notation	"10_D35_E39" ;
	skos:topConceptOf	ns1:breakdown ;
	ns11:membership	<http://semantic.digital-agenda-data.eu/codelist/breakdown-group/econsector/10_d35_e39> ;
	skos:altLabel	"Electricity, gas, steam, air conditioning; water supply, sewerage, waste management&remediation 10+" ;
	skos:prefLabel	"Electricity, gas, steam, air conditioning; water supply, sewerage, waste management&remediation 10+" .
<http://semantic.digital-agenda-data.eu/codelist/breakdown/10_g45>	rdf:type	ns10:Breakdown ,
		skos:Concept ;
	skos:notation	"10_G45" ;
	skos:topConceptOf	ns1:breakdown ;
	ns11:membership	<http://semantic.digital-agenda-data.eu/codelist/breakdown-group/econsector/10_g45> ;
	skos:altLabel	"Trade of motor vehicles and motorcycles 10+" ;
	skos:prefLabel	"Trade of motor vehicles and motorcycles 10+" .
ns7:y25_54	rdf:type	ns10:Breakdown ,
		skos:Concept ;
	rdfs:seeAlso	ns68:Y25_54 ;
	skos:notation	"Y25_54" ;
	skos:topConceptOf	ns1:breakdown ;
	ns11:membership	ns13:y25_54 ;
	skos:altLabel	"25-54" ;
	skos:prefLabel	"Individuals, 25 to 54 years old" .
ns7:csk_me	rdf:type	ns10:Breakdown ,
		skos:Concept ;
	rdfs:seeAlso	ns69:I_CSK_ME ;
	skos:notation	"csk_me" ;
	skos:definition	"Individuals having ever carried out 3 or 4 of the following 6 activities: coping or moving a file or folder, using copy and paste tools, using basic arithmetic formula in a spreadsheet, compressing (or zipping) files, connecting and installing new devices, writing a computer program using a specialised programming language. Only those having ever used a computer were proposed the question." ;
	skos:topConceptOf	ns1:breakdown ;
	ns11:membership	ns32:csk_me ;
	skos:altLabel	"medium computer skills" ;
	skos:prefLabel	"Individuals with medium computer skills" .
@prefix ns70:	<http://semantic.digital-agenda-data.eu/codelist/breakdown-group/e_gov_1_ucg/> .
ns70:e_gov_1a_ucg_oa	rdf:type	ns10:BreakdownToGroupMembership ;
	rdfs:label	"e_gov_1_UCG" ;
	ns11:member-of	ns12:e_gov_1_ucg ;
	ns11:order	"1" .
ns70:e_gov_1b_ucg_us	rdf:type	ns10:BreakdownToGroupMembership ;
	rdfs:label	"e_gov_1_UCG" ;
	ns11:member-of	ns12:e_gov_1_ucg ;
	ns11:order	"2" .
ns70:e_gov_1c_ucg_mf	rdf:type	ns10:BreakdownToGroupMembership ;
	rdfs:label	"e_gov_1_UCG" ;
	ns11:member-of	ns12:e_gov_1_ucg ;
	ns11:order	"3" .
ns70:e_gov_1d_ucg_eu	rdf:type	ns10:BreakdownToGroupMembership ;
	rdfs:label	"e_gov_1_UCG" ;
	ns11:member-of	ns12:e_gov_1_ucg ;
	ns11:order	"4" .
ns70:e_gov_1e_ucg_su	rdf:type	ns10:BreakdownToGroupMembership ;
	rdfs:label	"e_gov_1_UCG" ;
	ns11:member-of	ns12:e_gov_1_ucg ;
	ns11:order	"5" .
@prefix ns71:	<http://semantic.digital-agenda-data.eu/codelist/breakdown-group/e_gov_2_tg/> .
ns71:e_gov_2a_tg_sd	rdf:type	ns10:BreakdownToGroupMembership ;
	rdfs:label	"e_gov_2_TG" ;
	ns11:member-of	ns12:e_gov_2_tg ;
	ns11:order	"1" .
ns71:e_gov_2b_tg_po	rdf:type	ns10:BreakdownToGroupMembership ;
	rdfs:label	"e_gov_2_TG" ;
	ns11:member-of	ns12:e_gov_2_tg ;
	ns11:order	"2" .
ns71:e_gov_2c_tg_pd	rdf:type	ns10:BreakdownToGroupMembership ;
	rdfs:label	"e_gov_2_TG" ;
	ns11:member-of	ns12:e_gov_2_tg ;
	ns11:order	"3" .
@prefix ns72:	<http://semantic.digital-agenda-data.eu/codelist/breakdown-group/e_gov_3_cm/> .
ns72:e_gov_3a_cm_oa	rdf:type	ns10:BreakdownToGroupMembership ;
	rdfs:label	"e_gov_3_CM" ;
	ns11:member-of	ns12:e_gov_3_cm ;
	ns11:order	"1" .
ns72:e_gov_3b_cm_us	rdf:type	ns10:BreakdownToGroupMembership ;
	rdfs:label	"e_gov_3_CM" ;
	ns11:member-of	ns12:e_gov_3_cm ;
	ns11:order	"2" .
ns72:e_gov_3c_cm_eidcb	rdf:type	ns10:BreakdownToGroupMembership ;
	rdfs:label	"e_gov_3_CM" ;
	ns11:member-of	ns12:e_gov_3_cm ;
	ns11:order	"3" .
ns72:e_gov_3d_cm_edoccb	rdf:type	ns10:BreakdownToGroupMembership ;
	rdfs:label	"e_gov_3_CM" ;
	ns11:member-of	ns12:e_gov_3_cm ;
	ns11:order	"4" .
ns72:e_gov_3e_cm_eu	rdf:type	ns10:BreakdownToGroupMembership ;
	rdfs:label	"e_gov_3_CM" ;
	ns11:member-of	ns12:e_gov_3_cm ;
	ns11:order	"5" .
ns72:e_gov_3f_cm_su	rdf:type	ns10:BreakdownToGroupMembership ;
	rdfs:label	"e_gov_3_CM" ;
	ns11:member-of	ns12:e_gov_3_cm ;
	ns11:order	"6" .
@prefix ns73:	<http://semantic.digital-agenda-data.eu/codelist/breakdown-group/e_gov_4_bm/> .
ns73:e_gov_4a_bm_oa	rdf:type	ns10:BreakdownToGroupMembership ;
	rdfs:label	"e_gov_4_BM" ;
	ns11:member-of	ns12:e_gov_4_bm ;
	ns11:order	"1" .
ns73:e_gov_4b_bm_us	rdf:type	ns10:BreakdownToGroupMembership ;
	rdfs:label	"e_gov_4_BM" ;
	ns11:member-of	ns12:e_gov_4_bm ;
	ns11:order	"2" .
ns73:e_gov_4c_bm_eidcb	rdf:type	ns10:BreakdownToGroupMembership ;
	rdfs:label	"e_gov_4_BM" ;
	ns11:member-of	ns12:e_gov_4_bm ;
	ns11:order	"3" .
ns73:e_gov_4d_bm_edoccb	rdf:type	ns10:BreakdownToGroupMembership ;
	rdfs:label	"e_gov_4_BM" ;
	ns11:member-of	ns12:e_gov_4_bm ;
	ns11:order	"4" .
ns73:e_gov_4e_bm_eu	rdf:type	ns10:BreakdownToGroupMembership ;
	rdfs:label	"e_gov_4_BM" ;
	ns11:member-of	ns12:e_gov_4_bm ;
	ns11:order	"5" .
ns73:e_gov_4f_bm_su	rdf:type	ns10:BreakdownToGroupMembership ;
	rdfs:label	"e_gov_4_BM" ;
	ns11:member-of	ns12:e_gov_4_bm ;
	ns11:order	"6" .
@prefix ns74:	<http://semantic.digital-agenda-data.eu/codelist/breakdown-group/e_gov_5_ke/> .
ns74:e_gov_5a_ke_eid	rdf:type	ns10:BreakdownToGroupMembership ;
	rdfs:label	"e_gov_5_KE" ;
	ns11:member-of	ns12:e_gov_5_ke ;
	ns11:order	"1" .
ns74:e_gov_5b_ke_edoc	rdf:type	ns10:BreakdownToGroupMembership ;
	rdfs:label	"e_gov_5_KE" ;
	ns11:member-of	ns12:e_gov_5_ke ;
	ns11:order	"2" .
ns74:e_gov_5c_ke_as	rdf:type	ns10:BreakdownToGroupMembership ;
	rdfs:label	"e_gov_5_KE" ;
	ns11:member-of	ns12:e_gov_5_ke ;
	ns11:order	"3" .
ns74:e_gov_5d_ke_dp	rdf:type	ns10:BreakdownToGroupMembership ;
	rdfs:label	"e_gov_5_KE" ;
	ns11:member-of	ns12:e_gov_5_ke ;
	ns11:order	"4" .
ns74:e_gov_5e_ke_esafe	rdf:type	ns10:BreakdownToGroupMembership ;
	rdfs:label	"e_gov_5_KE" ;
	ns11:member-of	ns12:e_gov_5_ke ;
	ns11:order	"5" .
ns74:e_gov_5f_ke_sso	rdf:type	ns10:BreakdownToGroupMembership ;
	rdfs:label	"e_gov_5_KE" ;
	ns11:member-of	ns12:e_gov_5_ke ;
	ns11:order	"6" .
@prefix ns75:	<http://semantic.digital-agenda-data.eu/codelist/breakdown-group/e_gov_events/> .
ns75:e_gov_events_1	rdf:type	ns10:BreakdownToGroupMembership ;
	rdfs:label	"e_gov_EVENTS" ;
	ns11:member-of	ns12:e_gov_events ;
	ns11:order	"1" .
ns75:e_gov_events_2	rdf:type	ns10:BreakdownToGroupMembership ;
	rdfs:label	"e_gov_EVENTS" ;
	ns11:member-of	ns12:e_gov_events ;
	ns11:order	"2" .
ns75:e_gov_events_3	rdf:type	ns10:BreakdownToGroupMembership ;
	rdfs:label	"e_gov_EVENTS" ;
	ns11:member-of	ns12:e_gov_events ;
	ns11:order	"3" .
ns75:e_gov_events_4	rdf:type	ns10:BreakdownToGroupMembership ;
	rdfs:label	"e_gov_EVENTS" ;
	ns11:member-of	ns12:e_gov_events ;
	ns11:order	"4" .
ns75:e_gov_events_5	rdf:type	ns10:BreakdownToGroupMembership ;
	rdfs:label	"e_gov_EVENTS" ;
	ns11:member-of	ns12:e_gov_events ;
	ns11:order	"5" .
ns75:e_gov_events_6	rdf:type	ns10:BreakdownToGroupMembership ;
	rdfs:label	"e_gov_EVENTS" ;
	ns11:member-of	ns12:e_gov_events ;
	ns11:order	"6" .
ns75:e_gov_events_7	rdf:type	ns10:BreakdownToGroupMembership ;
	rdfs:label	"e_gov_EVENTS" ;
	ns11:member-of	ns12:e_gov_events ;
	ns11:order	"7" .
ns75:e_gov_events_8	rdf:type	ns10:BreakdownToGroupMembership ;
	rdfs:label	"e_gov_EVENTS" ;
	ns11:member-of	ns12:e_gov_events ;
	ns11:order	"8" .
ns67:egov_life_events	rdf:type	ns10:BreakdownToGroupMembership ;
	rdfs:label	"total" ;
	ns11:member-of	ns12:total ;
	ns11:order	"1" .
ns7:e_gov_1a_ucg_oa	rdf:type	ns10:Breakdown ,
		skos:Concept ;
	skos:notation	"e_gov_1a_UCG_OA" ;
	skos:definition	"eGovernment services related to User Centric Government - Online availability" ;
	skos:topConceptOf	ns1:breakdown ;
	ns11:membership	ns70:e_gov_1a_ucg_oa ;
	skos:altLabel	"1a User Centric Government - Online availability" ;
	skos:prefLabel	"1a User Centric Government - Online availability" .
ns7:e_gov_1b_ucg_us	rdf:type	ns10:Breakdown ,
		skos:Concept ;
	skos:notation	"e_gov_1b_UCG_US" ;
	skos:definition	"eGovernment services related to User Centric Government - Usability" ;
	skos:topConceptOf	ns1:breakdown ;
	ns11:membership	ns70:e_gov_1b_ucg_us ;
	skos:altLabel	"1b User Centric Government - Usability" ;
	skos:prefLabel	"1b User Centric Government - Usability" .
ns7:e_gov_1c_ucg_mf	rdf:type	ns10:Breakdown ,
		skos:Concept ;
	skos:notation	"e_gov_1c_UCG_MF" ;
	skos:definition	"eGovernment services related to User Centric Government - Mobile Friendliness" ;
	skos:topConceptOf	ns1:breakdown ;
	ns11:membership	ns70:e_gov_1c_ucg_mf ;
	skos:altLabel	"1c User Centric Government - Mobile Friendliness" ;
	skos:prefLabel	"1c User Centric Government - Mobile Friendliness" .
ns7:e_gov_1d_ucg_eu	rdf:type	ns10:Breakdown ,
		skos:Concept ;
	skos:notation	"e_gov_1d_UCG_EU" ;
	skos:definition	"eGovernment services related to User Centric Government - Ease of Use" ;
	skos:topConceptOf	ns1:breakdown ;
	ns11:membership	ns70:e_gov_1d_ucg_eu ;
	skos:altLabel	"1d User Centric Government - Ease of Use" ;
	skos:prefLabel	"1d User Centric Government - Ease of Use" .
ns7:e_gov_1e_ucg_su	rdf:type	ns10:Breakdown ,
		skos:Concept ;
	skos:notation	"e_gov_1e_UCG_SU" ;
	skos:definition	"eGovernment services related to User Centric Government - Speed of Use" ;
	skos:topConceptOf	ns1:breakdown ;
	ns11:membership	ns70:e_gov_1e_ucg_su ;
	skos:altLabel	"1e User Centric Government - Speed of Use" ;
	skos:prefLabel	"1e User Centric Government - Speed of Use" .
ns7:e_gov_2a_tg_sd	rdf:type	ns10:Breakdown ,
		skos:Concept ;
	skos:notation	"e_gov_2a_TG_SD" ;
	skos:definition	"eGovernment services related to Transparent Government - Service delivery" ;
	skos:topConceptOf	ns1:breakdown ;
	ns11:membership	ns71:e_gov_2a_tg_sd ;
	skos:altLabel	"2a Transparent Government - Service delivery" ;
	skos:prefLabel	"2a Transparent Government - Service delivery" .
ns7:e_gov_2b_tg_po	rdf:type	ns10:Breakdown ,
		skos:Concept ;
	skos:notation	"e_gov_2b_TG_PO" ;
	skos:definition	"eGovernment services related to Transparent Government - Public organisations" ;
	skos:topConceptOf	ns1:breakdown ;
	ns11:membership	ns71:e_gov_2b_tg_po ;
	skos:altLabel	"2b Transparent Government - Public organisations" ;
	skos:prefLabel	"2b Transparent Government - Public organisations" .
ns7:e_gov_2c_tg_pd	rdf:type	ns10:Breakdown ,
		skos:Concept ;
	skos:notation	"e_gov_2c_TG_PD" ;
	skos:definition	"eGovernment services related to Transparent Government - Personal data" ;
	skos:topConceptOf	ns1:breakdown ;
	ns11:membership	ns71:e_gov_2c_tg_pd ;
	skos:altLabel	"2c Transparent Government - Personal data" ;
	skos:prefLabel	"2c Transparent Government - Personal data" .
ns7:e_gov_3a_cm_oa	rdf:type	ns10:Breakdown ,
		skos:Concept ;
	skos:notation	"e_gov_3a_CM_OA" ;
	skos:definition	"eGovernment services related to Citizen Mobility - Online availability" ;
	skos:topConceptOf	ns1:breakdown ;
	ns11:membership	ns72:e_gov_3a_cm_oa ;
	skos:altLabel	"3a Citizen Mobility - Online availability" ;
	skos:prefLabel	"3a Citizen Mobility - Online availability" .
ns7:e_gov_3b_cm_us	rdf:type	ns10:Breakdown ,
		skos:Concept ;
	skos:notation	"e_gov_3b_CM_US" ;
	skos:definition	"eGovernment services related to Citizen Mobility - Usability" ;
	skos:topConceptOf	ns1:breakdown ;
	ns11:membership	ns72:e_gov_3b_cm_us ;
	skos:altLabel	"3b Citizen Mobility - Usability" ;
	skos:prefLabel	"3b Citizen Mobility - Usability" .
ns7:e_gov_3c_cm_eidcb	rdf:type	ns10:Breakdown ,
		skos:Concept ;
	skos:notation	"e_gov_3c_CM_EIDCB" ;
	skos:definition	"eGovernment services related to Citizen Mobility - eID Cross Borders" ;
	skos:topConceptOf	ns1:breakdown ;
	ns11:membership	ns72:e_gov_3c_cm_eidcb ;
	skos:altLabel	"3c Citizen Mobility - eID Cross Borders" ;
	skos:prefLabel	"3c Citizen Mobility - eID Cross Borders" .
ns7:e_gov_3d_cm_edoccb	rdf:type	ns10:Breakdown ,
		skos:Concept ;
	skos:notation	"e_gov_3d_CM_EDOCCB" ;
	skos:definition	"eGovernment services related to Citizen Mobility - eDocuments Cross Borders" ;
	skos:topConceptOf	ns1:breakdown ;
	ns11:membership	ns72:e_gov_3d_cm_edoccb ;
	skos:altLabel	"3d Citizen Mobility - eDocuments Cross Borders" ;
	skos:prefLabel	"3d Citizen Mobility - eDocuments Cross Borders" .
ns7:e_gov_3e_cm_eu	rdf:type	ns10:Breakdown ,
		skos:Concept ;
	skos:notation	"e_gov_3e_CM_EU" ;
	skos:definition	"eGovernment services related to Citizen Mobility - Ease of Use" ;
	skos:topConceptOf	ns1:breakdown ;
	ns11:membership	ns72:e_gov_3e_cm_eu ;
	skos:altLabel	"3e Citizen Mobility - Ease of Use" ;
	skos:prefLabel	"3e Citizen Mobility - Ease of Use" .
ns7:e_gov_3f_cm_su	rdf:type	ns10:Breakdown ,
		skos:Concept ;
	skos:notation	"e_gov_3f_CM_SU" ;
	skos:definition	"eGovernment services related to Citizen Mobility - Speed of Use" ;
	skos:topConceptOf	ns1:breakdown ;
	ns11:membership	ns72:e_gov_3f_cm_su ;
	skos:altLabel	"3f Citizen Mobility - Speed of Use" ;
	skos:prefLabel	"3f Citizen Mobility - Speed of Use" .
ns7:e_gov_4a_bm_oa	rdf:type	ns10:Breakdown ,
		skos:Concept ;
	skos:notation	"e_gov_4a_BM_OA" ;
	skos:definition	"eGovernment services related to Business Mobility - Online availability" ;
	skos:topConceptOf	ns1:breakdown ;
	ns11:membership	ns73:e_gov_4a_bm_oa ;
	skos:altLabel	"4a Business Mobility - Online availability" ;
	skos:prefLabel	"4a Business Mobility - Online availability" .
ns7:e_gov_4b_bm_us	rdf:type	ns10:Breakdown ,
		skos:Concept ;
	skos:notation	"e_gov_4b_BM_US" ;
	skos:definition	"eGovernment services related to Business Mobility - Usability" ;
	skos:topConceptOf	ns1:breakdown ;
	ns11:membership	ns73:e_gov_4b_bm_us ;
	skos:altLabel	"4b Business Mobility - Usability" ;
	skos:prefLabel	"4b Business Mobility - Usability" .
ns7:e_gov_4c_bm_eidcb	rdf:type	ns10:Breakdown ,
		skos:Concept ;
	skos:notation	"e_gov_4c_BM_EIDCB" ;
	skos:definition	"eGovernment services related to Business Mobility - eID Cross Borders" ;
	skos:topConceptOf	ns1:breakdown ;
	ns11:membership	ns73:e_gov_4c_bm_eidcb ;
	skos:altLabel	"4c Business Mobility - eID Cross Borders" ;
	skos:prefLabel	"4c Business Mobility - eID Cross Borders" .
ns7:e_gov_4d_bm_edoccb	rdf:type	ns10:Breakdown ,
		skos:Concept ;
	skos:notation	"e_gov_4d_BM_EDOCCB" ;
	skos:definition	"eGovernment services related to Business Mobility - eDocuments Cross Borders" ;
	skos:topConceptOf	ns1:breakdown ;
	ns11:membership	ns73:e_gov_4d_bm_edoccb ;
	skos:altLabel	"4d Business Mobility - eDocuments Cross Borders" ;
	skos:prefLabel	"4d Business Mobility - eDocuments Cross Borders" .
ns7:e_gov_4e_bm_eu	rdf:type	ns10:Breakdown ,
		skos:Concept ;
	skos:notation	"e_gov_4e_BM_EU" ;
	skos:definition	"eGovernment services related to Business Mobility - Ease of Use" ;
	skos:topConceptOf	ns1:breakdown ;
	ns11:membership	ns73:e_gov_4e_bm_eu ;
	skos:altLabel	"4e Business Mobility - Ease of Use" ;
	skos:prefLabel	"4e Business Mobility - Ease of Use" .
ns7:e_gov_4f_bm_su	rdf:type	ns10:Breakdown ,
		skos:Concept ;
	skos:notation	"e_gov_4f_BM_SU" ;
	skos:definition	"eGovernment services related to Business Mobility - Speed of Use" ;
	skos:topConceptOf	ns1:breakdown ;
	ns11:membership	ns73:e_gov_4f_bm_su ;
	skos:altLabel	"4f Business Mobility - Speed of Use" ;
	skos:prefLabel	"4f Business Mobility - Speed of Use" .
ns7:e_gov_5a_ke_eid	rdf:type	ns10:Breakdown ,
		skos:Concept ;
	skos:notation	"e_gov_5a_KE_EID" ;
	skos:definition	"eGovernment services related to Key Enablers - eID. A government-issued, electronic identification solution to determine if the use is who he claims to be. Using eID enables online transactions, saves time and reduces costs for all actors involved. " ;
	skos:topConceptOf	ns1:breakdown ;
	ns11:membership	ns74:e_gov_5a_ke_eid ;
	skos:altLabel	"5a Key Enablers - eID" ;
	skos:prefLabel	"5a Key Enablers - eID" .
ns7:e_gov_5b_ke_edoc	rdf:type	ns10:Breakdown ,
		skos:Concept ;
	skos:notation	"e_gov_5b_KE_EDOC" ;
	skos:definition	"eGovernment services related to Key Enablers - eDocuments. An electronic document reduces offline \npaper processes by allowing citizens and businesses to send authenticated documents online. " ;
	skos:topConceptOf	ns1:breakdown ;
	ns11:membership	ns74:e_gov_5b_ke_edoc ;
	skos:altLabel	"5b Key Enablers - eDocuments" ;
	skos:prefLabel	"5b Key Enablers - eDocuments" .
ns7:e_gov_5c_ke_as	rdf:type	ns10:Breakdown ,
		skos:Concept ;
	skos:notation	"e_gov_5c_KE_AS" ;
	skos:definition	"eGovernment services related to Key Enablers - Authentic sources" ;
	skos:topConceptOf	ns1:breakdown ;
	ns11:membership	ns74:e_gov_5c_ke_as ;
	skos:altLabel	"5c Key Enablers - Authentic sources" ;
	skos:prefLabel	"5c Key Enablers - Authentic sources" .
ns7:e_gov_5d_ke_dp	rdf:type	ns10:Breakdown ,
		skos:Concept ;
	skos:notation	"e_gov_5d_KE_DP" ;
	skos:definition	"eGovernment services related to Key Enablers - Digital Post. Public administrations should allow citizens to receive mail in a digital format and help reduce paper mailing. Governments should provide the possibility to communicate electronically-only with citizens or entrepreneurs through personal mailboxes or other digital post solutions. This represents a novelty of the 2016 measurement. " ;
	skos:topConceptOf	ns1:breakdown ;
	ns11:membership	ns74:e_gov_5d_ke_dp ;
	skos:altLabel	"5d Key Enablers - Digital Post" ;
	skos:prefLabel	"5d Key Enablers - Digital Post" .
ns7:e_gov_5e_ke_esafe	rdf:type	ns10:Breakdown ,
		skos:Concept ;
	skos:notation	"e_gov_5e_KE_ESAFE" ;
	skos:definition	"eGovernment services related to Key Enablers - eSafe" ;
	skos:topConceptOf	ns1:breakdown ;
	ns11:membership	ns74:e_gov_5e_ke_esafe ;
	skos:altLabel	"5e Key Enablers - eSafe" ;
	skos:prefLabel	"5e Key Enablers - eSafe" .
ns7:e_gov_5f_ke_sso	rdf:type	ns10:Breakdown ,
		skos:Concept ;
	skos:notation	"e_gov_5f_KE_SSO" ;
	skos:definition	"eGovernment services related to Key Enablers - Single Sign On (SSO)" ;
	skos:topConceptOf	ns1:breakdown ;
	ns11:membership	ns74:e_gov_5f_ke_sso ;
	skos:altLabel	"5f Key Enablers - Single Sign On (SSO)" ;
	skos:prefLabel	"5f Key Enablers - Single Sign On (SSO)" .
ns7:e_gov_events_1	rdf:type	ns10:Breakdown ,
		skos:Concept ;
	skos:notation	"e_gov_EVENTS_1" ;
	skos:definition	"A business life event that covers 11 services related to regular business operations, such as administrative and tax requirements, human resources and refund of VAT." ;
	skos:topConceptOf	ns1:breakdown ;
	ns11:membership	ns75:e_gov_events_1 ;
	skos:altLabel	"Regular business operations" ;
	skos:prefLabel	"Regular business operations" .
ns7:e_gov_events_2	rdf:type	ns10:Breakdown ,
		skos:Concept ;
	skos:notation	"e_gov_EVENTS_2" ;
	skos:definition	"This concise life event illustrates the journey in case of moving places: from deregistering to registering address in the new town. It also includes notifications to other public organizations and utilities." ;
	skos:topConceptOf	ns1:breakdown ;
	ns11:membership	ns75:e_gov_events_2 ;
	skos:altLabel	"General administration: moving" ;
	skos:prefLabel	"General administration: moving" .
ns7:e_gov_events_3	rdf:type	ns10:Breakdown ,
		skos:Concept ;
	skos:notation	"e_gov_EVENTS_3" ;
	skos:definition	"A total of 12 services concerning buying and registering a car and driving fines, and related to car taxes, parking permits and other administrative requirements." ;
	skos:topConceptOf	ns1:breakdown ;
	ns11:membership	ns75:e_gov_events_3 ;
	skos:altLabel	"Owning and driving a car" ;
	skos:prefLabel	"Owning and driving a car" .
ns7:e_gov_events_4	rdf:type	ns10:Breakdown ,
		skos:Concept ;
	skos:notation	"e_gov_EVENTS_4" ;
	skos:definition	"This life event is part of the Justice domain, and captures the journey of someone willing to start a small claims procedure: from orientation and initiation to retrieving verdict and appeal." ;
	skos:topConceptOf	ns1:breakdown ;
	ns11:membership	ns75:e_gov_events_4 ;
	skos:altLabel	"Starting a small claims procedure" ;
	skos:prefLabel	"Starting a small claims procedure" .
ns7:e_gov_events_5	rdf:type	ns10:Breakdown ,
		skos:Concept ;
	skos:notation	"e_gov_EVENTS_5" ;
	skos:definition	"This life event covers 33 services, both mandatory services as well as information needs, that allow an entrepreneur to start his business. It includes orientation, administrative and register requirements, and tax and insurance related matters. Early trading operations refers to activities regarding hiring employees and requesting an environmental permit." ;
	skos:topConceptOf	ns1:breakdown ;
	ns11:membership	ns75:e_gov_events_5 ;
	skos:altLabel	"Business Start-up" ;
	skos:prefLabel	"Business Start-up" .
ns7:e_gov_events_6	rdf:type	ns10:Breakdown ,
		skos:Concept ;
	skos:notation	"e_gov_EVENTS_6" ;
	skos:definition	"Including services that are typical for young families, such as: marriage (or other partnerships), birth and related (financial) rights, renovating a house, and also looking forward to your financial situation at a later age." ;
	skos:topConceptOf	ns1:breakdown ;
	ns11:membership	ns75:e_gov_events_6 ;
	skos:altLabel	"Family" ;
	skos:prefLabel	"Family" .
ns7:e_gov_events_7	rdf:type	ns10:Breakdown ,
		skos:Concept ;
	skos:notation	"e_gov_EVENTS_7" ;
	skos:definition	"From immediate actions for unemployed to applications for additional benefits and allowances, this life event captures vital elements when becoming unemployed. It also include various services concerning job search and participating in training programs, supporting people to find a job. A complete set of 22 services is assessed." ;
	skos:topConceptOf	ns1:breakdown ;
	ns11:membership	ns75:e_gov_events_7 ;
	skos:altLabel	"Losing and Finding a Job" ;
	skos:prefLabel	"Losing and Finding a Job" .
ns7:e_gov_events_8	rdf:type	ns10:Breakdown ,
		skos:Concept ;
	skos:notation	"e_gov_EVENTS_8" ;
	skos:definition	"In this life event, comprising of 14 services, it is evaluated to what extent enrolment in higher education can be done online. It also includes the orientation, such as gaining a clear understanding of admission requirements. Furthermore support services during study are part of the assessment, for instance career advice and portability of student grant when studying abroad." ;
	skos:topConceptOf	ns1:breakdown ;
	ns11:membership	ns75:e_gov_events_8 ;
	skos:altLabel	"Studying" ;
	skos:prefLabel	"Studying" .
ns7:egov_life_events	rdf:type	ns10:Breakdown ,
		skos:Concept ;
	skos:notation	"EGOV_LIFE_EVENTS" ;
	skos:definition	"Biennial average over 8 (7 before 2016) life events. 4 life events being measured in odd years (e.g.2013, 2015, 2017 etc.) and 4 life events in even years (2012, 2014, 2016 etc.). \nOdd years life events consist of: Regular business operations;  General administration: moving; Owning and driving a car; Starting a small claims procedure. Even years life events consists of: Business Start-up; Losing and Finding a Job; Studying and Family*. \n*Family life event was introduced in 2016, therefore for the scores of 2013, 2014 and 2016 the total score was calculated over 7 life events." ;
	skos:topConceptOf	ns1:breakdown ;
	ns11:membership	ns67:egov_life_events ;
	skos:altLabel	"All Life Events" ;
	skos:prefLabel	"All Life Events" .
ns67:egov_le_bus	rdf:type	ns10:BreakdownToGroupMembership ;
	rdfs:label	"total" ;
	ns11:member-of	ns12:total ;
	ns11:order	"1" .
ns7:egov_le_bus	rdf:type	ns10:Breakdown ,
		skos:Concept ;
	skos:notation	"eGov_le_bus" ;
	skos:definition	"The indicator is calculated for the basic services (therefore excluding extended services) of the life events of \u201CRegular business operations\u201D and \u201CStarting-up a business\u201D. These life events are calculated in alternate years. Therefore, each year the indicator will be a (moving) average of the latest available year of data for each indicator." ;
	skos:topConceptOf	ns1:breakdown ;
	ns11:membership	ns67:egov_le_bus ;
	skos:altLabel	"Life Events for Businesses" ;
	skos:prefLabel	"Life Events for Businesses" .
ns7:wid_score	rdf:type	ns10:Breakdown ,
		skos:Concept ;
	skos:notation	"WID_score" ;
	skos:topConceptOf	ns1:breakdown .
@prefix ns76:	<http://semantic.digital-agenda-data.eu/codelist/breakdown-group/wid_score/> .
ns7:wid_score	ns11:membership	ns76:wid_score ;
	skos:altLabel	"Score for Women in Digital" ;
	skos:prefLabel	"Score for Women in Digital" .
ns76:wid_score	rdf:type	ns10:BreakdownToGroupMembership ;
	rdfs:label	"wid_score" ;
	ns11:member-of	ns12:wid_score ;
	ns11:order	"1"^^xsd:byte .
ns36:desi_1d_ultra	rdf:type	ns10:BreakdownToGroupMembership ;
	rdfs:label	"desi_1_conn" ;
	ns11:member-of	ns12:desi_1_conn ;
	ns11:order	"5" .
ns36:desi_1e_bbpi	rdf:type	ns10:BreakdownToGroupMembership ;
	rdfs:label	"desi_1_conn" ;
	ns11:member-of	ns12:desi_1_conn ;
	ns11:order	"6" .
ns38:desi_1b1_4g	rdf:type	ns10:BreakdownToGroupMembership ;
	rdfs:label	"desi_1b_mbb" ;
	ns11:member-of	ns12:desi_1b_mbb ;
	ns11:order	"1" .
ns38:desi_1b2_mbbtu	rdf:type	ns10:BreakdownToGroupMembership ;
	rdfs:label	"desi_1b_mbb" ;
	ns11:member-of	ns12:desi_1b_mbb ;
	ns11:order	"2" .
@prefix ns77:	<http://semantic.digital-agenda-data.eu/codelist/breakdown-group/desi_1d_ultra/> .
ns77:desi_1d1_ubbc	rdf:type	ns10:BreakdownToGroupMembership ;
	rdfs:label	"desi_1d_ultra" ;
	ns11:member-of	ns12:desi_1d_ultra ;
	ns11:order	"1" .
ns77:desi_1d2_ubbta	rdf:type	ns10:BreakdownToGroupMembership ;
	rdfs:label	"desi_1d_ultra" ;
	ns11:member-of	ns12:desi_1d_ultra ;
	ns11:order	"2" .
@prefix ns78:	<http://semantic.digital-agenda-data.eu/codelist/breakdown-group/desi_1e_bbpi/> .
ns78:desi_1e1_bbpi	rdf:type	ns10:BreakdownToGroupMembership ;
	rdfs:label	"desi_1e_bbpi" ;
	ns11:member-of	ns12:desi_1e_bbpi ;
	ns11:order	"1" .
ns51:desi_5b_ehs	rdf:type	ns10:BreakdownToGroupMembership ;
	rdfs:label	"desi_5_dps" ;
	ns11:member-of	ns12:desi_5_dps ;
	ns11:order	"2" .
ns52:desi_5a4_psb	rdf:type	ns10:BreakdownToGroupMembership ;
	rdfs:label	"desi_5a_egov" ;
	ns11:member-of	ns12:desi_5a_egov ;
	ns11:order	"4" .
ns52:desi_5a5_opendata	rdf:type	ns10:BreakdownToGroupMembership ;
	rdfs:label	"desi_5a_egov" ;
	ns11:member-of	ns12:desi_5a_egov ;
	ns11:order	"5" .
@prefix ns79:	<http://semantic.digital-agenda-data.eu/codelist/breakdown-group/desi_5b_ehs/> .
ns79:desi_5b1_ehs	rdf:type	ns10:BreakdownToGroupMembership ;
	rdfs:label	"desi_5b_ehs" ;
	ns11:member-of	ns12:desi_5b_ehs .
@prefix ns80:	<http://semantic.digital-agenda-data.eu/codelist/breakdown-group/egov_ke/> .
ns80:authentic_sources	rdf:type	ns10:BreakdownToGroupMembership ;
	rdfs:label	"egov_ke" ;
	ns11:member-of	ns12:egov_ke ;
	ns11:order	"18" .
ns80:digital_post	rdf:type	ns10:BreakdownToGroupMembership ;
	rdfs:label	"egov_ke" ;
	ns11:member-of	ns12:egov_ke ;
	ns11:order	"19" .
ns80:edocuments	rdf:type	ns10:BreakdownToGroupMembership ;
	rdfs:label	"egov_ke" ;
	ns11:member-of	ns12:egov_ke ;
	ns11:order	"17" .
ns80:eid	rdf:type	ns10:BreakdownToGroupMembership ;
	rdfs:label	"egov_ke" ;
	ns11:member-of	ns12:egov_ke ;
	ns11:order	"16" .
ns57:family	rdf:type	ns10:BreakdownToGroupMembership ;
	rdfs:label	"egov_le" ;
	ns11:member-of	ns12:egov_le ;
	ns11:order	"9" .
@prefix ns81:	<http://semantic.digital-agenda-data.eu/codelist/breakdown-group/egov_ser/> .
ns81:auto_service	rdf:type	ns10:BreakdownToGroupMembership ;
	rdfs:label	"egov_ser" ;
	ns11:member-of	ns12:egov_ser ;
	ns11:order	"10" .
ns81:info_online_no_portal	rdf:type	ns10:BreakdownToGroupMembership ;
	rdfs:label	"egov_ser" ;
	ns11:member-of	ns12:egov_ser ;
	ns11:order	"14" .
ns81:info_online_portal	rdf:type	ns10:BreakdownToGroupMembership ;
	rdfs:label	"egov_ser" ;
	ns11:member-of	ns12:egov_ser ;
	ns11:order	"13" .
ns81:offline	rdf:type	ns10:BreakdownToGroupMembership ;
	rdfs:label	"egov_ser" ;
	ns11:member-of	ns12:egov_ser ;
	ns11:order	"15" .
ns81:serv_online_no_portal	rdf:type	ns10:BreakdownToGroupMembership ;
	rdfs:label	"egov_ser" ;
	ns11:member-of	ns12:egov_ser ;
	ns11:order	"12" .
ns81:serv_online_portal	rdf:type	ns10:BreakdownToGroupMembership ;
	rdfs:label	"egov_ser" ;
	ns11:member-of	ns12:egov_ser ;
	ns11:order	"11" .
ns7:authentic_sources	rdf:type	skos:Concept ,
		ns10:Breakdown ;
	skos:notation	"Authentic_sources" ;
	skos:definition	"Base registries used by governments to automatically validate or fetch data relating to citizens or businesses. It facilitates prefilling of online forms and the implementation of the \u2018once-only principle\u2019, which implies that governments re-use data to deliver services automatically. " ;
	skos:topConceptOf	ns1:breakdown ;
	ns11:membership	ns80:authentic_sources ;
	skos:altLabel	"Authentic sources" ,
		"Authentic_sources" ;
	skos:prefLabel	"Authentic sources" ,
		"Authentic_sources" .
ns7:auto_service	rdf:type	skos:Concept ,
		ns10:Breakdown ;
	skos:notation	"auto_service" ;
	skos:definition	"eGovernment automated service" ;
	skos:topConceptOf	ns1:breakdown ;
	ns11:membership	ns81:auto_service ;
	skos:altLabel	"Automated service" ;
	skos:prefLabel	"Automated service" .
ns7:desi_1b1_4g	rdf:type	skos:Concept ,
		ns10:Breakdown ;
	skos:notation	"DESI_1B1_4G" ;
	skos:topConceptOf	ns1:breakdown ;
	ns11:membership	ns38:desi_1b1_4g ;
	skos:altLabel	"1b1 4G Coverage" ;
	skos:prefLabel	"1b1 4G Coverage" .
ns7:desi_1b2_mbbtu	rdf:type	skos:Concept ,
		ns10:Breakdown ;
	skos:notation	"DESI_1B2_MBBTU" ;
	skos:topConceptOf	ns1:breakdown ;
	ns11:membership	ns38:desi_1b2_mbbtu ;
	skos:altLabel	"1b2 Mobile BB Take-up" ;
	skos:prefLabel	"1b2 Mobile BB Take-up" .
ns7:desi_1d1_ubbc	rdf:type	skos:Concept ,
		ns10:Breakdown ;
	skos:notation	"DESI_1D1_UBBC" ;
	skos:topConceptOf	ns1:breakdown ;
	ns11:membership	ns77:desi_1d1_ubbc ;
	skos:altLabel	"1d1 Ultrafast BB Coverage" ;
	skos:prefLabel	"1d1 Ultrafast BB Coverage" .
ns7:desi_1d2_ubbta	rdf:type	skos:Concept ,
		ns10:Breakdown ;
	skos:notation	"DESI_1D2_UBBTA" ;
	skos:topConceptOf	ns1:breakdown ;
	ns11:membership	ns77:desi_1d2_ubbta ;
	skos:altLabel	"1d2 Ultrafast BB Take-up" ;
	skos:prefLabel	"1d2 Ultrafast BB Take-up" .
ns7:desi_1d_ultra	rdf:type	skos:Concept ,
		ns10:Breakdown ;
	skos:notation	"DESI_1D_ULTRA" ;
	skos:topConceptOf	ns1:breakdown ;
	ns11:membership	ns36:desi_1d_ultra ;
	skos:altLabel	"1d Ultrafast Broadband" ;
	skos:prefLabel	"1d Ultrafast Broadband" .
ns7:desi_1e1_bbpi	rdf:type	skos:Concept ,
		ns10:Breakdown ;
	skos:notation	"DESI_1E1_BBPI" ;
	skos:topConceptOf	ns1:breakdown ;
	ns11:membership	ns78:desi_1e1_bbpi ;
	skos:altLabel	"1e1 Broadband Price Index" ;
	skos:prefLabel	"1e1 Broadband Price Index" .
ns7:desi_1e_bbpi	rdf:type	skos:Concept ,
		ns10:Breakdown ;
	skos:notation	"DESI_1E_BBPI" ;
	skos:topConceptOf	ns1:breakdown ;
	ns11:membership	ns36:desi_1e_bbpi ;
	skos:altLabel	"1e Broadband Price Index" ;
	skos:prefLabel	"1e Broadband Price Index" .
ns7:desi_5a4_psb	rdf:type	skos:Concept ,
		ns10:Breakdown ;
	skos:notation	"DESI_5A4_PSB" ;
	skos:topConceptOf	ns1:breakdown ;
	ns11:membership	ns52:desi_5a4_psb ;
	skos:altLabel	"5a4 eGo vernment Services for Businesses" ;
	skos:prefLabel	"5a4 eGo vernment Services for Businesses" .
ns7:desi_5a5_opendata	rdf:type	skos:Concept ,
		ns10:Breakdown ;
	skos:notation	"DESI_5A5_OPENDATA" ;
	skos:topConceptOf	ns1:breakdown ;
	ns11:membership	ns52:desi_5a5_opendata ;
	skos:altLabel	"5a5 Open Data" ;
	skos:prefLabel	"5a5 Open Data" .
ns7:desi_5b1_ehs	rdf:type	skos:Concept ,
		ns10:Breakdown ;
	skos:notation	"DESI_5B1_EHS" ;
	skos:topConceptOf	ns1:breakdown ;
	ns11:membership	ns79:desi_5b1_ehs ;
	skos:altLabel	"5b eHealth" ;
	skos:prefLabel	"5b eHealth" .
ns7:desi_5b_ehs	rdf:type	skos:Concept ,
		ns10:Breakdown ;
	skos:notation	"DESI_5B_EHS" ;
	skos:topConceptOf	ns1:breakdown ;
	ns11:membership	ns51:desi_5b_ehs ;
	skos:altLabel	"5b eHealth" ;
	skos:prefLabel	"5b eHealth" .
ns7:digital_post	rdf:type	skos:Concept ,
		ns10:Breakdown ;
	skos:notation	"Digital_Post" ;
	skos:definition	"Public administrations should allow citizens to receive mail in a digital format and help reduce paper mailing. Governments should provide the possibility to communicate electronically-only with citizens or entrepreneurs through personal mailboxes or other digital post solutions. This represents a novelty of the 2016 measurement. " ;
	skos:topConceptOf	ns1:breakdown ;
	ns11:membership	ns80:digital_post ;
	skos:altLabel	"Digital_Post" ,
		"Digital Post" ;
	skos:prefLabel	"Digital_Post" ,
		"Digital Post" .
ns7:edocuments	rdf:type	skos:Concept ,
		ns10:Breakdown ;
	skos:notation	"eDocuments" ;
	skos:definition	"An electronic document reduces offline \npaper processes by allowing citizens and businesses to send authenticated documents online. " ;
	skos:topConceptOf	ns1:breakdown ;
	ns11:membership	ns80:edocuments ;
	skos:altLabel	"eDocuments" ;
	skos:prefLabel	"eDocuments" .
ns7:eid	rdf:type	skos:Concept ,
		ns10:Breakdown ;
	skos:notation	"eID" ;
	skos:definition	"A government-issued, electronic identification solution to determine if the use is who he claims to be. Using eID enables online transactions, saves time and reduces costs for all actors involved. " ;
	skos:topConceptOf	ns1:breakdown ;
	ns11:membership	ns80:eid ;
	skos:altLabel	"eID" ;
	skos:prefLabel	"eID" .
ns7:family	rdf:type	skos:Concept ,
		ns10:Breakdown ;
	skos:notation	"family" ;
	skos:definition	"eGovernment services related to the life event: Life" ;
	skos:topConceptOf	ns1:breakdown ;
	ns11:membership	ns57:family ;
	skos:altLabel	"Family" ;
	skos:prefLabel	"Family Life Event" .
ns7:info_online_no_portal	rdf:type	skos:Concept ,
		ns10:Breakdown ;
	skos:notation	"info_online_no_portal" ;
	skos:definition	"eGovernment information provided online but not through a portal" ;
	skos:topConceptOf	ns1:breakdown ;
	ns11:membership	ns81:info_online_no_portal ;
	skos:altLabel	"Information online but not through portal" ;
	skos:prefLabel	"Information online but not through portal" .
ns7:info_online_portal	rdf:type	skos:Concept ,
		ns10:Breakdown ;
	skos:notation	"info_online_portal" ;
	skos:definition	"eGovernment information provided online and through a portal" ;
	skos:topConceptOf	ns1:breakdown ;
	ns11:membership	ns81:info_online_portal ;
	skos:altLabel	"Information online and through portal" ;
	skos:prefLabel	"Information online and through portal" .
ns7:offline	rdf:type	skos:Concept ,
		ns10:Breakdown ;
	skos:notation	"offline" ;
	skos:definition	"eGovernment service or information provided offline" ;
	skos:topConceptOf	ns1:breakdown ;
	ns11:membership	ns81:offline ;
	skos:altLabel	"Offline" ;
	skos:prefLabel	"Offline" .
ns7:serv_online_no_portal	rdf:type	skos:Concept ,
		ns10:Breakdown ;
	skos:notation	"serv_online_no_portal" ;
	skos:definition	"eGovernment service provided online but not through a portal" ;
	skos:topConceptOf	ns1:breakdown ;
	ns11:membership	ns81:serv_online_no_portal ;
	skos:altLabel	"Service online but not through portal" ;
	skos:prefLabel	"Service online but not through portal" .
ns7:serv_online_portal	rdf:type	skos:Concept ,
		ns10:Breakdown ;
	skos:notation	"serv_online_portal" ;
	skos:definition	"eGovernment service provided online and through a portal" ;
	skos:topConceptOf	ns1:breakdown ;
	ns11:membership	ns81:serv_online_portal ;
	skos:altLabel	"Service online and through portal" ;
	skos:prefLabel	"Service online and through portal" .