@prefix rdf:	<http://www.w3.org/1999/02/22-rdf-syntax-ns#> .
@prefix rdfs:	<http://www.w3.org/2000/01/rdf-schema#> .
@prefix xsd:	<http://www.w3.org/2001/XMLSchema#> .
@prefix qb:	<http://purl.org/linked-data/cube#> .
@prefix dcat:	<http://www.w3.org/ns/dcat#> .
@prefix dcterms:	<http://purl.org/dc/terms/> .
@prefix org:	<http://www.w3.org/ns/org#> .
@prefix foaf:	<http://xmlns.com/foaf/0.1/> .
@prefix odp:	<http://ec.europa.eu/open-data/ontologies/ec-odp#> .
@prefix adms:	<http://www.w3.org/ns/adms#> .
@prefix schema:	<http://schema.org/> .
@prefix vcard:	<http://www.w3.org/2006/vcard/ns#> .
@prefix skos:	<http://www.w3.org/2004/02/skos/core#> .
@prefix sdmx:	<http://purl.org/linked-data/sdmx#> .
@prefix sdmx-attribute:	<http://purl.org/linked-data/sdmx/2009/attribute#> .
@prefix sdmx-concept:	<http://purl.org/linked-data/sdmx/2009/concept#> .
@prefix sdmx-dimension:	<http://purl.org/linked-data/sdmx/2009/dimension#> .
@prefix sdmx-measure:	<http://purl.org/linked-data/sdmx/2009/measure#> .
@prefix sdmx-subject:	<http://purl.org/linked-data/sdmx/2009/subject#> .

@prefix ld-api:	<http://purl.org/linked-data/api/vocab#> .

@prefix dad-attribute:	<http://semantic.digital-agenda-data.eu/def/dsd/scoreboard/attribute/> .
@prefix dad-class:	<http://semantic.digital-agenda-data.eu/def/class/> .
@prefix dad-codelist:	<http://semantic.digital-agenda-data.eu/codelist/> .
@prefix dad-concept:	<http://semantic.digital-agenda-data.eu/def/concept/> .
@prefix dad-def:	<http://semantic.digital-agenda-data.eu/def/> .
@prefix dad-dimension:	<http://semantic.digital-agenda-data.eu/def/dsd/scoreboard/dimension/> .
@prefix dad-dsd:	<http://semantic.digital-agenda-data.eu/def/dsd/> .
@prefix dad-prop:	<http://semantic.digital-agenda-data.eu/def/property/> .

# DATASET METADATA
<http://semantic.digital-agenda-data.eu/dataset/DESI>
	rdf:type qb:DataSet , dcat:Dataset ;
# DCAT Mandatory
	dcterms:title	"Digital Economy and Society Index"@en ;
	dcterms:description	"The Digital Economy and Society Index (DESI) is a composite index that summarises relevant indicators on Europe’s digital performance and tracks the evolution of EU member states in digital competitiveness, across five main dimensions: Connectivity, Human Capital, Use of Internet, Integration of Digital Technology, Digital Public Services."@en ;
# QB recommended properties
	rdfs:label	"Digital Economy and Society Index"@en ;
	rdfs:comment	"The Digital Economy and Society Index (DESI) is a composite index that summarises relevant indicators on Europe’s digital performance and tracks the evolution of EU member states in digital competitiveness, across five main dimensions: Connectivity, Human Capital, Use of Internet, Integration of Digital Technology, Digital Public Services."@en ;
	dcterms:subject	sdmx-subject:3.3.3 ;

	dcterms:license	<http://ec.europa.eu/geninfo/legal_notices_en.htm#copyright> ;
# DCAT-AP recommended properties
	dcat:contactPoint	<http://publications.europa.eu/resource/authority/corporate-body/CNECT/F4> ;
	dcat:distribution	<http://semantic.digital-agenda-data.eu/dataset/DESI/distribution/download> ;
	dcat:distribution	<http://semantic.digital-agenda-data.eu/dataset/DESI/distribution/visualisation> ;
	dcat:keyword	
		"Connectivity"@en ,
		"Human capital"@en ,
		"Internet"@en ,
		"Digital Technology"@en ,
		"Digital Public Services"@en ,
		"Information society"@en ,
		"Digital Economy"@en ;

	dcterms:publisher	<http://publications.europa.eu/resource/authority/corporate-body/CNECT> ;
	dcat:theme	
		<http://publications.europa.eu/resource/authority/data-theme/GOVE> ,
		<http://publications.europa.eu/resource/authority/data-theme/SOCI> ,
		<http://publications.europa.eu/resource/authority/data-theme/TECH> ;
# TODO more themes


# DCAT-AP optional properties / DCAT recommended properties
	dcterms:accessRights	<http://publications.europa.eu/resource/authority/access-right/PUBLIC>;
	dcat:landingPage	<http://digital-agenda-data.eu/> ;
	foaf:page	<http://digital-agenda-data.eu/> ;
	dcat:accrualPeriodicity	<http://publications.europa.eu/resource/authority/frequency/ANNUAL_2> ;
	dcterms:language <http://publications.europa.eu/resource/authority/language/ENG> ;
	dcterms:spatial	<http://publications.europa.eu/resource/authority/country/EUR>;
	dcterms:temporal	[ schema:startDate "2014-01-01"^^xsd:date ] ;
	dcterms:identifier	"DESI" ;
	#adms:identifier	[ skos:notation "DESI" ]
	dcterms:issued	"2011-05-01T00:00:00Z"^^xsd:dateTime ;
	dcterms:modified	"2016-06-01T00:00:00Z"^^xsd:dateTime ;


# QB
	qb:structure	<http://semantic.digital-agenda-data.eu/def/dsd/scoreboard>;

# Linked data
	foaf:isPrimaryTopicOf	<http://semantic.digital-agenda-data.eu/API/dataset/DESI.rdf> ;

# ODP
	adms:status	<http://purl.org/adms/status/Completed> .

# RELATED ENTITIES

# License
<http://ec.europa.eu/geninfo/legal_notices_en.htm#copyright>	dcterms:title	"Europa Legal Notice" .

# DCAT Distribution
<http://semantic.digital-agenda-data.eu/dataset/DESI/distribution/download>
	rdf:type	dcat:Distribution ;
	dcat:accessURL	<http://digital-agenda-data.eu/datasets/desi#download> ;
	dcterms:description	"Download instructions";
	dcterms:type	<http://publications.europa.eu/resource/authority/distribution-type/DOWNLOADABLE_FILE> ;
	dcterms:format	<http://publications.europa.eu/resource/authority/file-type/RDF_TURTLE> ;
	dcat:mediaType	"text/turtle" .

# DCAT Distribution
<http://semantic.digital-agenda-data.eu/dataset/DESI/distribution/visualisation>
	rdf:type	dcat:Distribution ;
	dcterms:type	<http://publications.europa.eu/resource/authority/distribution-type/VISUALIZATION> ;
	dcat:accessURL	<http://digital-agenda-data.eu/datasets/desi> ;
	dcterms:description	"Dataset visualisation".

# LD API page
<http://semantic.digital-agenda-data.eu/API/dataset/DESI.rdf>
	rdf:type	ld-api:Page ;
	foaf:primaryTopic	<http://semantic.digital-agenda-data.eu/dataset/DESI> ;
	ld-api:definition	<http://semantic.digital-agenda-data.eu/API/meta/dataset/_id.rdf> ;
	ld-api:extendedMetadataVersion	<http://semantic.digital-agenda-data.eu/API/dataset/DESI.rdf?_metadata=all> .

# Organization (contact point)
<http://publications.europa.eu/resource/authority/corporate-body/CNECT/F4>
	a vcard:Organization, foaf:Organization;
	rdfs:label "DG CONNECT - Digital Economy and Skills (Unit F.4)" ;
	foaf:mbox	"mailto:CNECT-F4@ec.europa.eu" ;
	foaf:name	"DG CONNECT - Digital Economy and Skills (Unit F.4)" ;
	foaf:workplaceHomepage	<https://ec.europa.eu/digital-single-market/en/dg-connect> .


## DATA STRUCTURE DEFINITION

# DSD Components

dad-dsd:scoreboard
	rdf:type	sdmx:DataStructureDefinition, qb:DataStructureDefinition .
dad-dsd:scoreboard
	qb:component
		dad-attribute:flag ,
		dad-attribute:note ,
		dad-dimension:indicator ,
		dad-dimension:breakdown ,
		dad-dimension:ref-area ,
		dad-dimension:time-period ,
		dad-dimension:unit-measure ,
		<http://semantic.digital-agenda-data.eu/def/dsd/scoreboard/measure/obsValue> ;
	sdmx:primaryMeasure	sdmx-measure:obsValue .

# DSD Component Specifications

dad-dimension:indicator	rdf:type	qb:ComponentSpecification ;
	qb:dimension	dad-prop:indicator ;
	qb:order	1 .
dad-dimension:breakdown	rdf:type	qb:ComponentSpecification ;
	qb:dimension	dad-prop:breakdown ;
	qb:order	2 .
dad-dimension:unit-measure	rdf:type	qb:ComponentSpecification ;
	qb:dimension	dad-prop:unit-measure ;
	qb:order	3 .
dad-dimension:ref-area	rdf:type	qb:ComponentSpecification ;
	qb:dimension	dad-prop:ref-area ;
	qb:order	4 .
dad-dimension:time-period	rdf:type	qb:ComponentSpecification ;
	qb:dimension	dad-prop:time-period ;
	qb:order	5 .

dad-attribute:flag	rdf:type	qb:ComponentSpecification ;
	qb:attribute	dad-prop:flag .
dad-attribute:note	rdf:type	qb:ComponentSpecification ;
	qb:attribute	dad-prop:note .

<http://semantic.digital-agenda-data.eu/def/dsd/scoreboard/measure/obsValue>	rdf:type	qb:ComponentSpecification ;
	qb:measure	sdmx-measure:obsValue .


# DSD Properties

dad-prop:breakdown
	rdf:type	qb:DimensionProperty , qb:CodedProperty , rdf:Property ;
	rdfs:label	"Breakdown"@en ;
	rdfs:range	dad-class:Breakdown ;
	rdfs:comment	"Values from codelist http://semantic.digital-agenda-data.eu/codelist/breakdown"@en ;
	skos:notation	"breakdown" ;
	qb:codeList	dad-codelist:breakdown ;
	qb:concept	dad-concept:breakdown ;
	dad-prop:grouped-using	dad-prop:breakdown-group ;
	skos:inScheme	dad-def:dad-scheme .
dad-prop:breakdown-group
	rdf:type	qb:CodedProperty , dad-class:DimensionGroupProperty , rdf:Property ;
	rdfs:label	"Breakdown group"@en ;
	rdfs:range	dad-class:BreakdownGroup ;
	rdfs:comment	"Values from codelist http://semantic.digital-agenda-data.eu/codelist/breakdown-group"@en ;
	skos:notation	"breakdown-group" ;
	qb:codeList	dad-codelist:breakdown-group ;
	qb:concept	dad-concept:breakdownGroup ;
	skos:inScheme	dad-def:dad-scheme .
dad-prop:indicator
	rdf:type	qb:DimensionProperty , qb:CodedProperty , rdf:Property ;
	rdfs:label	"Indicator"@en ;
	rdfs:range	dad-class:Indicator ;
	rdfs:comment	"Values from codelist http://semantic.digital-agenda-data.eu/codelist/indicator"@en ;
	skos:notation	"indicator" ;
	qb:codeList	dad-codelist:indicator ;
	qb:concept	dad-concept:indicator ;
	dad-prop:grouped-using	dad-prop:indicator-group ;
	skos:inScheme	dad-def:dad-scheme .
dad-prop:indicator-group
	rdf:type	dad-class:DimensionGroupProperty , qb:CodedProperty , rdf:Property ;
	rdfs:label	"Indicator group"@en ;
	rdfs:range	dad-class:IndicatorGroup ;
	rdfs:comment	"Values from codelist http://semantic.digital-agenda-data.eu/codelist/indicator-group"@en ;
	skos:notation	"indicator-group" ;
	qb:codeList	dad-codelist:indicator-group ;
	qb:concept	dad-concept:indicatorGroup ;
	skos:inScheme	dad-def:dad-scheme .
dad-prop:ref-area
	rdf:type	qb:DimensionProperty , qb:CodedProperty , rdf:Property ;
	rdfs:subPropertyOf	sdmx-dimension:refArea ;
	rdfs:label	"Country"@en ;
	rdfs:range	skos:Concept ;
	rdfs:comment	"Values from codelist http://eurostat.linked-statistics.org/dic/geo#"@en ;
	skos:notation	"ref-area" ;
	qb:codeList	<http://eurostat.linked-statistics.org/dic/geo> ;
	qb:concept	sdmx-concept:refArea ;
	skos:inScheme	dad-def:dad-scheme .
dad-prop:time-period
	rdf:type	qb:DimensionProperty , rdf:Property ;
	rdfs:subPropertyOf	sdmx-dimension:timePeriod ;
	rdfs:label	"Time period"@en ;
	rdfs:range	skos:Concept ;
	rdfs:comment	"Vocabulary allows Year, Half, Quarter, Month"@en ;
	rdfs:seeAlso	<http://reference.data.gov.uk/def/intervals> ;
	skos:notation	"time-period" ;
	qb:codeList	dad-codelist:time-period ;
	qb:concept	sdmx-concept:timePeriod ;
	skos:inScheme	dad-def:dad-scheme .
dad-prop:unit-measure
	rdf:type	qb:CodedProperty , qb:DimensionProperty , rdf:Property ;
	rdfs:label	"Unit of measure"@en ;
	rdfs:range	dad-class:UnitMeasure ;
	rdfs:comment	"Values from codelist http://semantic.digital-agenda-data.eu/codelist/unit-measure"@en ;
	skos:notation	"unit-measure" ;
	qb:codeList	dad-codelist:unit-measure ;
	qb:concept	sdmx-concept:unitMeasure ;
	skos:inScheme	dad-def:dad-scheme .
dad-prop:flag
	rdf:type	qb:AttributeProperty , qb:CodedProperty , rdf:Property ;
	rdfs:label	"Flag"@en ;
	rdfs:comment	"Values from Eurostat codelist: http://eurostat.linked-statistics.org/dic/flags"@en ;
	skos:notation	"flag" ;
	qb:codeList	<http://eurostat.linked-statistics.org/dic/flags> ;
	qb:concept	dad-concept:flag ;
	skos:inScheme	dad-def:dad-scheme .
dad-prop:note
	rdf:type	qb:AttributeProperty , rdf:Property ;
	rdfs:label	"Note"@en ;
	rdfs:range	xsd:string ;
	rdfs:comment	"Free text, optional"@en ;
	skos:notation	"note" ;
	qb:concept	dad-concept:note ;
	skos:inScheme	dad-def:dad-scheme .
