@prefix rdf:	<http://www.w3.org/1999/02/22-rdf-syntax-ns#> .
@prefix rdfs:	<http://www.w3.org/2000/01/rdf-schema#> .
@prefix xsd:	<http://www.w3.org/2001/XMLSchema#> .
@prefix qb:	<http://purl.org/linked-data/cube#> .
@prefix dcat:	<http://www.w3.org/ns/dcat#> .
@prefix dcterms:	<http://purl.org/dc/terms/> .
@prefix org:	<http://www.w3.org/ns/org#> .
@prefix foaf:	<http://xmlns.com/foaf/0.1/> .
@prefix odp:	<http://ec.europa.eu/open-data/ontologies/ec-odp#> .
@prefix adms:	<http://www.w3.org/ns/adms#> .
@prefix schema:	<http://schema.org/> .
@prefix vcard:	<http://www.w3.org/2006/vcard/ns#> .
@prefix skos:	<http://www.w3.org/2004/02/skos/core#> .
@prefix sdmx:	<http://purl.org/linked-data/sdmx#> .
@prefix sdmx-attribute:	<http://purl.org/linked-data/sdmx/2009/attribute#> .
@prefix sdmx-concept:	<http://purl.org/linked-data/sdmx/2009/concept#> .
@prefix sdmx-dimension:	<http://purl.org/linked-data/sdmx/2009/dimension#> .
@prefix sdmx-measure:	<http://purl.org/linked-data/sdmx/2009/measure#> .
@prefix sdmx-subject:	<http://purl.org/linked-data/sdmx/2009/subject#> .

@prefix ld-api:	<http://purl.org/linked-data/api/vocab#> .

@prefix dad-attribute:	<http://semantic.digital-agenda-data.eu/def/dsd/scoreboard/attribute/> .
@prefix dad-class:	<http://semantic.digital-agenda-data.eu/def/class/> .
@prefix dad-codelist:	<http://semantic.digital-agenda-data.eu/codelist/> .
@prefix dad-concept:	<http://semantic.digital-agenda-data.eu/def/concept/> .
@prefix dad-def:	<http://semantic.digital-agenda-data.eu/def/> .
@prefix dad-dimension:	<http://semantic.digital-agenda-data.eu/def/dsd/scoreboard/dimension/> .
@prefix dad-dsd:	<http://semantic.digital-agenda-data.eu/def/dsd/> .
@prefix dad-prop:	<http://semantic.digital-agenda-data.eu/def/property/> .

# DATASET METADATA
<http://semantic.digital-agenda-data.eu/dataset/digital-agenda-scoreboard-key-indicators>
	rdf:type qb:DataSet , dcat:Dataset ;
# DCAT Mandatory
	dcterms:title	"Digital Agenda Key Indicators"@en ;
	dcterms:description	"European Commission services selected more than 100 indicators, divided into thematic groups, which illustrate some key dimensions of the European information society (Telecom sector, Broadband, Mobile, Internet usage, Internet services, eGovernment, eCommerce, eBusiness, ICT Skills, Research and Development).\nThese indicators allow a comparison of progress across European countries as well as over time.\nYou can also browse the data with the help of a visualisation tools going at http://digital-agenda-data.eu/, where you are also able to download selected information."@en ;
# QB recommended properties
	rdfs:label	"Digital Agenda Key Indicators"@en ;
	rdfs:comment	"European Commission services selected more than 100 indicators, divided into thematic groups, which illustrate some key dimensions of the European information society (Telecom sector, Broadband, Mobile, Internet usage, Internet services, eGovernment, eCommerce, eBusiness, ICT Skills, Research and Development).\nThese indicators allow a comparison of progress across European countries as well as over time.\nYou can also browse the data with the help of a visualisation tools going at http://digital-agenda-data.eu/, where you are also able to download selected information."@en ;
	dcterms:subject	sdmx-subject:3.3.3 ;
		# TODO: here all concepts from dcat:theme could be listed

	dcterms:license	<http://ec.europa.eu/geninfo/legal_notices_en.htm#copyright> ;
# DCAT-AP recommended properties
	dcat:contactPoint	[
		a vcard:Organization;
		vcard:fn "DG CONNECT - Digital Economy and Skills (Unit F.4)" ;
		vcard:hasEmail <mailto:CNECT-F4@ec.europa.eu> ;
		vcard:hasURL <https://ec.europa.eu/digital-single-market/en/content/digital-economy-and-skills-unit-f4> ;
		rdfs:label "DG CONNECT - Digital Economy and Skills (Unit F.4)" ;
	];

	dcat:distribution	<http://semantic.digital-agenda-data.eu/dataset/digital-agenda-scoreboard-key-indicators/distribution/download> ;
	dcat:distribution	<http://semantic.digital-agenda-data.eu/dataset/digital-agenda-scoreboard-key-indicators/distribution/visualisation> ;
	dcat:keyword	
		"ICT research"@en ,
		"ICT skills"@en ,
		"telecom market"@en ,
		"ebusiness"@en ,
		"ecommerce"@en ,
		"information-society"@en ,
		"digital agenda"@en ,
		"internet"@en ,
		"broadband"@en ;

	dcterms:publisher	<http://publications.europa.eu/resource/authority/corporate-body/CNECT> ;
	dcat:theme	
		<http://publications.europa.eu/resource/authority/data-theme/GOVE> ,
		<http://publications.europa.eu/resource/authority/data-theme/SOCI> ,
		<http://publications.europa.eu/resource/authority/data-theme/TECH> ;

# DCAT-AP optional properties / DCAT recommended properties
	dcterms:accessRights	<http://publications.europa.eu/resource/authority/access-right/PUBLIC>;
	dcat:landingPage	<http://digital-agenda-data.eu/> ;
	foaf:page	<http://digital-agenda-data.eu/> ;
	dcterms:accrualPeriodicity	<http://publications.europa.eu/resource/authority/frequency/ANNUAL_2> ;
	dcterms:language <http://publications.europa.eu/resource/authority/language/ENG> ;
	dcterms:spatial	
		<http://publications.europa.eu/resource/authority/country/EUR>,
		<http://publications.europa.eu/resource/authority/country/CHE>,
		<http://publications.europa.eu/resource/authority/country/NOR>,
		<http://publications.europa.eu/resource/authority/country/ISL>,
		<http://publications.europa.eu/resource/authority/country/TUR>;
	dcterms:temporal	[ schema:startDate "2002-01-01"^^xsd:date ] ;
	dcterms:identifier	"digital-agenda-scoreboard-key-indicators" ;
	#adms:identifier	[ skos:notation "digital-agenda-scoreboard-key-indicators" ]
	dcterms:issued	"2011-05-01T00:00:00Z"^^xsd:dateTime ;
	dcterms:modified	"2016-06-01T00:00:00Z"^^xsd:dateTime ;
	dcterms:conformsTo	<http://purl.org/linked-data/cube> ;


# QB
	qb:structure	<http://semantic.digital-agenda-data.eu/def/dsd/scoreboard>;

# Linked data
	foaf:isPrimaryTopicOf	<http://semantic.digital-agenda-data.eu/API/dataset/digital-agenda-scoreboard-key-indicators.rdf> ;

# ODP
	adms:status	<http://purl.org/adms/status/Completed> .
	# TODO: change to http://publications.europa.eu/resource/authority/dataset-status/COMPLETED

# RELATED ENTITIES

# License
<http://ec.europa.eu/geninfo/legal_notices_en.htm#copyright>	dcterms:title	"Europa Legal Notice" .

# DCAT Distribution
<http://semantic.digital-agenda-data.eu/dataset/digital-agenda-scoreboard-key-indicators/distribution/download>	
	rdf:type	dcat:Distribution ;
	dcat:accessURL	<https://digital-agenda-data.eu/datasets/digital_agenda_scoreboard_key_indicators#download> ;
	dcterms:description	"Download instructions";
	dcterms:type	<http://publications.europa.eu/resource/authority/distribution-type/DOWNLOADABLE_FILE> ;
	dcterms:format	<http://publications.europa.eu/resource/authority/file-type/RDF_TURTLE> ;
	dcterms:license	<http://ec.europa.eu/geninfo/legal_notices_en.htm#copyright> ;
	dcat:mediaType	"text/turtle" .

# StatDCAT Visualisation
<http://semantic.digital-agenda-data.eu/dataset/digital-agenda-scoreboard-key-indicators/distribution/visualisation>
	rdf:type	dcat:Distribution ;
	dcterms:type	<http://publications.europa.eu/resource/authority/distribution-type/VISUALIZATION> ;
	dcat:accessURL	<https://digital-agenda-data.eu/datasets/digital_agenda_scoreboard_key_indicators> ;
	dcterms:license	<http://ec.europa.eu/geninfo/legal_notices_en.htm#copyright> ;
	dcterms:description	"Dataset visualisations".

# LD API page
<http://semantic.digital-agenda-data.eu/API/dataset/digital-agenda-scoreboard-key-indicators.rdf>
	rdf:type	ld-api:Page ;
	foaf:primaryTopic	<http://semantic.digital-agenda-data.eu/dataset/digital-agenda-scoreboard-key-indicators> ;
	ld-api:definition	<http://semantic.digital-agenda-data.eu/API/meta/dataset/_id.rdf> ;
	ld-api:extendedMetadataVersion	<http://semantic.digital-agenda-data.eu/API/dataset/digital-agenda-scoreboard-key-indicators.rdf?_metadata=all> .

## DATA STRUCTURE DEFINITION

# DSD Components

dad-dsd:scoreboard
	rdf:type	sdmx:DataStructureDefinition, qb:DataStructureDefinition .
dad-dsd:scoreboard
	qb:component
		dad-attribute:flag ,
		dad-attribute:note ,
		dad-dimension:indicator ,
		dad-dimension:breakdown ,
		dad-dimension:ref-area ,
		dad-dimension:time-period ,
		dad-dimension:unit-measure ,
		<http://semantic.digital-agenda-data.eu/def/dsd/scoreboard/measure/obsValue> ;
	sdmx:primaryMeasure	sdmx-measure:obsValue .

# DSD Component Specifications

dad-dimension:indicator	rdf:type	qb:ComponentSpecification ;
	qb:dimension	dad-prop:indicator ;
	qb:order	1 .
dad-dimension:breakdown	rdf:type	qb:ComponentSpecification ;
	qb:dimension	dad-prop:breakdown ;
	qb:order	2 .
dad-dimension:unit-measure	rdf:type	qb:ComponentSpecification ;
	qb:dimension	dad-prop:unit-measure ;
	qb:order	3 .
dad-dimension:ref-area	rdf:type	qb:ComponentSpecification ;
	qb:dimension	dad-prop:ref-area ;
	qb:order	4 .
dad-dimension:time-period	rdf:type	qb:ComponentSpecification ;
	qb:dimension	dad-prop:time-period ;
	qb:order	5 .

dad-attribute:flag	rdf:type	qb:ComponentSpecification ;
	qb:attribute	dad-prop:flag .
dad-attribute:note	rdf:type	qb:ComponentSpecification ;
	qb:attribute	dad-prop:note .

<http://semantic.digital-agenda-data.eu/def/dsd/scoreboard/measure/obsValue>	rdf:type	qb:ComponentSpecification ;
	qb:measure	sdmx-measure:obsValue .


# DSD Properties

dad-prop:breakdown
	rdf:type	qb:DimensionProperty , qb:CodedProperty , rdf:Property ;
	rdfs:label	"Breakdown"@en ;
	rdfs:range	dad-class:Breakdown ;
	rdfs:comment	"Values from codelist http://semantic.digital-agenda-data.eu/codelist/breakdown"@en ;
	skos:notation	"breakdown" ;
	qb:codeList	dad-codelist:breakdown ;
	qb:concept	dad-concept:breakdown ;
	dad-prop:grouped-using	dad-prop:breakdown-group ;
	skos:inScheme	dad-def:dad-scheme .
dad-prop:breakdown-group
	rdf:type	qb:CodedProperty , dad-class:DimensionGroupProperty , rdf:Property ;
	rdfs:label	"Breakdown group"@en ;
	rdfs:range	dad-class:BreakdownGroup ;
	rdfs:comment	"Values from codelist http://semantic.digital-agenda-data.eu/codelist/breakdown-group"@en ;
	skos:notation	"breakdown-group" ;
	qb:codeList	dad-codelist:breakdown-group ;
	qb:concept	dad-concept:breakdownGroup ;
	skos:inScheme	dad-def:dad-scheme .
dad-prop:indicator
	rdf:type	qb:DimensionProperty , qb:CodedProperty , rdf:Property ;
	rdfs:label	"Indicator"@en ;
	rdfs:range	dad-class:Indicator ;
	rdfs:comment	"Values from codelist http://semantic.digital-agenda-data.eu/codelist/indicator"@en ;
	skos:notation	"indicator" ;
	qb:codeList	dad-codelist:indicator ;
	qb:concept	dad-concept:indicator ;
	dad-prop:grouped-using	dad-prop:indicator-group ;
	skos:inScheme	dad-def:dad-scheme .
dad-prop:indicator-group
	rdf:type	dad-class:DimensionGroupProperty , qb:CodedProperty , rdf:Property ;
	rdfs:label	"Indicator group"@en ;
	rdfs:range	dad-class:IndicatorGroup ;
	rdfs:comment	"Values from codelist http://semantic.digital-agenda-data.eu/codelist/indicator-group"@en ;
	skos:notation	"indicator-group" ;
	qb:codeList	dad-codelist:indicator-group ;
	qb:concept	dad-concept:indicatorGroup ;
	skos:inScheme	dad-def:dad-scheme .
dad-prop:ref-area
	rdf:type	qb:DimensionProperty , qb:CodedProperty , rdf:Property ;
	rdfs:subPropertyOf	sdmx-dimension:refArea ;
	rdfs:label	"Country"@en ;
	rdfs:range	skos:Concept ;
	rdfs:comment	"Values from codelist http://eurostat.linked-statistics.org/dic/geo#"@en ;
	skos:notation	"ref-area" ;
	qb:codeList	<http://eurostat.linked-statistics.org/dic/geo> ;
	qb:concept	sdmx-concept:refArea ;
	skos:inScheme	dad-def:dad-scheme .
dad-prop:time-period
	rdf:type	qb:DimensionProperty , rdf:Property ;
	rdfs:subPropertyOf	sdmx-dimension:timePeriod ;
	rdfs:label	"Time period"@en ;
	rdfs:range	skos:Concept ;
	rdfs:comment	"Vocabulary allows Year, Half, Quarter, Month"@en ;
	rdfs:seeAlso	<http://reference.data.gov.uk/def/intervals> ;
	skos:notation	"time-period" ;
	qb:codeList	dad-codelist:time-period ;
	qb:concept	sdmx-concept:timePeriod ;
	skos:inScheme	dad-def:dad-scheme .
dad-prop:unit-measure
	rdf:type	qb:CodedProperty , qb:DimensionProperty , rdf:Property ;
	rdfs:label	"Unit of measure"@en ;
	rdfs:range	dad-class:UnitMeasure ;
	rdfs:comment	"Values from codelist http://semantic.digital-agenda-data.eu/codelist/unit-measure"@en ;
	skos:notation	"unit-measure" ;
	qb:codeList	dad-codelist:unit-measure ;
	qb:concept	sdmx-concept:unitMeasure ;
	skos:inScheme	dad-def:dad-scheme .
dad-prop:flag
	rdf:type	qb:AttributeProperty , qb:CodedProperty , rdf:Property ;
	rdfs:label	"Flag"@en ;
	rdfs:comment	"Values from Eurostat codelist: http://eurostat.linked-statistics.org/dic/flags"@en ;
	skos:notation	"flag" ;
	qb:codeList	<http://eurostat.linked-statistics.org/dic/flags> ;
	qb:concept	dad-concept:flag ;
	skos:inScheme	dad-def:dad-scheme .
dad-prop:note
	rdf:type	qb:AttributeProperty , rdf:Property ;
	rdfs:label	"Note"@en ;
	rdfs:range	xsd:string ;
	rdfs:comment	"Free text, optional"@en ;
	skos:notation	"note" ;
	qb:concept	dad-concept:note ;
	skos:inScheme	dad-def:dad-scheme .
